<?xml version="1.0"?>
<rdf:RDF xmlns="http://ids.maastrichtuniversity.nl/ontologies/cbm/eu-cm-ontology#"
     xml:base="http://ids.maastrichtuniversity.nl/ontologies/cbm/eu-cm-ontology"
     xmlns:rdf="http://www.w3.org/1999/02/22-rdf-syntax-ns#"
     xmlns:terms="http://purl.org/dc/terms/"
     xmlns:owl="http://www.w3.org/2002/07/owl#"
     xmlns:xml="http://www.w3.org/XML/1998/namespace"
     xmlns:cbcm="http://w3id.org/um/cbcm/eu-cm-ontology#"
     xmlns:xsd="http://www.w3.org/2001/XMLSchema#"
     xmlns:opla-sd="http://ontologydesignpatterns.org/opla-sd#"
     xmlns:rdfs="http://www.w3.org/2000/01/rdf-schema#"
     xmlns:prov="http://www.w3.org/ns/prov#"
     xmlns:dc="http://purl.org/dc/elements/1.1/">
    <owl:Ontology rdf:about="http://w3id.org/um/cbcm/eu-cm-ontology">
        <owl:versionIRI rdf:resource="http://w3id.org/um/cbcm/eu-cm-ontology/1.2.1"/>
        <terms:contributor rdf:datatype="http://www.w3.org/2001/XMLSchema#string">Stephan Rammeloo</terms:contributor>
        <prov:wasAttributedTo rdf:datatype="http://www.w3.org/2001/XMLSchema#string">The Maastricht Law &amp; Techlab</prov:wasAttributedTo>
        <prov:wasAttributedTo rdf:datatype="http://www.w3.org/2001/XMLSchema#string">Maastricht University</prov:wasAttributedTo>
        <terms:license rdf:datatype="http://www.w3.org/2001/XMLSchema#string">Creative Commons Attribution 3.0 (CC BY 3.0)</terms:license>
        <prov:wasAttributedTo rdf:datatype="http://www.w3.org/2001/XMLSchema#string">Institute of Data Science at Maastricht University</prov:wasAttributedTo>
        <terms:contributor rdf:datatype="http://www.w3.org/2001/XMLSchema#string">Tobias Breuer</terms:contributor>
        <dc:description rdf:datatype="http://www.w3.org/2001/XMLSchema#string">This ontology describes terms concerning companies, their cross-border movements within the European Union (EU), and associated EU company legislation.Société agricole</dc:description>
        <owl:versionInfo rdf:datatype="http://www.w3.org/2001/XMLSchema#string">1.2.1</owl:versionInfo>
        <terms:contributor rdf:datatype="http://www.w3.org/2001/XMLSchema#string">Ruta Liepina</terms:contributor>
        <terms:contributor rdf:datatype="http://www.w3.org/2001/XMLSchema#string">Walter Simoncini</terms:contributor>
        <terms:contributor rdf:datatype="http://www.w3.org/2001/XMLSchema#string">Marcus Meyer</terms:contributor>
        <dc:title rdf:datatype="http://www.w3.org/2001/XMLSchema#string">The European Union Company Mobility Ontology (EU-CMO)</dc:title>
        <rdfs:seeAlso rdf:datatype="http://www.w3.org/2001/XMLSchema#anyURI">https://maastrichtu-ids.github.io/cbcm-ontology</rdfs:seeAlso>
        <terms:contributor rdf:datatype="http://www.w3.org/2001/XMLSchema#string">Thomas Biermeyer</terms:contributor>
        <terms:contributor rdf:datatype="http://www.w3.org/2001/XMLSchema#string">Kody Moodley</terms:contributor>
    </owl:Ontology>
    


    <!-- 
    ///////////////////////////////////////////////////////////////////////////////////////
    //
    // Annotation properties
    //
    ///////////////////////////////////////////////////////////////////////////////////////
     -->

    


    <!-- http://ontologydesignpatterns.org/opla-sd#entityPosition -->

    <owl:AnnotationProperty rdf:about="http://ontologydesignpatterns.org/opla-sd#entityPosition"/>
    


    <!-- http://ontologydesignpatterns.org/opla-sd#entityPositionX -->

    <owl:AnnotationProperty rdf:about="http://ontologydesignpatterns.org/opla-sd#entityPositionX"/>
    


    <!-- http://ontologydesignpatterns.org/opla-sd#entityPositionY -->

    <owl:AnnotationProperty rdf:about="http://ontologydesignpatterns.org/opla-sd#entityPositionY"/>
    


    <!-- http://purl.org/dc/elements/1.1/description -->

    <owl:AnnotationProperty rdf:about="http://purl.org/dc/elements/1.1/description"/>
    


    <!-- http://purl.org/dc/elements/1.1/title -->

    <owl:AnnotationProperty rdf:about="http://purl.org/dc/elements/1.1/title"/>
    


    <!-- http://purl.org/dc/terms/contributor -->

    <owl:AnnotationProperty rdf:about="http://purl.org/dc/terms/contributor"/>
    


    <!-- http://purl.org/dc/terms/description -->

    <owl:AnnotationProperty rdf:about="http://purl.org/dc/terms/description"/>
    


    <!-- http://purl.org/dc/terms/license -->

    <owl:AnnotationProperty rdf:about="http://purl.org/dc/terms/license"/>
    


    <!-- http://w3id.org/um/cbcm/eu-cm-ontology#example -->

    <owl:AnnotationProperty rdf:about="http://w3id.org/um/cbcm/eu-cm-ontology#example">
        <rdfs:comment xml:lang="en">Provides a human-readable written example of the entity in question.</rdfs:comment>
        <rdfs:label xml:lang="en">Example</rdfs:label>
        <rdfs:subPropertyOf rdf:resource="http://www.w3.org/2000/01/rdf-schema#comment"/>
    </owl:AnnotationProperty>
    


    <!-- http://w3id.org/um/cbcm/eu-cm-ontology#iso2code -->

    <owl:AnnotationProperty rdf:about="http://w3id.org/um/cbcm/eu-cm-ontology#iso2code">
        <rdfs:subPropertyOf rdf:resource="http://www.w3.org/2000/01/rdf-schema#label"/>
    </owl:AnnotationProperty>
    


    <!-- http://w3id.org/um/cbcm/eu-cm-ontology#requirement-level -->

    <owl:AnnotationProperty rdf:about="http://w3id.org/um/cbcm/eu-cm-ontology#requirement-level">
        <cbcm:example xml:lang="en">Examples include: MUST, SHOULD, RECOMMENDED and OPTIONAL</cbcm:example>
        <rdfs:comment xml:lang="en">Specifies a phrase to indicate the degree to which the providing of a value for the entity (e.g. a data or object property) in question is compulsory, recommended or optional.</rdfs:comment>
        <rdfs:label xml:lang="en">Requirement level</rdfs:label>
        <rdfs:subPropertyOf rdf:resource="http://www.w3.org/2000/01/rdf-schema#comment"/>
    </owl:AnnotationProperty>
    


    <!-- http://www.w3.org/ns/prov#wasAttributedTo -->

    <owl:AnnotationProperty rdf:about="http://www.w3.org/ns/prov#wasAttributedTo"/>
    


    <!-- 
    ///////////////////////////////////////////////////////////////////////////////////////
    //
    // Object Properties
    //
    ///////////////////////////////////////////////////////////////////////////////////////
     -->

    


    <!-- http://w3id.org/um/cbcm/eu-cm-ontology#applicableTo -->

    <owl:ObjectProperty rdf:about="http://w3id.org/um/cbcm/eu-cm-ontology#applicableTo">
        <rdfs:subPropertyOf rdf:resource="http://w3id.org/um/cbcm/eu-cm-ontology#cbcmObjectRelation"/>
        <rdfs:domain rdf:resource="http://w3id.org/um/cbcm/eu-cm-ontology#TransactionRight"/>
        <rdfs:range rdf:resource="http://w3id.org/um/cbcm/eu-cm-ontology#Agent"/>
        <cbcm:example xml:lang="en">(applicableTo creditorRight1 person1)</cbcm:example>
        <rdfs:comment xml:lang="en">(applicableTo ?ENTITY1 ?ENTITY2) means that some legal right ?ENTITY1 is awarded or assigned to a particular person or agent ?ENTITY2.</rdfs:comment>
        <rdfs:label xml:lang="en">applicable to</rdfs:label>
    </owl:ObjectProperty>
    


    <!-- http://w3id.org/um/cbcm/eu-cm-ontology#associatedWith -->

    <owl:ObjectProperty rdf:about="http://w3id.org/um/cbcm/eu-cm-ontology#associatedWith">
        <rdfs:subPropertyOf rdf:resource="http://w3id.org/um/cbcm/eu-cm-ontology#cbcmDataProvenanceRelation"/>
        <rdfs:domain rdf:resource="http://w3id.org/um/cbcm/eu-cm-ontology#Process"/>
        <rdfs:range rdf:resource="http://w3id.org/um/cbcm/eu-cm-ontology#Agent"/>
        <rdfs:comment xml:lang="en">An activity association is an assignment of responsibility to an agent for a process, indicating that the agent had a role in the activity.

Based on: https://www.w3.org/TR/prov-o/#wasAssociatedWith</rdfs:comment>
        <rdfs:label xml:lang="en">Associated with</rdfs:label>
    </owl:ObjectProperty>
    


    <!-- http://w3id.org/um/cbcm/eu-cm-ontology#attributedTo -->

    <owl:ObjectProperty rdf:about="http://w3id.org/um/cbcm/eu-cm-ontology#attributedTo">
        <rdfs:subPropertyOf rdf:resource="http://w3id.org/um/cbcm/eu-cm-ontology#cbcmDataProvenanceRelation"/>
        <rdfs:domain rdf:resource="http://w3id.org/um/cbcm/eu-cm-ontology#Entity"/>
        <rdfs:range rdf:resource="http://w3id.org/um/cbcm/eu-cm-ontology#Agent"/>
        <rdfs:comment xml:lang="en">Attribution is the ascribing of an entity to an agent.

Based on: https://www.w3.org/TR/prov-o/#wasAttributedTo</rdfs:comment>
        <rdfs:label xml:lang="en">Attributed to</rdfs:label>
    </owl:ObjectProperty>
    


    <!-- http://w3id.org/um/cbcm/eu-cm-ontology#authoredBy -->

    <owl:ObjectProperty rdf:about="http://w3id.org/um/cbcm/eu-cm-ontology#authoredBy">
        <rdfs:subPropertyOf rdf:resource="http://w3id.org/um/cbcm/eu-cm-ontology#cbcmDocumentRelation"/>
        <owl:inverseOf rdf:resource="http://w3id.org/um/cbcm/eu-cm-ontology#authors"/>
        <rdfs:domain rdf:resource="http://w3id.org/um/cbcm/eu-cm-ontology#CompanyMobilityDocument"/>
        <rdfs:range>
            <owl:Class>
                <owl:unionOf rdf:parseType="Collection">
                    <rdf:Description rdf:about="http://w3id.org/um/cbcm/eu-cm-ontology#Organisation"/>
                    <rdf:Description rdf:about="http://w3id.org/um/cbcm/eu-cm-ontology#Person"/>
                </owl:unionOf>
            </owl:Class>
        </rdfs:range>
        <cbcm:example>(authoredBy independentExpertReport1 independentExpert1)</cbcm:example>
        <rdfs:comment xml:lang="en">(authoredBy ?ENTITY1 ?ENTITY2) means that ?ENTITY1 is an instance of a publication that is created primarily by the entity referred to by ?ENTITY2.</rdfs:comment>
        <rdfs:label xml:lang="en">authored by</rdfs:label>
        <rdfs:seeAlso rdf:resource="http://w3id.org/um/cbcm/eu-cm-ontology#authors"/>
    </owl:ObjectProperty>
    


    <!-- http://w3id.org/um/cbcm/eu-cm-ontology#authors -->

    <owl:ObjectProperty rdf:about="http://w3id.org/um/cbcm/eu-cm-ontology#authors">
        <rdfs:subPropertyOf rdf:resource="http://w3id.org/um/cbcm/eu-cm-ontology#cbcmDocumentRelation"/>
        <rdfs:comment xml:lang="en">(authors ?ENTITY1 ?ENTITY2) means that (authoredBy ?ENTITY2 ?ENTITY1)</rdfs:comment>
        <rdfs:label xml:lang="en">authors</rdfs:label>
        <rdfs:seeAlso rdf:resource="http://w3id.org/um/cbcm/eu-cm-ontology#authoredBy"/>
    </owl:ObjectProperty>
    


    <!-- http://w3id.org/um/cbcm/eu-cm-ontology#cbcmDataProvenanceRelation -->

    <owl:ObjectProperty rdf:about="http://w3id.org/um/cbcm/eu-cm-ontology#cbcmDataProvenanceRelation">
        <rdfs:subPropertyOf rdf:resource="http://w3id.org/um/cbcm/eu-cm-ontology#cbcmEntityRelation"/>
        <rdfs:comment xml:lang="en">(cbcmDataProvenanceRelation ?ENTITY1 ?ENTITY2) means that the relation between ?ENTITY1 and ?ENTITY2 captures provenance information for company transaction data.</rdfs:comment>
        <rdfs:label xml:lang="en">Cross-border company mobility data provenance relation</rdfs:label>
    </owl:ObjectProperty>
    


    <!-- http://w3id.org/um/cbcm/eu-cm-ontology#cbcmDocumentRelation -->

    <owl:ObjectProperty rdf:about="http://w3id.org/um/cbcm/eu-cm-ontology#cbcmDocumentRelation">
        <rdfs:subPropertyOf rdf:resource="http://w3id.org/um/cbcm/eu-cm-ontology#cbcmEntityRelation"/>
        <rdfs:comment xml:lang="en">(cbcmDocumentRelation ?ENTITY1 ?ENTITY2) means that the relation between ?ENTITY1 and ?ENTITY2 captures information pertaining to a company mobility document or similar information source relevant to corporate mobility.</rdfs:comment>
        <rdfs:label xml:lang="en">Cross-border company mobility document relation</rdfs:label>
        <rdfs:seeAlso rdf:resource="http://w3id.org/um/cbcm/eu-cm-ontology#CompanyMobilityDocument"/>
    </owl:ObjectProperty>
    


    <!-- http://w3id.org/um/cbcm/eu-cm-ontology#cbcmEntityRelation -->

    <owl:ObjectProperty rdf:about="http://w3id.org/um/cbcm/eu-cm-ontology#cbcmEntityRelation">
        <rdfs:comment xml:lang="en">(cbcmEntityRelation ?ENTITY1 ?ENTITY2) means that ?ENTITY1 is related to ?ENTITY2.</rdfs:comment>
        <rdfs:label xml:lang="en">Cross-border company mobility entity relation</rdfs:label>
    </owl:ObjectProperty>
    


    <!-- http://w3id.org/um/cbcm/eu-cm-ontology#cbcmObjectRelation -->

    <owl:ObjectProperty rdf:about="http://w3id.org/um/cbcm/eu-cm-ontology#cbcmObjectRelation">
        <rdfs:subPropertyOf rdf:resource="http://w3id.org/um/cbcm/eu-cm-ontology#cbcmEntityRelation"/>
        <rdfs:comment xml:lang="en">(cbcmObjectRelation ?ENTITY1 ?ENTITY2) means that the relation between ?ENTITY1 and ?ENTITY2 captures information pertaining to an object.</rdfs:comment>
        <rdfs:label xml:lang="en">Cross-border company mobility object relation</rdfs:label>
        <rdfs:seeAlso rdf:resource="http://w3id.org/um/cbcm/eu-cm-ontology#Object"/>
    </owl:ObjectProperty>
    


    <!-- http://w3id.org/um/cbcm/eu-cm-ontology#cbcmOrganisationRelation -->

    <owl:ObjectProperty rdf:about="http://w3id.org/um/cbcm/eu-cm-ontology#cbcmOrganisationRelation">
        <rdfs:subPropertyOf rdf:resource="http://w3id.org/um/cbcm/eu-cm-ontology#cbcmEntityRelation"/>
        <rdfs:comment xml:lang="en">(cbcmOrganisationRelation ?ENTITY1 ?ENTITY2) means that the relation between ?ENTITY1 and ?ENTITY2 captures information pertaining to an organisation.</rdfs:comment>
        <rdfs:label xml:lang="en">Cross-border company mobility organisation relation</rdfs:label>
        <rdfs:seeAlso rdf:resource="http://w3id.org/um/cbcm/eu-cm-ontology#Organisation"/>
    </owl:ObjectProperty>
    


    <!-- http://w3id.org/um/cbcm/eu-cm-ontology#cbcmTransactionRelation -->

    <owl:ObjectProperty rdf:about="http://w3id.org/um/cbcm/eu-cm-ontology#cbcmTransactionRelation">
        <rdfs:subPropertyOf rdf:resource="http://w3id.org/um/cbcm/eu-cm-ontology#cbcmEntityRelation"/>
        <rdfs:comment xml:lang="en">(cbcmTransactionRelation ?ENTITY1 ?ENTITY2) means that the relation between ?ENTITY1 and ?ENTITY2 captures information pertaining to a company mobility transaction.</rdfs:comment>
        <rdfs:label xml:lang="en">Cross-border company mobility transaction relation</rdfs:label>
        <rdfs:seeAlso rdf:resource="http://w3id.org/um/cbcm/eu-cm-ontology#CompanyTransaction"/>
    </owl:ObjectProperty>
    


    <!-- http://w3id.org/um/cbcm/eu-cm-ontology#containedIn -->

    <owl:ObjectProperty rdf:about="http://w3id.org/um/cbcm/eu-cm-ontology#containedIn">
        <rdfs:subPropertyOf rdf:resource="http://w3id.org/um/cbcm/eu-cm-ontology#cbcmDocumentRelation"/>
        <rdfs:domain rdf:resource="http://w3id.org/um/cbcm/eu-cm-ontology#CompanyMobilityDocument"/>
        <rdfs:range rdf:resource="http://w3id.org/um/cbcm/eu-cm-ontology#DocumentRepository"/>
        <cbcm:example xml:lang="en">(containedIn transactionNotice1 nationalRegistry1)</cbcm:example>
        <rdfs:comment xml:lang="en">(containedIn ?ENTITY1 ?ENTITY2) means that some document or publication ?ENTITY1 is archived or stored in some other document collection, database or data repository referred to by ?ENTITY2.</rdfs:comment>
        <rdfs:label xml:lang="en">contained in</rdfs:label>
    </owl:ObjectProperty>
    


    <!-- http://w3id.org/um/cbcm/eu-cm-ontology#countryHasCompanyForm -->

    <owl:ObjectProperty rdf:about="http://w3id.org/um/cbcm/eu-cm-ontology#countryHasCompanyForm">
        <rdfs:subPropertyOf rdf:resource="http://w3id.org/um/cbcm/eu-cm-ontology#cbcmEntityRelation"/>
        <owl:inverseOf rdf:resource="http://w3id.org/um/cbcm/eu-cm-ontology#isCompanyFormOfCountry"/>
        <rdfs:domain rdf:resource="http://w3id.org/um/cbcm/eu-cm-ontology#Country"/>
        <rdfs:range rdf:resource="http://w3id.org/um/cbcm/eu-cm-ontology#CompanyLegalForm"/>
        <rdfs:comment xml:lang="en">(countryHasCompanyForm ?ENTITY1 ?ENTITY2) means that ?ENTITY1 refers to a country the corporate law in that country permits and / or has occurrences of companies in that country which have the corporate legal structure (company legal form) referred to by ?ENTITY2.</rdfs:comment>
        <rdfs:label xml:lang="en">country has company form</rdfs:label>
    </owl:ObjectProperty>
    


    <!-- http://w3id.org/um/cbcm/eu-cm-ontology#documentValidatedByDocument -->

    <owl:ObjectProperty rdf:about="http://w3id.org/um/cbcm/eu-cm-ontology#documentValidatedByDocument">
        <rdfs:subPropertyOf rdf:resource="http://w3id.org/um/cbcm/eu-cm-ontology#cbcmDocumentRelation"/>
        <rdfs:domain rdf:resource="http://w3id.org/um/cbcm/eu-cm-ontology#CompanyMobilityDocument"/>
        <rdfs:range rdf:resource="http://w3id.org/um/cbcm/eu-cm-ontology#CompanyMobilityDocument"/>
        <cbcm:example xml:lang="en">(documentValidatedByDocument mergerPlan1 mergerCertificate1)</cbcm:example>
        <rdfs:comment xml:lang="en">(documentValidatedByDocument ?ENTITY1 ?ENTITY2) means that some document or publication, ?ENTITY1, went through a process of approval and assessment through various criteria such as veracity, eligibility, legal relevance etc. and another document ?ENTITY2 was produced to prove the satisfaction of the critieria by ?ENTITY1.</rdfs:comment>
        <rdfs:label xml:lang="en">document validated by document</rdfs:label>
    </owl:ObjectProperty>
    


    <!-- http://w3id.org/um/cbcm/eu-cm-ontology#employedBy -->

    <owl:ObjectProperty rdf:about="http://w3id.org/um/cbcm/eu-cm-ontology#employedBy">
        <rdfs:subPropertyOf rdf:resource="http://w3id.org/um/cbcm/eu-cm-ontology#hasCompanyStakeholder"/>
        <owl:inverseOf rdf:resource="http://w3id.org/um/cbcm/eu-cm-ontology#employs"/>
        <rdfs:domain>
            <owl:Class>
                <owl:unionOf rdf:parseType="Collection">
                    <rdf:Description rdf:about="http://w3id.org/um/cbcm/eu-cm-ontology#Organisation"/>
                    <rdf:Description rdf:about="http://w3id.org/um/cbcm/eu-cm-ontology#Person"/>
                </owl:unionOf>
            </owl:Class>
        </rdfs:domain>
        <rdfs:range>
            <owl:Class>
                <owl:unionOf rdf:parseType="Collection">
                    <rdf:Description rdf:about="http://w3id.org/um/cbcm/eu-cm-ontology#Organisation"/>
                    <rdf:Description rdf:about="http://w3id.org/um/cbcm/eu-cm-ontology#Person"/>
                </owl:unionOf>
            </owl:Class>
        </rdfs:range>
        <cbcm:example xml:lang="en">(employedBy person1 company1)</cbcm:example>
        <rdfs:comment xml:lang="en">(employedBy ?ENTITY1 ?ENTITY2) means that some agent (person or organisation) ?ENTITY1 is promised and delivered an incentive (usually financial) to perform some work for ?ENTITY2 where ?ENTITY2 is an organisation. This exchange is usually governed by law and formal regulations in the particular country or social context in which the work is being performed.</rdfs:comment>
        <rdfs:label xml:lang="en">employed by</rdfs:label>
    </owl:ObjectProperty>
    


    <!-- http://w3id.org/um/cbcm/eu-cm-ontology#employs -->

    <owl:ObjectProperty rdf:about="http://w3id.org/um/cbcm/eu-cm-ontology#employs">
        <rdfs:subPropertyOf rdf:resource="http://w3id.org/um/cbcm/eu-cm-ontology#hasCompanyStakeholder"/>
        <rdfs:comment xml:lang="en">(employs ?ENTITY1 ?ENTITY2) means (employedBy ?ENTITY2 ?ENTITY1)</rdfs:comment>
        <rdfs:label xml:lang="en">employs</rdfs:label>
        <rdfs:seeAlso rdf:resource="http://w3id.org/um/cbcm/eu-cm-ontology#employedBy"/>
    </owl:ObjectProperty>
    


    <!-- http://w3id.org/um/cbcm/eu-cm-ontology#generatedBy -->

    <owl:ObjectProperty rdf:about="http://w3id.org/um/cbcm/eu-cm-ontology#generatedBy">
        <rdfs:subPropertyOf rdf:resource="http://w3id.org/um/cbcm/eu-cm-ontology#cbcmDataProvenanceRelation"/>
        <rdfs:domain rdf:resource="http://w3id.org/um/cbcm/eu-cm-ontology#Entity"/>
        <rdfs:range rdf:resource="http://w3id.org/um/cbcm/eu-cm-ontology#Process"/>
        <rdfs:comment xml:lang="en">Generation is the completion of production of a new entity by a process. This entity did not exist before generation and becomes available for usage after this generation.

Based on: https://www.w3.org/TR/prov-o/#wasGeneratedBy</rdfs:comment>
        <rdfs:label xml:lang="en">Generated by</rdfs:label>
    </owl:ObjectProperty>
    


    <!-- http://w3id.org/um/cbcm/eu-cm-ontology#hasAcquiringCompany -->

    <owl:ObjectProperty rdf:about="http://w3id.org/um/cbcm/eu-cm-ontology#hasAcquiringCompany">
        <rdfs:subPropertyOf rdf:resource="http://w3id.org/um/cbcm/eu-cm-ontology#hasTransactionResult"/>
        <rdfs:domain rdf:resource="http://w3id.org/um/cbcm/eu-cm-ontology#CompanyMerger"/>
        <rdfs:range rdf:resource="http://w3id.org/um/cbcm/eu-cm-ontology#Company"/>
        <cbcm:example>(hasAcquiringCompany crossBorderMerger1 company1)</cbcm:example>
        <rdfs:comment xml:lang="en">(hasAcquiringCompany ?ENTITY1 ?ENTITY2) means that some company merger transaction ?ENTITY1 produces a new company or alters an existing one (?ENTITY2) such that ?ENTITY2 will acquire (via a universal transfer of assets and liabilities) one or more other companies involved in the process ?ENTITY1.</rdfs:comment>
        <rdfs:label xml:lang="en">has acquiring company</rdfs:label>
        <rdfs:seeAlso rdf:resource="http://w3id.org/um/cbcm/eu-cm-ontology#AcquiringCompany"/>
        <rdfs:seeAlso rdf:resource="http://w3id.org/um/cbcm/eu-cm-ontology#CompanyMerger"/>
        <rdfs:seeAlso rdf:resource="http://w3id.org/um/cbcm/eu-cm-ontology#MergingCompany"/>
    </owl:ObjectProperty>
    


    <!-- http://w3id.org/um/cbcm/eu-cm-ontology#hasCompanyForm -->

    <owl:ObjectProperty rdf:about="http://w3id.org/um/cbcm/eu-cm-ontology#hasCompanyForm">
        <rdfs:subPropertyOf rdf:resource="http://w3id.org/um/cbcm/eu-cm-ontology#cbcmOrganisationRelation"/>
        <rdfs:domain rdf:resource="http://w3id.org/um/cbcm/eu-cm-ontology#Company"/>
        <rdfs:range rdf:resource="http://w3id.org/um/cbcm/eu-cm-ontology#CompanyLegalForm"/>
        <rdfs:comment xml:lang="en">Company legal form. Name given to describe the structure of a corporation or buiness in the different legal orders. For example Limited (Ltd.), Public Limited Company (PLC), Gesellschaft mit beschränkter Haftung (GmbH), Aktiengesellschaft (AG). The company legal form is regulated under national law and grants specific rights and obligations to the company stakeholders (such as shareholders, management &amp; employees).</rdfs:comment>
        <rdfs:label xml:lang="en">Company Form</rdfs:label>
    </owl:ObjectProperty>
    


    <!-- http://w3id.org/um/cbcm/eu-cm-ontology#hasCompanyStakeholder -->

    <owl:ObjectProperty rdf:about="http://w3id.org/um/cbcm/eu-cm-ontology#hasCompanyStakeholder">
        <rdfs:subPropertyOf rdf:resource="http://w3id.org/um/cbcm/eu-cm-ontology#cbcmOrganisationRelation"/>
        <rdfs:domain>
            <owl:Class>
                <owl:unionOf rdf:parseType="Collection">
                    <rdf:Description rdf:about="http://w3id.org/um/cbcm/eu-cm-ontology#Agent"/>
                    <rdf:Description rdf:about="http://w3id.org/um/cbcm/eu-cm-ontology#Process"/>
                </owl:unionOf>
            </owl:Class>
        </rdfs:domain>
        <rdfs:range rdf:resource="http://w3id.org/um/cbcm/eu-cm-ontology#Agent"/>
        <cbcm:example xml:lang="en">(hasCompanyStakeholder company1 person1)</cbcm:example>
        <rdfs:comment xml:lang="en">(hasCompanyStakeholder ?ENTITY1 ?ENTITY2) means that some entity ?ENTITY1, which is either a significant process or agent has another agent ?ENTITY2 with personal interests in benefiting either financially or otherwise from the outcomes of ?ENTITY1 (if it is an event or process), or in its byproducts and profits (if it is an agent).</rdfs:comment>
        <rdfs:label xml:lang="en">has company stakeholder</rdfs:label>
    </owl:ObjectProperty>
    


    <!-- http://w3id.org/um/cbcm/eu-cm-ontology#hasDataProvenanceDocumentSource -->

    <owl:ObjectProperty rdf:about="http://w3id.org/um/cbcm/eu-cm-ontology#hasDataProvenanceDocumentSource">
        <rdfs:subPropertyOf rdf:resource="http://w3id.org/um/cbcm/eu-cm-ontology#hasPrimarySource"/>
        <rdfs:domain rdf:resource="http://w3id.org/um/cbcm/eu-cm-ontology#CompanyTransaction"/>
        <rdfs:range rdf:resource="http://w3id.org/um/cbcm/eu-cm-ontology#CompanyMobilityDocument"/>
        <rdfs:comment xml:lang="en">In which countries&apos; registry did the researcher find information about the transaction?</rdfs:comment>
        <rdfs:label xml:lang="en">has document source</rdfs:label>
    </owl:ObjectProperty>
    


    <!-- http://w3id.org/um/cbcm/eu-cm-ontology#hasDataProvenanceRegistryCountry -->

    <owl:ObjectProperty rdf:about="http://w3id.org/um/cbcm/eu-cm-ontology#hasDataProvenanceRegistryCountry">
        <rdfs:subPropertyOf rdf:resource="http://w3id.org/um/cbcm/eu-cm-ontology#hasPrimarySource"/>
        <rdfs:domain rdf:resource="http://w3id.org/um/cbcm/eu-cm-ontology#CompanyTransaction"/>
        <rdfs:range rdf:resource="http://w3id.org/um/cbcm/eu-cm-ontology#Country"/>
        <rdfs:comment xml:lang="en">In which countries&apos; registry did the researcher find information about the transaction?</rdfs:comment>
        <rdfs:label xml:lang="en">data found in registry from country</rdfs:label>
    </owl:ObjectProperty>
    


    <!-- http://w3id.org/um/cbcm/eu-cm-ontology#hasMember -->

    <owl:ObjectProperty rdf:about="http://w3id.org/um/cbcm/eu-cm-ontology#hasMember">
        <rdfs:subPropertyOf rdf:resource="http://w3id.org/um/cbcm/eu-cm-ontology#hasCompanyStakeholder"/>
        <rdfs:domain rdf:resource="http://w3id.org/um/cbcm/eu-cm-ontology#Organisation"/>
        <rdfs:range rdf:resource="http://w3id.org/um/cbcm/eu-cm-ontology#Person"/>
        <cbcm:example xml:lang="en">(hasMember worksCouncil1 employee1)</cbcm:example>
        <rdfs:comment xml:lang="en">(hasMember ?ENTITY1 ?ENTITY2) means that some agent ?ENTITY1 (usually an organisation) has a person ?ENTITY2 that participates in its activities. This need not represent an employment role nor imply financial incentives between the organisation and person.</rdfs:comment>
        <rdfs:label xml:lang="en">has member</rdfs:label>
        <rdfs:seeAlso rdf:resource="http://w3id.org/um/cbcm/eu-cm-ontology#employs"/>
    </owl:ObjectProperty>
    


    <!-- http://w3id.org/um/cbcm/eu-cm-ontology#hasMergingCompany -->

    <owl:ObjectProperty rdf:about="http://w3id.org/um/cbcm/eu-cm-ontology#hasMergingCompany">
        <rdfs:subPropertyOf rdf:resource="http://w3id.org/um/cbcm/eu-cm-ontology#hasTransactionInput"/>
        <rdfs:domain rdf:resource="http://w3id.org/um/cbcm/eu-cm-ontology#CompanyMerger"/>
        <rdfs:range rdf:resource="http://w3id.org/um/cbcm/eu-cm-ontology#Company"/>
        <cbcm:example>(hasMergingCompany crossBorderMerger1 company1)</cbcm:example>
        <rdfs:comment xml:lang="en">(hasMergingCompany ?ENTITY1 ?ENTITY2) means that some company merger transaction ?ENTITY1 involves a company ?ENTITY2 which will be dissolved during the process of ?ENTITY1 and will be acquired (via a universal transfer of assets and liabilities) by another distinct company involved in ?ENTITY1.</rdfs:comment>
        <rdfs:label xml:lang="en">has merging company</rdfs:label>
        <rdfs:seeAlso rdf:resource="http://w3id.org/um/cbcm/eu-cm-ontology#AcquiringCompany"/>
        <rdfs:seeAlso rdf:resource="http://w3id.org/um/cbcm/eu-cm-ontology#CompanyMerger"/>
        <rdfs:seeAlso rdf:resource="http://w3id.org/um/cbcm/eu-cm-ontology#MergingCompany"/>
    </owl:ObjectProperty>
    


    <!-- http://w3id.org/um/cbcm/eu-cm-ontology#hasOriginalCompany -->

    <owl:ObjectProperty rdf:about="http://w3id.org/um/cbcm/eu-cm-ontology#hasOriginalCompany">
        <rdfs:subPropertyOf rdf:resource="http://w3id.org/um/cbcm/eu-cm-ontology#hasTransactionInput"/>
        <rdfs:domain rdf:resource="http://w3id.org/um/cbcm/eu-cm-ontology#CompanyDivision"/>
        <rdfs:range rdf:resource="http://w3id.org/um/cbcm/eu-cm-ontology#Company"/>
        <cbcm:example>(hasOriginalCompany crossBorderDivision1 company1)</cbcm:example>
        <rdfs:comment xml:lang="en">(hasOriginalCompany ?ENTITY1 ?ENTITY2) means that some company division transaction ?ENTITY1 involves a company ?ENTITY2 which will be divided (or &quot;split&quot;) into multiple recipient or emerging companies.</rdfs:comment>
        <rdfs:label xml:lang="en">has original company</rdfs:label>
        <rdfs:seeAlso rdf:resource="http://w3id.org/um/cbcm/eu-cm-ontology#CompanyDivision"/>
        <rdfs:seeAlso rdf:resource="http://w3id.org/um/cbcm/eu-cm-ontology#EmergingCompany"/>
        <rdfs:seeAlso rdf:resource="http://w3id.org/um/cbcm/eu-cm-ontology#OriginalCompany"/>
        <rdfs:seeAlso rdf:resource="http://w3id.org/um/cbcm/eu-cm-ontology#RecipientCompany"/>
    </owl:ObjectProperty>
    


    <!-- http://w3id.org/um/cbcm/eu-cm-ontology#hasParentCompany -->

    <owl:ObjectProperty rdf:about="http://w3id.org/um/cbcm/eu-cm-ontology#hasParentCompany">
        <rdfs:subPropertyOf rdf:resource="http://w3id.org/um/cbcm/eu-cm-ontology#cbcmOrganisationRelation"/>
        <owl:inverseOf rdf:resource="http://w3id.org/um/cbcm/eu-cm-ontology#hasSubsidiaryCompany"/>
        <rdfs:domain rdf:resource="http://w3id.org/um/cbcm/eu-cm-ontology#Company"/>
        <rdfs:range rdf:resource="http://w3id.org/um/cbcm/eu-cm-ontology#Company"/>
        <cbcm:example xml:lang="en">(hasParentCompany company1 company2)</cbcm:example>
        <rdfs:comment xml:lang="en">(hasParentCompany ?ENTITY1 ?ENTITY2) means that some company ?ENTITY1 is owned and under direct or indirect control by the company ?ENTITY2.</rdfs:comment>
        <rdfs:label xml:lang="en">has parent company</rdfs:label>
        <rdfs:seeAlso rdf:resource="http://w3id.org/um/cbcm/eu-cm-ontology#hasSubsidiaryCompany"/>
    </owl:ObjectProperty>
    


    <!-- http://w3id.org/um/cbcm/eu-cm-ontology#hasPart -->

    <owl:ObjectProperty rdf:about="http://w3id.org/um/cbcm/eu-cm-ontology#hasPart">
        <rdfs:subPropertyOf rdf:resource="http://w3id.org/um/cbcm/eu-cm-ontology#cbcmEntityRelation"/>
        <owl:inverseOf rdf:resource="http://w3id.org/um/cbcm/eu-cm-ontology#partOf"/>
        <rdfs:comment xml:lang="en">(hasPart ?ENTITY1 ?ENTITY2) means that the entity referred to by ?ENTITY1 has a constituent entity referred to by ?ENTITY2.</rdfs:comment>
        <rdfs:label xml:lang="en">has part</rdfs:label>
        <rdfs:seeAlso rdf:resource="http://w3id.org/um/cbcm/eu-cm-ontology#partOf"/>
    </owl:ObjectProperty>
    


    <!-- http://w3id.org/um/cbcm/eu-cm-ontology#hasPrimaryRegistrationLocation -->

    <owl:ObjectProperty rdf:about="http://w3id.org/um/cbcm/eu-cm-ontology#hasPrimaryRegistrationLocation">
        <rdfs:subPropertyOf rdf:resource="http://w3id.org/um/cbcm/eu-cm-ontology#locatedIn"/>
        <rdfs:domain rdf:resource="http://w3id.org/um/cbcm/eu-cm-ontology#Company"/>
        <rdfs:range rdf:resource="http://w3id.org/um/cbcm/eu-cm-ontology#Country"/>
        <rdfs:comment xml:lang="en">Primary country of registration (location) of a company as a full country name</rdfs:comment>
        <rdfs:label xml:lang="en">Company primary registration location</rdfs:label>
    </owl:ObjectProperty>
    


    <!-- http://w3id.org/um/cbcm/eu-cm-ontology#hasPrimarySource -->

    <owl:ObjectProperty rdf:about="http://w3id.org/um/cbcm/eu-cm-ontology#hasPrimarySource">
        <rdfs:subPropertyOf rdf:resource="http://w3id.org/um/cbcm/eu-cm-ontology#cbcmDataProvenanceRelation"/>
        <rdfs:domain rdf:resource="http://w3id.org/um/cbcm/eu-cm-ontology#Entity"/>
        <rdfs:range rdf:resource="http://w3id.org/um/cbcm/eu-cm-ontology#Entity"/>
        <rdfs:comment xml:lang="en">Primary data source which indicates where the data was collected. A primary source could for instance be a national registry or a competent authority.</rdfs:comment>
        <rdfs:label xml:lang="en">Primary source</rdfs:label>
    </owl:ObjectProperty>
    


    <!-- http://w3id.org/um/cbcm/eu-cm-ontology#hasRecipientCompany -->

    <owl:ObjectProperty rdf:about="http://w3id.org/um/cbcm/eu-cm-ontology#hasRecipientCompany">
        <rdfs:subPropertyOf rdf:resource="http://w3id.org/um/cbcm/eu-cm-ontology#hasTransactionResult"/>
        <rdfs:domain rdf:resource="http://w3id.org/um/cbcm/eu-cm-ontology#CompanyDivision"/>
        <rdfs:range rdf:resource="http://w3id.org/um/cbcm/eu-cm-ontology#Company"/>
        <cbcm:example>(hasMergingCompany crossBorderMerger1 company1)</cbcm:example>
        <rdfs:comment xml:lang="en">(hasRecipientCompany ?ENTITY1 ?ENTITY2) means that some company division transaction ?ENTITY1 produces two or more distinct companies, one of which is ?ENTITY2 (a so-called &quot;recipient company&quot;).</rdfs:comment>
        <rdfs:label xml:lang="en">has recipient company</rdfs:label>
        <rdfs:seeAlso rdf:resource="http://w3id.org/um/cbcm/eu-cm-ontology#AcquiringCompany"/>
        <rdfs:seeAlso rdf:resource="http://w3id.org/um/cbcm/eu-cm-ontology#CompanyMerger"/>
        <rdfs:seeAlso rdf:resource="http://w3id.org/um/cbcm/eu-cm-ontology#MergingCompany"/>
    </owl:ObjectProperty>
    


    <!-- http://w3id.org/um/cbcm/eu-cm-ontology#hasSecondaryRegistrationLocation -->

    <owl:ObjectProperty rdf:about="http://w3id.org/um/cbcm/eu-cm-ontology#hasSecondaryRegistrationLocation">
        <rdfs:subPropertyOf rdf:resource="http://w3id.org/um/cbcm/eu-cm-ontology#locatedIn"/>
        <rdfs:domain rdf:resource="http://w3id.org/um/cbcm/eu-cm-ontology#Company"/>
        <rdfs:range rdf:resource="http://w3id.org/um/cbcm/eu-cm-ontology#Country"/>
        <rdfs:comment xml:lang="en">Country of secondary registration (location) of a company</rdfs:comment>
        <rdfs:label xml:lang="en">Company secondary registration location</rdfs:label>
    </owl:ObjectProperty>
    


    <!-- http://w3id.org/um/cbcm/eu-cm-ontology#hasSubProcedure -->

    <owl:ObjectProperty rdf:about="http://w3id.org/um/cbcm/eu-cm-ontology#hasSubProcedure">
        <rdfs:subPropertyOf rdf:resource="http://w3id.org/um/cbcm/eu-cm-ontology#cbcmTransactionRelation"/>
        <rdfs:domain rdf:resource="http://w3id.org/um/cbcm/eu-cm-ontology#CompanyTransaction"/>
        <rdfs:range rdf:resource="http://w3id.org/um/cbcm/eu-cm-ontology#Process"/>
        <cbcm:example>(hasSubProcedure seatTransfer1 changeOfCompanyAddress1)</cbcm:example>
        <rdfs:comment xml:lang="en">(hasSubProcedure ?ENTITY1 ?ENTITY2) means that some process ?ENTITY1 contains another (shorter) process ?ENTITY2 that should be completed before ?ENTITY1 can complete.</rdfs:comment>
        <rdfs:label xml:lang="en">has sub procedure</rdfs:label>
        <rdfs:seeAlso rdf:resource="http://w3id.org/um/cbcm/eu-cm-ontology#Process"/>
    </owl:ObjectProperty>
    


    <!-- http://w3id.org/um/cbcm/eu-cm-ontology#hasSubsidiaryCompany -->

    <owl:ObjectProperty rdf:about="http://w3id.org/um/cbcm/eu-cm-ontology#hasSubsidiaryCompany">
        <rdfs:subPropertyOf rdf:resource="http://w3id.org/um/cbcm/eu-cm-ontology#cbcmOrganisationRelation"/>
        <rdfs:comment xml:lang="en">(hasSubsidiaryCompany ?ENTITY1 ?ENTITY2) means (hasParentCompany ?ENTITY2 ?ENTITY1)</rdfs:comment>
        <rdfs:label xml:lang="en">has subsidiary company</rdfs:label>
        <rdfs:seeAlso rdf:resource="http://w3id.org/um/cbcm/eu-cm-ontology#hasParentCompany"/>
    </owl:ObjectProperty>
    


    <!-- http://w3id.org/um/cbcm/eu-cm-ontology#hasTransactionInput -->

    <owl:ObjectProperty rdf:about="http://w3id.org/um/cbcm/eu-cm-ontology#hasTransactionInput">
        <rdfs:subPropertyOf rdf:resource="http://w3id.org/um/cbcm/eu-cm-ontology#cbcmTransactionRelation"/>
        <owl:inverseOf rdf:resource="http://w3id.org/um/cbcm/eu-cm-ontology#isTransactionInputOf"/>
        <rdfs:domain rdf:resource="http://w3id.org/um/cbcm/eu-cm-ontology#CompanyTransaction"/>
        <rdfs:range rdf:resource="http://w3id.org/um/cbcm/eu-cm-ontology#Company"/>
        <cbcm:example>(hasTransactionInput crossBorderMerger1 company1)</cbcm:example>
        <rdfs:comment xml:lang="en">(hasTransactionInput ?ENTITY1 ?ENTITY2) means that some company transaction ?ENTITY1 has a prerequisite entity ?ENTITY2 that needs to be considered, assessed, or modified during the transaction referred to by ?ENTITY1.</rdfs:comment>
        <rdfs:label xml:lang="en">has transaction input</rdfs:label>
        <rdfs:seeAlso rdf:resource="http://w3id.org/um/cbcm/eu-cm-ontology#CompanyTransaction"/>
    </owl:ObjectProperty>
    


    <!-- http://w3id.org/um/cbcm/eu-cm-ontology#hasTransactionResult -->

    <owl:ObjectProperty rdf:about="http://w3id.org/um/cbcm/eu-cm-ontology#hasTransactionResult">
        <rdfs:subPropertyOf rdf:resource="http://w3id.org/um/cbcm/eu-cm-ontology#cbcmTransactionRelation"/>
        <owl:inverseOf rdf:resource="http://w3id.org/um/cbcm/eu-cm-ontology#isTransactionResultOf"/>
        <rdfs:domain rdf:resource="http://w3id.org/um/cbcm/eu-cm-ontology#CompanyTransaction"/>
        <rdfs:range rdf:resource="http://w3id.org/um/cbcm/eu-cm-ontology#Company"/>
        <cbcm:example>(hasTransactionResult crossBorderMerger1 acquiringCompany1)</cbcm:example>
        <cbcm:example>(hasTransactionResult crossBorderMerger1 mergerCertificate1)</cbcm:example>
        <rdfs:comment xml:lang="en">(hasTransactionResult ?ENTITY1 ?ENTITY2) means that some company transaction ?ENTITY1 has a byproduct ?ENTITY2 (e.g. a company, transaction certificate etc.) after completion of the process.</rdfs:comment>
        <rdfs:label xml:lang="en">has transaction result</rdfs:label>
        <rdfs:seeAlso rdf:resource="http://w3id.org/um/cbcm/eu-cm-ontology#CompanyTransaction"/>
    </owl:ObjectProperty>
    


    <!-- http://w3id.org/um/cbcm/eu-cm-ontology#involvesChangeOf -->

    <owl:ObjectProperty rdf:about="http://w3id.org/um/cbcm/eu-cm-ontology#involvesChangeOf">
        <rdfs:subPropertyOf rdf:resource="http://w3id.org/um/cbcm/eu-cm-ontology#cbcmEntityRelation"/>
        <rdfs:domain rdf:resource="http://w3id.org/um/cbcm/eu-cm-ontology#Process"/>
        <rdfs:range rdf:resource="http://w3id.org/um/cbcm/eu-cm-ontology#Entity"/>
        <cbcm:example xml:lang="en">(involvesChangeOf seatTransfer1 businessAddress1)</cbcm:example>
        <rdfs:comment xml:lang="en">(involvesChangeOf ?ENTITY1 ?ENTITY2) means that the process ?ENTITY1 requires the modification or alteration of the entity or object ?ENTITY2.</rdfs:comment>
        <rdfs:label xml:lang="en">involves the change of</rdfs:label>
    </owl:ObjectProperty>
    


    <!-- http://w3id.org/um/cbcm/eu-cm-ontology#involvesCountry -->

    <owl:ObjectProperty rdf:about="http://w3id.org/um/cbcm/eu-cm-ontology#involvesCountry">
        <rdfs:subPropertyOf rdf:resource="http://w3id.org/um/cbcm/eu-cm-ontology#cbcmTransactionRelation"/>
        <rdfs:domain rdf:resource="http://w3id.org/um/cbcm/eu-cm-ontology#CompanyTransaction"/>
        <rdfs:range rdf:resource="http://w3id.org/um/cbcm/eu-cm-ontology#Country"/>
        <cbcm:example>(involvesCountry crossBorderMerger1 france)</cbcm:example>
        <rdfs:comment xml:lang="en">(involvesCountry ?ENTITY1 ?ENTITY2) means that some company transaction ?ENTITY1 includes the modification of a company whose place of business is located in the country referred to by ?ENTITY2</rdfs:comment>
        <rdfs:label xml:lang="en">involves country</rdfs:label>
        <rdfs:seeAlso rdf:resource="http://w3id.org/um/cbcm/eu-cm-ontology#Company"/>
        <rdfs:seeAlso rdf:resource="http://w3id.org/um/cbcm/eu-cm-ontology#Country"/>
    </owl:ObjectProperty>

    <!-- http://w3id.org/um/cbcm/eu-cm-ontology#isCompanyFormOfCountry -->

    <owl:ObjectProperty rdf:about="http://w3id.org/um/cbcm/eu-cm-ontology#isCompanyFormOfCountry">
        <rdfs:subPropertyOf rdf:resource="http://w3id.org/um/cbcm/eu-cm-ontology#cbcmEntityRelation"/>
    </owl:ObjectProperty>
    


    <!-- http://w3id.org/um/cbcm/eu-cm-ontology#isTransactionInputOf -->

    <owl:ObjectProperty rdf:about="http://w3id.org/um/cbcm/eu-cm-ontology#isTransactionInputOf">
        <rdfs:subPropertyOf rdf:resource="http://w3id.org/um/cbcm/eu-cm-ontology#cbcmTransactionRelation"/>
        <cbcm:example rdf:resource="http://w3id.org/um/cbcm/eu-cm-ontology#hasTransactionInput"/>
        <rdfs:comment xml:lang="en">(isTransactionInputOf ?ENTITY1 ?ENTITY2) means (hasTransactionInput ?ENTITY2 ?ENTITY1)</rdfs:comment>
        <rdfs:label xml:lang="en">is transaction input of</rdfs:label>
    </owl:ObjectProperty>
    


    <!-- http://w3id.org/um/cbcm/eu-cm-ontology#isTransactionResultOf -->

    <owl:ObjectProperty rdf:about="http://w3id.org/um/cbcm/eu-cm-ontology#isTransactionResultOf">
        <rdfs:subPropertyOf rdf:resource="http://w3id.org/um/cbcm/eu-cm-ontology#cbcmTransactionRelation"/>
        <cbcm:example rdf:resource="http://w3id.org/um/cbcm/eu-cm-ontology#hasTransactionResult"/>
        <rdfs:comment xml:lang="en">(isTransactionResultOf ?ENTITY1 ?ENTITY2) means (hasTransactionResult ?ENTITY2 ?ENTITY1)</rdfs:comment>
        <rdfs:label xml:lang="en">is transaction result of</rdfs:label>
    </owl:ObjectProperty>
    


    <!-- http://w3id.org/um/cbcm/eu-cm-ontology#issuedByOrganisation -->

    <owl:ObjectProperty rdf:about="http://w3id.org/um/cbcm/eu-cm-ontology#issuedByOrganisation">
        <rdfs:subPropertyOf rdf:resource="http://w3id.org/um/cbcm/eu-cm-ontology#cbcmDocumentRelation"/>
        <rdfs:domain rdf:resource="http://w3id.org/um/cbcm/eu-cm-ontology#CompanyMobilityDocument"/>
        <rdfs:range rdf:resource="http://w3id.org/um/cbcm/eu-cm-ontology#Organisation"/>
        <cbcm:example xml:lang="en">(issuedByOrganisation document1 organisation1)</cbcm:example>
        <rdfs:comment xml:lang="en">(issuedByOrganisation ?ENTITY1 ?ENTITY2) means that some document or publication, ?ENTITY1, was created (and possibly delivered or administered to another entity) by some entity ?ENTITY2.</rdfs:comment>
        <rdfs:label xml:lang="en">issued by organisation</rdfs:label>
    </owl:ObjectProperty>
    


    <!-- http://w3id.org/um/cbcm/eu-cm-ontology#locatedIn -->

    <owl:ObjectProperty rdf:about="http://w3id.org/um/cbcm/eu-cm-ontology#locatedIn">
        <rdfs:subPropertyOf rdf:resource="http://w3id.org/um/cbcm/eu-cm-ontology#cbcmOrganisationRelation"/>
        <rdfs:range rdf:resource="http://w3id.org/um/cbcm/eu-cm-ontology#SpatialRegion"/>
        <rdfs:comment xml:lang="en">(locatedIn ?ENTITY1 ?ENTITY2) means that some entity ?ENTITY1 occupies the spatial region referred to by ?ENTITY2.</rdfs:comment>
        <rdfs:label xml:lang="en">located in</rdfs:label>
        <rdfs:seeAlso rdf:resource="http://w3id.org/um/cbcm/eu-cm-ontology#SpatialRegion"/>
    </owl:ObjectProperty>
    


    <!-- http://w3id.org/um/cbcm/eu-cm-ontology#maintainedBy -->

    <owl:ObjectProperty rdf:about="http://w3id.org/um/cbcm/eu-cm-ontology#maintainedBy">
        <rdfs:subPropertyOf rdf:resource="http://w3id.org/um/cbcm/eu-cm-ontology#cbcmDocumentRelation"/>
        <owl:inverseOf rdf:resource="http://w3id.org/um/cbcm/eu-cm-ontology#maintains"/>
        <cbcm:example xml:lang="en">(maintainedBy officialJournalRepository1 officialJournalAdministration1)</cbcm:example>
        <rdfs:comment xml:lang="en">(maintainedBy ?ENTITY1 ?ENTITY2) means that some digital resource ?ENTITY1 (e.g. database, website, document repository etc.) has stewardship by some agent or organisation ?ENTITY2 who is responsible for the upkeep of ?ENTITY1.</rdfs:comment>
        <rdfs:label xml:lang="en">maintained by</rdfs:label>
    </owl:ObjectProperty>
    


    <!-- http://w3id.org/um/cbcm/eu-cm-ontology#maintains -->

    <owl:ObjectProperty rdf:about="http://w3id.org/um/cbcm/eu-cm-ontology#maintains">
        <rdfs:subPropertyOf rdf:resource="http://w3id.org/um/cbcm/eu-cm-ontology#cbcmDocumentRelation"/>
        <rdfs:comment xml:lang="en">(maintains ?ENTITY1 ?ENTITY2) means (maintainedBy ?ENTITY2 ?ENTITY1)</rdfs:comment>
        <rdfs:label xml:lang="en">maintains</rdfs:label>
        <rdfs:seeAlso rdf:resource="http://w3id.org/um/cbcm/eu-cm-ontology#maintainedBy"/>
    </owl:ObjectProperty>
    


    <!-- http://w3id.org/um/cbcm/eu-cm-ontology#ownedBy -->

    <owl:ObjectProperty rdf:about="http://w3id.org/um/cbcm/eu-cm-ontology#ownedBy">
        <rdfs:subPropertyOf rdf:resource="http://w3id.org/um/cbcm/eu-cm-ontology#hasCompanyStakeholder"/>
        <owl:inverseOf rdf:resource="http://w3id.org/um/cbcm/eu-cm-ontology#owns"/>
        <cbcm:example xml:lang="en">(ownedBy company1 company2)</cbcm:example>
        <rdfs:comment xml:lang="en">(ownedBy ?ENTITY1 ?ENTITY2) means that some agent ?ENTITY2 has proprietorship over another object or organisational agent ?ENTITY1.</rdfs:comment>
        <rdfs:label xml:lang="en">owned by</rdfs:label>
        <rdfs:seeAlso rdf:resource="http://w3id.org/um/cbcm/eu-cm-ontology#owns"/>
    </owl:ObjectProperty>
    


    <!-- http://w3id.org/um/cbcm/eu-cm-ontology#owns -->

    <owl:ObjectProperty rdf:about="http://w3id.org/um/cbcm/eu-cm-ontology#owns">
        <rdfs:subPropertyOf rdf:resource="http://w3id.org/um/cbcm/eu-cm-ontology#hasCompanyStakeholder"/>
        <rdfs:domain>
            <owl:Class>
                <owl:unionOf rdf:parseType="Collection">
                    <rdf:Description rdf:about="http://w3id.org/um/cbcm/eu-cm-ontology#Organisation"/>
                    <rdf:Description rdf:about="http://w3id.org/um/cbcm/eu-cm-ontology#Person"/>
                </owl:unionOf>
            </owl:Class>
        </rdfs:domain>
        <rdfs:range rdf:resource="http://w3id.org/um/cbcm/eu-cm-ontology#Organisation"/>
        <rdfs:comment xml:lang="en">(owns ?ENTITY1 ?ENTITY2) means (owns ?ENTITY2 ?ENTITY1)</rdfs:comment>
        <rdfs:label xml:lang="en">owns</rdfs:label>
        <rdfs:seeAlso rdf:resource="http://w3id.org/um/cbcm/eu-cm-ontology#ownedBy"/>
    </owl:ObjectProperty>
    


    <!-- http://w3id.org/um/cbcm/eu-cm-ontology#partOf -->

    <owl:ObjectProperty rdf:about="http://w3id.org/um/cbcm/eu-cm-ontology#partOf">
        <rdfs:subPropertyOf rdf:resource="http://w3id.org/um/cbcm/eu-cm-ontology#cbcmEntityRelation"/>
        <rdfs:comment xml:lang="en">(partOf ?ENTITY1 ?ENTITY2) means (hasPart ?ENTITY2 ?ENTITY1)</rdfs:comment>
        <rdfs:label xml:lang="en">part of</rdfs:label>
        <rdfs:seeAlso rdf:resource="http://w3id.org/um/cbcm/eu-cm-ontology#hasPart"/>
    </owl:ObjectProperty>
    


    <!-- http://w3id.org/um/cbcm/eu-cm-ontology#reportedIn -->

    <owl:ObjectProperty rdf:about="http://w3id.org/um/cbcm/eu-cm-ontology#reportedIn">
        <rdfs:subPropertyOf rdf:resource="http://w3id.org/um/cbcm/eu-cm-ontology#cbcmDocumentRelation"/>
        <rdfs:domain rdf:resource="http://w3id.org/um/cbcm/eu-cm-ontology#CompanyTransaction"/>
        <rdfs:range rdf:resource="http://w3id.org/um/cbcm/eu-cm-ontology#TransactionNotice"/>
        <cbcm:example xml:lang="en">(reportedIn crossBorderMerger1 transactionNotice1)</cbcm:example>
        <rdfs:comment xml:lang="en">(reportedIn ?ENTITY1 ?ENTITY2) means that some significant event, process or statement ?ENTITY1 is published or mentioned or declared in writing in some publication, document or database ?ENTITY2.</rdfs:comment>
        <rdfs:label xml:lang="en">reported in</rdfs:label>
    </owl:ObjectProperty>
    


    <!-- http://w3id.org/um/cbcm/eu-cm-ontology#requiresDocument -->

    <owl:ObjectProperty rdf:about="http://w3id.org/um/cbcm/eu-cm-ontology#requiresDocument">
        <rdfs:subPropertyOf rdf:resource="http://w3id.org/um/cbcm/eu-cm-ontology#cbcmDocumentRelation"/>
        <rdfs:domain rdf:resource="http://w3id.org/um/cbcm/eu-cm-ontology#CompanyTransaction"/>
        <rdfs:range rdf:resource="http://w3id.org/um/cbcm/eu-cm-ontology#CompanyMobilityDocument"/>
        <cbcm:example xml:lang="en">(requiresDocument crossBorderMerger1 mergerPlan1)</cbcm:example>
        <rdfs:comment xml:lang="en">(requiresDocument ?ENTITY1 ?ENTITY2) means that some significant event or process ?ENTITY1 needs a compulsory document ?ENTITY2 to be submitted and reviewed before the process ?ENTITY1 can be completed.</rdfs:comment>
        <rdfs:label xml:lang="en">requires document</rdfs:label>
    </owl:ObjectProperty>
    


    <!-- http://w3id.org/um/cbcm/eu-cm-ontology#sourceCountry -->

    <owl:ObjectProperty rdf:about="http://w3id.org/um/cbcm/eu-cm-ontology#sourceCountry">
        <rdfs:subPropertyOf rdf:resource="http://w3id.org/um/cbcm/eu-cm-ontology#involvesCountry"/>
        <cbcm:example>(sourceCountry crossBorderMerger1 france)</cbcm:example>
        <rdfs:comment xml:lang="en">(sourceCountry ?ENTITY1 ?ENTITY2) means that some company transaction ?ENTITY1 has some transaction input (a company) whose place of business is located in the country ?ENTITY2.</rdfs:comment>
        <rdfs:label xml:lang="en">source country</rdfs:label>
        <rdfs:seeAlso rdf:resource="http://w3id.org/um/cbcm/eu-cm-ontology#Country"/>
        <rdfs:seeAlso rdf:resource="http://w3id.org/um/cbcm/eu-cm-ontology#hasTransactionInput"/>
    </owl:ObjectProperty>
    


    <!-- http://w3id.org/um/cbcm/eu-cm-ontology#targetCountry -->

    <owl:ObjectProperty rdf:about="http://w3id.org/um/cbcm/eu-cm-ontology#targetCountry">
        <rdfs:subPropertyOf rdf:resource="http://w3id.org/um/cbcm/eu-cm-ontology#involvesCountry"/>
        <cbcm:example>(targetCountry crossBorderMerger1 belgium)</cbcm:example>
        <rdfs:comment xml:lang="en">(targetCountry ?ENTITY1 ?ENTITY2) means that some company transaction ?ENTITY1 has some transaction result (a company) whose place of business is located in the country ?ENTITY2.</rdfs:comment>
        <rdfs:label xml:lang="en">target country</rdfs:label>
        <rdfs:seeAlso rdf:resource="http://w3id.org/um/cbcm/eu-cm-ontology#Country"/>
        <rdfs:seeAlso rdf:resource="http://w3id.org/um/cbcm/eu-cm-ontology#hasTransactionResult"/>
    </owl:ObjectProperty>
    


    <!-- http://w3id.org/um/cbcm/eu-cm-ontology#transactionValidatedByDocument -->

    <owl:ObjectProperty rdf:about="http://w3id.org/um/cbcm/eu-cm-ontology#transactionValidatedByDocument">
        <rdfs:subPropertyOf rdf:resource="http://w3id.org/um/cbcm/eu-cm-ontology#cbcmDocumentRelation"/>
        <rdfs:domain rdf:resource="http://w3id.org/um/cbcm/eu-cm-ontology#CompanyTransaction"/>
        <rdfs:range rdf:resource="http://w3id.org/um/cbcm/eu-cm-ontology#CompanyMobilityDocument"/>
        <cbcm:example xml:lang="en">(transactionValidatedByDocument crossBorderMerger1 mergerCertificate1)</cbcm:example>
        <rdfs:comment xml:lang="en">(transactionValidatedByDocument ?ENTITY1 ?ENTITY2) means that some company transaction ?ENTITY1 went through a process of approval and assessment through various criteria such as veracity, eligibility, legal relevance etc. and a document ?ENTITY2 was produced to prove the satisfaction of the critieria by ?ENTITY1.</rdfs:comment>
        <rdfs:label xml:lang="en">transaction validated by document</rdfs:label>
        <rdfs:seeAlso rdf:resource="http://w3id.org/um/cbcm/eu-cm-ontology#CompanyMobilityDocument"/>
        <rdfs:seeAlso rdf:resource="http://w3id.org/um/cbcm/eu-cm-ontology#CompanyTransaction"/>
    </owl:ObjectProperty>
    


    <!-- http://w3id.org/um/cbcm/eu-cm-ontology#typeOfSE -->

    <owl:ObjectProperty rdf:about="http://w3id.org/um/cbcm/eu-cm-ontology#typeOfSE">
        <rdfs:subPropertyOf rdf:resource="http://w3id.org/um/cbcm/eu-cm-ontology#cbcmTransactionRelation"/>
        <rdfs:domain rdf:resource="http://w3id.org/um/cbcm/eu-cm-ontology#CompanyTransaction"/>
        <rdfs:range rdf:resource="http://w3id.org/um/cbcm/eu-cm-ontology#SEType"/>
        <rdfs:comment xml:lang="en">Variable indicating the SE-establishment mode: by merger, conversion, holding-SE, subsidiary-SE or unsure</rdfs:comment>
        <rdfs:label xml:lang="en">Type of SE</rdfs:label>
    </owl:ObjectProperty>
    


    <!-- 
    ///////////////////////////////////////////////////////////////////////////////////////
    //
    // Data properties
    //
    ///////////////////////////////////////////////////////////////////////////////////////
     -->

    


    <!-- http://w3id.org/um/cbcm/eu-cm-ontology#ACEmploymentFigureAtTransaction -->

    <owl:DatatypeProperty rdf:about="http://w3id.org/um/cbcm/eu-cm-ontology#ACEmploymentFigureAtTransaction">
        <rdfs:domain rdf:resource="http://w3id.org/um/cbcm/eu-cm-ontology#CompanyTransaction"/>
        <rdfs:range rdf:resource="http://www.w3.org/2001/XMLSchema#nonNegativeInteger"/>
        <rdfs:comment xml:lang="en">number of employees of the acquiring company - at the moment of the transaction</rdfs:comment>
        <rdfs:label xml:lang="en">AC Employees count at transaction</rdfs:label>
    </owl:DatatypeProperty>
    


    <!-- http://w3id.org/um/cbcm/eu-cm-ontology#ACLastEmploymentFigure -->

    <owl:DatatypeProperty rdf:about="http://w3id.org/um/cbcm/eu-cm-ontology#ACLastEmploymentFigure">
        <rdfs:domain rdf:resource="http://w3id.org/um/cbcm/eu-cm-ontology#CompanyTransaction"/>
        <rdfs:range rdf:resource="http://www.w3.org/2001/XMLSchema#nonNegativeInteger"/>
        <rdfs:comment xml:lang="en">The last available annual employment figure for the acquiring company</rdfs:comment>
        <rdfs:label xml:lang="en">Last employment figure for the acquiring company</rdfs:label>
    </owl:DatatypeProperty>
    


    <!-- http://w3id.org/um/cbcm/eu-cm-ontology#ACTotalEUEmploymentFigure -->

    <owl:DatatypeProperty rdf:about="http://w3id.org/um/cbcm/eu-cm-ontology#ACTotalEUEmploymentFigure">
        <rdfs:domain rdf:resource="http://w3id.org/um/cbcm/eu-cm-ontology#CompanyTransaction"/>
        <rdfs:range rdf:resource="http://www.w3.org/2001/XMLSchema#nonNegativeInteger"/>
        <rdfs:comment xml:lang="en">total number of employees of the acquiring company in the EU at the moment of the transaction</rdfs:comment>
        <rdfs:label xml:lang="en">Total EU employees</rdfs:label>
    </owl:DatatypeProperty>
    


    <!-- http://w3id.org/um/cbcm/eu-cm-ontology#ACYearEmploymentFigure -->

    <owl:DatatypeProperty rdf:about="http://w3id.org/um/cbcm/eu-cm-ontology#ACYearEmploymentFigure">
        <rdfs:domain rdf:resource="http://w3id.org/um/cbcm/eu-cm-ontology#CompanyTransaction"/>
        <rdfs:range rdf:resource="http://www.w3.org/2001/XMLSchema#dateTime"/>
        <rdfs:comment xml:lang="en">The year the last annual employment figure was obtained for acquiring companies</rdfs:comment>
        <rdfs:label xml:lang="en">AC Last employment figure year</rdfs:label>
    </owl:DatatypeProperty>
    


    <!-- http://w3id.org/um/cbcm/eu-cm-ontology#BLER -->

    <owl:DatatypeProperty rdf:about="http://w3id.org/um/cbcm/eu-cm-ontology#BLER">
        <rdfs:domain rdf:resource="http://w3id.org/um/cbcm/eu-cm-ontology#CompanyTransaction"/>
        <rdfs:range rdf:resource="http://www.w3.org/2001/XMLSchema#boolean"/>
        <rdfs:comment xml:lang="en">Is an employee board level representation/participation (BLER) mechanism applicable prior to the cross-border transaction?

0 = no BLER prior to cross-border transaction
1 = BLER existing prior to cross-border transaction</rdfs:comment>
        <rdfs:label xml:lang="en">is BLER existing prior</rdfs:label>
        <rdfs:seeAlso rdf:resource="http://w3id.org/um/cbcm/eu-cm-ontology#BoardLevelEmployeeRepresentationRight"/>
    </owl:DatatypeProperty>
    


    <!-- http://w3id.org/um/cbcm/eu-cm-ontology#BLERComposition -->

    <owl:DatatypeProperty rdf:about="http://w3id.org/um/cbcm/eu-cm-ontology#BLERComposition">
        <rdfs:domain rdf:resource="http://w3id.org/um/cbcm/eu-cm-ontology#CompanyTransaction"/>
        <rdfs:range>
            <rdfs:Datatype>
                <owl:onDatatype rdf:resource="http://www.w3.org/2001/XMLSchema#float"/>
                <owl:withRestrictions rdf:parseType="Collection">
                    <rdf:Description>
                        <xsd:minInclusive rdf:datatype="http://www.w3.org/2001/XMLSchema#float">0.0</xsd:minInclusive>
                    </rdf:Description>
                    <rdf:Description>
                        <xsd:maxInclusive rdf:datatype="http://www.w3.org/2001/XMLSchema#float">1.0</xsd:maxInclusive>
                    </rdf:Description>
                </owl:withRestrictions>
            </rdfs:Datatype>
        </rdfs:range>
        <rdfs:comment xml:lang="en">What is the employee board level representation (BLER) ratio going to be after the completion of the transaction?

The ratio is ranging from 0.00 (no BLER) to 0.33 (1/3 BLER) to 0.5 (50-50 Mitbestimmung) to (theoretically) 1.00, which would be 100% employee representatives on the board and no shareholder representatives.</rdfs:comment>
        <rdfs:label xml:lang="en">BLER composition</rdfs:label>
    </owl:DatatypeProperty>
    


    <!-- http://w3id.org/um/cbcm/eu-cm-ontology#EWC -->

    <owl:DatatypeProperty rdf:about="http://w3id.org/um/cbcm/eu-cm-ontology#EWC">
        <rdfs:domain rdf:resource="http://w3id.org/um/cbcm/eu-cm-ontology#Company"/>
        <rdfs:range rdf:resource="http://www.w3.org/2001/XMLSchema#boolean"/>
        <rdfs:comment xml:lang="en">Is the company having a European Works Council (EWC)?</rdfs:comment>
        <rdfs:label xml:lang="en">Has EWC</rdfs:label>
    </owl:DatatypeProperty>
    


    <!-- http://w3id.org/um/cbcm/eu-cm-ontology#MCEmploymentFigureAtTransaction -->

    <owl:DatatypeProperty rdf:about="http://w3id.org/um/cbcm/eu-cm-ontology#MCEmploymentFigureAtTransaction">
        <rdfs:domain rdf:resource="http://w3id.org/um/cbcm/eu-cm-ontology#CompanyTransaction"/>
        <rdfs:range rdf:resource="http://www.w3.org/2001/XMLSchema#nonNegativeInteger"/>
        <rdfs:comment xml:lang="en">Number of employees of the acquiring company - at the moment of the transaction</rdfs:comment>
        <rdfs:label xml:lang="en">MC Employees count at transaction</rdfs:label>
    </owl:DatatypeProperty>
    


    <!-- http://w3id.org/um/cbcm/eu-cm-ontology#MCLastEmploymentFigure -->

    <owl:DatatypeProperty rdf:about="http://w3id.org/um/cbcm/eu-cm-ontology#MCLastEmploymentFigure">
        <rdfs:domain rdf:resource="http://w3id.org/um/cbcm/eu-cm-ontology#CompanyTransaction"/>
        <rdfs:range rdf:resource="http://www.w3.org/2001/XMLSchema#nonNegativeInteger"/>
        <rdfs:comment xml:lang="en">The last available annual employment figure for the merging company</rdfs:comment>
        <rdfs:label xml:lang="en">Last employment figure for the merging company</rdfs:label>
    </owl:DatatypeProperty>
    


    <!-- http://w3id.org/um/cbcm/eu-cm-ontology#MCYearEmploymentFigure -->

    <owl:DatatypeProperty rdf:about="http://w3id.org/um/cbcm/eu-cm-ontology#MCYearEmploymentFigure">
        <rdfs:domain rdf:resource="http://w3id.org/um/cbcm/eu-cm-ontology#CompanyTransaction"/>
        <rdfs:range rdf:resource="http://www.w3.org/2001/XMLSchema#dateTime"/>
        <rdfs:comment xml:lang="en">The year the last annual employment figure was obtained for merging companies</rdfs:comment>
        <rdfs:label xml:lang="en">MC Last employment figure year</rdfs:label>
    </owl:DatatypeProperty>
    


    <!-- http://w3id.org/um/cbcm/eu-cm-ontology#NACECode -->

    <owl:DatatypeProperty rdf:about="http://w3id.org/um/cbcm/eu-cm-ontology#NACECode">
        <rdfs:domain rdf:resource="http://w3id.org/um/cbcm/eu-cm-ontology#Company"/>
        <rdfs:range>
            <rdfs:Datatype>
                <owl:onDatatype rdf:resource="http://www.w3.org/2001/XMLSchema#positiveInteger"/>
                <owl:withRestrictions rdf:parseType="Collection">
                    <rdf:Description>
                        <xsd:minInclusive rdf:datatype="http://www.w3.org/2001/XMLSchema#positiveInteger">1000</xsd:minInclusive>
                    </rdf:Description>
                    <rdf:Description>
                        <xsd:maxInclusive rdf:datatype="http://www.w3.org/2001/XMLSchema#positiveInteger">9999</xsd:maxInclusive>
                    </rdf:Description>
                </owl:withRestrictions>
            </rdfs:Datatype>
        </rdfs:range>
        <rdfs:comment xml:lang="en">NACE Classification Code for companies. NACE (Nomenclature des Activités Économiques dans la Communauté Européenne) is a European industry standard classification system similar in function to Standard Industry Classification (SIC) and North American Industry Classification System (NAICS) for classifying business activities. From EUROSTAT</rdfs:comment>
        <rdfs:label xml:lang="en">NACE code</rdfs:label>
    </owl:DatatypeProperty>
    


    <!-- http://w3id.org/um/cbcm/eu-cm-ontology#NACESector -->

    <owl:DatatypeProperty rdf:about="http://w3id.org/um/cbcm/eu-cm-ontology#NACESector">
        <rdfs:domain rdf:resource="http://w3id.org/um/cbcm/eu-cm-ontology#Company"/>
        <rdfs:range>
            <rdfs:Datatype>
                <owl:onDatatype rdf:resource="http://www.w3.org/2001/XMLSchema#string"/>
                <owl:withRestrictions rdf:parseType="Collection">
                    <rdf:Description>
                        <xsd:length rdf:datatype="http://www.w3.org/2001/XMLSchema#positiveInteger">1</xsd:length>
                    </rdf:Description>
                </owl:withRestrictions>
            </rdfs:Datatype>
        </rdfs:range>
        <rdfs:comment xml:lang="en">Company NACE sector. NACE (Nomenclature of Economic Activities) is the European statistical classification of economic activities. Classification of a company according to which kinds of sector (i.e. industry / market / product type) they deal in. From EUROSTAT</rdfs:comment>
        <rdfs:label xml:lang="en">NACE sector</rdfs:label>
    </owl:DatatypeProperty>
    


    <!-- http://w3id.org/um/cbcm/eu-cm-ontology#SNBVoluntaryApplication -->

    <owl:DatatypeProperty rdf:about="http://w3id.org/um/cbcm/eu-cm-ontology#SNBVoluntaryApplication">
        <rdfs:domain rdf:resource="http://w3id.org/um/cbcm/eu-cm-ontology#CompanyTransaction"/>
        <rdfs:range rdf:resource="http://www.w3.org/2001/XMLSchema#string"/>
        <rdfs:comment xml:lang="en">Is a Special Negotiating Body (SNB) set up voluntary?

Whether or not a SNB is created/will be created voluntarily.

- Yes: an SNB is created voluntarily;
- No: no voluntary SNB set up;
- Not applicable: the conditions are not met (e.g. no employees, BLER threshold not met) for this criterion to be applicable;
- Unclear: the wording of the document is unclear with regard to the impact/effect/measures taken;
- Not mentioned: given the parameters, this aspect should be addressed in the transaction document, but is not mentioned</rdfs:comment>
        <rdfs:label xml:lang="en">SNB voluntary application</rdfs:label>
    </owl:DatatypeProperty>
    


    <!-- http://w3id.org/um/cbcm/eu-cm-ontology#TNIC -->

    <owl:DatatypeProperty rdf:about="http://w3id.org/um/cbcm/eu-cm-ontology#TNIC">
        <rdfs:domain rdf:resource="http://w3id.org/um/cbcm/eu-cm-ontology#Company"/>
        <rdfs:range rdf:resource="http://www.w3.org/2001/XMLSchema#boolean"/>
        <rdfs:comment xml:lang="en">Is the company having a transnational information and consultation agreement in place? Does the company have an internal body which discusses employee rights and welfare?

Different from works council. TNIC is global.</rdfs:comment>
        <rdfs:label xml:lang="en">Has TNIC</rdfs:label>
    </owl:DatatypeProperty>
    


    <!-- http://w3id.org/um/cbcm/eu-cm-ontology#WWEmploymentFigureAtTransaction -->

    <owl:DatatypeProperty rdf:about="http://w3id.org/um/cbcm/eu-cm-ontology#WWEmploymentFigureAtTransaction">
        <rdfs:domain rdf:resource="http://w3id.org/um/cbcm/eu-cm-ontology#CompanyTransaction"/>
        <rdfs:range rdf:resource="http://www.w3.org/2001/XMLSchema#nonNegativeInteger"/>
        <rdfs:comment xml:lang="en">number of employees of company group worldwide at the moment of the transaction</rdfs:comment>
        <rdfs:label xml:lang="en">Total WW employees at transaction</rdfs:label>
    </owl:DatatypeProperty>
    


    <!-- http://w3id.org/um/cbcm/eu-cm-ontology#companiesHaveEconomicCommittee -->

    <owl:DatatypeProperty rdf:about="http://w3id.org/um/cbcm/eu-cm-ontology#companiesHaveEconomicCommittee">
        <rdfs:domain rdf:resource="http://w3id.org/um/cbcm/eu-cm-ontology#CompanyTransaction"/>
        <rdfs:range rdf:resource="http://www.w3.org/2001/XMLSchema#boolean"/>
        <rdfs:comment xml:lang="en">Are the companies involved in the transaction having an economic committee?

An economic committee advises the work council about the financial parts of the transaction.</rdfs:comment>
        <rdfs:label xml:lang="en">Companies have Economic Committee</rdfs:label>
    </owl:DatatypeProperty>
    


    <!-- http://w3id.org/um/cbcm/eu-cm-ontology#companiesHaveEmployees -->

    <owl:DatatypeProperty rdf:about="http://w3id.org/um/cbcm/eu-cm-ontology#companiesHaveEmployees">
        <rdfs:domain rdf:resource="http://w3id.org/um/cbcm/eu-cm-ontology#CompanyTransaction"/>
        <rdfs:range rdf:resource="http://www.w3.org/2001/XMLSchema#boolean"/>
        <rdfs:comment xml:lang="en">Are the companies involved in the transaction having employees? Only one company needs to have employees for this property to be true</rdfs:comment>
        <rdfs:label xml:lang="en">Companies have employees</rdfs:label>
    </owl:DatatypeProperty>
    


    <!-- http://w3id.org/um/cbcm/eu-cm-ontology#companiesHaveWorksCouncil -->

    <owl:DatatypeProperty rdf:about="http://w3id.org/um/cbcm/eu-cm-ontology#companiesHaveWorksCouncil">
        <rdfs:domain rdf:resource="http://w3id.org/um/cbcm/eu-cm-ontology#CompanyTransaction"/>
        <rdfs:range rdf:resource="http://www.w3.org/2001/XMLSchema#boolean"/>
        <rdfs:comment xml:lang="en">Are the companies involved in the transaction having a works council? Works councils safeguard employees&apos; welfare</rdfs:comment>
        <rdfs:label xml:lang="en">Companies have Works Council</rdfs:label>
    </owl:DatatypeProperty>
    


    <!-- http://w3id.org/um/cbcm/eu-cm-ontology#divergingEmploymentFigure -->

    <owl:DatatypeProperty rdf:about="http://w3id.org/um/cbcm/eu-cm-ontology#divergingEmploymentFigure">
        <rdfs:domain rdf:resource="http://w3id.org/um/cbcm/eu-cm-ontology#CompanyTransaction"/>
        <rdfs:range rdf:resource="http://www.w3.org/2001/XMLSchema#nonNegativeInteger"/>
        <rdfs:comment xml:lang="en">If a different employee number for the acquiring company is found, it is recorded in this field</rdfs:comment>
        <rdfs:label xml:lang="en">Diverging employment figure</rdfs:label>
    </owl:DatatypeProperty>
    


    <!-- http://w3id.org/um/cbcm/eu-cm-ontology#generatedAtTime -->

    <owl:DatatypeProperty rdf:about="http://w3id.org/um/cbcm/eu-cm-ontology#generatedAtTime">
        <rdfs:domain rdf:resource="http://w3id.org/um/cbcm/eu-cm-ontology#Entity"/>
        <rdfs:range rdf:resource="http://www.w3.org/2001/XMLSchema#dateTime"/>
        <rdfs:comment xml:lang="en">The date and time at which an entity was generated by a process</rdfs:comment>
        <rdfs:label xml:lang="en">Generated at time</rdfs:label>
    </owl:DatatypeProperty>
    


    <!-- http://w3id.org/um/cbcm/eu-cm-ontology#impactOnEmployees -->

    <owl:DatatypeProperty rdf:about="http://w3id.org/um/cbcm/eu-cm-ontology#impactOnEmployees">
        <rdfs:domain rdf:resource="http://w3id.org/um/cbcm/eu-cm-ontology#CompanyTransaction"/>
        <rdfs:range rdf:resource="http://www.w3.org/2001/XMLSchema#string"/>
        <rdfs:comment xml:lang="en">Is the impact on employees of the envisaged transaction specified in the transaction document (e.g. the merger plan)?

Part of merger plan that specifies how the transaction will affect employees.

- Yes: there is an impact on employees (positive or negative);
- No: no impact on employees;
- Not applicable: the conditions are not met (e.g. no employees, BLER threshold not met) for this criterion to be applicable;
- Unclear: the wording of the document is unclear with regard to the impact/effect/measures taken;
- Not mentioned: given the parameters, this aspect should be addressed in the transaction document, but is not mentioned</rdfs:comment>
        <rdfs:label xml:lang="en">Impact on employees</rdfs:label>
    </owl:DatatypeProperty>
    


    <!-- http://w3id.org/um/cbcm/eu-cm-ontology#isListed -->

    <owl:DatatypeProperty rdf:about="http://w3id.org/um/cbcm/eu-cm-ontology#isListed">
        <rdfs:domain rdf:resource="http://w3id.org/um/cbcm/eu-cm-ontology#Company"/>
        <rdfs:range rdf:resource="http://www.w3.org/2001/XMLSchema#boolean"/>
        <rdfs:comment xml:lang="en">Whether the company is publicly listed. A company whose shares are bought and sold on a particular stock market.</rdfs:comment>
        <rdfs:label xml:lang="en">Is listed</rdfs:label>
    </owl:DatatypeProperty>
    


    <!-- http://w3id.org/um/cbcm/eu-cm-ontology#isSECreation -->

    <owl:DatatypeProperty rdf:about="http://w3id.org/um/cbcm/eu-cm-ontology#isSECreation">
        <rdfs:domain rdf:resource="http://w3id.org/um/cbcm/eu-cm-ontology#CompanyTransaction"/>
        <rdfs:range rdf:resource="http://www.w3.org/2001/XMLSchema#boolean"/>
        <rdfs:comment xml:lang="en">Variable indicating whether this case concerns an SE-creation (yes/no) to distinguish creations of SEs from other transactions</rdfs:comment>
        <rdfs:label xml:lang="en">Is SE creation</rdfs:label>
    </owl:DatatypeProperty>
    


    <!-- http://w3id.org/um/cbcm/eu-cm-ontology#lastWWEmploymentFigure -->

    <owl:DatatypeProperty rdf:about="http://w3id.org/um/cbcm/eu-cm-ontology#lastWWEmploymentFigure">
        <rdfs:domain rdf:resource="http://w3id.org/um/cbcm/eu-cm-ontology#Company"/>
        <rdfs:range rdf:resource="http://www.w3.org/2001/XMLSchema#nonNegativeInteger"/>
        <rdfs:comment xml:lang="en">Last available employment figure for the total worldwide employees</rdfs:comment>
        <rdfs:label xml:lang="en">Last WW employment figure</rdfs:label>
    </owl:DatatypeProperty>
    


    <!-- http://w3id.org/um/cbcm/eu-cm-ontology#lawfirm -->

    <owl:DatatypeProperty rdf:about="http://w3id.org/um/cbcm/eu-cm-ontology#lawfirm">
        <rdfs:domain rdf:resource="http://w3id.org/um/cbcm/eu-cm-ontology#CompanyTransaction"/>
        <rdfs:range rdf:resource="http://www.w3.org/2001/XMLSchema#string"/>
        <rdfs:comment xml:lang="en">Name of the lawfirm involved in the transaction, if available (for internal use; cross-border divisions and seat transfers are currently not possible within an EU legal framework.)</rdfs:comment>
        <rdfs:label xml:lang="en">Law Firm</rdfs:label>
    </owl:DatatypeProperty>
    


    <!-- http://w3id.org/um/cbcm/eu-cm-ontology#multiCBM -->

    <owl:DatatypeProperty rdf:about="http://w3id.org/um/cbcm/eu-cm-ontology#multiCBM">
        <rdfs:domain rdf:resource="http://w3id.org/um/cbcm/eu-cm-ontology#CompanyTransaction"/>
        <rdfs:range rdf:resource="http://www.w3.org/2001/XMLSchema#boolean"/>
        <rdfs:comment xml:lang="en">A transaction whereby more than two companies (i.e. multiple merging companies) are involved and merged into one acquiring company</rdfs:comment>
        <rdfs:label xml:lang="en">Multi-transaction</rdfs:label>
    </owl:DatatypeProperty>
    


    <!-- http://w3id.org/um/cbcm/eu-cm-ontology#name -->

    <owl:DatatypeProperty rdf:about="http://w3id.org/um/cbcm/eu-cm-ontology#name">
        <rdfs:range rdf:resource="http://www.w3.org/2001/XMLSchema#string"/>
        <rdfs:comment xml:lang="en">The name of the organization</rdfs:comment>
        <rdfs:label xml:lang="en">Organization name</rdfs:label>
    </owl:DatatypeProperty>
    


    <!-- http://w3id.org/um/cbcm/eu-cm-ontology#natRegistrationNumber -->

    <owl:DatatypeProperty rdf:about="http://w3id.org/um/cbcm/eu-cm-ontology#natRegistrationNumber">
        <rdfs:domain rdf:resource="http://w3id.org/um/cbcm/eu-cm-ontology#Company"/>
        <rdfs:range rdf:resource="http://www.w3.org/2001/XMLSchema#string"/>
        <rdfs:comment xml:lang="en">The national registration number of an acquiring/receiving/entry company. A company registration number is a unique combination of numbers and/or letters. It is used to identify a company and verify its legal existence as an incorporated entity.</rdfs:comment>
        <rdfs:label xml:lang="en">NAT registration number</rdfs:label>
    </owl:DatatypeProperty>
    


    <!-- http://w3id.org/um/cbcm/eu-cm-ontology#negotiatedAgreement -->

    <owl:DatatypeProperty rdf:about="http://w3id.org/um/cbcm/eu-cm-ontology#negotiatedAgreement">
        <rdfs:domain rdf:resource="http://w3id.org/um/cbcm/eu-cm-ontology#CompanyTransaction"/>
        <rdfs:range rdf:resource="http://www.w3.org/2001/XMLSchema#string"/>
        <rdfs:comment xml:lang="en">Is the management of the companies involved starting the process of setting up a Special Negotiating Body (SNB) in order to reach a negotiated agreement on the future employee participation mechanism (BLER) after the transaction?

BLER (Board-Level Employee Represenation): highest level of employee involvement in a company in the supervisory board. They can take co-determine decisions of the company&apos;s management and where the company is heading.

- Yes: there is a negotiated agreement to be negotiated with the SNB;
- No: no negotiated agreement;
- Not applicable: the conditions are not met (e.g. no employees, BLER threshold not met) for this criterion to be applicable;
- Unclear: the wording of the document is unclear with regard to the impact/effect/measures taken;
- Not mentioned: given the parameters, this aspect should be addressed in the transaction document, but is not mentioned</rdfs:comment>
        <rdfs:label xml:lang="en">Has negotiated agreement</rdfs:label>
    </owl:DatatypeProperty>
    


    <!-- http://w3id.org/um/cbcm/eu-cm-ontology#rawTransactionID -->

    <owl:DatatypeProperty rdf:about="http://w3id.org/um/cbcm/eu-cm-ontology#rawTransactionID">
        <rdfs:domain rdf:resource="http://w3id.org/um/cbcm/eu-cm-ontology#CompanyTransaction"/>
        <rdfs:range rdf:resource="http://www.w3.org/2001/XMLSchema#positiveInteger"/>
        <rdfs:comment xml:lang="en">unique identifier before database entry.

This id is the old ID-structure used before entry into the CbCMdb</rdfs:comment>
        <rdfs:label xml:lang="en">Raw transaction ID</rdfs:label>
    </owl:DatatypeProperty>
    


    <!-- http://w3id.org/um/cbcm/eu-cm-ontology#registeredOffice -->

    <owl:DatatypeProperty rdf:about="http://w3id.org/um/cbcm/eu-cm-ontology#registeredOffice"/>
    


    <!-- http://w3id.org/um/cbcm/eu-cm-ontology#standardRulesApplication -->

    <owl:DatatypeProperty rdf:about="http://w3id.org/um/cbcm/eu-cm-ontology#standardRulesApplication">
        <rdfs:domain rdf:resource="http://w3id.org/um/cbcm/eu-cm-ontology#CompanyTransaction"/>
        <rdfs:range rdf:resource="http://www.w3.org/2001/XMLSchema#string"/>
        <rdfs:comment xml:lang="en">Are the standard rules applied directly without and instead of the start of negotiations with a Special Negotiating Body (SNB)?

Instead of an SNB being set up, the standard rules are applied instead.

- Yes: the standard rules are applied;
- No: standard rules ar enot applied;
- Not applicable: the conditions are not met (e.g. no employees, BLER threshold not met) for this criterion to be applicable;
- Unclear: the wording of the document is unclear with regard to the impact/effect/measures taken;
- Not mentioned: given the parameters, this aspect should be addressed in the transaction document, but is not mentioned</rdfs:comment>
        <rdfs:label xml:lang="en">Standard rules application</rdfs:label>
    </owl:DatatypeProperty>
    


    <!-- http://w3id.org/um/cbcm/eu-cm-ontology#toBeNegotiatedBLER -->

    <owl:DatatypeProperty rdf:about="http://w3id.org/um/cbcm/eu-cm-ontology#toBeNegotiatedBLER">
        <rdfs:domain rdf:resource="http://w3id.org/um/cbcm/eu-cm-ontology#CompanyTransaction"/>
        <rdfs:range rdf:resource="http://www.w3.org/2001/XMLSchema#string"/>
        <rdfs:comment xml:lang="en">Is an employee board level representation/participation (BLER) mechanism going to be re-negotiated in the process of the cross-border transaction?

- Yes: BLER be (re-)negotiated with the SNB;
- No: no BLER-(re-)negotiation;
- Not applicable: the conditions are not met (e.g. no employees, BLER threshold not met) for this criterion to be applicable;
- Unclear: the wording of the document is unclear with regard to the impact/effect/measures taken;
- Not mentioned: given the parameters, this aspect should be addressed in the transaction document, but is not mentioned</rdfs:comment>
        <rdfs:label xml:lang="en">BLER to be negotiated</rdfs:label>
    </owl:DatatypeProperty>
    


    <!-- http://w3id.org/um/cbcm/eu-cm-ontology#transactionComment -->

    <owl:DatatypeProperty rdf:about="http://w3id.org/um/cbcm/eu-cm-ontology#transactionComment">
        <rdfs:domain rdf:resource="http://w3id.org/um/cbcm/eu-cm-ontology#CompanyTransaction"/>
        <rdfs:range rdf:resource="http://www.w3.org/2001/XMLSchema#string"/>
        <rdfs:comment xml:lang="en">Notes from researcher about the transaction</rdfs:comment>
        <rdfs:label xml:lang="en">Transaction comment</rdfs:label>
    </owl:DatatypeProperty>
    


    <!-- http://w3id.org/um/cbcm/eu-cm-ontology#transactionCompletionDate -->

    <owl:DatatypeProperty rdf:about="http://w3id.org/um/cbcm/eu-cm-ontology#transactionCompletionDate">
        <rdfs:domain rdf:resource="http://w3id.org/um/cbcm/eu-cm-ontology#CompanyTransaction"/>
        <rdfs:range rdf:resource="http://www.w3.org/2001/XMLSchema#dateTime"/>
        <rdfs:comment xml:lang="en">Date on which the transaction was effectuated (the date that the competent authority e.g., business registry of that country, says that the criteria have been met by merging and acquiring companies and the merging/transferring company is dissolved).

This is the final step of a transaction process</rdfs:comment>
        <rdfs:label xml:lang="en">Transaction completion date</rdfs:label>
    </owl:DatatypeProperty>
    


    <!-- http://w3id.org/um/cbcm/eu-cm-ontology#transactionID -->

    <owl:DatatypeProperty rdf:about="http://w3id.org/um/cbcm/eu-cm-ontology#transactionID">
        <rdfs:domain rdf:resource="http://w3id.org/um/cbcm/eu-cm-ontology#CompanyTransaction"/>
        <rdfs:range rdf:resource="http://www.w3.org/2001/XMLSchema#positiveInteger"/>
        <rdfs:comment xml:lang="en">unique identifier for a transaction</rdfs:comment>
        <rdfs:label xml:lang="en">Transaction ID</rdfs:label>
    </owl:DatatypeProperty>
    


    <!-- http://w3id.org/um/cbcm/eu-cm-ontology#transactionPlan -->

    <owl:DatatypeProperty rdf:about="http://w3id.org/um/cbcm/eu-cm-ontology#transactionPlan">
        <rdfs:domain rdf:resource="http://w3id.org/um/cbcm/eu-cm-ontology#CompanyTransaction"/>
        <rdfs:range rdf:resource="http://www.w3.org/2001/XMLSchema#boolean"/>
        <rdfs:comment xml:lang="en">Is the transaction plan available for analysis?

Merger plan, Seat transfer plan or Division plan. Transaction notice is where the transaction is announced. The other documents are where the nature and details of the transaction are specified.</rdfs:comment>
        <rdfs:label xml:lang="en">Transaction plan available</rdfs:label>
    </owl:DatatypeProperty>
    


    <!-- http://w3id.org/um/cbcm/eu-cm-ontology#transactionStartDate -->

    <owl:DatatypeProperty rdf:about="http://w3id.org/um/cbcm/eu-cm-ontology#transactionStartDate">
        <rdfs:domain rdf:resource="http://w3id.org/um/cbcm/eu-cm-ontology#CompanyTransaction"/>
        <rdfs:range rdf:resource="http://www.w3.org/2001/XMLSchema#dateTime"/>
        <rdfs:comment xml:lang="en">Date of the transaction notice (document announcing the transaction) constituting the start of the transaction process. Date that the document was published (which is the important date because this is when it becomes legally binding)</rdfs:comment>
        <rdfs:label xml:lang="en">Transaction notice date</rdfs:label>
    </owl:DatatypeProperty>
    


    <!-- http://w3id.org/um/cbcm/eu-cm-ontology#website -->

    <owl:DatatypeProperty rdf:about="http://w3id.org/um/cbcm/eu-cm-ontology#website">
        <rdfs:domain rdf:resource="http://w3id.org/um/cbcm/eu-cm-ontology#Organisation"/>
        <rdfs:range rdf:resource="http://www.w3.org/2001/XMLSchema#string"/>
        <rdfs:comment xml:lang="en">Homepage of a company/organization website</rdfs:comment>
        <rdfs:label xml:lang="en">Website</rdfs:label>
    </owl:DatatypeProperty>
    


    <!-- http://w3id.org/um/cbcm/eu-cm-ontology#yearDivergingEmploymentFigure -->

    <owl:DatatypeProperty rdf:about="http://w3id.org/um/cbcm/eu-cm-ontology#yearDivergingEmploymentFigure">
        <rdfs:domain rdf:resource="http://w3id.org/um/cbcm/eu-cm-ontology#CompanyTransaction"/>
        <rdfs:range rdf:resource="http://www.w3.org/2001/XMLSchema#dateTime"/>
        <rdfs:comment xml:lang="en">The year for which a diverging employee number is recorded</rdfs:comment>
        <rdfs:label xml:lang="en">Diverging employment figure year</rdfs:label>
    </owl:DatatypeProperty>
    


    <!-- http://w3id.org/um/cbcm/eu-cm-ontology#yearWWEmploymentFigure -->

    <owl:DatatypeProperty rdf:about="http://w3id.org/um/cbcm/eu-cm-ontology#yearWWEmploymentFigure">
        <rdfs:domain rdf:resource="http://w3id.org/um/cbcm/eu-cm-ontology#CompanyTransaction"/>
        <rdfs:range rdf:resource="http://www.w3.org/2001/XMLSchema#dateTime"/>
        <rdfs:comment xml:lang="en">Year in which the last worldwide employment figure was recorded</rdfs:comment>
        <rdfs:label xml:lang="en">Last WW employment figure year</rdfs:label>
    </owl:DatatypeProperty>
    


    <!-- 
    ///////////////////////////////////////////////////////////////////////////////////////
    //
    // Classes
    //
    ///////////////////////////////////////////////////////////////////////////////////////
     -->

    


    <!-- http://w3id.org/um/cbcm/eu-cm-ontology#AcquiringCompany -->

    <owl:Class rdf:about="http://w3id.org/um/cbcm/eu-cm-ontology#AcquiringCompany">
        <rdfs:subClassOf rdf:resource="http://w3id.org/um/cbcm/eu-cm-ontology#Company"/>
        <rdfs:subClassOf>
            <owl:Restriction>
                <owl:onProperty rdf:resource="http://w3id.org/um/cbcm/eu-cm-ontology#isTransactionResultOf"/>
                <owl:someValuesFrom rdf:resource="http://w3id.org/um/cbcm/eu-cm-ontology#CompanyMerger"/>
            </owl:Restriction>
        </rdfs:subClassOf>
        <opla-sd:entityPosition>
            <rdf:Description>
                <opla-sd:entityPositionX rdf:datatype="http://www.w3.org/2001/XMLSchema#double">142.23301817604346</opla-sd:entityPositionX>
                <opla-sd:entityPositionY rdf:datatype="http://www.w3.org/2001/XMLSchema#double">127.8720311884132</opla-sd:entityPositionY>
                <rdfs:comment xml:lang="en">This is an entity positioning annotation generated by CoModIDE (https://comodide.com/). Removing this annotation will break rendering the CoModIDE schema diagram view.</rdfs:comment>
            </rdf:Description>
        </opla-sd:entityPosition>
        <rdfs:comment xml:lang="en">Acquiring Company means the resulting or surviving company in a transaction that takes over another, merging company.</rdfs:comment>
        <rdfs:label xml:lang="en">Acquiring company</rdfs:label>
        <rdfs:seeAlso rdf:resource="http://data.europa.eu/eli/dir/2017/1132/oj"/>
    </owl:Class>
    


    <!-- http://w3id.org/um/cbcm/eu-cm-ontology#Agent -->

    <owl:Class rdf:about="http://w3id.org/um/cbcm/eu-cm-ontology#Agent">
        <rdfs:subClassOf rdf:resource="http://w3id.org/um/cbcm/eu-cm-ontology#Entity"/>
        <opla-sd:entityPosition>
            <rdf:Description>
                <opla-sd:entityPositionX rdf:datatype="http://www.w3.org/2001/XMLSchema#double">46.82985876509674</opla-sd:entityPositionX>
                <opla-sd:entityPositionY rdf:datatype="http://www.w3.org/2001/XMLSchema#double">252.14393321570253</opla-sd:entityPositionY>
                <rdfs:comment xml:lang="en">This is an entity positioning annotation generated by CoModIDE (https://comodide.com/). Removing this annotation will break rendering the CoModIDE schema diagram view.</rdfs:comment>
            </rdf:Description>
        </opla-sd:entityPosition>
        <terms:description xml:lang="en">An entity or group of entities (either biological or non-biological) that is able to perform actions autonomously in the world.</terms:description>
        <rdfs:label>Agent</rdfs:label>
    </owl:Class>
    


    <!-- http://w3id.org/um/cbcm/eu-cm-ontology#AnnualAccount -->

    <owl:Class rdf:about="http://w3id.org/um/cbcm/eu-cm-ontology#AnnualAccount">
        <owl:equivalentClass rdf:resource="http://w3id.org/um/cbcm/eu-cm-ontology#AnnualReport"/>
        <rdfs:subClassOf rdf:resource="http://w3id.org/um/cbcm/eu-cm-ontology#CompanyMobilityDocument"/>
        <opla-sd:entityPosition>
            <rdf:Description>
                <opla-sd:entityPositionX rdf:datatype="http://www.w3.org/2001/XMLSchema#double">143.69597681603065</opla-sd:entityPositionX>
                <opla-sd:entityPositionY rdf:datatype="http://www.w3.org/2001/XMLSchema#double">191.57516634769303</opla-sd:entityPositionY>
                <rdfs:comment xml:lang="en">This is an entity positioning annotation generated by CoModIDE (https://comodide.com/). Removing this annotation will break rendering the CoModIDE schema diagram view.</rdfs:comment>
            </rdf:Description>
        </opla-sd:entityPosition>
        <rdfs:comment xml:lang="en">Annual reports measure a company&apos;s financial health. They focus on past and present financial performance, and make predictions about future prospects. The revenue and financial performance of a company.</rdfs:comment>
        <rdfs:label xml:lang="en">Annual account</rdfs:label>
    </owl:Class>
    


    <!-- http://w3id.org/um/cbcm/eu-cm-ontology#AnnualReport -->

    <owl:Class rdf:about="http://w3id.org/um/cbcm/eu-cm-ontology#AnnualReport">
        <rdfs:subClassOf rdf:resource="http://w3id.org/um/cbcm/eu-cm-ontology#CompanyMobilityDocument"/>
        <opla-sd:entityPosition>
            <rdf:Description>
                <opla-sd:entityPositionX rdf:datatype="http://www.w3.org/2001/XMLSchema#double">53.00501234049062</opla-sd:entityPositionX>
                <opla-sd:entityPositionY rdf:datatype="http://www.w3.org/2001/XMLSchema#double">249.16432506444053</opla-sd:entityPositionY>
                <rdfs:comment xml:lang="en">This is an entity positioning annotation generated by CoModIDE (https://comodide.com/). Removing this annotation will break rendering the CoModIDE schema diagram view.</rdfs:comment>
            </rdf:Description>
        </opla-sd:entityPosition>
        <rdfs:comment xml:lang="en">Annual reports measure a company&apos;s financial health. They focus on past and present financial performance, and make predictions about future prospects. The revenue and financial performance of a company.</rdfs:comment>
        <rdfs:label xml:lang="en">Annual report</rdfs:label>
    </owl:Class>
    


    <!-- http://w3id.org/um/cbcm/eu-cm-ontology#Attribute -->

    <owl:Class rdf:about="http://w3id.org/um/cbcm/eu-cm-ontology#Attribute">
        <rdfs:subClassOf rdf:resource="http://w3id.org/um/cbcm/eu-cm-ontology#Entity"/>
        <opla-sd:entityPosition>
            <rdf:Description>
                <opla-sd:entityPositionX rdf:datatype="http://www.w3.org/2001/XMLSchema#double">90.9861772743164</opla-sd:entityPositionX>
                <opla-sd:entityPositionY rdf:datatype="http://www.w3.org/2001/XMLSchema#double">109.03647135579364</opla-sd:entityPositionY>
                <rdfs:comment xml:lang="en">This is an entity positioning annotation generated by CoModIDE (https://comodide.com/). Removing this annotation will break rendering the CoModIDE schema diagram view.</rdfs:comment>
            </rdf:Description>
        </opla-sd:entityPosition>
        <terms:description xml:lang="en">An attribute is a characteristic of some entity.</terms:description>
        <rdfs:label>Attribute</rdfs:label>
    </owl:Class>
    


    <!-- http://w3id.org/um/cbcm/eu-cm-ontology#Behaviour -->

    <owl:Class rdf:about="http://w3id.org/um/cbcm/eu-cm-ontology#Behaviour">
        <rdfs:subClassOf rdf:resource="http://w3id.org/um/cbcm/eu-cm-ontology#Process"/>
        <owl:disjointWith rdf:resource="http://w3id.org/um/cbcm/eu-cm-ontology#Procedure"/>
        <opla-sd:entityPosition>
            <rdf:Description>
                <opla-sd:entityPositionX rdf:datatype="http://www.w3.org/2001/XMLSchema#double">92.06451662706473</opla-sd:entityPositionX>
                <opla-sd:entityPositionY rdf:datatype="http://www.w3.org/2001/XMLSchema#double">273.0177715932372</opla-sd:entityPositionY>
                <rdfs:comment xml:lang="en">This is an entity positioning annotation generated by CoModIDE (https://comodide.com/). Removing this annotation will break rendering the CoModIDE schema diagram view.</rdfs:comment>
            </rdf:Description>
        </opla-sd:entityPosition>
        <terms:description xml:lang="en">Behaviour is the set of actions and mannerisms made by systems (biological or otherwise) in response to stimuli or inputs, whether internal or external, conscious or subconscious, overt or covert, and voluntary or involuntary.</terms:description>
        <rdfs:label>Behaviour</rdfs:label>
    </owl:Class>
    


    <!-- http://w3id.org/um/cbcm/eu-cm-ontology#BoardLevelEmployeeRepresentationRight -->

    <owl:Class rdf:about="http://w3id.org/um/cbcm/eu-cm-ontology#BoardLevelEmployeeRepresentationRight">
        <rdfs:subClassOf rdf:resource="http://w3id.org/um/cbcm/eu-cm-ontology#SocialRight"/>
        <opla-sd:entityPosition>
            <rdf:Description>
                <opla-sd:entityPositionX rdf:datatype="http://www.w3.org/2001/XMLSchema#double">117.7666860918943</opla-sd:entityPositionX>
                <opla-sd:entityPositionY rdf:datatype="http://www.w3.org/2001/XMLSchema#double">216.65703424349607</opla-sd:entityPositionY>
                <rdfs:comment xml:lang="en">This is an entity positioning annotation generated by CoModIDE (https://comodide.com/). Removing this annotation will break rendering the CoModIDE schema diagram view.</rdfs:comment>
            </rdf:Description>
        </opla-sd:entityPosition>
        <rdfs:comment xml:lang="en">Board-level representation of employees (BLER) refers to the phenomenon where employees or their representatives elect or appoint representatives to the strategic decision-making body of a company (i.e. the supervisory board or non-executive board in a one-tier system). The BLER right requires that if such a system of BLER exists prior to a cross-border company transaction, such a right must be upheld in the acquiring/recipient company under the &quot;before-and-after-principle&quot;.</rdfs:comment>
        <rdfs:label xml:lang="en">Board-level employee representation right</rdfs:label>
        <rdfs:seeAlso rdf:resource="http://data.europa.eu/eli/dir/2017/1132/oj"/>
    </owl:Class>
    


    <!-- http://w3id.org/um/cbcm/eu-cm-ontology#BoardResolution -->

    <owl:Class rdf:about="http://w3id.org/um/cbcm/eu-cm-ontology#BoardResolution">
        <rdfs:subClassOf rdf:resource="http://w3id.org/um/cbcm/eu-cm-ontology#Resolution"/>
        <opla-sd:entityPosition>
            <rdf:Description>
                <opla-sd:entityPositionX rdf:datatype="http://www.w3.org/2001/XMLSchema#double">115.67252467915873</opla-sd:entityPositionX>
                <opla-sd:entityPositionY rdf:datatype="http://www.w3.org/2001/XMLSchema#double">107.91167534620872</opla-sd:entityPositionY>
                <rdfs:comment xml:lang="en">This is an entity positioning annotation generated by CoModIDE (https://comodide.com/). Removing this annotation will break rendering the CoModIDE schema diagram view.</rdfs:comment>
            </rdf:Description>
        </opla-sd:entityPosition>
        <rdfs:comment xml:lang="en">A Board Resolution, or Company Resolution, is a way of documenting a decision made by a Company&apos;s Board of Directors on behalf of the company. After the resolution is made during a meeting, a Board Resolution document is typically used to get the specifics of the resolution in writing.</rdfs:comment>
        <rdfs:label xml:lang="en">Board resolution</rdfs:label>
    </owl:Class>
    


    <!-- http://w3id.org/um/cbcm/eu-cm-ontology#CBCMResearcher -->

    <owl:Class rdf:about="http://w3id.org/um/cbcm/eu-cm-ontology#CBCMResearcher">
        <rdfs:subClassOf rdf:resource="http://w3id.org/um/cbcm/eu-cm-ontology#Person"/>
        <opla-sd:entityPosition>
            <rdf:Description>
                <opla-sd:entityPositionX rdf:datatype="http://www.w3.org/2001/XMLSchema#double">275.757905503565</opla-sd:entityPositionX>
                <opla-sd:entityPositionY rdf:datatype="http://www.w3.org/2001/XMLSchema#double">240.72812695479394</opla-sd:entityPositionY>
                <rdfs:comment xml:lang="en">This is an entity positioning annotation generated by CoModIDE (https://comodide.com/). Removing this annotation will break rendering the CoModIDE schema diagram view.</rdfs:comment>
            </rdf:Description>
        </opla-sd:entityPosition>
        <rdfs:comment xml:lang="en">A person that is interested in research about cross-border company mobility, and actively collects and analyses data concerning cross-border company mobility.</rdfs:comment>
        <rdfs:label xml:lang="en">Cross-border company mobility researcher</rdfs:label>
    </owl:Class>
    


    <!-- http://w3id.org/um/cbcm/eu-cm-ontology#City -->

    <owl:Class rdf:about="http://w3id.org/um/cbcm/eu-cm-ontology#City">
        <rdfs:subClassOf rdf:resource="http://w3id.org/um/cbcm/eu-cm-ontology#GeoPoliticalRegion"/>
        <rdfs:subClassOf>
            <owl:Restriction>
                <owl:onProperty rdf:resource="http://w3id.org/um/cbcm/eu-cm-ontology#locatedIn"/>
                <owl:qualifiedCardinality rdf:datatype="http://www.w3.org/2001/XMLSchema#nonNegativeInteger">1</owl:qualifiedCardinality>
                <owl:onClass rdf:resource="http://w3id.org/um/cbcm/eu-cm-ontology#Country"/>
            </owl:Restriction>
        </rdfs:subClassOf>
        <opla-sd:entityPosition>
            <rdf:Description>
                <opla-sd:entityPositionX rdf:datatype="http://www.w3.org/2001/XMLSchema#double">190.6864679082266</opla-sd:entityPositionX>
                <opla-sd:entityPositionY rdf:datatype="http://www.w3.org/2001/XMLSchema#double">133.79335356253344</opla-sd:entityPositionY>
                <rdfs:comment xml:lang="en">This is an entity positioning annotation generated by CoModIDE (https://comodide.com/). Removing this annotation will break rendering the CoModIDE schema diagram view.</rdfs:comment>
            </rdf:Description>
        </opla-sd:entityPosition>
        <rdfs:comment xml:lang="en">A city (plural &quot;cities&quot;) is a geo-political region in which there is a large human settlement. The distinction with the term &quot;town&quot; (plural &quot;towns&quot;) is that cities are generally larger than towns. Countries are generally larger than cities and, in fact, usually consist of multiple cities.</rdfs:comment>
        <rdfs:label xml:lang="en">City</rdfs:label>
    </owl:Class>
    


    <!-- http://w3id.org/um/cbcm/eu-cm-ontology#Company -->

    <owl:Class rdf:about="http://w3id.org/um/cbcm/eu-cm-ontology#Company">
        <rdfs:subClassOf rdf:resource="http://w3id.org/um/cbcm/eu-cm-ontology#Organisation"/>
        <rdfs:subClassOf>
            <owl:Restriction>
                <owl:onProperty rdf:resource="http://w3id.org/um/cbcm/eu-cm-ontology#hasMember"/>
                <owl:someValuesFrom rdf:resource="http://w3id.org/um/cbcm/eu-cm-ontology#Employee"/>
            </owl:Restriction>
        </rdfs:subClassOf>
        <rdfs:subClassOf>
            <owl:Restriction>
                <owl:onProperty rdf:resource="http://w3id.org/um/cbcm/eu-cm-ontology#hasPart"/>
                <owl:qualifiedCardinality rdf:datatype="http://www.w3.org/2001/XMLSchema#nonNegativeInteger">1</owl:qualifiedCardinality>
                <owl:onClass rdf:resource="http://w3id.org/um/cbcm/eu-cm-ontology#CompanyCentralAdministration"/>
            </owl:Restriction>
        </rdfs:subClassOf>
        <rdfs:subClassOf>
            <owl:Restriction>
                <owl:onProperty rdf:resource="http://w3id.org/um/cbcm/eu-cm-ontology#hasPart"/>
                <owl:qualifiedCardinality rdf:datatype="http://www.w3.org/2001/XMLSchema#nonNegativeInteger">1</owl:qualifiedCardinality>
                <owl:onClass rdf:resource="http://w3id.org/um/cbcm/eu-cm-ontology#CompanyRegisteredOffice"/>
            </owl:Restriction>
        </rdfs:subClassOf>
        <opla-sd:entityPosition>
            <rdf:Description>
                <opla-sd:entityPositionX rdf:datatype="http://www.w3.org/2001/XMLSchema#double">241.61522720124236</opla-sd:entityPositionX>
                <opla-sd:entityPositionY rdf:datatype="http://www.w3.org/2001/XMLSchema#double">148.61742870165108</opla-sd:entityPositionY>
                <rdfs:comment xml:lang="en">This is an entity positioning annotation generated by CoModIDE (https://comodide.com/). Removing this annotation will break rendering the CoModIDE schema diagram view.</rdfs:comment>
            </rdf:Description>
        </opla-sd:entityPosition>
        <rdfs:comment xml:lang="en">A company is a legal entity formed by a group of individuals to engage in and operate a business—commercial or industrial—enterprise. A company may be organized in various ways for tax and financial liability purposes depending on the corporate law of its jurisdiction.</rdfs:comment>
        <rdfs:label xml:lang="en">Company</rdfs:label>
    </owl:Class>
    


    <!-- http://w3id.org/um/cbcm/eu-cm-ontology#CompanyCentralAdministration -->

    <owl:Class rdf:about="http://w3id.org/um/cbcm/eu-cm-ontology#CompanyCentralAdministration">
        <owl:equivalentClass rdf:resource="http://w3id.org/um/cbcm/eu-cm-ontology#CompanyHeadQuarter"/>
        <rdfs:subClassOf rdf:resource="http://w3id.org/um/cbcm/eu-cm-ontology#OrganisationalUnit"/>
        <opla-sd:entityPosition>
            <rdf:Description>
                <opla-sd:entityPositionX rdf:datatype="http://www.w3.org/2001/XMLSchema#double">276.0115870665009</opla-sd:entityPositionX>
                <opla-sd:entityPositionY rdf:datatype="http://www.w3.org/2001/XMLSchema#double">294.9635318549822</opla-sd:entityPositionY>
                <rdfs:comment xml:lang="en">This is an entity positioning annotation generated by CoModIDE (https://comodide.com/). Removing this annotation will break rendering the CoModIDE schema diagram view.</rdfs:comment>
            </rdf:Description>
        </opla-sd:entityPosition>
        <rdfs:comment xml:lang="en">The headquarters or body of a company which governs it&apos;s financial and administrative activities</rdfs:comment>
        <rdfs:label xml:lang="en">Central Administration</rdfs:label>
    </owl:Class>
    


    <!-- http://w3id.org/um/cbcm/eu-cm-ontology#CompanyConversion -->

    <owl:Class rdf:about="http://w3id.org/um/cbcm/eu-cm-ontology#CompanyConversion">
        <owl:equivalentClass>
            <owl:Class>
                <owl:intersectionOf rdf:parseType="Collection">
                    <rdf:Description rdf:about="http://w3id.org/um/cbcm/eu-cm-ontology#CompanyTransaction"/>
                    <owl:Restriction>
                        <owl:onProperty rdf:resource="http://w3id.org/um/cbcm/eu-cm-ontology#hasTransactionInput"/>
                        <owl:qualifiedCardinality rdf:datatype="http://www.w3.org/2001/XMLSchema#nonNegativeInteger">1</owl:qualifiedCardinality>
                        <owl:onClass rdf:resource="http://w3id.org/um/cbcm/eu-cm-ontology#Company"/>
                    </owl:Restriction>
                    <owl:Restriction>
                        <owl:onProperty rdf:resource="http://w3id.org/um/cbcm/eu-cm-ontology#hasTransactionResult"/>
                        <owl:qualifiedCardinality rdf:datatype="http://www.w3.org/2001/XMLSchema#nonNegativeInteger">1</owl:qualifiedCardinality>
                        <owl:onClass rdf:resource="http://w3id.org/um/cbcm/eu-cm-ontology#Company"/>
                    </owl:Restriction>
                    <owl:Restriction>
                        <owl:onProperty rdf:resource="http://w3id.org/um/cbcm/eu-cm-ontology#involvesChangeOf"/>
                        <owl:qualifiedCardinality rdf:datatype="http://www.w3.org/2001/XMLSchema#nonNegativeInteger">1</owl:qualifiedCardinality>
                        <owl:onClass rdf:resource="http://w3id.org/um/cbcm/eu-cm-ontology#CompanyLegalForm"/>
                    </owl:Restriction>
                </owl:intersectionOf>
            </owl:Class>
        </owl:equivalentClass>
        <rdfs:subClassOf rdf:resource="http://w3id.org/um/cbcm/eu-cm-ontology#CompanyTransaction"/>
        <rdfs:subClassOf>
            <owl:Restriction>
                <owl:onProperty rdf:resource="http://w3id.org/um/cbcm/eu-cm-ontology#requiresDocument"/>
                <owl:someValuesFrom rdf:resource="http://w3id.org/um/cbcm/eu-cm-ontology#ConversionPlan"/>
            </owl:Restriction>
        </rdfs:subClassOf>
        <rdfs:subClassOf>
            <owl:Restriction>
                <owl:onProperty rdf:resource="http://w3id.org/um/cbcm/eu-cm-ontology#sourceCountry"/>
                <owl:someValuesFrom rdf:resource="http://w3id.org/um/cbcm/eu-cm-ontology#Country"/>
            </owl:Restriction>
        </rdfs:subClassOf>
        <rdfs:subClassOf>
            <owl:Restriction>
                <owl:onProperty rdf:resource="http://w3id.org/um/cbcm/eu-cm-ontology#targetCountry"/>
                <owl:someValuesFrom rdf:resource="http://w3id.org/um/cbcm/eu-cm-ontology#Country"/>
            </owl:Restriction>
        </rdfs:subClassOf>
        <opla-sd:entityPosition>
            <rdf:Description>
                <opla-sd:entityPositionX rdf:datatype="http://www.w3.org/2001/XMLSchema#double">139.10665490384542</opla-sd:entityPositionX>
                <opla-sd:entityPositionY rdf:datatype="http://www.w3.org/2001/XMLSchema#double">171.75380343990585</opla-sd:entityPositionY>
                <rdfs:comment xml:lang="en">This is an entity positioning annotation generated by CoModIDE (https://comodide.com/). Removing this annotation will break rendering the CoModIDE schema diagram view.</rdfs:comment>
            </rdf:Description>
        </opla-sd:entityPosition>
        <rdfs:comment xml:lang="en">The process of changing or converting the corporate structure of a company. For example, a limited liability company of one country to one of another country, or from a private to a public limited liability company, or vice-versa by means of the continuance of an entity into another entity.</rdfs:comment>
        <rdfs:label xml:lang="en">Company conversion</rdfs:label>
    </owl:Class>
    


    <!-- http://w3id.org/um/cbcm/eu-cm-ontology#CompanyDivision -->

    <owl:Class rdf:about="http://w3id.org/um/cbcm/eu-cm-ontology#CompanyDivision">
        <owl:equivalentClass>
            <owl:Class>
                <owl:intersectionOf rdf:parseType="Collection">
                    <rdf:Description rdf:about="http://w3id.org/um/cbcm/eu-cm-ontology#CompanyTransaction"/>
                    <owl:Restriction>
                        <owl:onProperty rdf:resource="http://w3id.org/um/cbcm/eu-cm-ontology#hasTransactionResult"/>
                        <owl:minQualifiedCardinality rdf:datatype="http://www.w3.org/2001/XMLSchema#nonNegativeInteger">2</owl:minQualifiedCardinality>
                        <owl:onClass rdf:resource="http://w3id.org/um/cbcm/eu-cm-ontology#Company"/>
                    </owl:Restriction>
                    <owl:Restriction>
                        <owl:onProperty rdf:resource="http://w3id.org/um/cbcm/eu-cm-ontology#hasTransactionInput"/>
                        <owl:qualifiedCardinality rdf:datatype="http://www.w3.org/2001/XMLSchema#nonNegativeInteger">1</owl:qualifiedCardinality>
                        <owl:onClass rdf:resource="http://w3id.org/um/cbcm/eu-cm-ontology#Company"/>
                    </owl:Restriction>
                </owl:intersectionOf>
            </owl:Class>
        </owl:equivalentClass>
        <rdfs:subClassOf rdf:resource="http://w3id.org/um/cbcm/eu-cm-ontology#CompanyTransaction"/>
        <rdfs:subClassOf>
            <owl:Restriction>
                <owl:onProperty rdf:resource="http://w3id.org/um/cbcm/eu-cm-ontology#hasRecipientCompany"/>
                <owl:someValuesFrom rdf:resource="http://w3id.org/um/cbcm/eu-cm-ontology#Company"/>
            </owl:Restriction>
        </rdfs:subClassOf>
        <rdfs:subClassOf>
            <owl:Restriction>
                <owl:onProperty rdf:resource="http://w3id.org/um/cbcm/eu-cm-ontology#requiresDocument"/>
                <owl:someValuesFrom rdf:resource="http://w3id.org/um/cbcm/eu-cm-ontology#DivisionPlan"/>
            </owl:Restriction>
        </rdfs:subClassOf>
        <rdfs:subClassOf>
            <owl:Restriction>
                <owl:onProperty rdf:resource="http://w3id.org/um/cbcm/eu-cm-ontology#sourceCountry"/>
                <owl:someValuesFrom rdf:resource="http://w3id.org/um/cbcm/eu-cm-ontology#Country"/>
            </owl:Restriction>
        </rdfs:subClassOf>
        <rdfs:subClassOf>
            <owl:Restriction>
                <owl:onProperty rdf:resource="http://w3id.org/um/cbcm/eu-cm-ontology#targetCountry"/>
                <owl:someValuesFrom rdf:resource="http://w3id.org/um/cbcm/eu-cm-ontology#Country"/>
            </owl:Restriction>
        </rdfs:subClassOf>
        <opla-sd:entityPosition>
            <rdf:Description>
                <opla-sd:entityPositionX rdf:datatype="http://www.w3.org/2001/XMLSchema#double">7.1808630554767</opla-sd:entityPositionX>
                <opla-sd:entityPositionY rdf:datatype="http://www.w3.org/2001/XMLSchema#double">241.6783288255424</opla-sd:entityPositionY>
                <rdfs:comment xml:lang="en">This is an entity positioning annotation generated by CoModIDE (https://comodide.com/). Removing this annotation will break rendering the CoModIDE schema diagram view.</rdfs:comment>
            </rdf:Description>
        </opla-sd:entityPosition>
        <rdfs:comment xml:lang="en">Article 160b - Division means:
a) company being divided, on being dissolved without going into liquidation, transfers all its assets and liabilities to two or more newly formed companies (‘the recipient companies’), in exchange for the issue to the members of the company being divided of securities or shares in the recipient companies and, if any, a cash payment not exceeding 10 % of the nominal value of those securities or shares or, where they have no nominal value, a cash payment not exceeding 10% of the accounting par value of their securities or shares (&apos;full division&apos;);

(b) 	a company being divided transfers part of its assets and liabilities to one or more newly formed companies (‘the recipient companies’), in exchange for the issue to the members of the company being divided of securities or shares in the recipient companies or in the company being divided or in both the recipient companies and in the company being divided, and if any a cash payment not exceeding 10 % of the nominal value of those securities or shares, or in the absence of a nominal value, a cash payment not exceeding 10 % of the accounting par value of their securities or shares (‘partial division’).
   	
(c) 	a company being divided transfers part of its assets and liabilities to one or more newly formed companies (‘the recipient companies’), in exchange for the issue of securities or shares in the recipient companies to the company being divided (‘division by separation’).</rdfs:comment>
        <rdfs:label xml:lang="en">Company division</rdfs:label>
        <rdfs:seeAlso rdf:resource="https://www.europarl.europa.eu/doceo/document/TA-8-2019-0429_EN.html"/>
    </owl:Class>
    


    <!-- http://w3id.org/um/cbcm/eu-cm-ontology#CompanyHeadQuarter -->

    <owl:Class rdf:about="http://w3id.org/um/cbcm/eu-cm-ontology#CompanyHeadQuarter">
        <rdfs:subClassOf rdf:resource="http://w3id.org/um/cbcm/eu-cm-ontology#OrganisationalUnit"/>
        <opla-sd:entityPosition>
            <rdf:Description>
                <opla-sd:entityPositionX rdf:datatype="http://www.w3.org/2001/XMLSchema#double">208.96179101635812</opla-sd:entityPositionX>
                <opla-sd:entityPositionY rdf:datatype="http://www.w3.org/2001/XMLSchema#double">248.0793141112707</opla-sd:entityPositionY>
                <rdfs:comment xml:lang="en">This is an entity positioning annotation generated by CoModIDE (https://comodide.com/). Removing this annotation will break rendering the CoModIDE schema diagram view.</rdfs:comment>
            </rdf:Description>
        </opla-sd:entityPosition>
        <rdfs:label xml:lang="en">Company headquarter</rdfs:label>
        <rdfs:seeAlso xml:lang="en">http://w3id.org/um/cbcm/eu-cm-ontology#CompanyCentralAdministration</rdfs:seeAlso>
    </owl:Class>
    


    <!-- http://w3id.org/um/cbcm/eu-cm-ontology#CompanyLegalForm -->

    <owl:Class rdf:about="http://w3id.org/um/cbcm/eu-cm-ontology#CompanyLegalForm">
        <rdfs:subClassOf rdf:resource="http://w3id.org/um/cbcm/eu-cm-ontology#Attribute"/>
        <opla-sd:entityPosition>
            <rdf:Description>
                <opla-sd:entityPositionX rdf:datatype="http://www.w3.org/2001/XMLSchema#double">214.11641253731037</opla-sd:entityPositionX>
                <opla-sd:entityPositionY rdf:datatype="http://www.w3.org/2001/XMLSchema#double">134.19157709173146</opla-sd:entityPositionY>
                <rdfs:comment xml:lang="en">This is an entity positioning annotation generated by CoModIDE (https://comodide.com/). Removing this annotation will break rendering the CoModIDE schema diagram view.</rdfs:comment>
            </rdf:Description>
        </opla-sd:entityPosition>
        <rdfs:comment xml:lang="en">Name given to describe the structure of a corporation or business in the different legal orders. For example Limited (Ltd.), Public Limited Company (PLC), Gesellschaft mit beschränkter Haftung (GmbH), Aktiengesellschaft (AG). The company legal form is regulated under national law and grants specific rights and obligations to the company stakeholders (such as shareholders, management &amp; employees).</rdfs:comment>
        <rdfs:label xml:lang="en">Company form</rdfs:label>
        <rdfs:seeAlso rdf:resource="https://www.ecb.europa.eu/stats/money/aggregates/anacredit/shared/pdf/List_of_legal_forms.xlsx"/>
    </owl:Class>
    


    <!-- http://w3id.org/um/cbcm/eu-cm-ontology#CompanyMerger -->

    <owl:Class rdf:about="http://w3id.org/um/cbcm/eu-cm-ontology#CompanyMerger">
        <owl:equivalentClass>
            <owl:Class>
                <owl:intersectionOf rdf:parseType="Collection">
                    <rdf:Description rdf:about="http://w3id.org/um/cbcm/eu-cm-ontology#CompanyTransaction"/>
                    <owl:Restriction>
                        <owl:onProperty rdf:resource="http://w3id.org/um/cbcm/eu-cm-ontology#hasTransactionInput"/>
                        <owl:minQualifiedCardinality rdf:datatype="http://www.w3.org/2001/XMLSchema#nonNegativeInteger">2</owl:minQualifiedCardinality>
                        <owl:onClass rdf:resource="http://w3id.org/um/cbcm/eu-cm-ontology#Company"/>
                    </owl:Restriction>
                    <owl:Restriction>
                        <owl:onProperty rdf:resource="http://w3id.org/um/cbcm/eu-cm-ontology#hasTransactionResult"/>
                        <owl:qualifiedCardinality rdf:datatype="http://www.w3.org/2001/XMLSchema#nonNegativeInteger">1</owl:qualifiedCardinality>
                        <owl:onClass rdf:resource="http://w3id.org/um/cbcm/eu-cm-ontology#Company"/>
                    </owl:Restriction>
                </owl:intersectionOf>
            </owl:Class>
        </owl:equivalentClass>
        <rdfs:subClassOf rdf:resource="http://w3id.org/um/cbcm/eu-cm-ontology#CompanyTransaction"/>
        <rdfs:subClassOf>
            <owl:Restriction>
                <owl:onProperty rdf:resource="http://w3id.org/um/cbcm/eu-cm-ontology#requiresDocument"/>
                <owl:someValuesFrom rdf:resource="http://w3id.org/um/cbcm/eu-cm-ontology#MergerPlan"/>
            </owl:Restriction>
        </rdfs:subClassOf>
        <opla-sd:entityPosition>
            <rdf:Description>
                <opla-sd:entityPositionX rdf:datatype="http://www.w3.org/2001/XMLSchema#double">276.9733905621957</opla-sd:entityPositionX>
                <opla-sd:entityPositionY rdf:datatype="http://www.w3.org/2001/XMLSchema#double">147.23970510616738</opla-sd:entityPositionY>
                <rdfs:comment xml:lang="en">This is an entity positioning annotation generated by CoModIDE (https://comodide.com/). Removing this annotation will break rendering the CoModIDE schema diagram view.</rdfs:comment>
            </rdf:Description>
        </opla-sd:entityPosition>
        <rdfs:comment xml:lang="en">‘merger’ in Directive (EU) 2017/1132 means an operation whereby:

(a) one or more companies, on being dissolved without going into liquidation, transfer all their assets and liabilities to another existing company, the acquiring company, in exchange for the issue to their members of securities or shares representing the capital of that other company and, if applicable, a cash payment not exceeding 10 % of the nominal value, or, in the absence of a nominal value, of the accounting par value of those securities or shares; or

(b) two or more companies, on being dissolved without going into liquidation, transfer all their assets and liabilities to a company that they form, the new company, in exchange for the issue to their members of securities or shares representing the capital of that new company and, if applicable, a cash payment not exceeding 10 % of the nominal value, or in the absence of a nominal value, of the accounting par value of those securities or shares; or

(c) a company, on being dissolved without going into liquidation, transfers all its assets and liabilities to the company holding all the securities or shares representing its capital;&quot;

(d) one or more companies, on being dissolved without going into liquidation, transfer all their assets and liabilities to another existing company, the acquiring company, without the issue of any new shares by the acquiring company, provided that one person holds directly or indirectly all the shares in the merging companies or the members of the merging companies hold their shares in the same proportion in all merging companies.&quot;;</rdfs:comment>
        <rdfs:label xml:lang="en">Company merger</rdfs:label>
    </owl:Class>
    


    <!-- http://w3id.org/um/cbcm/eu-cm-ontology#CompanyMobilityDocument -->

    <owl:Class rdf:about="http://w3id.org/um/cbcm/eu-cm-ontology#CompanyMobilityDocument">
        <rdfs:subClassOf rdf:resource="http://w3id.org/um/cbcm/eu-cm-ontology#Object"/>
        <opla-sd:entityPosition>
            <rdf:Description>
                <opla-sd:entityPositionX rdf:datatype="http://www.w3.org/2001/XMLSchema#double">179.4149954335206</opla-sd:entityPositionX>
                <opla-sd:entityPositionY rdf:datatype="http://www.w3.org/2001/XMLSchema#double">174.28300216841396</opla-sd:entityPositionY>
                <rdfs:comment xml:lang="en">This is an entity positioning annotation generated by CoModIDE (https://comodide.com/). Removing this annotation will break rendering the CoModIDE schema diagram view.</rdfs:comment>
            </rdf:Description>
        </opla-sd:entityPosition>
        <rdfs:comment xml:lang="en">A legal document which provides information related to, or influencing, a company&apos;s mobility within a specific country or across national boundaries.</rdfs:comment>
        <rdfs:label xml:lang="en">Company mobility document</rdfs:label>
    </owl:Class>
    


    <!-- http://w3id.org/um/cbcm/eu-cm-ontology#CompanyRegisteredOffice -->

    <owl:Class rdf:about="http://w3id.org/um/cbcm/eu-cm-ontology#CompanyRegisteredOffice">
        <rdfs:subClassOf rdf:resource="http://w3id.org/um/cbcm/eu-cm-ontology#GeoPoliticalRegion"/>
        <opla-sd:entityPosition>
            <rdf:Description>
                <opla-sd:entityPositionX rdf:datatype="http://www.w3.org/2001/XMLSchema#double">250.935230379447</opla-sd:entityPositionX>
                <opla-sd:entityPositionY rdf:datatype="http://www.w3.org/2001/XMLSchema#double">217.644898075059</opla-sd:entityPositionY>
                <rdfs:comment xml:lang="en">This is an entity positioning annotation generated by CoModIDE (https://comodide.com/). Removing this annotation will break rendering the CoModIDE schema diagram view.</rdfs:comment>
            </rdf:Description>
        </opla-sd:entityPosition>
        <rdfs:comment xml:lang="en">The physical address or location at which the primary business activities of a company are carried out.</rdfs:comment>
        <rdfs:label xml:lang="en">Registered office</rdfs:label>
    </owl:Class>
    


    <!-- http://w3id.org/um/cbcm/eu-cm-ontology#CompanySeatTransfer -->

    <owl:Class rdf:about="http://w3id.org/um/cbcm/eu-cm-ontology#CompanySeatTransfer">
        <owl:equivalentClass>
            <owl:Class>
                <owl:intersectionOf rdf:parseType="Collection">
                    <rdf:Description rdf:about="http://w3id.org/um/cbcm/eu-cm-ontology#CompanyTransaction"/>
                    <owl:Restriction>
                        <owl:onProperty rdf:resource="http://w3id.org/um/cbcm/eu-cm-ontology#hasTransactionInput"/>
                        <owl:qualifiedCardinality rdf:datatype="http://www.w3.org/2001/XMLSchema#nonNegativeInteger">1</owl:qualifiedCardinality>
                        <owl:onClass rdf:resource="http://w3id.org/um/cbcm/eu-cm-ontology#Company"/>
                    </owl:Restriction>
                    <owl:Restriction>
                        <owl:onProperty rdf:resource="http://w3id.org/um/cbcm/eu-cm-ontology#hasTransactionResult"/>
                        <owl:qualifiedCardinality rdf:datatype="http://www.w3.org/2001/XMLSchema#nonNegativeInteger">1</owl:qualifiedCardinality>
                        <owl:onClass rdf:resource="http://w3id.org/um/cbcm/eu-cm-ontology#Company"/>
                    </owl:Restriction>
                    <owl:Restriction>
                        <owl:onProperty rdf:resource="http://w3id.org/um/cbcm/eu-cm-ontology#involvesChangeOf"/>
                        <owl:qualifiedCardinality rdf:datatype="http://www.w3.org/2001/XMLSchema#nonNegativeInteger">1</owl:qualifiedCardinality>
                        <owl:onClass rdf:resource="http://w3id.org/um/cbcm/eu-cm-ontology#CompanyCentralAdministration"/>
                    </owl:Restriction>
                    <owl:Restriction>
                        <owl:onProperty rdf:resource="http://w3id.org/um/cbcm/eu-cm-ontology#involvesChangeOf"/>
                        <owl:qualifiedCardinality rdf:datatype="http://www.w3.org/2001/XMLSchema#nonNegativeInteger">1</owl:qualifiedCardinality>
                        <owl:onClass rdf:resource="http://w3id.org/um/cbcm/eu-cm-ontology#CompanyRegisteredOffice"/>
                    </owl:Restriction>
                </owl:intersectionOf>
            </owl:Class>
        </owl:equivalentClass>
        <rdfs:subClassOf rdf:resource="http://w3id.org/um/cbcm/eu-cm-ontology#CompanyTransaction"/>
        <rdfs:subClassOf>
            <owl:Restriction>
                <owl:onProperty rdf:resource="http://w3id.org/um/cbcm/eu-cm-ontology#requiresDocument"/>
                <owl:someValuesFrom rdf:resource="http://w3id.org/um/cbcm/eu-cm-ontology#SeatTransferPlan"/>
            </owl:Restriction>
        </rdfs:subClassOf>
        <rdfs:subClassOf>
            <owl:Restriction>
                <owl:onProperty rdf:resource="http://w3id.org/um/cbcm/eu-cm-ontology#sourceCountry"/>
                <owl:someValuesFrom rdf:resource="http://w3id.org/um/cbcm/eu-cm-ontology#Country"/>
            </owl:Restriction>
        </rdfs:subClassOf>
        <rdfs:subClassOf>
            <owl:Restriction>
                <owl:onProperty rdf:resource="http://w3id.org/um/cbcm/eu-cm-ontology#targetCountry"/>
                <owl:someValuesFrom rdf:resource="http://w3id.org/um/cbcm/eu-cm-ontology#Country"/>
            </owl:Restriction>
        </rdfs:subClassOf>
        <rdfs:subClassOf>
            <owl:Restriction>
                <owl:onProperty rdf:resource="http://w3id.org/um/cbcm/eu-cm-ontology#hasSubProcedure"/>
                <owl:qualifiedCardinality rdf:datatype="http://www.w3.org/2001/XMLSchema#nonNegativeInteger">1</owl:qualifiedCardinality>
                <owl:onClass rdf:resource="http://w3id.org/um/cbcm/eu-cm-ontology#TransferOfCentralAdministration"/>
            </owl:Restriction>
        </rdfs:subClassOf>
        <rdfs:subClassOf>
            <owl:Restriction>
                <owl:onProperty rdf:resource="http://w3id.org/um/cbcm/eu-cm-ontology#hasSubProcedure"/>
                <owl:qualifiedCardinality rdf:datatype="http://www.w3.org/2001/XMLSchema#nonNegativeInteger">1</owl:qualifiedCardinality>
                <owl:onClass rdf:resource="http://w3id.org/um/cbcm/eu-cm-ontology#TransferOfRegisteredOffice"/>
            </owl:Restriction>
        </rdfs:subClassOf>
        <rdfs:subClassOf>
            <owl:Restriction>
                <owl:onProperty rdf:resource="http://w3id.org/um/cbcm/eu-cm-ontology#hasTransactionInput"/>
                <owl:qualifiedCardinality rdf:datatype="http://www.w3.org/2001/XMLSchema#nonNegativeInteger">1</owl:qualifiedCardinality>
                <owl:onClass rdf:resource="http://w3id.org/um/cbcm/eu-cm-ontology#Company"/>
            </owl:Restriction>
        </rdfs:subClassOf>
        <rdfs:subClassOf>
            <owl:Restriction>
                <owl:onProperty rdf:resource="http://w3id.org/um/cbcm/eu-cm-ontology#hasTransactionResult"/>
                <owl:qualifiedCardinality rdf:datatype="http://www.w3.org/2001/XMLSchema#nonNegativeInteger">1</owl:qualifiedCardinality>
                <owl:onClass rdf:resource="http://w3id.org/um/cbcm/eu-cm-ontology#Company"/>
            </owl:Restriction>
        </rdfs:subClassOf>
        <opla-sd:entityPosition>
            <rdf:Description>
                <opla-sd:entityPositionX rdf:datatype="http://www.w3.org/2001/XMLSchema#double">56.79302020727886</opla-sd:entityPositionX>
                <opla-sd:entityPositionY rdf:datatype="http://www.w3.org/2001/XMLSchema#double">120.19618503015933</opla-sd:entityPositionY>
                <rdfs:comment xml:lang="en">This is an entity positioning annotation generated by CoModIDE (https://comodide.com/). Removing this annotation will break rendering the CoModIDE schema diagram view.</rdfs:comment>
            </rdf:Description>
        </opla-sd:entityPosition>
        <rdfs:comment xml:lang="en">The act of changing the location where the company’s business was managed (registered office or headquarters) or the place where that company’s primary business was actually conducted (central administration).</rdfs:comment>
        <rdfs:label xml:lang="en">Company seat transfer</rdfs:label>
    </owl:Class>
    


    <!-- http://w3id.org/um/cbcm/eu-cm-ontology#CompanyShareholder -->

    <owl:Class rdf:about="http://w3id.org/um/cbcm/eu-cm-ontology#CompanyShareholder">
        <rdfs:subClassOf rdf:resource="http://w3id.org/um/cbcm/eu-cm-ontology#CompanyStakeholder"/>
        <rdfs:subClassOf>
            <owl:Restriction>
                <owl:onProperty rdf:resource="http://w3id.org/um/cbcm/eu-cm-ontology#partOf"/>
                <owl:someValuesFrom rdf:resource="http://w3id.org/um/cbcm/eu-cm-ontology#Company"/>
            </owl:Restriction>
        </rdfs:subClassOf>
        <opla-sd:entityPosition>
            <rdf:Description/>
        </opla-sd:entityPosition>
        <rdfs:comment xml:lang="en">An individual, group, or organization that owns one or more shares in a company, and in whose name the share certificate is issued.</rdfs:comment>
        <rdfs:label xml:lang="en">Company shareholder</rdfs:label>
    </owl:Class>
    


    <!-- http://w3id.org/um/cbcm/eu-cm-ontology#CompanyStakeholder -->

    <owl:Class rdf:about="http://w3id.org/um/cbcm/eu-cm-ontology#CompanyStakeholder">
        <rdfs:subClassOf rdf:resource="http://w3id.org/um/cbcm/eu-cm-ontology#Agent"/>
        <rdfs:subClassOf>
            <owl:Class>
                <owl:unionOf rdf:parseType="Collection">
                    <rdf:Description rdf:about="http://w3id.org/um/cbcm/eu-cm-ontology#Organisation"/>
                    <rdf:Description rdf:about="http://w3id.org/um/cbcm/eu-cm-ontology#Person"/>
                </owl:unionOf>
            </owl:Class>
        </rdfs:subClassOf>
        <opla-sd:entityPosition>
            <rdf:Description>
                <opla-sd:entityPositionX rdf:datatype="http://www.w3.org/2001/XMLSchema#double">187.87257061929267</opla-sd:entityPositionX>
                <opla-sd:entityPositionY rdf:datatype="http://www.w3.org/2001/XMLSchema#double">273.08685625360033</opla-sd:entityPositionY>
                <rdfs:comment xml:lang="en">This is an entity positioning annotation generated by CoModIDE (https://comodide.com/). Removing this annotation will break rendering the CoModIDE schema diagram view.</rdfs:comment>
            </rdf:Description>
        </opla-sd:entityPosition>
        <rdfs:comment xml:lang="en">A person, group or organization that has interest or concern in an organization or company in particular. Stakeholders can affect or be affected by the company&apos;s actions, objectives and policies.</rdfs:comment>
        <rdfs:label xml:lang="en">Stakeholder in a company</rdfs:label>
    </owl:Class>
    


    <!-- http://w3id.org/um/cbcm/eu-cm-ontology#CompanyTransaction -->

    <owl:Class rdf:about="http://w3id.org/um/cbcm/eu-cm-ontology#CompanyTransaction">
        <rdfs:subClassOf rdf:resource="http://w3id.org/um/cbcm/eu-cm-ontology#Procedure"/>
        <rdfs:subClassOf>
            <owl:Restriction>
                <owl:onProperty rdf:resource="http://w3id.org/um/cbcm/eu-cm-ontology#hasTransactionResult"/>
                <owl:someValuesFrom rdf:resource="http://w3id.org/um/cbcm/eu-cm-ontology#Company"/>
            </owl:Restriction>
        </rdfs:subClassOf>
        <rdfs:subClassOf>
            <owl:Restriction>
                <owl:onProperty rdf:resource="http://w3id.org/um/cbcm/eu-cm-ontology#reportedIn"/>
                <owl:someValuesFrom rdf:resource="http://w3id.org/um/cbcm/eu-cm-ontology#TransactionNotice"/>
            </owl:Restriction>
        </rdfs:subClassOf>
        <rdfs:subClassOf>
            <owl:Restriction>
                <owl:onProperty rdf:resource="http://w3id.org/um/cbcm/eu-cm-ontology#transactionValidatedByDocument"/>
                <owl:someValuesFrom rdf:resource="http://w3id.org/um/cbcm/eu-cm-ontology#TransactionCertificate"/>
            </owl:Restriction>
        </rdfs:subClassOf>
        <opla-sd:entityPosition>
            <rdf:Description>
                <opla-sd:entityPositionX rdf:datatype="http://www.w3.org/2001/XMLSchema#double">165.18606165349766</opla-sd:entityPositionX>
                <opla-sd:entityPositionY rdf:datatype="http://www.w3.org/2001/XMLSchema#double">243.95669794464655</opla-sd:entityPositionY>
                <rdfs:comment xml:lang="en">This is an entity positioning annotation generated by CoModIDE (https://comodide.com/). Removing this annotation will break rendering the CoModIDE schema diagram view.</rdfs:comment>
            </rdf:Description>
        </opla-sd:entityPosition>
        <rdfs:comment xml:lang="en">An action taken by a company that modifies its corporate structure with a change of control (for e.g. through either a merger, division, conversion or seat transfer in a domestic or cross-border setting). It involves one or more companies, each of which have a company legal form valid in a Member State of the European Union.</rdfs:comment>
        <rdfs:label xml:lang="en">Company transaction</rdfs:label>
    </owl:Class>
    


    <!-- http://w3id.org/um/cbcm/eu-cm-ontology#CompetentAuthority -->

    <owl:Class rdf:about="http://w3id.org/um/cbcm/eu-cm-ontology#CompetentAuthority">
        <rdfs:subClassOf rdf:resource="http://w3id.org/um/cbcm/eu-cm-ontology#Organisation"/>
        <opla-sd:entityPosition>
            <rdf:Description>
                <opla-sd:entityPositionX rdf:datatype="http://www.w3.org/2001/XMLSchema#double">18.60762027636168</opla-sd:entityPositionX>
                <opla-sd:entityPositionY rdf:datatype="http://www.w3.org/2001/XMLSchema#double">158.12098050565604</opla-sd:entityPositionY>
                <rdfs:comment xml:lang="en">This is an entity positioning annotation generated by CoModIDE (https://comodide.com/). Removing this annotation will break rendering the CoModIDE schema diagram view.</rdfs:comment>
            </rdf:Description>
        </opla-sd:entityPosition>
        <rdfs:comment xml:lang="en">The monitoring of the completion and legality of the decision-making process in each company involved in a transaction is carried out by a national authority having jurisdiction over each of those companies. The national authority could be a court, a notary or any other competent authority appointed by the Member State concerned.</rdfs:comment>
        <rdfs:label xml:lang="en">Competent authority</rdfs:label>
        <rdfs:seeAlso rdf:resource="http://data.europa.eu/eli/dir/2017/1132/oj"/>
    </owl:Class>
    


    <!-- http://w3id.org/um/cbcm/eu-cm-ontology#ConsultationRight -->

    <owl:Class rdf:about="http://w3id.org/um/cbcm/eu-cm-ontology#ConsultationRight">
        <rdfs:subClassOf rdf:resource="http://w3id.org/um/cbcm/eu-cm-ontology#SocialRight"/>
        <opla-sd:entityPosition>
            <rdf:Description>
                <opla-sd:entityPositionX rdf:datatype="http://www.w3.org/2001/XMLSchema#double">60.72612280576839</opla-sd:entityPositionX>
                <opla-sd:entityPositionY rdf:datatype="http://www.w3.org/2001/XMLSchema#double">216.53692750322864</opla-sd:entityPositionY>
                <rdfs:comment xml:lang="en">This is an entity positioning annotation generated by CoModIDE (https://comodide.com/). Removing this annotation will break rendering the CoModIDE schema diagram view.</rdfs:comment>
            </rdf:Description>
        </opla-sd:entityPosition>
        <rdfs:comment xml:lang="en">The right of employees or their representatives to be consulted and to give advice on a business decision, such as an intended merger/division/conversion/seat transfer.</rdfs:comment>
        <rdfs:label xml:lang="en">Consultation right</rdfs:label>
        <rdfs:seeAlso rdf:resource="http://data.europa.eu/eli/dir/2002/14/oj"/>
        <rdfs:seeAlso rdf:resource="http://data.europa.eu/eli/dir/2017/1132/oj"/>
    </owl:Class>
    


    <!-- http://w3id.org/um/cbcm/eu-cm-ontology#ConversionCertificate -->

    <owl:Class rdf:about="http://w3id.org/um/cbcm/eu-cm-ontology#ConversionCertificate">
        <rdfs:subClassOf rdf:resource="http://w3id.org/um/cbcm/eu-cm-ontology#TransactionCertificate"/>
        <opla-sd:entityPosition>
            <rdf:Description>
                <opla-sd:entityPositionX rdf:datatype="http://www.w3.org/2001/XMLSchema#double">107.24090116681467</opla-sd:entityPositionX>
                <opla-sd:entityPositionY rdf:datatype="http://www.w3.org/2001/XMLSchema#double">97.57588854422639</opla-sd:entityPositionY>
                <rdfs:comment xml:lang="en">This is an entity positioning annotation generated by CoModIDE (https://comodide.com/). Removing this annotation will break rendering the CoModIDE schema diagram view.</rdfs:comment>
            </rdf:Description>
        </opla-sd:entityPosition>
        <rdfs:comment xml:lang="en">A document issued by a Competent Authority declaring that the legally required steps of a conversion are completed. The certificate needs to be presented by a company to either be registered in another company registry or to be removed from a company register.</rdfs:comment>
        <rdfs:label xml:lang="en">Company conversion certificate</rdfs:label>
    </owl:Class>
    


    <!-- http://w3id.org/um/cbcm/eu-cm-ontology#ConversionPlan -->

    <owl:Class rdf:about="http://w3id.org/um/cbcm/eu-cm-ontology#ConversionPlan">
        <rdfs:subClassOf rdf:resource="http://w3id.org/um/cbcm/eu-cm-ontology#TransactionDocument"/>
        <opla-sd:entityPosition>
            <rdf:Description>
                <opla-sd:entityPositionX rdf:datatype="http://www.w3.org/2001/XMLSchema#double">58.06505889581793</opla-sd:entityPositionX>
                <opla-sd:entityPositionY rdf:datatype="http://www.w3.org/2001/XMLSchema#double">291.31313144550154</opla-sd:entityPositionY>
                <rdfs:comment xml:lang="en">This is an entity positioning annotation generated by CoModIDE (https://comodide.com/). Removing this annotation will break rendering the CoModIDE schema diagram view.</rdfs:comment>
            </rdf:Description>
        </opla-sd:entityPosition>
        <rdfs:comment xml:lang="en">A document providing details of how the conversion of a company will be implemented. Article 86d: The management or administrative organ of the company shall draw up the draft terms of a cross-border conversion. The draft terms of a cross-border conversion shall include at least the particulars listed in article 86d</rdfs:comment>
        <rdfs:label xml:lang="en">Company conversion plan</rdfs:label>
        <rdfs:seeAlso rdf:resource="https://www.europarl.europa.eu/doceo/document/TA-8-2019-0429_EN.html"/>
    </owl:Class>
    


    <!-- http://w3id.org/um/cbcm/eu-cm-ontology#Country -->

    <owl:Class rdf:about="http://w3id.org/um/cbcm/eu-cm-ontology#Country">
        <rdfs:subClassOf rdf:resource="http://w3id.org/um/cbcm/eu-cm-ontology#GeoPoliticalRegion"/>
        <opla-sd:entityPosition>
            <rdf:Description>
                <opla-sd:entityPositionX rdf:datatype="http://www.w3.org/2001/XMLSchema#double">282.45502237433436</opla-sd:entityPositionX>
                <opla-sd:entityPositionY rdf:datatype="http://www.w3.org/2001/XMLSchema#double">231.05248398309334</opla-sd:entityPositionY>
                <rdfs:comment xml:lang="en">This is an entity positioning annotation generated by CoModIDE (https://comodide.com/). Removing this annotation will break rendering the CoModIDE schema diagram view.</rdfs:comment>
            </rdf:Description>
        </opla-sd:entityPosition>
        <terms:description xml:lang="en">A geo-political region that has a distinct and common political governance structure for people that inhabit it for a significant portion of their lives. The majority of people that inhabit such a region are also usually united by common descent, history, culture and language.</terms:description>
        <rdfs:label>Country</rdfs:label>
    </owl:Class>
    


    <!-- http://w3id.org/um/cbcm/eu-cm-ontology#Court -->

    <owl:Class rdf:about="http://w3id.org/um/cbcm/eu-cm-ontology#Court">
        <rdfs:subClassOf rdf:resource="http://w3id.org/um/cbcm/eu-cm-ontology#CompetentAuthority"/>
        <opla-sd:entityPosition>
            <rdf:Description>
                <opla-sd:entityPositionX rdf:datatype="http://www.w3.org/2001/XMLSchema#double">66.72994749890702</opla-sd:entityPositionX>
                <opla-sd:entityPositionY rdf:datatype="http://www.w3.org/2001/XMLSchema#double">29.763459687986888</opla-sd:entityPositionY>
                <rdfs:comment xml:lang="en">This is an entity positioning annotation generated by CoModIDE (https://comodide.com/). Removing this annotation will break rendering the CoModIDE schema diagram view.</rdfs:comment>
            </rdf:Description>
        </opla-sd:entityPosition>
        <rdfs:comment xml:lang="en">Legal forum in which a body of people presided over by a judge, judges, or magistrate, and acting as a tribunal in civil and criminal cases resolve legal disputes.</rdfs:comment>
        <rdfs:label xml:lang="en">Court</rdfs:label>
    </owl:Class>
    


    <!-- http://w3id.org/um/cbcm/eu-cm-ontology#Creditor -->

    <owl:Class rdf:about="http://w3id.org/um/cbcm/eu-cm-ontology#Creditor">
        <rdfs:subClassOf rdf:resource="http://w3id.org/um/cbcm/eu-cm-ontology#CompanyStakeholder"/>
        <opla-sd:entityPosition>
            <rdf:Description>
                <opla-sd:entityPositionX rdf:datatype="http://www.w3.org/2001/XMLSchema#double">221.92898583435658</opla-sd:entityPositionX>
                <opla-sd:entityPositionY rdf:datatype="http://www.w3.org/2001/XMLSchema#double">196.58312903470244</opla-sd:entityPositionY>
                <rdfs:comment xml:lang="en">This is an entity positioning annotation generated by CoModIDE (https://comodide.com/). Removing this annotation will break rendering the CoModIDE schema diagram view.</rdfs:comment>
            </rdf:Description>
        </opla-sd:entityPosition>
        <rdfs:comment xml:lang="en">A person, organization, or government that is owed money. A creditor&apos;s claims and the safeguarding of these creditor rights is laid down in the company law of the Member States and EU law.</rdfs:comment>
        <rdfs:label xml:lang="en">Creditor</rdfs:label>
        <rdfs:seeAlso rdf:resource="http://data.europa.eu/eli/dir/2017/1132/oj"/>
    </owl:Class>
    


    <!-- http://w3id.org/um/cbcm/eu-cm-ontology#CreditorDecisionRight -->

    <owl:Class rdf:about="http://w3id.org/um/cbcm/eu-cm-ontology#CreditorDecisionRight">
        <rdfs:subClassOf rdf:resource="http://w3id.org/um/cbcm/eu-cm-ontology#CreditorRight"/>
        <opla-sd:entityPosition>
            <rdf:Description>
                <opla-sd:entityPositionX rdf:datatype="http://www.w3.org/2001/XMLSchema#double">18.896356430331895</opla-sd:entityPositionX>
                <opla-sd:entityPositionY rdf:datatype="http://www.w3.org/2001/XMLSchema#double">293.2391048416998</opla-sd:entityPositionY>
                <rdfs:comment xml:lang="en">This is an entity positioning annotation generated by CoModIDE (https://comodide.com/). Removing this annotation will break rendering the CoModIDE schema diagram view.</rdfs:comment>
            </rdf:Description>
        </opla-sd:entityPosition>
        <rdfs:comment xml:lang="en">The right of a creditor to influence or take a decision in the context of a transaction.</rdfs:comment>
        <rdfs:label xml:lang="en">Creditor decision right</rdfs:label>
        <rdfs:seeAlso rdf:resource="http://data.europa.eu/eli/dir/2017/1132/oj"/>
    </owl:Class>
    


    <!-- http://w3id.org/um/cbcm/eu-cm-ontology#CreditorExitRight -->

    <owl:Class rdf:about="http://w3id.org/um/cbcm/eu-cm-ontology#CreditorExitRight">
        <rdfs:subClassOf rdf:resource="http://w3id.org/um/cbcm/eu-cm-ontology#CreditorRight"/>
        <opla-sd:entityPosition>
            <rdf:Description>
                <opla-sd:entityPositionX rdf:datatype="http://www.w3.org/2001/XMLSchema#double">222.20200062208355</opla-sd:entityPositionX>
                <opla-sd:entityPositionY rdf:datatype="http://www.w3.org/2001/XMLSchema#double">9.301752353902469</opla-sd:entityPositionY>
                <rdfs:comment xml:lang="en">This is an entity positioning annotation generated by CoModIDE (https://comodide.com/). Removing this annotation will break rendering the CoModIDE schema diagram view.</rdfs:comment>
            </rdf:Description>
        </opla-sd:entityPosition>
        <rdfs:comment xml:lang="en">The creditors right to be paid out and therefore to exit the company in the context of a transaction.</rdfs:comment>
        <rdfs:label xml:lang="en">Creditor exit right</rdfs:label>
        <rdfs:seeAlso rdf:resource="http://data.europa.eu/eli/dir/2017/1132/oj"/>
    </owl:Class>
    


    <!-- http://w3id.org/um/cbcm/eu-cm-ontology#CreditorInformationRight -->

    <owl:Class rdf:about="http://w3id.org/um/cbcm/eu-cm-ontology#CreditorInformationRight">
        <rdfs:subClassOf rdf:resource="http://w3id.org/um/cbcm/eu-cm-ontology#CreditorRight"/>
        <opla-sd:entityPosition>
            <rdf:Description>
                <opla-sd:entityPositionX rdf:datatype="http://www.w3.org/2001/XMLSchema#double">51.581143916293996</opla-sd:entityPositionX>
                <opla-sd:entityPositionY rdf:datatype="http://www.w3.org/2001/XMLSchema#double">284.32699686683605</opla-sd:entityPositionY>
                <rdfs:comment xml:lang="en">This is an entity positioning annotation generated by CoModIDE (https://comodide.com/). Removing this annotation will break rendering the CoModIDE schema diagram view.</rdfs:comment>
            </rdf:Description>
        </opla-sd:entityPosition>
        <rdfs:comment xml:lang="en">The information rights of creditors in the context of a company transaction, which includes for instance access to documents.</rdfs:comment>
        <rdfs:label xml:lang="en">Creditor information right</rdfs:label>
        <rdfs:seeAlso rdf:resource="http://data.europa.eu/eli/dir/2017/1132/oj"/>
    </owl:Class>
    


    <!-- http://w3id.org/um/cbcm/eu-cm-ontology#CreditorRight -->

    <owl:Class rdf:about="http://w3id.org/um/cbcm/eu-cm-ontology#CreditorRight">
        <rdfs:subClassOf rdf:resource="http://w3id.org/um/cbcm/eu-cm-ontology#TransactionRight"/>
        <rdfs:subClassOf>
            <owl:Restriction>
                <owl:onProperty rdf:resource="http://w3id.org/um/cbcm/eu-cm-ontology#applicableTo"/>
                <owl:someValuesFrom rdf:resource="http://w3id.org/um/cbcm/eu-cm-ontology#Creditor"/>
            </owl:Restriction>
        </rdfs:subClassOf>
        <opla-sd:entityPosition>
            <rdf:Description>
                <opla-sd:entityPositionX rdf:datatype="http://www.w3.org/2001/XMLSchema#double">181.12999496968988</opla-sd:entityPositionX>
                <opla-sd:entityPositionY rdf:datatype="http://www.w3.org/2001/XMLSchema#double">149.5393386146698</opla-sd:entityPositionY>
                <rdfs:comment xml:lang="en">This is an entity positioning annotation generated by CoModIDE (https://comodide.com/). Removing this annotation will break rendering the CoModIDE schema diagram view.</rdfs:comment>
            </rdf:Description>
        </opla-sd:entityPosition>
        <rdfs:comment xml:lang="en">The rights of creditors, which includes debenture holders, vis-a-vis the company that obtained credit from the individual or organisation. Legal safeguards are put in place to ensure that rights of creditors are not negatively affected by a company transaction.</rdfs:comment>
        <rdfs:label xml:lang="en">Creditor right</rdfs:label>
        <rdfs:seeAlso rdf:resource="http://data.europa.eu/eli/dir/2017/1132/oj"/>
    </owl:Class>
    


    <!-- http://w3id.org/um/cbcm/eu-cm-ontology#CreditorSecurityRight -->

    <owl:Class rdf:about="http://w3id.org/um/cbcm/eu-cm-ontology#CreditorSecurityRight">
        <rdfs:subClassOf rdf:resource="http://w3id.org/um/cbcm/eu-cm-ontology#CreditorRight"/>
        <opla-sd:entityPosition>
            <rdf:Description>
                <opla-sd:entityPositionX rdf:datatype="http://www.w3.org/2001/XMLSchema#double">270.6598611213299</opla-sd:entityPositionX>
                <opla-sd:entityPositionY rdf:datatype="http://www.w3.org/2001/XMLSchema#double">230.17239798563722</opla-sd:entityPositionY>
                <rdfs:comment xml:lang="en">This is an entity positioning annotation generated by CoModIDE (https://comodide.com/). Removing this annotation will break rendering the CoModIDE schema diagram view.</rdfs:comment>
            </rdf:Description>
        </opla-sd:entityPosition>
        <rdfs:comment xml:lang="en">Member States shall provide for an adequate system of protection of the interest of creditors, and shall ensure that creditors who are dissatisfied with the safeguards offered in the draft terms of the transaction, as provided for in Article 86d (1) point (f), may apply to the appropriate administrative or judicial authority for adequate safeguards provided that they can credibly demonstrate that due to the transaction the satisfaction of their claims is at stake and that no adequate safeguards have been obtained from the company.</rdfs:comment>
        <rdfs:label xml:lang="en">Creditor security right</rdfs:label>
        <rdfs:seeAlso rdf:resource="http://data.europa.eu/eli/dir/2017/1132/oj"/>
        <rdfs:seeAlso rdf:resource="https://www.europarl.europa.eu/doceo/document/TA-8-2019-0429_EN.html"/>
    </owl:Class>
    


    <!-- http://w3id.org/um/cbcm/eu-cm-ontology#CrossBorderConversion -->

    <owl:Class rdf:about="http://w3id.org/um/cbcm/eu-cm-ontology#CrossBorderConversion">
        <rdfs:subClassOf rdf:resource="http://w3id.org/um/cbcm/eu-cm-ontology#CompanyConversion"/>
        <rdfs:subClassOf>
            <owl:Restriction>
                <owl:onProperty rdf:resource="http://w3id.org/um/cbcm/eu-cm-ontology#hasTransactionResult"/>
                <owl:someValuesFrom rdf:resource="http://w3id.org/um/cbcm/eu-cm-ontology#Company"/>
            </owl:Restriction>
        </rdfs:subClassOf>
        <rdfs:subClassOf>
            <owl:Restriction>
                <owl:onProperty rdf:resource="http://w3id.org/um/cbcm/eu-cm-ontology#requiresDocument"/>
                <owl:someValuesFrom rdf:resource="http://w3id.org/um/cbcm/eu-cm-ontology#PreConversionCertificate"/>
            </owl:Restriction>
        </rdfs:subClassOf>
        <rdfs:subClassOf>
            <owl:Restriction>
                <owl:onProperty rdf:resource="http://w3id.org/um/cbcm/eu-cm-ontology#involvesCountry"/>
                <owl:qualifiedCardinality rdf:datatype="http://www.w3.org/2001/XMLSchema#nonNegativeInteger">2</owl:qualifiedCardinality>
                <owl:onClass rdf:resource="http://w3id.org/um/cbcm/eu-cm-ontology#Country"/>
            </owl:Restriction>
        </rdfs:subClassOf>
        <opla-sd:entityPosition>
            <rdf:Description>
                <opla-sd:entityPositionX rdf:datatype="http://www.w3.org/2001/XMLSchema#double">69.33316759149946</opla-sd:entityPositionX>
                <opla-sd:entityPositionY rdf:datatype="http://www.w3.org/2001/XMLSchema#double">221.56037559499444</opla-sd:entityPositionY>
                <rdfs:comment xml:lang="en">This is an entity positioning annotation generated by CoModIDE (https://comodide.com/). Removing this annotation will break rendering the CoModIDE schema diagram view.</rdfs:comment>
            </rdf:Description>
        </opla-sd:entityPosition>
        <rdfs:comment xml:lang="en">A cross-border conversion is an operation through which a company, formed in one country (with the EU/EEA set of countries) is converted into a company governed by the law of another.</rdfs:comment>
        <rdfs:label xml:lang="en">Cross-border conversion</rdfs:label>
    </owl:Class>
    


    <!-- http://w3id.org/um/cbcm/eu-cm-ontology#CrossBorderDivision -->

    <owl:Class rdf:about="http://w3id.org/um/cbcm/eu-cm-ontology#CrossBorderDivision">
        <owl:equivalentClass>
            <owl:Class>
                <owl:intersectionOf rdf:parseType="Collection">
                    <rdf:Description rdf:about="http://w3id.org/um/cbcm/eu-cm-ontology#CompanyDivision"/>
                    <owl:Restriction>
                        <owl:onProperty rdf:resource="http://w3id.org/um/cbcm/eu-cm-ontology#involvesCountry"/>
                        <owl:minQualifiedCardinality rdf:datatype="http://www.w3.org/2001/XMLSchema#nonNegativeInteger">2</owl:minQualifiedCardinality>
                        <owl:onClass rdf:resource="http://w3id.org/um/cbcm/eu-cm-ontology#Country"/>
                    </owl:Restriction>
                </owl:intersectionOf>
            </owl:Class>
        </owl:equivalentClass>
        <rdfs:subClassOf rdf:resource="http://w3id.org/um/cbcm/eu-cm-ontology#CompanyDivision"/>
        <opla-sd:entityPosition>
            <rdf:Description>
                <opla-sd:entityPositionX rdf:datatype="http://www.w3.org/2001/XMLSchema#double">11.505726890655758</opla-sd:entityPositionX>
                <opla-sd:entityPositionY rdf:datatype="http://www.w3.org/2001/XMLSchema#double">298.46981551503904</opla-sd:entityPositionY>
                <rdfs:comment xml:lang="en">This is an entity positioning annotation generated by CoModIDE (https://comodide.com/). Removing this annotation will break rendering the CoModIDE schema diagram view.</rdfs:comment>
            </rdf:Description>
        </opla-sd:entityPosition>
        <rdfs:comment xml:lang="en">A company which in a process of the cross-border division in case of a full division transfers all its assets and liabilities to two or more companies, or in case of a partial division or division by separation transfers part of its assets and liabilities to one or more companies. The companies involved in the process are located in multiple (two or more) distinct countries.</rdfs:comment>
        <rdfs:label xml:lang="en">Cross-border company division</rdfs:label>
    </owl:Class>
    


    <!-- http://w3id.org/um/cbcm/eu-cm-ontology#CrossBorderMerger -->

    <owl:Class rdf:about="http://w3id.org/um/cbcm/eu-cm-ontology#CrossBorderMerger">
        <owl:equivalentClass>
            <owl:Class>
                <owl:intersectionOf rdf:parseType="Collection">
                    <rdf:Description rdf:about="http://w3id.org/um/cbcm/eu-cm-ontology#CompanyMerger"/>
                    <owl:Restriction>
                        <owl:onProperty rdf:resource="http://w3id.org/um/cbcm/eu-cm-ontology#sourceCountry"/>
                        <owl:someValuesFrom rdf:resource="http://w3id.org/um/cbcm/eu-cm-ontology#Country"/>
                    </owl:Restriction>
                    <owl:Restriction>
                        <owl:onProperty rdf:resource="http://w3id.org/um/cbcm/eu-cm-ontology#involvesCountry"/>
                        <owl:minQualifiedCardinality rdf:datatype="http://www.w3.org/2001/XMLSchema#nonNegativeInteger">2</owl:minQualifiedCardinality>
                        <owl:onClass rdf:resource="http://w3id.org/um/cbcm/eu-cm-ontology#Country"/>
                    </owl:Restriction>
                    <owl:Restriction>
                        <owl:onProperty rdf:resource="http://w3id.org/um/cbcm/eu-cm-ontology#targetCountry"/>
                        <owl:qualifiedCardinality rdf:datatype="http://www.w3.org/2001/XMLSchema#nonNegativeInteger">1</owl:qualifiedCardinality>
                        <owl:onClass rdf:resource="http://w3id.org/um/cbcm/eu-cm-ontology#Country"/>
                    </owl:Restriction>
                </owl:intersectionOf>
            </owl:Class>
        </owl:equivalentClass>
        <rdfs:subClassOf rdf:resource="http://w3id.org/um/cbcm/eu-cm-ontology#CompanyMerger"/>
        <rdfs:subClassOf>
            <owl:Restriction>
                <owl:onProperty rdf:resource="http://w3id.org/um/cbcm/eu-cm-ontology#hasTransactionInput"/>
                <owl:someValuesFrom rdf:resource="http://w3id.org/um/cbcm/eu-cm-ontology#AcquiringCompany"/>
            </owl:Restriction>
        </rdfs:subClassOf>
        <rdfs:subClassOf>
            <owl:Restriction>
                <owl:onProperty rdf:resource="http://w3id.org/um/cbcm/eu-cm-ontology#hasTransactionInput"/>
                <owl:someValuesFrom rdf:resource="http://w3id.org/um/cbcm/eu-cm-ontology#MergingCompany"/>
            </owl:Restriction>
        </rdfs:subClassOf>
        <rdfs:subClassOf>
            <owl:Restriction>
                <owl:onProperty rdf:resource="http://w3id.org/um/cbcm/eu-cm-ontology#sourceCountry"/>
                <owl:someValuesFrom rdf:resource="http://w3id.org/um/cbcm/eu-cm-ontology#Country"/>
            </owl:Restriction>
        </rdfs:subClassOf>
        <rdfs:subClassOf>
            <owl:Restriction>
                <owl:onProperty rdf:resource="http://w3id.org/um/cbcm/eu-cm-ontology#targetCountry"/>
                <owl:qualifiedCardinality rdf:datatype="http://www.w3.org/2001/XMLSchema#nonNegativeInteger">1</owl:qualifiedCardinality>
                <owl:onClass rdf:resource="http://w3id.org/um/cbcm/eu-cm-ontology#Country"/>
            </owl:Restriction>
        </rdfs:subClassOf>
        <opla-sd:entityPosition>
            <rdf:Description>
                <opla-sd:entityPositionX rdf:datatype="http://www.w3.org/2001/XMLSchema#double">143.6432675101612</opla-sd:entityPositionX>
                <opla-sd:entityPositionY rdf:datatype="http://www.w3.org/2001/XMLSchema#double">123.39626348456598</opla-sd:entityPositionY>
                <rdfs:comment xml:lang="en">This is an entity positioning annotation generated by CoModIDE (https://comodide.com/). Removing this annotation will break rendering the CoModIDE schema diagram view.</rdfs:comment>
            </rdf:Description>
        </opla-sd:entityPosition>
        <rdfs:comment xml:lang="en">A cross border merger involves at least one company based in an EU Member State and one company that is registered elsewhere within the European Union and is leading to a universal transfer of assets and liabilities from the merging company to the acquiring company.</rdfs:comment>
        <rdfs:label xml:lang="en">Cross-border merger</rdfs:label>
        <rdfs:seeAlso rdf:resource="http://data.europa.eu/eli/dir/2017/1132/oj"/>
    </owl:Class>
    


    <!-- http://w3id.org/um/cbcm/eu-cm-ontology#CrossBorderMergerByAcquisition -->

    <owl:Class rdf:about="http://w3id.org/um/cbcm/eu-cm-ontology#CrossBorderMergerByAcquisition">
        <owl:equivalentClass>
            <owl:Class>
                <owl:intersectionOf rdf:parseType="Collection">
                    <rdf:Description rdf:about="http://w3id.org/um/cbcm/eu-cm-ontology#CrossBorderMerger"/>
                    <owl:Restriction>
                        <owl:onProperty rdf:resource="http://w3id.org/um/cbcm/eu-cm-ontology#hasMergingCompany"/>
                        <owl:someValuesFrom rdf:resource="http://w3id.org/um/cbcm/eu-cm-ontology#Company"/>
                    </owl:Restriction>
                    <owl:Restriction>
                        <owl:onProperty rdf:resource="http://w3id.org/um/cbcm/eu-cm-ontology#hasAcquiringCompany"/>
                        <owl:qualifiedCardinality rdf:datatype="http://www.w3.org/2001/XMLSchema#nonNegativeInteger">1</owl:qualifiedCardinality>
                        <owl:onClass rdf:resource="http://w3id.org/um/cbcm/eu-cm-ontology#Company"/>
                    </owl:Restriction>
                </owl:intersectionOf>
            </owl:Class>
        </owl:equivalentClass>
        <rdfs:subClassOf rdf:resource="http://w3id.org/um/cbcm/eu-cm-ontology#CrossBorderMerger"/>
        <opla-sd:entityPosition>
            <rdf:Description>
                <opla-sd:entityPositionX rdf:datatype="http://www.w3.org/2001/XMLSchema#double">107.43623102247348</opla-sd:entityPositionX>
                <opla-sd:entityPositionY rdf:datatype="http://www.w3.org/2001/XMLSchema#double">129.88046751595175</opla-sd:entityPositionY>
                <rdfs:comment xml:lang="en">This is an entity positioning annotation generated by CoModIDE (https://comodide.com/). Removing this annotation will break rendering the CoModIDE schema diagram view.</rdfs:comment>
            </rdf:Description>
        </opla-sd:entityPosition>
        <rdfs:comment xml:lang="en">Article 89: The operation whereby one or more companies are wound up without going into liquidation and transfer to another all their assets and liabilities in exchange for the issue to the shareholders of the company or companies being acquired of shares in the acquiring company and a cash payment, if any, not exceeding 10 % of the nominal value of the shares so issued or, where they have no nominal value, of their accounting par value. Companies involved come from two or more distinct countries.</rdfs:comment>
        <rdfs:label xml:lang="en">Cross-border company merger by acquisition</rdfs:label>
    </owl:Class>
    


    <!-- http://w3id.org/um/cbcm/eu-cm-ontology#CrossBorderMergerIntoNewCompany -->

    <owl:Class rdf:about="http://w3id.org/um/cbcm/eu-cm-ontology#CrossBorderMergerIntoNewCompany">
        <rdfs:subClassOf rdf:resource="http://w3id.org/um/cbcm/eu-cm-ontology#CrossBorderMerger"/>
        <opla-sd:entityPosition>
            <rdf:Description>
                <opla-sd:entityPositionX rdf:datatype="http://www.w3.org/2001/XMLSchema#double">269.5633829773079</opla-sd:entityPositionX>
                <opla-sd:entityPositionY rdf:datatype="http://www.w3.org/2001/XMLSchema#double">122.87965078063148</opla-sd:entityPositionY>
                <rdfs:comment xml:lang="en">This is an entity positioning annotation generated by CoModIDE (https://comodide.com/). Removing this annotation will break rendering the CoModIDE schema diagram view.</rdfs:comment>
            </rdf:Description>
        </opla-sd:entityPosition>
        <rdfs:comment xml:lang="en">Article 90: the operation whereby several companies are wound up without going into liquidation and transfer to a company that they set up all their assets and liabilities in exchange for the issue to their shareholders of shares in the new company and a cash payment, if any, not exceeding 10 % of the nominal value of the shares so issued or, where they have no nominal value, of their accounting par value. Companies involved come from two or more distinct countries.</rdfs:comment>
        <rdfs:label xml:lang="en">Cross-border merger into a new company</rdfs:label>
    </owl:Class>
    


    <!-- http://w3id.org/um/cbcm/eu-cm-ontology#CrossBorderSeatTransfer -->

    <owl:Class rdf:about="http://w3id.org/um/cbcm/eu-cm-ontology#CrossBorderSeatTransfer">
        <owl:equivalentClass>
            <owl:Class>
                <owl:intersectionOf rdf:parseType="Collection">
                    <rdf:Description rdf:about="http://w3id.org/um/cbcm/eu-cm-ontology#CompanySeatTransfer"/>
                    <owl:Restriction>
                        <owl:onProperty rdf:resource="http://w3id.org/um/cbcm/eu-cm-ontology#involvesCountry"/>
                        <owl:qualifiedCardinality rdf:datatype="http://www.w3.org/2001/XMLSchema#nonNegativeInteger">2</owl:qualifiedCardinality>
                        <owl:onClass rdf:resource="http://w3id.org/um/cbcm/eu-cm-ontology#Country"/>
                    </owl:Restriction>
                    <owl:Restriction>
                        <owl:onProperty rdf:resource="http://w3id.org/um/cbcm/eu-cm-ontology#sourceCountry"/>
                        <owl:qualifiedCardinality rdf:datatype="http://www.w3.org/2001/XMLSchema#nonNegativeInteger">1</owl:qualifiedCardinality>
                        <owl:onClass rdf:resource="http://w3id.org/um/cbcm/eu-cm-ontology#Country"/>
                    </owl:Restriction>
                    <owl:Restriction>
                        <owl:onProperty rdf:resource="http://w3id.org/um/cbcm/eu-cm-ontology#targetCountry"/>
                        <owl:qualifiedCardinality rdf:datatype="http://www.w3.org/2001/XMLSchema#nonNegativeInteger">1</owl:qualifiedCardinality>
                        <owl:onClass rdf:resource="http://w3id.org/um/cbcm/eu-cm-ontology#Country"/>
                    </owl:Restriction>
                </owl:intersectionOf>
            </owl:Class>
        </owl:equivalentClass>
        <rdfs:subClassOf rdf:resource="http://w3id.org/um/cbcm/eu-cm-ontology#CompanySeatTransfer"/>
        <rdfs:subClassOf>
            <owl:Restriction>
                <owl:onProperty rdf:resource="http://w3id.org/um/cbcm/eu-cm-ontology#hasTransactionInput"/>
                <owl:qualifiedCardinality rdf:datatype="http://www.w3.org/2001/XMLSchema#nonNegativeInteger">1</owl:qualifiedCardinality>
                <owl:onClass rdf:resource="http://w3id.org/um/cbcm/eu-cm-ontology#Company"/>
            </owl:Restriction>
        </rdfs:subClassOf>
        <rdfs:subClassOf>
            <owl:Restriction>
                <owl:onProperty rdf:resource="http://w3id.org/um/cbcm/eu-cm-ontology#sourceCountry"/>
                <owl:qualifiedCardinality rdf:datatype="http://www.w3.org/2001/XMLSchema#nonNegativeInteger">1</owl:qualifiedCardinality>
                <owl:onClass rdf:resource="http://w3id.org/um/cbcm/eu-cm-ontology#Country"/>
            </owl:Restriction>
        </rdfs:subClassOf>
        <rdfs:subClassOf>
            <owl:Restriction>
                <owl:onProperty rdf:resource="http://w3id.org/um/cbcm/eu-cm-ontology#targetCountry"/>
                <owl:qualifiedCardinality rdf:datatype="http://www.w3.org/2001/XMLSchema#nonNegativeInteger">1</owl:qualifiedCardinality>
                <owl:onClass rdf:resource="http://w3id.org/um/cbcm/eu-cm-ontology#Country"/>
            </owl:Restriction>
        </rdfs:subClassOf>
        <opla-sd:entityPosition>
            <rdf:Description>
                <opla-sd:entityPositionX rdf:datatype="http://www.w3.org/2001/XMLSchema#double">233.50701415067806</opla-sd:entityPositionX>
                <opla-sd:entityPositionY rdf:datatype="http://www.w3.org/2001/XMLSchema#double">84.30831286232869</opla-sd:entityPositionY>
                <rdfs:comment xml:lang="en">This is an entity positioning annotation generated by CoModIDE (https://comodide.com/). Removing this annotation will break rendering the CoModIDE schema diagram view.</rdfs:comment>
            </rdf:Description>
        </opla-sd:entityPosition>
        <rdfs:comment xml:lang="en">The act of changing the location where the company’s business was managed (registered office or headquarters) or the place where that company’s primary business was actually conducted (central administration), across national boundaries.</rdfs:comment>
        <rdfs:label xml:lang="en">Cross-border company seat transfer</rdfs:label>
    </owl:Class>
    


    <!-- http://w3id.org/um/cbcm/eu-cm-ontology#DataCurationActivity -->

    <owl:Class rdf:about="http://w3id.org/um/cbcm/eu-cm-ontology#DataCurationActivity">
        <rdfs:subClassOf rdf:resource="http://w3id.org/um/cbcm/eu-cm-ontology#Process"/>
        <rdfs:subClassOf>
            <owl:Restriction>
                <owl:onProperty rdf:resource="http://w3id.org/um/cbcm/eu-cm-ontology#associatedWith"/>
                <owl:qualifiedCardinality rdf:datatype="http://www.w3.org/2001/XMLSchema#nonNegativeInteger">1</owl:qualifiedCardinality>
                <owl:onClass rdf:resource="http://w3id.org/um/cbcm/eu-cm-ontology#Agent"/>
            </owl:Restriction>
        </rdfs:subClassOf>
        <rdfs:comment xml:lang="en">A data curation activity represents a researcher&apos;s involvement in annotating cross border transactions</rdfs:comment>
        <rdfs:label xml:lang="en">Data curation activity</rdfs:label>
    </owl:Class>
    


    <!-- http://w3id.org/um/cbcm/eu-cm-ontology#DecisionRight -->

    <owl:Class rdf:about="http://w3id.org/um/cbcm/eu-cm-ontology#DecisionRight">
        <rdfs:subClassOf rdf:resource="http://w3id.org/um/cbcm/eu-cm-ontology#ShareholderRight"/>
        <opla-sd:entityPosition>
            <rdf:Description>
                <opla-sd:entityPositionX rdf:datatype="http://www.w3.org/2001/XMLSchema#double">50.302555531775546</opla-sd:entityPositionX>
                <opla-sd:entityPositionY rdf:datatype="http://www.w3.org/2001/XMLSchema#double">246.93820263180197</opla-sd:entityPositionY>
                <rdfs:comment xml:lang="en">This is an entity positioning annotation generated by CoModIDE (https://comodide.com/). Removing this annotation will break rendering the CoModIDE schema diagram view.</rdfs:comment>
            </rdf:Description>
        </opla-sd:entityPosition>
        <rdfs:comment xml:lang="en">The shareholders can take a number of decisions affecting the company, such as amending the company&apos;s articles of association, appointing or dismissing board members and to approve important transactions (e.g. mergers, divisions and conversions/seat transfers). These are taken through a shareholder resolution.</rdfs:comment>
        <rdfs:label xml:lang="en">Shareholder decision right</rdfs:label>
        <rdfs:seeAlso rdf:resource="http://data.europa.eu/eli/dir/2017/1132/oj"/>
    </owl:Class>
    


    <!-- http://w3id.org/um/cbcm/eu-cm-ontology#DivisionCertificate -->

    <owl:Class rdf:about="http://w3id.org/um/cbcm/eu-cm-ontology#DivisionCertificate">
        <rdfs:subClassOf rdf:resource="http://w3id.org/um/cbcm/eu-cm-ontology#TransactionCertificate"/>
        <opla-sd:entityPosition>
            <rdf:Description>
                <opla-sd:entityPositionX rdf:datatype="http://www.w3.org/2001/XMLSchema#double">255.74268679131885</opla-sd:entityPositionX>
                <opla-sd:entityPositionY rdf:datatype="http://www.w3.org/2001/XMLSchema#double">42.2059024226523</opla-sd:entityPositionY>
                <rdfs:comment xml:lang="en">This is an entity positioning annotation generated by CoModIDE (https://comodide.com/). Removing this annotation will break rendering the CoModIDE schema diagram view.</rdfs:comment>
            </rdf:Description>
        </opla-sd:entityPosition>
        <rdfs:comment xml:lang="en">A document issued by a Competent Authority declaring that the legally required steps of a division are completed. The certificate needs to be presented by a company to either be registered (or register a newly established emerging/recipient company) in another company registry or to be removed from a company register.</rdfs:comment>
        <rdfs:label xml:lang="en">Company division certificate</rdfs:label>
    </owl:Class>
    


    <!-- http://w3id.org/um/cbcm/eu-cm-ontology#DivisionPlan -->

    <owl:Class rdf:about="http://w3id.org/um/cbcm/eu-cm-ontology#DivisionPlan">
        <rdfs:subClassOf rdf:resource="http://w3id.org/um/cbcm/eu-cm-ontology#TransactionDocument"/>
        <opla-sd:entityPosition>
            <rdf:Description>
                <opla-sd:entityPositionX rdf:datatype="http://www.w3.org/2001/XMLSchema#double">271.4060191302092</opla-sd:entityPositionX>
                <opla-sd:entityPositionY rdf:datatype="http://www.w3.org/2001/XMLSchema#double">136.12357204672944</opla-sd:entityPositionY>
                <rdfs:comment xml:lang="en">This is an entity positioning annotation generated by CoModIDE (https://comodide.com/). Removing this annotation will break rendering the CoModIDE schema diagram view.</rdfs:comment>
            </rdf:Description>
        </opla-sd:entityPosition>
        <rdfs:comment xml:lang="en">The management or administrative organ of the company shall draw up the draft terms of a division. The draft terms of a division shall include at least the particulars listed in article 160d.</rdfs:comment>
        <rdfs:label xml:lang="en">Company division plan</rdfs:label>
        <rdfs:seeAlso rdf:resource="https://www.europarl.europa.eu/doceo/document/TA-8-2019-0429_EN.html"/>
    </owl:Class>
    


    <!-- http://w3id.org/um/cbcm/eu-cm-ontology#DocumentRepository -->

    <owl:Class rdf:about="http://w3id.org/um/cbcm/eu-cm-ontology#DocumentRepository">
        <rdfs:subClassOf rdf:resource="http://w3id.org/um/cbcm/eu-cm-ontology#Object"/>
        <opla-sd:entityPosition>
            <rdf:Description>
                <opla-sd:entityPositionX rdf:datatype="http://www.w3.org/2001/XMLSchema#double">102.97791164894174</opla-sd:entityPositionX>
                <opla-sd:entityPositionY rdf:datatype="http://www.w3.org/2001/XMLSchema#double">220.50340919371476</opla-sd:entityPositionY>
                <rdfs:comment xml:lang="en">This is an entity positioning annotation generated by CoModIDE (https://comodide.com/). Removing this annotation will break rendering the CoModIDE schema diagram view.</rdfs:comment>
            </rdf:Description>
        </opla-sd:entityPosition>
        <rdfs:comment xml:lang="en">A digital document repository containing documents related to company mobility.</rdfs:comment>
        <rdfs:label xml:lang="en">Company mobility document repository</rdfs:label>
    </owl:Class>
    


    <!-- http://w3id.org/um/cbcm/eu-cm-ontology#DomesticConversion -->

    <owl:Class rdf:about="http://w3id.org/um/cbcm/eu-cm-ontology#DomesticConversion">
        <rdfs:subClassOf rdf:resource="http://w3id.org/um/cbcm/eu-cm-ontology#CompanyConversion"/>
        <rdfs:subClassOf>
            <owl:Restriction>
                <owl:onProperty rdf:resource="http://w3id.org/um/cbcm/eu-cm-ontology#involvesCountry"/>
                <owl:qualifiedCardinality rdf:datatype="http://www.w3.org/2001/XMLSchema#nonNegativeInteger">1</owl:qualifiedCardinality>
                <owl:onClass rdf:resource="http://w3id.org/um/cbcm/eu-cm-ontology#Country"/>
            </owl:Restriction>
        </rdfs:subClassOf>
        <opla-sd:entityPosition>
            <rdf:Description>
                <opla-sd:entityPositionX rdf:datatype="http://www.w3.org/2001/XMLSchema#double">209.7252878494862</opla-sd:entityPositionX>
                <opla-sd:entityPositionY rdf:datatype="http://www.w3.org/2001/XMLSchema#double">288.0907141087795</opla-sd:entityPositionY>
                <rdfs:comment xml:lang="en">This is an entity positioning annotation generated by CoModIDE (https://comodide.com/). Removing this annotation will break rendering the CoModIDE schema diagram view.</rdfs:comment>
            </rdf:Description>
        </opla-sd:entityPosition>
        <rdfs:comment xml:lang="en">A domestic conversion is an operation through which a company&apos;s form is converted into a another while still remaining governed by the same law as the original company. For instance, the modification of a company&apos;s form from a public to a private limited company.</rdfs:comment>
        <rdfs:label xml:lang="en">Domestic company conversion</rdfs:label>
    </owl:Class>
    


    <!-- http://w3id.org/um/cbcm/eu-cm-ontology#DomesticDivision -->

    <owl:Class rdf:about="http://w3id.org/um/cbcm/eu-cm-ontology#DomesticDivision">
        <rdfs:subClassOf rdf:resource="http://w3id.org/um/cbcm/eu-cm-ontology#CompanyDivision"/>
        <rdfs:subClassOf>
            <owl:Restriction>
                <owl:onProperty rdf:resource="http://w3id.org/um/cbcm/eu-cm-ontology#involvesCountry"/>
                <owl:qualifiedCardinality rdf:datatype="http://www.w3.org/2001/XMLSchema#nonNegativeInteger">1</owl:qualifiedCardinality>
                <owl:onClass rdf:resource="http://w3id.org/um/cbcm/eu-cm-ontology#Country"/>
            </owl:Restriction>
        </rdfs:subClassOf>
        <opla-sd:entityPosition>
            <rdf:Description>
                <opla-sd:entityPositionX rdf:datatype="http://www.w3.org/2001/XMLSchema#double">115.5742918611993</opla-sd:entityPositionX>
                <opla-sd:entityPositionY rdf:datatype="http://www.w3.org/2001/XMLSchema#double">78.99288710365471</opla-sd:entityPositionY>
                <rdfs:comment xml:lang="en">This is an entity positioning annotation generated by CoModIDE (https://comodide.com/). Removing this annotation will break rendering the CoModIDE schema diagram view.</rdfs:comment>
            </rdf:Description>
        </opla-sd:entityPosition>
        <rdfs:comment xml:lang="en">A company which in a process of the domestic division - in case of a full division - transfers all its assets and liabilities to two or more companies, or - in case of a partial division or division by separation - transfers part of its assets and liabilities to one or more companies. All companies involved in the process are located in a single country.</rdfs:comment>
        <rdfs:label xml:lang="en">Company domestic division</rdfs:label>
    </owl:Class>
    


    <!-- http://w3id.org/um/cbcm/eu-cm-ontology#DomesticMerger -->

    <owl:Class rdf:about="http://w3id.org/um/cbcm/eu-cm-ontology#DomesticMerger">
        <rdfs:subClassOf rdf:resource="http://w3id.org/um/cbcm/eu-cm-ontology#CompanyMerger"/>
        <rdfs:subClassOf>
            <owl:Restriction>
                <owl:onProperty rdf:resource="http://w3id.org/um/cbcm/eu-cm-ontology#hasTransactionInput"/>
                <owl:someValuesFrom rdf:resource="http://w3id.org/um/cbcm/eu-cm-ontology#AcquiringCompany"/>
            </owl:Restriction>
        </rdfs:subClassOf>
        <rdfs:subClassOf>
            <owl:Restriction>
                <owl:onProperty rdf:resource="http://w3id.org/um/cbcm/eu-cm-ontology#hasTransactionInput"/>
                <owl:someValuesFrom rdf:resource="http://w3id.org/um/cbcm/eu-cm-ontology#MergingCompany"/>
            </owl:Restriction>
        </rdfs:subClassOf>
        <rdfs:subClassOf>
            <owl:Restriction>
                <owl:onProperty rdf:resource="http://w3id.org/um/cbcm/eu-cm-ontology#involvesCountry"/>
                <owl:qualifiedCardinality rdf:datatype="http://www.w3.org/2001/XMLSchema#nonNegativeInteger">1</owl:qualifiedCardinality>
                <owl:onClass rdf:resource="http://w3id.org/um/cbcm/eu-cm-ontology#Country"/>
            </owl:Restriction>
        </rdfs:subClassOf>
        <opla-sd:entityPosition>
            <rdf:Description>
                <opla-sd:entityPositionX rdf:datatype="http://www.w3.org/2001/XMLSchema#double">11.806501569175973</opla-sd:entityPositionX>
                <opla-sd:entityPositionY rdf:datatype="http://www.w3.org/2001/XMLSchema#double">266.3880979890687</opla-sd:entityPositionY>
                <rdfs:comment xml:lang="en">This is an entity positioning annotation generated by CoModIDE (https://comodide.com/). Removing this annotation will break rendering the CoModIDE schema diagram view.</rdfs:comment>
            </rdf:Description>
        </opla-sd:entityPosition>
        <rdfs:comment xml:lang="en">A domestic merger involves at least two companies based in the same EU Member State and is leading to a universal transfer of assets and liabilities from the merging company to the acquiring company.</rdfs:comment>
        <rdfs:label xml:lang="en">Company domestic merger</rdfs:label>
    </owl:Class>
    


    <!-- http://w3id.org/um/cbcm/eu-cm-ontology#DomesticMergerByAcquisition -->

    <owl:Class rdf:about="http://w3id.org/um/cbcm/eu-cm-ontology#DomesticMergerByAcquisition">
        <rdfs:subClassOf rdf:resource="http://w3id.org/um/cbcm/eu-cm-ontology#DomesticMerger"/>
        <rdfs:subClassOf>
            <owl:Restriction>
                <owl:onProperty rdf:resource="http://w3id.org/um/cbcm/eu-cm-ontology#hasTransactionResult"/>
                <owl:someValuesFrom rdf:resource="http://w3id.org/um/cbcm/eu-cm-ontology#MergingCompany"/>
            </owl:Restriction>
        </rdfs:subClassOf>
        <rdfs:subClassOf>
            <owl:Restriction>
                <owl:onProperty rdf:resource="http://w3id.org/um/cbcm/eu-cm-ontology#hasTransactionInput"/>
                <owl:qualifiedCardinality rdf:datatype="http://www.w3.org/2001/XMLSchema#nonNegativeInteger">1</owl:qualifiedCardinality>
                <owl:onClass rdf:resource="http://w3id.org/um/cbcm/eu-cm-ontology#AcquiringCompany"/>
            </owl:Restriction>
        </rdfs:subClassOf>
        <owl:disjointWith rdf:resource="http://w3id.org/um/cbcm/eu-cm-ontology#DomesticMergerIntoNewCompany"/>
        <opla-sd:entityPosition>
            <rdf:Description>
                <opla-sd:entityPositionX rdf:datatype="http://www.w3.org/2001/XMLSchema#double">256.9075679272785</opla-sd:entityPositionX>
                <opla-sd:entityPositionY rdf:datatype="http://www.w3.org/2001/XMLSchema#double">53.80105649965677</opla-sd:entityPositionY>
                <rdfs:comment xml:lang="en">This is an entity positioning annotation generated by CoModIDE (https://comodide.com/). Removing this annotation will break rendering the CoModIDE schema diagram view.</rdfs:comment>
            </rdf:Description>
        </opla-sd:entityPosition>
        <rdfs:comment xml:lang="en">Article 89: The operation whereby one or more companies are wound up without going into liquidation and transfer to another all their assets and liabilities in exchange for the issue to the shareholders of the company or companies being acquired of shares in the acquiring company and a cash payment, if any, not exceeding 10 % of the nominal value of the shares so issued or, where they have no nominal value, of their accounting par value. All companies involved are from a single country.</rdfs:comment>
        <rdfs:label xml:lang="en">Domestic company merger by acquisition</rdfs:label>
        <rdfs:seeAlso rdf:resource="http://data.europa.eu/eli/dir/2017/1132/oj"/>
    </owl:Class>
    


    <!-- http://w3id.org/um/cbcm/eu-cm-ontology#DomesticMergerIntoNewCompany -->

    <owl:Class rdf:about="http://w3id.org/um/cbcm/eu-cm-ontology#DomesticMergerIntoNewCompany">
        <rdfs:subClassOf rdf:resource="http://w3id.org/um/cbcm/eu-cm-ontology#DomesticMerger"/>
        <rdfs:subClassOf>
            <owl:Restriction>
                <owl:onProperty rdf:resource="http://w3id.org/um/cbcm/eu-cm-ontology#hasTransactionInput"/>
                <owl:someValuesFrom rdf:resource="http://w3id.org/um/cbcm/eu-cm-ontology#MergingCompany"/>
            </owl:Restriction>
        </rdfs:subClassOf>
        <rdfs:subClassOf>
            <owl:Restriction>
                <owl:onProperty rdf:resource="http://w3id.org/um/cbcm/eu-cm-ontology#hasTransactionResult"/>
                <owl:someValuesFrom rdf:resource="http://w3id.org/um/cbcm/eu-cm-ontology#EmergingCompany"/>
            </owl:Restriction>
        </rdfs:subClassOf>
        <opla-sd:entityPosition>
            <rdf:Description>
                <opla-sd:entityPositionX rdf:datatype="http://www.w3.org/2001/XMLSchema#double">200.92840759111368</opla-sd:entityPositionX>
                <opla-sd:entityPositionY rdf:datatype="http://www.w3.org/2001/XMLSchema#double">14.241868874997104</opla-sd:entityPositionY>
                <rdfs:comment xml:lang="en">This is an entity positioning annotation generated by CoModIDE (https://comodide.com/). Removing this annotation will break rendering the CoModIDE schema diagram view.</rdfs:comment>
            </rdf:Description>
        </opla-sd:entityPosition>
        <rdfs:comment xml:lang="en">Article 90: the operation whereby several companies are wound up without going into liquidation and transfer to a company that they set up all their assets and liabilities in exchange for the issue to their shareholders of shares in the new company and a cash payment, if any, not exceeding 10 % of the nominal value of the shares so issued or, where they have no nominal value, of their accounting par value. All companies involved are from a single country.</rdfs:comment>
        <rdfs:label xml:lang="en">Domestic merger into a new company</rdfs:label>
        <rdfs:seeAlso rdf:resource="http://data.europa.eu/eli/dir/2017/1132/oj"/>
    </owl:Class>
    


    <!-- http://w3id.org/um/cbcm/eu-cm-ontology#DomesticSeatTransfer -->

    <owl:Class rdf:about="http://w3id.org/um/cbcm/eu-cm-ontology#DomesticSeatTransfer">
        <owl:equivalentClass>
            <owl:Class>
                <owl:intersectionOf rdf:parseType="Collection">
                    <rdf:Description rdf:about="http://w3id.org/um/cbcm/eu-cm-ontology#CompanySeatTransfer"/>
                    <owl:Restriction>
                        <owl:onProperty rdf:resource="http://w3id.org/um/cbcm/eu-cm-ontology#involvesCountry"/>
                        <owl:qualifiedCardinality rdf:datatype="http://www.w3.org/2001/XMLSchema#nonNegativeInteger">1</owl:qualifiedCardinality>
                        <owl:onClass rdf:resource="http://w3id.org/um/cbcm/eu-cm-ontology#Country"/>
                    </owl:Restriction>
                    <owl:Restriction>
                        <owl:onProperty rdf:resource="http://w3id.org/um/cbcm/eu-cm-ontology#sourceCountry"/>
                        <owl:qualifiedCardinality rdf:datatype="http://www.w3.org/2001/XMLSchema#nonNegativeInteger">1</owl:qualifiedCardinality>
                        <owl:onClass rdf:resource="http://w3id.org/um/cbcm/eu-cm-ontology#Country"/>
                    </owl:Restriction>
                    <owl:Restriction>
                        <owl:onProperty rdf:resource="http://w3id.org/um/cbcm/eu-cm-ontology#targetCountry"/>
                        <owl:qualifiedCardinality rdf:datatype="http://www.w3.org/2001/XMLSchema#nonNegativeInteger">1</owl:qualifiedCardinality>
                        <owl:onClass rdf:resource="http://w3id.org/um/cbcm/eu-cm-ontology#Country"/>
                    </owl:Restriction>
                </owl:intersectionOf>
            </owl:Class>
        </owl:equivalentClass>
        <rdfs:subClassOf rdf:resource="http://w3id.org/um/cbcm/eu-cm-ontology#CompanySeatTransfer"/>
        <rdfs:subClassOf>
            <owl:Restriction>
                <owl:onProperty rdf:resource="http://w3id.org/um/cbcm/eu-cm-ontology#involvesCountry"/>
                <owl:qualifiedCardinality rdf:datatype="http://www.w3.org/2001/XMLSchema#nonNegativeInteger">1</owl:qualifiedCardinality>
                <owl:onClass rdf:resource="http://w3id.org/um/cbcm/eu-cm-ontology#Country"/>
            </owl:Restriction>
        </rdfs:subClassOf>
        <rdfs:comment xml:lang="en">The act of changing the location where the company’s business was managed (registered office or headquarters) or the place where that company’s primary business was actually conducted (central administration), within a specific country.</rdfs:comment>
        <rdfs:label xml:lang="en">Domestic company seat transfer</rdfs:label>
    </owl:Class>
    


    <!-- http://w3id.org/um/cbcm/eu-cm-ontology#EEACountry -->

    <owl:Class rdf:about="http://w3id.org/um/cbcm/eu-cm-ontology#EEACountry">
        <rdfs:subClassOf rdf:resource="http://w3id.org/um/cbcm/eu-cm-ontology#Country"/>
        <owl:disjointWith rdf:resource="http://w3id.org/um/cbcm/eu-cm-ontology#NonEEACountry"/>
        <opla-sd:entityPosition>
            <rdf:Description>
                <opla-sd:entityPositionX rdf:datatype="http://www.w3.org/2001/XMLSchema#double">151.79064556421153</opla-sd:entityPositionX>
                <opla-sd:entityPositionY rdf:datatype="http://www.w3.org/2001/XMLSchema#double">223.262266343131</opla-sd:entityPositionY>
                <rdfs:comment xml:lang="en">This is an entity positioning annotation generated by CoModIDE (https://comodide.com/). Removing this annotation will break rendering the CoModIDE schema diagram view.</rdfs:comment>
            </rdf:Description>
        </opla-sd:entityPosition>
        <rdfs:comment xml:lang="en">Created in 1994, the European Economic Area (EEA) combines the countries of the European Union (EU) and member countries of the European Free Trade Association (EFTA) to facilitate participation in the European Market trade and movement without having to apply to be one of the EU member countries</rdfs:comment>
        <rdfs:label xml:lang="en">European Economic Area country</rdfs:label>
    </owl:Class>
    


    <!-- http://w3id.org/um/cbcm/eu-cm-ontology#EUCountry -->

    <owl:Class rdf:about="http://w3id.org/um/cbcm/eu-cm-ontology#EUCountry">
        <rdfs:subClassOf rdf:resource="http://w3id.org/um/cbcm/eu-cm-ontology#EEACountry"/>
        <owl:disjointWith rdf:resource="http://w3id.org/um/cbcm/eu-cm-ontology#NonEUCountry"/>
        <opla-sd:entityPosition>
            <rdf:Description>
                <opla-sd:entityPositionX rdf:datatype="http://www.w3.org/2001/XMLSchema#double">35.78319291697038</opla-sd:entityPositionX>
                <opla-sd:entityPositionY rdf:datatype="http://www.w3.org/2001/XMLSchema#double">101.48120003940404</opla-sd:entityPositionY>
                <rdfs:comment xml:lang="en">This is an entity positioning annotation generated by CoModIDE (https://comodide.com/). Removing this annotation will break rendering the CoModIDE schema diagram view.</rdfs:comment>
            </rdf:Description>
        </opla-sd:entityPosition>
        <terms:description xml:lang="en">A country which forms part of the European Union. The European Union is a conglomeration of European countries whose governance structures agree to abide with common political and economic criteria to improve efficiency of goods and services trading as well as movement and migration of inhabitants between these countries</terms:description>
        <rdfs:label>EU country</rdfs:label>
    </owl:Class>
    


    <!-- http://w3id.org/um/cbcm/eu-cm-ontology#EmergingCompany -->

    <owl:Class rdf:about="http://w3id.org/um/cbcm/eu-cm-ontology#EmergingCompany">
        <rdfs:subClassOf rdf:resource="http://w3id.org/um/cbcm/eu-cm-ontology#Company"/>
        <opla-sd:entityPosition>
            <rdf:Description>
                <opla-sd:entityPositionX rdf:datatype="http://www.w3.org/2001/XMLSchema#double">143.0760569786945</opla-sd:entityPositionX>
                <opla-sd:entityPositionY rdf:datatype="http://www.w3.org/2001/XMLSchema#double">205.74953025622148</opla-sd:entityPositionY>
                <rdfs:comment xml:lang="en">This is an entity positioning annotation generated by CoModIDE (https://comodide.com/). Removing this annotation will break rendering the CoModIDE schema diagram view.</rdfs:comment>
            </rdf:Description>
        </opla-sd:entityPosition>
        <rdfs:comment xml:lang="en">A company being divided transfers part of its assets and liabilities to one or more newly formed companies, which are the recipient companies in a (cross-border) division.</rdfs:comment>
        <rdfs:label xml:lang="en">Emerging company</rdfs:label>
    </owl:Class>
    


    <!-- http://w3id.org/um/cbcm/eu-cm-ontology#Employee -->

    <owl:Class rdf:about="http://w3id.org/um/cbcm/eu-cm-ontology#Employee">
        <owl:equivalentClass>
            <owl:Class>
                <owl:intersectionOf rdf:parseType="Collection">
                    <rdf:Description rdf:about="http://w3id.org/um/cbcm/eu-cm-ontology#Person"/>
                    <owl:Restriction>
                        <owl:onProperty rdf:resource="http://w3id.org/um/cbcm/eu-cm-ontology#employedBy"/>
                        <owl:someValuesFrom rdf:resource="http://www.w3.org/2002/07/owl#Thing"/>
                    </owl:Restriction>
                </owl:intersectionOf>
            </owl:Class>
        </owl:equivalentClass>
        <rdfs:subClassOf rdf:resource="http://w3id.org/um/cbcm/eu-cm-ontology#CompanyStakeholder"/>
        <rdfs:subClassOf rdf:resource="http://w3id.org/um/cbcm/eu-cm-ontology#Person"/>
        <opla-sd:entityPosition>
            <rdf:Description>
                <opla-sd:entityPositionX rdf:datatype="http://www.w3.org/2001/XMLSchema#double">133.07894884155147</opla-sd:entityPositionX>
                <opla-sd:entityPositionY rdf:datatype="http://www.w3.org/2001/XMLSchema#double">204.49364169261378</opla-sd:entityPositionY>
                <rdfs:comment xml:lang="en">This is an entity positioning annotation generated by CoModIDE (https://comodide.com/). Removing this annotation will break rendering the CoModIDE schema diagram view.</rdfs:comment>
            </rdf:Description>
        </opla-sd:entityPosition>
        <rdfs:comment xml:lang="en">The workforce of a company. An employee is a party to an employment relationship characterised as a contract of employment (or contract of service) between the employer and employee. However, this is only one of several different legal formulations of the concept of ‘worker’ in the EU which differ between Member States.</rdfs:comment>
        <rdfs:label xml:lang="en">Company employee</rdfs:label>
        <rdfs:seeAlso rdf:resource="https://www.eurofound.europa.eu/observatories/eurwork/industrial-relations-dictionary/employee"/>
    </owl:Class>
    


    <!-- http://w3id.org/um/cbcm/eu-cm-ontology#Entity -->

    <owl:Class rdf:about="http://w3id.org/um/cbcm/eu-cm-ontology#Entity">
        <opla-sd:entityPosition>
            <rdf:Description>
                <opla-sd:entityPositionX rdf:datatype="http://www.w3.org/2001/XMLSchema#double">13.492948758835098</opla-sd:entityPositionX>
                <opla-sd:entityPositionY rdf:datatype="http://www.w3.org/2001/XMLSchema#double">254.38646259999092</opla-sd:entityPositionY>
                <rdfs:comment xml:lang="en">This is an entity positioning annotation generated by CoModIDE (https://comodide.com/). Removing this annotation will break rendering the CoModIDE schema diagram view.</rdfs:comment>
            </rdf:Description>
        </opla-sd:entityPosition>
        <terms:description xml:lang="en">Every thing is an entity.</terms:description>
        <rdfs:label>Entity</rdfs:label>
    </owl:Class>
    


    <!-- http://w3id.org/um/cbcm/eu-cm-ontology#FinancialServiceAuthority -->

    <owl:Class rdf:about="http://w3id.org/um/cbcm/eu-cm-ontology#FinancialServiceAuthority">
        <rdfs:subClassOf rdf:resource="http://w3id.org/um/cbcm/eu-cm-ontology#CompetentAuthority"/>
        <opla-sd:entityPosition>
            <rdf:Description>
                <opla-sd:entityPositionX rdf:datatype="http://www.w3.org/2001/XMLSchema#double">73.05750474990312</opla-sd:entityPositionX>
                <opla-sd:entityPositionY rdf:datatype="http://www.w3.org/2001/XMLSchema#double">213.43746597077725</opla-sd:entityPositionY>
                <rdfs:comment xml:lang="en">This is an entity positioning annotation generated by CoModIDE (https://comodide.com/). Removing this annotation will break rendering the CoModIDE schema diagram view.</rdfs:comment>
            </rdf:Description>
        </opla-sd:entityPosition>
        <rdfs:comment xml:lang="en">A body that regulates the financial services industry in a country (e.g. the UK), including most financial services markets, exchanges and firms.</rdfs:comment>
        <rdfs:label xml:lang="en">Financial service authority</rdfs:label>
    </owl:Class>
    


    <!-- http://w3id.org/um/cbcm/eu-cm-ontology#GeoPoliticalRegion -->

    <owl:Class rdf:about="http://w3id.org/um/cbcm/eu-cm-ontology#GeoPoliticalRegion">
        <rdfs:subClassOf rdf:resource="http://w3id.org/um/cbcm/eu-cm-ontology#SpatialRegion"/>
        <opla-sd:entityPosition>
            <rdf:Description>
                <opla-sd:entityPositionX rdf:datatype="http://www.w3.org/2001/XMLSchema#double">21.38698645493781</opla-sd:entityPositionX>
                <opla-sd:entityPositionY rdf:datatype="http://www.w3.org/2001/XMLSchema#double">257.0334908946398</opla-sd:entityPositionY>
                <rdfs:comment xml:lang="en">This is an entity positioning annotation generated by CoModIDE (https://comodide.com/). Removing this annotation will break rendering the CoModIDE schema diagram view.</rdfs:comment>
            </rdf:Description>
        </opla-sd:entityPosition>
        <terms:description xml:lang="en">A spatial region on earth whose boundaries are determined by a combination of geographical, ecological, climatic, socio-economic and political criteria.</terms:description>
        <rdfs:label>Geo-political region</rdfs:label>
    </owl:Class>
    


    <!-- http://w3id.org/um/cbcm/eu-cm-ontology#GlobalUltimateOwner -->

    <owl:Class rdf:about="http://w3id.org/um/cbcm/eu-cm-ontology#GlobalUltimateOwner">
        <rdfs:subClassOf rdf:resource="http://w3id.org/um/cbcm/eu-cm-ontology#CompanyStakeholder"/>
        <rdfs:subClassOf>
            <owl:Restriction>
                <owl:onProperty rdf:resource="http://w3id.org/um/cbcm/eu-cm-ontology#owns"/>
                <owl:someValuesFrom rdf:resource="http://w3id.org/um/cbcm/eu-cm-ontology#Company"/>
            </owl:Restriction>
        </rdfs:subClassOf>
        <opla-sd:entityPosition>
            <rdf:Description>
                <opla-sd:entityPositionX rdf:datatype="http://www.w3.org/2001/XMLSchema#double">108.15208532227724</opla-sd:entityPositionX>
                <opla-sd:entityPositionY rdf:datatype="http://www.w3.org/2001/XMLSchema#double">178.8167600210412</opla-sd:entityPositionY>
                <rdfs:comment xml:lang="en">This is an entity positioning annotation generated by CoModIDE (https://comodide.com/). Removing this annotation will break rendering the CoModIDE schema diagram view.</rdfs:comment>
            </rdf:Description>
        </opla-sd:entityPosition>
        <rdfs:comment xml:lang="en">A global ultimate owner (GUO) is the individual or entity at the top of the corporate ownership structure.</rdfs:comment>
        <rdfs:label xml:lang="en">Global ultimate owner</rdfs:label>
    </owl:Class>
    


    <!-- http://w3id.org/um/cbcm/eu-cm-ontology#ImpactOnEmploymentRight -->

    <owl:Class rdf:about="http://w3id.org/um/cbcm/eu-cm-ontology#ImpactOnEmploymentRight">
        <rdfs:subClassOf rdf:resource="http://w3id.org/um/cbcm/eu-cm-ontology#InformationRight"/>
        <opla-sd:entityPosition>
            <rdf:Description>
                <opla-sd:entityPositionX rdf:datatype="http://www.w3.org/2001/XMLSchema#double">56.39142121243984</opla-sd:entityPositionX>
                <opla-sd:entityPositionY rdf:datatype="http://www.w3.org/2001/XMLSchema#double">216.7825777726235</opla-sd:entityPositionY>
                <rdfs:comment xml:lang="en">This is an entity positioning annotation generated by CoModIDE (https://comodide.com/). Removing this annotation will break rendering the CoModIDE schema diagram view.</rdfs:comment>
            </rdf:Description>
        </opla-sd:entityPosition>
        <rdfs:comment xml:lang="en">The right of employees or their representatives to be informed on the likely repercussions of the cross-border transaction on employment, which includes the dismissal as well as the hiring of employees or relocation of work. See for instance article 122 of Directive 2017/1132.</rdfs:comment>
        <rdfs:label xml:lang="en">Impact on employment information right</rdfs:label>
        <rdfs:seeAlso rdf:resource="http://data.europa.eu/eli/dir/2017/1132/oj"/>
    </owl:Class>
    


    <!-- http://w3id.org/um/cbcm/eu-cm-ontology#IndependentExpert -->

    <owl:Class rdf:about="http://w3id.org/um/cbcm/eu-cm-ontology#IndependentExpert">
        <rdfs:subClassOf rdf:resource="http://w3id.org/um/cbcm/eu-cm-ontology#CompanyStakeholder"/>
        <opla-sd:entityPosition>
            <rdf:Description>
                <opla-sd:entityPositionX rdf:datatype="http://www.w3.org/2001/XMLSchema#double">140.1633297609779</opla-sd:entityPositionX>
                <opla-sd:entityPositionY rdf:datatype="http://www.w3.org/2001/XMLSchema#double">87.43539384190532</opla-sd:entityPositionY>
                <rdfs:comment xml:lang="en">This is an entity positioning annotation generated by CoModIDE (https://comodide.com/). Removing this annotation will break rendering the CoModIDE schema diagram view.</rdfs:comment>
            </rdf:Description>
        </opla-sd:entityPosition>
        <rdfs:comment xml:lang="en">An Independent Expert provides impartial advice to shareholders and other company stakeholders on the fairness and/or reasonableness of a transaction.  A company may be required to commission an Independent Expert Report (IER) in the case of a (cross-border) merger, division or conversion.</rdfs:comment>
        <rdfs:label xml:lang="en">Independent expert</rdfs:label>
        <rdfs:seeAlso rdf:resource="http://data.europa.eu/eli/dir/2017/1132/oj"/>
        <rdfs:seeAlso rdf:resource="https://www.europarl.europa.eu/doceo/document/TA-8-2019-0429_EN.html"/>
    </owl:Class>
    


    <!-- http://w3id.org/um/cbcm/eu-cm-ontology#IndependentExpertReport -->

    <owl:Class rdf:about="http://w3id.org/um/cbcm/eu-cm-ontology#IndependentExpertReport">
        <rdfs:subClassOf rdf:resource="http://w3id.org/um/cbcm/eu-cm-ontology#TransactionDocument"/>
        <rdfs:subClassOf>
            <owl:Restriction>
                <owl:onProperty rdf:resource="http://w3id.org/um/cbcm/eu-cm-ontology#authoredBy"/>
                <owl:someValuesFrom rdf:resource="http://w3id.org/um/cbcm/eu-cm-ontology#IndependentExpert"/>
            </owl:Restriction>
        </rdfs:subClassOf>
        <opla-sd:entityPosition>
            <rdf:Description>
                <opla-sd:entityPositionX rdf:datatype="http://www.w3.org/2001/XMLSchema#double">61.530578065886296</opla-sd:entityPositionX>
                <opla-sd:entityPositionY rdf:datatype="http://www.w3.org/2001/XMLSchema#double">60.210456156221056</opla-sd:entityPositionY>
                <rdfs:comment xml:lang="en">This is an entity positioning annotation generated by CoModIDE (https://comodide.com/). Removing this annotation will break rendering the CoModIDE schema diagram view.</rdfs:comment>
            </rdf:Description>
        </opla-sd:entityPosition>
        <rdfs:comment xml:lang="en">Article 86g and 160i: Member States must ensure that an independent expert examines the draft terms of the transaction and draws up a report intended for members which is made available to them not less than one month before the date of the general meeting. Depending on the law of Member States, the expert may be a natural person or a legal person. The report must assess the cash compensation proposed and valuation method.</rdfs:comment>
        <rdfs:label xml:lang="en">Report by an independent expert</rdfs:label>
        <rdfs:seeAlso rdf:resource="https://www.europarl.europa.eu/doceo/document/TA-8-2019-0429_EN.html"/>
    </owl:Class>
    


    <!-- http://w3id.org/um/cbcm/eu-cm-ontology#InformationRight -->

    <owl:Class rdf:about="http://w3id.org/um/cbcm/eu-cm-ontology#InformationRight">
        <rdfs:subClassOf rdf:resource="http://w3id.org/um/cbcm/eu-cm-ontology#SocialRight"/>
        <opla-sd:entityPosition>
            <rdf:Description>
                <opla-sd:entityPositionX rdf:datatype="http://www.w3.org/2001/XMLSchema#double">35.933964425097344</opla-sd:entityPositionX>
                <opla-sd:entityPositionY rdf:datatype="http://www.w3.org/2001/XMLSchema#double">258.5099794114055</opla-sd:entityPositionY>
                <rdfs:comment xml:lang="en">This is an entity positioning annotation generated by CoModIDE (https://comodide.com/). Removing this annotation will break rendering the CoModIDE schema diagram view.</rdfs:comment>
            </rdf:Description>
        </opla-sd:entityPosition>
        <rdfs:comment xml:lang="en">The right of employees or their representatives to be informed and to receive any documents necessary for the exercise of their consultation and board-level employee representation rights in the context of an intended merger/division/conversion/seat transfer.</rdfs:comment>
        <rdfs:label xml:lang="en">Information right</rdfs:label>
        <rdfs:seeAlso rdf:resource="http://data.europa.eu/eli/dir/2002/14/oj"/>
        <rdfs:seeAlso rdf:resource="http://data.europa.eu/eli/dir/2017/1132/oj"/>
    </owl:Class>
    


    <!-- http://w3id.org/um/cbcm/eu-cm-ontology#InterimAccount -->

    <owl:Class rdf:about="http://w3id.org/um/cbcm/eu-cm-ontology#InterimAccount">
        <rdfs:subClassOf rdf:resource="http://w3id.org/um/cbcm/eu-cm-ontology#AnnualAccount"/>
        <opla-sd:entityPosition>
            <rdf:Description>
                <opla-sd:entityPositionX rdf:datatype="http://www.w3.org/2001/XMLSchema#double">255.33845538498926</opla-sd:entityPositionX>
                <opla-sd:entityPositionY rdf:datatype="http://www.w3.org/2001/XMLSchema#double">160.2244819330443</opla-sd:entityPositionY>
                <rdfs:comment xml:lang="en">This is an entity positioning annotation generated by CoModIDE (https://comodide.com/). Removing this annotation will break rendering the CoModIDE schema diagram view.</rdfs:comment>
            </rdf:Description>
        </opla-sd:entityPosition>
        <rdfs:comment xml:lang="en">Interim accounts are accounts that are published during a company&apos;s financial year and that show the financial situation on a given accounting date.</rdfs:comment>
        <rdfs:label xml:lang="en">Interim account</rdfs:label>
    </owl:Class>
    


    <!-- http://w3id.org/um/cbcm/eu-cm-ontology#ManagementBoard -->

    <owl:Class rdf:about="http://w3id.org/um/cbcm/eu-cm-ontology#ManagementBoard">
        <rdfs:subClassOf rdf:resource="http://w3id.org/um/cbcm/eu-cm-ontology#Manager"/>
        <rdfs:subClassOf>
            <owl:Restriction>
                <owl:onProperty rdf:resource="http://w3id.org/um/cbcm/eu-cm-ontology#partOf"/>
                <owl:someValuesFrom rdf:resource="http://w3id.org/um/cbcm/eu-cm-ontology#Company"/>
            </owl:Restriction>
        </rdfs:subClassOf>
        <opla-sd:entityPosition>
            <rdf:Description>
                <opla-sd:entityPositionX rdf:datatype="http://www.w3.org/2001/XMLSchema#double">64.26195094994145</opla-sd:entityPositionX>
                <opla-sd:entityPositionY rdf:datatype="http://www.w3.org/2001/XMLSchema#double">130.33558418291966</opla-sd:entityPositionY>
                <rdfs:comment xml:lang="en">This is an entity positioning annotation generated by CoModIDE (https://comodide.com/). Removing this annotation will break rendering the CoModIDE schema diagram view.</rdfs:comment>
            </rdf:Description>
        </opla-sd:entityPosition>
        <rdfs:comment xml:lang="en">The group of persons comprising the governing body of the legal entity that is entrusted with the decision-making in the company. It is also called Executive Board in a one-tier board system.</rdfs:comment>
        <rdfs:label xml:lang="en">Management board</rdfs:label>
    </owl:Class>
    


    <!-- http://w3id.org/um/cbcm/eu-cm-ontology#ManagementReport -->

    <owl:Class rdf:about="http://w3id.org/um/cbcm/eu-cm-ontology#ManagementReport">
        <rdfs:subClassOf rdf:resource="http://w3id.org/um/cbcm/eu-cm-ontology#TransactionDocument"/>
        <opla-sd:entityPosition>
            <rdf:Description>
                <opla-sd:entityPositionX rdf:datatype="http://www.w3.org/2001/XMLSchema#double">159.33996695202816</opla-sd:entityPositionX>
                <opla-sd:entityPositionY rdf:datatype="http://www.w3.org/2001/XMLSchema#double">229.01179631361057</opla-sd:entityPositionY>
                <rdfs:comment xml:lang="en">This is an entity positioning annotation generated by CoModIDE (https://comodide.com/). Removing this annotation will break rendering the CoModIDE schema diagram view.</rdfs:comment>
            </rdf:Description>
        </opla-sd:entityPosition>
        <rdfs:comment xml:lang="en">A report drawn up by the company&apos;s management on the intended transaction, laying out the main features of the transactions and its consequences.</rdfs:comment>
        <rdfs:label xml:lang="en">Management report</rdfs:label>
    </owl:Class>
    


    <!-- http://w3id.org/um/cbcm/eu-cm-ontology#Manager -->

    <owl:Class rdf:about="http://w3id.org/um/cbcm/eu-cm-ontology#Manager">
        <rdfs:subClassOf rdf:resource="http://w3id.org/um/cbcm/eu-cm-ontology#CompanyStakeholder"/>
        <rdfs:comment xml:lang="en">A person or group of persons that are responsible for overseeing the operations of a company.</rdfs:comment>
        <rdfs:label xml:lang="en">Manager</rdfs:label>
    </owl:Class>
    


    <!-- http://w3id.org/um/cbcm/eu-cm-ontology#ManagerDecisionRight -->

    <owl:Class rdf:about="http://w3id.org/um/cbcm/eu-cm-ontology#ManagerDecisionRight">
        <rdfs:subClassOf rdf:resource="http://w3id.org/um/cbcm/eu-cm-ontology#ManagerRight"/>
        <opla-sd:entityPosition>
            <rdf:Description>
                <opla-sd:entityPositionX rdf:datatype="http://www.w3.org/2001/XMLSchema#double">80.8771489838024</opla-sd:entityPositionX>
                <opla-sd:entityPositionY rdf:datatype="http://www.w3.org/2001/XMLSchema#double">17.963298319155722</opla-sd:entityPositionY>
                <rdfs:comment xml:lang="en">This is an entity positioning annotation generated by CoModIDE (https://comodide.com/). Removing this annotation will break rendering the CoModIDE schema diagram view.</rdfs:comment>
            </rdf:Description>
        </opla-sd:entityPosition>
        <rdfs:comment xml:lang="en">The right of the board of management or individual managers to take decisions or to not take a decision in the context of a transaction. These are in the form of a board resolution.</rdfs:comment>
        <rdfs:label xml:lang="en">Manager decision right</rdfs:label>
    </owl:Class>
    


    <!-- http://w3id.org/um/cbcm/eu-cm-ontology#ManagerExitRight -->

    <owl:Class rdf:about="http://w3id.org/um/cbcm/eu-cm-ontology#ManagerExitRight">
        <rdfs:subClassOf rdf:resource="http://w3id.org/um/cbcm/eu-cm-ontology#ManagerRight"/>
        <opla-sd:entityPosition>
            <rdf:Description>
                <opla-sd:entityPositionX rdf:datatype="http://www.w3.org/2001/XMLSchema#double">5.230804892398894</opla-sd:entityPositionX>
                <opla-sd:entityPositionY rdf:datatype="http://www.w3.org/2001/XMLSchema#double">190.27823337848955</opla-sd:entityPositionY>
                <rdfs:comment xml:lang="en">This is an entity positioning annotation generated by CoModIDE (https://comodide.com/). Removing this annotation will break rendering the CoModIDE schema diagram view.</rdfs:comment>
            </rdf:Description>
        </opla-sd:entityPosition>
        <rdfs:comment xml:lang="en">The right of a manager or the board of management to resign and therefore exit a company.</rdfs:comment>
        <rdfs:label xml:lang="en">Manager exit right</rdfs:label>
    </owl:Class>
    


    <!-- http://w3id.org/um/cbcm/eu-cm-ontology#ManagerInformationRight -->

    <owl:Class rdf:about="http://w3id.org/um/cbcm/eu-cm-ontology#ManagerInformationRight">
        <rdfs:subClassOf rdf:resource="http://w3id.org/um/cbcm/eu-cm-ontology#ManagerRight"/>
        <opla-sd:entityPosition>
            <rdf:Description>
                <opla-sd:entityPositionX rdf:datatype="http://www.w3.org/2001/XMLSchema#double">131.1694963522508</opla-sd:entityPositionX>
                <opla-sd:entityPositionY rdf:datatype="http://www.w3.org/2001/XMLSchema#double">116.43831846425745</opla-sd:entityPositionY>
                <rdfs:comment xml:lang="en">This is an entity positioning annotation generated by CoModIDE (https://comodide.com/). Removing this annotation will break rendering the CoModIDE schema diagram view.</rdfs:comment>
            </rdf:Description>
        </opla-sd:entityPosition>
        <rdfs:comment xml:lang="en">The right of a manager to information and access to documents that he or she has in accordance with national or European company law.</rdfs:comment>
        <rdfs:label xml:lang="en">Manager information right</rdfs:label>
    </owl:Class>
    


    <!-- http://w3id.org/um/cbcm/eu-cm-ontology#ManagerRight -->

    <owl:Class rdf:about="http://w3id.org/um/cbcm/eu-cm-ontology#ManagerRight">
        <rdfs:subClassOf rdf:resource="http://w3id.org/um/cbcm/eu-cm-ontology#TransactionRight"/>
        <rdfs:subClassOf>
            <owl:Restriction>
                <owl:onProperty rdf:resource="http://w3id.org/um/cbcm/eu-cm-ontology#applicableTo"/>
                <owl:someValuesFrom rdf:resource="http://w3id.org/um/cbcm/eu-cm-ontology#Manager"/>
            </owl:Restriction>
        </rdfs:subClassOf>
        <opla-sd:entityPosition>
            <rdf:Description>
                <opla-sd:entityPositionX rdf:datatype="http://www.w3.org/2001/XMLSchema#double">259.8641767341787</opla-sd:entityPositionX>
                <opla-sd:entityPositionY rdf:datatype="http://www.w3.org/2001/XMLSchema#double">141.81062591873996</opla-sd:entityPositionY>
                <rdfs:comment xml:lang="en">This is an entity positioning annotation generated by CoModIDE (https://comodide.com/). Removing this annotation will break rendering the CoModIDE schema diagram view.</rdfs:comment>
            </rdf:Description>
        </opla-sd:entityPosition>
        <rdfs:comment xml:lang="en">The rights of members of the management in the context of a company transaction.</rdfs:comment>
        <rdfs:label xml:lang="en">Manager right</rdfs:label>
    </owl:Class>
    


    <!-- http://w3id.org/um/cbcm/eu-cm-ontology#MemberStateOfficialJournal -->

    <owl:Class rdf:about="http://w3id.org/um/cbcm/eu-cm-ontology#MemberStateOfficialJournal">
        <rdfs:subClassOf rdf:resource="http://w3id.org/um/cbcm/eu-cm-ontology#OfficialJournal"/>
        <opla-sd:entityPosition>
            <rdf:Description>
                <opla-sd:entityPositionX rdf:datatype="http://www.w3.org/2001/XMLSchema#double">76.24578994947785</opla-sd:entityPositionX>
                <opla-sd:entityPositionY rdf:datatype="http://www.w3.org/2001/XMLSchema#double">294.15047197456164</opla-sd:entityPositionY>
                <rdfs:comment xml:lang="en">This is an entity positioning annotation generated by CoModIDE (https://comodide.com/). Removing this annotation will break rendering the CoModIDE schema diagram view.</rdfs:comment>
            </rdf:Description>
        </opla-sd:entityPosition>
        <rdfs:comment xml:lang="en">The national gazette or record in a particular Member State. In the official journal companies publish company transaction notices in order to inform concerned stakeholders and interested parties.</rdfs:comment>
        <rdfs:label>Member State Official Journal</rdfs:label>
    </owl:Class>
    


    <!-- http://w3id.org/um/cbcm/eu-cm-ontology#MergerCertificate -->

    <owl:Class rdf:about="http://w3id.org/um/cbcm/eu-cm-ontology#MergerCertificate">
        <rdfs:subClassOf rdf:resource="http://w3id.org/um/cbcm/eu-cm-ontology#TransactionCertificate"/>
        <opla-sd:entityPosition>
            <rdf:Description>
                <opla-sd:entityPositionX rdf:datatype="http://www.w3.org/2001/XMLSchema#double">189.1653478306684</opla-sd:entityPositionX>
                <opla-sd:entityPositionY rdf:datatype="http://www.w3.org/2001/XMLSchema#double">289.9707044471894</opla-sd:entityPositionY>
                <rdfs:comment xml:lang="en">This is an entity positioning annotation generated by CoModIDE (https://comodide.com/). Removing this annotation will break rendering the CoModIDE schema diagram view.</rdfs:comment>
            </rdf:Description>
        </opla-sd:entityPosition>
        <rdfs:comment xml:lang="en">A document issued by a Competent Authority declaring that the legally required steps of a merger are completed. The certificate needs to be presented by a company to either be registered in another company registry or to be removed from a company register (depending on the company being the merging or acquiring company).</rdfs:comment>
        <rdfs:label xml:lang="en">Company merger certificate</rdfs:label>
        <rdfs:seeAlso rdf:resource="http://data.europa.eu/eli/dir/2017/1132/oj"/>
    </owl:Class>
    


    <!-- http://w3id.org/um/cbcm/eu-cm-ontology#MergerPlan -->

    <owl:Class rdf:about="http://w3id.org/um/cbcm/eu-cm-ontology#MergerPlan">
        <rdfs:subClassOf rdf:resource="http://w3id.org/um/cbcm/eu-cm-ontology#TransactionDocument"/>
        <opla-sd:entityPosition>
            <rdf:Description>
                <opla-sd:entityPositionX rdf:datatype="http://www.w3.org/2001/XMLSchema#double">68.478522511586</opla-sd:entityPositionX>
                <opla-sd:entityPositionY rdf:datatype="http://www.w3.org/2001/XMLSchema#double">223.39629614148157</opla-sd:entityPositionY>
                <rdfs:comment xml:lang="en">This is an entity positioning annotation generated by CoModIDE (https://comodide.com/). Removing this annotation will break rendering the CoModIDE schema diagram view.</rdfs:comment>
            </rdf:Description>
        </opla-sd:entityPosition>
        <rdfs:comment xml:lang="en">Article 91: The administrative or management bodies of the merging companies shall draw up draft terms of merger in writing by specifying at least the elements mentioned in article 91.</rdfs:comment>
        <rdfs:label xml:lang="en">Company merger plan</rdfs:label>
        <rdfs:seeAlso rdf:resource="http://data.europa.eu/eli/dir/2017/1132/oj"/>
    </owl:Class>
    


    <!-- http://w3id.org/um/cbcm/eu-cm-ontology#MergingCompany -->

    <owl:Class rdf:about="http://w3id.org/um/cbcm/eu-cm-ontology#MergingCompany">
        <rdfs:subClassOf rdf:resource="http://w3id.org/um/cbcm/eu-cm-ontology#Company"/>
        <rdfs:subClassOf>
            <owl:Restriction>
                <owl:onProperty rdf:resource="http://w3id.org/um/cbcm/eu-cm-ontology#isTransactionInputOf"/>
                <owl:someValuesFrom rdf:resource="http://w3id.org/um/cbcm/eu-cm-ontology#CompanyMerger"/>
            </owl:Restriction>
        </rdfs:subClassOf>
        <opla-sd:entityPosition>
            <rdf:Description>
                <opla-sd:entityPositionX rdf:datatype="http://www.w3.org/2001/XMLSchema#double">89.07393569063014</opla-sd:entityPositionX>
                <opla-sd:entityPositionY rdf:datatype="http://www.w3.org/2001/XMLSchema#double">255.2221941277188</opla-sd:entityPositionY>
                <rdfs:comment xml:lang="en">This is an entity positioning annotation generated by CoModIDE (https://comodide.com/). Removing this annotation will break rendering the CoModIDE schema diagram view.</rdfs:comment>
            </rdf:Description>
        </opla-sd:entityPosition>
        <rdfs:comment xml:lang="en">Merging Company means the dissolving company that is being acquired by another (acquiring) company in the process of a transaction. In the context of company mobility, this means a universal transfer of assets and liabilities from the merging to the acquiring company (see article 131 of Directive 2017/1132).</rdfs:comment>
        <rdfs:label xml:lang="en">Merging company</rdfs:label>
        <rdfs:seeAlso rdf:resource="http://data.europa.eu/eli/dir/2017/1132/oj"/>
    </owl:Class>
    


    <!-- http://w3id.org/um/cbcm/eu-cm-ontology#NationalRegistry -->

    <owl:Class rdf:about="http://w3id.org/um/cbcm/eu-cm-ontology#NationalRegistry">
        <rdfs:subClassOf rdf:resource="http://w3id.org/um/cbcm/eu-cm-ontology#Organisation"/>
        <opla-sd:entityPosition>
            <rdf:Description>
                <opla-sd:entityPositionX rdf:datatype="http://www.w3.org/2001/XMLSchema#double">208.525212634583</opla-sd:entityPositionX>
                <opla-sd:entityPositionY rdf:datatype="http://www.w3.org/2001/XMLSchema#double">206.33370239048014</opla-sd:entityPositionY>
                <rdfs:comment xml:lang="en">This is an entity positioning annotation generated by CoModIDE (https://comodide.com/). Removing this annotation will break rendering the CoModIDE schema diagram view.</rdfs:comment>
            </rdf:Description>
        </opla-sd:entityPosition>
        <rdfs:comment xml:lang="en">A national registry is a business registry in a Member State, which includes information on the population of companies in the jurisdiction and holds inter alia data on registration numbers, place of registration, notices and transaction documents in the national registry repository.</rdfs:comment>
        <rdfs:label xml:lang="en">National registry</rdfs:label>
    </owl:Class>
    


    <!-- http://w3id.org/um/cbcm/eu-cm-ontology#NationalRegistryRepository -->

    <owl:Class rdf:about="http://w3id.org/um/cbcm/eu-cm-ontology#NationalRegistryRepository">
        <rdfs:subClassOf rdf:resource="http://w3id.org/um/cbcm/eu-cm-ontology#DocumentRepository"/>
        <rdfs:subClassOf>
            <owl:Restriction>
                <owl:onProperty rdf:resource="http://w3id.org/um/cbcm/eu-cm-ontology#maintainedBy"/>
                <owl:someValuesFrom rdf:resource="http://w3id.org/um/cbcm/eu-cm-ontology#NationalRegistry"/>
            </owl:Restriction>
        </rdfs:subClassOf>
        <opla-sd:entityPosition>
            <rdf:Description>
                <opla-sd:entityPositionX rdf:datatype="http://www.w3.org/2001/XMLSchema#double">135.9577611146716</opla-sd:entityPositionX>
                <opla-sd:entityPositionY rdf:datatype="http://www.w3.org/2001/XMLSchema#double">5.799956832418123</opla-sd:entityPositionY>
                <rdfs:comment xml:lang="en">This is an entity positioning annotation generated by CoModIDE (https://comodide.com/). Removing this annotation will break rendering the CoModIDE schema diagram view.</rdfs:comment>
            </rdf:Description>
        </opla-sd:entityPosition>
        <rdfs:comment xml:lang="en">The digital repository in which documents published in the official journal or by by the national registry (on behalf of a company) are kept as well as related documents. In some EU Member States, this repository is overlapping or identical with the Official Journal Repository.</rdfs:comment>
        <rdfs:label xml:lang="en">National registry repository</rdfs:label>
    </owl:Class>
    


    <!-- http://w3id.org/um/cbcm/eu-cm-ontology#NonEEACountry -->

    <owl:Class rdf:about="http://w3id.org/um/cbcm/eu-cm-ontology#NonEEACountry">
        <rdfs:subClassOf rdf:resource="http://w3id.org/um/cbcm/eu-cm-ontology#NonEUCountry"/>
        <opla-sd:entityPosition>
            <rdf:Description>
                <opla-sd:entityPositionX rdf:datatype="http://www.w3.org/2001/XMLSchema#double">4.045785894080908</opla-sd:entityPositionX>
                <opla-sd:entityPositionY rdf:datatype="http://www.w3.org/2001/XMLSchema#double">258.29866804820614</opla-sd:entityPositionY>
                <rdfs:comment xml:lang="en">This is an entity positioning annotation generated by CoModIDE (https://comodide.com/). Removing this annotation will break rendering the CoModIDE schema diagram view.</rdfs:comment>
            </rdf:Description>
        </opla-sd:entityPosition>
        <rdfs:comment xml:lang="en">A country which does not belong to the European Economic Area (EEA).</rdfs:comment>
        <rdfs:label xml:lang="en">Non-EEA country</rdfs:label>
    </owl:Class>
    


    <!-- http://w3id.org/um/cbcm/eu-cm-ontology#NonEUCountry -->

    <owl:Class rdf:about="http://w3id.org/um/cbcm/eu-cm-ontology#NonEUCountry">
        <rdfs:subClassOf rdf:resource="http://w3id.org/um/cbcm/eu-cm-ontology#Country"/>
        <opla-sd:entityPosition>
            <rdf:Description>
                <opla-sd:entityPositionX rdf:datatype="http://www.w3.org/2001/XMLSchema#double">39.890708486514455</opla-sd:entityPositionX>
                <opla-sd:entityPositionY rdf:datatype="http://www.w3.org/2001/XMLSchema#double">90.27129916163625</opla-sd:entityPositionY>
                <rdfs:comment xml:lang="en">This is an entity positioning annotation generated by CoModIDE (https://comodide.com/). Removing this annotation will break rendering the CoModIDE schema diagram view.</rdfs:comment>
            </rdf:Description>
        </opla-sd:entityPosition>
        <rdfs:comment xml:lang="en">A country that does not officially belong to the EU conglomeration</rdfs:comment>
        <rdfs:label xml:lang="en">Non-EU country</rdfs:label>
    </owl:Class>
    


    <!-- http://w3id.org/um/cbcm/eu-cm-ontology#Notary -->

    <owl:Class rdf:about="http://w3id.org/um/cbcm/eu-cm-ontology#Notary">
        <rdfs:subClassOf rdf:resource="http://w3id.org/um/cbcm/eu-cm-ontology#CompetentAuthority"/>
        <opla-sd:entityPosition>
            <rdf:Description>
                <opla-sd:entityPositionX rdf:datatype="http://www.w3.org/2001/XMLSchema#double">217.12121779262185</opla-sd:entityPositionX>
                <opla-sd:entityPositionY rdf:datatype="http://www.w3.org/2001/XMLSchema#double">100.83729366048524</opla-sd:entityPositionY>
                <rdfs:comment xml:lang="en">This is an entity positioning annotation generated by CoModIDE (https://comodide.com/). Removing this annotation will break rendering the CoModIDE schema diagram view.</rdfs:comment>
            </rdf:Description>
        </opla-sd:entityPosition>
        <rdfs:comment xml:lang="en">A person authorized to perform certain legal formalities, especially to draw up or certify contracts, deeds, and other documents for use in other jurisdictions.</rdfs:comment>
        <rdfs:label xml:lang="en">Notary</rdfs:label>
    </owl:Class>
    


    <!-- http://w3id.org/um/cbcm/eu-cm-ontology#Object -->

    <owl:Class rdf:about="http://w3id.org/um/cbcm/eu-cm-ontology#Object">
        <rdfs:subClassOf rdf:resource="http://w3id.org/um/cbcm/eu-cm-ontology#Entity"/>
        <opla-sd:entityPosition>
            <rdf:Description>
                <opla-sd:entityPositionX rdf:datatype="http://www.w3.org/2001/XMLSchema#double">155.30759761766964</opla-sd:entityPositionX>
                <opla-sd:entityPositionY rdf:datatype="http://www.w3.org/2001/XMLSchema#double">245.90165854196664</opla-sd:entityPositionY>
                <rdfs:comment xml:lang="en">This is an entity positioning annotation generated by CoModIDE (https://comodide.com/). Removing this annotation will break rendering the CoModIDE schema diagram view.</rdfs:comment>
            </rdf:Description>
        </opla-sd:entityPosition>
        <terms:description xml:lang="en">An object is an inert entity that is wholly identifiable at any instant of time during which it exists. It is inert in the sense that it cannot perform any action autonomously.</terms:description>
        <rdfs:label>Object</rdfs:label>
    </owl:Class>
    


    <!-- http://w3id.org/um/cbcm/eu-cm-ontology#OfficialJournal -->

    <owl:Class rdf:about="http://w3id.org/um/cbcm/eu-cm-ontology#OfficialJournal">
        <rdfs:subClassOf rdf:resource="http://w3id.org/um/cbcm/eu-cm-ontology#Organisation"/>
        <opla-sd:entityPosition>
            <rdf:Description>
                <opla-sd:entityPositionX rdf:datatype="http://www.w3.org/2001/XMLSchema#double">232.05108775996405</opla-sd:entityPositionX>
                <opla-sd:entityPositionY rdf:datatype="http://www.w3.org/2001/XMLSchema#double">94.87943358517005</opla-sd:entityPositionY>
                <rdfs:comment xml:lang="en">This is an entity positioning annotation generated by CoModIDE (https://comodide.com/). Removing this annotation will break rendering the CoModIDE schema diagram view.</rdfs:comment>
            </rdf:Description>
        </opla-sd:entityPosition>
        <rdfs:comment xml:lang="en">The official gazette of record for the European Union or national gazette of record of a Member State. In the official journal companies publish transaction notices in order to inform concerned stakeholders and interested parties.</rdfs:comment>
        <rdfs:label xml:lang="en">Official journal</rdfs:label>
    </owl:Class>
    


    <!-- http://w3id.org/um/cbcm/eu-cm-ontology#OfficialJournalPublication -->

    <owl:Class rdf:about="http://w3id.org/um/cbcm/eu-cm-ontology#OfficialJournalPublication">
        <rdfs:subClassOf rdf:resource="http://w3id.org/um/cbcm/eu-cm-ontology#CompanyMobilityDocument"/>
        <opla-sd:entityPosition>
            <rdf:Description>
                <opla-sd:entityPositionX rdf:datatype="http://www.w3.org/2001/XMLSchema#double">77.00914110402874</opla-sd:entityPositionX>
                <opla-sd:entityPositionY rdf:datatype="http://www.w3.org/2001/XMLSchema#double">293.9661756024349</opla-sd:entityPositionY>
                <rdfs:comment xml:lang="en">This is an entity positioning annotation generated by CoModIDE (https://comodide.com/). Removing this annotation will break rendering the CoModIDE schema diagram view.</rdfs:comment>
            </rdf:Description>
        </opla-sd:entityPosition>
        <rdfs:comment xml:lang="en">Publication of a legally valid record or act in an official national gazette to inform stakeholders.</rdfs:comment>
        <rdfs:label xml:lang="en">Official journal publication</rdfs:label>
    </owl:Class>
    


    <!-- http://w3id.org/um/cbcm/eu-cm-ontology#OfficialJournalRepository -->

    <owl:Class rdf:about="http://w3id.org/um/cbcm/eu-cm-ontology#OfficialJournalRepository">
        <rdfs:subClassOf rdf:resource="http://w3id.org/um/cbcm/eu-cm-ontology#DocumentRepository"/>
        <rdfs:subClassOf>
            <owl:Restriction>
                <owl:onProperty rdf:resource="http://w3id.org/um/cbcm/eu-cm-ontology#maintainedBy"/>
                <owl:someValuesFrom rdf:resource="http://w3id.org/um/cbcm/eu-cm-ontology#OfficialJournal"/>
            </owl:Restriction>
        </rdfs:subClassOf>
        <opla-sd:entityPosition>
            <rdf:Description>
                <opla-sd:entityPositionX rdf:datatype="http://www.w3.org/2001/XMLSchema#double">118.49018012003486</opla-sd:entityPositionX>
                <opla-sd:entityPositionY rdf:datatype="http://www.w3.org/2001/XMLSchema#double">283.37643375648975</opla-sd:entityPositionY>
                <rdfs:comment xml:lang="en">This is an entity positioning annotation generated by CoModIDE (https://comodide.com/). Removing this annotation will break rendering the CoModIDE schema diagram view.</rdfs:comment>
            </rdf:Description>
        </opla-sd:entityPosition>
        <rdfs:comment xml:lang="en">The digital repository in which documents published in the official journal are kept as well as related documents. In some EU Member States, this repository is overlapping or identical with the National Registry Repository.</rdfs:comment>
        <rdfs:label xml:lang="en">Official journal repository</rdfs:label>
    </owl:Class>
    


    <!-- http://w3id.org/um/cbcm/eu-cm-ontology#Organisation -->

    <owl:Class rdf:about="http://w3id.org/um/cbcm/eu-cm-ontology#Organisation">
        <rdfs:subClassOf rdf:resource="http://w3id.org/um/cbcm/eu-cm-ontology#Agent"/>
        <owl:disjointWith rdf:resource="http://w3id.org/um/cbcm/eu-cm-ontology#Person"/>
        <opla-sd:entityPosition>
            <rdf:Description>
                <opla-sd:entityPositionX rdf:datatype="http://www.w3.org/2001/XMLSchema#double">248.07165150045202</opla-sd:entityPositionX>
                <opla-sd:entityPositionY rdf:datatype="http://www.w3.org/2001/XMLSchema#double">159.6891664652149</opla-sd:entityPositionY>
                <rdfs:comment xml:lang="en">This is an entity positioning annotation generated by CoModIDE (https://comodide.com/). Removing this annotation will break rendering the CoModIDE schema diagram view.</rdfs:comment>
            </rdf:Description>
        </opla-sd:entityPosition>
        <rdfs:comment xml:lang="en">Represents a collection of people organized together into a community or other social, commercial or political structure. The group has some common purpose or reason for existence which goes beyond the set of people belonging to it and can act as an Agent. Organizations are often decomposable into hierarchical structures.</rdfs:comment>
        <rdfs:label xml:lang="en">Organisation</rdfs:label>
    </owl:Class>
    


    <!-- http://w3id.org/um/cbcm/eu-cm-ontology#OrganisationalUnit -->

    <owl:Class rdf:about="http://w3id.org/um/cbcm/eu-cm-ontology#OrganisationalUnit">
        <rdfs:subClassOf rdf:resource="http://w3id.org/um/cbcm/eu-cm-ontology#Agent"/>
        <owl:disjointWith rdf:resource="http://w3id.org/um/cbcm/eu-cm-ontology#Person"/>
        <opla-sd:entityPosition>
            <rdf:Description>
                <opla-sd:entityPositionX rdf:datatype="http://www.w3.org/2001/XMLSchema#double">240.0027724881138</opla-sd:entityPositionX>
                <opla-sd:entityPositionY rdf:datatype="http://www.w3.org/2001/XMLSchema#double">111.43258260074302</opla-sd:entityPositionY>
                <rdfs:comment xml:lang="en">This is an entity positioning annotation generated by CoModIDE (https://comodide.com/). Removing this annotation will break rendering the CoModIDE schema diagram view.</rdfs:comment>
            </rdf:Description>
        </opla-sd:entityPosition>
        <rdfs:comment xml:lang="en">A division of a large organization such as a government, university, or business, dealing with a specific area of activity.</rdfs:comment>
        <rdfs:label xml:lang="en">Organisational unit</rdfs:label>
    </owl:Class>
    


    <!-- http://w3id.org/um/cbcm/eu-cm-ontology#OriginalCompany -->

    <owl:Class rdf:about="http://w3id.org/um/cbcm/eu-cm-ontology#OriginalCompany">
        <rdfs:subClassOf rdf:resource="http://w3id.org/um/cbcm/eu-cm-ontology#Company"/>
        <rdfs:subClassOf>
            <owl:Restriction>
                <owl:onProperty rdf:resource="http://w3id.org/um/cbcm/eu-cm-ontology#isTransactionInputOf"/>
                <owl:someValuesFrom rdf:resource="http://w3id.org/um/cbcm/eu-cm-ontology#CompanyTransaction"/>
            </owl:Restriction>
        </rdfs:subClassOf>
        <opla-sd:entityPosition>
            <rdf:Description>
                <opla-sd:entityPositionX rdf:datatype="http://www.w3.org/2001/XMLSchema#double">118.52899267564982</opla-sd:entityPositionX>
                <opla-sd:entityPositionY rdf:datatype="http://www.w3.org/2001/XMLSchema#double">235.53118442980525</opla-sd:entityPositionY>
                <rdfs:comment xml:lang="en">This is an entity positioning annotation generated by CoModIDE (https://comodide.com/). Removing this annotation will break rendering the CoModIDE schema diagram view.</rdfs:comment>
            </rdf:Description>
        </opla-sd:entityPosition>
        <rdfs:comment xml:lang="en">An original company, in the context of a (cross-border) division, means a company which - in case of a full division - transfers all its assets and liabilities to two or more companies, or - in case of a partial division or division by separation - transfers part of its assets and liabilities to one or more companies.</rdfs:comment>
        <rdfs:label xml:lang="en">Original company</rdfs:label>
        <rdfs:seeAlso rdf:resource="https://www.europarl.europa.eu/doceo/document/TA-8-2019-0429_EN.html"/>
    </owl:Class>
    


    <!-- http://w3id.org/um/cbcm/eu-cm-ontology#ParentCompany -->

    <owl:Class rdf:about="http://w3id.org/um/cbcm/eu-cm-ontology#ParentCompany">
        <owl:equivalentClass>
            <owl:Class>
                <owl:intersectionOf rdf:parseType="Collection">
                    <rdf:Description rdf:about="http://w3id.org/um/cbcm/eu-cm-ontology#Company"/>
                    <owl:Restriction>
                        <owl:onProperty rdf:resource="http://w3id.org/um/cbcm/eu-cm-ontology#hasSubsidiaryCompany"/>
                        <owl:someValuesFrom rdf:resource="http://w3id.org/um/cbcm/eu-cm-ontology#Company"/>
                    </owl:Restriction>
                </owl:intersectionOf>
            </owl:Class>
        </owl:equivalentClass>
        <opla-sd:entityPosition>
            <rdf:Description>
                <opla-sd:entityPositionX rdf:datatype="http://www.w3.org/2001/XMLSchema#double">205.63858499468532</opla-sd:entityPositionX>
                <opla-sd:entityPositionY rdf:datatype="http://www.w3.org/2001/XMLSchema#double">211.08101379570442</opla-sd:entityPositionY>
                <rdfs:comment xml:lang="en">This is an entity positioning annotation generated by CoModIDE (https://comodide.com/). Removing this annotation will break rendering the CoModIDE schema diagram view.</rdfs:comment>
            </rdf:Description>
        </opla-sd:entityPosition>
        <rdfs:comment xml:lang="en">A parent company is a company that has a controlling interest in another company, the subsidiary company, giving it control of its operations through a majority stock-ownership, decisive control over management appointments and therefore over the decision-making process. In the absence of a natural person as ultimate beneficial owner, the highest parent company in a chain of companies is the global ultimate owner.</rdfs:comment>
        <rdfs:label xml:lang="en">Parent company</rdfs:label>
        <rdfs:seeAlso rdf:resource="http://data.europa.eu/eli/dir/2017/1132/oj"/>
    </owl:Class>
    


    <!-- http://w3id.org/um/cbcm/eu-cm-ontology#Person -->

    <owl:Class rdf:about="http://w3id.org/um/cbcm/eu-cm-ontology#Person">
        <rdfs:subClassOf rdf:resource="http://w3id.org/um/cbcm/eu-cm-ontology#Agent"/>
        <opla-sd:entityPosition>
            <rdf:Description>
                <opla-sd:entityPositionX rdf:datatype="http://www.w3.org/2001/XMLSchema#double">209.24203764870728</opla-sd:entityPositionX>
                <opla-sd:entityPositionY rdf:datatype="http://www.w3.org/2001/XMLSchema#double">27.153209016526702</opla-sd:entityPositionY>
                <rdfs:comment xml:lang="en">This is an entity positioning annotation generated by CoModIDE (https://comodide.com/). Removing this annotation will break rendering the CoModIDE schema diagram view.</rdfs:comment>
            </rdf:Description>
        </opla-sd:entityPosition>
        <terms:description xml:lang="en">A person is an object that has certain capacities or attributes constituting personhood. A human being that has existed or continues to exist in the world (either deceased or living). Fictional human beings cannot be  instances of this class.</terms:description>
        <rdfs:label xml:lang="en">Person</rdfs:label>
    </owl:Class>
    


    <!-- http://w3id.org/um/cbcm/eu-cm-ontology#PreConversionCertificate -->

    <owl:Class rdf:about="http://w3id.org/um/cbcm/eu-cm-ontology#PreConversionCertificate">
        <rdfs:subClassOf rdf:resource="http://w3id.org/um/cbcm/eu-cm-ontology#TransactionCertificate"/>
        <opla-sd:entityPosition>
            <rdf:Description>
                <opla-sd:entityPositionX rdf:datatype="http://www.w3.org/2001/XMLSchema#double">38.09816258693692</opla-sd:entityPositionX>
                <opla-sd:entityPositionY rdf:datatype="http://www.w3.org/2001/XMLSchema#double">78.83721973670418</opla-sd:entityPositionY>
                <rdfs:comment xml:lang="en">This is an entity positioning annotation generated by CoModIDE (https://comodide.com/). Removing this annotation will break rendering the CoModIDE schema diagram view.</rdfs:comment>
            </rdf:Description>
        </opla-sd:entityPosition>
        <rdfs:comment xml:lang="en">Article 86m: a pre-conversion certificate attests compliance with all the relevant conditions and the proper completion of all procedures and formalities in the departure Member State.</rdfs:comment>
        <rdfs:label xml:lang="en">Company pre-conversion certificate</rdfs:label>
        <rdfs:seeAlso rdf:resource="https://www.europarl.europa.eu/doceo/document/TA-8-2019-0429_EN.html"/>
    </owl:Class>
    


    <!-- http://w3id.org/um/cbcm/eu-cm-ontology#PreDivisionCertificate -->

    <owl:Class rdf:about="http://w3id.org/um/cbcm/eu-cm-ontology#PreDivisionCertificate">
        <rdfs:subClassOf rdf:resource="http://w3id.org/um/cbcm/eu-cm-ontology#TransactionCertificate"/>
        <opla-sd:entityPosition>
            <rdf:Description>
                <opla-sd:entityPositionX rdf:datatype="http://www.w3.org/2001/XMLSchema#double">266.3774679637017</opla-sd:entityPositionX>
                <opla-sd:entityPositionY rdf:datatype="http://www.w3.org/2001/XMLSchema#double">151.75255166372014</opla-sd:entityPositionY>
                <rdfs:comment xml:lang="en">This is an entity positioning annotation generated by CoModIDE (https://comodide.com/). Removing this annotation will break rendering the CoModIDE schema diagram view.</rdfs:comment>
            </rdf:Description>
        </opla-sd:entityPosition>
        <rdfs:comment xml:lang="en">Article 160o: a pre-division certificate attests compliance with all the relevant conditions and the proper completion of all procedures and formalities in the Member State concerned.</rdfs:comment>
        <rdfs:label xml:lang="en">Company pre-division certificate</rdfs:label>
        <rdfs:seeAlso rdf:resource="https://www.europarl.europa.eu/doceo/document/TA-8-2019-0429_EN.html"/>
    </owl:Class>
    


    <!-- http://w3id.org/um/cbcm/eu-cm-ontology#PreMergerCertificate -->

    <owl:Class rdf:about="http://w3id.org/um/cbcm/eu-cm-ontology#PreMergerCertificate">
        <rdfs:subClassOf rdf:resource="http://w3id.org/um/cbcm/eu-cm-ontology#TransactionCertificate"/>
        <opla-sd:entityPosition>
            <rdf:Description>
                <opla-sd:entityPositionX rdf:datatype="http://www.w3.org/2001/XMLSchema#double">45.54262094480286</opla-sd:entityPositionX>
                <opla-sd:entityPositionY rdf:datatype="http://www.w3.org/2001/XMLSchema#double">22.868311703824315</opla-sd:entityPositionY>
                <rdfs:comment xml:lang="en">This is an entity positioning annotation generated by CoModIDE (https://comodide.com/). Removing this annotation will break rendering the CoModIDE schema diagram view.</rdfs:comment>
            </rdf:Description>
        </opla-sd:entityPosition>
        <rdfs:comment xml:lang="en">Article 127: a pre-merger certificate attests compliance with all the relevant conditions and the proper completion of all procedures and formalities in the Member State of the merging company.</rdfs:comment>
        <rdfs:label xml:lang="en">Company pre-merger certificate</rdfs:label>
        <rdfs:seeAlso rdf:resource="http://data.europa.eu/eli/dir/2017/1132/oj"/>
    </owl:Class>
    


    <!-- http://w3id.org/um/cbcm/eu-cm-ontology#Procedure -->

    <owl:Class rdf:about="http://w3id.org/um/cbcm/eu-cm-ontology#Procedure">
        <rdfs:subClassOf rdf:resource="http://w3id.org/um/cbcm/eu-cm-ontology#Process"/>
        <opla-sd:entityPosition>
            <rdf:Description>
                <opla-sd:entityPositionX rdf:datatype="http://www.w3.org/2001/XMLSchema#double">69.33559435098756</opla-sd:entityPositionX>
                <opla-sd:entityPositionY rdf:datatype="http://www.w3.org/2001/XMLSchema#double">50.91336898555698</opla-sd:entityPositionY>
                <rdfs:comment xml:lang="en">This is an entity positioning annotation generated by CoModIDE (https://comodide.com/). Removing this annotation will break rendering the CoModIDE schema diagram view.</rdfs:comment>
            </rdf:Description>
        </opla-sd:entityPosition>
        <terms:description xml:lang="en">A procedure is a process that attempts to achieve one or more objectives by following an established set of actions.</terms:description>
        <rdfs:label>Procedure</rdfs:label>
    </owl:Class>
    


    <!-- http://w3id.org/um/cbcm/eu-cm-ontology#Process -->

    <owl:Class rdf:about="http://w3id.org/um/cbcm/eu-cm-ontology#Process">
        <rdfs:subClassOf rdf:resource="http://w3id.org/um/cbcm/eu-cm-ontology#Entity"/>
        <opla-sd:entityPosition>
            <rdf:Description>
                <opla-sd:entityPositionX rdf:datatype="http://www.w3.org/2001/XMLSchema#double">260.3444008641074</opla-sd:entityPositionX>
                <opla-sd:entityPositionY rdf:datatype="http://www.w3.org/2001/XMLSchema#double">17.15921205433361</opla-sd:entityPositionY>
                <rdfs:comment xml:lang="en">This is an entity positioning annotation generated by CoModIDE (https://comodide.com/). Removing this annotation will break rendering the CoModIDE schema diagram view.</rdfs:comment>
            </rdf:Description>
        </opla-sd:entityPosition>
        <terms:description xml:lang="en">A process is an entity that is identifiable only through the unfolding of time, has temporal parts, and unless otherwise specified/predicted, cannot be fully identified at any instant of time in which it exists.</terms:description>
        <rdfs:label>Process</rdfs:label>
    </owl:Class>
    


    <!-- http://w3id.org/um/cbcm/eu-cm-ontology#RecipientCompany -->

    <owl:Class rdf:about="http://w3id.org/um/cbcm/eu-cm-ontology#RecipientCompany">
        <rdfs:subClassOf rdf:resource="http://w3id.org/um/cbcm/eu-cm-ontology#Company"/>
        <rdfs:subClassOf>
            <owl:Restriction>
                <owl:onProperty rdf:resource="http://w3id.org/um/cbcm/eu-cm-ontology#isTransactionResultOf"/>
                <owl:someValuesFrom rdf:resource="http://w3id.org/um/cbcm/eu-cm-ontology#CompanyDivision"/>
            </owl:Restriction>
        </rdfs:subClassOf>
        <opla-sd:entityPosition>
            <rdf:Description>
                <opla-sd:entityPositionX rdf:datatype="http://www.w3.org/2001/XMLSchema#double">234.4838716249161</opla-sd:entityPositionX>
                <opla-sd:entityPositionY rdf:datatype="http://www.w3.org/2001/XMLSchema#double">260.13785809555594</opla-sd:entityPositionY>
                <rdfs:comment xml:lang="en">This is an entity positioning annotation generated by CoModIDE (https://comodide.com/). Removing this annotation will break rendering the CoModIDE schema diagram view.</rdfs:comment>
            </rdf:Description>
        </opla-sd:entityPosition>
        <rdfs:comment xml:lang="en">A company being divided transfers part of its assets and liabilities to one or more newly formed companies, which are the recipient companies in a (cross-border) division.</rdfs:comment>
        <rdfs:label xml:lang="en">Recipient company</rdfs:label>
    </owl:Class>
    


    <!-- http://w3id.org/um/cbcm/eu-cm-ontology#Resolution -->

    <owl:Class rdf:about="http://w3id.org/um/cbcm/eu-cm-ontology#Resolution">
        <rdfs:subClassOf rdf:resource="http://w3id.org/um/cbcm/eu-cm-ontology#TransactionDocument"/>
        <opla-sd:entityPosition>
            <rdf:Description>
                <opla-sd:entityPositionX rdf:datatype="http://www.w3.org/2001/XMLSchema#double">81.75626708582863</opla-sd:entityPositionX>
                <opla-sd:entityPositionY rdf:datatype="http://www.w3.org/2001/XMLSchema#double">128.8863631880492</opla-sd:entityPositionY>
                <rdfs:comment xml:lang="en">This is an entity positioning annotation generated by CoModIDE (https://comodide.com/). Removing this annotation will break rendering the CoModIDE schema diagram view.</rdfs:comment>
            </rdf:Description>
        </opla-sd:entityPosition>
        <rdfs:comment xml:lang="en">A document detailing a decision made by an individual or group of natural or legal persons. This can be a decision concerning the restructuring of a company by its shareholders.</rdfs:comment>
        <rdfs:label xml:lang="en">Resolution</rdfs:label>
    </owl:Class>
    


    <!-- http://w3id.org/um/cbcm/eu-cm-ontology#SEType -->

    <owl:Class rdf:about="http://w3id.org/um/cbcm/eu-cm-ontology#SEType">
        <rdfs:subClassOf rdf:resource="http://w3id.org/um/cbcm/eu-cm-ontology#Attribute"/>
        <rdfs:comment xml:lang="en">Variable indicating the SE-establishment mode: by merger, conversion, holding-SE, subsidiary-SE or unsure (cases)</rdfs:comment>
        <rdfs:label xml:lang="en">Societas Europaea (SE) type</rdfs:label>
    </owl:Class>
    


    <!-- http://w3id.org/um/cbcm/eu-cm-ontology#SeatTransferPlan -->

    <owl:Class rdf:about="http://w3id.org/um/cbcm/eu-cm-ontology#SeatTransferPlan">
        <rdfs:subClassOf rdf:resource="http://w3id.org/um/cbcm/eu-cm-ontology#TransactionDocument"/>
        <opla-sd:entityPosition>
            <rdf:Description>
                <opla-sd:entityPositionX rdf:datatype="http://www.w3.org/2001/XMLSchema#double">95.57191324621544</opla-sd:entityPositionX>
                <opla-sd:entityPositionY rdf:datatype="http://www.w3.org/2001/XMLSchema#double">18.09904131507916</opla-sd:entityPositionY>
                <rdfs:comment xml:lang="en">This is an entity positioning annotation generated by CoModIDE (https://comodide.com/). Removing this annotation will break rendering the CoModIDE schema diagram view.</rdfs:comment>
            </rdf:Description>
        </opla-sd:entityPosition>
        <rdfs:comment xml:lang="en">The management or administrative organ of the company draws up the draft terms of a cross-border seat transfer. The draft terms of a cross-border seat transfer must include at least the particulars specified under national law.</rdfs:comment>
        <rdfs:label xml:lang="en">Company seat transfer plan</rdfs:label>
    </owl:Class>
    


    <!-- http://w3id.org/um/cbcm/eu-cm-ontology#ShareholderExitRight -->

    <owl:Class rdf:about="http://w3id.org/um/cbcm/eu-cm-ontology#ShareholderExitRight">
        <rdfs:subClassOf rdf:resource="http://w3id.org/um/cbcm/eu-cm-ontology#ShareholderRight"/>
        <opla-sd:entityPosition>
            <rdf:Description>
                <opla-sd:entityPositionX rdf:datatype="http://www.w3.org/2001/XMLSchema#double">31.733812683874483</opla-sd:entityPositionX>
                <opla-sd:entityPositionY rdf:datatype="http://www.w3.org/2001/XMLSchema#double">124.25202636218214</opla-sd:entityPositionY>
                <rdfs:comment xml:lang="en">This is an entity positioning annotation generated by CoModIDE (https://comodide.com/). Removing this annotation will break rendering the CoModIDE schema diagram view.</rdfs:comment>
            </rdf:Description>
        </opla-sd:entityPosition>
        <rdfs:comment xml:lang="en">The right of a shareholder to exit the company by being bought out.</rdfs:comment>
        <rdfs:label xml:lang="en">Shareholder exit right</rdfs:label>
        <rdfs:seeAlso rdf:resource="http://data.europa.eu/eli/dir/2017/1132/oj"/>
    </owl:Class>
    


    <!-- http://w3id.org/um/cbcm/eu-cm-ontology#ShareholderInformationRight -->

    <owl:Class rdf:about="http://w3id.org/um/cbcm/eu-cm-ontology#ShareholderInformationRight">
        <rdfs:subClassOf rdf:resource="http://w3id.org/um/cbcm/eu-cm-ontology#ShareholderRight"/>
        <opla-sd:entityPosition>
            <rdf:Description>
                <opla-sd:entityPositionX rdf:datatype="http://www.w3.org/2001/XMLSchema#double">138.3469489059055</opla-sd:entityPositionX>
                <opla-sd:entityPositionY rdf:datatype="http://www.w3.org/2001/XMLSchema#double">99.0876742197817</opla-sd:entityPositionY>
                <rdfs:comment xml:lang="en">This is an entity positioning annotation generated by CoModIDE (https://comodide.com/). Removing this annotation will break rendering the CoModIDE schema diagram view.</rdfs:comment>
            </rdf:Description>
        </opla-sd:entityPosition>
        <rdfs:comment xml:lang="en">It is particularly important that the shareholders of the companies involved in a transaction be kept adequately informed in an objective manner, and that their rights be suitably protected. This includes for instance the availability of documents for inspection by shareholders (e.g. article 97 of Directive 2017/1132).</rdfs:comment>
        <rdfs:label xml:lang="en">Shareholder information right</rdfs:label>
        <rdfs:seeAlso rdf:resource="http://data.europa.eu/eli/dir/2017/1132/oj"/>
    </owl:Class>
    


    <!-- http://w3id.org/um/cbcm/eu-cm-ontology#ShareholderResolution -->

    <owl:Class rdf:about="http://w3id.org/um/cbcm/eu-cm-ontology#ShareholderResolution">
        <rdfs:subClassOf rdf:resource="http://w3id.org/um/cbcm/eu-cm-ontology#Resolution"/>
        <opla-sd:entityPosition>
            <rdf:Description>
                <opla-sd:entityPositionX rdf:datatype="http://www.w3.org/2001/XMLSchema#double">293.41528659106655</opla-sd:entityPositionX>
                <opla-sd:entityPositionY rdf:datatype="http://www.w3.org/2001/XMLSchema#double">32.344300374582026</opla-sd:entityPositionY>
                <rdfs:comment xml:lang="en">This is an entity positioning annotation generated by CoModIDE (https://comodide.com/). Removing this annotation will break rendering the CoModIDE schema diagram view.</rdfs:comment>
            </rdf:Description>
        </opla-sd:entityPosition>
        <rdfs:comment xml:lang="en">a shareholder resolution is a proposal submitted by shareholders for a vote at the company&apos;s shareholder meeting.</rdfs:comment>
        <rdfs:label xml:lang="en">Shareholder resolution</rdfs:label>
    </owl:Class>
    


    <!-- http://w3id.org/um/cbcm/eu-cm-ontology#ShareholderRight -->

    <owl:Class rdf:about="http://w3id.org/um/cbcm/eu-cm-ontology#ShareholderRight">
        <rdfs:subClassOf rdf:resource="http://w3id.org/um/cbcm/eu-cm-ontology#TransactionRight"/>
        <rdfs:subClassOf>
            <owl:Restriction>
                <owl:onProperty rdf:resource="http://w3id.org/um/cbcm/eu-cm-ontology#applicableTo"/>
                <owl:someValuesFrom rdf:resource="http://w3id.org/um/cbcm/eu-cm-ontology#CompanyShareholder"/>
            </owl:Restriction>
        </rdfs:subClassOf>
        <opla-sd:entityPosition>
            <rdf:Description>
                <opla-sd:entityPositionX rdf:datatype="http://www.w3.org/2001/XMLSchema#double">90.9580734272183</opla-sd:entityPositionX>
                <opla-sd:entityPositionY rdf:datatype="http://www.w3.org/2001/XMLSchema#double">177.1083906910626</opla-sd:entityPositionY>
                <rdfs:comment xml:lang="en">This is an entity positioning annotation generated by CoModIDE (https://comodide.com/). Removing this annotation will break rendering the CoModIDE schema diagram view.</rdfs:comment>
            </rdf:Description>
        </opla-sd:entityPosition>
        <rdfs:comment xml:lang="en">The rights of shareholders of a company in the context of a transaction. Often, shreholder resolutions are used to effectuate shareholder rights. Many rights are laid down in the so-called Shareholder Rights Directive.</rdfs:comment>
        <rdfs:label xml:lang="en">Shareholder right</rdfs:label>
        <rdfs:seeAlso rdf:resource="http://data.europa.eu/eli/dir/2017/1132/oj"/>
    </owl:Class>
    


    <!-- http://w3id.org/um/cbcm/eu-cm-ontology#SocialRight -->

    <owl:Class rdf:about="http://w3id.org/um/cbcm/eu-cm-ontology#SocialRight">
        <rdfs:subClassOf rdf:resource="http://w3id.org/um/cbcm/eu-cm-ontology#TransactionRight"/>
        <rdfs:subClassOf>
            <owl:Restriction>
                <owl:onProperty rdf:resource="http://w3id.org/um/cbcm/eu-cm-ontology#applicableTo"/>
                <owl:someValuesFrom rdf:resource="http://w3id.org/um/cbcm/eu-cm-ontology#Employee"/>
            </owl:Restriction>
        </rdfs:subClassOf>
        <opla-sd:entityPosition>
            <rdf:Description>
                <opla-sd:entityPositionX rdf:datatype="http://www.w3.org/2001/XMLSchema#double">176.73319936385965</opla-sd:entityPositionX>
                <opla-sd:entityPositionY rdf:datatype="http://www.w3.org/2001/XMLSchema#double">168.4700518123201</opla-sd:entityPositionY>
                <rdfs:comment xml:lang="en">This is an entity positioning annotation generated by CoModIDE (https://comodide.com/). Removing this annotation will break rendering the CoModIDE schema diagram view.</rdfs:comment>
            </rdf:Description>
        </opla-sd:entityPosition>
        <rdfs:comment xml:lang="en">Social rights, as opposed to rights arising from natural law, are rights for legal entities that entitle them to certain levels of societal living conditions (e.g. the right to housing, to food, to health care etc.)</rdfs:comment>
        <rdfs:label xml:lang="en">Social right</rdfs:label>
    </owl:Class>
    


    <!-- http://w3id.org/um/cbcm/eu-cm-ontology#Society -->

    <owl:Class rdf:about="http://w3id.org/um/cbcm/eu-cm-ontology#Society">
        <rdfs:subClassOf rdf:resource="http://w3id.org/um/cbcm/eu-cm-ontology#CompanyStakeholder"/>
        <opla-sd:entityPosition>
            <rdf:Description>
                <opla-sd:entityPositionX rdf:datatype="http://www.w3.org/2001/XMLSchema#double">169.3838654440731</opla-sd:entityPositionX>
                <opla-sd:entityPositionY rdf:datatype="http://www.w3.org/2001/XMLSchema#double">16.55813918693264</opla-sd:entityPositionY>
                <rdfs:comment xml:lang="en">This is an entity positioning annotation generated by CoModIDE (https://comodide.com/). Removing this annotation will break rendering the CoModIDE schema diagram view.</rdfs:comment>
            </rdf:Description>
        </opla-sd:entityPosition>
        <rdfs:comment xml:lang="en">The society at large is a stakeholder in a company through, inter alia, the government and its agencies, suppliers, customers, trade unions and the communities from which the business draws its resources.</rdfs:comment>
        <rdfs:label xml:lang="en">Society</rdfs:label>
    </owl:Class>
    


    <!-- http://w3id.org/um/cbcm/eu-cm-ontology#SpatialRegion -->

    <owl:Class rdf:about="http://w3id.org/um/cbcm/eu-cm-ontology#SpatialRegion">
        <rdfs:subClassOf rdf:resource="http://w3id.org/um/cbcm/eu-cm-ontology#Entity"/>
        <opla-sd:entityPosition>
            <rdf:Description>
                <opla-sd:entityPositionX rdf:datatype="http://www.w3.org/2001/XMLSchema#double">24.25001224840435</opla-sd:entityPositionX>
                <opla-sd:entityPositionY rdf:datatype="http://www.w3.org/2001/XMLSchema#double">264.57556265040444</opla-sd:entityPositionY>
                <rdfs:comment xml:lang="en">This is an entity positioning annotation generated by CoModIDE (https://comodide.com/). Removing this annotation will break rendering the CoModIDE schema diagram view.</rdfs:comment>
            </rdf:Description>
        </opla-sd:entityPosition>
        <terms:description xml:lang="en">A spatial region is an object contained in some region of space.</terms:description>
        <rdfs:label>Spatial region</rdfs:label>
    </owl:Class>
    


    <!-- http://w3id.org/um/cbcm/eu-cm-ontology#SpecialNegotiationBody -->

    <owl:Class rdf:about="http://w3id.org/um/cbcm/eu-cm-ontology#SpecialNegotiationBody">
        <rdfs:subClassOf rdf:resource="http://w3id.org/um/cbcm/eu-cm-ontology#Organisation"/>
        <opla-sd:entityPosition>
            <rdf:Description>
                <opla-sd:entityPositionX rdf:datatype="http://www.w3.org/2001/XMLSchema#double">272.05118963883785</opla-sd:entityPositionX>
                <opla-sd:entityPositionY rdf:datatype="http://www.w3.org/2001/XMLSchema#double">279.7317598351278</opla-sd:entityPositionY>
                <rdfs:comment xml:lang="en">This is an entity positioning annotation generated by CoModIDE (https://comodide.com/). Removing this annotation will break rendering the CoModIDE schema diagram view.</rdfs:comment>
            </rdf:Description>
        </opla-sd:entityPosition>
        <rdfs:comment xml:lang="en">The Special Negotiation Body (SNB) or Special Negotiating Body is an organisation that represents the employees of companies in negotiations with the company authorities in order to reach a written agreement on the involvement of employees in company transactions.</rdfs:comment>
        <rdfs:label xml:lang="en">Special negotiating body</rdfs:label>
    </owl:Class>
    


    <!-- http://w3id.org/um/cbcm/eu-cm-ontology#SpecialNegotiationBodyAgreement -->

    <owl:Class rdf:about="http://w3id.org/um/cbcm/eu-cm-ontology#SpecialNegotiationBodyAgreement">
        <rdfs:subClassOf rdf:resource="http://w3id.org/um/cbcm/eu-cm-ontology#TransactionDocument"/>
        <opla-sd:entityPosition>
            <rdf:Description>
                <opla-sd:entityPositionX rdf:datatype="http://www.w3.org/2001/XMLSchema#double">127.92838937233955</opla-sd:entityPositionX>
                <opla-sd:entityPositionY rdf:datatype="http://www.w3.org/2001/XMLSchema#double">295.2726163109125</opla-sd:entityPositionY>
                <rdfs:comment xml:lang="en">This is an entity positioning annotation generated by CoModIDE (https://comodide.com/). Removing this annotation will break rendering the CoModIDE schema diagram view.</rdfs:comment>
            </rdf:Description>
        </opla-sd:entityPosition>
        <rdfs:comment xml:lang="en">A written agreement concerning the involvement of employees in company transactions. Special Negotiating Body (SNB) organisation represents employees in the negotiation of the terms of this agreement with the company authorities. The agreement must be reached in accordance with the EU Company Law Directive and is laid down in the SNB-agreement.</rdfs:comment>
        <rdfs:label xml:lang="en">Special negotiating body agreement</rdfs:label>
        <rdfs:seeAlso rdf:resource="http://data.europa.eu/eli/dir/2017/1132/oj"/>
        <rdfs:seeAlso rdf:resource="http://w3id.org/um/cbcm/eu-cm-ontology#SpecialNegotiationBody"/>
    </owl:Class>
    


    <!-- http://w3id.org/um/cbcm/eu-cm-ontology#SubsidiaryCompany -->

    <owl:Class rdf:about="http://w3id.org/um/cbcm/eu-cm-ontology#SubsidiaryCompany">
        <owl:equivalentClass>
            <owl:Class>
                <owl:intersectionOf rdf:parseType="Collection">
                    <rdf:Description rdf:about="http://w3id.org/um/cbcm/eu-cm-ontology#Company"/>
                    <owl:Restriction>
                        <owl:onProperty rdf:resource="http://w3id.org/um/cbcm/eu-cm-ontology#hasParentCompany"/>
                        <owl:someValuesFrom rdf:resource="http://w3id.org/um/cbcm/eu-cm-ontology#Company"/>
                    </owl:Restriction>
                </owl:intersectionOf>
            </owl:Class>
        </owl:equivalentClass>
        <opla-sd:entityPosition>
            <rdf:Description>
                <opla-sd:entityPositionX rdf:datatype="http://www.w3.org/2001/XMLSchema#double">101.5931884899861</opla-sd:entityPositionX>
                <opla-sd:entityPositionY rdf:datatype="http://www.w3.org/2001/XMLSchema#double">186.71127758816417</opla-sd:entityPositionY>
                <rdfs:comment xml:lang="en">This is an entity positioning annotation generated by CoModIDE (https://comodide.com/). Removing this annotation will break rendering the CoModIDE schema diagram view.</rdfs:comment>
            </rdf:Description>
        </opla-sd:entityPosition>
        <rdfs:comment xml:lang="en">A subsidiary, subsidiary company or daughter company is a company that is owned or controlled by another company, which is called the parent company, parent, or holding company.</rdfs:comment>
        <rdfs:label xml:lang="en">Subsidiary company</rdfs:label>
    </owl:Class>
    


    <!-- http://w3id.org/um/cbcm/eu-cm-ontology#SupervisoryAuthority -->

    <owl:Class rdf:about="http://w3id.org/um/cbcm/eu-cm-ontology#SupervisoryAuthority">
        <rdfs:subClassOf rdf:resource="http://w3id.org/um/cbcm/eu-cm-ontology#Organisation"/>
        <opla-sd:entityPosition>
            <rdf:Description>
                <opla-sd:entityPositionX rdf:datatype="http://www.w3.org/2001/XMLSchema#double">245.79476251487904</opla-sd:entityPositionX>
                <opla-sd:entityPositionY rdf:datatype="http://www.w3.org/2001/XMLSchema#double">275.1033741128023</opla-sd:entityPositionY>
                <rdfs:comment xml:lang="en">This is an entity positioning annotation generated by CoModIDE (https://comodide.com/). Removing this annotation will break rendering the CoModIDE schema diagram view.</rdfs:comment>
            </rdf:Description>
        </opla-sd:entityPosition>
        <rdfs:comment xml:lang="en">An individual authority established by its member state to supervise the compliance with a specific regulation.</rdfs:comment>
        <rdfs:label xml:lang="en">SupervisoryAuthority</rdfs:label>
    </owl:Class>
    


    <!-- http://w3id.org/um/cbcm/eu-cm-ontology#SupervisoryBoard -->

    <owl:Class rdf:about="http://w3id.org/um/cbcm/eu-cm-ontology#SupervisoryBoard">
        <rdfs:subClassOf rdf:resource="http://w3id.org/um/cbcm/eu-cm-ontology#Manager"/>
        <rdfs:subClassOf>
            <owl:Restriction>
                <owl:onProperty rdf:resource="http://w3id.org/um/cbcm/eu-cm-ontology#partOf"/>
                <owl:someValuesFrom rdf:resource="http://w3id.org/um/cbcm/eu-cm-ontology#Company"/>
            </owl:Restriction>
        </rdfs:subClassOf>
        <opla-sd:entityPosition>
            <rdf:Description>
                <opla-sd:entityPositionX rdf:datatype="http://www.w3.org/2001/XMLSchema#double">164.92255628203452</opla-sd:entityPositionX>
                <opla-sd:entityPositionY rdf:datatype="http://www.w3.org/2001/XMLSchema#double">195.7746040140031</opla-sd:entityPositionY>
                <rdfs:comment xml:lang="en">This is an entity positioning annotation generated by CoModIDE (https://comodide.com/). Removing this annotation will break rendering the CoModIDE schema diagram view.</rdfs:comment>
            </rdf:Description>
        </opla-sd:entityPosition>
        <rdfs:comment xml:lang="en">A supervisory board must approve of major business decisions. It is a group of individuals chosen by the shareholders - and employee representatives in board-level employee representation systems - of a company to promote their interests through the governance of the company and to hire and supervise the management board. It is also called non-executive board in a one-tier board system.</rdfs:comment>
        <rdfs:label xml:lang="en">Supervisory board</rdfs:label>
    </owl:Class>
    


    <!-- http://w3id.org/um/cbcm/eu-cm-ontology#TaxAuthority -->

    <owl:Class rdf:about="http://w3id.org/um/cbcm/eu-cm-ontology#TaxAuthority">
        <rdfs:subClassOf rdf:resource="http://w3id.org/um/cbcm/eu-cm-ontology#CompetentAuthority"/>
        <opla-sd:entityPosition>
            <rdf:Description>
                <opla-sd:entityPositionX rdf:datatype="http://www.w3.org/2001/XMLSchema#double">80.17428163453475</opla-sd:entityPositionX>
                <opla-sd:entityPositionY rdf:datatype="http://www.w3.org/2001/XMLSchema#double">275.24668244143015</opla-sd:entityPositionY>
                <rdfs:comment xml:lang="en">This is an entity positioning annotation generated by CoModIDE (https://comodide.com/). Removing this annotation will break rendering the CoModIDE schema diagram view.</rdfs:comment>
            </rdf:Description>
        </opla-sd:entityPosition>
        <rdfs:comment xml:lang="en">Tax Authority means any governmental authority having jurisdiction over the assessment, determination, collection or imposition of any tax.</rdfs:comment>
        <rdfs:label xml:lang="en">Tax authority</rdfs:label>
    </owl:Class>
    


    <!-- http://w3id.org/um/cbcm/eu-cm-ontology#TransactionCertificate -->

    <owl:Class rdf:about="http://w3id.org/um/cbcm/eu-cm-ontology#TransactionCertificate">
        <rdfs:subClassOf rdf:resource="http://w3id.org/um/cbcm/eu-cm-ontology#TransactionDocument"/>
        <opla-sd:entityPosition>
            <rdf:Description>
                <opla-sd:entityPositionX rdf:datatype="http://www.w3.org/2001/XMLSchema#double">266.18798107220033</opla-sd:entityPositionX>
                <opla-sd:entityPositionY rdf:datatype="http://www.w3.org/2001/XMLSchema#double">177.08003492861513</opla-sd:entityPositionY>
                <rdfs:comment xml:lang="en">This is an entity positioning annotation generated by CoModIDE (https://comodide.com/). Removing this annotation will break rendering the CoModIDE schema diagram view.</rdfs:comment>
            </rdf:Description>
        </opla-sd:entityPosition>
        <rdfs:comment xml:lang="en">A document issued by a Competent Authority declaring that certain steps of the transaction are completed.</rdfs:comment>
        <rdfs:label xml:lang="en">Company transaction certificate</rdfs:label>
    </owl:Class>
    


    <!-- http://w3id.org/um/cbcm/eu-cm-ontology#TransactionDocument -->

    <owl:Class rdf:about="http://w3id.org/um/cbcm/eu-cm-ontology#TransactionDocument">
        <rdfs:subClassOf rdf:resource="http://w3id.org/um/cbcm/eu-cm-ontology#CompanyMobilityDocument"/>
        <opla-sd:entityPosition>
            <rdf:Description>
                <opla-sd:entityPositionX rdf:datatype="http://www.w3.org/2001/XMLSchema#double">270.8596897409068</opla-sd:entityPositionX>
                <opla-sd:entityPositionY rdf:datatype="http://www.w3.org/2001/XMLSchema#double">157.43078465846642</opla-sd:entityPositionY>
                <rdfs:comment xml:lang="en">This is an entity positioning annotation generated by CoModIDE (https://comodide.com/). Removing this annotation will break rendering the CoModIDE schema diagram view.</rdfs:comment>
            </rdf:Description>
        </opla-sd:entityPosition>
        <rdfs:comment xml:lang="en">Document required by law to document the step of a company transaction or an agreement made between stakeholders involved in the transaction that are either printed, inserted and mailed, or electronically presented.</rdfs:comment>
        <rdfs:label xml:lang="en">Transaction document</rdfs:label>
    </owl:Class>
    


    <!-- http://w3id.org/um/cbcm/eu-cm-ontology#TransactionNotice -->

    <owl:Class rdf:about="http://w3id.org/um/cbcm/eu-cm-ontology#TransactionNotice">
        <rdfs:subClassOf rdf:resource="http://w3id.org/um/cbcm/eu-cm-ontology#TransactionDocument"/>
        <rdfs:subClassOf>
            <owl:Restriction>
                <owl:onProperty rdf:resource="http://w3id.org/um/cbcm/eu-cm-ontology#containedIn"/>
                <owl:someValuesFrom rdf:resource="http://w3id.org/um/cbcm/eu-cm-ontology#OfficialJournalRepository"/>
            </owl:Restriction>
        </rdfs:subClassOf>
        <opla-sd:entityPosition>
            <rdf:Description>
                <opla-sd:entityPositionX rdf:datatype="http://www.w3.org/2001/XMLSchema#double">297.4816662483587</opla-sd:entityPositionX>
                <opla-sd:entityPositionY rdf:datatype="http://www.w3.org/2001/XMLSchema#double">103.23498423096065</opla-sd:entityPositionY>
                <rdfs:comment xml:lang="en">This is an entity positioning annotation generated by CoModIDE (https://comodide.com/). Removing this annotation will break rendering the CoModIDE schema diagram view.</rdfs:comment>
            </rdf:Description>
        </opla-sd:entityPosition>
        <rdfs:comment xml:lang="en">A written notice, published in an official journal of a Member State of the EU and/or the European Official Journal indicating the intention to engage in a transaction and which informs  the members, creditors and representatives of the employees of the company, or, where there are no such representatives, the employees themselves of said transaction.</rdfs:comment>
        <rdfs:label xml:lang="en">Company transaction notice</rdfs:label>
    </owl:Class>
    


    <!-- http://w3id.org/um/cbcm/eu-cm-ontology#TransactionRight -->

    <owl:Class rdf:about="http://w3id.org/um/cbcm/eu-cm-ontology#TransactionRight">
        <rdfs:subClassOf rdf:resource="http://w3id.org/um/cbcm/eu-cm-ontology#Object"/>
        <opla-sd:entityPosition>
            <rdf:Description>
                <opla-sd:entityPositionX rdf:datatype="http://www.w3.org/2001/XMLSchema#double">141.60152732818455</opla-sd:entityPositionX>
                <opla-sd:entityPositionY rdf:datatype="http://www.w3.org/2001/XMLSchema#double">232.75293984177262</opla-sd:entityPositionY>
                <rdfs:comment xml:lang="en">This is an entity positioning annotation generated by CoModIDE (https://comodide.com/). Removing this annotation will break rendering the CoModIDE schema diagram view.</rdfs:comment>
            </rdf:Description>
        </opla-sd:entityPosition>
        <rdfs:comment xml:lang="en">A legal right of a legal entity involved in the process of a company transaction. A legal right here refers to the entitlement of a person to be allowed to perform an activity, or to possess or obtain access to an object.</rdfs:comment>
        <rdfs:label xml:lang="en">Transaction right</rdfs:label>
    </owl:Class>
    


    <!-- http://w3id.org/um/cbcm/eu-cm-ontology#TransferOfCentralAdministration -->

    <owl:Class rdf:about="http://w3id.org/um/cbcm/eu-cm-ontology#TransferOfCentralAdministration">
        <rdfs:subClassOf rdf:resource="http://w3id.org/um/cbcm/eu-cm-ontology#Procedure"/>
        <opla-sd:entityPosition>
            <rdf:Description>
                <opla-sd:entityPositionX rdf:datatype="http://www.w3.org/2001/XMLSchema#double">100.68738477341026</opla-sd:entityPositionX>
                <opla-sd:entityPositionY rdf:datatype="http://www.w3.org/2001/XMLSchema#double">213.01461505654413</opla-sd:entityPositionY>
                <rdfs:comment xml:lang="en">This is an entity positioning annotation generated by CoModIDE (https://comodide.com/). Removing this annotation will break rendering the CoModIDE schema diagram view.</rdfs:comment>
            </rdf:Description>
        </opla-sd:entityPosition>
        <rdfs:comment xml:lang="en">Act of modifying the location where the company’s business was managed or the place where that company’s business was actually conducted.</rdfs:comment>
        <rdfs:label xml:lang="en">Transfer of company central administration</rdfs:label>
    </owl:Class>
    


    <!-- http://w3id.org/um/cbcm/eu-cm-ontology#TransferOfRegisteredOffice -->

    <owl:Class rdf:about="http://w3id.org/um/cbcm/eu-cm-ontology#TransferOfRegisteredOffice">
        <rdfs:subClassOf rdf:resource="http://w3id.org/um/cbcm/eu-cm-ontology#Procedure"/>
        <opla-sd:entityPosition>
            <rdf:Description>
                <opla-sd:entityPositionX rdf:datatype="http://www.w3.org/2001/XMLSchema#double">28.54350686833721</opla-sd:entityPositionX>
                <opla-sd:entityPositionY rdf:datatype="http://www.w3.org/2001/XMLSchema#double">279.13445695705747</opla-sd:entityPositionY>
                <rdfs:comment xml:lang="en">This is an entity positioning annotation generated by CoModIDE (https://comodide.com/). Removing this annotation will break rendering the CoModIDE schema diagram view.</rdfs:comment>
            </rdf:Description>
        </opla-sd:entityPosition>
        <rdfs:comment xml:lang="en">The act of changing the registered office, which is the official address of an incorporated company, association or any other legal entity.</rdfs:comment>
        <rdfs:label xml:lang="en">Transfer of company registered office</rdfs:label>
    </owl:Class>
    


    <!-- http://w3id.org/um/cbcm/eu-cm-ontology#TransferringCompany -->

    <owl:Class rdf:about="http://w3id.org/um/cbcm/eu-cm-ontology#TransferringCompany">
        <rdfs:subClassOf rdf:resource="http://w3id.org/um/cbcm/eu-cm-ontology#Company"/>
        <opla-sd:entityPosition>
            <rdf:Description>
                <opla-sd:entityPositionX rdf:datatype="http://www.w3.org/2001/XMLSchema#double">34.232942432039486</opla-sd:entityPositionX>
                <opla-sd:entityPositionY rdf:datatype="http://www.w3.org/2001/XMLSchema#double">43.59706388390724</opla-sd:entityPositionY>
                <rdfs:comment xml:lang="en">This is an entity positioning annotation generated by CoModIDE (https://comodide.com/). Removing this annotation will break rendering the CoModIDE schema diagram view.</rdfs:comment>
            </rdf:Description>
        </opla-sd:entityPosition>
        <rdfs:comment xml:lang="en">Transferring Company means the company transferring its assets and liabilities to a recipient company.</rdfs:comment>
        <rdfs:label xml:lang="en">Transferring company</rdfs:label>
    </owl:Class>
    


    <!-- http://w3id.org/um/cbcm/eu-cm-ontology#UltimateBeneficialOwner -->

    <owl:Class rdf:about="http://w3id.org/um/cbcm/eu-cm-ontology#UltimateBeneficialOwner">
        <rdfs:subClassOf rdf:resource="http://w3id.org/um/cbcm/eu-cm-ontology#CompanyShareholder"/>
        <rdfs:subClassOf rdf:resource="http://w3id.org/um/cbcm/eu-cm-ontology#Person"/>
        <rdfs:subClassOf>
            <owl:Restriction>
                <owl:onProperty rdf:resource="http://w3id.org/um/cbcm/eu-cm-ontology#owns"/>
                <owl:someValuesFrom>
                    <owl:Class>
                        <owl:intersectionOf rdf:parseType="Collection">
                            <rdf:Description rdf:about="http://w3id.org/um/cbcm/eu-cm-ontology#Company"/>
                            <owl:Class>
                                <owl:complementOf>
                                    <owl:Restriction>
                                        <owl:onProperty rdf:resource="http://w3id.org/um/cbcm/eu-cm-ontology#hasParentCompany"/>
                                        <owl:someValuesFrom rdf:resource="http://www.w3.org/2002/07/owl#Thing"/>
                                    </owl:Restriction>
                                </owl:complementOf>
                            </owl:Class>
                        </owl:intersectionOf>
                    </owl:Class>
                </owl:someValuesFrom>
            </owl:Restriction>
        </rdfs:subClassOf>
        <opla-sd:entityPosition>
            <rdf:Description>
                <opla-sd:entityPositionX rdf:datatype="http://www.w3.org/2001/XMLSchema#double">210.0879626302195</opla-sd:entityPositionX>
                <opla-sd:entityPositionY rdf:datatype="http://www.w3.org/2001/XMLSchema#double">24.487612524612793</opla-sd:entityPositionY>
                <rdfs:comment xml:lang="en">This is an entity positioning annotation generated by CoModIDE (https://comodide.com/). Removing this annotation will break rendering the CoModIDE schema diagram view.</rdfs:comment>
            </rdf:Description>
        </opla-sd:entityPosition>
        <rdfs:comment xml:lang="en">Ultimate Beneficial owner refers to the natural person(s) who ultimately owns or controls a customer and/or the natural person on whose behalf a transaction is being conducted. It also includes those persons who exercise ultimate effective control over a legal person or arrangement.</rdfs:comment>
        <rdfs:label xml:lang="en">Ultimate beneficial owner</rdfs:label>
    </owl:Class>
    


    <!-- http://w3id.org/um/cbcm/eu-cm-ontology#WorksCouncil -->

    <owl:Class rdf:about="http://w3id.org/um/cbcm/eu-cm-ontology#WorksCouncil">
        <rdfs:subClassOf rdf:resource="http://w3id.org/um/cbcm/eu-cm-ontology#CompanyStakeholder"/>
        <rdfs:subClassOf rdf:resource="http://w3id.org/um/cbcm/eu-cm-ontology#Organisation"/>
        <rdfs:subClassOf rdf:resource="http://w3id.org/um/cbcm/eu-cm-ontology#OrganisationalUnit"/>
        <rdfs:subClassOf>
            <owl:Restriction>
                <owl:onProperty rdf:resource="http://w3id.org/um/cbcm/eu-cm-ontology#hasMember"/>
                <owl:someValuesFrom rdf:resource="http://w3id.org/um/cbcm/eu-cm-ontology#Employee"/>
            </owl:Restriction>
        </rdfs:subClassOf>
        <rdfs:subClassOf>
            <owl:Restriction>
                <owl:onProperty rdf:resource="http://w3id.org/um/cbcm/eu-cm-ontology#partOf"/>
                <owl:someValuesFrom rdf:resource="http://w3id.org/um/cbcm/eu-cm-ontology#Company"/>
            </owl:Restriction>
        </rdfs:subClassOf>
        <opla-sd:entityPosition>
            <rdf:Description>
                <opla-sd:entityPositionX rdf:datatype="http://www.w3.org/2001/XMLSchema#double">65.42451098340007</opla-sd:entityPositionX>
                <opla-sd:entityPositionY rdf:datatype="http://www.w3.org/2001/XMLSchema#double">177.53694512511427</opla-sd:entityPositionY>
                <rdfs:comment xml:lang="en">This is an entity positioning annotation generated by CoModIDE (https://comodide.com/). Removing this annotation will break rendering the CoModIDE schema diagram view.</rdfs:comment>
            </rdf:Description>
        </opla-sd:entityPosition>
        <rdfs:comment xml:lang="en">The exercise of employee participation through the representation of employees vis-a-vis the management of a company. The works council is a shop-floor level representation mechanism with information, consultation and veto-rights - depending on the extent of rights given in a Member State - and also at EU level through European Works Councils.</rdfs:comment>
        <rdfs:label xml:lang="en">Employee works council</rdfs:label>
        <rdfs:seeAlso rdf:resource="http://data.europa.eu/eli/dir/2002/14/oj"/>
        <rdfs:seeAlso rdf:resource="https://www.worker-participation.eu/National-Industrial-Relations/Across-Europe"/>
    </owl:Class>
    


    <!-- 
    ///////////////////////////////////////////////////////////////////////////////////////
    //
    // Individuals
    //
    ///////////////////////////////////////////////////////////////////////////////////////
     -->


    <!-- http://w3id.org/um/cbcm/eu-cm-ontology#at102 -->

    <owl:NamedIndividual rdf:about="http://w3id.org/um/cbcm/eu-cm-ontology#at102">
        <rdf:type rdf:resource="http://w3id.org/um/cbcm/eu-cm-ontology#CompanyLegalForm"/>
        <dc:title xml:lang="en">General partnership</dc:title>
        <dc:title xml:lang="at">Offene Gesellschaft</dc:title>
        <rdfs:label rdf:datatype="http://www.w3.org/2001/XMLSchema#string">OG</rdfs:label>
    </owl:NamedIndividual>
    


    <!-- http://w3id.org/um/cbcm/eu-cm-ontology#at103 -->

    <owl:NamedIndividual rdf:about="http://w3id.org/um/cbcm/eu-cm-ontology#at103">
        <rdf:type rdf:resource="http://w3id.org/um/cbcm/eu-cm-ontology#CompanyLegalForm"/>
        <dc:title xml:lang="at">Kommanditgesellschaft</dc:title>
        <dc:title xml:lang="en">Limited partnership</dc:title>
        <rdfs:label rdf:datatype="http://www.w3.org/2001/XMLSchema#string">KG</rdfs:label>
    </owl:NamedIndividual>
    


    <!-- http://w3id.org/um/cbcm/eu-cm-ontology#at201 -->

    <owl:NamedIndividual rdf:about="http://w3id.org/um/cbcm/eu-cm-ontology#at201">
        <rdf:type rdf:resource="http://w3id.org/um/cbcm/eu-cm-ontology#CompanyLegalForm"/>
        <dc:title xml:lang="at">Aktiengesellschaft</dc:title>
        <dc:title xml:lang="en">Plc (UK)</dc:title>
        <rdfs:label rdf:datatype="http://www.w3.org/2001/XMLSchema#string">AG</rdfs:label>
    </owl:NamedIndividual>
    


    <!-- http://w3id.org/um/cbcm/eu-cm-ontology#at202 -->

    <owl:NamedIndividual rdf:about="http://w3id.org/um/cbcm/eu-cm-ontology#at202">
        <rdf:type rdf:resource="http://w3id.org/um/cbcm/eu-cm-ontology#CompanyLegalForm"/>
        <dc:title xml:lang="at">Gesellschaft mit beschränkter Haftung</dc:title>
        <dc:title xml:lang="en">Ltd (UK)</dc:title>
        <rdfs:label rdf:datatype="http://www.w3.org/2001/XMLSchema#string">GmbH</rdfs:label>
    </owl:NamedIndividual>
    


    <!-- http://w3id.org/um/cbcm/eu-cm-ontology#at401 -->

    <owl:NamedIndividual rdf:about="http://w3id.org/um/cbcm/eu-cm-ontology#at401">
        <rdf:type rdf:resource="http://w3id.org/um/cbcm/eu-cm-ontology#CompanyLegalForm"/>
        <dc:title xml:lang="en">Cooperative</dc:title>
        <dc:title xml:lang="at">Erwerbs- und Wirtschaftsgenossenschaft</dc:title>
        <rdfs:label rdf:datatype="http://www.w3.org/2001/XMLSchema#string">GEN</rdfs:label>
    </owl:NamedIndividual>
    


    <!-- http://w3id.org/um/cbcm/eu-cm-ontology#at501 -->

    <owl:NamedIndividual rdf:about="http://w3id.org/um/cbcm/eu-cm-ontology#at501">
        <rdf:type rdf:resource="http://w3id.org/um/cbcm/eu-cm-ontology#CompanyLegalForm"/>
        <dc:title xml:lang="en">Mutual Insurance Corporation </dc:title>
        <dc:title xml:lang="at">Versicherungsverein auf Gegenseitigkeit</dc:title>
        <rdfs:label rdf:datatype="http://www.w3.org/2001/XMLSchema#string">V</rdfs:label>
    </owl:NamedIndividual>
    


    <!-- http://w3id.org/um/cbcm/eu-cm-ontology#at603 -->

    <owl:NamedIndividual rdf:about="http://w3id.org/um/cbcm/eu-cm-ontology#at603">
        <rdf:type rdf:resource="http://w3id.org/um/cbcm/eu-cm-ontology#CompanyLegalForm"/>
        <dc:title xml:lang="en">Private foundation</dc:title>
        <dc:title xml:lang="at">Privatstiftung </dc:title>
        <rdfs:label rdf:datatype="http://www.w3.org/2001/XMLSchema#string">P</rdfs:label>
    </owl:NamedIndividual>
    


    <!-- http://w3id.org/um/cbcm/eu-cm-ontology#at604 -->

    <owl:NamedIndividual rdf:about="http://w3id.org/um/cbcm/eu-cm-ontology#at604">
        <rdf:type rdf:resource="http://w3id.org/um/cbcm/eu-cm-ontology#CompanyLegalForm"/>
        <dc:title xml:lang="en">Mutual Savings Bank</dc:title>
        <dc:title xml:lang="at">Sparkasse</dc:title>
        <rdfs:label rdf:datatype="http://www.w3.org/2001/XMLSchema#string">S</rdfs:label>
    </owl:NamedIndividual>
    


    <!-- http://w3id.org/um/cbcm/eu-cm-ontology#at605 -->

    <owl:NamedIndividual rdf:about="http://w3id.org/um/cbcm/eu-cm-ontology#at605">
        <rdf:type rdf:resource="http://w3id.org/um/cbcm/eu-cm-ontology#CompanyLegalForm"/>
        <dc:title xml:lang="en">Other Legal Entity</dc:title>
        <dc:title xml:lang="at">Sonstiger Rechtsträger</dc:title>
        <rdfs:label rdf:datatype="http://www.w3.org/2001/XMLSchema#string">SR</rdfs:label>
    </owl:NamedIndividual>
    


    <!-- http://w3id.org/um/cbcm/eu-cm-ontology#at610 -->

    <owl:NamedIndividual rdf:about="http://w3id.org/um/cbcm/eu-cm-ontology#at610">
        <rdf:type rdf:resource="http://w3id.org/um/cbcm/eu-cm-ontology#CompanyLegalForm"/>
        <dc:title xml:lang="en"> corporation of public law</dc:title>
        <dc:title xml:lang="en">public corporation</dc:title>
        <dc:title xml:lang="at">Öffentlich rechtliche Körperschaften</dc:title>
        <rdfs:label rdf:datatype="http://www.w3.org/2001/XMLSchema#string">ÖrK</rdfs:label>
    </owl:NamedIndividual>
    


    <!-- http://w3id.org/um/cbcm/eu-cm-ontology#at611 -->

    <owl:NamedIndividual rdf:about="http://w3id.org/um/cbcm/eu-cm-ontology#at611">
        <rdf:type rdf:resource="http://w3id.org/um/cbcm/eu-cm-ontology#CompanyLegalForm"/>
        <dc:title xml:lang="en"> corporation of public law</dc:title>
        <dc:title xml:lang="en">public trust</dc:title>
        <dc:title xml:lang="at">Öffentlich rechtliche Stiftungen</dc:title>
        <rdfs:label rdf:datatype="http://www.w3.org/2001/XMLSchema#string">ÖrS</rdfs:label>
    </owl:NamedIndividual>
    


    <!-- http://w3id.org/um/cbcm/eu-cm-ontology#at612 -->

    <owl:NamedIndividual rdf:about="http://w3id.org/um/cbcm/eu-cm-ontology#at612">
        <rdf:type rdf:resource="http://w3id.org/um/cbcm/eu-cm-ontology#CompanyLegalForm"/>
        <dc:title xml:lang="en"> corporation of public law</dc:title>
        <dc:title xml:lang="at">Vereine</dc:title>
        <dc:title xml:lang="en">registered association</dc:title>
        <rdfs:label rdf:datatype="http://www.w3.org/2001/XMLSchema#string">VER</rdfs:label>
    </owl:NamedIndividual>
    


    <!-- http://w3id.org/um/cbcm/eu-cm-ontology#at613 -->

    <owl:NamedIndividual rdf:about="http://w3id.org/um/cbcm/eu-cm-ontology#at613">
        <rdf:type rdf:resource="http://w3id.org/um/cbcm/eu-cm-ontology#CompanyLegalForm"/>
        <dc:title xml:lang="at">Eigentümergemeinschaft</dc:title>
        <dc:title xml:lang="en">owner association</dc:title>
        <rdfs:label rdf:datatype="http://www.w3.org/2001/XMLSchema#string">EG</rdfs:label>
    </owl:NamedIndividual>
    


    <!-- http://w3id.org/um/cbcm/eu-cm-ontology#austria -->

    <owl:NamedIndividual rdf:about="http://w3id.org/um/cbcm/eu-cm-ontology#austria">
        <rdf:type rdf:resource="http://w3id.org/um/cbcm/eu-cm-ontology#EUCountry"/>
        <cbcm:countryHasCompanyForm rdf:resource="http://w3id.org/um/cbcm/eu-cm-ontology#at102"/>
        <cbcm:countryHasCompanyForm rdf:resource="http://w3id.org/um/cbcm/eu-cm-ontology#at103"/>
        <cbcm:countryHasCompanyForm rdf:resource="http://w3id.org/um/cbcm/eu-cm-ontology#at201"/>
        <cbcm:countryHasCompanyForm rdf:resource="http://w3id.org/um/cbcm/eu-cm-ontology#at202"/>
        <cbcm:countryHasCompanyForm rdf:resource="http://w3id.org/um/cbcm/eu-cm-ontology#at401"/>
        <cbcm:countryHasCompanyForm rdf:resource="http://w3id.org/um/cbcm/eu-cm-ontology#at501"/>
        <cbcm:countryHasCompanyForm rdf:resource="http://w3id.org/um/cbcm/eu-cm-ontology#at603"/>
        <cbcm:countryHasCompanyForm rdf:resource="http://w3id.org/um/cbcm/eu-cm-ontology#at604"/>
        <cbcm:countryHasCompanyForm rdf:resource="http://w3id.org/um/cbcm/eu-cm-ontology#at605"/>
        <cbcm:countryHasCompanyForm rdf:resource="http://w3id.org/um/cbcm/eu-cm-ontology#at610"/>
        <cbcm:countryHasCompanyForm rdf:resource="http://w3id.org/um/cbcm/eu-cm-ontology#at611"/>
        <cbcm:countryHasCompanyForm rdf:resource="http://w3id.org/um/cbcm/eu-cm-ontology#at612"/>
        <cbcm:countryHasCompanyForm rdf:resource="http://w3id.org/um/cbcm/eu-cm-ontology#at613"/>
        <cbcm:iso2code>AT</cbcm:iso2code>
        <rdfs:label xml:lang="en">Austria</rdfs:label>
        <rdfs:label xml:lang="de">Österreich</rdfs:label>
    </owl:NamedIndividual>
    


    <!-- http://w3id.org/um/cbcm/eu-cm-ontology#be000 -->

    <owl:NamedIndividual rdf:about="http://w3id.org/um/cbcm/eu-cm-ontology#be000">
        <rdf:type rdf:resource="http://w3id.org/um/cbcm/eu-cm-ontology#CompanyLegalForm"/>
        <dc:title xml:lang="be">  Alte Rechtsformen (nicht mehr anwendbar)</dc:title>
        <dc:title xml:lang="be">  Oude rechtsvormen (niet langer van toepassing) </dc:title>
        <dc:title xml:lang="be">Anciennes formes juridiques (plus applicable) </dc:title>
        <dc:title xml:lang="en">Old or dismissed legal forms (no longer applicable)</dc:title>
        <rdfs:label rdf:datatype="http://www.w3.org/2001/XMLSchema#string">Inactief</rdfs:label>
        <rdfs:label rdf:datatype="http://www.w3.org/2001/XMLSchema#string">Nichtaktiv</rdfs:label>
        <rdfs:label rdf:datatype="http://www.w3.org/2001/XMLSchema#string">Nonactif</rdfs:label>
    </owl:NamedIndividual>
    


    <!-- http://w3id.org/um/cbcm/eu-cm-ontology#be002 -->

    <owl:NamedIndividual rdf:about="http://w3id.org/um/cbcm/eu-cm-ontology#be002">
        <rdf:type rdf:resource="http://w3id.org/um/cbcm/eu-cm-ontology#CompanyLegalForm"/>
        <dc:title xml:lang="be">  Organisme voor de Financiering van Pensioenen </dc:title>
        <dc:title xml:lang="be">  Organismus für die Finanzierung von Pensionen</dc:title>
        <dc:title xml:lang="en">Organisation for financing pensions</dc:title>
        <dc:title xml:lang="be">Organisme de financement de pensions </dc:title>
        <rdfs:label rdf:datatype="http://www.w3.org/2001/XMLSchema#string">OFP</rdfs:label>
    </owl:NamedIndividual>
    


    <!-- http://w3id.org/um/cbcm/eu-cm-ontology#be003 -->

    <owl:NamedIndividual rdf:about="http://w3id.org/um/cbcm/eu-cm-ontology#be003">
        <rdf:type rdf:resource="http://w3id.org/um/cbcm/eu-cm-ontology#CompanyLegalForm"/>
        <dc:title xml:lang="be">  BTW-eenheid </dc:title>
        <dc:title xml:lang="be">  Mehrwertsteuereinheit</dc:title>
        <dc:title xml:lang="be">Unité TVA </dc:title>
        <dc:title xml:lang="en">VAT Group</dc:title>
        <rdfs:label rdf:datatype="http://www.w3.org/2001/XMLSchema#string">BTWE</rdfs:label>
        <rdfs:label rdf:datatype="http://www.w3.org/2001/XMLSchema#string">MWSE</rdfs:label>
        <rdfs:label rdf:datatype="http://www.w3.org/2001/XMLSchema#string">UTVA</rdfs:label>
    </owl:NamedIndividual>
    


    <!-- http://w3id.org/um/cbcm/eu-cm-ontology#be006 -->

    <owl:NamedIndividual rdf:about="http://w3id.org/um/cbcm/eu-cm-ontology#be006">
        <rdf:type rdf:resource="http://w3id.org/um/cbcm/eu-cm-ontology#CompanyLegalForm"/>
        <dc:title xml:lang="be">  Coöperatieve vennootschap met onbeperkte aansprakelijkheid </dc:title>
        <dc:title xml:lang="be">  Genossenschaft mit unbeschränkter Haftung</dc:title>
        <dc:title xml:lang="en">Cooperative partnership with unlimited liability</dc:title>
        <dc:title xml:lang="be">Société coopérative à responsabilité illimitée </dc:title>
        <rdfs:label rdf:datatype="http://www.w3.org/2001/XMLSchema#string">CVOA</rdfs:label>
        <rdfs:label rdf:datatype="http://www.w3.org/2001/XMLSchema#string">Gen.mubH</rdfs:label>
        <rdfs:label rdf:datatype="http://www.w3.org/2001/XMLSchema#string">SCRI</rdfs:label>
    </owl:NamedIndividual>
    


    <!-- http://w3id.org/um/cbcm/eu-cm-ontology#be008 -->

    <owl:NamedIndividual rdf:about="http://w3id.org/um/cbcm/eu-cm-ontology#be008">
        <rdf:type rdf:resource="http://w3id.org/um/cbcm/eu-cm-ontology#CompanyLegalForm"/>
        <dc:title xml:lang="be">  Coöperatieve vennootschap met beperkte aansprakelijkheid </dc:title>
        <dc:title xml:lang="be">  Genossenschaft mit beschränkter Haftung</dc:title>
        <dc:title xml:lang="en">Cooperative company with limited liability</dc:title>
        <dc:title xml:lang="be">Société coopérative à responsabilité limitée </dc:title>
        <rdfs:label rdf:datatype="http://www.w3.org/2001/XMLSchema#string">CVBA</rdfs:label>
        <rdfs:label rdf:datatype="http://www.w3.org/2001/XMLSchema#string">Gen.mbH</rdfs:label>
        <rdfs:label rdf:datatype="http://www.w3.org/2001/XMLSchema#string">SCRL</rdfs:label>
    </owl:NamedIndividual>
    


    <!-- http://w3id.org/um/cbcm/eu-cm-ontology#be011 -->

    <owl:NamedIndividual rdf:about="http://w3id.org/um/cbcm/eu-cm-ontology#be011">
        <rdf:type rdf:resource="http://w3id.org/um/cbcm/eu-cm-ontology#CompanyLegalForm"/>
        <dc:title xml:lang="be">  Offene Handelsgesellschaft</dc:title>
        <dc:title xml:lang="be">  Vennootschap onder firma </dc:title>
        <dc:title xml:lang="en">General partnership</dc:title>
        <dc:title xml:lang="be">Société en nom collectif </dc:title>
        <rdfs:label rdf:datatype="http://www.w3.org/2001/XMLSchema#string">OHG</rdfs:label>
        <rdfs:label rdf:datatype="http://www.w3.org/2001/XMLSchema#string">SNC</rdfs:label>
        <rdfs:label rdf:datatype="http://www.w3.org/2001/XMLSchema#string">V.O.F.</rdfs:label>
    </owl:NamedIndividual>
    


    <!-- http://w3id.org/um/cbcm/eu-cm-ontology#be012 -->

    <owl:NamedIndividual rdf:about="http://w3id.org/um/cbcm/eu-cm-ontology#be012">
        <rdf:type rdf:resource="http://w3id.org/um/cbcm/eu-cm-ontology#CompanyLegalForm"/>
        <dc:title xml:lang="be">  Einfache Kommanditgesellschaft</dc:title>
        <dc:title xml:lang="be">  Gewone commanditaire vennootschap </dc:title>
        <dc:title xml:lang="en">Ordinary limited partnership</dc:title>
        <dc:title xml:lang="be">Société en commandite simple </dc:title>
        <rdfs:label rdf:datatype="http://www.w3.org/2001/XMLSchema#string">Comm.V</rdfs:label>
        <rdfs:label rdf:datatype="http://www.w3.org/2001/XMLSchema#string">EKG</rdfs:label>
        <rdfs:label rdf:datatype="http://www.w3.org/2001/XMLSchema#string">SCS</rdfs:label>
    </owl:NamedIndividual>
    


    <!-- http://w3id.org/um/cbcm/eu-cm-ontology#be013 -->

    <owl:NamedIndividual rdf:about="http://w3id.org/um/cbcm/eu-cm-ontology#be013">
        <rdf:type rdf:resource="http://w3id.org/um/cbcm/eu-cm-ontology#CompanyLegalForm"/>
        <dc:title xml:lang="be">  Commanditaire vennootschap op aandelen </dc:title>
        <dc:title xml:lang="be">  Kommanditgesellschaft auf Aktien</dc:title>
        <dc:title xml:lang="en">Partnership limited by shares</dc:title>
        <dc:title xml:lang="be">Société en commandite par actions </dc:title>
        <rdfs:label rdf:datatype="http://www.w3.org/2001/XMLSchema#string">Comm.VA</rdfs:label>
        <rdfs:label rdf:datatype="http://www.w3.org/2001/XMLSchema#string">KGaA</rdfs:label>
        <rdfs:label rdf:datatype="http://www.w3.org/2001/XMLSchema#string">SCA</rdfs:label>
    </owl:NamedIndividual>
    


    <!-- http://w3id.org/um/cbcm/eu-cm-ontology#be014 -->

    <owl:NamedIndividual rdf:about="http://w3id.org/um/cbcm/eu-cm-ontology#be014">
        <rdf:type rdf:resource="http://w3id.org/um/cbcm/eu-cm-ontology#CompanyLegalForm"/>
        <dc:title xml:lang="be">  Aktiengesellschaft</dc:title>
        <dc:title xml:lang="be">  Naamloze vennootschap </dc:title>
        <dc:title xml:lang="en">Public limited company</dc:title>
        <dc:title xml:lang="be">Société anonyme </dc:title>
        <rdfs:label rdf:datatype="http://www.w3.org/2001/XMLSchema#string">AG</rdfs:label>
        <rdfs:label rdf:datatype="http://www.w3.org/2001/XMLSchema#string">NV</rdfs:label>
        <rdfs:label rdf:datatype="http://www.w3.org/2001/XMLSchema#string">SA</rdfs:label>
    </owl:NamedIndividual>
    


    <!-- http://w3id.org/um/cbcm/eu-cm-ontology#be015 -->

    <owl:NamedIndividual rdf:about="http://w3id.org/um/cbcm/eu-cm-ontology#be015">
        <rdf:type rdf:resource="http://w3id.org/um/cbcm/eu-cm-ontology#CompanyLegalForm"/>
        <dc:title xml:lang="be">  Besloten vennootschap met beperkte aansprakelijkheid </dc:title>
        <dc:title xml:lang="be">  Privatgesellschaft mit beschränkter Haftung</dc:title>
        <dc:title xml:lang="en">Private limited liability company</dc:title>
        <dc:title xml:lang="be">Société privée à responsabilité limitée </dc:title>
        <rdfs:label rdf:datatype="http://www.w3.org/2001/XMLSchema#string">BVBA</rdfs:label>
        <rdfs:label rdf:datatype="http://www.w3.org/2001/XMLSchema#string">PGmbH</rdfs:label>
        <rdfs:label rdf:datatype="http://www.w3.org/2001/XMLSchema#string">SPRL</rdfs:label>
    </owl:NamedIndividual>
    


    <!-- http://w3id.org/um/cbcm/eu-cm-ontology#be017 -->

    <owl:NamedIndividual rdf:about="http://w3id.org/um/cbcm/eu-cm-ontology#be017">
        <rdf:type rdf:resource="http://w3id.org/um/cbcm/eu-cm-ontology#CompanyLegalForm"/>
        <dc:title xml:lang="be">  Vereinigung ohne Gewinnerzielungsabsicht</dc:title>
        <dc:title xml:lang="be">  Vereniging zonder winstoogmerk </dc:title>
        <dc:title xml:lang="be">Association sans but lucratif </dc:title>
        <dc:title xml:lang="en">Non-profit association</dc:title>
        <rdfs:label rdf:datatype="http://www.w3.org/2001/XMLSchema#string">ASBL</rdfs:label>
        <rdfs:label rdf:datatype="http://www.w3.org/2001/XMLSchema#string">VZW</rdfs:label>
        <rdfs:label rdf:datatype="http://www.w3.org/2001/XMLSchema#string">VoG</rdfs:label>
    </owl:NamedIndividual>
    


    <!-- http://w3id.org/um/cbcm/eu-cm-ontology#be019 -->

    <owl:NamedIndividual rdf:about="http://w3id.org/um/cbcm/eu-cm-ontology#be019">
        <rdf:type rdf:resource="http://w3id.org/um/cbcm/eu-cm-ontology#CompanyLegalForm"/>
        <dc:title xml:lang="be">  Gesellschaft auf Gegenseitigkeit </dc:title>
        <dc:title xml:lang="be">  Krankenkasse </dc:title>
        <dc:title xml:lang="be">  Krankenkassenlandesverband</dc:title>
        <dc:title xml:lang="be">  Landsbond van ziekenfondsen </dc:title>
        <dc:title xml:lang="be">  Maatschappij van onderlinge bijstand </dc:title>
        <dc:title xml:lang="be">  Société Mutualiste </dc:title>
        <dc:title xml:lang="be">  Union nationale de mutualités </dc:title>
        <dc:title xml:lang="be">  Ziekenfonds </dc:title>
        <dc:title xml:lang="en">Mutual health fund / Mutual Benefit Society / National Union of mutual health funds</dc:title>
        <dc:title xml:lang="be">Mutualité </dc:title>
        <rdfs:label rdf:datatype="http://www.w3.org/2001/XMLSchema#string">Kankenka</rdfs:label>
        <rdfs:label rdf:datatype="http://www.w3.org/2001/XMLSchema#string">MUTU</rdfs:label>
        <rdfs:label rdf:datatype="http://www.w3.org/2001/XMLSchema#string">ZIEKF</rdfs:label>
    </owl:NamedIndividual>
    


    <!-- http://w3id.org/um/cbcm/eu-cm-ontology#be020 -->

    <owl:NamedIndividual rdf:about="http://w3id.org/um/cbcm/eu-cm-ontology#be020">
        <rdf:type rdf:resource="http://w3id.org/um/cbcm/eu-cm-ontology#CompanyLegalForm"/>
        <dc:title xml:lang="be">  Beroepsvereniging </dc:title>
        <dc:title xml:lang="be">  Berufsvereinigung</dc:title>
        <dc:title xml:lang="en">Professional association</dc:title>
        <dc:title xml:lang="be">Union professionnelle </dc:title>
        <rdfs:label rdf:datatype="http://www.w3.org/2001/XMLSchema#string">BV</rdfs:label>
        <rdfs:label rdf:datatype="http://www.w3.org/2001/XMLSchema#string">UP</rdfs:label>
    </owl:NamedIndividual>
    


    <!-- http://w3id.org/um/cbcm/eu-cm-ontology#be021 -->

    <owl:NamedIndividual rdf:about="http://w3id.org/um/cbcm/eu-cm-ontology#be021">
        <rdf:type rdf:resource="http://w3id.org/um/cbcm/eu-cm-ontology#CompanyLegalForm"/>
        <dc:title xml:lang="be">  Caisse commune dassurances de droit privé </dc:title>
        <dc:title xml:lang="be">  Gemeenschappelijke verzekeringskas van privaat recht </dc:title>
        <dc:title xml:lang="be">  Onderlinge verzekeringsvereniging </dc:title>
        <dc:title xml:lang="be">  Privatrechtliche Versicherungsgesellschaft</dc:title>
        <dc:title xml:lang="be">  Versicherungsvereinigung auf Gegenseitigkeit </dc:title>
        <dc:title xml:lang="be">Association dassurances mutuelles </dc:title>
        <dc:title xml:lang="en">Mutual insurance association / Mutual insurance fund under private law</dc:title>
        <rdfs:label rdf:datatype="http://www.w3.org/2001/XMLSchema#string">AAM</rdfs:label>
        <rdfs:label rdf:datatype="http://www.w3.org/2001/XMLSchema#string">OVV</rdfs:label>
        <rdfs:label rdf:datatype="http://www.w3.org/2001/XMLSchema#string">PRVGaG</rdfs:label>
    </owl:NamedIndividual>
    


    <!-- http://w3id.org/um/cbcm/eu-cm-ontology#be025 -->

    <owl:NamedIndividual rdf:about="http://w3id.org/um/cbcm/eu-cm-ontology#be025">
        <rdf:type rdf:resource="http://w3id.org/um/cbcm/eu-cm-ontology#CompanyLegalForm"/>
        <dc:title xml:lang="be">  Landbouwvennootschap </dc:title>
        <dc:title xml:lang="be">  Landwirtschaftliche Gesellschaft</dc:title>
        <dc:title xml:lang="en">Agricultural company</dc:title>
        <dc:title xml:lang="be">Société agricole </dc:title>
        <rdfs:label rdf:datatype="http://www.w3.org/2001/XMLSchema#string">LG</rdfs:label>
        <rdfs:label rdf:datatype="http://www.w3.org/2001/XMLSchema#string">LV</rdfs:label>
        <rdfs:label rdf:datatype="http://www.w3.org/2001/XMLSchema#string">S.Agr.</rdfs:label>
    </owl:NamedIndividual>
    


    <!-- http://w3id.org/um/cbcm/eu-cm-ontology#be026 -->

    <owl:NamedIndividual rdf:about="http://w3id.org/um/cbcm/eu-cm-ontology#be026">
        <rdf:type rdf:resource="http://w3id.org/um/cbcm/eu-cm-ontology#CompanyLegalForm"/>
        <dc:title xml:lang="be">  Private stichting </dc:title>
        <dc:title xml:lang="be">  Privatstiftung</dc:title>
        <dc:title xml:lang="be">Fondation privée </dc:title>
        <dc:title xml:lang="en">Private Foundation</dc:title>
        <rdfs:label rdf:datatype="http://www.w3.org/2001/XMLSchema#string">FP</rdfs:label>
        <rdfs:label rdf:datatype="http://www.w3.org/2001/XMLSchema#string">PS</rdfs:label>
        <rdfs:label rdf:datatype="http://www.w3.org/2001/XMLSchema#string">PrSt</rdfs:label>
    </owl:NamedIndividual>
    


    <!-- http://w3id.org/um/cbcm/eu-cm-ontology#be028 -->

    <owl:NamedIndividual rdf:about="http://w3id.org/um/cbcm/eu-cm-ontology#be028">
        <rdf:type rdf:resource="http://w3id.org/um/cbcm/eu-cm-ontology#CompanyLegalForm"/>
        <dc:title xml:lang="be">  Einrichtung ohne Gewinnerzielungsabsicht</dc:title>
        <dc:title xml:lang="be">  Instelling zonder winstoogmerk </dc:title>
        <dc:title xml:lang="be">Institution sans but lucratif </dc:title>
        <dc:title xml:lang="en">Non-profit institution</dc:title>
        <rdfs:label rdf:datatype="http://www.w3.org/2001/XMLSchema#string">EoG</rdfs:label>
        <rdfs:label rdf:datatype="http://www.w3.org/2001/XMLSchema#string">ISBL</rdfs:label>
        <rdfs:label rdf:datatype="http://www.w3.org/2001/XMLSchema#string">IZW</rdfs:label>
    </owl:NamedIndividual>
    


    <!-- http://w3id.org/um/cbcm/eu-cm-ontology#be029 -->

    <owl:NamedIndividual rdf:about="http://w3id.org/um/cbcm/eu-cm-ontology#be029">
        <rdf:type rdf:resource="http://w3id.org/um/cbcm/eu-cm-ontology#CompanyLegalForm"/>
        <dc:title xml:lang="be">  Gemeinnützige Stiftung</dc:title>
        <dc:title xml:lang="be">  Stichting van openbaar nut </dc:title>
        <dc:title xml:lang="be">Fondation dutilité publique </dc:title>
        <dc:title xml:lang="en">Public utility foundation</dc:title>
        <rdfs:label rdf:datatype="http://www.w3.org/2001/XMLSchema#string">FUP</rdfs:label>
        <rdfs:label rdf:datatype="http://www.w3.org/2001/XMLSchema#string">SON</rdfs:label>
        <rdfs:label rdf:datatype="http://www.w3.org/2001/XMLSchema#string">gnS</rdfs:label>
    </owl:NamedIndividual>
    


    <!-- http://w3id.org/um/cbcm/eu-cm-ontology#be051 -->

    <owl:NamedIndividual rdf:about="http://w3id.org/um/cbcm/eu-cm-ontology#be051">
        <rdf:type rdf:resource="http://w3id.org/um/cbcm/eu-cm-ontology#CompanyLegalForm"/>
        <dc:title xml:lang="be">  Andere privaatrechtelijke vorm met rechtspersoonlijkheid </dc:title>
        <dc:title xml:lang="be">  Andere privatrechtliche Rechtsform mit Rechtspersönlichkeit</dc:title>
        <dc:title xml:lang="be">Autre forme de droit privé avec personnalité juridique </dc:title>
        <dc:title xml:lang="en">Other private-law form with legal personality</dc:title>
        <rdfs:label rdf:datatype="http://www.w3.org/2001/XMLSchema#string">AFDPPJ</rdfs:label>
        <rdfs:label rdf:datatype="http://www.w3.org/2001/XMLSchema#string">APRVRP</rdfs:label>
        <rdfs:label rdf:datatype="http://www.w3.org/2001/XMLSchema#string">PRRFmRP</rdfs:label>
    </owl:NamedIndividual>
    


    <!-- http://w3id.org/um/cbcm/eu-cm-ontology#be060 -->

    <owl:NamedIndividual rdf:about="http://w3id.org/um/cbcm/eu-cm-ontology#be060">
        <rdf:type rdf:resource="http://w3id.org/um/cbcm/eu-cm-ontology#CompanyLegalForm"/>
        <dc:title xml:lang="be">  Economisch samenwerkingsverband  </dc:title>
        <dc:title xml:lang="be">  Wirtschaftliche Interessenvereinigung</dc:title>
        <dc:title xml:lang="en">Economic interest grouping</dc:title>
        <dc:title xml:lang="be">Groupement dintérêt économique </dc:title>
        <rdfs:label rdf:datatype="http://www.w3.org/2001/XMLSchema#string">ESV</rdfs:label>
        <rdfs:label rdf:datatype="http://www.w3.org/2001/XMLSchema#string">GIE</rdfs:label>
        <rdfs:label rdf:datatype="http://www.w3.org/2001/XMLSchema#string">WIV</rdfs:label>
    </owl:NamedIndividual>
    


    <!-- http://w3id.org/um/cbcm/eu-cm-ontology#be070 -->

    <owl:NamedIndividual rdf:about="http://w3id.org/um/cbcm/eu-cm-ontology#be070">
        <rdf:type rdf:resource="http://w3id.org/um/cbcm/eu-cm-ontology#CompanyLegalForm"/>
        <dc:title xml:lang="be">  Miteigentümervereinigung</dc:title>
        <dc:title xml:lang="be">  Vereniging van mede-eigenaars </dc:title>
        <dc:title xml:lang="be">Association des copropriétaires </dc:title>
        <dc:title xml:lang="en">Joint owners association</dc:title>
        <rdfs:label rdf:datatype="http://www.w3.org/2001/XMLSchema#string">ACP</rdfs:label>
        <rdfs:label rdf:datatype="http://www.w3.org/2001/XMLSchema#string">MEV</rdfs:label>
        <rdfs:label rdf:datatype="http://www.w3.org/2001/XMLSchema#string">VME</rdfs:label>
    </owl:NamedIndividual>
    


    <!-- http://w3id.org/um/cbcm/eu-cm-ontology#be107 -->

    <owl:NamedIndividual rdf:about="http://w3id.org/um/cbcm/eu-cm-ontology#be107">
        <rdf:type rdf:resource="http://w3id.org/um/cbcm/eu-cm-ontology#CompanyLegalForm"/>
        <dc:title xml:lang="be">  Coöperatieve vennootschap met onbeperkte aansprakelijkheid</dc:title>
        <dc:title xml:lang="be">  Öffentlich-rechtliche Genossenschaft mit unbeschränkter Haftung</dc:title>
        <dc:title xml:lang="be"> Genossenschaft auf Beteiligung</dc:title>
        <dc:title xml:lang="en"> Participating cooperative</dc:title>
        <dc:title xml:lang="be"> bij wijze van deelneming van publiek recht </dc:title>
        <dc:title xml:lang="be"> coopérative de participation</dc:title>
        <dc:title xml:lang="be"> de droit public </dc:title>
        <dc:title xml:lang="en"> governed by public law</dc:title>
        <dc:title xml:lang="en">Cooperative company with unlimited liability</dc:title>
        <dc:title xml:lang="be">Coopérative à responsabilité illimitée</dc:title>
        <rdfs:label rdf:datatype="http://www.w3.org/2001/XMLSchema#string">CVOACD</rdfs:label>
        <rdfs:label rdf:datatype="http://www.w3.org/2001/XMLSchema#string">GmuHGB</rdfs:label>
        <rdfs:label rdf:datatype="http://www.w3.org/2001/XMLSchema#string">SCRICP</rdfs:label>
    </owl:NamedIndividual>
    


    <!-- http://w3id.org/um/cbcm/eu-cm-ontology#be108 -->

    <owl:NamedIndividual rdf:about="http://w3id.org/um/cbcm/eu-cm-ontology#be108">
        <rdf:type rdf:resource="http://w3id.org/um/cbcm/eu-cm-ontology#CompanyLegalForm"/>
        <dc:title xml:lang="be">  Coöperatieve vennootschap met beperkte aansprakelijkheid van publiek recht </dc:title>
        <dc:title xml:lang="be">  Öffentlich-rechtliche Genossenschaft mit beschränkter Haftung</dc:title>
        <dc:title xml:lang="en"> governed by public law</dc:title>
        <dc:title xml:lang="en">Cooperative company with limited liability</dc:title>
        <dc:title xml:lang="be">Société coopérative à responsabilité limitée de droit public </dc:title>
        <rdfs:label rdf:datatype="http://www.w3.org/2001/XMLSchema#string">CVBAPR</rdfs:label>
        <rdfs:label rdf:datatype="http://www.w3.org/2001/XMLSchema#string">SCRLDPU</rdfs:label>
        <rdfs:label rdf:datatype="http://www.w3.org/2001/XMLSchema#string">ÖfrGmbH</rdfs:label>
    </owl:NamedIndividual>
    


    <!-- http://w3id.org/um/cbcm/eu-cm-ontology#be114 -->

    <owl:NamedIndividual rdf:about="http://w3id.org/um/cbcm/eu-cm-ontology#be114">
        <rdf:type rdf:resource="http://w3id.org/um/cbcm/eu-cm-ontology#CompanyLegalForm"/>
        <dc:title xml:lang="be">  Naamloze vennootschap van publiek recht </dc:title>
        <dc:title xml:lang="be">  Öffentlich-rechtliche Aktiengesellschaft</dc:title>
        <dc:title xml:lang="en"> governed by public law</dc:title>
        <dc:title xml:lang="en">Public limited company</dc:title>
        <dc:title xml:lang="be">Société anonyme de droit public </dc:title>
        <rdfs:label rdf:datatype="http://www.w3.org/2001/XMLSchema#string">NVPR</rdfs:label>
        <rdfs:label rdf:datatype="http://www.w3.org/2001/XMLSchema#string">SADPU</rdfs:label>
        <rdfs:label rdf:datatype="http://www.w3.org/2001/XMLSchema#string">Ö.-r.AG</rdfs:label>
    </owl:NamedIndividual>
    


    <!-- http://w3id.org/um/cbcm/eu-cm-ontology#be117 -->

    <owl:NamedIndividual rdf:about="http://w3id.org/um/cbcm/eu-cm-ontology#be117">
        <rdf:type rdf:resource="http://w3id.org/um/cbcm/eu-cm-ontology#CompanyLegalForm"/>
        <dc:title xml:lang="be">  Vereniging zonder winstoogmerk van publiek recht </dc:title>
        <dc:title xml:lang="be">  Öffentlich-rechtliche Vereinigung ohne Gewinnerzielungsabsicht</dc:title>
        <dc:title xml:lang="en"> governed by public law</dc:title>
        <dc:title xml:lang="be">Association sans but lucratif de droit public </dc:title>
        <dc:title xml:lang="en">Non-profit association</dc:title>
        <rdfs:label rdf:datatype="http://www.w3.org/2001/XMLSchema#string">ASBLDPU</rdfs:label>
        <rdfs:label rdf:datatype="http://www.w3.org/2001/XMLSchema#string">VZWPR</rdfs:label>
        <rdfs:label rdf:datatype="http://www.w3.org/2001/XMLSchema#string">ÖrVohGza</rdfs:label>
    </owl:NamedIndividual>
    


    <!-- http://w3id.org/um/cbcm/eu-cm-ontology#be121 -->

    <owl:NamedIndividual rdf:about="http://w3id.org/um/cbcm/eu-cm-ontology#be121">
        <rdf:type rdf:resource="http://w3id.org/um/cbcm/eu-cm-ontology#CompanyLegalForm"/>
        <dc:title xml:lang="be">  Onderlinge verzekeringsvereniging van publiek recht </dc:title>
        <dc:title xml:lang="be">  Öffentlich-rechtliche Versicherungsvereinigung auf Gegenseitigkeit</dc:title>
        <dc:title xml:lang="en"> governed by public law</dc:title>
        <dc:title xml:lang="be">Association dassurances mutuelles de droit public </dc:title>
        <dc:title xml:lang="en">Mutual insurance association</dc:title>
        <rdfs:label rdf:datatype="http://www.w3.org/2001/XMLSchema#string">OVVPR</rdfs:label>
        <rdfs:label rdf:datatype="http://www.w3.org/2001/XMLSchema#string">SAMDPU</rdfs:label>
        <rdfs:label rdf:datatype="http://www.w3.org/2001/XMLSchema#string">ÖrVgGe</rdfs:label>
    </owl:NamedIndividual>
    


    <!-- http://w3id.org/um/cbcm/eu-cm-ontology#be124 -->

    <owl:NamedIndividual rdf:about="http://w3id.org/um/cbcm/eu-cm-ontology#be124">
        <rdf:type rdf:resource="http://w3id.org/um/cbcm/eu-cm-ontology#CompanyLegalForm"/>
        <dc:title xml:lang="be">  Openbare instelling </dc:title>
        <dc:title xml:lang="be">  Öffentliche Einrichtung</dc:title>
        <dc:title xml:lang="be">Etablissement public </dc:title>
        <dc:title xml:lang="en">Public institution</dc:title>
        <rdfs:label rdf:datatype="http://www.w3.org/2001/XMLSchema#string">ETSPUBLI</rdfs:label>
        <rdfs:label rdf:datatype="http://www.w3.org/2001/XMLSchema#string">OI</rdfs:label>
        <rdfs:label rdf:datatype="http://www.w3.org/2001/XMLSchema#string">ÖE</rdfs:label>
    </owl:NamedIndividual>
    


    <!-- http://w3id.org/um/cbcm/eu-cm-ontology#be125 -->

    <owl:NamedIndividual rdf:about="http://w3id.org/um/cbcm/eu-cm-ontology#be125">
        <rdf:type rdf:resource="http://w3id.org/um/cbcm/eu-cm-ontology#CompanyLegalForm"/>
        <dc:title xml:lang="be">  Internationale Vereinigung ohne Gewinnerzielungsabsicht</dc:title>
        <dc:title xml:lang="be">  Internationale vereniging zonder winstoogmerk </dc:title>
        <dc:title xml:lang="be">Association internationale sans but lucratif </dc:title>
        <dc:title xml:lang="en">International non-profit association</dc:title>
        <rdfs:label rdf:datatype="http://www.w3.org/2001/XMLSchema#string">AISBL</rdfs:label>
        <rdfs:label rdf:datatype="http://www.w3.org/2001/XMLSchema#string">IVZW</rdfs:label>
        <rdfs:label rdf:datatype="http://www.w3.org/2001/XMLSchema#string">IVoG</rdfs:label>
    </owl:NamedIndividual>
    


    <!-- http://w3id.org/um/cbcm/eu-cm-ontology#be127 -->

    <owl:NamedIndividual rdf:about="http://w3id.org/um/cbcm/eu-cm-ontology#be127">
        <rdf:type rdf:resource="http://w3id.org/um/cbcm/eu-cm-ontology#CompanyLegalForm"/>
        <dc:title xml:lang="be">  Berg van Barmhartigheid </dc:title>
        <dc:title xml:lang="be">  Pfandleihhaus</dc:title>
        <dc:title xml:lang="be">Monts-de-Piété </dc:title>
        <dc:title xml:lang="en">Pawnshop</dc:title>
        <rdfs:label rdf:datatype="http://www.w3.org/2001/XMLSchema#string">BVB</rdfs:label>
        <rdfs:label rdf:datatype="http://www.w3.org/2001/XMLSchema#string">LH</rdfs:label>
        <rdfs:label rdf:datatype="http://www.w3.org/2001/XMLSchema#string">PIETE</rdfs:label>
    </owl:NamedIndividual>
    


    <!-- http://w3id.org/um/cbcm/eu-cm-ontology#be129 -->

    <owl:NamedIndividual rdf:about="http://w3id.org/um/cbcm/eu-cm-ontology#be129">
        <rdf:type rdf:resource="http://w3id.org/um/cbcm/eu-cm-ontology#CompanyLegalForm"/>
        <dc:title xml:lang="be">  Entwässerungsgenossenschaft - Bewässerungsgenossenschaft</dc:title>
        <dc:title xml:lang="be">  Polder - Watering </dc:title>
        <dc:title xml:lang="en">Polder - watering</dc:title>
        <dc:title xml:lang="be">Polder - wateringue </dc:title>
        <rdfs:label rdf:datatype="http://www.w3.org/2001/XMLSchema#string">Ewg-Bwg</rdfs:label>
        <rdfs:label rdf:datatype="http://www.w3.org/2001/XMLSchema#string">PW</rdfs:label>
    </owl:NamedIndividual>
    


    <!-- http://w3id.org/um/cbcm/eu-cm-ontology#be151 -->

    <owl:NamedIndividual rdf:about="http://w3id.org/um/cbcm/eu-cm-ontology#be151">
        <rdf:type rdf:resource="http://w3id.org/um/cbcm/eu-cm-ontology#CompanyLegalForm"/>
        <dc:title xml:lang="be">  Andere Rechtsform</dc:title>
        <dc:title xml:lang="be">  Andere rechtsvorm </dc:title>
        <dc:title xml:lang="be">Autre forme juridique </dc:title>
        <dc:title xml:lang="en">Other legal form (active)</dc:title>
        <rdfs:label rdf:datatype="http://www.w3.org/2001/XMLSchema#string">AFL</rdfs:label>
        <rdfs:label rdf:datatype="http://www.w3.org/2001/XMLSchema#string">ARF</rdfs:label>
        <rdfs:label rdf:datatype="http://www.w3.org/2001/XMLSchema#string">AV</rdfs:label>
    </owl:NamedIndividual>
    


    <!-- http://w3id.org/um/cbcm/eu-cm-ontology#be200 -->

    <owl:NamedIndividual rdf:about="http://w3id.org/um/cbcm/eu-cm-ontology#be200">
        <rdf:type rdf:resource="http://w3id.org/um/cbcm/eu-cm-ontology#CompanyLegalForm"/>
        <dc:title xml:lang="be">  In Gründung befindliche Gesellschaft</dc:title>
        <dc:title xml:lang="be">  Vennootschap in oprichting </dc:title>
        <dc:title xml:lang="en">Company under formation</dc:title>
        <dc:title xml:lang="be">Société en formation </dc:title>
        <rdfs:label rdf:datatype="http://www.w3.org/2001/XMLSchema#string">GbG</rdfs:label>
        <rdfs:label rdf:datatype="http://www.w3.org/2001/XMLSchema#string">SF</rdfs:label>
        <rdfs:label rdf:datatype="http://www.w3.org/2001/XMLSchema#string">VV</rdfs:label>
    </owl:NamedIndividual>
    


    <!-- http://w3id.org/um/cbcm/eu-cm-ontology#be206 -->

    <owl:NamedIndividual rdf:about="http://w3id.org/um/cbcm/eu-cm-ontology#be206">
        <rdf:type rdf:resource="http://w3id.org/um/cbcm/eu-cm-ontology#CompanyLegalForm"/>
        <dc:title xml:lang="be">  Burgerlijke vennootschap onder vorm van coöperatieve vennootschap met onbeperkte aansprakelijkheid </dc:title>
        <dc:title xml:lang="be">  Zivilrechtliche Gesellschaft in der Rechtsform einer Genossenschaft mit unbeschränkter Haftung</dc:title>
        <dc:title xml:lang="en">Non-trading company in the form of a cooperative company with unlimited liability</dc:title>
        <dc:title xml:lang="be">Société civile sous forme de société coopérative à responsabilité illimitée </dc:title>
        <rdfs:label rdf:datatype="http://www.w3.org/2001/XMLSchema#string">BVCVOA</rdfs:label>
        <rdfs:label rdf:datatype="http://www.w3.org/2001/XMLSchema#string">SCSCRI</rdfs:label>
        <rdfs:label rdf:datatype="http://www.w3.org/2001/XMLSchema#string">ZvGGugcH</rdfs:label>
    </owl:NamedIndividual>
    


    <!-- http://w3id.org/um/cbcm/eu-cm-ontology#be208 -->

    <owl:NamedIndividual rdf:about="http://w3id.org/um/cbcm/eu-cm-ontology#be208">
        <rdf:type rdf:resource="http://w3id.org/um/cbcm/eu-cm-ontology#CompanyLegalForm"/>
        <dc:title xml:lang="be">  Burgerlijke vennootschap onder vorm van coöperatieve vennootschap met beperkte aansprakelijkheid </dc:title>
        <dc:title xml:lang="be">  Zivilrechtliche Gesellschaft in der Rechtsform einer Genossenschaft mit beschränkter Haftung</dc:title>
        <dc:title xml:lang="en">Non-trading company in the form of a cooperative company with limited liability</dc:title>
        <dc:title xml:lang="be">Société civile sous forme de société coopérative à responsabilité limitée </dc:title>
        <rdfs:label rdf:datatype="http://www.w3.org/2001/XMLSchema#string">BVCVBA</rdfs:label>
        <rdfs:label rdf:datatype="http://www.w3.org/2001/XMLSchema#string">SCSCRL</rdfs:label>
        <rdfs:label rdf:datatype="http://www.w3.org/2001/XMLSchema#string">ZvGGbH</rdfs:label>
    </owl:NamedIndividual>
    


    <!-- http://w3id.org/um/cbcm/eu-cm-ontology#be211 -->

    <owl:NamedIndividual rdf:about="http://w3id.org/um/cbcm/eu-cm-ontology#be211">
        <rdf:type rdf:resource="http://w3id.org/um/cbcm/eu-cm-ontology#CompanyLegalForm"/>
        <dc:title xml:lang="be">  Burgerlijke vennootschap onder vorm van vennootschap onder firma </dc:title>
        <dc:title xml:lang="be">  Zivilrechtliche Gesellschaft in der Rechtsform einer offenen Handelsgesellschaft</dc:title>
        <dc:title xml:lang="en">Non-trading company in the form of a general partnership</dc:title>
        <dc:title xml:lang="be">Société civile sous forme de société en nom collectif </dc:title>
        <rdfs:label rdf:datatype="http://www.w3.org/2001/XMLSchema#string">BVVOF</rdfs:label>
        <rdfs:label rdf:datatype="http://www.w3.org/2001/XMLSchema#string">SCSNC</rdfs:label>
        <rdfs:label rdf:datatype="http://www.w3.org/2001/XMLSchema#string">ZRGOHG</rdfs:label>
    </owl:NamedIndividual>
    


    <!-- http://w3id.org/um/cbcm/eu-cm-ontology#be212 -->

    <owl:NamedIndividual rdf:about="http://w3id.org/um/cbcm/eu-cm-ontology#be212">
        <rdf:type rdf:resource="http://w3id.org/um/cbcm/eu-cm-ontology#CompanyLegalForm"/>
        <dc:title xml:lang="be">  Burgerlijke vennootschap onder vorm van gewone commanditaire vennootschap </dc:title>
        <dc:title xml:lang="be">  Zivilrechtliche Gesellschaft in der Rechtsform einer einfachen Kommanditgesellschaft</dc:title>
        <dc:title xml:lang="en">Non-trading company in the form of an ordinary limited partnership</dc:title>
        <dc:title xml:lang="be">Société civile sous forme de société en commandite simple </dc:title>
        <rdfs:label rdf:datatype="http://www.w3.org/2001/XMLSchema#string">BVGCV</rdfs:label>
        <rdfs:label rdf:datatype="http://www.w3.org/2001/XMLSchema#string">SCSCS</rdfs:label>
        <rdfs:label rdf:datatype="http://www.w3.org/2001/XMLSchema#string">ZRGEKG</rdfs:label>
    </owl:NamedIndividual>
    


    <!-- http://w3id.org/um/cbcm/eu-cm-ontology#be213 -->

    <owl:NamedIndividual rdf:about="http://w3id.org/um/cbcm/eu-cm-ontology#be213">
        <rdf:type rdf:resource="http://w3id.org/um/cbcm/eu-cm-ontology#CompanyLegalForm"/>
        <dc:title xml:lang="be">  Burgerlijke vennootschap onder vorm van commanditaire vennootschap op aandelen </dc:title>
        <dc:title xml:lang="be">  Zivilrechtliche Gesellschaft in der Rechtsform einer Kommanditgesellschaft auf Aktien</dc:title>
        <dc:title xml:lang="en">Non-trading company in the form of a partnership limited by shares</dc:title>
        <dc:title xml:lang="be">Société civile sous forme de société en commandite par actions </dc:title>
        <rdfs:label rdf:datatype="http://www.w3.org/2001/XMLSchema#string">BVCVA</rdfs:label>
        <rdfs:label rdf:datatype="http://www.w3.org/2001/XMLSchema#string">SCSCA</rdfs:label>
        <rdfs:label rdf:datatype="http://www.w3.org/2001/XMLSchema#string">ZRGKGaA</rdfs:label>
    </owl:NamedIndividual>
    


    <!-- http://w3id.org/um/cbcm/eu-cm-ontology#be214 -->

    <owl:NamedIndividual rdf:about="http://w3id.org/um/cbcm/eu-cm-ontology#be214">
        <rdf:type rdf:resource="http://w3id.org/um/cbcm/eu-cm-ontology#CompanyLegalForm"/>
        <dc:title xml:lang="be">  Burgerlijke vennootschap onder vorm van naamloze vennootschap </dc:title>
        <dc:title xml:lang="be">  Zivilrechtliche Gesellschaft in der Rechtsform einer Aktiengesellschaft</dc:title>
        <dc:title xml:lang="en">Non-trading company in the form of a public limited company</dc:title>
        <dc:title xml:lang="be">Société civile sous forme de société anonyme </dc:title>
        <rdfs:label rdf:datatype="http://www.w3.org/2001/XMLSchema#string">BVNV</rdfs:label>
        <rdfs:label rdf:datatype="http://www.w3.org/2001/XMLSchema#string">SCSA</rdfs:label>
        <rdfs:label rdf:datatype="http://www.w3.org/2001/XMLSchema#string">ZRGAG</rdfs:label>
    </owl:NamedIndividual>
    


    <!-- http://w3id.org/um/cbcm/eu-cm-ontology#be215 -->

    <owl:NamedIndividual rdf:about="http://w3id.org/um/cbcm/eu-cm-ontology#be215">
        <rdf:type rdf:resource="http://w3id.org/um/cbcm/eu-cm-ontology#CompanyLegalForm"/>
        <dc:title xml:lang="be">  Burgerlijke vennootschap onder vorm van besloten vennootschap met beperkte aansprakelijkheid </dc:title>
        <dc:title xml:lang="be">  Zivilrechtliche Gesellschaft in der Rechtsform einer Privatgesellschaft mit beschränkter Haftung</dc:title>
        <dc:title xml:lang="en">Non-trading company in the form of a private limited liability company</dc:title>
        <dc:title xml:lang="be">Société civile sous forme de société privée à responsabilité limitée </dc:title>
        <rdfs:label rdf:datatype="http://www.w3.org/2001/XMLSchema#string">BVBVBA</rdfs:label>
        <rdfs:label rdf:datatype="http://www.w3.org/2001/XMLSchema#string">SCSPRL</rdfs:label>
        <rdfs:label rdf:datatype="http://www.w3.org/2001/XMLSchema#string">ZvGPgbH</rdfs:label>
    </owl:NamedIndividual>
    


    <!-- http://w3id.org/um/cbcm/eu-cm-ontology#be217 -->

    <owl:NamedIndividual rdf:about="http://w3id.org/um/cbcm/eu-cm-ontology#be217">
        <rdf:type rdf:resource="http://w3id.org/um/cbcm/eu-cm-ontology#CompanyLegalForm"/>
        <dc:title xml:lang="be">  Europese politieke partij </dc:title>
        <dc:title xml:lang="be">  Europäische politische Partei</dc:title>
        <dc:title xml:lang="en">European political party</dc:title>
        <dc:title xml:lang="be">Parti politique européen </dc:title>
        <rdfs:label rdf:datatype="http://www.w3.org/2001/XMLSchema#string">EUPP</rdfs:label>
        <rdfs:label rdf:datatype="http://www.w3.org/2001/XMLSchema#string">PPEU</rdfs:label>
    </owl:NamedIndividual>
    


    <!-- http://w3id.org/um/cbcm/eu-cm-ontology#be218 -->

    <owl:NamedIndividual rdf:about="http://w3id.org/um/cbcm/eu-cm-ontology#be218">
        <rdf:type rdf:resource="http://w3id.org/um/cbcm/eu-cm-ontology#CompanyLegalForm"/>
        <dc:title xml:lang="be">  Europese politieke stichting </dc:title>
        <dc:title xml:lang="be">  Europäische politische Stiftung</dc:title>
        <dc:title xml:lang="en">European political foundation</dc:title>
        <dc:title xml:lang="be">Fondation politique européenne </dc:title>
        <rdfs:label rdf:datatype="http://www.w3.org/2001/XMLSchema#string">EUPS</rdfs:label>
        <rdfs:label rdf:datatype="http://www.w3.org/2001/XMLSchema#string">FPEU</rdfs:label>
    </owl:NamedIndividual>
    


    <!-- http://w3id.org/um/cbcm/eu-cm-ontology#be225 -->

    <owl:NamedIndividual rdf:about="http://w3id.org/um/cbcm/eu-cm-ontology#be225">
        <rdf:type rdf:resource="http://w3id.org/um/cbcm/eu-cm-ontology#CompanyLegalForm"/>
        <dc:title xml:lang="be">  Burgerlijke Vennootschap onder vorm van Landbouwvennootschap (BV LV) </dc:title>
        <dc:title xml:lang="be">  Zivilrechtliche Gesellschaft in der Rechtsform einer landwirtschaftlichen Gesellschaft</dc:title>
        <dc:title xml:lang="en">Non-trading company in the form of an agricultural company</dc:title>
        <dc:title xml:lang="be">Société civile sous forme de société agricole </dc:title>
        <rdfs:label rdf:datatype="http://www.w3.org/2001/XMLSchema#string">BVLV</rdfs:label>
        <rdfs:label rdf:datatype="http://www.w3.org/2001/XMLSchema#string">SCSAGR</rdfs:label>
        <rdfs:label rdf:datatype="http://www.w3.org/2001/XMLSchema#string">ZRGLG</rdfs:label>
    </owl:NamedIndividual>
    


    <!-- http://w3id.org/um/cbcm/eu-cm-ontology#be301 -->

    <owl:NamedIndividual rdf:about="http://w3id.org/um/cbcm/eu-cm-ontology#be301">
        <rdf:type rdf:resource="http://w3id.org/um/cbcm/eu-cm-ontology#CompanyLegalForm"/>
        <dc:title xml:lang="be">  Federale overheidsdienst </dc:title>
        <dc:title xml:lang="be">  Föderaler öffentlicher Dienst</dc:title>
        <dc:title xml:lang="en">Federal Public Service</dc:title>
        <dc:title xml:lang="be">Service public fédéral </dc:title>
        <rdfs:label rdf:datatype="http://www.w3.org/2001/XMLSchema#string">FOD</rdfs:label>
        <rdfs:label rdf:datatype="http://www.w3.org/2001/XMLSchema#string">FÖD</rdfs:label>
        <rdfs:label rdf:datatype="http://www.w3.org/2001/XMLSchema#string">SPF</rdfs:label>
    </owl:NamedIndividual>
    


    <!-- http://w3id.org/um/cbcm/eu-cm-ontology#be302 -->

    <owl:NamedIndividual rdf:about="http://w3id.org/um/cbcm/eu-cm-ontology#be302">
        <rdf:type rdf:resource="http://w3id.org/um/cbcm/eu-cm-ontology#CompanyLegalForm"/>
        <dc:title xml:lang="be">  Föderaler öffentlicher Programmierungsdienst</dc:title>
        <dc:title xml:lang="be">  Programmatorische federale overheidsdienst </dc:title>
        <dc:title xml:lang="en">Federal Public Planning Service </dc:title>
        <dc:title xml:lang="be">Service public fédéral de programmation </dc:title>
        <rdfs:label rdf:datatype="http://www.w3.org/2001/XMLSchema#string">FÖP</rdfs:label>
        <rdfs:label rdf:datatype="http://www.w3.org/2001/XMLSchema#string">POD</rdfs:label>
        <rdfs:label rdf:datatype="http://www.w3.org/2001/XMLSchema#string">SPP</rdfs:label>
    </owl:NamedIndividual>
    


    <!-- http://w3id.org/um/cbcm/eu-cm-ontology#be303 -->

    <owl:NamedIndividual rdf:about="http://w3id.org/um/cbcm/eu-cm-ontology#be303">
        <rdf:type rdf:resource="http://w3id.org/um/cbcm/eu-cm-ontology#CompanyLegalForm"/>
        <dc:title xml:lang="be">  Andere federale dienst </dc:title>
        <dc:title xml:lang="be">  Anderer föderale Dienst</dc:title>
        <dc:title xml:lang="be">Autre service fédéral </dc:title>
        <dc:title xml:lang="en">Other federal service</dc:title>
        <rdfs:label rdf:datatype="http://www.w3.org/2001/XMLSchema#string">FEDEDIEN</rdfs:label>
        <rdfs:label rdf:datatype="http://www.w3.org/2001/XMLSchema#string">FödD</rdfs:label>
        <rdfs:label rdf:datatype="http://www.w3.org/2001/XMLSchema#string">SERVFEDE</rdfs:label>
    </owl:NamedIndividual>
    


    <!-- http://w3id.org/um/cbcm/eu-cm-ontology#be310 -->

    <owl:NamedIndividual rdf:about="http://w3id.org/um/cbcm/eu-cm-ontology#be310">
        <rdf:type rdf:resource="http://w3id.org/um/cbcm/eu-cm-ontology#CompanyLegalForm"/>
        <dc:title xml:lang="be">  Behörde der Flämischen Region und der Flämischen Gemeinschaft</dc:title>
        <dc:title xml:lang="be">  Overheid van het Vlaamse Gewest en van de Vlaamse Gemeenschap </dc:title>
        <dc:title xml:lang="en">Authorities of the Flemish Region and the Flemish Community</dc:title>
        <dc:title xml:lang="be">Autorité de la Région flamande et de la Communauté flamande </dc:title>
        <rdfs:label rdf:datatype="http://www.w3.org/2001/XMLSchema#string">FlRG</rdfs:label>
        <rdfs:label rdf:datatype="http://www.w3.org/2001/XMLSchema#string">REGCOMNL</rdfs:label>
        <rdfs:label rdf:datatype="http://www.w3.org/2001/XMLSchema#string">VLGEWGEM</rdfs:label>
    </owl:NamedIndividual>
    


    <!-- http://w3id.org/um/cbcm/eu-cm-ontology#be320 -->

    <owl:NamedIndividual rdf:about="http://w3id.org/um/cbcm/eu-cm-ontology#be320">
        <rdf:type rdf:resource="http://w3id.org/um/cbcm/eu-cm-ontology#CompanyLegalForm"/>
        <dc:title xml:lang="be">  Behörde der Wallonischen Region</dc:title>
        <dc:title xml:lang="be">  Overheid van het Waalse Gewest </dc:title>
        <dc:title xml:lang="en">Authorities of the Walloon Region</dc:title>
        <dc:title xml:lang="be">Autorité de la Région wallonne </dc:title>
        <rdfs:label rdf:datatype="http://www.w3.org/2001/XMLSchema#string">RW</rdfs:label>
        <rdfs:label rdf:datatype="http://www.w3.org/2001/XMLSchema#string">WG</rdfs:label>
        <rdfs:label rdf:datatype="http://www.w3.org/2001/XMLSchema#string">WR</rdfs:label>
    </owl:NamedIndividual>
    


    <!-- http://w3id.org/um/cbcm/eu-cm-ontology#be325 -->

    <owl:NamedIndividual rdf:about="http://w3id.org/um/cbcm/eu-cm-ontology#be325">
        <rdf:type rdf:resource="http://w3id.org/um/cbcm/eu-cm-ontology#CompanyLegalForm"/>
        <dc:title xml:lang="be">  Internationale vereniging zonder winstoogmerk van publiek recht </dc:title>
        <dc:title xml:lang="be">  Öffentlich-rechtliche Internationale Vereinigung ohne Gewinnerzielungsabsicht</dc:title>
        <dc:title xml:lang="en"> governed by public law</dc:title>
        <dc:title xml:lang="be">Association internationale sans but lucratif de droit public</dc:title>
        <dc:title xml:lang="en">International non-profit association</dc:title>
        <rdfs:label rdf:datatype="http://www.w3.org/2001/XMLSchema#string">AISBLDPU</rdfs:label>
        <rdfs:label rdf:datatype="http://www.w3.org/2001/XMLSchema#string">IVZWPR</rdfs:label>
        <rdfs:label rdf:datatype="http://www.w3.org/2001/XMLSchema#string">ÖrIVoG</rdfs:label>
    </owl:NamedIndividual>
    


    <!-- http://w3id.org/um/cbcm/eu-cm-ontology#be330 -->

    <owl:NamedIndividual rdf:about="http://w3id.org/um/cbcm/eu-cm-ontology#be330">
        <rdf:type rdf:resource="http://w3id.org/um/cbcm/eu-cm-ontology#CompanyLegalForm"/>
        <dc:title xml:lang="be">  Behörde der Region Brüssel-Hauptstadt</dc:title>
        <dc:title xml:lang="be">  Overheid van het Brusselse Hoofdstedelijk Gewest </dc:title>
        <dc:title xml:lang="en">Authorities of the Brussels Capital Region</dc:title>
        <dc:title xml:lang="be">Autorité de la Région de Bruxelles-Capitale </dc:title>
        <rdfs:label rdf:datatype="http://www.w3.org/2001/XMLSchema#string">BRUHOOGE</rdfs:label>
        <rdfs:label rdf:datatype="http://www.w3.org/2001/XMLSchema#string">RBH</rdfs:label>
        <rdfs:label rdf:datatype="http://www.w3.org/2001/XMLSchema#string">REGBRXCA</rdfs:label>
    </owl:NamedIndividual>
    


    <!-- http://w3id.org/um/cbcm/eu-cm-ontology#be340 -->

    <owl:NamedIndividual rdf:about="http://w3id.org/um/cbcm/eu-cm-ontology#be340">
        <rdf:type rdf:resource="http://w3id.org/um/cbcm/eu-cm-ontology#CompanyLegalForm"/>
        <dc:title xml:lang="be">  Behörde der Französischen Gemeinschaft</dc:title>
        <dc:title xml:lang="be">  Overheid van de Franse Gemeenschap </dc:title>
        <dc:title xml:lang="en">Authorities of the French Community</dc:title>
        <dc:title xml:lang="be">Autorité de la Communauté française </dc:title>
        <rdfs:label rdf:datatype="http://www.w3.org/2001/XMLSchema#string">COMMFRAN</rdfs:label>
        <rdfs:label rdf:datatype="http://www.w3.org/2001/XMLSchema#string">FRAGEMEE</rdfs:label>
        <rdfs:label rdf:datatype="http://www.w3.org/2001/XMLSchema#string">FrG</rdfs:label>
    </owl:NamedIndividual>
    


    <!-- http://w3id.org/um/cbcm/eu-cm-ontology#be350 -->

    <owl:NamedIndividual rdf:about="http://w3id.org/um/cbcm/eu-cm-ontology#be350">
        <rdf:type rdf:resource="http://w3id.org/um/cbcm/eu-cm-ontology#CompanyLegalForm"/>
        <dc:title xml:lang="be">  Behörde der Deutschsprachigen Gemeinschaft</dc:title>
        <dc:title xml:lang="be">  Overheid van de Duitstalige Gemeenschap </dc:title>
        <dc:title xml:lang="en">Authorities of the German-speaking Community</dc:title>
        <dc:title xml:lang="be">Autorité de la Communauté germanophone </dc:title>
        <rdfs:label rdf:datatype="http://www.w3.org/2001/XMLSchema#string">COMGERMA</rdfs:label>
        <rdfs:label rdf:datatype="http://www.w3.org/2001/XMLSchema#string">DG</rdfs:label>
        <rdfs:label rdf:datatype="http://www.w3.org/2001/XMLSchema#string">DUITGEME</rdfs:label>
    </owl:NamedIndividual>
    


    <!-- http://w3id.org/um/cbcm/eu-cm-ontology#be400 -->

    <owl:NamedIndividual rdf:about="http://w3id.org/um/cbcm/eu-cm-ontology#be400">
        <rdf:type rdf:resource="http://w3id.org/um/cbcm/eu-cm-ontology#CompanyLegalForm"/>
        <dc:title xml:lang="be">  Provinciale overheid </dc:title>
        <dc:title xml:lang="be">  Provinzialbehörde</dc:title>
        <dc:title xml:lang="be">Autorité provinciale </dc:title>
        <dc:title xml:lang="en">Provincial Authority</dc:title>
        <rdfs:label rdf:datatype="http://www.w3.org/2001/XMLSchema#string">AUTOPROV</rdfs:label>
        <rdfs:label rdf:datatype="http://www.w3.org/2001/XMLSchema#string">PROVOVER</rdfs:label>
        <rdfs:label rdf:datatype="http://www.w3.org/2001/XMLSchema#string">Provbehö</rdfs:label>
    </owl:NamedIndividual>
    


    <!-- http://w3id.org/um/cbcm/eu-cm-ontology#be411 -->

    <owl:NamedIndividual rdf:about="http://w3id.org/um/cbcm/eu-cm-ontology#be411">
        <rdf:type rdf:resource="http://w3id.org/um/cbcm/eu-cm-ontology#CompanyLegalForm"/>
        <dc:title xml:lang="be"> Gemeinde</dc:title>
        <dc:title xml:lang="be"> Stad</dc:title>
        <dc:title xml:lang="be"> Stadt</dc:title>
        <dc:title xml:lang="be"> commune</dc:title>
        <dc:title xml:lang="be"> gemeente</dc:title>
        <dc:title xml:lang="en">City/municipality</dc:title>
        <dc:title xml:lang="be">Ville</dc:title>
        <rdfs:label rdf:datatype="http://www.w3.org/2001/XMLSchema#string">COMMUNES</rdfs:label>
        <rdfs:label rdf:datatype="http://www.w3.org/2001/XMLSchema#string">GEMEENTE</rdfs:label>
        <rdfs:label rdf:datatype="http://www.w3.org/2001/XMLSchema#string">Gemeinde</rdfs:label>
    </owl:NamedIndividual>
    


    <!-- http://w3id.org/um/cbcm/eu-cm-ontology#be412 -->

    <owl:NamedIndividual rdf:about="http://w3id.org/um/cbcm/eu-cm-ontology#be412">
        <rdf:type rdf:resource="http://w3id.org/um/cbcm/eu-cm-ontology#CompanyLegalForm"/>
        <dc:title xml:lang="be">  Openbaar centrum voor maatschappelijk welzijn </dc:title>
        <dc:title xml:lang="be">  Öffentliches Sozialhilfezentrum</dc:title>
        <dc:title xml:lang="be">Centre public daction sociale </dc:title>
        <dc:title xml:lang="en">Public social welfare centre</dc:title>
        <rdfs:label rdf:datatype="http://www.w3.org/2001/XMLSchema#string">CPAS</rdfs:label>
        <rdfs:label rdf:datatype="http://www.w3.org/2001/XMLSchema#string">OCMW</rdfs:label>
        <rdfs:label rdf:datatype="http://www.w3.org/2001/XMLSchema#string">ÖSHZ</rdfs:label>
    </owl:NamedIndividual>
    


    <!-- http://w3id.org/um/cbcm/eu-cm-ontology#be413 -->

    <owl:NamedIndividual rdf:about="http://w3id.org/um/cbcm/eu-cm-ontology#be413">
        <rdf:type rdf:resource="http://w3id.org/um/cbcm/eu-cm-ontology#CompanyLegalForm"/>
        <dc:title xml:lang="be">  Lokale Polizeizone</dc:title>
        <dc:title xml:lang="be">  Lokale politiezone </dc:title>
        <dc:title xml:lang="en">Local Police</dc:title>
        <dc:title xml:lang="be">Police locale </dc:title>
        <rdfs:label rdf:datatype="http://www.w3.org/2001/XMLSchema#string">LOKPOL</rdfs:label>
        <rdfs:label rdf:datatype="http://www.w3.org/2001/XMLSchema#string">LP</rdfs:label>
        <rdfs:label rdf:datatype="http://www.w3.org/2001/XMLSchema#string">POLLOC</rdfs:label>
    </owl:NamedIndividual>
    


    <!-- http://w3id.org/um/cbcm/eu-cm-ontology#be414 -->

    <owl:NamedIndividual rdf:about="http://w3id.org/um/cbcm/eu-cm-ontology#be414">
        <rdf:type rdf:resource="http://w3id.org/um/cbcm/eu-cm-ontology#CompanyLegalForm"/>
        <dc:title xml:lang="be"> Intercommunale</dc:title>
        <dc:title xml:lang="be"> Interkommunale</dc:title>
        <dc:title xml:lang="be">Intercommunale</dc:title>
        <dc:title xml:lang="en">Intermunicipal company</dc:title>
        <rdfs:label rdf:datatype="http://www.w3.org/2001/XMLSchema#string">IC</rdfs:label>
        <rdfs:label rdf:datatype="http://www.w3.org/2001/XMLSchema#string">IK</rdfs:label>
    </owl:NamedIndividual>
    


    <!-- http://w3id.org/um/cbcm/eu-cm-ontology#be415 -->

    <owl:NamedIndividual rdf:about="http://w3id.org/um/cbcm/eu-cm-ontology#be415">
        <rdf:type rdf:resource="http://w3id.org/um/cbcm/eu-cm-ontology#CompanyLegalForm"/>
        <dc:title xml:lang="be">  Projectvereniging </dc:title>
        <dc:title xml:lang="be">  Projektvereinigung</dc:title>
        <dc:title xml:lang="be">Association de projet </dc:title>
        <dc:title xml:lang="en">Project association</dc:title>
        <rdfs:label rdf:datatype="http://www.w3.org/2001/XMLSchema#string">APROJ</rdfs:label>
        <rdfs:label rdf:datatype="http://www.w3.org/2001/XMLSchema#string">PROJV</rdfs:label>
        <rdfs:label rdf:datatype="http://www.w3.org/2001/XMLSchema#string">Prjverng</rdfs:label>
    </owl:NamedIndividual>
    


    <!-- http://w3id.org/um/cbcm/eu-cm-ontology#be416 -->

    <owl:NamedIndividual rdf:about="http://w3id.org/um/cbcm/eu-cm-ontology#be416">
        <rdf:type rdf:resource="http://w3id.org/um/cbcm/eu-cm-ontology#CompanyLegalForm"/>
        <dc:title xml:lang="be">  Dienstleistungsvereinigung (Flämische Region)</dc:title>
        <dc:title xml:lang="be">  Dienstverlenende vereniging (Vlaams Gewest) </dc:title>
        <dc:title xml:lang="be">Association prestataire de services (Région flamande) </dc:title>
        <dc:title xml:lang="en">Services provider association (Flemish Region)</dc:title>
        <rdfs:label rdf:datatype="http://www.w3.org/2001/XMLSchema#string">ASSSERV</rdfs:label>
        <rdfs:label rdf:datatype="http://www.w3.org/2001/XMLSchema#string">DIENSTV</rdfs:label>
        <rdfs:label rdf:datatype="http://www.w3.org/2001/XMLSchema#string">DlvFL</rdfs:label>
    </owl:NamedIndividual>
    


    <!-- http://w3id.org/um/cbcm/eu-cm-ontology#be417 -->

    <owl:NamedIndividual rdf:about="http://w3id.org/um/cbcm/eu-cm-ontology#be417">
        <rdf:type rdf:resource="http://w3id.org/um/cbcm/eu-cm-ontology#CompanyLegalForm"/>
        <dc:title xml:lang="be">  Beauftragte Vereinigung (Flämische Region)</dc:title>
        <dc:title xml:lang="be">  Opdrachthoudende vereniging (Vlaams Gewest) </dc:title>
        <dc:title xml:lang="be">Association chargée de mission (Région flamande) </dc:title>
        <dc:title xml:lang="en">Project entrusted association (Flemish Region)</dc:title>
        <rdfs:label rdf:datatype="http://www.w3.org/2001/XMLSchema#string">ACMISS</rdfs:label>
        <rdfs:label rdf:datatype="http://www.w3.org/2001/XMLSchema#string">BVerFL</rdfs:label>
        <rdfs:label rdf:datatype="http://www.w3.org/2001/XMLSchema#string">OPDRAVER</rdfs:label>
    </owl:NamedIndividual>
    


    <!-- http://w3id.org/um/cbcm/eu-cm-ontology#be418 -->

    <owl:NamedIndividual rdf:about="http://w3id.org/um/cbcm/eu-cm-ontology#be418">
        <rdf:type rdf:resource="http://w3id.org/um/cbcm/eu-cm-ontology#CompanyLegalForm"/>
        <dc:title xml:lang="be">  Autonome Gemeinderegie</dc:title>
        <dc:title xml:lang="be">  Autonoom gemeentebedrijf </dc:title>
        <dc:title xml:lang="en">Autonomous municipal company</dc:title>
        <dc:title xml:lang="be">Régie communale autonome </dc:title>
        <rdfs:label rdf:datatype="http://www.w3.org/2001/XMLSchema#string">AUTOGEMB</rdfs:label>
        <rdfs:label rdf:datatype="http://www.w3.org/2001/XMLSchema#string">AutGemRg</rdfs:label>
        <rdfs:label rdf:datatype="http://www.w3.org/2001/XMLSchema#string">RCOMAUT</rdfs:label>
    </owl:NamedIndividual>
    


    <!-- http://w3id.org/um/cbcm/eu-cm-ontology#be419 -->

    <owl:NamedIndividual rdf:about="http://w3id.org/um/cbcm/eu-cm-ontology#be419">
        <rdf:type rdf:resource="http://w3id.org/um/cbcm/eu-cm-ontology#CompanyLegalForm"/>
        <dc:title xml:lang="be">  Autonome Provinzialregie</dc:title>
        <dc:title xml:lang="be">  Autonoom provinciebedrijf </dc:title>
        <dc:title xml:lang="en">Autonomous provincial company</dc:title>
        <dc:title xml:lang="be">Régie provinciale autonome </dc:title>
        <rdfs:label rdf:datatype="http://www.w3.org/2001/XMLSchema#string">AUTOPRB</rdfs:label>
        <rdfs:label rdf:datatype="http://www.w3.org/2001/XMLSchema#string">AutPrvRg</rdfs:label>
        <rdfs:label rdf:datatype="http://www.w3.org/2001/XMLSchema#string">RPROVAUT</rdfs:label>
    </owl:NamedIndividual>
    


    <!-- http://w3id.org/um/cbcm/eu-cm-ontology#be420 -->

    <owl:NamedIndividual rdf:about="http://w3id.org/um/cbcm/eu-cm-ontology#be420">
        <rdf:type rdf:resource="http://w3id.org/um/cbcm/eu-cm-ontology#CompanyLegalForm"/>
        <dc:title xml:lang="be">  Vereinigung von öffentlichen Sozialhilfezentren</dc:title>
        <dc:title xml:lang="be">  Vereniging van OCMWs </dc:title>
        <dc:title xml:lang="be">Association de CPAS </dc:title>
        <dc:title xml:lang="en">Association of public centres for social welfare</dc:title>
        <rdfs:label rdf:datatype="http://www.w3.org/2001/XMLSchema#string">Ass.CPAS</rdfs:label>
        <rdfs:label rdf:datatype="http://www.w3.org/2001/XMLSchema#string">Ver.OCMW</rdfs:label>
        <rdfs:label rdf:datatype="http://www.w3.org/2001/XMLSchema#string">VÖSHZ</rdfs:label>
    </owl:NamedIndividual>
    


    <!-- http://w3id.org/um/cbcm/eu-cm-ontology#be422 -->

    <owl:NamedIndividual rdf:about="http://w3id.org/um/cbcm/eu-cm-ontology#be422">
        <rdf:type rdf:resource="http://w3id.org/um/cbcm/eu-cm-ontology#CompanyLegalForm"/>
        <dc:title xml:lang="be">  Hilfeleistungszone</dc:title>
        <dc:title xml:lang="be">  Hulpverleningszone </dc:title>
        <dc:title xml:lang="en">Relief zone</dc:title>
        <dc:title xml:lang="be">Zone de secours </dc:title>
        <rdfs:label rdf:datatype="http://www.w3.org/2001/XMLSchema#string">HLZ</rdfs:label>
        <rdfs:label rdf:datatype="http://www.w3.org/2001/XMLSchema#string">HVZ</rdfs:label>
        <rdfs:label rdf:datatype="http://www.w3.org/2001/XMLSchema#string">ZDS</rdfs:label>
    </owl:NamedIndividual>
    


    <!-- http://w3id.org/um/cbcm/eu-cm-ontology#be506 -->

    <owl:NamedIndividual rdf:about="http://w3id.org/um/cbcm/eu-cm-ontology#be506">
        <rdf:type rdf:resource="http://w3id.org/um/cbcm/eu-cm-ontology#CompanyLegalForm"/>
        <dc:title xml:lang="be">  Coöperatieve vennootschap met onbeperkte aansprakelijkheid met een sociaal oogmerk </dc:title>
        <dc:title xml:lang="be">  Genossenschaft mit unbeschränkter Haftung mit sozialer Zielsetzung</dc:title>
        <dc:title xml:lang="en">Cooperative company with unlimited liability with a social purpose</dc:title>
        <dc:title xml:lang="be">Société coopérative à responsabilité illimitée à finalité sociale </dc:title>
        <rdfs:label rdf:datatype="http://www.w3.org/2001/XMLSchema#string">CVOASO</rdfs:label>
        <rdfs:label rdf:datatype="http://www.w3.org/2001/XMLSchema#string">GuHsZ</rdfs:label>
        <rdfs:label rdf:datatype="http://www.w3.org/2001/XMLSchema#string">SCRIFS</rdfs:label>
    </owl:NamedIndividual>
    


    <!-- http://w3id.org/um/cbcm/eu-cm-ontology#be508 -->

    <owl:NamedIndividual rdf:about="http://w3id.org/um/cbcm/eu-cm-ontology#be508">
        <rdf:type rdf:resource="http://w3id.org/um/cbcm/eu-cm-ontology#CompanyLegalForm"/>
        <dc:title xml:lang="be">  Coöperatieve vennootschap met beperkte aansprakelijkheid met een sociaal oogmerk </dc:title>
        <dc:title xml:lang="be">  Genossenschaft mit beschränkter Haftung mit sozialer Zielsetzung</dc:title>
        <dc:title xml:lang="en">Cooperative company with limited liability with a social purpose</dc:title>
        <dc:title xml:lang="be">Société coopérative à responsabilité limitée à finalité sociale </dc:title>
        <rdfs:label rdf:datatype="http://www.w3.org/2001/XMLSchema#string">CVBASO</rdfs:label>
        <rdfs:label rdf:datatype="http://www.w3.org/2001/XMLSchema#string">GbHsZ</rdfs:label>
        <rdfs:label rdf:datatype="http://www.w3.org/2001/XMLSchema#string">SCRLFS</rdfs:label>
    </owl:NamedIndividual>
    


    <!-- http://w3id.org/um/cbcm/eu-cm-ontology#be511 -->

    <owl:NamedIndividual rdf:about="http://w3id.org/um/cbcm/eu-cm-ontology#be511">
        <rdf:type rdf:resource="http://w3id.org/um/cbcm/eu-cm-ontology#CompanyLegalForm"/>
        <dc:title xml:lang="be">  Offene Handelsgesellschaft mit sozialer Zielsetzung</dc:title>
        <dc:title xml:lang="be">  Vennootschap onder firma met een sociaal oogmerk </dc:title>
        <dc:title xml:lang="en">General partnership with a social purpose</dc:title>
        <dc:title xml:lang="be">Société en nom collectif à finalité sociale </dc:title>
        <rdfs:label rdf:datatype="http://www.w3.org/2001/XMLSchema#string">OHGmsZ</rdfs:label>
        <rdfs:label rdf:datatype="http://www.w3.org/2001/XMLSchema#string">SNCFS</rdfs:label>
        <rdfs:label rdf:datatype="http://www.w3.org/2001/XMLSchema#string">VOFSO</rdfs:label>
    </owl:NamedIndividual>
    


    <!-- http://w3id.org/um/cbcm/eu-cm-ontology#be512 -->

    <owl:NamedIndividual rdf:about="http://w3id.org/um/cbcm/eu-cm-ontology#be512">
        <rdf:type rdf:resource="http://w3id.org/um/cbcm/eu-cm-ontology#CompanyLegalForm"/>
        <dc:title xml:lang="be">  Einfache Kommanditgesellschaft mit sozialer Zielsetzung</dc:title>
        <dc:title xml:lang="be">  Gewone commanditaire vennootschap met een sociaal oogmerk </dc:title>
        <dc:title xml:lang="en">Ordinary limited partnership with a social purpose</dc:title>
        <dc:title xml:lang="be">Société en commandite simple à finalité sociale </dc:title>
        <rdfs:label rdf:datatype="http://www.w3.org/2001/XMLSchema#string">EKGmsZ</rdfs:label>
        <rdfs:label rdf:datatype="http://www.w3.org/2001/XMLSchema#string">GCWSO</rdfs:label>
        <rdfs:label rdf:datatype="http://www.w3.org/2001/XMLSchema#string">SCSFS</rdfs:label>
    </owl:NamedIndividual>
    


    <!-- http://w3id.org/um/cbcm/eu-cm-ontology#be513 -->

    <owl:NamedIndividual rdf:about="http://w3id.org/um/cbcm/eu-cm-ontology#be513">
        <rdf:type rdf:resource="http://w3id.org/um/cbcm/eu-cm-ontology#CompanyLegalForm"/>
        <dc:title xml:lang="be">  Commanditaire vennootschap op aandelen met een sociaal oogmerk </dc:title>
        <dc:title xml:lang="be">  Kommanditgesellschaft auf Aktien mit sozialer Zielsetzung</dc:title>
        <dc:title xml:lang="en">Partnership limited by shares with a social purpose</dc:title>
        <dc:title xml:lang="be">Société en commandite par actions à finalité sociale </dc:title>
        <rdfs:label rdf:datatype="http://www.w3.org/2001/XMLSchema#string">CVASO</rdfs:label>
        <rdfs:label rdf:datatype="http://www.w3.org/2001/XMLSchema#string">KGaAmsZ</rdfs:label>
        <rdfs:label rdf:datatype="http://www.w3.org/2001/XMLSchema#string">SCAFS</rdfs:label>
    </owl:NamedIndividual>
    


    <!-- http://w3id.org/um/cbcm/eu-cm-ontology#be514 -->

    <owl:NamedIndividual rdf:about="http://w3id.org/um/cbcm/eu-cm-ontology#be514">
        <rdf:type rdf:resource="http://w3id.org/um/cbcm/eu-cm-ontology#CompanyLegalForm"/>
        <dc:title xml:lang="be">  Aktiengesellschaft mit sozialer Zielsetzung</dc:title>
        <dc:title xml:lang="be">  Naamloze vennootschap met een sociaal oogmerk </dc:title>
        <dc:title xml:lang="en">Public limited company with a social purpose</dc:title>
        <dc:title xml:lang="be">Société anonyme à finalité sociale </dc:title>
        <rdfs:label rdf:datatype="http://www.w3.org/2001/XMLSchema#string">AGmsZ</rdfs:label>
        <rdfs:label rdf:datatype="http://www.w3.org/2001/XMLSchema#string">NVSO</rdfs:label>
        <rdfs:label rdf:datatype="http://www.w3.org/2001/XMLSchema#string">SAFS</rdfs:label>
    </owl:NamedIndividual>
    


    <!-- http://w3id.org/um/cbcm/eu-cm-ontology#be515 -->

    <owl:NamedIndividual rdf:about="http://w3id.org/um/cbcm/eu-cm-ontology#be515">
        <rdf:type rdf:resource="http://w3id.org/um/cbcm/eu-cm-ontology#CompanyLegalForm"/>
        <dc:title xml:lang="be">  Besloten vennootschap met beperkte aansprakelijkheid met een sociaal oogmerk </dc:title>
        <dc:title xml:lang="be">  Privatgesellschaft mit beschränkter Haftung mit sozialer Zielsetzung</dc:title>
        <dc:title xml:lang="en">Private limited liability company with a social purpose</dc:title>
        <dc:title xml:lang="be">Société privée à responsabilité limitée à finalité sociale </dc:title>
        <rdfs:label rdf:datatype="http://www.w3.org/2001/XMLSchema#string">BVBASO</rdfs:label>
        <rdfs:label rdf:datatype="http://www.w3.org/2001/XMLSchema#string">PmbHsZ</rdfs:label>
        <rdfs:label rdf:datatype="http://www.w3.org/2001/XMLSchema#string">SPRLFS</rdfs:label>
    </owl:NamedIndividual>
    


    <!-- http://w3id.org/um/cbcm/eu-cm-ontology#be560 -->

    <owl:NamedIndividual rdf:about="http://w3id.org/um/cbcm/eu-cm-ontology#be560">
        <rdf:type rdf:resource="http://w3id.org/um/cbcm/eu-cm-ontology#CompanyLegalForm"/>
        <dc:title xml:lang="be">  Economisch samenwerkingsverband met een sociaal oogmerk </dc:title>
        <dc:title xml:lang="be">  Wirtschaftliche Interessenvereinigung mit sozialer Zielsetzung</dc:title>
        <dc:title xml:lang="en">Economic interest grouping with a social purpose</dc:title>
        <dc:title xml:lang="be">Groupement dintérêt économique à finalité sociale </dc:title>
        <rdfs:label rdf:datatype="http://www.w3.org/2001/XMLSchema#string">ESVSO</rdfs:label>
        <rdfs:label rdf:datatype="http://www.w3.org/2001/XMLSchema#string">GIEFS</rdfs:label>
        <rdfs:label rdf:datatype="http://www.w3.org/2001/XMLSchema#string">WIVmsZ</rdfs:label>
    </owl:NamedIndividual>
    


    <!-- http://w3id.org/um/cbcm/eu-cm-ontology#be610 -->

    <owl:NamedIndividual rdf:about="http://w3id.org/um/cbcm/eu-cm-ontology#be610">
        <rdf:type rdf:resource="http://w3id.org/um/cbcm/eu-cm-ontology#CompanyLegalForm"/>
        <dc:title xml:lang="be">  Besloten Vennootschap </dc:title>
        <dc:title xml:lang="be">  Gesellschaft mit beschränkter Haftung</dc:title>
        <dc:title xml:lang="en">Limited liability company</dc:title>
        <dc:title xml:lang="be">Société à responsabilité limitée </dc:title>
        <rdfs:label rdf:datatype="http://www.w3.org/2001/XMLSchema#string">BV</rdfs:label>
        <rdfs:label rdf:datatype="http://www.w3.org/2001/XMLSchema#string">GmbH</rdfs:label>
        <rdfs:label rdf:datatype="http://www.w3.org/2001/XMLSchema#string">SRL</rdfs:label>
    </owl:NamedIndividual>
    


    <!-- http://w3id.org/um/cbcm/eu-cm-ontology#be612 -->

    <owl:NamedIndividual rdf:about="http://w3id.org/um/cbcm/eu-cm-ontology#be612">
        <rdf:type rdf:resource="http://w3id.org/um/cbcm/eu-cm-ontology#CompanyLegalForm"/>
        <dc:title xml:lang="be">  Commanditaire vennootschap </dc:title>
        <dc:title xml:lang="be">  Kommanditgesellschaft</dc:title>
        <dc:title xml:lang="en">Limited partnership</dc:title>
        <dc:title xml:lang="be">Société en commandite </dc:title>
        <rdfs:label rdf:datatype="http://www.w3.org/2001/XMLSchema#string">CommV</rdfs:label>
        <rdfs:label rdf:datatype="http://www.w3.org/2001/XMLSchema#string">KommG</rdfs:label>
        <rdfs:label rdf:datatype="http://www.w3.org/2001/XMLSchema#string">SComm</rdfs:label>
    </owl:NamedIndividual>
    


    <!-- http://w3id.org/um/cbcm/eu-cm-ontology#be616 -->

    <owl:NamedIndividual rdf:about="http://w3id.org/um/cbcm/eu-cm-ontology#be616">
        <rdf:type rdf:resource="http://w3id.org/um/cbcm/eu-cm-ontology#CompanyLegalForm"/>
        <dc:title xml:lang="be">  Besloten Vennootschap van publiek recht </dc:title>
        <dc:title xml:lang="be">  Öffentlich-rechtliche Gesellschaft mit beschränkter Haftung</dc:title>
        <dc:title xml:lang="en"> governed by public law</dc:title>
        <dc:title xml:lang="en">Limited liability company</dc:title>
        <dc:title xml:lang="be">Société à responsabilité limitée de droit public </dc:title>
        <rdfs:label rdf:datatype="http://www.w3.org/2001/XMLSchema#string">BVPR</rdfs:label>
        <rdfs:label rdf:datatype="http://www.w3.org/2001/XMLSchema#string">SRLDPU</rdfs:label>
        <rdfs:label rdf:datatype="http://www.w3.org/2001/XMLSchema#string">ÖrGmbH</rdfs:label>
    </owl:NamedIndividual>
    


    <!-- http://w3id.org/um/cbcm/eu-cm-ontology#be617 -->

    <owl:NamedIndividual rdf:about="http://w3id.org/um/cbcm/eu-cm-ontology#be617">
        <rdf:type rdf:resource="http://w3id.org/um/cbcm/eu-cm-ontology#CompanyLegalForm"/>
        <dc:title xml:lang="be">  Commanditaire vennootschap van publiek recht </dc:title>
        <dc:title xml:lang="be">  Öffentlich-rechtliche Kommanditgesellschaft</dc:title>
        <dc:title xml:lang="en"> governed by public law</dc:title>
        <dc:title xml:lang="en">Limited partnership</dc:title>
        <dc:title xml:lang="be">Société en commandite de droit public </dc:title>
        <rdfs:label rdf:datatype="http://www.w3.org/2001/XMLSchema#string">CommVPR</rdfs:label>
        <rdfs:label rdf:datatype="http://www.w3.org/2001/XMLSchema#string">SCommDPU</rdfs:label>
        <rdfs:label rdf:datatype="http://www.w3.org/2001/XMLSchema#string">ÖrKommG</rdfs:label>
    </owl:NamedIndividual>
    


    <!-- http://w3id.org/um/cbcm/eu-cm-ontology#be651 -->

    <owl:NamedIndividual rdf:about="http://w3id.org/um/cbcm/eu-cm-ontology#be651">
        <rdf:type rdf:resource="http://w3id.org/um/cbcm/eu-cm-ontology#CompanyLegalForm"/>
        <dc:title xml:lang="be">  Andere vorm met een sociaal oogmerk van publiek recht </dc:title>
        <dc:title xml:lang="be">  Andere öffentlich-rechtliche Rechtsform mit sozialer Zielsetzung</dc:title>
        <dc:title xml:lang="en"> governed by public law</dc:title>
        <dc:title xml:lang="be">Autre forme à finalité sociale de droit public </dc:title>
        <dc:title xml:lang="en">Other form with a social purpose</dc:title>
        <rdfs:label rdf:datatype="http://www.w3.org/2001/XMLSchema#string">FORMEFS</rdfs:label>
        <rdfs:label rdf:datatype="http://www.w3.org/2001/XMLSchema#string">RFmsZ</rdfs:label>
        <rdfs:label rdf:datatype="http://www.w3.org/2001/XMLSchema#string">VORMSO</rdfs:label>
    </owl:NamedIndividual>
    


    <!-- http://w3id.org/um/cbcm/eu-cm-ontology#be702 -->

    <owl:NamedIndividual rdf:about="http://w3id.org/um/cbcm/eu-cm-ontology#be702">
        <rdf:type rdf:resource="http://w3id.org/um/cbcm/eu-cm-ontology#CompanyLegalForm"/>
        <dc:title xml:lang="be">  Gesellschaft des allgemeinen Rechts</dc:title>
        <dc:title xml:lang="be">  Maatschap </dc:title>
        <dc:title xml:lang="en">Partnership</dc:title>
        <dc:title xml:lang="be">Société de droit commun </dc:title>
        <rdfs:label rdf:datatype="http://www.w3.org/2001/XMLSchema#string">GaR</rdfs:label>
        <rdfs:label rdf:datatype="http://www.w3.org/2001/XMLSchema#string">MS</rdfs:label>
        <rdfs:label rdf:datatype="http://www.w3.org/2001/XMLSchema#string">SDC</rdfs:label>
    </owl:NamedIndividual>
    


    <!-- http://w3id.org/um/cbcm/eu-cm-ontology#be706 -->

    <owl:NamedIndividual rdf:about="http://w3id.org/um/cbcm/eu-cm-ontology#be706">
        <rdf:type rdf:resource="http://w3id.org/um/cbcm/eu-cm-ontology#CompanyLegalForm"/>
        <dc:title xml:lang="be">   Coöperatieve vennootschap </dc:title>
        <dc:title xml:lang="be">  Genossenschaft</dc:title>
        <dc:title xml:lang="en">Cooperative partnership</dc:title>
        <dc:title xml:lang="be">Société coopérative </dc:title>
        <rdfs:label rdf:datatype="http://www.w3.org/2001/XMLSchema#string">CV</rdfs:label>
        <rdfs:label rdf:datatype="http://www.w3.org/2001/XMLSchema#string">Gen</rdfs:label>
        <rdfs:label rdf:datatype="http://www.w3.org/2001/XMLSchema#string">SC</rdfs:label>
    </owl:NamedIndividual>
    


    <!-- http://w3id.org/um/cbcm/eu-cm-ontology#be716 -->

    <owl:NamedIndividual rdf:about="http://w3id.org/um/cbcm/eu-cm-ontology#be716">
        <rdf:type rdf:resource="http://w3id.org/um/cbcm/eu-cm-ontology#CompanyLegalForm"/>
        <dc:title xml:lang="be">  Coöperatieve vennootschap van publiek recht </dc:title>
        <dc:title xml:lang="be">  Öffentlich rechtliche Genossenschaft</dc:title>
        <dc:title xml:lang="en"> governed by public law</dc:title>
        <dc:title xml:lang="en">Cooperative partnership</dc:title>
        <dc:title xml:lang="be">Société coopérative de droit public </dc:title>
        <rdfs:label rdf:datatype="http://www.w3.org/2001/XMLSchema#string">CVPR</rdfs:label>
        <rdfs:label rdf:datatype="http://www.w3.org/2001/XMLSchema#string">SCDPU</rdfs:label>
        <rdfs:label rdf:datatype="http://www.w3.org/2001/XMLSchema#string">ÖrGen</rdfs:label>
    </owl:NamedIndividual>
    


    <!-- http://w3id.org/um/cbcm/eu-cm-ontology#be721 -->

    <owl:NamedIndividual rdf:about="http://w3id.org/um/cbcm/eu-cm-ontology#be721">
        <rdf:type rdf:resource="http://w3id.org/um/cbcm/eu-cm-ontology#CompanyLegalForm"/>
        <dc:title xml:lang="be">  Gesellschaften oder Vereinigungen ohne Rechtspersönlichkeit</dc:title>
        <dc:title xml:lang="be">  Vennootschap of vereniging zonder rechtspersoonlijkheid </dc:title>
        <dc:title xml:lang="en">Company or association without legal personality</dc:title>
        <dc:title xml:lang="be">Société ou association sans personnalité juridique </dc:title>
        <rdfs:label rdf:datatype="http://www.w3.org/2001/XMLSchema#string">GVoRP</rdfs:label>
        <rdfs:label rdf:datatype="http://www.w3.org/2001/XMLSchema#string">SASPJ</rdfs:label>
        <rdfs:label rdf:datatype="http://www.w3.org/2001/XMLSchema#string">VVZRL</rdfs:label>
    </owl:NamedIndividual>
    


    <!-- http://w3id.org/um/cbcm/eu-cm-ontology#belgium -->

    <owl:NamedIndividual rdf:about="http://w3id.org/um/cbcm/eu-cm-ontology#belgium">
        <rdf:type rdf:resource="http://w3id.org/um/cbcm/eu-cm-ontology#EUCountry"/>
        <cbcm:countryHasCompanyForm rdf:resource="http://w3id.org/um/cbcm/eu-cm-ontology#be000"/>
        <cbcm:countryHasCompanyForm rdf:resource="http://w3id.org/um/cbcm/eu-cm-ontology#be002"/>
        <cbcm:countryHasCompanyForm rdf:resource="http://w3id.org/um/cbcm/eu-cm-ontology#be003"/>
        <cbcm:countryHasCompanyForm rdf:resource="http://w3id.org/um/cbcm/eu-cm-ontology#be006"/>
        <cbcm:countryHasCompanyForm rdf:resource="http://w3id.org/um/cbcm/eu-cm-ontology#be008"/>
        <cbcm:countryHasCompanyForm rdf:resource="http://w3id.org/um/cbcm/eu-cm-ontology#be011"/>
        <cbcm:countryHasCompanyForm rdf:resource="http://w3id.org/um/cbcm/eu-cm-ontology#be012"/>
        <cbcm:countryHasCompanyForm rdf:resource="http://w3id.org/um/cbcm/eu-cm-ontology#be013"/>
        <cbcm:countryHasCompanyForm rdf:resource="http://w3id.org/um/cbcm/eu-cm-ontology#be014"/>
        <cbcm:countryHasCompanyForm rdf:resource="http://w3id.org/um/cbcm/eu-cm-ontology#be015"/>
        <cbcm:countryHasCompanyForm rdf:resource="http://w3id.org/um/cbcm/eu-cm-ontology#be017"/>
        <cbcm:countryHasCompanyForm rdf:resource="http://w3id.org/um/cbcm/eu-cm-ontology#be019"/>
        <cbcm:countryHasCompanyForm rdf:resource="http://w3id.org/um/cbcm/eu-cm-ontology#be020"/>
        <cbcm:countryHasCompanyForm rdf:resource="http://w3id.org/um/cbcm/eu-cm-ontology#be021"/>
        <cbcm:countryHasCompanyForm rdf:resource="http://w3id.org/um/cbcm/eu-cm-ontology#be025"/>
        <cbcm:countryHasCompanyForm rdf:resource="http://w3id.org/um/cbcm/eu-cm-ontology#be026"/>
        <cbcm:countryHasCompanyForm rdf:resource="http://w3id.org/um/cbcm/eu-cm-ontology#be028"/>
        <cbcm:countryHasCompanyForm rdf:resource="http://w3id.org/um/cbcm/eu-cm-ontology#be029"/>
        <cbcm:countryHasCompanyForm rdf:resource="http://w3id.org/um/cbcm/eu-cm-ontology#be051"/>
        <cbcm:countryHasCompanyForm rdf:resource="http://w3id.org/um/cbcm/eu-cm-ontology#be060"/>
        <cbcm:countryHasCompanyForm rdf:resource="http://w3id.org/um/cbcm/eu-cm-ontology#be070"/>
        <cbcm:countryHasCompanyForm rdf:resource="http://w3id.org/um/cbcm/eu-cm-ontology#be107"/>
        <cbcm:countryHasCompanyForm rdf:resource="http://w3id.org/um/cbcm/eu-cm-ontology#be108"/>
        <cbcm:countryHasCompanyForm rdf:resource="http://w3id.org/um/cbcm/eu-cm-ontology#be114"/>
        <cbcm:countryHasCompanyForm rdf:resource="http://w3id.org/um/cbcm/eu-cm-ontology#be117"/>
        <cbcm:countryHasCompanyForm rdf:resource="http://w3id.org/um/cbcm/eu-cm-ontology#be121"/>
        <cbcm:countryHasCompanyForm rdf:resource="http://w3id.org/um/cbcm/eu-cm-ontology#be124"/>
        <cbcm:countryHasCompanyForm rdf:resource="http://w3id.org/um/cbcm/eu-cm-ontology#be125"/>
        <cbcm:countryHasCompanyForm rdf:resource="http://w3id.org/um/cbcm/eu-cm-ontology#be127"/>
        <cbcm:countryHasCompanyForm rdf:resource="http://w3id.org/um/cbcm/eu-cm-ontology#be129"/>
        <cbcm:countryHasCompanyForm rdf:resource="http://w3id.org/um/cbcm/eu-cm-ontology#be151"/>
        <cbcm:countryHasCompanyForm rdf:resource="http://w3id.org/um/cbcm/eu-cm-ontology#be200"/>
        <cbcm:countryHasCompanyForm rdf:resource="http://w3id.org/um/cbcm/eu-cm-ontology#be206"/>
        <cbcm:countryHasCompanyForm rdf:resource="http://w3id.org/um/cbcm/eu-cm-ontology#be208"/>
        <cbcm:countryHasCompanyForm rdf:resource="http://w3id.org/um/cbcm/eu-cm-ontology#be211"/>
        <cbcm:countryHasCompanyForm rdf:resource="http://w3id.org/um/cbcm/eu-cm-ontology#be212"/>
        <cbcm:countryHasCompanyForm rdf:resource="http://w3id.org/um/cbcm/eu-cm-ontology#be213"/>
        <cbcm:countryHasCompanyForm rdf:resource="http://w3id.org/um/cbcm/eu-cm-ontology#be214"/>
        <cbcm:countryHasCompanyForm rdf:resource="http://w3id.org/um/cbcm/eu-cm-ontology#be215"/>
        <cbcm:countryHasCompanyForm rdf:resource="http://w3id.org/um/cbcm/eu-cm-ontology#be217"/>
        <cbcm:countryHasCompanyForm rdf:resource="http://w3id.org/um/cbcm/eu-cm-ontology#be218"/>
        <cbcm:countryHasCompanyForm rdf:resource="http://w3id.org/um/cbcm/eu-cm-ontology#be225"/>
        <cbcm:countryHasCompanyForm rdf:resource="http://w3id.org/um/cbcm/eu-cm-ontology#be301"/>
        <cbcm:countryHasCompanyForm rdf:resource="http://w3id.org/um/cbcm/eu-cm-ontology#be302"/>
        <cbcm:countryHasCompanyForm rdf:resource="http://w3id.org/um/cbcm/eu-cm-ontology#be303"/>
        <cbcm:countryHasCompanyForm rdf:resource="http://w3id.org/um/cbcm/eu-cm-ontology#be310"/>
        <cbcm:countryHasCompanyForm rdf:resource="http://w3id.org/um/cbcm/eu-cm-ontology#be320"/>
        <cbcm:countryHasCompanyForm rdf:resource="http://w3id.org/um/cbcm/eu-cm-ontology#be325"/>
        <cbcm:countryHasCompanyForm rdf:resource="http://w3id.org/um/cbcm/eu-cm-ontology#be330"/>
        <cbcm:countryHasCompanyForm rdf:resource="http://w3id.org/um/cbcm/eu-cm-ontology#be340"/>
        <cbcm:countryHasCompanyForm rdf:resource="http://w3id.org/um/cbcm/eu-cm-ontology#be350"/>
        <cbcm:countryHasCompanyForm rdf:resource="http://w3id.org/um/cbcm/eu-cm-ontology#be400"/>
        <cbcm:countryHasCompanyForm rdf:resource="http://w3id.org/um/cbcm/eu-cm-ontology#be411"/>
        <cbcm:countryHasCompanyForm rdf:resource="http://w3id.org/um/cbcm/eu-cm-ontology#be412"/>
        <cbcm:countryHasCompanyForm rdf:resource="http://w3id.org/um/cbcm/eu-cm-ontology#be413"/>
        <cbcm:countryHasCompanyForm rdf:resource="http://w3id.org/um/cbcm/eu-cm-ontology#be414"/>
        <cbcm:countryHasCompanyForm rdf:resource="http://w3id.org/um/cbcm/eu-cm-ontology#be415"/>
        <cbcm:countryHasCompanyForm rdf:resource="http://w3id.org/um/cbcm/eu-cm-ontology#be416"/>
        <cbcm:countryHasCompanyForm rdf:resource="http://w3id.org/um/cbcm/eu-cm-ontology#be417"/>
        <cbcm:countryHasCompanyForm rdf:resource="http://w3id.org/um/cbcm/eu-cm-ontology#be418"/>
        <cbcm:countryHasCompanyForm rdf:resource="http://w3id.org/um/cbcm/eu-cm-ontology#be419"/>
        <cbcm:countryHasCompanyForm rdf:resource="http://w3id.org/um/cbcm/eu-cm-ontology#be420"/>
        <cbcm:countryHasCompanyForm rdf:resource="http://w3id.org/um/cbcm/eu-cm-ontology#be422"/>
        <cbcm:countryHasCompanyForm rdf:resource="http://w3id.org/um/cbcm/eu-cm-ontology#be506"/>
        <cbcm:countryHasCompanyForm rdf:resource="http://w3id.org/um/cbcm/eu-cm-ontology#be508"/>
        <cbcm:countryHasCompanyForm rdf:resource="http://w3id.org/um/cbcm/eu-cm-ontology#be511"/>
        <cbcm:countryHasCompanyForm rdf:resource="http://w3id.org/um/cbcm/eu-cm-ontology#be512"/>
        <cbcm:countryHasCompanyForm rdf:resource="http://w3id.org/um/cbcm/eu-cm-ontology#be513"/>
        <cbcm:countryHasCompanyForm rdf:resource="http://w3id.org/um/cbcm/eu-cm-ontology#be514"/>
        <cbcm:countryHasCompanyForm rdf:resource="http://w3id.org/um/cbcm/eu-cm-ontology#be515"/>
        <cbcm:countryHasCompanyForm rdf:resource="http://w3id.org/um/cbcm/eu-cm-ontology#be560"/>
        <cbcm:countryHasCompanyForm rdf:resource="http://w3id.org/um/cbcm/eu-cm-ontology#be610"/>
        <cbcm:countryHasCompanyForm rdf:resource="http://w3id.org/um/cbcm/eu-cm-ontology#be612"/>
        <cbcm:countryHasCompanyForm rdf:resource="http://w3id.org/um/cbcm/eu-cm-ontology#be616"/>
        <cbcm:countryHasCompanyForm rdf:resource="http://w3id.org/um/cbcm/eu-cm-ontology#be617"/>
        <cbcm:countryHasCompanyForm rdf:resource="http://w3id.org/um/cbcm/eu-cm-ontology#be651"/>
        <cbcm:countryHasCompanyForm rdf:resource="http://w3id.org/um/cbcm/eu-cm-ontology#be702"/>
        <cbcm:countryHasCompanyForm rdf:resource="http://w3id.org/um/cbcm/eu-cm-ontology#be706"/>
        <cbcm:countryHasCompanyForm rdf:resource="http://w3id.org/um/cbcm/eu-cm-ontology#be716"/>
        <cbcm:countryHasCompanyForm rdf:resource="http://w3id.org/um/cbcm/eu-cm-ontology#be721"/>
        <cbcm:iso2code>BE</cbcm:iso2code>
        <rdfs:label xml:lang="fr">Belgique</rdfs:label>
        <rdfs:label xml:lang="en">Belgium</rdfs:label>
    </owl:NamedIndividual>
    


    <!-- http://w3id.org/um/cbcm/eu-cm-ontology#bg101 -->

    <owl:NamedIndividual rdf:about="http://w3id.org/um/cbcm/eu-cm-ontology#bg101">
        <rdf:type rdf:resource="http://w3id.org/um/cbcm/eu-cm-ontology#CompanyLegalForm"/>
        <dc:title xml:lang="en">Joint-stock company</dc:title>
        <dc:title xml:lang="bg">Акционерно дружество (АД)</dc:title>
        <rdfs:label rdf:datatype="http://www.w3.org/2001/XMLSchema#string">AD</rdfs:label>
    </owl:NamedIndividual>
    


    <!-- http://w3id.org/um/cbcm/eu-cm-ontology#bg102 -->

    <owl:NamedIndividual rdf:about="http://w3id.org/um/cbcm/eu-cm-ontology#bg102">
        <rdf:type rdf:resource="http://w3id.org/um/cbcm/eu-cm-ontology#CompanyLegalForm"/>
        <dc:title xml:lang="en">Limited liability company</dc:title>
        <dc:title xml:lang="bg">Дружество с ограничена отговорност (ООД)</dc:title>
        <rdfs:label rdf:datatype="http://www.w3.org/2001/XMLSchema#string">OOD</rdfs:label>
    </owl:NamedIndividual>
    


    <!-- http://w3id.org/um/cbcm/eu-cm-ontology#bg103 -->

    <owl:NamedIndividual rdf:about="http://w3id.org/um/cbcm/eu-cm-ontology#bg103">
        <rdf:type rdf:resource="http://w3id.org/um/cbcm/eu-cm-ontology#CompanyLegalForm"/>
        <dc:title xml:lang="en">Partnership limited by shares</dc:title>
        <dc:title xml:lang="bg">Командиртно дружество с акции (КДА)</dc:title>
        <rdfs:label rdf:datatype="http://www.w3.org/2001/XMLSchema#string">KDA</rdfs:label>
    </owl:NamedIndividual>
    


    <!-- http://w3id.org/um/cbcm/eu-cm-ontology#bg104 -->

    <owl:NamedIndividual rdf:about="http://w3id.org/um/cbcm/eu-cm-ontology#bg104">
        <rdf:type rdf:resource="http://w3id.org/um/cbcm/eu-cm-ontology#CompanyLegalForm"/>
        <dc:title xml:lang="en">Single person joint-stock company</dc:title>
        <dc:title xml:lang="bg">Еднолично акционерно дружество (ЕАД)</dc:title>
        <rdfs:label rdf:datatype="http://www.w3.org/2001/XMLSchema#string">EAD</rdfs:label>
    </owl:NamedIndividual>
    


    <!-- http://w3id.org/um/cbcm/eu-cm-ontology#bg105 -->

    <owl:NamedIndividual rdf:about="http://w3id.org/um/cbcm/eu-cm-ontology#bg105">
        <rdf:type rdf:resource="http://w3id.org/um/cbcm/eu-cm-ontology#CompanyLegalForm"/>
        <dc:title xml:lang="en">Single person limited liability company</dc:title>
        <dc:title xml:lang="bg">Еднолично дружество с ограничена отговорност (ЕООД)</dc:title>
        <rdfs:label rdf:datatype="http://www.w3.org/2001/XMLSchema#string">EOOD</rdfs:label>
    </owl:NamedIndividual>
    


    <!-- http://w3id.org/um/cbcm/eu-cm-ontology#bg106 -->

    <owl:NamedIndividual rdf:about="http://w3id.org/um/cbcm/eu-cm-ontology#bg106">
        <rdf:type rdf:resource="http://w3id.org/um/cbcm/eu-cm-ontology#CompanyLegalForm"/>
        <dc:title xml:lang="en">Limited partnership</dc:title>
        <dc:title xml:lang="bg">Командиртно дружество (КД)</dc:title>
        <rdfs:label rdf:datatype="http://www.w3.org/2001/XMLSchema#string">KD</rdfs:label>
    </owl:NamedIndividual>
    


    <!-- http://w3id.org/um/cbcm/eu-cm-ontology#bg107 -->

    <owl:NamedIndividual rdf:about="http://w3id.org/um/cbcm/eu-cm-ontology#bg107">
        <rdf:type rdf:resource="http://w3id.org/um/cbcm/eu-cm-ontology#CompanyLegalForm"/>
        <dc:title xml:lang="bg"> Съдружие (С-ие)</dc:title>
        <dc:title xml:lang="en">General partnership</dc:title>
        <dc:title xml:lang="bg">Събирателно дружество (СД)</dc:title>
        <rdfs:label rdf:datatype="http://www.w3.org/2001/XMLSchema#string">S-ie</rdfs:label>
        <rdfs:label rdf:datatype="http://www.w3.org/2001/XMLSchema#string">SD</rdfs:label>
    </owl:NamedIndividual>
    


    <!-- http://w3id.org/um/cbcm/eu-cm-ontology#bg1539 -->

    <owl:NamedIndividual rdf:about="http://w3id.org/um/cbcm/eu-cm-ontology#bg1539">
        <rdf:type rdf:resource="http://w3id.org/um/cbcm/eu-cm-ontology#CompanyLegalForm"/>
        <dc:title xml:lang="en">Joint-Stock Special Investment Company</dc:title>
        <dc:title xml:lang="bg">Акционерно дружество със специална инвестиционна цел (АДСИЦ)</dc:title>
        <rdfs:label rdf:datatype="http://www.w3.org/2001/XMLSchema#string">ADSIC</rdfs:label>
    </owl:NamedIndividual>
    


    <!-- http://w3id.org/um/cbcm/eu-cm-ontology#bg462 -->

    <owl:NamedIndividual rdf:about="http://w3id.org/um/cbcm/eu-cm-ontology#bg462">
        <rdf:type rdf:resource="http://w3id.org/um/cbcm/eu-cm-ontology#CompanyLegalForm"/>
        <dc:title xml:lang="en">Sole proprietor</dc:title>
        <dc:title xml:lang="bg">Едноличен търговец (ЕТ)</dc:title>
        <rdfs:label rdf:datatype="http://www.w3.org/2001/XMLSchema#string">ET</rdfs:label>
    </owl:NamedIndividual>
    


    <!-- http://w3id.org/um/cbcm/eu-cm-ontology#bg466 -->

    <owl:NamedIndividual rdf:about="http://w3id.org/um/cbcm/eu-cm-ontology#bg466">
        <rdf:type rdf:resource="http://w3id.org/um/cbcm/eu-cm-ontology#CompanyLegalForm"/>
        <dc:title xml:lang="en">Cooperation / Cooperative society</dc:title>
        <dc:title xml:lang="bg">Кооперация</dc:title>
        <rdfs:label rdf:datatype="http://www.w3.org/2001/XMLSchema#string">Coop</rdfs:label>
    </owl:NamedIndividual>
    


    <!-- http://w3id.org/um/cbcm/eu-cm-ontology#bg472 -->

    <owl:NamedIndividual rdf:about="http://w3id.org/um/cbcm/eu-cm-ontology#bg472">
        <rdf:type rdf:resource="http://w3id.org/um/cbcm/eu-cm-ontology#CompanyLegalForm"/>
        <dc:title xml:lang="en">Partnership by Law of Obligations And Contracts</dc:title>
        <dc:title xml:lang="bg">Дружество учредено по Закона за задълженията и договорите (ДЗЗД)</dc:title>
        <rdfs:label rdf:datatype="http://www.w3.org/2001/XMLSchema#string">DZZD</rdfs:label>
    </owl:NamedIndividual>
    


    <!-- http://w3id.org/um/cbcm/eu-cm-ontology#bulgaria -->

    <owl:NamedIndividual rdf:about="http://w3id.org/um/cbcm/eu-cm-ontology#bulgaria">
        <rdf:type rdf:resource="http://w3id.org/um/cbcm/eu-cm-ontology#EUCountry"/>
        <cbcm:countryHasCompanyForm rdf:resource="http://w3id.org/um/cbcm/eu-cm-ontology#bg101"/>
        <cbcm:countryHasCompanyForm rdf:resource="http://w3id.org/um/cbcm/eu-cm-ontology#bg102"/>
        <cbcm:countryHasCompanyForm rdf:resource="http://w3id.org/um/cbcm/eu-cm-ontology#bg103"/>
        <cbcm:countryHasCompanyForm rdf:resource="http://w3id.org/um/cbcm/eu-cm-ontology#bg104"/>
        <cbcm:countryHasCompanyForm rdf:resource="http://w3id.org/um/cbcm/eu-cm-ontology#bg105"/>
        <cbcm:countryHasCompanyForm rdf:resource="http://w3id.org/um/cbcm/eu-cm-ontology#bg106"/>
        <cbcm:countryHasCompanyForm rdf:resource="http://w3id.org/um/cbcm/eu-cm-ontology#bg107"/>
        <cbcm:countryHasCompanyForm rdf:resource="http://w3id.org/um/cbcm/eu-cm-ontology#bg1539"/>
        <cbcm:countryHasCompanyForm rdf:resource="http://w3id.org/um/cbcm/eu-cm-ontology#bg462"/>
        <cbcm:countryHasCompanyForm rdf:resource="http://w3id.org/um/cbcm/eu-cm-ontology#bg466"/>
        <cbcm:countryHasCompanyForm rdf:resource="http://w3id.org/um/cbcm/eu-cm-ontology#bg472"/>
        <cbcm:iso2code>BG</cbcm:iso2code>
        <rdfs:label xml:lang="en">Bulgaria</rdfs:label>
        <rdfs:label xml:lang="bg">Bǎlgariya</rdfs:label>
        <rdfs:label xml:lang="bg">България</rdfs:label>
    </owl:NamedIndividual>
    


    <!-- http://w3id.org/um/cbcm/eu-cm-ontology#croatia -->

    <owl:NamedIndividual rdf:about="http://w3id.org/um/cbcm/eu-cm-ontology#croatia">
        <rdf:type rdf:resource="http://w3id.org/um/cbcm/eu-cm-ontology#EUCountry"/>
        <cbcm:countryHasCompanyForm rdf:resource="http://w3id.org/um/cbcm/eu-cm-ontology#hr01"/>
        <cbcm:countryHasCompanyForm rdf:resource="http://w3id.org/um/cbcm/eu-cm-ontology#hr02"/>
        <cbcm:countryHasCompanyForm rdf:resource="http://w3id.org/um/cbcm/eu-cm-ontology#hr03"/>
        <cbcm:countryHasCompanyForm rdf:resource="http://w3id.org/um/cbcm/eu-cm-ontology#hr04"/>
        <cbcm:countryHasCompanyForm rdf:resource="http://w3id.org/um/cbcm/eu-cm-ontology#hr08"/>
        <cbcm:countryHasCompanyForm rdf:resource="http://w3id.org/um/cbcm/eu-cm-ontology#hr16"/>
        <cbcm:countryHasCompanyForm rdf:resource="http://w3id.org/um/cbcm/eu-cm-ontology#hr45"/>
        <cbcm:iso2code>HR</cbcm:iso2code>
        <rdfs:label xml:lang="en">Croatia</rdfs:label>
        <rdfs:label xml:lang="hr">Hrvatska</rdfs:label>
    </owl:NamedIndividual>
    


    <!-- http://w3id.org/um/cbcm/eu-cm-ontology#cy102 -->

    <owl:NamedIndividual rdf:about="http://w3id.org/um/cbcm/eu-cm-ontology#cy102">
        <rdf:type rdf:resource="http://w3id.org/um/cbcm/eu-cm-ontology#CompanyLegalForm"/>
        <dc:title xml:lang="en">Private limited company / Ltd</dc:title>
        <dc:title xml:lang="cy">Ιδιωτική Εταιρεία</dc:title>
        <rdfs:label rdf:datatype="http://www.w3.org/2001/XMLSchema#string">LTD</rdfs:label>
    </owl:NamedIndividual>
    


    <!-- http://w3id.org/um/cbcm/eu-cm-ontology#cy103 -->

    <owl:NamedIndividual rdf:about="http://w3id.org/um/cbcm/eu-cm-ontology#cy103">
        <rdf:type rdf:resource="http://w3id.org/um/cbcm/eu-cm-ontology#CompanyLegalForm"/>
        <dc:title xml:lang="en">Public limited company / Plc</dc:title>
        <dc:title xml:lang="cy">Δημόσια Εταιρεία</dc:title>
        <rdfs:label rdf:datatype="http://www.w3.org/2001/XMLSchema#string">PLC</rdfs:label>
    </owl:NamedIndividual>
    


    <!-- http://w3id.org/um/cbcm/eu-cm-ontology#cy109 -->

    <owl:NamedIndividual rdf:about="http://w3id.org/um/cbcm/eu-cm-ontology#cy109">
        <rdf:type rdf:resource="http://w3id.org/um/cbcm/eu-cm-ontology#CompanyLegalForm"/>
        <dc:title xml:lang="en">Partnership</dc:title>
        <dc:title xml:lang="cy">Συνεταιρισμός </dc:title>
        <rdfs:label rdf:datatype="http://www.w3.org/2001/XMLSchema#string">P</rdfs:label>
    </owl:NamedIndividual>
    


    <!-- http://w3id.org/um/cbcm/eu-cm-ontology#cy111 -->

    <owl:NamedIndividual rdf:about="http://w3id.org/um/cbcm/eu-cm-ontology#cy111">
        <rdf:type rdf:resource="http://w3id.org/um/cbcm/eu-cm-ontology#CompanyLegalForm"/>
        <dc:title xml:lang="en">Cooperative Credit Societies</dc:title>
        <dc:title xml:lang="cy">Συνεργατικά Πιστωτικά Ιδρύματα </dc:title>
        <rdfs:label rdf:datatype="http://www.w3.org/2001/XMLSchema#string">COOP</rdfs:label>
    </owl:NamedIndividual>
    


    <!-- http://w3id.org/um/cbcm/eu-cm-ontology#cy112 -->

    <owl:NamedIndividual rdf:about="http://w3id.org/um/cbcm/eu-cm-ontology#cy112">
        <rdf:type rdf:resource="http://w3id.org/um/cbcm/eu-cm-ontology#CompanyLegalForm"/>
        <dc:title xml:lang="en">Sole proprietorship</dc:title>
        <dc:title xml:lang="cy">Αυτοτελώς εργαζόμενος</dc:title>
        <rdfs:label rdf:datatype="http://www.w3.org/2001/XMLSchema#string">SP</rdfs:label>
    </owl:NamedIndividual>
    


    <!-- http://w3id.org/um/cbcm/eu-cm-ontology#cy113 -->

    <owl:NamedIndividual rdf:about="http://w3id.org/um/cbcm/eu-cm-ontology#cy113">
        <rdf:type rdf:resource="http://w3id.org/um/cbcm/eu-cm-ontology#CompanyLegalForm"/>
        <dc:title xml:lang="en">Societies &amp; Foundations</dc:title>
        <dc:title xml:lang="cy">Σωματεία και Ιδρυμάτα </dc:title>
        <rdfs:label rdf:datatype="http://www.w3.org/2001/XMLSchema#string">SF</rdfs:label>
    </owl:NamedIndividual>
    


    <!-- http://w3id.org/um/cbcm/eu-cm-ontology#cy114 -->

    <owl:NamedIndividual rdf:about="http://w3id.org/um/cbcm/eu-cm-ontology#cy114">
        <rdf:type rdf:resource="http://w3id.org/um/cbcm/eu-cm-ontology#CompanyLegalForm"/>
        <dc:title xml:lang="en">Entities governed by public law</dc:title>
        <dc:title xml:lang="cy">Οντότητες που διέπονται από το δημόσιο δίκαιο</dc:title>
        <rdfs:label rdf:datatype="http://www.w3.org/2001/XMLSchema#string">PUBLaw</rdfs:label>
    </owl:NamedIndividual>
    


    <!-- http://w3id.org/um/cbcm/eu-cm-ontology#cy116 -->

    <owl:NamedIndividual rdf:about="http://w3id.org/um/cbcm/eu-cm-ontology#cy116">
        <rdf:type rdf:resource="http://w3id.org/um/cbcm/eu-cm-ontology#CompanyLegalForm"/>
        <dc:title xml:lang="cy">  Συντάξεως</dc:title>
        <dc:title xml:lang="en">Pension / Provident Funds</dc:title>
        <dc:title xml:lang="cy">Ταμεία Προνοίας</dc:title>
        <rdfs:label rdf:datatype="http://www.w3.org/2001/XMLSchema#string">PF</rdfs:label>
    </owl:NamedIndividual>
    


    <!-- http://w3id.org/um/cbcm/eu-cm-ontology#cy117 -->

    <owl:NamedIndividual rdf:about="http://w3id.org/um/cbcm/eu-cm-ontology#cy117">
        <rdf:type rdf:resource="http://w3id.org/um/cbcm/eu-cm-ontology#CompanyLegalForm"/>
        <dc:title xml:lang="en">Other legal form</dc:title>
        <dc:title xml:lang="cy">Άλλη νομική μορφή</dc:title>
        <rdfs:label rdf:datatype="http://www.w3.org/2001/XMLSchema#string">OTH</rdfs:label>
    </owl:NamedIndividual>
    


    <!-- http://w3id.org/um/cbcm/eu-cm-ontology#cyprus -->

    <owl:NamedIndividual rdf:about="http://w3id.org/um/cbcm/eu-cm-ontology#cyprus">
        <rdf:type rdf:resource="http://w3id.org/um/cbcm/eu-cm-ontology#EUCountry"/>
        <cbcm:countryHasCompanyForm rdf:resource="http://w3id.org/um/cbcm/eu-cm-ontology#cy102"/>
        <cbcm:countryHasCompanyForm rdf:resource="http://w3id.org/um/cbcm/eu-cm-ontology#cy103"/>
        <cbcm:countryHasCompanyForm rdf:resource="http://w3id.org/um/cbcm/eu-cm-ontology#cy109"/>
        <cbcm:countryHasCompanyForm rdf:resource="http://w3id.org/um/cbcm/eu-cm-ontology#cy111"/>
        <cbcm:countryHasCompanyForm rdf:resource="http://w3id.org/um/cbcm/eu-cm-ontology#cy112"/>
        <cbcm:countryHasCompanyForm rdf:resource="http://w3id.org/um/cbcm/eu-cm-ontology#cy113"/>
        <cbcm:countryHasCompanyForm rdf:resource="http://w3id.org/um/cbcm/eu-cm-ontology#cy114"/>
        <cbcm:countryHasCompanyForm rdf:resource="http://w3id.org/um/cbcm/eu-cm-ontology#cy116"/>
        <cbcm:countryHasCompanyForm rdf:resource="http://w3id.org/um/cbcm/eu-cm-ontology#cy117"/>
        <cbcm:iso2code>CY</cbcm:iso2code>
        <rdfs:label xml:lang="en">Cyprus</rdfs:label>
    </owl:NamedIndividual>
    


    <!-- http://w3id.org/um/cbcm/eu-cm-ontology#cz111 -->

    <owl:NamedIndividual rdf:about="http://w3id.org/um/cbcm/eu-cm-ontology#cz111">
        <rdf:type rdf:resource="http://w3id.org/um/cbcm/eu-cm-ontology#CompanyLegalForm"/>
        <dc:title xml:lang="en">General partnership</dc:title>
        <dc:title xml:lang="cz">Veřejná obchodní společnost</dc:title>
        <rdfs:label rdf:datatype="http://www.w3.org/2001/XMLSchema#string">v.o.s.</rdfs:label>
    </owl:NamedIndividual>
    


    <!-- http://w3id.org/um/cbcm/eu-cm-ontology#cz112 -->

    <owl:NamedIndividual rdf:about="http://w3id.org/um/cbcm/eu-cm-ontology#cz112">
        <rdf:type rdf:resource="http://w3id.org/um/cbcm/eu-cm-ontology#CompanyLegalForm"/>
        <dc:title xml:lang="en">Ltd (UK)</dc:title>
        <dc:title xml:lang="cz">Společnost s ručením omezeným</dc:title>
        <rdfs:label rdf:datatype="http://www.w3.org/2001/XMLSchema#string">s.r.o.</rdfs:label>
    </owl:NamedIndividual>
    


    <!-- http://w3id.org/um/cbcm/eu-cm-ontology#cz113 -->

    <owl:NamedIndividual rdf:about="http://w3id.org/um/cbcm/eu-cm-ontology#cz113">
        <rdf:type rdf:resource="http://w3id.org/um/cbcm/eu-cm-ontology#CompanyLegalForm"/>
        <dc:title xml:lang="en">Limited partnership</dc:title>
        <dc:title xml:lang="cz">Společnost komanditní</dc:title>
        <rdfs:label rdf:datatype="http://www.w3.org/2001/XMLSchema#string">k.s.</rdfs:label>
    </owl:NamedIndividual>
    


    <!-- http://w3id.org/um/cbcm/eu-cm-ontology#cz121 -->

    <owl:NamedIndividual rdf:about="http://w3id.org/um/cbcm/eu-cm-ontology#cz121">
        <rdf:type rdf:resource="http://w3id.org/um/cbcm/eu-cm-ontology#CompanyLegalForm"/>
        <dc:title xml:lang="cz">Akciová společnost</dc:title>
        <dc:title xml:lang="en">Plc (UK)</dc:title>
        <rdfs:label rdf:datatype="http://www.w3.org/2001/XMLSchema#string">a.s.</rdfs:label>
    </owl:NamedIndividual>
    


    <!-- http://w3id.org/um/cbcm/eu-cm-ontology#cz141 -->

    <owl:NamedIndividual rdf:about="http://w3id.org/um/cbcm/eu-cm-ontology#cz141">
        <rdf:type rdf:resource="http://w3id.org/um/cbcm/eu-cm-ontology#CompanyLegalForm"/>
        <dc:title xml:lang="cz">Obecně prospěšná společnost</dc:title>
        <dc:title xml:lang="en">One of the legal forms for non-governmental non-profit organizations</dc:title>
        <rdfs:label rdf:datatype="http://www.w3.org/2001/XMLSchema#string">o.p.s.</rdfs:label>
    </owl:NamedIndividual>
    


    <!-- http://w3id.org/um/cbcm/eu-cm-ontology#cz145 -->

    <owl:NamedIndividual rdf:about="http://w3id.org/um/cbcm/eu-cm-ontology#cz145">
        <rdf:type rdf:resource="http://w3id.org/um/cbcm/eu-cm-ontology#CompanyLegalForm"/>
        <dc:title xml:lang="en">Owners’ association (apartment owners’ association)</dc:title>
        <dc:title xml:lang="cz">Společenství vlastníků jednotek</dc:title>
        <rdfs:label rdf:datatype="http://www.w3.org/2001/XMLSchema#string">svj</rdfs:label>
    </owl:NamedIndividual>
    


    <!-- http://w3id.org/um/cbcm/eu-cm-ontology#cz301 -->

    <owl:NamedIndividual rdf:about="http://w3id.org/um/cbcm/eu-cm-ontology#cz301">
        <rdf:type rdf:resource="http://w3id.org/um/cbcm/eu-cm-ontology#CompanyLegalForm"/>
        <dc:title xml:lang="en">State enterprise</dc:title>
        <dc:title xml:lang="cz">Státní podnik</dc:title>
        <rdfs:label rdf:datatype="http://www.w3.org/2001/XMLSchema#string">s.p.</rdfs:label>
    </owl:NamedIndividual>
    


    <!-- http://w3id.org/um/cbcm/eu-cm-ontology#czechia -->

    <owl:NamedIndividual rdf:about="http://w3id.org/um/cbcm/eu-cm-ontology#czechia">
        <rdf:type rdf:resource="http://w3id.org/um/cbcm/eu-cm-ontology#EUCountry"/>
        <cbcm:countryHasCompanyForm rdf:resource="http://w3id.org/um/cbcm/eu-cm-ontology#cz111"/>
        <cbcm:countryHasCompanyForm rdf:resource="http://w3id.org/um/cbcm/eu-cm-ontology#cz112"/>
        <cbcm:countryHasCompanyForm rdf:resource="http://w3id.org/um/cbcm/eu-cm-ontology#cz113"/>
        <cbcm:countryHasCompanyForm rdf:resource="http://w3id.org/um/cbcm/eu-cm-ontology#cz121"/>
        <cbcm:countryHasCompanyForm rdf:resource="http://w3id.org/um/cbcm/eu-cm-ontology#cz141"/>
        <cbcm:countryHasCompanyForm rdf:resource="http://w3id.org/um/cbcm/eu-cm-ontology#cz145"/>
        <cbcm:countryHasCompanyForm rdf:resource="http://w3id.org/um/cbcm/eu-cm-ontology#cz301"/>
        <cbcm:iso2code>CZ</cbcm:iso2code>
        <rdfs:label xml:lang="en">Czech Republic</rdfs:label>
        <rdfs:label xml:lang="en">Czechia</rdfs:label>
        <rdfs:label xml:lang="cz">Česká republika</rdfs:label>
    </owl:NamedIndividual>
    


    <!-- http://w3id.org/um/cbcm/eu-cm-ontology#de101 -->

    <owl:NamedIndividual rdf:about="http://w3id.org/um/cbcm/eu-cm-ontology#de101">
        <rdf:type rdf:resource="http://w3id.org/um/cbcm/eu-cm-ontology#CompanyLegalForm"/>
        <dc:title xml:lang="de">  BGB-Gesellschaft (Außen-GbR)</dc:title>
        <dc:title xml:lang="en"> recognisable as such to the public</dc:title>
        <dc:title xml:lang="de">Gesellschaft bürgerlichen Rechts </dc:title>
        <dc:title xml:lang="en">Partnership under civil law</dc:title>
        <rdfs:label rdf:datatype="http://www.w3.org/2001/XMLSchema#string">GbR</rdfs:label>
    </owl:NamedIndividual>
    


    <!-- http://w3id.org/um/cbcm/eu-cm-ontology#de102 -->

    <owl:NamedIndividual rdf:about="http://w3id.org/um/cbcm/eu-cm-ontology#de102">
        <rdf:type rdf:resource="http://w3id.org/um/cbcm/eu-cm-ontology#CompanyLegalForm"/>
        <dc:title xml:lang="en">General partnership</dc:title>
        <dc:title xml:lang="de">Offene Handelsgesellschaft</dc:title>
        <rdfs:label rdf:datatype="http://www.w3.org/2001/XMLSchema#string">OHG</rdfs:label>
    </owl:NamedIndividual>
    


    <!-- http://w3id.org/um/cbcm/eu-cm-ontology#de103 -->

    <owl:NamedIndividual rdf:about="http://w3id.org/um/cbcm/eu-cm-ontology#de103">
        <rdf:type rdf:resource="http://w3id.org/um/cbcm/eu-cm-ontology#CompanyLegalForm"/>
        <dc:title xml:lang="de">Kommanditgesellschaft</dc:title>
        <dc:title xml:lang="en">Limited partnership</dc:title>
        <rdfs:label rdf:datatype="http://www.w3.org/2001/XMLSchema#string">KG</rdfs:label>
    </owl:NamedIndividual>
    


    <!-- http://w3id.org/um/cbcm/eu-cm-ontology#de105 -->

    <owl:NamedIndividual rdf:about="http://w3id.org/um/cbcm/eu-cm-ontology#de105">
        <rdf:type rdf:resource="http://w3id.org/um/cbcm/eu-cm-ontology#CompanyLegalForm"/>
        <dc:title xml:lang="de">Partnerschaftsgesellschaft</dc:title>
        <dc:title xml:lang="en">Registered partnership company</dc:title>
        <rdfs:label rdf:datatype="http://www.w3.org/2001/XMLSchema#string">PartG</rdfs:label>
    </owl:NamedIndividual>
    


    <!-- http://w3id.org/um/cbcm/eu-cm-ontology#de108 -->

    <owl:NamedIndividual rdf:about="http://w3id.org/um/cbcm/eu-cm-ontology#de108">
        <rdf:type rdf:resource="http://w3id.org/um/cbcm/eu-cm-ontology#CompanyLegalForm"/>
        <dc:title xml:lang="de">Kommanditgesellschaft mit haftungsbeschränktem Komplementär</dc:title>
        <dc:title xml:lang="en">Limited partnership (fully limited) </dc:title>
        <rdfs:label rdf:datatype="http://www.w3.org/2001/XMLSchema#string">..&amp;Co.KG</rdfs:label>
    </owl:NamedIndividual>
    


    <!-- http://w3id.org/um/cbcm/eu-cm-ontology#de109 -->

    <owl:NamedIndividual rdf:about="http://w3id.org/um/cbcm/eu-cm-ontology#de109">
        <rdf:type rdf:resource="http://w3id.org/um/cbcm/eu-cm-ontology#CompanyLegalForm"/>
        <dc:title xml:lang="de">Kommanditgesellschaft auf Aktien mit haftungsbeschränktem Komplementär</dc:title>
        <dc:title xml:lang="en">Partnership limited by shares (fully lmited)</dc:title>
        <rdfs:label rdf:datatype="http://www.w3.org/2001/XMLSchema#string">..&amp;Co.KGaA</rdfs:label>
    </owl:NamedIndividual>
    


    <!-- http://w3id.org/um/cbcm/eu-cm-ontology#de110 -->

    <owl:NamedIndividual rdf:about="http://w3id.org/um/cbcm/eu-cm-ontology#de110">
        <rdf:type rdf:resource="http://w3id.org/um/cbcm/eu-cm-ontology#CompanyLegalForm"/>
        <dc:title xml:lang="en">General partnership (partially limited)</dc:title>
        <dc:title xml:lang="de">Offene Handelsgesellschaft mit haftungsbeschränktem Gesellschafter</dc:title>
        <rdfs:label rdf:datatype="http://www.w3.org/2001/XMLSchema#string">..&amp;Co.OHG</rdfs:label>
    </owl:NamedIndividual>
    


    <!-- http://w3id.org/um/cbcm/eu-cm-ontology#de201 -->

    <owl:NamedIndividual rdf:about="http://w3id.org/um/cbcm/eu-cm-ontology#de201">
        <rdf:type rdf:resource="http://w3id.org/um/cbcm/eu-cm-ontology#CompanyLegalForm"/>
        <dc:title xml:lang="de">Aktiengesellschaft</dc:title>
        <dc:title xml:lang="en">Public limited company</dc:title>
        <rdfs:label rdf:datatype="http://www.w3.org/2001/XMLSchema#string">AG</rdfs:label>
    </owl:NamedIndividual>
    


    <!-- http://w3id.org/um/cbcm/eu-cm-ontology#de202 -->

    <owl:NamedIndividual rdf:about="http://w3id.org/um/cbcm/eu-cm-ontology#de202">
        <rdf:type rdf:resource="http://w3id.org/um/cbcm/eu-cm-ontology#CompanyLegalForm"/>
        <dc:title xml:lang="de">Kommanditgesellschaft auf Aktien</dc:title>
        <dc:title xml:lang="en">Partnership limited by shares</dc:title>
        <rdfs:label rdf:datatype="http://www.w3.org/2001/XMLSchema#string">KGaA</rdfs:label>
    </owl:NamedIndividual>
    


    <!-- http://w3id.org/um/cbcm/eu-cm-ontology#de205 -->

    <owl:NamedIndividual rdf:about="http://w3id.org/um/cbcm/eu-cm-ontology#de205">
        <rdf:type rdf:resource="http://w3id.org/um/cbcm/eu-cm-ontology#CompanyLegalForm"/>
        <dc:title xml:lang="de">Investmentaktiengesellschaft</dc:title>
        <dc:title xml:lang="en">Public limited investment company</dc:title>
        <rdfs:label rdf:datatype="http://www.w3.org/2001/XMLSchema#string">InvAG</rdfs:label>
    </owl:NamedIndividual>
    


    <!-- http://w3id.org/um/cbcm/eu-cm-ontology#de206 -->

    <owl:NamedIndividual rdf:about="http://w3id.org/um/cbcm/eu-cm-ontology#de206">
        <rdf:type rdf:resource="http://w3id.org/um/cbcm/eu-cm-ontology#CompanyLegalForm"/>
        <dc:title xml:lang="de">Gesellschaft mit beschränkter Haftung</dc:title>
        <dc:title xml:lang="en">Private limited company</dc:title>
        <rdfs:label rdf:datatype="http://www.w3.org/2001/XMLSchema#string">GmbH</rdfs:label>
    </owl:NamedIndividual>
    


    <!-- http://w3id.org/um/cbcm/eu-cm-ontology#de207 -->

    <owl:NamedIndividual rdf:about="http://w3id.org/um/cbcm/eu-cm-ontology#de207">
        <rdf:type rdf:resource="http://w3id.org/um/cbcm/eu-cm-ontology#CompanyLegalForm"/>
        <dc:title xml:lang="en">Entrepreneurial company (limited liability)</dc:title>
        <dc:title xml:lang="de">Unternehmergesellschaft (haftungsbeschränkt)</dc:title>
        <rdfs:label rdf:datatype="http://www.w3.org/2001/XMLSchema#string">UG(haftungsbeschränkt)</rdfs:label>
    </owl:NamedIndividual>
    


    <!-- http://w3id.org/um/cbcm/eu-cm-ontology#de209 -->

    <owl:NamedIndividual rdf:about="http://w3id.org/um/cbcm/eu-cm-ontology#de209">
        <rdf:type rdf:resource="http://w3id.org/um/cbcm/eu-cm-ontology#CompanyLegalForm"/>
        <dc:title xml:lang="en">Registered association by charter </dc:title>
        <dc:title xml:lang="de">Wirtschaftlicher Verein</dc:title>
        <rdfs:label rdf:datatype="http://www.w3.org/2001/XMLSchema#string">wV</rdfs:label>
    </owl:NamedIndividual>
    


    <!-- http://w3id.org/um/cbcm/eu-cm-ontology#de211 -->

    <owl:NamedIndividual rdf:about="http://w3id.org/um/cbcm/eu-cm-ontology#de211">
        <rdf:type rdf:resource="http://w3id.org/um/cbcm/eu-cm-ontology#CompanyLegalForm"/>
        <dc:title xml:lang="de">Juristische Person alten hamburgischen Rechts</dc:title>
        <dc:title xml:lang="en">Legal entity under old Hamburg law</dc:title>
        <rdfs:label rdf:datatype="http://www.w3.org/2001/XMLSchema#string">JPahR</rdfs:label>
    </owl:NamedIndividual>
    


    <!-- http://w3id.org/um/cbcm/eu-cm-ontology#de301 -->

    <owl:NamedIndividual rdf:about="http://w3id.org/um/cbcm/eu-cm-ontology#de301">
        <rdf:type rdf:resource="http://w3id.org/um/cbcm/eu-cm-ontology#CompanyLegalForm"/>
        <dc:title xml:lang="de">Eingetragene Genossenschaft</dc:title>
        <dc:title xml:lang="en">Registered cooperative company</dc:title>
        <rdfs:label rdf:datatype="http://www.w3.org/2001/XMLSchema#string">eG</rdfs:label>
    </owl:NamedIndividual>
    


    <!-- http://w3id.org/um/cbcm/eu-cm-ontology#de401 -->

    <owl:NamedIndividual rdf:about="http://w3id.org/um/cbcm/eu-cm-ontology#de401">
        <rdf:type rdf:resource="http://w3id.org/um/cbcm/eu-cm-ontology#CompanyLegalForm"/>
        <dc:title xml:lang="en">Mutual insurance company</dc:title>
        <dc:title xml:lang="de">Versicherungsverein auf Gegenseitigkeit</dc:title>
        <rdfs:label rdf:datatype="http://www.w3.org/2001/XMLSchema#string">VVaG</rdfs:label>
    </owl:NamedIndividual>
    


    <!-- http://w3id.org/um/cbcm/eu-cm-ontology#de501 -->

    <owl:NamedIndividual rdf:about="http://w3id.org/um/cbcm/eu-cm-ontology#de501">
        <rdf:type rdf:resource="http://w3id.org/um/cbcm/eu-cm-ontology#CompanyLegalForm"/>
        <dc:title xml:lang="de">Gebietskörperschaft</dc:title>
        <dc:title xml:lang="en">Regional Authority</dc:title>
        <rdfs:label rdf:datatype="http://www.w3.org/2001/XMLSchema#string">G</rdfs:label>
    </owl:NamedIndividual>
    


    <!-- http://w3id.org/um/cbcm/eu-cm-ontology#de502 -->

    <owl:NamedIndividual rdf:about="http://w3id.org/um/cbcm/eu-cm-ontology#de502">
        <rdf:type rdf:resource="http://w3id.org/um/cbcm/eu-cm-ontology#CompanyLegalForm"/>
        <dc:title xml:lang="de">Anstalt des öffentlichen Rechts</dc:title>
        <dc:title xml:lang="en">Institution established under public law</dc:title>
        <rdfs:label rdf:datatype="http://www.w3.org/2001/XMLSchema#string">AöR</rdfs:label>
    </owl:NamedIndividual>
    


    <!-- http://w3id.org/um/cbcm/eu-cm-ontology#de503 -->

    <owl:NamedIndividual rdf:about="http://w3id.org/um/cbcm/eu-cm-ontology#de503">
        <rdf:type rdf:resource="http://w3id.org/um/cbcm/eu-cm-ontology#CompanyLegalForm"/>
        <dc:title xml:lang="de">Körperschaft des öffentlichen Rechts</dc:title>
        <dc:title xml:lang="en">Public body / statutory company</dc:title>
        <rdfs:label rdf:datatype="http://www.w3.org/2001/XMLSchema#string">KöR</rdfs:label>
    </owl:NamedIndividual>
    


    <!-- http://w3id.org/um/cbcm/eu-cm-ontology#de504 -->

    <owl:NamedIndividual rdf:about="http://w3id.org/um/cbcm/eu-cm-ontology#de504">
        <rdf:type rdf:resource="http://w3id.org/um/cbcm/eu-cm-ontology#CompanyLegalForm"/>
        <dc:title xml:lang="en">Public foundation</dc:title>
        <dc:title xml:lang="de">Stiftung des öffentlichen Rechts</dc:title>
        <rdfs:label rdf:datatype="http://www.w3.org/2001/XMLSchema#string">SöR</rdfs:label>
    </owl:NamedIndividual>
    


    <!-- http://w3id.org/um/cbcm/eu-cm-ontology#de505 -->

    <owl:NamedIndividual rdf:about="http://w3id.org/um/cbcm/eu-cm-ontology#de505">
        <rdf:type rdf:resource="http://w3id.org/um/cbcm/eu-cm-ontology#CompanyLegalForm"/>
        <dc:title xml:lang="de">Betriebe der Gebietskörperschaften</dc:title>
        <dc:title xml:lang="en">Municipal undertaking</dc:title>
        <rdfs:label rdf:datatype="http://www.w3.org/2001/XMLSchema#string">BeG</rdfs:label>
    </owl:NamedIndividual>
    


    <!-- http://w3id.org/um/cbcm/eu-cm-ontology#de507 -->

    <owl:NamedIndividual rdf:about="http://w3id.org/um/cbcm/eu-cm-ontology#de507">
        <rdf:type rdf:resource="http://w3id.org/um/cbcm/eu-cm-ontology#CompanyLegalForm"/>
        <dc:title xml:lang="en">Special-purpose association</dc:title>
        <dc:title xml:lang="de">Zweckverband</dc:title>
        <rdfs:label rdf:datatype="http://www.w3.org/2001/XMLSchema#string">ZweckV</rdfs:label>
    </owl:NamedIndividual>
    


    <!-- http://w3id.org/um/cbcm/eu-cm-ontology#de601 -->

    <owl:NamedIndividual rdf:about="http://w3id.org/um/cbcm/eu-cm-ontology#de601">
        <rdf:type rdf:resource="http://w3id.org/um/cbcm/eu-cm-ontology#CompanyLegalForm"/>
        <dc:title xml:lang="en">Private foundation</dc:title>
        <dc:title xml:lang="de">Stiftung des privaten Rechts</dc:title>
        <rdfs:label rdf:datatype="http://www.w3.org/2001/XMLSchema#string">SpR</rdfs:label>
    </owl:NamedIndividual>
    


    <!-- http://w3id.org/um/cbcm/eu-cm-ontology#de602 -->

    <owl:NamedIndividual rdf:about="http://w3id.org/um/cbcm/eu-cm-ontology#de602">
        <rdf:type rdf:resource="http://w3id.org/um/cbcm/eu-cm-ontology#CompanyLegalForm"/>
        <dc:title xml:lang="de">Eingetragener Verein</dc:title>
        <dc:title xml:lang="en">Registered association</dc:title>
        <rdfs:label rdf:datatype="http://www.w3.org/2001/XMLSchema#string">e.V.</rdfs:label>
    </owl:NamedIndividual>
    


    <!-- http://w3id.org/um/cbcm/eu-cm-ontology#de603 -->

    <owl:NamedIndividual rdf:about="http://w3id.org/um/cbcm/eu-cm-ontology#de603">
        <rdf:type rdf:resource="http://w3id.org/um/cbcm/eu-cm-ontology#CompanyLegalForm"/>
        <dc:title xml:lang="en">Religious community</dc:title>
        <dc:title xml:lang="de">Weltanschauungs- und Religionsgemeinschaft</dc:title>
        <rdfs:label rdf:datatype="http://www.w3.org/2001/XMLSchema#string">WuR</rdfs:label>
    </owl:NamedIndividual>
    


    <!-- http://w3id.org/um/cbcm/eu-cm-ontology#denmark -->

    <owl:NamedIndividual rdf:about="http://w3id.org/um/cbcm/eu-cm-ontology#denmark">
        <rdf:type rdf:resource="http://w3id.org/um/cbcm/eu-cm-ontology#EUCountry"/>
        <cbcm:countryHasCompanyForm rdf:resource="http://w3id.org/um/cbcm/eu-cm-ontology#dk140"/>
        <cbcm:countryHasCompanyForm rdf:resource="http://w3id.org/um/cbcm/eu-cm-ontology#dk151"/>
        <cbcm:countryHasCompanyForm rdf:resource="http://w3id.org/um/cbcm/eu-cm-ontology#dk152"/>
        <cbcm:countryHasCompanyForm rdf:resource="http://w3id.org/um/cbcm/eu-cm-ontology#dk30"/>
        <cbcm:countryHasCompanyForm rdf:resource="http://w3id.org/um/cbcm/eu-cm-ontology#dk40"/>
        <cbcm:countryHasCompanyForm rdf:resource="http://w3id.org/um/cbcm/eu-cm-ontology#dk60"/>
        <cbcm:countryHasCompanyForm rdf:resource="http://w3id.org/um/cbcm/eu-cm-ontology#dk80"/>
        <cbcm:countryHasCompanyForm rdf:resource="http://w3id.org/um/cbcm/eu-cm-ontology#dk81"/>
        <cbcm:iso2code>DK</cbcm:iso2code>
        <rdfs:label xml:lang="dk">Danmark</rdfs:label>
        <rdfs:label xml:lang="en">Denmark</rdfs:label>
        <rdfs:label xml:lang="en">Kingdom of Denmark</rdfs:label>
    </owl:NamedIndividual>
    


    <!-- http://w3id.org/um/cbcm/eu-cm-ontology#dk140 -->

    <owl:NamedIndividual rdf:about="http://w3id.org/um/cbcm/eu-cm-ontology#dk140">
        <rdf:type rdf:resource="http://w3id.org/um/cbcm/eu-cm-ontology#CompanyLegalForm"/>
        <dc:title xml:lang="dk">Andelsselskab (-forening) begr. ansvar</dc:title>
        <dc:title xml:lang="en">Limited liability cooperative society</dc:title>
        <rdfs:label rdf:datatype="http://www.w3.org/2001/XMLSchema#string">a.m.b.a.</rdfs:label>
    </owl:NamedIndividual>
    


    <!-- http://w3id.org/um/cbcm/eu-cm-ontology#dk151 -->

    <owl:NamedIndividual rdf:about="http://w3id.org/um/cbcm/eu-cm-ontology#dk151">
        <rdf:type rdf:resource="http://w3id.org/um/cbcm/eu-cm-ontology#CompanyLegalForm"/>
        <dc:title xml:lang="en">Limited liability company</dc:title>
        <dc:title xml:lang="dk">Selskab med begrænset ansvar</dc:title>
        <rdfs:label rdf:datatype="http://www.w3.org/2001/XMLSchema#string">s.m.b.a.</rdfs:label>
    </owl:NamedIndividual>
    


    <!-- http://w3id.org/um/cbcm/eu-cm-ontology#dk152 -->

    <owl:NamedIndividual rdf:about="http://w3id.org/um/cbcm/eu-cm-ontology#dk152">
        <rdf:type rdf:resource="http://w3id.org/um/cbcm/eu-cm-ontology#CompanyLegalForm"/>
        <dc:title xml:lang="dk">Forening med begrænset ansvar</dc:title>
        <dc:title xml:lang="en">Limited liability association</dc:title>
        <rdfs:label rdf:datatype="http://www.w3.org/2001/XMLSchema#string">f.m.b.a.</rdfs:label>
    </owl:NamedIndividual>
    


    <!-- http://w3id.org/um/cbcm/eu-cm-ontology#dk30 -->

    <owl:NamedIndividual rdf:about="http://w3id.org/um/cbcm/eu-cm-ontology#dk30">
        <rdf:type rdf:resource="http://w3id.org/um/cbcm/eu-cm-ontology#CompanyLegalForm"/>
        <dc:title xml:lang="en">General partnership</dc:title>
        <dc:title xml:lang="dk">Interessentskab</dc:title>
        <rdfs:label rdf:datatype="http://www.w3.org/2001/XMLSchema#string">I</rdfs:label>
        <rdfs:label rdf:datatype="http://www.w3.org/2001/XMLSchema#string">S</rdfs:label>
    </owl:NamedIndividual>
    


    <!-- http://w3id.org/um/cbcm/eu-cm-ontology#dk40 -->

    <owl:NamedIndividual rdf:about="http://w3id.org/um/cbcm/eu-cm-ontology#dk40">
        <rdf:type rdf:resource="http://w3id.org/um/cbcm/eu-cm-ontology#CompanyLegalForm"/>
        <dc:title xml:lang="dk">Kommanditselskab</dc:title>
        <dc:title xml:lang="en">Limited partnership</dc:title>
        <rdfs:label rdf:datatype="http://www.w3.org/2001/XMLSchema#string">K</rdfs:label>
        <rdfs:label rdf:datatype="http://www.w3.org/2001/XMLSchema#string">S</rdfs:label>
    </owl:NamedIndividual>
    


    <!-- http://w3id.org/um/cbcm/eu-cm-ontology#dk60 -->

    <owl:NamedIndividual rdf:about="http://w3id.org/um/cbcm/eu-cm-ontology#dk60">
        <rdf:type rdf:resource="http://w3id.org/um/cbcm/eu-cm-ontology#CompanyLegalForm"/>
        <dc:title xml:lang="dk">Aktieselskab</dc:title>
        <dc:title xml:lang="en">Limited company </dc:title>
        <rdfs:label rdf:datatype="http://www.w3.org/2001/XMLSchema#string">A</rdfs:label>
        <rdfs:label rdf:datatype="http://www.w3.org/2001/XMLSchema#string">S</rdfs:label>
    </owl:NamedIndividual>
    


    <!-- http://w3id.org/um/cbcm/eu-cm-ontology#dk80 -->

    <owl:NamedIndividual rdf:about="http://w3id.org/um/cbcm/eu-cm-ontology#dk80">
        <rdf:type rdf:resource="http://w3id.org/um/cbcm/eu-cm-ontology#CompanyLegalForm"/>
        <dc:title xml:lang="dk">Anpartselskab</dc:title>
        <dc:title xml:lang="en">Private limited company </dc:title>
        <rdfs:label rdf:datatype="http://www.w3.org/2001/XMLSchema#string">ApS</rdfs:label>
    </owl:NamedIndividual>
    


    <!-- http://w3id.org/um/cbcm/eu-cm-ontology#dk81 -->

    <owl:NamedIndividual rdf:about="http://w3id.org/um/cbcm/eu-cm-ontology#dk81">
        <rdf:type rdf:resource="http://w3id.org/um/cbcm/eu-cm-ontology#CompanyLegalForm"/>
        <dc:title xml:lang="en">Entrepreneurial limited company</dc:title>
        <dc:title xml:lang="dk">Iværksætterselskab</dc:title>
        <rdfs:label rdf:datatype="http://www.w3.org/2001/XMLSchema#string">IVS</rdfs:label>
    </owl:NamedIndividual>
    


    <!-- http://w3id.org/um/cbcm/eu-cm-ontology#ee101 -->

    <owl:NamedIndividual rdf:about="http://w3id.org/um/cbcm/eu-cm-ontology#ee101">
        <rdf:type rdf:resource="http://w3id.org/um/cbcm/eu-cm-ontology#CompanyLegalForm"/>
        <dc:title xml:lang="ee">Aktsiaselts</dc:title>
        <dc:title xml:lang="en">Public limited company </dc:title>
        <rdfs:label rdf:datatype="http://www.w3.org/2001/XMLSchema#string">AS</rdfs:label>
    </owl:NamedIndividual>
    


    <!-- http://w3id.org/um/cbcm/eu-cm-ontology#ee102 -->

    <owl:NamedIndividual rdf:about="http://w3id.org/um/cbcm/eu-cm-ontology#ee102">
        <rdf:type rdf:resource="http://w3id.org/um/cbcm/eu-cm-ontology#CompanyLegalForm"/>
        <dc:title xml:lang="ee">Osaühing</dc:title>
        <dc:title xml:lang="en">Private limited company</dc:title>
        <rdfs:label rdf:datatype="http://www.w3.org/2001/XMLSchema#string">OÜ</rdfs:label>
    </owl:NamedIndividual>
    


    <!-- http://w3id.org/um/cbcm/eu-cm-ontology#ee201 -->

    <owl:NamedIndividual rdf:about="http://w3id.org/um/cbcm/eu-cm-ontology#ee201">
        <rdf:type rdf:resource="http://w3id.org/um/cbcm/eu-cm-ontology#CompanyLegalForm"/>
        <dc:title xml:lang="en">General partnership</dc:title>
        <dc:title xml:lang="ee">Täisühing</dc:title>
        <rdfs:label rdf:datatype="http://www.w3.org/2001/XMLSchema#string">TÜ</rdfs:label>
    </owl:NamedIndividual>
    


    <!-- http://w3id.org/um/cbcm/eu-cm-ontology#ee202 -->

    <owl:NamedIndividual rdf:about="http://w3id.org/um/cbcm/eu-cm-ontology#ee202">
        <rdf:type rdf:resource="http://w3id.org/um/cbcm/eu-cm-ontology#CompanyLegalForm"/>
        <dc:title xml:lang="en">Limited partnership</dc:title>
        <dc:title xml:lang="ee">Usaldusühing</dc:title>
        <rdfs:label rdf:datatype="http://www.w3.org/2001/XMLSchema#string">UÜ</rdfs:label>
    </owl:NamedIndividual>
    


    <!-- http://w3id.org/um/cbcm/eu-cm-ontology#ee203 -->

    <owl:NamedIndividual rdf:about="http://w3id.org/um/cbcm/eu-cm-ontology#ee203">
        <rdf:type rdf:resource="http://w3id.org/um/cbcm/eu-cm-ontology#CompanyLegalForm"/>
        <dc:title xml:lang="ee">Mittetulundusühing</dc:title>
        <dc:title xml:lang="en">Non-profit association</dc:title>
        <rdfs:label rdf:datatype="http://www.w3.org/2001/XMLSchema#string">MTÜ</rdfs:label>
    </owl:NamedIndividual>
    


    <!-- http://w3id.org/um/cbcm/eu-cm-ontology#ee204 -->

    <owl:NamedIndividual rdf:about="http://w3id.org/um/cbcm/eu-cm-ontology#ee204">
        <rdf:type rdf:resource="http://w3id.org/um/cbcm/eu-cm-ontology#CompanyLegalForm"/>
        <dc:title xml:lang="en">Commercial association</dc:title>
        <dc:title xml:lang="ee">Tulundusühistu</dc:title>
        <rdfs:label rdf:datatype="http://www.w3.org/2001/XMLSchema#string">TuÜ</rdfs:label>
    </owl:NamedIndividual>
    


    <!-- http://w3id.org/um/cbcm/eu-cm-ontology#ee205 -->

    <owl:NamedIndividual rdf:about="http://w3id.org/um/cbcm/eu-cm-ontology#ee205">
        <rdf:type rdf:resource="http://w3id.org/um/cbcm/eu-cm-ontology#CompanyLegalForm"/>
        <dc:title xml:lang="en">Foundation</dc:title>
        <dc:title xml:lang="ee">Sihtasutus</dc:title>
        <rdfs:label rdf:datatype="http://www.w3.org/2001/XMLSchema#string">SA</rdfs:label>
    </owl:NamedIndividual>
    


    <!-- http://w3id.org/um/cbcm/eu-cm-ontology#ee206 -->

    <owl:NamedIndividual rdf:about="http://w3id.org/um/cbcm/eu-cm-ontology#ee206">
        <rdf:type rdf:resource="http://w3id.org/um/cbcm/eu-cm-ontology#CompanyLegalForm"/>
        <dc:title xml:lang="en">Central and local government authorities </dc:title>
        <dc:title xml:lang="ee">Riigi ja kohaliku omavalitsuse asutused</dc:title>
        <rdfs:label rdf:datatype="http://www.w3.org/2001/XMLSchema#string">RKOA</rdfs:label>
    </owl:NamedIndividual>
    


    <!-- http://w3id.org/um/cbcm/eu-cm-ontology#ee207 -->

    <owl:NamedIndividual rdf:about="http://w3id.org/um/cbcm/eu-cm-ontology#ee207">
        <rdf:type rdf:resource="http://w3id.org/um/cbcm/eu-cm-ontology#CompanyLegalForm"/>
        <dc:title xml:lang="en">Apartment association</dc:title>
        <dc:title xml:lang="ee">Korteriühistu</dc:title>
        <rdfs:label rdf:datatype="http://www.w3.org/2001/XMLSchema#string">KÜ</rdfs:label>
    </owl:NamedIndividual>
    


    <!-- http://w3id.org/um/cbcm/eu-cm-ontology#esc04 -->

    <owl:NamedIndividual rdf:about="http://w3id.org/um/cbcm/eu-cm-ontology#esc04">
        <rdf:type rdf:resource="http://w3id.org/um/cbcm/eu-cm-ontology#CompanyLegalForm"/>
        <dc:title xml:lang="en">Public limited company</dc:title>
        <dc:title xml:lang="es">Sociedad Anónima</dc:title>
        <rdfs:label rdf:datatype="http://www.w3.org/2001/XMLSchema#string">SA</rdfs:label>
    </owl:NamedIndividual>
    


    <!-- http://w3id.org/um/cbcm/eu-cm-ontology#esc05 -->

    <owl:NamedIndividual rdf:about="http://w3id.org/um/cbcm/eu-cm-ontology#esc05">
        <rdf:type rdf:resource="http://w3id.org/um/cbcm/eu-cm-ontology#CompanyLegalForm"/>
        <dc:title xml:lang="en">Single-member public limited company</dc:title>
        <dc:title xml:lang="es">Sociedad Anónima Unipersonal</dc:title>
        <rdfs:label rdf:datatype="http://www.w3.org/2001/XMLSchema#string">SAU</rdfs:label>
    </owl:NamedIndividual>
    


    <!-- http://w3id.org/um/cbcm/eu-cm-ontology#esc06 -->

    <owl:NamedIndividual rdf:about="http://w3id.org/um/cbcm/eu-cm-ontology#esc06">
        <rdf:type rdf:resource="http://w3id.org/um/cbcm/eu-cm-ontology#CompanyLegalForm"/>
        <dc:title xml:lang="es">Sociedad Anónima Laboral</dc:title>
        <dc:title xml:lang="en">Worker-owned public limited company </dc:title>
        <rdfs:label rdf:datatype="http://www.w3.org/2001/XMLSchema#string">SAL</rdfs:label>
        <rdfs:label rdf:datatype="http://www.w3.org/2001/XMLSchema#string">SALABORAL</rdfs:label>
    </owl:NamedIndividual>
    


    <!-- http://w3id.org/um/cbcm/eu-cm-ontology#esc07 -->

    <owl:NamedIndividual rdf:about="http://w3id.org/um/cbcm/eu-cm-ontology#esc07">
        <rdf:type rdf:resource="http://w3id.org/um/cbcm/eu-cm-ontology#CompanyLegalForm"/>
        <dc:title xml:lang="en">Private limited company</dc:title>
        <dc:title xml:lang="es">Sociedad de responsabilidad limitada</dc:title>
        <rdfs:label rdf:datatype="http://www.w3.org/2001/XMLSchema#string">SL</rdfs:label>
        <rdfs:label rdf:datatype="http://www.w3.org/2001/XMLSchema#string">SRL</rdfs:label>
    </owl:NamedIndividual>
    


    <!-- http://w3id.org/um/cbcm/eu-cm-ontology#esc08 -->

    <owl:NamedIndividual rdf:about="http://w3id.org/um/cbcm/eu-cm-ontology#esc08">
        <rdf:type rdf:resource="http://w3id.org/um/cbcm/eu-cm-ontology#CompanyLegalForm"/>
        <dc:title xml:lang="en">Single-member private limited company</dc:title>
        <dc:title xml:lang="es">Sociedad Limitada Unipersonal</dc:title>
        <rdfs:label rdf:datatype="http://www.w3.org/2001/XMLSchema#string">SLU</rdfs:label>
        <rdfs:label rdf:datatype="http://www.w3.org/2001/XMLSchema#string">SRLU</rdfs:label>
    </owl:NamedIndividual>
    


    <!-- http://w3id.org/um/cbcm/eu-cm-ontology#esc09 -->

    <owl:NamedIndividual rdf:about="http://w3id.org/um/cbcm/eu-cm-ontology#esc09">
        <rdf:type rdf:resource="http://w3id.org/um/cbcm/eu-cm-ontology#CompanyLegalForm"/>
        <dc:title xml:lang="es">Sociedad Limitada Laboral</dc:title>
        <dc:title xml:lang="en">Worker-owned private limited company </dc:title>
        <rdfs:label rdf:datatype="http://www.w3.org/2001/XMLSchema#string">SLL</rdfs:label>
        <rdfs:label rdf:datatype="http://www.w3.org/2001/XMLSchema#string">SLLABORAL</rdfs:label>
    </owl:NamedIndividual>
    


    <!-- http://w3id.org/um/cbcm/eu-cm-ontology#esc10 -->

    <owl:NamedIndividual rdf:about="http://w3id.org/um/cbcm/eu-cm-ontology#esc10">
        <rdf:type rdf:resource="http://w3id.org/um/cbcm/eu-cm-ontology#CompanyLegalForm"/>
        <dc:title xml:lang="en">New firm private limited company </dc:title>
        <dc:title xml:lang="es">Sociedad Limitada Nueva Empresa</dc:title>
        <rdfs:label rdf:datatype="http://www.w3.org/2001/XMLSchema#string">SLNE</rdfs:label>
    </owl:NamedIndividual>
    


    <!-- http://w3id.org/um/cbcm/eu-cm-ontology#esc11 -->

    <owl:NamedIndividual rdf:about="http://w3id.org/um/cbcm/eu-cm-ontology#esc11">
        <rdf:type rdf:resource="http://w3id.org/um/cbcm/eu-cm-ontology#CompanyLegalForm"/>
        <dc:title xml:lang="en">General partnerships</dc:title>
        <dc:title xml:lang="es">Sociedad colectiva</dc:title>
        <rdfs:label rdf:datatype="http://www.w3.org/2001/XMLSchema#string">SC</rdfs:label>
        <rdfs:label rdf:datatype="http://www.w3.org/2001/XMLSchema#string">SRC</rdfs:label>
    </owl:NamedIndividual>
    


    <!-- http://w3id.org/um/cbcm/eu-cm-ontology#esc12 -->

    <owl:NamedIndividual rdf:about="http://w3id.org/um/cbcm/eu-cm-ontology#esc12">
        <rdf:type rdf:resource="http://w3id.org/um/cbcm/eu-cm-ontology#CompanyLegalForm"/>
        <dc:title xml:lang="en">Simple limited partnership</dc:title>
        <dc:title xml:lang="es">Sociedad Comanditaria Simple</dc:title>
        <rdfs:label rdf:datatype="http://www.w3.org/2001/XMLSchema#string">S.ENC.oS.COM.</rdfs:label>
    </owl:NamedIndividual>
    


    <!-- http://w3id.org/um/cbcm/eu-cm-ontology#esc13 -->

    <owl:NamedIndividual rdf:about="http://w3id.org/um/cbcm/eu-cm-ontology#esc13">
        <rdf:type rdf:resource="http://w3id.org/um/cbcm/eu-cm-ontology#CompanyLegalForm"/>
        <dc:title xml:lang="en">Limited stock partnership</dc:title>
        <dc:title xml:lang="es">Sociedad Comanditaria por acciones</dc:title>
        <rdfs:label rdf:datatype="http://www.w3.org/2001/XMLSchema#string">S.COM.P.A.</rdfs:label>
    </owl:NamedIndividual>
    


    <!-- http://w3id.org/um/cbcm/eu-cm-ontology#esc14 -->

    <owl:NamedIndividual rdf:about="http://w3id.org/um/cbcm/eu-cm-ontology#esc14">
        <rdf:type rdf:resource="http://w3id.org/um/cbcm/eu-cm-ontology#CompanyLegalForm"/>
        <dc:title xml:lang="en">Cooperative company</dc:title>
        <dc:title xml:lang="es">Sociedad Cooperativa</dc:title>
        <rdfs:label rdf:datatype="http://www.w3.org/2001/XMLSchema#string">SCOOP</rdfs:label>
    </owl:NamedIndividual>
    


    <!-- http://w3id.org/um/cbcm/eu-cm-ontology#esc16 -->

    <owl:NamedIndividual rdf:about="http://w3id.org/um/cbcm/eu-cm-ontology#esc16">
        <rdf:type rdf:resource="http://w3id.org/um/cbcm/eu-cm-ontology#CompanyLegalForm"/>
        <dc:title xml:lang="en">Mutual Guarantee Company</dc:title>
        <dc:title xml:lang="es">Sociedad de garantía recíproca</dc:title>
        <rdfs:label rdf:datatype="http://www.w3.org/2001/XMLSchema#string">SGR</rdfs:label>
    </owl:NamedIndividual>
    


    <!-- http://w3id.org/um/cbcm/eu-cm-ontology#esc17 -->

    <owl:NamedIndividual rdf:about="http://w3id.org/um/cbcm/eu-cm-ontology#esc17">
        <rdf:type rdf:resource="http://w3id.org/um/cbcm/eu-cm-ontology#CompanyLegalForm"/>
        <dc:title xml:lang="en">Farming partnerships</dc:title>
        <dc:title xml:lang="es">Sociedad agraria de transformación</dc:title>
        <rdfs:label rdf:datatype="http://www.w3.org/2001/XMLSchema#string">SAT</rdfs:label>
    </owl:NamedIndividual>
    


    <!-- http://w3id.org/um/cbcm/eu-cm-ontology#esc21 -->

    <owl:NamedIndividual rdf:about="http://w3id.org/um/cbcm/eu-cm-ontology#esc21">
        <rdf:type rdf:resource="http://w3id.org/um/cbcm/eu-cm-ontology#CompanyLegalForm"/>
        <dc:title xml:lang="es">Agrupación de Interés económico</dc:title>
        <dc:title xml:lang="en">Economic interest grouping</dc:title>
        <rdfs:label rdf:datatype="http://www.w3.org/2001/XMLSchema#string">AIE</rdfs:label>
    </owl:NamedIndividual>
    


    <!-- http://w3id.org/um/cbcm/eu-cm-ontology#esc30 -->

    <owl:NamedIndividual rdf:about="http://w3id.org/um/cbcm/eu-cm-ontology#esc30">
        <rdf:type rdf:resource="http://w3id.org/um/cbcm/eu-cm-ontology#CompanyLegalForm"/>
        <dc:title xml:lang="en">Private company of professional members</dc:title>
        <dc:title xml:lang="es">Sociedad profesional</dc:title>
        <rdfs:label rdf:datatype="http://www.w3.org/2001/XMLSchema#string">SP</rdfs:label>
    </owl:NamedIndividual>
    


    <!-- http://w3id.org/um/cbcm/eu-cm-ontology#estonia -->

    <owl:NamedIndividual rdf:about="http://w3id.org/um/cbcm/eu-cm-ontology#estonia">
        <rdf:type rdf:resource="http://w3id.org/um/cbcm/eu-cm-ontology#EUCountry"/>
        <cbcm:countryHasCompanyForm rdf:resource="http://w3id.org/um/cbcm/eu-cm-ontology#ee101"/>
        <cbcm:countryHasCompanyForm rdf:resource="http://w3id.org/um/cbcm/eu-cm-ontology#ee102"/>
        <cbcm:countryHasCompanyForm rdf:resource="http://w3id.org/um/cbcm/eu-cm-ontology#ee201"/>
        <cbcm:countryHasCompanyForm rdf:resource="http://w3id.org/um/cbcm/eu-cm-ontology#ee202"/>
        <cbcm:countryHasCompanyForm rdf:resource="http://w3id.org/um/cbcm/eu-cm-ontology#ee203"/>
        <cbcm:countryHasCompanyForm rdf:resource="http://w3id.org/um/cbcm/eu-cm-ontology#ee204"/>
        <cbcm:countryHasCompanyForm rdf:resource="http://w3id.org/um/cbcm/eu-cm-ontology#ee205"/>
        <cbcm:countryHasCompanyForm rdf:resource="http://w3id.org/um/cbcm/eu-cm-ontology#ee206"/>
        <cbcm:countryHasCompanyForm rdf:resource="http://w3id.org/um/cbcm/eu-cm-ontology#ee207"/>
        <cbcm:iso2code>EE</cbcm:iso2code>
        <rdfs:label xml:lang="ee">Eesti</rdfs:label>
        <rdfs:label xml:lang="en">Estonia</rdfs:label>
    </owl:NamedIndividual>
    


    <!-- http://w3id.org/um/cbcm/eu-cm-ontology#eu100 -->

    <owl:NamedIndividual rdf:about="http://w3id.org/um/cbcm/eu-cm-ontology#eu100">
        <rdf:type rdf:resource="http://w3id.org/um/cbcm/eu-cm-ontology#CompanyLegalForm"/>
        <dc:title xml:lang="en"> limited-liability company regulated under EU law)</dc:title>
        <dc:title xml:lang="en">European company (a type of public</dc:title>
        <dc:title xml:lang="-">Societas Europea</dc:title>
        <rdfs:label rdf:datatype="http://www.w3.org/2001/XMLSchema#string">SE</rdfs:label>
    </owl:NamedIndividual>
    


    <!-- http://w3id.org/um/cbcm/eu-cm-ontology#eu200 -->

    <owl:NamedIndividual rdf:about="http://w3id.org/um/cbcm/eu-cm-ontology#eu200">
        <rdf:type rdf:resource="http://w3id.org/um/cbcm/eu-cm-ontology#CompanyLegalForm"/>
        <dc:title xml:lang="en">European cooperative society</dc:title>
        <dc:title xml:lang="-">Societas Cooperativa Europea</dc:title>
        <rdfs:label rdf:datatype="http://www.w3.org/2001/XMLSchema#string">SCE</rdfs:label>
    </owl:NamedIndividual>
    


    <!-- http://w3id.org/um/cbcm/eu-cm-ontology#eu300 -->

    <owl:NamedIndividual rdf:about="http://w3id.org/um/cbcm/eu-cm-ontology#eu300">
        <rdf:type rdf:resource="http://w3id.org/um/cbcm/eu-cm-ontology#CompanyLegalForm"/>
        <dc:title xml:lang="-">European Economic Interest Grouping</dc:title>
        <dc:title xml:lang="en">European economic interest grouping</dc:title>
        <rdfs:label rdf:datatype="http://www.w3.org/2001/XMLSchema#string">EEIG</rdfs:label>
    </owl:NamedIndividual>
    


    <!-- http://w3id.org/um/cbcm/eu-cm-ontology#eu400 -->

    <owl:NamedIndividual rdf:about="http://w3id.org/um/cbcm/eu-cm-ontology#eu400">
        <rdf:type rdf:resource="http://w3id.org/um/cbcm/eu-cm-ontology#CompanyLegalForm"/>
        <dc:title xml:lang="-">European Grouping of Territorial cooperation</dc:title>
        <dc:title xml:lang="en">European Grouping of Territorial cooperation</dc:title>
        <rdfs:label rdf:datatype="http://www.w3.org/2001/XMLSchema#string">EGTC</rdfs:label>
    </owl:NamedIndividual>
    


    <!-- http://w3id.org/um/cbcm/eu-cm-ontology#euOfficialJournal -->

    <owl:NamedIndividual rdf:about="http://w3id.org/um/cbcm/eu-cm-ontology#euOfficialJournal">
        <rdf:type rdf:resource="http://w3id.org/um/cbcm/eu-cm-ontology#OfficialJournal"/>
    </owl:NamedIndividual>
    


    <!-- http://w3id.org/um/cbcm/eu-cm-ontology#fi11 -->

    <owl:NamedIndividual rdf:about="http://w3id.org/um/cbcm/eu-cm-ontology#fi11">
        <rdf:type rdf:resource="http://w3id.org/um/cbcm/eu-cm-ontology#CompanyLegalForm"/>
        <dc:title xml:lang="fi">Kommandiittiyhtiö</dc:title>
        <dc:title xml:lang="en">Limited partnership</dc:title>
        <rdfs:label rdf:datatype="http://www.w3.org/2001/XMLSchema#string">kb</rdfs:label>
        <rdfs:label rdf:datatype="http://www.w3.org/2001/XMLSchema#string">ky</rdfs:label>
    </owl:NamedIndividual>
    


    <!-- http://w3id.org/um/cbcm/eu-cm-ontology#fi12 -->

    <owl:NamedIndividual rdf:about="http://w3id.org/um/cbcm/eu-cm-ontology#fi12">
        <rdf:type rdf:resource="http://w3id.org/um/cbcm/eu-cm-ontology#CompanyLegalForm"/>
        <dc:title xml:lang="en">Limited company</dc:title>
        <dc:title xml:lang="fi">Osakeyhtiö</dc:title>
        <rdfs:label rdf:datatype="http://www.w3.org/2001/XMLSchema#string">ab</rdfs:label>
        <rdfs:label rdf:datatype="http://www.w3.org/2001/XMLSchema#string">abp</rdfs:label>
        <rdfs:label rdf:datatype="http://www.w3.org/2001/XMLSchema#string">oy</rdfs:label>
        <rdfs:label rdf:datatype="http://www.w3.org/2001/XMLSchema#string">oyj</rdfs:label>
    </owl:NamedIndividual>
    


    <!-- http://w3id.org/um/cbcm/eu-cm-ontology#fi13 -->

    <owl:NamedIndividual rdf:about="http://w3id.org/um/cbcm/eu-cm-ontology#fi13">
        <rdf:type rdf:resource="http://w3id.org/um/cbcm/eu-cm-ontology#CompanyLegalForm"/>
        <dc:title xml:lang="fi">Asunto-osakeyhtiö</dc:title>
        <dc:title xml:lang="en">Housing company</dc:title>
        <rdfs:label rdf:datatype="http://www.w3.org/2001/XMLSchema#string">asoy</rdfs:label>
    </owl:NamedIndividual>
    


    <!-- http://w3id.org/um/cbcm/eu-cm-ontology#fi24 -->

    <owl:NamedIndividual rdf:about="http://w3id.org/um/cbcm/eu-cm-ontology#fi24">
        <rdf:type rdf:resource="http://w3id.org/um/cbcm/eu-cm-ontology#CompanyLegalForm"/>
        <dc:title xml:lang="en">Cooperative bank</dc:title>
        <dc:title xml:lang="fi">Osuuspankki</dc:title>
        <rdfs:label rdf:datatype="http://www.w3.org/2001/XMLSchema#string">op</rdfs:label>
    </owl:NamedIndividual>
    


    <!-- http://w3id.org/um/cbcm/eu-cm-ontology#fi25 -->

    <owl:NamedIndividual rdf:about="http://w3id.org/um/cbcm/eu-cm-ontology#fi25">
        <rdf:type rdf:resource="http://w3id.org/um/cbcm/eu-cm-ontology#CompanyLegalForm"/>
        <dc:title xml:lang="en">Co-operative society</dc:title>
        <dc:title xml:lang="fi">Osuuskunta</dc:title>
        <rdfs:label rdf:datatype="http://www.w3.org/2001/XMLSchema#string">osk</rdfs:label>
    </owl:NamedIndividual>
    


    <!-- http://w3id.org/um/cbcm/eu-cm-ontology#fi30 -->

    <owl:NamedIndividual rdf:about="http://w3id.org/um/cbcm/eu-cm-ontology#fi30">
        <rdf:type rdf:resource="http://w3id.org/um/cbcm/eu-cm-ontology#CompanyLegalForm"/>
        <dc:title xml:lang="en">Foundation (according to the Foundations Act)</dc:title>
        <dc:title xml:lang="fi">Säätiö (säätiölain mukainen)</dc:title>
        <rdfs:label rdf:datatype="http://www.w3.org/2001/XMLSchema#string">sr</rdfs:label>
    </owl:NamedIndividual>
    


    <!-- http://w3id.org/um/cbcm/eu-cm-ontology#fi31 -->

    <owl:NamedIndividual rdf:about="http://w3id.org/um/cbcm/eu-cm-ontology#fi31">
        <rdf:type rdf:resource="http://w3id.org/um/cbcm/eu-cm-ontology#CompanyLegalForm"/>
        <dc:title xml:lang="en">Savings bank</dc:title>
        <dc:title xml:lang="fi">Säästöpankki</dc:title>
        <rdfs:label rdf:datatype="http://www.w3.org/2001/XMLSchema#string">sp</rdfs:label>
    </owl:NamedIndividual>
    


    <!-- http://w3id.org/um/cbcm/eu-cm-ontology#finland -->

    <owl:NamedIndividual rdf:about="http://w3id.org/um/cbcm/eu-cm-ontology#finland">
        <rdf:type rdf:resource="http://w3id.org/um/cbcm/eu-cm-ontology#EUCountry"/>
        <cbcm:countryHasCompanyForm rdf:resource="http://w3id.org/um/cbcm/eu-cm-ontology#fi11"/>
        <cbcm:countryHasCompanyForm rdf:resource="http://w3id.org/um/cbcm/eu-cm-ontology#fi12"/>
        <cbcm:countryHasCompanyForm rdf:resource="http://w3id.org/um/cbcm/eu-cm-ontology#fi13"/>
        <cbcm:countryHasCompanyForm rdf:resource="http://w3id.org/um/cbcm/eu-cm-ontology#fi24"/>
        <cbcm:countryHasCompanyForm rdf:resource="http://w3id.org/um/cbcm/eu-cm-ontology#fi25"/>
        <cbcm:countryHasCompanyForm rdf:resource="http://w3id.org/um/cbcm/eu-cm-ontology#fi30"/>
        <cbcm:countryHasCompanyForm rdf:resource="http://w3id.org/um/cbcm/eu-cm-ontology#fi31"/>
        <cbcm:iso2code>FI</cbcm:iso2code>
        <rdfs:label xml:lang="en">Finland</rdfs:label>
        <rdfs:label xml:lang="fi">Suomi</rdfs:label>
    </owl:NamedIndividual>
    


    <!-- http://w3id.org/um/cbcm/eu-cm-ontology#fr5130 -->

    <owl:NamedIndividual rdf:about="http://w3id.org/um/cbcm/eu-cm-ontology#fr5130">
        <rdf:type rdf:resource="http://w3id.org/um/cbcm/eu-cm-ontology#CompanyLegalForm"/>
        <dc:title xml:lang="en">French limited partnership</dc:title>
        <dc:title xml:lang="fr">Société de libre partenariat</dc:title>
        <rdfs:label rdf:datatype="http://www.w3.org/2001/XMLSchema#string">SLP</rdfs:label>
    </owl:NamedIndividual>
    


    <!-- http://w3id.org/um/cbcm/eu-cm-ontology#fr5370 -->

    <owl:NamedIndividual rdf:about="http://w3id.org/um/cbcm/eu-cm-ontology#fr5370">
        <rdf:type rdf:resource="http://w3id.org/um/cbcm/eu-cm-ontology#CompanyLegalForm"/>
        <dc:title xml:lang="en">Professional holding company Partnership limited by shares</dc:title>
        <dc:title xml:lang="fr">Société de Participations Financières de Profession Libérale Société en commandite par actions</dc:title>
        <rdfs:label rdf:datatype="http://www.w3.org/2001/XMLSchema#string">SPFPLSCA</rdfs:label>
    </owl:NamedIndividual>
    


    <!-- http://w3id.org/um/cbcm/eu-cm-ontology#fr5470 -->

    <owl:NamedIndividual rdf:about="http://w3id.org/um/cbcm/eu-cm-ontology#fr5470">
        <rdf:type rdf:resource="http://w3id.org/um/cbcm/eu-cm-ontology#CompanyLegalForm"/>
        <dc:title xml:lang="en">Professional holding company Limited liability company</dc:title>
        <dc:title xml:lang="fr">Société de Participations Financières de Profession Libérale Société à responsabilité limitée</dc:title>
        <rdfs:label rdf:datatype="http://www.w3.org/2001/XMLSchema#string">SPFPLSARL</rdfs:label>
    </owl:NamedIndividual>
    


    <!-- http://w3id.org/um/cbcm/eu-cm-ontology#fr5770 -->

    <owl:NamedIndividual rdf:about="http://w3id.org/um/cbcm/eu-cm-ontology#fr5770">
        <rdf:type rdf:resource="http://w3id.org/um/cbcm/eu-cm-ontology#CompanyLegalForm"/>
        <dc:title xml:lang="en">Professional holding company Simplified joint stock company</dc:title>
        <dc:title xml:lang="fr">Société de Participations Financières de Profession Libérale Société par actions simplifiée</dc:title>
        <rdfs:label rdf:datatype="http://www.w3.org/2001/XMLSchema#string">SPFPLSAS</rdfs:label>
    </owl:NamedIndividual>
    


    <!-- http://w3id.org/um/cbcm/eu-cm-ontology#fr6220 -->

    <owl:NamedIndividual rdf:about="http://w3id.org/um/cbcm/eu-cm-ontology#fr6220">
        <rdf:type rdf:resource="http://w3id.org/um/cbcm/eu-cm-ontology#CompanyLegalForm"/>
        <dc:title xml:lang="en">Economic interest grouping</dc:title>
        <dc:title xml:lang="fr">Groupement dintérêt économique </dc:title>
        <rdfs:label rdf:datatype="http://www.w3.org/2001/XMLSchema#string">GIE</rdfs:label>
    </owl:NamedIndividual>
    


    <!-- http://w3id.org/um/cbcm/eu-cm-ontology#fr6316 -->

    <owl:NamedIndividual rdf:about="http://w3id.org/um/cbcm/eu-cm-ontology#fr6316">
        <rdf:type rdf:resource="http://w3id.org/um/cbcm/eu-cm-ontology#CompanyLegalForm"/>
        <dc:title xml:lang="en">Cooperative for shared use of agricultural equipment</dc:title>
        <dc:title xml:lang="fr">Coopérative dutilisation de matériel agricole en commun </dc:title>
        <rdfs:label rdf:datatype="http://www.w3.org/2001/XMLSchema#string">CUMA</rdfs:label>
    </owl:NamedIndividual>
    


    <!-- http://w3id.org/um/cbcm/eu-cm-ontology#fr6521 -->

    <owl:NamedIndividual rdf:about="http://w3id.org/um/cbcm/eu-cm-ontology#fr6521">
        <rdf:type rdf:resource="http://w3id.org/um/cbcm/eu-cm-ontology#CompanyLegalForm"/>
        <dc:title xml:lang="en">Collective real estate investment civil-law company</dc:title>
        <dc:title xml:lang="fr">Société civile de placement collectif immobilier</dc:title>
        <rdfs:label rdf:datatype="http://www.w3.org/2001/XMLSchema#string">SCPI</rdfs:label>
    </owl:NamedIndividual>
    


    <!-- http://w3id.org/um/cbcm/eu-cm-ontology#fr6533 -->

    <owl:NamedIndividual rdf:about="http://w3id.org/um/cbcm/eu-cm-ontology#fr6533">
        <rdf:type rdf:resource="http://w3id.org/um/cbcm/eu-cm-ontology#CompanyLegalForm"/>
        <dc:title xml:lang="en">Collective farming grouping </dc:title>
        <dc:title xml:lang="fr">Groupement agricole dexploitation en commun</dc:title>
        <rdfs:label rdf:datatype="http://www.w3.org/2001/XMLSchema#string">GAEC</rdfs:label>
    </owl:NamedIndividual>
    


    <!-- http://w3id.org/um/cbcm/eu-cm-ontology#fr7345 -->

    <owl:NamedIndividual rdf:about="http://w3id.org/um/cbcm/eu-cm-ontology#fr7345">
        <rdf:type rdf:resource="http://w3id.org/um/cbcm/eu-cm-ontology#CompanyLegalForm"/>
        <dc:title xml:lang="en">Inter-municipality syndicate with multiple aims</dc:title>
        <dc:title xml:lang="fr">Syndicat intercommunal à vocation multiple </dc:title>
        <rdfs:label rdf:datatype="http://www.w3.org/2001/XMLSchema#string">SIVOM</rdfs:label>
    </owl:NamedIndividual>
    


    <!-- http://w3id.org/um/cbcm/eu-cm-ontology#fr7353 -->

    <owl:NamedIndividual rdf:about="http://w3id.org/um/cbcm/eu-cm-ontology#fr7353">
        <rdf:type rdf:resource="http://w3id.org/um/cbcm/eu-cm-ontology#CompanyLegalForm"/>
        <dc:title xml:lang="en">Inter-municipality syndicate with a single aim</dc:title>
        <dc:title xml:lang="fr">Syndicat intercommunal à vocation unique </dc:title>
        <rdfs:label rdf:datatype="http://www.w3.org/2001/XMLSchema#string">SIVU</rdfs:label>
    </owl:NamedIndividual>
    


    <!-- http://w3id.org/um/cbcm/eu-cm-ontology#fr7357 -->

    <owl:NamedIndividual rdf:about="http://w3id.org/um/cbcm/eu-cm-ontology#fr7357">
        <rdf:type rdf:resource="http://w3id.org/um/cbcm/eu-cm-ontology#CompanyLegalForm"/>
        <dc:title xml:lang="en">Centre for territorial and rural balance</dc:title>
        <dc:title xml:lang="fr">Pôle déquilibre territorial et rural </dc:title>
        <rdfs:label rdf:datatype="http://www.w3.org/2001/XMLSchema#string">PETR</rdfs:label>
    </owl:NamedIndividual>
    


    <!-- http://w3id.org/um/cbcm/eu-cm-ontology#fr7367 -->

    <owl:NamedIndividual rdf:about="http://w3id.org/um/cbcm/eu-cm-ontology#fr7367">
        <rdf:type rdf:resource="http://w3id.org/um/cbcm/eu-cm-ontology#CompanyLegalForm"/>
        <dc:title xml:lang="fr">Centre Intercommunal daction sociale </dc:title>
        <dc:title xml:lang="en">Inter-municipality social welfare centre</dc:title>
        <rdfs:label rdf:datatype="http://www.w3.org/2001/XMLSchema#string">CIAS</rdfs:label>
    </owl:NamedIndividual>
    


    <!-- http://w3id.org/um/cbcm/eu-cm-ontology#fr7371 -->

    <owl:NamedIndividual rdf:about="http://w3id.org/um/cbcm/eu-cm-ontology#fr7371">
        <rdf:type rdf:resource="http://w3id.org/um/cbcm/eu-cm-ontology#CompanyLegalForm"/>
        <dc:title xml:lang="fr">Office public dhabitation à loyer modéré </dc:title>
        <dc:title xml:lang="en">Public affordable housing office</dc:title>
        <rdfs:label rdf:datatype="http://www.w3.org/2001/XMLSchema#string">OPHLM</rdfs:label>
    </owl:NamedIndividual>
    


    <!-- http://w3id.org/um/cbcm/eu-cm-ontology#fr7372 -->

    <owl:NamedIndividual rdf:about="http://w3id.org/um/cbcm/eu-cm-ontology#fr7372">
        <rdf:type rdf:resource="http://w3id.org/um/cbcm/eu-cm-ontology#CompanyLegalForm"/>
        <dc:title xml:lang="en">Departmental fire and safety department</dc:title>
        <dc:title xml:lang="fr">Service départemental dincendie et de secours </dc:title>
        <rdfs:label rdf:datatype="http://www.w3.org/2001/XMLSchema#string">SDIS</rdfs:label>
    </owl:NamedIndividual>
    


    <!-- http://w3id.org/um/cbcm/eu-cm-ontology#fr7410 -->

    <owl:NamedIndividual rdf:about="http://w3id.org/um/cbcm/eu-cm-ontology#fr7410">
        <rdf:type rdf:resource="http://w3id.org/um/cbcm/eu-cm-ontology#CompanyLegalForm"/>
        <dc:title xml:lang="fr">Groupement dintérêt public </dc:title>
        <dc:title xml:lang="en">Public interest grouping</dc:title>
        <rdfs:label rdf:datatype="http://www.w3.org/2001/XMLSchema#string">GIP</rdfs:label>
    </owl:NamedIndividual>
    


    <!-- http://w3id.org/um/cbcm/eu-cm-ontology#france -->

    <owl:NamedIndividual rdf:about="http://w3id.org/um/cbcm/eu-cm-ontology#france">
        <rdf:type rdf:resource="http://w3id.org/um/cbcm/eu-cm-ontology#EUCountry"/>
        <cbcm:countryHasCompanyForm rdf:resource="http://w3id.org/um/cbcm/eu-cm-ontology#fr5130"/>
        <cbcm:countryHasCompanyForm rdf:resource="http://w3id.org/um/cbcm/eu-cm-ontology#fr5370"/>
        <cbcm:countryHasCompanyForm rdf:resource="http://w3id.org/um/cbcm/eu-cm-ontology#fr5470"/>
        <cbcm:countryHasCompanyForm rdf:resource="http://w3id.org/um/cbcm/eu-cm-ontology#fr5770"/>
        <cbcm:countryHasCompanyForm rdf:resource="http://w3id.org/um/cbcm/eu-cm-ontology#fr6220"/>
        <cbcm:countryHasCompanyForm rdf:resource="http://w3id.org/um/cbcm/eu-cm-ontology#fr6316"/>
        <cbcm:countryHasCompanyForm rdf:resource="http://w3id.org/um/cbcm/eu-cm-ontology#fr6521"/>
        <cbcm:countryHasCompanyForm rdf:resource="http://w3id.org/um/cbcm/eu-cm-ontology#fr6533"/>
        <cbcm:countryHasCompanyForm rdf:resource="http://w3id.org/um/cbcm/eu-cm-ontology#fr7345"/>
        <cbcm:countryHasCompanyForm rdf:resource="http://w3id.org/um/cbcm/eu-cm-ontology#fr7353"/>
        <cbcm:countryHasCompanyForm rdf:resource="http://w3id.org/um/cbcm/eu-cm-ontology#fr7357"/>
        <cbcm:countryHasCompanyForm rdf:resource="http://w3id.org/um/cbcm/eu-cm-ontology#fr7367"/>
        <cbcm:countryHasCompanyForm rdf:resource="http://w3id.org/um/cbcm/eu-cm-ontology#fr7371"/>
        <cbcm:countryHasCompanyForm rdf:resource="http://w3id.org/um/cbcm/eu-cm-ontology#fr7372"/>
        <cbcm:countryHasCompanyForm rdf:resource="http://w3id.org/um/cbcm/eu-cm-ontology#fr7410"/>
        <cbcm:iso2code>FR</cbcm:iso2code>
        <rdfs:label xml:lang="en">France</rdfs:label>
        <rdfs:label xml:lang="en">French Republic</rdfs:label>
        <rdfs:label xml:lang="fr">République française</rdfs:label>
    </owl:NamedIndividual>
    


    <!-- http://w3id.org/um/cbcm/eu-cm-ontology#germany -->

    <owl:NamedIndividual rdf:about="http://w3id.org/um/cbcm/eu-cm-ontology#germany">
        <rdf:type rdf:resource="http://w3id.org/um/cbcm/eu-cm-ontology#EUCountry"/>
        <cbcm:countryHasCompanyForm rdf:resource="http://w3id.org/um/cbcm/eu-cm-ontology#de101"/>
        <cbcm:countryHasCompanyForm rdf:resource="http://w3id.org/um/cbcm/eu-cm-ontology#de102"/>
        <cbcm:countryHasCompanyForm rdf:resource="http://w3id.org/um/cbcm/eu-cm-ontology#de103"/>
        <cbcm:countryHasCompanyForm rdf:resource="http://w3id.org/um/cbcm/eu-cm-ontology#de105"/>
        <cbcm:countryHasCompanyForm rdf:resource="http://w3id.org/um/cbcm/eu-cm-ontology#de108"/>
        <cbcm:countryHasCompanyForm rdf:resource="http://w3id.org/um/cbcm/eu-cm-ontology#de109"/>
        <cbcm:countryHasCompanyForm rdf:resource="http://w3id.org/um/cbcm/eu-cm-ontology#de110"/>
        <cbcm:countryHasCompanyForm rdf:resource="http://w3id.org/um/cbcm/eu-cm-ontology#de201"/>
        <cbcm:countryHasCompanyForm rdf:resource="http://w3id.org/um/cbcm/eu-cm-ontology#de202"/>
        <cbcm:countryHasCompanyForm rdf:resource="http://w3id.org/um/cbcm/eu-cm-ontology#de205"/>
        <cbcm:countryHasCompanyForm rdf:resource="http://w3id.org/um/cbcm/eu-cm-ontology#de206"/>
        <cbcm:countryHasCompanyForm rdf:resource="http://w3id.org/um/cbcm/eu-cm-ontology#de207"/>
        <cbcm:countryHasCompanyForm rdf:resource="http://w3id.org/um/cbcm/eu-cm-ontology#de209"/>
        <cbcm:countryHasCompanyForm rdf:resource="http://w3id.org/um/cbcm/eu-cm-ontology#de211"/>
        <cbcm:countryHasCompanyForm rdf:resource="http://w3id.org/um/cbcm/eu-cm-ontology#de301"/>
        <cbcm:countryHasCompanyForm rdf:resource="http://w3id.org/um/cbcm/eu-cm-ontology#de401"/>
        <cbcm:countryHasCompanyForm rdf:resource="http://w3id.org/um/cbcm/eu-cm-ontology#de501"/>
        <cbcm:countryHasCompanyForm rdf:resource="http://w3id.org/um/cbcm/eu-cm-ontology#de502"/>
        <cbcm:countryHasCompanyForm rdf:resource="http://w3id.org/um/cbcm/eu-cm-ontology#de503"/>
        <cbcm:countryHasCompanyForm rdf:resource="http://w3id.org/um/cbcm/eu-cm-ontology#de504"/>
        <cbcm:countryHasCompanyForm rdf:resource="http://w3id.org/um/cbcm/eu-cm-ontology#de505"/>
        <cbcm:countryHasCompanyForm rdf:resource="http://w3id.org/um/cbcm/eu-cm-ontology#de507"/>
        <cbcm:countryHasCompanyForm rdf:resource="http://w3id.org/um/cbcm/eu-cm-ontology#de601"/>
        <cbcm:countryHasCompanyForm rdf:resource="http://w3id.org/um/cbcm/eu-cm-ontology#de602"/>
        <cbcm:countryHasCompanyForm rdf:resource="http://w3id.org/um/cbcm/eu-cm-ontology#de603"/>
        <cbcm:iso2code>DE</cbcm:iso2code>
        <rdfs:label xml:lang="de">Deutschland</rdfs:label>
        <rdfs:label xml:lang="en">Germany</rdfs:label>
    </owl:NamedIndividual>
    


    <!-- http://w3id.org/um/cbcm/eu-cm-ontology#gr901 -->

    <owl:NamedIndividual rdf:about="http://w3id.org/um/cbcm/eu-cm-ontology#gr901">
        <rdf:type rdf:resource="http://w3id.org/um/cbcm/eu-cm-ontology#CompanyLegalForm"/>
        <dc:title xml:lang="gr">  Astiki  Etería</dc:title>
        <dc:title xml:lang="en">Civil-law Association</dc:title>
        <dc:title xml:lang="gr">Αστική  Εταιρεία </dc:title>
        <rdfs:label rdf:datatype="http://www.w3.org/2001/XMLSchema#string">CLA</rdfs:label>
    </owl:NamedIndividual>
    


    <!-- http://w3id.org/um/cbcm/eu-cm-ontology#gr902 -->

    <owl:NamedIndividual rdf:about="http://w3id.org/um/cbcm/eu-cm-ontology#gr902">
        <rdf:type rdf:resource="http://w3id.org/um/cbcm/eu-cm-ontology#CompanyLegalForm"/>
        <dc:title xml:lang="gr">  Omórithmi Etería</dc:title>
        <dc:title xml:lang="en">General Partnership</dc:title>
        <dc:title xml:lang="gr">Ομόρρυθμη Εταιρεία </dc:title>
        <rdfs:label rdf:datatype="http://www.w3.org/2001/XMLSchema#string">OE</rdfs:label>
    </owl:NamedIndividual>
    


    <!-- http://w3id.org/um/cbcm/eu-cm-ontology#gr903 -->

    <owl:NamedIndividual rdf:about="http://w3id.org/um/cbcm/eu-cm-ontology#gr903">
        <rdf:type rdf:resource="http://w3id.org/um/cbcm/eu-cm-ontology#CompanyLegalForm"/>
        <dc:title xml:lang="gr">  Eterórithmi Etería</dc:title>
        <dc:title xml:lang="en">Limited partnership (partnership company)</dc:title>
        <dc:title xml:lang="gr">Ετερόρρυθμη Εταιρεία </dc:title>
        <rdfs:label rdf:datatype="http://www.w3.org/2001/XMLSchema#string">EE</rdfs:label>
    </owl:NamedIndividual>
    


    <!-- http://w3id.org/um/cbcm/eu-cm-ontology#gr904 -->

    <owl:NamedIndividual rdf:about="http://w3id.org/um/cbcm/eu-cm-ontology#gr904">
        <rdf:type rdf:resource="http://w3id.org/um/cbcm/eu-cm-ontology#CompanyLegalForm"/>
        <dc:title xml:lang="gr">  Afanis Eteria</dc:title>
        <dc:title xml:lang="en">Silent Partnership</dc:title>
        <dc:title xml:lang="gr">Αφανής Εταιρεία </dc:title>
        <rdfs:label rdf:datatype="http://www.w3.org/2001/XMLSchema#string">SLP</rdfs:label>
    </owl:NamedIndividual>
    


    <!-- http://w3id.org/um/cbcm/eu-cm-ontology#gr905 -->

    <owl:NamedIndividual rdf:about="http://w3id.org/um/cbcm/eu-cm-ontology#gr905">
        <rdf:type rdf:resource="http://w3id.org/um/cbcm/eu-cm-ontology#CompanyLegalForm"/>
        <dc:title xml:lang="gr">  Anónimi Etería</dc:title>
        <dc:title xml:lang="en"> Incorporated Company</dc:title>
        <dc:title xml:lang="en"> Joint-stock Company</dc:title>
        <dc:title xml:lang="en"> Societe Anonyme</dc:title>
        <dc:title xml:lang="en">Public Limited Company</dc:title>
        <dc:title xml:lang="gr">Ανώνυμη Εταιρεία </dc:title>
        <rdfs:label rdf:datatype="http://www.w3.org/2001/XMLSchema#string">SA</rdfs:label>
    </owl:NamedIndividual>
    


    <!-- http://w3id.org/um/cbcm/eu-cm-ontology#gr906 -->

    <owl:NamedIndividual rdf:about="http://w3id.org/um/cbcm/eu-cm-ontology#gr906">
        <rdf:type rdf:resource="http://w3id.org/um/cbcm/eu-cm-ontology#CompanyLegalForm"/>
        <dc:title xml:lang="gr">  Etería Periorisménis Euthínis</dc:title>
        <dc:title xml:lang="en">Limited Liability Company</dc:title>
        <dc:title xml:lang="gr">Εταιρεία Περιορισμένης Ευθύνης </dc:title>
        <rdfs:label rdf:datatype="http://www.w3.org/2001/XMLSchema#string">EPE</rdfs:label>
    </owl:NamedIndividual>
    


    <!-- http://w3id.org/um/cbcm/eu-cm-ontology#gr907 -->

    <owl:NamedIndividual rdf:about="http://w3id.org/um/cbcm/eu-cm-ontology#gr907">
        <rdf:type rdf:resource="http://w3id.org/um/cbcm/eu-cm-ontology#CompanyLegalForm"/>
        <dc:title xml:lang="gr">  Idiotiki kefaleouhiki Eteria</dc:title>
        <dc:title xml:lang="en">Private Capital Company</dc:title>
        <dc:title xml:lang="gr">Ιδιωτική Κεφαλαιουχική Εταιρεία </dc:title>
        <rdfs:label rdf:datatype="http://www.w3.org/2001/XMLSchema#string">IKE</rdfs:label>
    </owl:NamedIndividual>
    


    <!-- http://w3id.org/um/cbcm/eu-cm-ontology#gr908 -->

    <owl:NamedIndividual rdf:about="http://w3id.org/um/cbcm/eu-cm-ontology#gr908">
        <rdf:type rdf:resource="http://w3id.org/um/cbcm/eu-cm-ontology#CompanyLegalForm"/>
        <dc:title xml:lang="gr"> Simplioktisia</dc:title>
        <dc:title xml:lang="en">Joint Ship-ownership</dc:title>
        <dc:title xml:lang="gr">Συμπλοιοκτησία</dc:title>
        <rdfs:label rdf:datatype="http://www.w3.org/2001/XMLSchema#string">JSO</rdfs:label>
    </owl:NamedIndividual>
    


    <!-- http://w3id.org/um/cbcm/eu-cm-ontology#gr909 -->

    <owl:NamedIndividual rdf:about="http://w3id.org/um/cbcm/eu-cm-ontology#gr909">
        <rdf:type rdf:resource="http://w3id.org/um/cbcm/eu-cm-ontology#CompanyLegalForm"/>
        <dc:title xml:lang="gr">  Naftiki eteria</dc:title>
        <dc:title xml:lang="en">Shipping Company</dc:title>
        <dc:title xml:lang="gr">Ναυτική εταιρία </dc:title>
        <rdfs:label rdf:datatype="http://www.w3.org/2001/XMLSchema#string">SC</rdfs:label>
    </owl:NamedIndividual>
    


    <!-- http://w3id.org/um/cbcm/eu-cm-ontology#gr910 -->

    <owl:NamedIndividual rdf:about="http://w3id.org/um/cbcm/eu-cm-ontology#gr910">
        <rdf:type rdf:resource="http://w3id.org/um/cbcm/eu-cm-ontology#CompanyLegalForm"/>
        <dc:title xml:lang="en"> Association</dc:title>
        <dc:title xml:lang="gr"> Sinetairismos</dc:title>
        <dc:title xml:lang="en">Cooperative Company</dc:title>
        <dc:title xml:lang="gr">Συνεταιρισμός</dc:title>
        <rdfs:label rdf:datatype="http://www.w3.org/2001/XMLSchema#string">COOP</rdfs:label>
    </owl:NamedIndividual>
    


    <!-- http://w3id.org/um/cbcm/eu-cm-ontology#gr911 -->

    <owl:NamedIndividual rdf:about="http://w3id.org/um/cbcm/eu-cm-ontology#gr911">
        <rdf:type rdf:resource="http://w3id.org/um/cbcm/eu-cm-ontology#CompanyLegalForm"/>
        <dc:title xml:lang="gr">  Somatia - Idrimata</dc:title>
        <dc:title xml:lang="en"> Foundation</dc:title>
        <dc:title xml:lang="en"> Syndicate</dc:title>
        <dc:title xml:lang="en"> Union</dc:title>
        <dc:title xml:lang="en">Club</dc:title>
        <dc:title xml:lang="gr">Σωματεία - Ιδρύματα </dc:title>
        <rdfs:label rdf:datatype="http://www.w3.org/2001/XMLSchema#string">CLF</rdfs:label>
    </owl:NamedIndividual>
    


    <!-- http://w3id.org/um/cbcm/eu-cm-ontology#gr912 -->

    <owl:NamedIndividual rdf:about="http://w3id.org/um/cbcm/eu-cm-ontology#gr912">
        <rdf:type rdf:resource="http://w3id.org/um/cbcm/eu-cm-ontology#CompanyLegalForm"/>
        <dc:title xml:lang="gr"> Kinopraxia</dc:title>
        <dc:title xml:lang="en">Joint Venture</dc:title>
        <dc:title xml:lang="gr">Κοινοπραξία</dc:title>
        <rdfs:label rdf:datatype="http://www.w3.org/2001/XMLSchema#string">JV</rdfs:label>
    </owl:NamedIndividual>
    


    <!-- http://w3id.org/um/cbcm/eu-cm-ontology#gr913 -->

    <owl:NamedIndividual rdf:about="http://w3id.org/um/cbcm/eu-cm-ontology#gr913">
        <rdf:type rdf:resource="http://w3id.org/um/cbcm/eu-cm-ontology#CompanyLegalForm"/>
        <dc:title xml:lang="gr">  Nomika Prosopa Dimosiou Dikeou</dc:title>
        <dc:title xml:lang="en">Legal Entities of Public Law</dc:title>
        <dc:title xml:lang="gr">Νομικά Πρόσωπα Δημοσίου Δικαίου </dc:title>
        <rdfs:label rdf:datatype="http://www.w3.org/2001/XMLSchema#string">PL</rdfs:label>
    </owl:NamedIndividual>
    


    <!-- http://w3id.org/um/cbcm/eu-cm-ontology#gr999 -->

    <owl:NamedIndividual rdf:about="http://w3id.org/um/cbcm/eu-cm-ontology#gr999">
        <rdf:type rdf:resource="http://w3id.org/um/cbcm/eu-cm-ontology#CompanyLegalForm"/>
        <dc:title xml:lang="gr"> Lipa</dc:title>
        <dc:title xml:lang="en">Other Legal Forms</dc:title>
        <dc:title xml:lang="gr">Λοιπά </dc:title>
        <rdfs:label rdf:datatype="http://www.w3.org/2001/XMLSchema#string">Other</rdfs:label>
    </owl:NamedIndividual>
    


    <!-- http://w3id.org/um/cbcm/eu-cm-ontology#greece -->

    <owl:NamedIndividual rdf:about="http://w3id.org/um/cbcm/eu-cm-ontology#greece">
        <rdf:type rdf:resource="http://w3id.org/um/cbcm/eu-cm-ontology#EUCountry"/>
        <cbcm:countryHasCompanyForm rdf:resource="http://w3id.org/um/cbcm/eu-cm-ontology#gr901"/>
        <cbcm:countryHasCompanyForm rdf:resource="http://w3id.org/um/cbcm/eu-cm-ontology#gr902"/>
        <cbcm:countryHasCompanyForm rdf:resource="http://w3id.org/um/cbcm/eu-cm-ontology#gr903"/>
        <cbcm:countryHasCompanyForm rdf:resource="http://w3id.org/um/cbcm/eu-cm-ontology#gr904"/>
        <cbcm:countryHasCompanyForm rdf:resource="http://w3id.org/um/cbcm/eu-cm-ontology#gr905"/>
        <cbcm:countryHasCompanyForm rdf:resource="http://w3id.org/um/cbcm/eu-cm-ontology#gr906"/>
        <cbcm:countryHasCompanyForm rdf:resource="http://w3id.org/um/cbcm/eu-cm-ontology#gr907"/>
        <cbcm:countryHasCompanyForm rdf:resource="http://w3id.org/um/cbcm/eu-cm-ontology#gr908"/>
        <cbcm:countryHasCompanyForm rdf:resource="http://w3id.org/um/cbcm/eu-cm-ontology#gr909"/>
        <cbcm:countryHasCompanyForm rdf:resource="http://w3id.org/um/cbcm/eu-cm-ontology#gr910"/>
        <cbcm:countryHasCompanyForm rdf:resource="http://w3id.org/um/cbcm/eu-cm-ontology#gr911"/>
        <cbcm:countryHasCompanyForm rdf:resource="http://w3id.org/um/cbcm/eu-cm-ontology#gr912"/>
        <cbcm:countryHasCompanyForm rdf:resource="http://w3id.org/um/cbcm/eu-cm-ontology#gr913"/>
        <cbcm:countryHasCompanyForm rdf:resource="http://w3id.org/um/cbcm/eu-cm-ontology#gr999"/>
        <cbcm:iso2code>EL</cbcm:iso2code>
        <cbcm:iso2code>GR</cbcm:iso2code>
        <rdfs:label xml:lang="gr">Ellada</rdfs:label>
        <rdfs:label xml:lang="en">Greece</rdfs:label>
        <rdfs:label xml:lang="gr">Ελλάδα</rdfs:label>
    </owl:NamedIndividual>
    


    <!-- http://w3id.org/um/cbcm/eu-cm-ontology#hr01 -->

    <owl:NamedIndividual rdf:about="http://w3id.org/um/cbcm/eu-cm-ontology#hr01">
        <rdf:type rdf:resource="http://w3id.org/um/cbcm/eu-cm-ontology#CompanyLegalForm"/>
        <dc:title xml:lang="hr">Dioničko društvo</dc:title>
        <dc:title xml:lang="en">Joint stock company</dc:title>
        <rdfs:label rdf:datatype="http://www.w3.org/2001/XMLSchema#string">d.d.</rdfs:label>
    </owl:NamedIndividual>
    


    <!-- http://w3id.org/um/cbcm/eu-cm-ontology#hr02 -->

    <owl:NamedIndividual rdf:about="http://w3id.org/um/cbcm/eu-cm-ontology#hr02">
        <rdf:type rdf:resource="http://w3id.org/um/cbcm/eu-cm-ontology#CompanyLegalForm"/>
        <dc:title xml:lang="hr">Društvo s ograničenom odgovornošću</dc:title>
        <dc:title xml:lang="en">Limited liability company</dc:title>
        <rdfs:label rdf:datatype="http://www.w3.org/2001/XMLSchema#string">d.o.o.</rdfs:label>
    </owl:NamedIndividual>
    


    <!-- http://w3id.org/um/cbcm/eu-cm-ontology#hr03 -->

    <owl:NamedIndividual rdf:about="http://w3id.org/um/cbcm/eu-cm-ontology#hr03">
        <rdf:type rdf:resource="http://w3id.org/um/cbcm/eu-cm-ontology#CompanyLegalForm"/>
        <dc:title xml:lang="hr">Javno trgovačko društvo</dc:title>
        <dc:title xml:lang="en">Public company</dc:title>
        <rdfs:label rdf:datatype="http://www.w3.org/2001/XMLSchema#string">j.t.d</rdfs:label>
    </owl:NamedIndividual>
    


    <!-- http://w3id.org/um/cbcm/eu-cm-ontology#hr04 -->

    <owl:NamedIndividual rdf:about="http://w3id.org/um/cbcm/eu-cm-ontology#hr04">
        <rdf:type rdf:resource="http://w3id.org/um/cbcm/eu-cm-ontology#CompanyLegalForm"/>
        <dc:title xml:lang="hr">Komanditno društvo</dc:title>
        <dc:title xml:lang="en">Limited partnership</dc:title>
        <rdfs:label rdf:datatype="http://www.w3.org/2001/XMLSchema#string">k.d.</rdfs:label>
    </owl:NamedIndividual>
    


    <!-- http://w3id.org/um/cbcm/eu-cm-ontology#hr08 -->

    <owl:NamedIndividual rdf:about="http://w3id.org/um/cbcm/eu-cm-ontology#hr08">
        <rdf:type rdf:resource="http://w3id.org/um/cbcm/eu-cm-ontology#CompanyLegalForm"/>
        <dc:title xml:lang="hr">Jednostavno društvo s ograničenom odgovornošću</dc:title>
        <dc:title xml:lang="en">Simple limited liability company</dc:title>
        <rdfs:label rdf:datatype="http://www.w3.org/2001/XMLSchema#string">j.d.o.o.</rdfs:label>
    </owl:NamedIndividual>
    


    <!-- http://w3id.org/um/cbcm/eu-cm-ontology#hr16 -->

    <owl:NamedIndividual rdf:about="http://w3id.org/um/cbcm/eu-cm-ontology#hr16">
        <rdf:type rdf:resource="http://w3id.org/um/cbcm/eu-cm-ontology#CompanyLegalForm"/>
        <dc:title xml:lang="en">Economic interest grouping</dc:title>
        <dc:title xml:lang="hr">Gospodarsko interesno udruženje</dc:title>
        <rdfs:label rdf:datatype="http://www.w3.org/2001/XMLSchema#string">GIU</rdfs:label>
    </owl:NamedIndividual>
    


    <!-- http://w3id.org/um/cbcm/eu-cm-ontology#hr45 -->

    <owl:NamedIndividual rdf:about="http://w3id.org/um/cbcm/eu-cm-ontology#hr45">
        <rdf:type rdf:resource="http://w3id.org/um/cbcm/eu-cm-ontology#CompanyLegalForm"/>
        <dc:title xml:lang="en">Sport joint-stock company</dc:title>
        <dc:title xml:lang="hr">Športsko dioničko društvo</dc:title>
        <rdfs:label rdf:datatype="http://www.w3.org/2001/XMLSchema#string">s.d.d</rdfs:label>
    </owl:NamedIndividual>
    


    <!-- http://w3id.org/um/cbcm/eu-cm-ontology#hu113 -->

    <owl:NamedIndividual rdf:about="http://w3id.org/um/cbcm/eu-cm-ontology#hu113">
        <rdf:type rdf:resource="http://w3id.org/um/cbcm/eu-cm-ontology#CompanyLegalForm"/>
        <dc:title xml:lang="hu">Korlátolt felelősségű társaság</dc:title>
        <dc:title xml:lang="en">Private limited-liability company</dc:title>
        <rdfs:label rdf:datatype="http://www.w3.org/2001/XMLSchema#string">Kft.</rdfs:label>
    </owl:NamedIndividual>
    


    <!-- http://w3id.org/um/cbcm/eu-cm-ontology#hu114 -->

    <owl:NamedIndividual rdf:about="http://w3id.org/um/cbcm/eu-cm-ontology#hu114">
        <rdf:type rdf:resource="http://w3id.org/um/cbcm/eu-cm-ontology#CompanyLegalForm"/>
        <dc:title xml:lang="en">Limited company</dc:title>
        <dc:title xml:lang="hu">Részvénytársaság</dc:title>
        <rdfs:label rdf:datatype="http://www.w3.org/2001/XMLSchema#string">Rt.</rdfs:label>
    </owl:NamedIndividual>
    


    <!-- http://w3id.org/um/cbcm/eu-cm-ontology#hu116 -->

    <owl:NamedIndividual rdf:about="http://w3id.org/um/cbcm/eu-cm-ontology#hu116">
        <rdf:type rdf:resource="http://w3id.org/um/cbcm/eu-cm-ontology#CompanyLegalForm"/>
        <dc:title xml:lang="en">General partnership</dc:title>
        <dc:title xml:lang="hu">Közkereseti társaság</dc:title>
        <rdfs:label rdf:datatype="http://www.w3.org/2001/XMLSchema#string">Kkt.</rdfs:label>
    </owl:NamedIndividual>
    


    <!-- http://w3id.org/um/cbcm/eu-cm-ontology#hu117 -->

    <owl:NamedIndividual rdf:about="http://w3id.org/um/cbcm/eu-cm-ontology#hu117">
        <rdf:type rdf:resource="http://w3id.org/um/cbcm/eu-cm-ontology#CompanyLegalForm"/>
        <dc:title xml:lang="hu">Betéti társaság</dc:title>
        <dc:title xml:lang="en">Limited partnership</dc:title>
        <rdfs:label rdf:datatype="http://www.w3.org/2001/XMLSchema#string">Bt.</rdfs:label>
    </owl:NamedIndividual>
    


    <!-- http://w3id.org/um/cbcm/eu-cm-ontology#hu736 -->

    <owl:NamedIndividual rdf:about="http://w3id.org/um/cbcm/eu-cm-ontology#hu736">
        <rdf:type rdf:resource="http://w3id.org/um/cbcm/eu-cm-ontology#CompanyLegalForm"/>
        <dc:title xml:lang="hu">Közhasznú társaság</dc:title>
        <dc:title xml:lang="en">Public benefit nonprofit institution</dc:title>
        <rdfs:label rdf:datatype="http://www.w3.org/2001/XMLSchema#string">Kht.</rdfs:label>
    </owl:NamedIndividual>
    


    <!-- http://w3id.org/um/cbcm/eu-cm-ontology#hu916 -->

    <owl:NamedIndividual rdf:about="http://w3id.org/um/cbcm/eu-cm-ontology#hu916">
        <rdf:type rdf:resource="http://w3id.org/um/cbcm/eu-cm-ontology#CompanyLegalForm"/>
        <dc:title xml:lang="en">National deposit insurance fund</dc:title>
        <dc:title xml:lang="hu">Országos betétbiztosítási alap</dc:title>
        <rdfs:label rdf:datatype="http://www.w3.org/2001/XMLSchema#string">OBA</rdfs:label>
    </owl:NamedIndividual>
    


    <!-- http://w3id.org/um/cbcm/eu-cm-ontology#hungary -->

    <owl:NamedIndividual rdf:about="http://w3id.org/um/cbcm/eu-cm-ontology#hungary">
        <rdf:type rdf:resource="http://w3id.org/um/cbcm/eu-cm-ontology#EUCountry"/>
        <cbcm:countryHasCompanyForm rdf:resource="http://w3id.org/um/cbcm/eu-cm-ontology#hu113"/>
        <cbcm:countryHasCompanyForm rdf:resource="http://w3id.org/um/cbcm/eu-cm-ontology#hu114"/>
        <cbcm:countryHasCompanyForm rdf:resource="http://w3id.org/um/cbcm/eu-cm-ontology#hu116"/>
        <cbcm:countryHasCompanyForm rdf:resource="http://w3id.org/um/cbcm/eu-cm-ontology#hu117"/>
        <cbcm:countryHasCompanyForm rdf:resource="http://w3id.org/um/cbcm/eu-cm-ontology#hu736"/>
        <cbcm:countryHasCompanyForm rdf:resource="http://w3id.org/um/cbcm/eu-cm-ontology#hu916"/>
        <cbcm:iso2code>HU</cbcm:iso2code>
        <rdfs:label xml:lang="en">Hungary</rdfs:label>
        <rdfs:label xml:lang="hu">Magyarország</rdfs:label>
    </owl:NamedIndividual>
    


    <!-- http://w3id.org/um/cbcm/eu-cm-ontology#iceland -->

    <owl:NamedIndividual rdf:about="http://w3id.org/um/cbcm/eu-cm-ontology#iceland">
        <rdf:type rdf:resource="http://w3id.org/um/cbcm/eu-cm-ontology#EEACountry"/>
        <cbcm:iso2code>IS</cbcm:iso2code>
        <rdfs:label xml:lang="en">Iceland</rdfs:label>
        <rdfs:label xml:lang="is">Ísland</rdfs:label>
    </owl:NamedIndividual>
    


    <!-- http://w3id.org/um/cbcm/eu-cm-ontology#ie01 -->

    <owl:NamedIndividual rdf:about="http://w3id.org/um/cbcm/eu-cm-ontology#ie01">
        <rdf:type rdf:resource="http://w3id.org/um/cbcm/eu-cm-ontology#CompanyLegalForm"/>
        <dc:title xml:lang="en"></dc:title>
        <dc:title xml:lang="ie">Private Company Limited by Shares (LTD company)</dc:title>
        <rdfs:label rdf:datatype="http://www.w3.org/2001/XMLSchema#string">LTD</rdfs:label>
    </owl:NamedIndividual>
    


    <!-- http://w3id.org/um/cbcm/eu-cm-ontology#ie02 -->

    <owl:NamedIndividual rdf:about="http://w3id.org/um/cbcm/eu-cm-ontology#ie02">
        <rdf:type rdf:resource="http://w3id.org/um/cbcm/eu-cm-ontology#CompanyLegalForm"/>
        <dc:title xml:lang="en"></dc:title>
        <dc:title xml:lang="ie">Designated Activity Company (DAC) – (limited by shares). </dc:title>
        <rdfs:label rdf:datatype="http://www.w3.org/2001/XMLSchema#string">DAC</rdfs:label>
    </owl:NamedIndividual>
    


    <!-- http://w3id.org/um/cbcm/eu-cm-ontology#ie03 -->

    <owl:NamedIndividual rdf:about="http://w3id.org/um/cbcm/eu-cm-ontology#ie03">
        <rdf:type rdf:resource="http://w3id.org/um/cbcm/eu-cm-ontology#CompanyLegalForm"/>
        <dc:title xml:lang="en"></dc:title>
        <dc:title xml:lang="ie">Designated Activity Company Limited by Guarantee (DAC) – (limited by guarantee)</dc:title>
        <rdfs:label rdf:datatype="http://www.w3.org/2001/XMLSchema#string">DAC</rdfs:label>
    </owl:NamedIndividual>
    


    <!-- http://w3id.org/um/cbcm/eu-cm-ontology#ie04 -->

    <owl:NamedIndividual rdf:about="http://w3id.org/um/cbcm/eu-cm-ontology#ie04">
        <rdf:type rdf:resource="http://w3id.org/um/cbcm/eu-cm-ontology#CompanyLegalForm"/>
        <dc:title xml:lang="en"></dc:title>
        <dc:title xml:lang="ie">Company Limited by Guarantee (CLG) (limited by guarantee not having a share capital)</dc:title>
        <rdfs:label rdf:datatype="http://www.w3.org/2001/XMLSchema#string">CLG</rdfs:label>
    </owl:NamedIndividual>
    


    <!-- http://w3id.org/um/cbcm/eu-cm-ontology#ie05 -->

    <owl:NamedIndividual rdf:about="http://w3id.org/um/cbcm/eu-cm-ontology#ie05">
        <rdf:type rdf:resource="http://w3id.org/um/cbcm/eu-cm-ontology#CompanyLegalForm"/>
        <dc:title xml:lang="en"></dc:title>
        <dc:title xml:lang="ie">Public Limited Company (PLC)</dc:title>
        <rdfs:label rdf:datatype="http://www.w3.org/2001/XMLSchema#string">PLC</rdfs:label>
    </owl:NamedIndividual>
    


    <!-- http://w3id.org/um/cbcm/eu-cm-ontology#ie06 -->

    <owl:NamedIndividual rdf:about="http://w3id.org/um/cbcm/eu-cm-ontology#ie06">
        <rdf:type rdf:resource="http://w3id.org/um/cbcm/eu-cm-ontology#CompanyLegalForm"/>
        <dc:title xml:lang="en"></dc:title>
        <dc:title xml:lang="ie">Single Member Company</dc:title>
        <rdfs:label rdf:datatype="http://www.w3.org/2001/XMLSchema#string">SMC</rdfs:label>
    </owl:NamedIndividual>
    


    <!-- http://w3id.org/um/cbcm/eu-cm-ontology#ie07 -->

    <owl:NamedIndividual rdf:about="http://w3id.org/um/cbcm/eu-cm-ontology#ie07">
        <rdf:type rdf:resource="http://w3id.org/um/cbcm/eu-cm-ontology#CompanyLegalForm"/>
        <dc:title xml:lang="en"></dc:title>
        <dc:title xml:lang="ie">Unlimited companyxa0</dc:title>
        <rdfs:label rdf:datatype="http://www.w3.org/2001/XMLSchema#string">UC</rdfs:label>
    </owl:NamedIndividual>
    


    <!-- http://w3id.org/um/cbcm/eu-cm-ontology#ie08 -->

    <owl:NamedIndividual rdf:about="http://w3id.org/um/cbcm/eu-cm-ontology#ie08">
        <rdf:type rdf:resource="http://w3id.org/um/cbcm/eu-cm-ontology#CompanyLegalForm"/>
        <dc:title xml:lang="en"></dc:title>
        <dc:title xml:lang="ie">Undertakings for Collective Investment in Transferable Securities (UCITS)xa0</dc:title>
        <rdfs:label rdf:datatype="http://www.w3.org/2001/XMLSchema#string">UCITS</rdfs:label>
    </owl:NamedIndividual>
    


    <!-- http://w3id.org/um/cbcm/eu-cm-ontology#ireland -->

    <owl:NamedIndividual rdf:about="http://w3id.org/um/cbcm/eu-cm-ontology#ireland">
        <rdf:type rdf:resource="http://w3id.org/um/cbcm/eu-cm-ontology#EUCountry"/>
        <cbcm:countryHasCompanyForm rdf:resource="http://w3id.org/um/cbcm/eu-cm-ontology#ie01"/>
        <cbcm:countryHasCompanyForm rdf:resource="http://w3id.org/um/cbcm/eu-cm-ontology#ie02"/>
        <cbcm:countryHasCompanyForm rdf:resource="http://w3id.org/um/cbcm/eu-cm-ontology#ie03"/>
        <cbcm:countryHasCompanyForm rdf:resource="http://w3id.org/um/cbcm/eu-cm-ontology#ie04"/>
        <cbcm:countryHasCompanyForm rdf:resource="http://w3id.org/um/cbcm/eu-cm-ontology#ie05"/>
        <cbcm:countryHasCompanyForm rdf:resource="http://w3id.org/um/cbcm/eu-cm-ontology#ie06"/>
        <cbcm:countryHasCompanyForm rdf:resource="http://w3id.org/um/cbcm/eu-cm-ontology#ie07"/>
        <cbcm:countryHasCompanyForm rdf:resource="http://w3id.org/um/cbcm/eu-cm-ontology#ie08"/>
        <cbcm:iso2code>IE</cbcm:iso2code>
        <rdfs:label xml:lang="en">Ireland</rdfs:label>
        <rdfs:label xml:lang="ga">Éire</rdfs:label>
    </owl:NamedIndividual>
    


    <!-- http://w3id.org/um/cbcm/eu-cm-ontology#it101 -->

    <owl:NamedIndividual rdf:about="http://w3id.org/um/cbcm/eu-cm-ontology#it101">
        <rdf:type rdf:resource="http://w3id.org/um/cbcm/eu-cm-ontology#CompanyLegalForm"/>
        <dc:title xml:lang="en">General government</dc:title>
        <dc:title xml:lang="it">PUBBLICA AMMINISTRAZIONE</dc:title>
        <rdfs:label rdf:datatype="http://www.w3.org/2001/XMLSchema#string">PA</rdfs:label>
    </owl:NamedIndividual>
    


    <!-- http://w3id.org/um/cbcm/eu-cm-ontology#it201 -->

    <owl:NamedIndividual rdf:about="http://w3id.org/um/cbcm/eu-cm-ontology#it201">
        <rdf:type rdf:resource="http://w3id.org/um/cbcm/eu-cm-ontology#CompanyLegalForm"/>
        <dc:title xml:lang="en">General partnership (commercial)</dc:title>
        <dc:title xml:lang="it">SOCIETA IN NOME COLLETTIVO</dc:title>
        <rdfs:label rdf:datatype="http://www.w3.org/2001/XMLSchema#string">SNC</rdfs:label>
    </owl:NamedIndividual>
    


    <!-- http://w3id.org/um/cbcm/eu-cm-ontology#it301 -->

    <owl:NamedIndividual rdf:about="http://w3id.org/um/cbcm/eu-cm-ontology#it301">
        <rdf:type rdf:resource="http://w3id.org/um/cbcm/eu-cm-ontology#CompanyLegalForm"/>
        <dc:title xml:lang="en">Limited partnership</dc:title>
        <dc:title xml:lang="it">SOCIETA IN ACCOMANDITA SEMPLICE</dc:title>
        <rdfs:label rdf:datatype="http://www.w3.org/2001/XMLSchema#string">SAS</rdfs:label>
    </owl:NamedIndividual>
    


    <!-- http://w3id.org/um/cbcm/eu-cm-ontology#it401 -->

    <owl:NamedIndividual rdf:about="http://w3id.org/um/cbcm/eu-cm-ontology#it401">
        <rdf:type rdf:resource="http://w3id.org/um/cbcm/eu-cm-ontology#CompanyLegalForm"/>
        <dc:title xml:lang="en">General partnership (non commercial)</dc:title>
        <dc:title xml:lang="it">SOCIETA SEMPLICE</dc:title>
        <rdfs:label rdf:datatype="http://www.w3.org/2001/XMLSchema#string">SS</rdfs:label>
    </owl:NamedIndividual>
    


    <!-- http://w3id.org/um/cbcm/eu-cm-ontology#it402 -->

    <owl:NamedIndividual rdf:about="http://w3id.org/um/cbcm/eu-cm-ontology#it402">
        <rdf:type rdf:resource="http://w3id.org/um/cbcm/eu-cm-ontology#CompanyLegalForm"/>
        <dc:title xml:lang="en">De facto corporation</dc:title>
        <dc:title xml:lang="it">SOCIETA DI FATTO</dc:title>
        <rdfs:label rdf:datatype="http://www.w3.org/2001/XMLSchema#string">SDF</rdfs:label>
    </owl:NamedIndividual>
    


    <!-- http://w3id.org/um/cbcm/eu-cm-ontology#it501 -->

    <owl:NamedIndividual rdf:about="http://w3id.org/um/cbcm/eu-cm-ontology#it501">
        <rdf:type rdf:resource="http://w3id.org/um/cbcm/eu-cm-ontology#CompanyLegalForm"/>
        <dc:title xml:lang="it">  CONSORZIO</dc:title>
        <dc:title xml:lang="it">AZIENDA PROVINCIALE </dc:title>
        <dc:title xml:lang="en">Consortium</dc:title>
        <rdfs:label rdf:datatype="http://www.w3.org/2001/XMLSchema#string">AIMP</rdfs:label>
    </owl:NamedIndividual>
    


    <!-- http://w3id.org/um/cbcm/eu-cm-ontology#it601 -->

    <owl:NamedIndividual rdf:about="http://w3id.org/um/cbcm/eu-cm-ontology#it601">
        <rdf:type rdf:resource="http://w3id.org/um/cbcm/eu-cm-ontology#CompanyLegalForm"/>
        <dc:title xml:lang="en">Cooperative society</dc:title>
        <dc:title xml:lang="it">SOCIETA COOPERATIVA</dc:title>
        <rdfs:label rdf:datatype="http://www.w3.org/2001/XMLSchema#string">COOP</rdfs:label>
    </owl:NamedIndividual>
    


    <!-- http://w3id.org/um/cbcm/eu-cm-ontology#it701 -->

    <owl:NamedIndividual rdf:about="http://w3id.org/um/cbcm/eu-cm-ontology#it701">
        <rdf:type rdf:resource="http://w3id.org/um/cbcm/eu-cm-ontology#CompanyLegalForm"/>
        <dc:title xml:lang="en">Plc (UK)</dc:title>
        <dc:title xml:lang="it">SOCIETA PER AZIONI</dc:title>
        <rdfs:label rdf:datatype="http://www.w3.org/2001/XMLSchema#string">SPA</rdfs:label>
    </owl:NamedIndividual>
    


    <!-- http://w3id.org/um/cbcm/eu-cm-ontology#it702 -->

    <owl:NamedIndividual rdf:about="http://w3id.org/um/cbcm/eu-cm-ontology#it702">
        <rdf:type rdf:resource="http://w3id.org/um/cbcm/eu-cm-ontology#CompanyLegalForm"/>
        <dc:title xml:lang="en">Partnership limited by shares</dc:title>
        <dc:title xml:lang="it">SOCIETA IN ACCOMANDITA PER AZIONI</dc:title>
        <rdfs:label rdf:datatype="http://www.w3.org/2001/XMLSchema#string">SAA</rdfs:label>
    </owl:NamedIndividual>
    


    <!-- http://w3id.org/um/cbcm/eu-cm-ontology#it703 -->

    <owl:NamedIndividual rdf:about="http://w3id.org/um/cbcm/eu-cm-ontology#it703">
        <rdf:type rdf:resource="http://w3id.org/um/cbcm/eu-cm-ontology#CompanyLegalForm"/>
        <dc:title xml:lang="en">Ltd (UK)</dc:title>
        <dc:title xml:lang="it">SOCIETA A RESPONSABILITA LIMITATA</dc:title>
        <rdfs:label rdf:datatype="http://www.w3.org/2001/XMLSchema#string">SRL</rdfs:label>
    </owl:NamedIndividual>
    


    <!-- http://w3id.org/um/cbcm/eu-cm-ontology#italy -->

    <owl:NamedIndividual rdf:about="http://w3id.org/um/cbcm/eu-cm-ontology#italy">
        <rdf:type rdf:resource="http://w3id.org/um/cbcm/eu-cm-ontology#EUCountry"/>
        <cbcm:countryHasCompanyForm rdf:resource="http://w3id.org/um/cbcm/eu-cm-ontology#it101"/>
        <cbcm:countryHasCompanyForm rdf:resource="http://w3id.org/um/cbcm/eu-cm-ontology#it201"/>
        <cbcm:countryHasCompanyForm rdf:resource="http://w3id.org/um/cbcm/eu-cm-ontology#it301"/>
        <cbcm:countryHasCompanyForm rdf:resource="http://w3id.org/um/cbcm/eu-cm-ontology#it401"/>
        <cbcm:countryHasCompanyForm rdf:resource="http://w3id.org/um/cbcm/eu-cm-ontology#it402"/>
        <cbcm:countryHasCompanyForm rdf:resource="http://w3id.org/um/cbcm/eu-cm-ontology#it501"/>
        <cbcm:countryHasCompanyForm rdf:resource="http://w3id.org/um/cbcm/eu-cm-ontology#it601"/>
        <cbcm:countryHasCompanyForm rdf:resource="http://w3id.org/um/cbcm/eu-cm-ontology#it701"/>
        <cbcm:countryHasCompanyForm rdf:resource="http://w3id.org/um/cbcm/eu-cm-ontology#it702"/>
        <cbcm:countryHasCompanyForm rdf:resource="http://w3id.org/um/cbcm/eu-cm-ontology#it703"/>
        <cbcm:iso2code>IT</cbcm:iso2code>
        <rdfs:label xml:lang="it">Italia</rdfs:label>
        <rdfs:label xml:lang="en">Italian Republic</rdfs:label>
        <rdfs:label xml:lang="en">Italy</rdfs:label>
        <rdfs:label xml:lang="it">Repubblica Italiana</rdfs:label>
    </owl:NamedIndividual>
    


    <!-- http://w3id.org/um/cbcm/eu-cm-ontology#latvia -->

    <owl:NamedIndividual rdf:about="http://w3id.org/um/cbcm/eu-cm-ontology#latvia">
        <rdf:type rdf:resource="http://w3id.org/um/cbcm/eu-cm-ontology#EUCountry"/>
        <cbcm:countryHasCompanyForm rdf:resource="http://w3id.org/um/cbcm/eu-cm-ontology#lv101"/>
        <cbcm:countryHasCompanyForm rdf:resource="http://w3id.org/um/cbcm/eu-cm-ontology#lv103"/>
        <cbcm:countryHasCompanyForm rdf:resource="http://w3id.org/um/cbcm/eu-cm-ontology#lv104"/>
        <cbcm:countryHasCompanyForm rdf:resource="http://w3id.org/um/cbcm/eu-cm-ontology#lv105"/>
        <cbcm:countryHasCompanyForm rdf:resource="http://w3id.org/um/cbcm/eu-cm-ontology#lv106"/>
        <cbcm:countryHasCompanyForm rdf:resource="http://w3id.org/um/cbcm/eu-cm-ontology#lv107"/>
        <cbcm:countryHasCompanyForm rdf:resource="http://w3id.org/um/cbcm/eu-cm-ontology#lv108"/>
        <cbcm:countryHasCompanyForm rdf:resource="http://w3id.org/um/cbcm/eu-cm-ontology#lv109"/>
        <cbcm:countryHasCompanyForm rdf:resource="http://w3id.org/um/cbcm/eu-cm-ontology#lv110"/>
        <cbcm:countryHasCompanyForm rdf:resource="http://w3id.org/um/cbcm/eu-cm-ontology#lv111"/>
        <cbcm:countryHasCompanyForm rdf:resource="http://w3id.org/um/cbcm/eu-cm-ontology#lv301"/>
        <cbcm:countryHasCompanyForm rdf:resource="http://w3id.org/um/cbcm/eu-cm-ontology#lv302"/>
        <cbcm:countryHasCompanyForm rdf:resource="http://w3id.org/um/cbcm/eu-cm-ontology#lv303"/>
        <cbcm:countryHasCompanyForm rdf:resource="http://w3id.org/um/cbcm/eu-cm-ontology#lv401"/>
        <cbcm:countryHasCompanyForm rdf:resource="http://w3id.org/um/cbcm/eu-cm-ontology#lv402"/>
        <cbcm:countryHasCompanyForm rdf:resource="http://w3id.org/um/cbcm/eu-cm-ontology#lv403"/>
        <cbcm:countryHasCompanyForm rdf:resource="http://w3id.org/um/cbcm/eu-cm-ontology#lv404"/>
        <cbcm:countryHasCompanyForm rdf:resource="http://w3id.org/um/cbcm/eu-cm-ontology#lv405"/>
        <cbcm:countryHasCompanyForm rdf:resource="http://w3id.org/um/cbcm/eu-cm-ontology#lv406"/>
        <cbcm:countryHasCompanyForm rdf:resource="http://w3id.org/um/cbcm/eu-cm-ontology#lv701"/>
        <cbcm:countryHasCompanyForm rdf:resource="http://w3id.org/um/cbcm/eu-cm-ontology#lv801"/>
        <cbcm:countryHasCompanyForm rdf:resource="http://w3id.org/um/cbcm/eu-cm-ontology#lv802"/>
        <cbcm:countryHasCompanyForm rdf:resource="http://w3id.org/um/cbcm/eu-cm-ontology#lv803"/>
        <cbcm:countryHasCompanyForm rdf:resource="http://w3id.org/um/cbcm/eu-cm-ontology#lv804"/>
        <cbcm:countryHasCompanyForm rdf:resource="http://w3id.org/um/cbcm/eu-cm-ontology#lv805"/>
        <cbcm:countryHasCompanyForm rdf:resource="http://w3id.org/um/cbcm/eu-cm-ontology#lv806"/>
        <cbcm:countryHasCompanyForm rdf:resource="http://w3id.org/um/cbcm/eu-cm-ontology#lv807"/>
        <cbcm:countryHasCompanyForm rdf:resource="http://w3id.org/um/cbcm/eu-cm-ontology#lv808"/>
        <cbcm:countryHasCompanyForm rdf:resource="http://w3id.org/um/cbcm/eu-cm-ontology#lv809"/>
        <cbcm:countryHasCompanyForm rdf:resource="http://w3id.org/um/cbcm/eu-cm-ontology#lv810"/>
        <cbcm:countryHasCompanyForm rdf:resource="http://w3id.org/um/cbcm/eu-cm-ontology#lv903"/>
        <cbcm:iso2code>LV</cbcm:iso2code>
        <rdfs:label xml:lang="en">Latvia</rdfs:label>
        <rdfs:label xml:lang="lv">Latvija</rdfs:label>
        <rdfs:label xml:lang="lv">Latvijas Republika</rdfs:label>
        <rdfs:label xml:lang="en">Republic of Latvia</rdfs:label>
    </owl:NamedIndividual>
    


    <!-- http://w3id.org/um/cbcm/eu-cm-ontology#liechtenstein -->

    <owl:NamedIndividual rdf:about="http://w3id.org/um/cbcm/eu-cm-ontology#liechtenstein">
        <rdf:type rdf:resource="http://w3id.org/um/cbcm/eu-cm-ontology#EEACountry"/>
        <cbcm:iso2code>LI</cbcm:iso2code>
        <rdfs:label xml:lang="de">Fürstentum Liechtenstein</rdfs:label>
        <rdfs:label xml:lang="en">Liechtenstein</rdfs:label>
        <rdfs:label xml:lang="en">Principality of Liechtenstein</rdfs:label>
    </owl:NamedIndividual>
    


    <!-- http://w3id.org/um/cbcm/eu-cm-ontology#lithuania -->

    <owl:NamedIndividual rdf:about="http://w3id.org/um/cbcm/eu-cm-ontology#lithuania">
        <rdf:type rdf:resource="http://w3id.org/um/cbcm/eu-cm-ontology#EUCountry"/>
        <cbcm:countryHasCompanyForm rdf:resource="http://w3id.org/um/cbcm/eu-cm-ontology#lt101"/>
        <cbcm:countryHasCompanyForm rdf:resource="http://w3id.org/um/cbcm/eu-cm-ontology#lt102"/>
        <cbcm:countryHasCompanyForm rdf:resource="http://w3id.org/um/cbcm/eu-cm-ontology#lt103"/>
        <cbcm:countryHasCompanyForm rdf:resource="http://w3id.org/um/cbcm/eu-cm-ontology#lt104"/>
        <cbcm:countryHasCompanyForm rdf:resource="http://w3id.org/um/cbcm/eu-cm-ontology#lt105"/>
        <cbcm:countryHasCompanyForm rdf:resource="http://w3id.org/um/cbcm/eu-cm-ontology#lt106"/>
        <cbcm:countryHasCompanyForm rdf:resource="http://w3id.org/um/cbcm/eu-cm-ontology#lt107"/>
        <cbcm:countryHasCompanyForm rdf:resource="http://w3id.org/um/cbcm/eu-cm-ontology#lt108"/>
        <cbcm:countryHasCompanyForm rdf:resource="http://w3id.org/um/cbcm/eu-cm-ontology#lt109"/>
        <cbcm:countryHasCompanyForm rdf:resource="http://w3id.org/um/cbcm/eu-cm-ontology#lt110"/>
        <cbcm:countryHasCompanyForm rdf:resource="http://w3id.org/um/cbcm/eu-cm-ontology#lt111"/>
        <cbcm:countryHasCompanyForm rdf:resource="http://w3id.org/um/cbcm/eu-cm-ontology#lt201"/>
        <cbcm:countryHasCompanyForm rdf:resource="http://w3id.org/um/cbcm/eu-cm-ontology#lt202"/>
        <cbcm:countryHasCompanyForm rdf:resource="http://w3id.org/um/cbcm/eu-cm-ontology#lt203"/>
        <cbcm:countryHasCompanyForm rdf:resource="http://w3id.org/um/cbcm/eu-cm-ontology#lt204"/>
        <cbcm:countryHasCompanyForm rdf:resource="http://w3id.org/um/cbcm/eu-cm-ontology#lt205"/>
        <cbcm:countryHasCompanyForm rdf:resource="http://w3id.org/um/cbcm/eu-cm-ontology#lt206"/>
        <cbcm:countryHasCompanyForm rdf:resource="http://w3id.org/um/cbcm/eu-cm-ontology#lt207"/>
        <cbcm:countryHasCompanyForm rdf:resource="http://w3id.org/um/cbcm/eu-cm-ontology#lt208"/>
        <cbcm:countryHasCompanyForm rdf:resource="http://w3id.org/um/cbcm/eu-cm-ontology#lt209"/>
        <cbcm:countryHasCompanyForm rdf:resource="http://w3id.org/um/cbcm/eu-cm-ontology#lt210"/>
        <cbcm:countryHasCompanyForm rdf:resource="http://w3id.org/um/cbcm/eu-cm-ontology#lt211"/>
        <cbcm:countryHasCompanyForm rdf:resource="http://w3id.org/um/cbcm/eu-cm-ontology#lt213"/>
        <cbcm:countryHasCompanyForm rdf:resource="http://w3id.org/um/cbcm/eu-cm-ontology#lt214"/>
        <cbcm:countryHasCompanyForm rdf:resource="http://w3id.org/um/cbcm/eu-cm-ontology#lt215"/>
        <cbcm:countryHasCompanyForm rdf:resource="http://w3id.org/um/cbcm/eu-cm-ontology#lt216"/>
        <cbcm:countryHasCompanyForm rdf:resource="http://w3id.org/um/cbcm/eu-cm-ontology#lt301"/>
        <cbcm:iso2code>LT</cbcm:iso2code>
        <rdfs:label xml:lang="lt">Lietuva</rdfs:label>
        <rdfs:label xml:lang="lt">Lietuvos Respublika</rdfs:label>
        <rdfs:label xml:lang="en">Lithuania</rdfs:label>
        <rdfs:label xml:lang="en">Republic of Lithuania</rdfs:label>
    </owl:NamedIndividual>
    


    <!-- http://w3id.org/um/cbcm/eu-cm-ontology#lt101 -->

    <owl:NamedIndividual rdf:about="http://w3id.org/um/cbcm/eu-cm-ontology#lt101">
        <rdf:type rdf:resource="http://w3id.org/um/cbcm/eu-cm-ontology#CompanyLegalForm"/>
        <dc:title xml:lang="lt">Akcinė bendrovė</dc:title>
        <dc:title xml:lang="en">Public Limited Company</dc:title>
        <rdfs:label rdf:datatype="http://www.w3.org/2001/XMLSchema#string">AB</rdfs:label>
    </owl:NamedIndividual>
    


    <!-- http://w3id.org/um/cbcm/eu-cm-ontology#lt102 -->

    <owl:NamedIndividual rdf:about="http://w3id.org/um/cbcm/eu-cm-ontology#lt102">
        <rdf:type rdf:resource="http://w3id.org/um/cbcm/eu-cm-ontology#CompanyLegalForm"/>
        <dc:title xml:lang="en">Private Limited Company</dc:title>
        <dc:title xml:lang="lt">Uždaroji akcinė bendrovė</dc:title>
        <rdfs:label rdf:datatype="http://www.w3.org/2001/XMLSchema#string">UAB</rdfs:label>
    </owl:NamedIndividual>
    


    <!-- http://w3id.org/um/cbcm/eu-cm-ontology#lt103 -->

    <owl:NamedIndividual rdf:about="http://w3id.org/um/cbcm/eu-cm-ontology#lt103">
        <rdf:type rdf:resource="http://w3id.org/um/cbcm/eu-cm-ontology#CompanyLegalForm"/>
        <dc:title xml:lang="en">Cooperative Society (Cooperative)</dc:title>
        <dc:title xml:lang="lt">Kooperatinė bendrovė (kooperatyvas)</dc:title>
        <rdfs:label rdf:datatype="http://www.w3.org/2001/XMLSchema#string">KO</rdfs:label>
    </owl:NamedIndividual>
    


    <!-- http://w3id.org/um/cbcm/eu-cm-ontology#lt104 -->

    <owl:NamedIndividual rdf:about="http://w3id.org/um/cbcm/eu-cm-ontology#lt104">
        <rdf:type rdf:resource="http://w3id.org/um/cbcm/eu-cm-ontology#CompanyLegalForm"/>
        <dc:title xml:lang="en">General Partnership</dc:title>
        <dc:title xml:lang="lt">Tikroji ūkinė bendrija</dc:title>
        <rdfs:label rdf:datatype="http://www.w3.org/2001/XMLSchema#string">TUB</rdfs:label>
    </owl:NamedIndividual>
    


    <!-- http://w3id.org/um/cbcm/eu-cm-ontology#lt105 -->

    <owl:NamedIndividual rdf:about="http://w3id.org/um/cbcm/eu-cm-ontology#lt105">
        <rdf:type rdf:resource="http://w3id.org/um/cbcm/eu-cm-ontology#CompanyLegalForm"/>
        <dc:title xml:lang="lt">Komanditinė ūkinė bendrija</dc:title>
        <dc:title xml:lang="en">Limited Partnership</dc:title>
        <rdfs:label rdf:datatype="http://www.w3.org/2001/XMLSchema#string">KUB</rdfs:label>
    </owl:NamedIndividual>
    


    <!-- http://w3id.org/um/cbcm/eu-cm-ontology#lt106 -->

    <owl:NamedIndividual rdf:about="http://w3id.org/um/cbcm/eu-cm-ontology#lt106">
        <rdf:type rdf:resource="http://w3id.org/um/cbcm/eu-cm-ontology#CompanyLegalForm"/>
        <dc:title xml:lang="lt">Asociacija</dc:title>
        <dc:title xml:lang="en">Association</dc:title>
        <rdfs:label rdf:datatype="http://www.w3.org/2001/XMLSchema#string">A</rdfs:label>
    </owl:NamedIndividual>
    


    <!-- http://w3id.org/um/cbcm/eu-cm-ontology#lt107 -->

    <owl:NamedIndividual rdf:about="http://w3id.org/um/cbcm/eu-cm-ontology#lt107">
        <rdf:type rdf:resource="http://w3id.org/um/cbcm/eu-cm-ontology#CompanyLegalForm"/>
        <dc:title xml:lang="lt">Mažoji bendrija</dc:title>
        <dc:title xml:lang="en">Small Partnership</dc:title>
        <rdfs:label rdf:datatype="http://www.w3.org/2001/XMLSchema#string">MB</rdfs:label>
    </owl:NamedIndividual>
    


    <!-- http://w3id.org/um/cbcm/eu-cm-ontology#lt108 -->

    <owl:NamedIndividual rdf:about="http://w3id.org/um/cbcm/eu-cm-ontology#lt108">
        <rdf:type rdf:resource="http://w3id.org/um/cbcm/eu-cm-ontology#CompanyLegalForm"/>
        <dc:title xml:lang="en">Agricultural Company</dc:title>
        <dc:title xml:lang="lt">Žemės ūkio bendrovė</dc:title>
        <rdfs:label rdf:datatype="http://www.w3.org/2001/XMLSchema#string">ZUB</rdfs:label>
    </owl:NamedIndividual>
    


    <!-- http://w3id.org/um/cbcm/eu-cm-ontology#lt109 -->

    <owl:NamedIndividual rdf:about="http://w3id.org/um/cbcm/eu-cm-ontology#lt109">
        <rdf:type rdf:resource="http://w3id.org/um/cbcm/eu-cm-ontology#CompanyLegalForm"/>
        <dc:title xml:lang="en">Individual Enterprise / Sole proprietorship</dc:title>
        <dc:title xml:lang="lt">Individuali įmonė</dc:title>
        <rdfs:label rdf:datatype="http://www.w3.org/2001/XMLSchema#string">II</rdfs:label>
    </owl:NamedIndividual>
    


    <!-- http://w3id.org/um/cbcm/eu-cm-ontology#lt110 -->

    <owl:NamedIndividual rdf:about="http://w3id.org/um/cbcm/eu-cm-ontology#lt110">
        <rdf:type rdf:resource="http://w3id.org/um/cbcm/eu-cm-ontology#CompanyLegalForm"/>
        <dc:title xml:lang="lt">Advokatų profesinė bendrija</dc:title>
        <dc:title xml:lang="en">Lawyers Professional Partnership</dc:title>
        <rdfs:label rdf:datatype="http://www.w3.org/2001/XMLSchema#string">APB</rdfs:label>
    </owl:NamedIndividual>
    


    <!-- http://w3id.org/um/cbcm/eu-cm-ontology#lt111 -->

    <owl:NamedIndividual rdf:about="http://w3id.org/um/cbcm/eu-cm-ontology#lt111">
        <rdf:type rdf:resource="http://w3id.org/um/cbcm/eu-cm-ontology#CompanyLegalForm"/>
        <dc:title xml:lang="lt">Privačių detektyvų bendrija</dc:title>
        <dc:title xml:lang="en">Society of Private Detectives</dc:title>
        <rdfs:label rdf:datatype="http://www.w3.org/2001/XMLSchema#string">PDB</rdfs:label>
    </owl:NamedIndividual>
    


    <!-- http://w3id.org/um/cbcm/eu-cm-ontology#lt201 -->

    <owl:NamedIndividual rdf:about="http://w3id.org/um/cbcm/eu-cm-ontology#lt201">
        <rdf:type rdf:resource="http://w3id.org/um/cbcm/eu-cm-ontology#CompanyLegalForm"/>
        <dc:title xml:lang="en">State Enterprise</dc:title>
        <dc:title xml:lang="lt">Valstybės įmonė</dc:title>
        <rdfs:label rdf:datatype="http://www.w3.org/2001/XMLSchema#string">VI</rdfs:label>
    </owl:NamedIndividual>
    


    <!-- http://w3id.org/um/cbcm/eu-cm-ontology#lt202 -->

    <owl:NamedIndividual rdf:about="http://w3id.org/um/cbcm/eu-cm-ontology#lt202">
        <rdf:type rdf:resource="http://w3id.org/um/cbcm/eu-cm-ontology#CompanyLegalForm"/>
        <dc:title xml:lang="en">Municipal Enterprise</dc:title>
        <dc:title xml:lang="lt">Savivaldybės įmonė</dc:title>
        <rdfs:label rdf:datatype="http://www.w3.org/2001/XMLSchema#string">SI</rdfs:label>
    </owl:NamedIndividual>
    


    <!-- http://w3id.org/um/cbcm/eu-cm-ontology#lt203 -->

    <owl:NamedIndividual rdf:about="http://w3id.org/um/cbcm/eu-cm-ontology#lt203">
        <rdf:type rdf:resource="http://w3id.org/um/cbcm/eu-cm-ontology#CompanyLegalForm"/>
        <dc:title xml:lang="en">Public Institution</dc:title>
        <dc:title xml:lang="lt">Viešoji įstaiga</dc:title>
        <rdfs:label rdf:datatype="http://www.w3.org/2001/XMLSchema#string">VS</rdfs:label>
    </owl:NamedIndividual>
    


    <!-- http://w3id.org/um/cbcm/eu-cm-ontology#lt204 -->

    <owl:NamedIndividual rdf:about="http://w3id.org/um/cbcm/eu-cm-ontology#lt204">
        <rdf:type rdf:resource="http://w3id.org/um/cbcm/eu-cm-ontology#CompanyLegalForm"/>
        <dc:title xml:lang="lt">Biudžetinė įstaiga</dc:title>
        <dc:title xml:lang="en">Budgetary Institution</dc:title>
        <rdfs:label rdf:datatype="http://www.w3.org/2001/XMLSchema#string">BI</rdfs:label>
    </owl:NamedIndividual>
    


    <!-- http://w3id.org/um/cbcm/eu-cm-ontology#lt205 -->

    <owl:NamedIndividual rdf:about="http://w3id.org/um/cbcm/eu-cm-ontology#lt205">
        <rdf:type rdf:resource="http://w3id.org/um/cbcm/eu-cm-ontology#CompanyLegalForm"/>
        <dc:title xml:lang="en">Charity and Sponsorship Fund</dc:title>
        <dc:title xml:lang="lt">Labdaros ir paramos fondas</dc:title>
        <rdfs:label rdf:datatype="http://www.w3.org/2001/XMLSchema#string">LF</rdfs:label>
    </owl:NamedIndividual>
    


    <!-- http://w3id.org/um/cbcm/eu-cm-ontology#lt206 -->

    <owl:NamedIndividual rdf:about="http://w3id.org/um/cbcm/eu-cm-ontology#lt206">
        <rdf:type rdf:resource="http://w3id.org/um/cbcm/eu-cm-ontology#CompanyLegalForm"/>
        <dc:title xml:lang="lt">Bendrija</dc:title>
        <dc:title xml:lang="en">Partnership</dc:title>
        <rdfs:label rdf:datatype="http://www.w3.org/2001/XMLSchema#string">BN</rdfs:label>
    </owl:NamedIndividual>
    


    <!-- http://w3id.org/um/cbcm/eu-cm-ontology#lt207 -->

    <owl:NamedIndividual rdf:about="http://w3id.org/um/cbcm/eu-cm-ontology#lt207">
        <rdf:type rdf:resource="http://w3id.org/um/cbcm/eu-cm-ontology#CompanyLegalForm"/>
        <dc:title xml:lang="en">Gardeners’ Partnership</dc:title>
        <dc:title xml:lang="lt">Sodininkų bendrija</dc:title>
        <rdfs:label rdf:datatype="http://www.w3.org/2001/XMLSchema#string">SD</rdfs:label>
    </owl:NamedIndividual>
    


    <!-- http://w3id.org/um/cbcm/eu-cm-ontology#lt208 -->

    <owl:NamedIndividual rdf:about="http://w3id.org/um/cbcm/eu-cm-ontology#lt208">
        <rdf:type rdf:resource="http://w3id.org/um/cbcm/eu-cm-ontology#CompanyLegalForm"/>
        <dc:title xml:lang="en">Political Party</dc:title>
        <dc:title xml:lang="lt">Politinė partija</dc:title>
        <rdfs:label rdf:datatype="http://www.w3.org/2001/XMLSchema#string">PP</rdfs:label>
    </owl:NamedIndividual>
    


    <!-- http://w3id.org/um/cbcm/eu-cm-ontology#lt209 -->

    <owl:NamedIndividual rdf:about="http://w3id.org/um/cbcm/eu-cm-ontology#lt209">
        <rdf:type rdf:resource="http://w3id.org/um/cbcm/eu-cm-ontology#CompanyLegalForm"/>
        <dc:title xml:lang="lt">Tradicinė religinė bendruomenė ar bendrija</dc:title>
        <dc:title xml:lang="en">Traditional Lithuanian Religious Congregation or Community</dc:title>
        <rdfs:label rdf:datatype="http://www.w3.org/2001/XMLSchema#string">TR</rdfs:label>
    </owl:NamedIndividual>
    


    <!-- http://w3id.org/um/cbcm/eu-cm-ontology#lt210 -->

    <owl:NamedIndividual rdf:about="http://w3id.org/um/cbcm/eu-cm-ontology#lt210">
        <rdf:type rdf:resource="http://w3id.org/um/cbcm/eu-cm-ontology#CompanyLegalForm"/>
        <dc:title xml:lang="lt">Religinė bendruomenė ar bendrija</dc:title>
        <dc:title xml:lang="en">Religious Community and Association</dc:title>
        <rdfs:label rdf:datatype="http://www.w3.org/2001/XMLSchema#string">RB</rdfs:label>
    </owl:NamedIndividual>
    


    <!-- http://w3id.org/um/cbcm/eu-cm-ontology#lt211 -->

    <owl:NamedIndividual rdf:about="http://w3id.org/um/cbcm/eu-cm-ontology#lt211">
        <rdf:type rdf:resource="http://w3id.org/um/cbcm/eu-cm-ontology#CompanyLegalForm"/>
        <dc:title xml:lang="lt">Profesinė sąjunga ar susivienijimas</dc:title>
        <dc:title xml:lang="en">Trade Union</dc:title>
        <rdfs:label rdf:datatype="http://www.w3.org/2001/XMLSchema#string">PS</rdfs:label>
    </owl:NamedIndividual>
    


    <!-- http://w3id.org/um/cbcm/eu-cm-ontology#lt213 -->

    <owl:NamedIndividual rdf:about="http://w3id.org/um/cbcm/eu-cm-ontology#lt213">
        <rdf:type rdf:resource="http://w3id.org/um/cbcm/eu-cm-ontology#CompanyLegalForm"/>
        <dc:title xml:lang="en">Foster Family</dc:title>
        <dc:title xml:lang="lt">Šeimyna</dc:title>
        <rdfs:label rdf:datatype="http://www.w3.org/2001/XMLSchema#string">S</rdfs:label>
    </owl:NamedIndividual>
    


    <!-- http://w3id.org/um/cbcm/eu-cm-ontology#lt214 -->

    <owl:NamedIndividual rdf:about="http://w3id.org/um/cbcm/eu-cm-ontology#lt214">
        <rdf:type rdf:resource="http://w3id.org/um/cbcm/eu-cm-ontology#CompanyLegalForm"/>
        <dc:title xml:lang="en"> industry and crafts</dc:title>
        <dc:title xml:lang="lt"> pramonės ir amatų rūmai</dc:title>
        <dc:title xml:lang="en">Chamber of commerce</dc:title>
        <dc:title xml:lang="lt">Prekybos</dc:title>
        <rdfs:label rdf:datatype="http://www.w3.org/2001/XMLSchema#string">PR</rdfs:label>
    </owl:NamedIndividual>
    


    <!-- http://w3id.org/um/cbcm/eu-cm-ontology#lt215 -->

    <owl:NamedIndividual rdf:about="http://w3id.org/um/cbcm/eu-cm-ontology#lt215">
        <rdf:type rdf:resource="http://w3id.org/um/cbcm/eu-cm-ontology#CompanyLegalForm"/>
        <dc:title xml:lang="en"> Industry and Crafts </dc:title>
        <dc:title xml:lang="lt"> pramonės ir amatų rūmų asociacija</dc:title>
        <dc:title xml:lang="lt">Lietuvos prekybos</dc:title>
        <dc:title xml:lang="en">The Association of Lithuanian Chambers of Commerce</dc:title>
        <rdfs:label rdf:datatype="http://www.w3.org/2001/XMLSchema#string">LPRA</rdfs:label>
    </owl:NamedIndividual>
    


    <!-- http://w3id.org/um/cbcm/eu-cm-ontology#lt216 -->

    <owl:NamedIndividual rdf:about="http://w3id.org/um/cbcm/eu-cm-ontology#lt216">
        <rdf:type rdf:resource="http://w3id.org/um/cbcm/eu-cm-ontology#CompanyLegalForm"/>
        <dc:title xml:lang="lt">Bendras valdymo ir pranešimų centras</dc:title>
        <dc:title xml:lang="en">Combined Control and Reporting Centre</dc:title>
        <rdfs:label rdf:datatype="http://www.w3.org/2001/XMLSchema#string">CRC</rdfs:label>
    </owl:NamedIndividual>
    


    <!-- http://w3id.org/um/cbcm/eu-cm-ontology#lt301 -->

    <owl:NamedIndividual rdf:about="http://w3id.org/um/cbcm/eu-cm-ontology#lt301">
        <rdf:type rdf:resource="http://w3id.org/um/cbcm/eu-cm-ontology#CompanyLegalForm"/>
        <dc:title xml:lang="en">Central Bank</dc:title>
        <dc:title xml:lang="lt">Centrinis bankas</dc:title>
        <rdfs:label rdf:datatype="http://www.w3.org/2001/XMLSchema#string">CB</rdfs:label>
    </owl:NamedIndividual>
    


    <!-- http://w3id.org/um/cbcm/eu-cm-ontology#lu01 -->

    <owl:NamedIndividual rdf:about="http://w3id.org/um/cbcm/eu-cm-ontology#lu01">
        <rdf:type rdf:resource="http://w3id.org/um/cbcm/eu-cm-ontology#CompanyLegalForm"/>
        <dc:title xml:lang="lu">Entreprise individuelle</dc:title>
        <dc:title xml:lang="en">Sole proprietorship</dc:title>
        <rdfs:label rdf:datatype="http://www.w3.org/2001/XMLSchema#string">EI</rdfs:label>
    </owl:NamedIndividual>
    


    <!-- http://w3id.org/um/cbcm/eu-cm-ontology#lu03 -->

    <owl:NamedIndividual rdf:about="http://w3id.org/um/cbcm/eu-cm-ontology#lu03">
        <rdf:type rdf:resource="http://w3id.org/um/cbcm/eu-cm-ontology#CompanyLegalForm"/>
        <dc:title xml:lang="en">Limited liability company</dc:title>
        <dc:title xml:lang="lu">Société à responsabilité limitée</dc:title>
        <rdfs:label rdf:datatype="http://www.w3.org/2001/XMLSchema#string">SARLxa0</rdfs:label>
    </owl:NamedIndividual>
    


    <!-- http://w3id.org/um/cbcm/eu-cm-ontology#lu04 -->

    <owl:NamedIndividual rdf:about="http://w3id.org/um/cbcm/eu-cm-ontology#lu04">
        <rdf:type rdf:resource="http://w3id.org/um/cbcm/eu-cm-ontology#CompanyLegalForm"/>
        <dc:title xml:lang="en">Simplified limited liability company</dc:title>
        <dc:title xml:lang="lu">Société à responsabilité limitée simplifiée</dc:title>
        <rdfs:label rdf:datatype="http://www.w3.org/2001/XMLSchema#string">SARLS</rdfs:label>
    </owl:NamedIndividual>
    


    <!-- http://w3id.org/um/cbcm/eu-cm-ontology#lu05 -->

    <owl:NamedIndividual rdf:about="http://w3id.org/um/cbcm/eu-cm-ontology#lu05">
        <rdf:type rdf:resource="http://w3id.org/um/cbcm/eu-cm-ontology#CompanyLegalForm"/>
        <dc:title xml:lang="en">Limited partnership</dc:title>
        <dc:title xml:lang="lu">Société en commandite simple </dc:title>
        <rdfs:label rdf:datatype="http://www.w3.org/2001/XMLSchema#string">SECS</rdfs:label>
    </owl:NamedIndividual>
    


    <!-- http://w3id.org/um/cbcm/eu-cm-ontology#lu06 -->

    <owl:NamedIndividual rdf:about="http://w3id.org/um/cbcm/eu-cm-ontology#lu06">
        <rdf:type rdf:resource="http://w3id.org/um/cbcm/eu-cm-ontology#CompanyLegalForm"/>
        <dc:title xml:lang="lu">Société en commandite speciale</dc:title>
        <dc:title xml:lang="en">Special limited partnership</dc:title>
        <rdfs:label rdf:datatype="http://www.w3.org/2001/XMLSchema#string">SECSP</rdfs:label>
    </owl:NamedIndividual>
    


    <!-- http://w3id.org/um/cbcm/eu-cm-ontology#lu07 -->

    <owl:NamedIndividual rdf:about="http://w3id.org/um/cbcm/eu-cm-ontology#lu07">
        <rdf:type rdf:resource="http://w3id.org/um/cbcm/eu-cm-ontology#CompanyLegalForm"/>
        <dc:title xml:lang="en">Public limited company</dc:title>
        <dc:title xml:lang="lu">Société anonyme</dc:title>
        <rdfs:label rdf:datatype="http://www.w3.org/2001/XMLSchema#string">SAxa0</rdfs:label>
    </owl:NamedIndividual>
    


    <!-- http://w3id.org/um/cbcm/eu-cm-ontology#lu08 -->

    <owl:NamedIndividual rdf:about="http://w3id.org/um/cbcm/eu-cm-ontology#lu08">
        <rdf:type rdf:resource="http://w3id.org/um/cbcm/eu-cm-ontology#CompanyLegalForm"/>
        <dc:title xml:lang="en">Partnership limited by shares</dc:title>
        <dc:title xml:lang="lu">Société en commandite par actions</dc:title>
        <rdfs:label rdf:datatype="http://www.w3.org/2001/XMLSchema#string">SECA</rdfs:label>
    </owl:NamedIndividual>
    


    <!-- http://w3id.org/um/cbcm/eu-cm-ontology#lu09 -->

    <owl:NamedIndividual rdf:about="http://w3id.org/um/cbcm/eu-cm-ontology#lu09">
        <rdf:type rdf:resource="http://w3id.org/um/cbcm/eu-cm-ontology#CompanyLegalForm"/>
        <dc:title xml:lang="en">Open-ended investment company</dc:title>
        <dc:title xml:lang="lu">Société dinvestissement à capital variable</dc:title>
        <rdfs:label rdf:datatype="http://www.w3.org/2001/XMLSchema#string">SICAV</rdfs:label>
    </owl:NamedIndividual>
    


    <!-- http://w3id.org/um/cbcm/eu-cm-ontology#lu10 -->

    <owl:NamedIndividual rdf:about="http://w3id.org/um/cbcm/eu-cm-ontology#lu10">
        <rdf:type rdf:resource="http://w3id.org/um/cbcm/eu-cm-ontology#CompanyLegalForm"/>
        <dc:title xml:lang="en">Closed-ended investment company</dc:title>
        <dc:title xml:lang="lu">Société dinvestissement à capital fixe</dc:title>
        <rdfs:label rdf:datatype="http://www.w3.org/2001/XMLSchema#string">SICAF</rdfs:label>
    </owl:NamedIndividual>
    


    <!-- http://w3id.org/um/cbcm/eu-cm-ontology#lu11 -->

    <owl:NamedIndividual rdf:about="http://w3id.org/um/cbcm/eu-cm-ontology#lu11">
        <rdf:type rdf:resource="http://w3id.org/um/cbcm/eu-cm-ontology#CompanyLegalForm"/>
        <dc:title xml:lang="lu">Société d’épargne-pension à capital variable </dc:title>
        <dc:title xml:lang="en">Variable Capital Pension Savings Company </dc:title>
        <rdfs:label rdf:datatype="http://www.w3.org/2001/XMLSchema#string">SEPCAV</rdfs:label>
    </owl:NamedIndividual>
    


    <!-- http://w3id.org/um/cbcm/eu-cm-ontology#lu12 -->

    <owl:NamedIndividual rdf:about="http://w3id.org/um/cbcm/eu-cm-ontology#lu12">
        <rdf:type rdf:resource="http://w3id.org/um/cbcm/eu-cm-ontology#CompanyLegalForm"/>
        <dc:title xml:lang="en">Cooperative company</dc:title>
        <dc:title xml:lang="lu">Société coopérative </dc:title>
        <rdfs:label rdf:datatype="http://www.w3.org/2001/XMLSchema#string">SCOP</rdfs:label>
    </owl:NamedIndividual>
    


    <!-- http://w3id.org/um/cbcm/eu-cm-ontology#lu13 -->

    <owl:NamedIndividual rdf:about="http://w3id.org/um/cbcm/eu-cm-ontology#lu13">
        <rdf:type rdf:resource="http://w3id.org/um/cbcm/eu-cm-ontology#CompanyLegalForm"/>
        <dc:title xml:lang="en">Civil company </dc:title>
        <dc:title xml:lang="lu">Société civile</dc:title>
        <rdfs:label rdf:datatype="http://www.w3.org/2001/XMLSchema#string">SC</rdfs:label>
    </owl:NamedIndividual>
    


    <!-- http://w3id.org/um/cbcm/eu-cm-ontology#lu15 -->

    <owl:NamedIndividual rdf:about="http://w3id.org/um/cbcm/eu-cm-ontology#lu15">
        <rdf:type rdf:resource="http://w3id.org/um/cbcm/eu-cm-ontology#CompanyLegalForm"/>
        <dc:title xml:lang="en">Economic interest group</dc:title>
        <dc:title xml:lang="lu">Groupement dintérêt économique</dc:title>
        <rdfs:label rdf:datatype="http://www.w3.org/2001/XMLSchema#string">GIE</rdfs:label>
    </owl:NamedIndividual>
    


    <!-- http://w3id.org/um/cbcm/eu-cm-ontology#lu16 -->

    <owl:NamedIndividual rdf:about="http://w3id.org/um/cbcm/eu-cm-ontology#lu16">
        <rdf:type rdf:resource="http://w3id.org/um/cbcm/eu-cm-ontology#CompanyLegalForm"/>
        <dc:title xml:lang="lu">Association sans but lucratif</dc:title>
        <dc:title xml:lang="en">Non-profit association </dc:title>
        <rdfs:label rdf:datatype="http://www.w3.org/2001/XMLSchema#string">ASBL</rdfs:label>
    </owl:NamedIndividual>
    


    <!-- http://w3id.org/um/cbcm/eu-cm-ontology#lu17 -->

    <owl:NamedIndividual rdf:about="http://w3id.org/um/cbcm/eu-cm-ontology#lu17">
        <rdf:type rdf:resource="http://w3id.org/um/cbcm/eu-cm-ontology#CompanyLegalForm"/>
        <dc:title xml:lang="lu">Fondation</dc:title>
        <dc:title xml:lang="en">Foundation</dc:title>
        <rdfs:label rdf:datatype="http://www.w3.org/2001/XMLSchema#string">FON</rdfs:label>
    </owl:NamedIndividual>
    


    <!-- http://w3id.org/um/cbcm/eu-cm-ontology#lu18 -->

    <owl:NamedIndividual rdf:about="http://w3id.org/um/cbcm/eu-cm-ontology#lu18">
        <rdf:type rdf:resource="http://w3id.org/um/cbcm/eu-cm-ontology#CompanyLegalForm"/>
        <dc:title xml:lang="lu">Association dépargne pension</dc:title>
        <dc:title xml:lang="en">Pensions Savings Association </dc:title>
        <rdfs:label rdf:datatype="http://www.w3.org/2001/XMLSchema#string">ASSEP</rdfs:label>
    </owl:NamedIndividual>
    


    <!-- http://w3id.org/um/cbcm/eu-cm-ontology#lu19 -->

    <owl:NamedIndividual rdf:about="http://w3id.org/um/cbcm/eu-cm-ontology#lu19">
        <rdf:type rdf:resource="http://w3id.org/um/cbcm/eu-cm-ontology#CompanyLegalForm"/>
        <dc:title xml:lang="lu">Association dassurances mutuelles</dc:title>
        <dc:title xml:lang="en">Mutual Insurance Association </dc:title>
        <rdfs:label rdf:datatype="http://www.w3.org/2001/XMLSchema#string">AAM</rdfs:label>
    </owl:NamedIndividual>
    


    <!-- http://w3id.org/um/cbcm/eu-cm-ontology#lu20 -->

    <owl:NamedIndividual rdf:about="http://w3id.org/um/cbcm/eu-cm-ontology#lu20">
        <rdf:type rdf:resource="http://w3id.org/um/cbcm/eu-cm-ontology#CompanyLegalForm"/>
        <dc:title xml:lang="en">Agricultural association </dc:title>
        <dc:title xml:lang="lu">Association agricole</dc:title>
        <rdfs:label rdf:datatype="http://www.w3.org/2001/XMLSchema#string">AA</rdfs:label>
    </owl:NamedIndividual>
    


    <!-- http://w3id.org/um/cbcm/eu-cm-ontology#lu21 -->

    <owl:NamedIndividual rdf:about="http://w3id.org/um/cbcm/eu-cm-ontology#lu21">
        <rdf:type rdf:resource="http://w3id.org/um/cbcm/eu-cm-ontology#CompanyLegalForm"/>
        <dc:title xml:lang="lu">Etablissement public</dc:title>
        <dc:title xml:lang="en">Public establishment</dc:title>
        <rdfs:label rdf:datatype="http://www.w3.org/2001/XMLSchema#string">EP</rdfs:label>
    </owl:NamedIndividual>
    


    <!-- http://w3id.org/um/cbcm/eu-cm-ontology#lu22 -->

    <owl:NamedIndividual rdf:about="http://w3id.org/um/cbcm/eu-cm-ontology#lu22">
        <rdf:type rdf:resource="http://w3id.org/um/cbcm/eu-cm-ontology#CompanyLegalForm"/>
        <dc:title xml:lang="en">Partnership</dc:title>
        <dc:title xml:lang="lu">Société en nom collectif</dc:title>
        <rdfs:label rdf:datatype="http://www.w3.org/2001/XMLSchema#string">SNC</rdfs:label>
    </owl:NamedIndividual>
    


    <!-- http://w3id.org/um/cbcm/eu-cm-ontology#lu26 -->

    <owl:NamedIndividual rdf:about="http://w3id.org/um/cbcm/eu-cm-ontology#lu26">
        <rdf:type rdf:resource="http://w3id.org/um/cbcm/eu-cm-ontology#CompanyLegalForm"/>
        <dc:title xml:lang="lu">Fonds commun de placement</dc:title>
        <dc:title xml:lang="en">Mutual Funds</dc:title>
        <rdfs:label rdf:datatype="http://www.w3.org/2001/XMLSchema#string">FCP</rdfs:label>
    </owl:NamedIndividual>
    


    <!-- http://w3id.org/um/cbcm/eu-cm-ontology#lu27 -->

    <owl:NamedIndividual rdf:about="http://w3id.org/um/cbcm/eu-cm-ontology#lu27">
        <rdf:type rdf:resource="http://w3id.org/um/cbcm/eu-cm-ontology#CompanyLegalForm"/>
        <dc:title xml:lang="en">Alternative investment funds reserved</dc:title>
        <dc:title xml:lang="lu">Fonds dinvestissement alternatif reservé </dc:title>
        <rdfs:label rdf:datatype="http://www.w3.org/2001/XMLSchema#string">FIAR</rdfs:label>
    </owl:NamedIndividual>
    


    <!-- http://w3id.org/um/cbcm/eu-cm-ontology#lu32 -->

    <owl:NamedIndividual rdf:about="http://w3id.org/um/cbcm/eu-cm-ontology#lu32">
        <rdf:type rdf:resource="http://w3id.org/um/cbcm/eu-cm-ontology#CompanyLegalForm"/>
        <dc:title xml:lang="lu">Autres Formes juridiques</dc:title>
        <dc:title xml:lang="en">Other legal form</dc:title>
        <rdfs:label rdf:datatype="http://www.w3.org/2001/XMLSchema#string">AUT</rdfs:label>
    </owl:NamedIndividual>
    


    <!-- http://w3id.org/um/cbcm/eu-cm-ontology#lu33 -->

    <owl:NamedIndividual rdf:about="http://w3id.org/um/cbcm/eu-cm-ontology#lu33">
        <rdf:type rdf:resource="http://w3id.org/um/cbcm/eu-cm-ontology#CompanyLegalForm"/>
        <dc:title xml:lang="en">Public sector</dc:title>
        <dc:title xml:lang="lu">Secteur public</dc:title>
        <rdfs:label rdf:datatype="http://www.w3.org/2001/XMLSchema#string">SP</rdfs:label>
    </owl:NamedIndividual>
    


    <!-- http://w3id.org/um/cbcm/eu-cm-ontology#lu34 -->

    <owl:NamedIndividual rdf:about="http://w3id.org/um/cbcm/eu-cm-ontology#lu34">
        <rdf:type rdf:resource="http://w3id.org/um/cbcm/eu-cm-ontology#CompanyLegalForm"/>
        <dc:title xml:lang="en">Risk capital investment company </dc:title>
        <dc:title xml:lang="lu">Société dinvestissement à capital risque </dc:title>
        <rdfs:label rdf:datatype="http://www.w3.org/2001/XMLSchema#string">SICAR</rdfs:label>
    </owl:NamedIndividual>
    


    <!-- http://w3id.org/um/cbcm/eu-cm-ontology#luxembourg -->

    <owl:NamedIndividual rdf:about="http://w3id.org/um/cbcm/eu-cm-ontology#luxembourg">
        <rdf:type rdf:resource="http://w3id.org/um/cbcm/eu-cm-ontology#EUCountry"/>
        <cbcm:countryHasCompanyForm rdf:resource="http://w3id.org/um/cbcm/eu-cm-ontology#lu01"/>
        <cbcm:countryHasCompanyForm rdf:resource="http://w3id.org/um/cbcm/eu-cm-ontology#lu03"/>
        <cbcm:countryHasCompanyForm rdf:resource="http://w3id.org/um/cbcm/eu-cm-ontology#lu04"/>
        <cbcm:countryHasCompanyForm rdf:resource="http://w3id.org/um/cbcm/eu-cm-ontology#lu05"/>
        <cbcm:countryHasCompanyForm rdf:resource="http://w3id.org/um/cbcm/eu-cm-ontology#lu06"/>
        <cbcm:countryHasCompanyForm rdf:resource="http://w3id.org/um/cbcm/eu-cm-ontology#lu07"/>
        <cbcm:countryHasCompanyForm rdf:resource="http://w3id.org/um/cbcm/eu-cm-ontology#lu08"/>
        <cbcm:countryHasCompanyForm rdf:resource="http://w3id.org/um/cbcm/eu-cm-ontology#lu09"/>
        <cbcm:countryHasCompanyForm rdf:resource="http://w3id.org/um/cbcm/eu-cm-ontology#lu10"/>
        <cbcm:countryHasCompanyForm rdf:resource="http://w3id.org/um/cbcm/eu-cm-ontology#lu11"/>
        <cbcm:countryHasCompanyForm rdf:resource="http://w3id.org/um/cbcm/eu-cm-ontology#lu12"/>
        <cbcm:countryHasCompanyForm rdf:resource="http://w3id.org/um/cbcm/eu-cm-ontology#lu13"/>
        <cbcm:countryHasCompanyForm rdf:resource="http://w3id.org/um/cbcm/eu-cm-ontology#lu15"/>
        <cbcm:countryHasCompanyForm rdf:resource="http://w3id.org/um/cbcm/eu-cm-ontology#lu16"/>
        <cbcm:countryHasCompanyForm rdf:resource="http://w3id.org/um/cbcm/eu-cm-ontology#lu17"/>
        <cbcm:countryHasCompanyForm rdf:resource="http://w3id.org/um/cbcm/eu-cm-ontology#lu18"/>
        <cbcm:countryHasCompanyForm rdf:resource="http://w3id.org/um/cbcm/eu-cm-ontology#lu19"/>
        <cbcm:countryHasCompanyForm rdf:resource="http://w3id.org/um/cbcm/eu-cm-ontology#lu20"/>
        <cbcm:countryHasCompanyForm rdf:resource="http://w3id.org/um/cbcm/eu-cm-ontology#lu21"/>
        <cbcm:countryHasCompanyForm rdf:resource="http://w3id.org/um/cbcm/eu-cm-ontology#lu22"/>
        <cbcm:countryHasCompanyForm rdf:resource="http://w3id.org/um/cbcm/eu-cm-ontology#lu26"/>
        <cbcm:countryHasCompanyForm rdf:resource="http://w3id.org/um/cbcm/eu-cm-ontology#lu27"/>
        <cbcm:countryHasCompanyForm rdf:resource="http://w3id.org/um/cbcm/eu-cm-ontology#lu32"/>
        <cbcm:countryHasCompanyForm rdf:resource="http://w3id.org/um/cbcm/eu-cm-ontology#lu33"/>
        <cbcm:countryHasCompanyForm rdf:resource="http://w3id.org/um/cbcm/eu-cm-ontology#lu34"/>
        <cbcm:iso2code>LU</cbcm:iso2code>
        <rdfs:label xml:lang="en">Grand Duchy of Luxembourg</rdfs:label>
        <rdfs:label xml:lang="fr">Grand-Duché de Luxembourg</rdfs:label>
        <rdfs:label xml:lang="lb">Groussherzogtum Lëtzebuerg</rdfs:label>
        <rdfs:label xml:lang="de">Großherzogtum Luxemburg​</rdfs:label>
        <rdfs:label xml:lang="en">Luxembourg</rdfs:label>
        <rdfs:label xml:lang="lb">Lëtzebuerg</rdfs:label>
    </owl:NamedIndividual>
    


    <!-- http://w3id.org/um/cbcm/eu-cm-ontology#lv101 -->

    <owl:NamedIndividual rdf:about="http://w3id.org/um/cbcm/eu-cm-ontology#lv101">
        <rdf:type rdf:resource="http://w3id.org/um/cbcm/eu-cm-ontology#CompanyLegalForm"/>
        <dc:title xml:lang="lv">Akciju sabiedrība</dc:title>
        <dc:title xml:lang="en">Joint stock company</dc:title>
        <rdfs:label rdf:datatype="http://www.w3.org/2001/XMLSchema#string">AS</rdfs:label>
    </owl:NamedIndividual>
    


    <!-- http://w3id.org/um/cbcm/eu-cm-ontology#lv103 -->

    <owl:NamedIndividual rdf:about="http://w3id.org/um/cbcm/eu-cm-ontology#lv103">
        <rdf:type rdf:resource="http://w3id.org/um/cbcm/eu-cm-ontology#CompanyLegalForm"/>
        <dc:title xml:lang="en">Limited liability company</dc:title>
        <dc:title xml:lang="lv">Sabiedrība ar ierobežotu atbildību</dc:title>
        <rdfs:label rdf:datatype="http://www.w3.org/2001/XMLSchema#string">SIA</rdfs:label>
    </owl:NamedIndividual>
    


    <!-- http://w3id.org/um/cbcm/eu-cm-ontology#lv104 -->

    <owl:NamedIndividual rdf:about="http://w3id.org/um/cbcm/eu-cm-ontology#lv104">
        <rdf:type rdf:resource="http://w3id.org/um/cbcm/eu-cm-ontology#CompanyLegalForm"/>
        <dc:title xml:lang="en">State enterprise</dc:title>
        <dc:title xml:lang="lv">Valsts uzņēmums </dc:title>
        <rdfs:label rdf:datatype="http://www.w3.org/2001/XMLSchema#string">VU</rdfs:label>
    </owl:NamedIndividual>
    


    <!-- http://w3id.org/um/cbcm/eu-cm-ontology#lv105 -->

    <owl:NamedIndividual rdf:about="http://w3id.org/um/cbcm/eu-cm-ontology#lv105">
        <rdf:type rdf:resource="http://w3id.org/um/cbcm/eu-cm-ontology#CompanyLegalForm"/>
        <dc:title xml:lang="en">Municipal enterprise</dc:title>
        <dc:title xml:lang="lv">Pašvaldības uzņēmums </dc:title>
        <rdfs:label rdf:datatype="http://www.w3.org/2001/XMLSchema#string">PSV</rdfs:label>
    </owl:NamedIndividual>
    


    <!-- http://w3id.org/um/cbcm/eu-cm-ontology#lv106 -->

    <owl:NamedIndividual rdf:about="http://w3id.org/um/cbcm/eu-cm-ontology#lv106">
        <rdf:type rdf:resource="http://w3id.org/um/cbcm/eu-cm-ontology#CompanyLegalForm"/>
        <dc:title xml:lang="en">Enterprise of the company</dc:title>
        <dc:title xml:lang="lv">Uzņēmējsabiedrības uzņēmums </dc:title>
        <rdfs:label rdf:datatype="http://www.w3.org/2001/XMLSchema#string">UZN</rdfs:label>
    </owl:NamedIndividual>
    


    <!-- http://w3id.org/um/cbcm/eu-cm-ontology#lv107 -->

    <owl:NamedIndividual rdf:about="http://w3id.org/um/cbcm/eu-cm-ontology#lv107">
        <rdf:type rdf:resource="http://w3id.org/um/cbcm/eu-cm-ontology#CompanyLegalForm"/>
        <dc:title xml:lang="en">General partnership</dc:title>
        <dc:title xml:lang="lv">Pilnsabiedrība</dc:title>
        <rdfs:label rdf:datatype="http://www.w3.org/2001/XMLSchema#string">PS</rdfs:label>
    </owl:NamedIndividual>
    


    <!-- http://w3id.org/um/cbcm/eu-cm-ontology#lv108 -->

    <owl:NamedIndividual rdf:about="http://w3id.org/um/cbcm/eu-cm-ontology#lv108">
        <rdf:type rdf:resource="http://w3id.org/um/cbcm/eu-cm-ontology#CompanyLegalForm"/>
        <dc:title xml:lang="lv">Komandītsabiedrība</dc:title>
        <dc:title xml:lang="en">Limited partnership</dc:title>
        <rdfs:label rdf:datatype="http://www.w3.org/2001/XMLSchema#string">KS</rdfs:label>
    </owl:NamedIndividual>
    


    <!-- http://w3id.org/um/cbcm/eu-cm-ontology#lv109 -->

    <owl:NamedIndividual rdf:about="http://w3id.org/um/cbcm/eu-cm-ontology#lv109">
        <rdf:type rdf:resource="http://w3id.org/um/cbcm/eu-cm-ontology#CompanyLegalForm"/>
        <dc:title xml:lang="lv">Līgumsabiedrība ar pilnu atbildību </dc:title>
        <dc:title xml:lang="en">Partnership with full responsibility</dc:title>
        <rdfs:label rdf:datatype="http://www.w3.org/2001/XMLSchema#string">LIG</rdfs:label>
    </owl:NamedIndividual>
    


    <!-- http://w3id.org/um/cbcm/eu-cm-ontology#lv110 -->

    <owl:NamedIndividual rdf:about="http://w3id.org/um/cbcm/eu-cm-ontology#lv110">
        <rdf:type rdf:resource="http://w3id.org/um/cbcm/eu-cm-ontology#CompanyLegalForm"/>
        <dc:title xml:lang="en">Cooperative Share Company</dc:title>
        <dc:title xml:lang="lv">Paju sabiedrība </dc:title>
        <rdfs:label rdf:datatype="http://www.w3.org/2001/XMLSchema#string">PAJ</rdfs:label>
    </owl:NamedIndividual>
    


    <!-- http://w3id.org/um/cbcm/eu-cm-ontology#lv111 -->

    <owl:NamedIndividual rdf:about="http://w3id.org/um/cbcm/eu-cm-ontology#lv111">
        <rdf:type rdf:resource="http://w3id.org/um/cbcm/eu-cm-ontology#CompanyLegalForm"/>
        <dc:title xml:lang="en">Additional liability company</dc:title>
        <dc:title xml:lang="lv">Sabiedrība ar papildu atbildību</dc:title>
        <rdfs:label rdf:datatype="http://www.w3.org/2001/XMLSchema#string">PAP</rdfs:label>
    </owl:NamedIndividual>
    


    <!-- http://w3id.org/um/cbcm/eu-cm-ontology#lv301 -->

    <owl:NamedIndividual rdf:about="http://w3id.org/um/cbcm/eu-cm-ontology#lv301">
        <rdf:type rdf:resource="http://w3id.org/um/cbcm/eu-cm-ontology#CompanyLegalForm"/>
        <dc:title xml:lang="en">Sole proprietorship (family enterprise)  </dc:title>
        <dc:title xml:lang="lv">Ģimenes uzņēmums </dc:title>
        <rdfs:label rdf:datatype="http://www.w3.org/2001/XMLSchema#string">GIM</rdfs:label>
    </owl:NamedIndividual>
    


    <!-- http://w3id.org/um/cbcm/eu-cm-ontology#lv302 -->

    <owl:NamedIndividual rdf:about="http://w3id.org/um/cbcm/eu-cm-ontology#lv302">
        <rdf:type rdf:resource="http://w3id.org/um/cbcm/eu-cm-ontology#CompanyLegalForm"/>
        <dc:title xml:lang="en">Individual merchant</dc:title>
        <dc:title xml:lang="lv">Individuālais komersants</dc:title>
        <rdfs:label rdf:datatype="http://www.w3.org/2001/XMLSchema#string">IK</rdfs:label>
    </owl:NamedIndividual>
    


    <!-- http://w3id.org/um/cbcm/eu-cm-ontology#lv303 -->

    <owl:NamedIndividual rdf:about="http://w3id.org/um/cbcm/eu-cm-ontology#lv303">
        <rdf:type rdf:resource="http://w3id.org/um/cbcm/eu-cm-ontology#CompanyLegalForm"/>
        <dc:title xml:lang="en">Individual undertaking</dc:title>
        <dc:title xml:lang="lv">Individuālais uzņēmums </dc:title>
        <rdfs:label rdf:datatype="http://www.w3.org/2001/XMLSchema#string">IND</rdfs:label>
    </owl:NamedIndividual>
    


    <!-- http://w3id.org/um/cbcm/eu-cm-ontology#lv401 -->

    <owl:NamedIndividual rdf:about="http://w3id.org/um/cbcm/eu-cm-ontology#lv401">
        <rdf:type rdf:resource="http://w3id.org/um/cbcm/eu-cm-ontology#CompanyLegalForm"/>
        <dc:title xml:lang="en">Cooperative society</dc:title>
        <dc:title xml:lang="lv">Kooperatīvā sabiedrība </dc:title>
        <rdfs:label rdf:datatype="http://www.w3.org/2001/XMLSchema#string">KB</rdfs:label>
    </owl:NamedIndividual>
    


    <!-- http://w3id.org/um/cbcm/eu-cm-ontology#lv402 -->

    <owl:NamedIndividual rdf:about="http://w3id.org/um/cbcm/eu-cm-ontology#lv402">
        <rdf:type rdf:resource="http://w3id.org/um/cbcm/eu-cm-ontology#CompanyLegalForm"/>
        <dc:title xml:lang="lv">Kooperatīvo biedrību savienība </dc:title>
        <dc:title xml:lang="en">Union of cooperative societies</dc:title>
        <rdfs:label rdf:datatype="http://www.w3.org/2001/XMLSchema#string">KBS</rdfs:label>
    </owl:NamedIndividual>
    


    <!-- http://w3id.org/um/cbcm/eu-cm-ontology#lv403 -->

    <owl:NamedIndividual rdf:about="http://w3id.org/um/cbcm/eu-cm-ontology#lv403">
        <rdf:type rdf:resource="http://w3id.org/um/cbcm/eu-cm-ontology#CompanyLegalForm"/>
        <dc:title xml:lang="en">Enterprise of cooperative societies</dc:title>
        <dc:title xml:lang="lv">Kooperatīvo biedrību uzņēmums </dc:title>
        <rdfs:label rdf:datatype="http://www.w3.org/2001/XMLSchema#string">KBU</rdfs:label>
    </owl:NamedIndividual>
    


    <!-- http://w3id.org/um/cbcm/eu-cm-ontology#lv404 -->

    <owl:NamedIndividual rdf:about="http://w3id.org/um/cbcm/eu-cm-ontology#lv404">
        <rdf:type rdf:resource="http://w3id.org/um/cbcm/eu-cm-ontology#CompanyLegalForm"/>
        <dc:title xml:lang="en">Enterprise of union of cooperative societies</dc:title>
        <dc:title xml:lang="lv">Kooperatīvo biedrību savienības uzņēmums </dc:title>
        <rdfs:label rdf:datatype="http://www.w3.org/2001/XMLSchema#string">KSS</rdfs:label>
    </owl:NamedIndividual>
    


    <!-- http://w3id.org/um/cbcm/eu-cm-ontology#lv405 -->

    <owl:NamedIndividual rdf:about="http://w3id.org/um/cbcm/eu-cm-ontology#lv405">
        <rdf:type rdf:resource="http://w3id.org/um/cbcm/eu-cm-ontology#CompanyLegalForm"/>
        <dc:title xml:lang="en">Farm (farming enterprise)</dc:title>
        <dc:title xml:lang="lv">Zemnieku saimniecība </dc:title>
        <rdfs:label rdf:datatype="http://www.w3.org/2001/XMLSchema#string">ZEM</rdfs:label>
    </owl:NamedIndividual>
    


    <!-- http://w3id.org/um/cbcm/eu-cm-ontology#lv406 -->

    <owl:NamedIndividual rdf:about="http://w3id.org/um/cbcm/eu-cm-ontology#lv406">
        <rdf:type rdf:resource="http://w3id.org/um/cbcm/eu-cm-ontology#CompanyLegalForm"/>
        <dc:title xml:lang="en">Farm (fishing enterprise)</dc:title>
        <dc:title xml:lang="lv">Zvejnieku saimniecība </dc:title>
        <rdfs:label rdf:datatype="http://www.w3.org/2001/XMLSchema#string">ZVJ</rdfs:label>
    </owl:NamedIndividual>
    


    <!-- http://w3id.org/um/cbcm/eu-cm-ontology#lv701 -->

    <owl:NamedIndividual rdf:about="http://w3id.org/um/cbcm/eu-cm-ontology#lv701">
        <rdf:type rdf:resource="http://w3id.org/um/cbcm/eu-cm-ontology#CompanyLegalForm"/>
        <dc:title xml:lang="en">Public persons and authorities </dc:title>
        <dc:title xml:lang="lv">Publiskās personas un iestādes </dc:title>
        <rdfs:label rdf:datatype="http://www.w3.org/2001/XMLSchema#string">PPI</rdfs:label>
    </owl:NamedIndividual>
    


    <!-- http://w3id.org/um/cbcm/eu-cm-ontology#lv801 -->

    <owl:NamedIndividual rdf:about="http://w3id.org/um/cbcm/eu-cm-ontology#lv801">
        <rdf:type rdf:resource="http://w3id.org/um/cbcm/eu-cm-ontology#CompanyLegalForm"/>
        <dc:title xml:lang="en">Enterprise of religious organisation</dc:title>
        <dc:title xml:lang="lv">Reliģiskas organizācijas uzņēmums </dc:title>
        <rdfs:label rdf:datatype="http://www.w3.org/2001/XMLSchema#string">REL</rdfs:label>
    </owl:NamedIndividual>
    


    <!-- http://w3id.org/um/cbcm/eu-cm-ontology#lv802 -->

    <owl:NamedIndividual rdf:about="http://w3id.org/um/cbcm/eu-cm-ontology#lv802">
        <rdf:type rdf:resource="http://w3id.org/um/cbcm/eu-cm-ontology#CompanyLegalForm"/>
        <dc:title xml:lang="en">Enterprise of NGO</dc:title>
        <dc:title xml:lang="lv">Sabiedriskās organizācijas uzņēmums </dc:title>
        <rdfs:label rdf:datatype="http://www.w3.org/2001/XMLSchema#string">SOU</rdfs:label>
    </owl:NamedIndividual>
    


    <!-- http://w3id.org/um/cbcm/eu-cm-ontology#lv803 -->

    <owl:NamedIndividual rdf:about="http://w3id.org/um/cbcm/eu-cm-ontology#lv803">
        <rdf:type rdf:resource="http://w3id.org/um/cbcm/eu-cm-ontology#CompanyLegalForm"/>
        <dc:title xml:lang="lv">Arodbiedrību apvienība</dc:title>
        <dc:title xml:lang="en">Trade union association / labour organisation association</dc:title>
        <rdfs:label rdf:datatype="http://www.w3.org/2001/XMLSchema#string">ARA</rdfs:label>
    </owl:NamedIndividual>
    


    <!-- http://w3id.org/um/cbcm/eu-cm-ontology#lv804 -->

    <owl:NamedIndividual rdf:about="http://w3id.org/um/cbcm/eu-cm-ontology#lv804">
        <rdf:type rdf:resource="http://w3id.org/um/cbcm/eu-cm-ontology#CompanyLegalForm"/>
        <dc:title xml:lang="lv">Arodbiedrība</dc:title>
        <dc:title xml:lang="en">Trade union / labour organisation</dc:title>
        <rdfs:label rdf:datatype="http://www.w3.org/2001/XMLSchema#string">ARB</rdfs:label>
    </owl:NamedIndividual>
    


    <!-- http://w3id.org/um/cbcm/eu-cm-ontology#lv805 -->

    <owl:NamedIndividual rdf:about="http://w3id.org/um/cbcm/eu-cm-ontology#lv805">
        <rdf:type rdf:resource="http://w3id.org/um/cbcm/eu-cm-ontology#CompanyLegalForm"/>
        <dc:title xml:lang="lv">Arodbiedrības patstāvīgā vienība</dc:title>
        <dc:title xml:lang="en">Trade union independent unit / labour organisation independent unit</dc:title>
        <rdfs:label rdf:datatype="http://www.w3.org/2001/XMLSchema#string">ARV</rdfs:label>
    </owl:NamedIndividual>
    


    <!-- http://w3id.org/um/cbcm/eu-cm-ontology#lv806 -->

    <owl:NamedIndividual rdf:about="http://w3id.org/um/cbcm/eu-cm-ontology#lv806">
        <rdf:type rdf:resource="http://w3id.org/um/cbcm/eu-cm-ontology#CompanyLegalForm"/>
        <dc:title xml:lang="en">Religious Organisations and institutions of Religious Organisations</dc:title>
        <dc:title xml:lang="lv">Reliģiskās organizācijas un reliģisko organizāciju iestādes</dc:title>
        <rdfs:label rdf:datatype="http://www.w3.org/2001/XMLSchema#string">ROROIG</rdfs:label>
    </owl:NamedIndividual>
    


    <!-- http://w3id.org/um/cbcm/eu-cm-ontology#lv807 -->

    <owl:NamedIndividual rdf:about="http://w3id.org/um/cbcm/eu-cm-ontology#lv807">
        <rdf:type rdf:resource="http://w3id.org/um/cbcm/eu-cm-ontology#CompanyLegalForm"/>
        <dc:title xml:lang="en">Association</dc:title>
        <dc:title xml:lang="lv">Biedrība</dc:title>
        <rdfs:label rdf:datatype="http://www.w3.org/2001/XMLSchema#string">BDR</rdfs:label>
    </owl:NamedIndividual>
    


    <!-- http://w3id.org/um/cbcm/eu-cm-ontology#lv808 -->

    <owl:NamedIndividual rdf:about="http://w3id.org/um/cbcm/eu-cm-ontology#lv808">
        <rdf:type rdf:resource="http://w3id.org/um/cbcm/eu-cm-ontology#CompanyLegalForm"/>
        <dc:title xml:lang="en">Fondation</dc:title>
        <dc:title xml:lang="lv">Nodibinājums</dc:title>
        <rdfs:label rdf:datatype="http://www.w3.org/2001/XMLSchema#string">NOD</rdfs:label>
    </owl:NamedIndividual>
    


    <!-- http://w3id.org/um/cbcm/eu-cm-ontology#lv809 -->

    <owl:NamedIndividual rdf:about="http://w3id.org/um/cbcm/eu-cm-ontology#lv809">
        <rdf:type rdf:resource="http://w3id.org/um/cbcm/eu-cm-ontology#CompanyLegalForm"/>
        <dc:title xml:lang="en">Political party </dc:title>
        <dc:title xml:lang="lv">Politiskā partija</dc:title>
        <rdfs:label rdf:datatype="http://www.w3.org/2001/XMLSchema#string">PP</rdfs:label>
    </owl:NamedIndividual>
    


    <!-- http://w3id.org/um/cbcm/eu-cm-ontology#lv810 -->

    <owl:NamedIndividual rdf:about="http://w3id.org/um/cbcm/eu-cm-ontology#lv810">
        <rdf:type rdf:resource="http://w3id.org/um/cbcm/eu-cm-ontology#CompanyLegalForm"/>
        <dc:title xml:lang="en">Association of political parties</dc:title>
        <dc:title xml:lang="lv">Politisko partiju apvienība</dc:title>
        <rdfs:label rdf:datatype="http://www.w3.org/2001/XMLSchema#string">PPA</rdfs:label>
    </owl:NamedIndividual>
    


    <!-- http://w3id.org/um/cbcm/eu-cm-ontology#lv903 -->

    <owl:NamedIndividual rdf:about="http://w3id.org/um/cbcm/eu-cm-ontology#lv903">
        <rdf:type rdf:resource="http://w3id.org/um/cbcm/eu-cm-ontology#CompanyLegalForm"/>
        <dc:title xml:lang="en">Permanent representative office</dc:title>
        <dc:title xml:lang="lv">Pārstāvniecība</dc:title>
        <rdfs:label rdf:datatype="http://www.w3.org/2001/XMLSchema#string">PAR</rdfs:label>
    </owl:NamedIndividual>
    


    <!-- http://w3id.org/um/cbcm/eu-cm-ontology#malta -->

    <owl:NamedIndividual rdf:about="http://w3id.org/um/cbcm/eu-cm-ontology#malta">
        <rdf:type rdf:resource="http://w3id.org/um/cbcm/eu-cm-ontology#EUCountry"/>
        <cbcm:countryHasCompanyForm rdf:resource="http://w3id.org/um/cbcm/eu-cm-ontology#mt020"/>
        <cbcm:countryHasCompanyForm rdf:resource="http://w3id.org/um/cbcm/eu-cm-ontology#mt021"/>
        <cbcm:countryHasCompanyForm rdf:resource="http://w3id.org/um/cbcm/eu-cm-ontology#mt030"/>
        <cbcm:countryHasCompanyForm rdf:resource="http://w3id.org/um/cbcm/eu-cm-ontology#mt033"/>
        <cbcm:countryHasCompanyForm rdf:resource="http://w3id.org/um/cbcm/eu-cm-ontology#mt040"/>
        <cbcm:countryHasCompanyForm rdf:resource="http://w3id.org/um/cbcm/eu-cm-ontology#mt060"/>
        <cbcm:countryHasCompanyForm rdf:resource="http://w3id.org/um/cbcm/eu-cm-ontology#mt080"/>
        <cbcm:iso2code>MT</cbcm:iso2code>
        <rdfs:label xml:lang="en">Malta</rdfs:label>
        <rdfs:label xml:lang="en">Melita</rdfs:label>
        <rdfs:label xml:lang="mt">Repubblika ta&apos; Malta</rdfs:label>
    </owl:NamedIndividual>
    


    <!-- http://w3id.org/um/cbcm/eu-cm-ontology#mt020 -->

    <owl:NamedIndividual rdf:about="http://w3id.org/um/cbcm/eu-cm-ontology#mt020">
        <rdf:type rdf:resource="http://w3id.org/um/cbcm/eu-cm-ontology#CompanyLegalForm"/>
        <dc:title xml:lang="en">A limited Partnership</dc:title>
        <dc:title xml:lang="mt">En commandite</dc:title>
        <rdfs:label rdf:datatype="http://www.w3.org/2001/XMLSchema#string">PCOMM</rdfs:label>
    </owl:NamedIndividual>
    


    <!-- http://w3id.org/um/cbcm/eu-cm-ontology#mt021 -->

    <owl:NamedIndividual rdf:about="http://w3id.org/um/cbcm/eu-cm-ontology#mt021">
        <rdf:type rdf:resource="http://w3id.org/um/cbcm/eu-cm-ontology#CompanyLegalForm"/>
        <dc:title xml:lang="en">A general Partnership</dc:title>
        <dc:title xml:lang="mt">En nom collectif</dc:title>
        <rdfs:label rdf:datatype="http://www.w3.org/2001/XMLSchema#string">P</rdfs:label>
    </owl:NamedIndividual>
    


    <!-- http://w3id.org/um/cbcm/eu-cm-ontology#mt030 -->

    <owl:NamedIndividual rdf:about="http://w3id.org/um/cbcm/eu-cm-ontology#mt030">
        <rdf:type rdf:resource="http://w3id.org/um/cbcm/eu-cm-ontology#CompanyLegalForm"/>
        <dc:title xml:lang="mt">Limited</dc:title>
        <dc:title xml:lang="en">Private limited company</dc:title>
        <rdfs:label rdf:datatype="http://www.w3.org/2001/XMLSchema#string">LTD</rdfs:label>
    </owl:NamedIndividual>
    


    <!-- http://w3id.org/um/cbcm/eu-cm-ontology#mt033 -->

    <owl:NamedIndividual rdf:about="http://w3id.org/um/cbcm/eu-cm-ontology#mt033">
        <rdf:type rdf:resource="http://w3id.org/um/cbcm/eu-cm-ontology#CompanyLegalForm"/>
        <dc:title xml:lang="en">Investment companies with variable share capital</dc:title>
        <dc:title xml:lang="mt">SICAV (Société d’Investissement à Capital Variable)</dc:title>
        <rdfs:label rdf:datatype="http://www.w3.org/2001/XMLSchema#string">SV</rdfs:label>
    </owl:NamedIndividual>
    


    <!-- http://w3id.org/um/cbcm/eu-cm-ontology#mt040 -->

    <owl:NamedIndividual rdf:about="http://w3id.org/um/cbcm/eu-cm-ontology#mt040">
        <rdf:type rdf:resource="http://w3id.org/um/cbcm/eu-cm-ontology#CompanyLegalForm"/>
        <dc:title xml:lang="mt">  Non-for profit Organisations</dc:title>
        <dc:title xml:lang="mt">Voluntary </dc:title>
        <dc:title xml:lang="en">Voluntary / Non-for profit Organisations</dc:title>
        <rdfs:label rdf:datatype="http://www.w3.org/2001/XMLSchema#string">VO</rdfs:label>
    </owl:NamedIndividual>
    


    <!-- http://w3id.org/um/cbcm/eu-cm-ontology#mt060 -->

    <owl:NamedIndividual rdf:about="http://w3id.org/um/cbcm/eu-cm-ontology#mt060">
        <rdf:type rdf:resource="http://w3id.org/um/cbcm/eu-cm-ontology#CompanyLegalForm"/>
        <dc:title xml:lang="en">Public limited company</dc:title>
        <dc:title xml:lang="mt">Public limited company</dc:title>
        <rdfs:label rdf:datatype="http://www.w3.org/2001/XMLSchema#string">PLC</rdfs:label>
    </owl:NamedIndividual>
    


    <!-- http://w3id.org/um/cbcm/eu-cm-ontology#mt080 -->

    <owl:NamedIndividual rdf:about="http://w3id.org/um/cbcm/eu-cm-ontology#mt080">
        <rdf:type rdf:resource="http://w3id.org/um/cbcm/eu-cm-ontology#CompanyLegalForm"/>
        <dc:title xml:lang="en">Cooperatives</dc:title>
        <dc:title xml:lang="mt">Cooperatives</dc:title>
        <rdfs:label rdf:datatype="http://www.w3.org/2001/XMLSchema#string">COOP</rdfs:label>
    </owl:NamedIndividual>
    


    <!-- http://w3id.org/um/cbcm/eu-cm-ontology#netherlands -->

    <owl:NamedIndividual rdf:about="http://w3id.org/um/cbcm/eu-cm-ontology#netherlands">
        <rdf:type rdf:resource="http://w3id.org/um/cbcm/eu-cm-ontology#EUCountry"/>
        <cbcm:countryHasCompanyForm rdf:resource="http://w3id.org/um/cbcm/eu-cm-ontology#nl101"/>
        <cbcm:countryHasCompanyForm rdf:resource="http://w3id.org/um/cbcm/eu-cm-ontology#nl102"/>
        <cbcm:countryHasCompanyForm rdf:resource="http://w3id.org/um/cbcm/eu-cm-ontology#nl202"/>
        <cbcm:countryHasCompanyForm rdf:resource="http://w3id.org/um/cbcm/eu-cm-ontology#nl204"/>
        <cbcm:iso2code>NL</cbcm:iso2code>
        <rdfs:label xml:lang="en">Holland</rdfs:label>
        <rdfs:label xml:lang="nl">Nederland</rdfs:label>
        <rdfs:label xml:lang="en">Netherlands</rdfs:label>
        <rdfs:label xml:lang="en">The Netherlands</rdfs:label>
    </owl:NamedIndividual>
    


    <!-- http://w3id.org/um/cbcm/eu-cm-ontology#nl101 -->

    <owl:NamedIndividual rdf:about="http://w3id.org/um/cbcm/eu-cm-ontology#nl101">
        <rdf:type rdf:resource="http://w3id.org/um/cbcm/eu-cm-ontology#CompanyLegalForm"/>
        <dc:title xml:lang="nl">Besloten vennootschap</dc:title>
        <dc:title xml:lang="en">private limited company</dc:title>
        <rdfs:label rdf:datatype="http://www.w3.org/2001/XMLSchema#string">BV</rdfs:label>
    </owl:NamedIndividual>
    


    <!-- http://w3id.org/um/cbcm/eu-cm-ontology#nl102 -->

    <owl:NamedIndividual rdf:about="http://w3id.org/um/cbcm/eu-cm-ontology#nl102">
        <rdf:type rdf:resource="http://w3id.org/um/cbcm/eu-cm-ontology#CompanyLegalForm"/>
        <dc:title xml:lang="nl">Naamloze vennootschap</dc:title>
        <dc:title xml:lang="en">public limited company</dc:title>
        <rdfs:label rdf:datatype="http://www.w3.org/2001/XMLSchema#string">NV</rdfs:label>
    </owl:NamedIndividual>
    


    <!-- http://w3id.org/um/cbcm/eu-cm-ontology#nl202 -->

    <owl:NamedIndividual rdf:about="http://w3id.org/um/cbcm/eu-cm-ontology#nl202">
        <rdf:type rdf:resource="http://w3id.org/um/cbcm/eu-cm-ontology#CompanyLegalForm"/>
        <dc:title xml:lang="nl">Onderlinge waarborgmaatschappij</dc:title>
        <dc:title xml:lang="en">mutual insurance association</dc:title>
        <rdfs:label rdf:datatype="http://www.w3.org/2001/XMLSchema#string">OWM</rdfs:label>
    </owl:NamedIndividual>
    


    <!-- http://w3id.org/um/cbcm/eu-cm-ontology#nl204 -->

    <owl:NamedIndividual rdf:about="http://w3id.org/um/cbcm/eu-cm-ontology#nl204">
        <rdf:type rdf:resource="http://w3id.org/um/cbcm/eu-cm-ontology#CompanyLegalForm"/>
        <dc:title xml:lang="en">(home) owners association</dc:title>
        <dc:title xml:lang="nl">Vereniging van eigenaars</dc:title>
        <rdfs:label rdf:datatype="http://www.w3.org/2001/XMLSchema#string">VVE</rdfs:label>
    </owl:NamedIndividual>
    


    <!-- http://w3id.org/um/cbcm/eu-cm-ontology#norway -->

    <owl:NamedIndividual rdf:about="http://w3id.org/um/cbcm/eu-cm-ontology#norway">
        <rdf:type rdf:resource="http://w3id.org/um/cbcm/eu-cm-ontology#EEACountry"/>
        <cbcm:iso2code>NO</cbcm:iso2code>
        <rdfs:label xml:lang="en">Kingdom of Norway</rdfs:label>
        <rdfs:label xml:lang="no">Kongeriket Noreg</rdfs:label>
        <rdfs:label xml:lang="no">Kongeriket Norge</rdfs:label>
        <rdfs:label xml:lang="no">Noreg</rdfs:label>
        <rdfs:label xml:lang="no">Norge</rdfs:label>
        <rdfs:label xml:lang="no">Norgga</rdfs:label>
        <rdfs:label xml:lang="no">Norgga gonagasriika</rdfs:label>
        <rdfs:label xml:lang="en">Norway</rdfs:label>
        <rdfs:label xml:lang="no">Nöörjen</rdfs:label>
        <rdfs:label xml:lang="no">Vuona</rdfs:label>
    </owl:NamedIndividual>
    


    <!-- http://w3id.org/um/cbcm/eu-cm-ontology#pla019 -->

    <owl:NamedIndividual rdf:about="http://w3id.org/um/cbcm/eu-cm-ontology#pla019">
        <rdf:type rdf:resource="http://w3id.org/um/cbcm/eu-cm-ontology#CompanyLegalForm"/>
        <dc:title xml:lang="en">civil law partnership</dc:title>
        <dc:title xml:lang="pl">spółki cywilne</dc:title>
        <rdfs:label rdf:datatype="http://www.w3.org/2001/XMLSchema#string">s.c.</rdfs:label>
    </owl:NamedIndividual>
    


    <!-- http://w3id.org/um/cbcm/eu-cm-ontology#pla115 -->

    <owl:NamedIndividual rdf:about="http://w3id.org/um/cbcm/eu-cm-ontology#pla115">
        <rdf:type rdf:resource="http://w3id.org/um/cbcm/eu-cm-ontology#CompanyLegalForm"/>
        <dc:title xml:lang="en">professional partnership</dc:title>
        <dc:title xml:lang="pl">spółki partnerskie</dc:title>
        <rdfs:label rdf:datatype="http://www.w3.org/2001/XMLSchema#string">sp.p.</rdfs:label>
    </owl:NamedIndividual>
    


    <!-- http://w3id.org/um/cbcm/eu-cm-ontology#pla116 -->

    <owl:NamedIndividual rdf:about="http://w3id.org/um/cbcm/eu-cm-ontology#pla116">
        <rdf:type rdf:resource="http://w3id.org/um/cbcm/eu-cm-ontology#CompanyLegalForm"/>
        <dc:title xml:lang="en">joint-stock company</dc:title>
        <dc:title xml:lang="pl">spółki akcyjne</dc:title>
        <rdfs:label rdf:datatype="http://www.w3.org/2001/XMLSchema#string">S.A.</rdfs:label>
    </owl:NamedIndividual>
    


    <!-- http://w3id.org/um/cbcm/eu-cm-ontology#pla117 -->

    <owl:NamedIndividual rdf:about="http://w3id.org/um/cbcm/eu-cm-ontology#pla117">
        <rdf:type rdf:resource="http://w3id.org/um/cbcm/eu-cm-ontology#CompanyLegalForm"/>
        <dc:title xml:lang="en">limited liability company</dc:title>
        <dc:title xml:lang="pl">spółki z ograniczoną odpowiedzialnością</dc:title>
        <rdfs:label rdf:datatype="http://www.w3.org/2001/XMLSchema#string">sp.zo.o.</rdfs:label>
    </owl:NamedIndividual>
    


    <!-- http://w3id.org/um/cbcm/eu-cm-ontology#pla118 -->

    <owl:NamedIndividual rdf:about="http://w3id.org/um/cbcm/eu-cm-ontology#pla118">
        <rdf:type rdf:resource="http://w3id.org/um/cbcm/eu-cm-ontology#CompanyLegalForm"/>
        <dc:title xml:lang="en">registered partnership</dc:title>
        <dc:title xml:lang="pl">spółki jawne</dc:title>
        <rdfs:label rdf:datatype="http://www.w3.org/2001/XMLSchema#string">s.j.</rdfs:label>
    </owl:NamedIndividual>
    


    <!-- http://w3id.org/um/cbcm/eu-cm-ontology#pla120 -->

    <owl:NamedIndividual rdf:about="http://w3id.org/um/cbcm/eu-cm-ontology#pla120">
        <rdf:type rdf:resource="http://w3id.org/um/cbcm/eu-cm-ontology#CompanyLegalForm"/>
        <dc:title xml:lang="en">limited partnership</dc:title>
        <dc:title xml:lang="pl">spółki komandytowe</dc:title>
        <rdfs:label rdf:datatype="http://www.w3.org/2001/XMLSchema#string">sp.k.</rdfs:label>
    </owl:NamedIndividual>
    


    <!-- http://w3id.org/um/cbcm/eu-cm-ontology#pla121 -->

    <owl:NamedIndividual rdf:about="http://w3id.org/um/cbcm/eu-cm-ontology#pla121">
        <rdf:type rdf:resource="http://w3id.org/um/cbcm/eu-cm-ontology#CompanyLegalForm"/>
        <dc:title xml:lang="en">limited joint-stock partnership</dc:title>
        <dc:title xml:lang="pl">spółki komandytowo - akcyjne</dc:title>
        <rdfs:label rdf:datatype="http://www.w3.org/2001/XMLSchema#string">S.K.A.</rdfs:label>
    </owl:NamedIndividual>
    


    <!-- http://w3id.org/um/cbcm/eu-cm-ontology#pla126 -->

    <owl:NamedIndividual rdf:about="http://w3id.org/um/cbcm/eu-cm-ontology#pla126">
        <rdf:type rdf:resource="http://w3id.org/um/cbcm/eu-cm-ontology#CompanyLegalForm"/>
        <dc:title xml:lang="en">mutual insurance society</dc:title>
        <dc:title xml:lang="pl">towarzystwa ubezpieczeń wzajemnych</dc:title>
        <rdfs:label rdf:datatype="http://www.w3.org/2001/XMLSchema#string">TUW</rdfs:label>
    </owl:NamedIndividual>
    


    <!-- http://w3id.org/um/cbcm/eu-cm-ontology#pld049 -->

    <owl:NamedIndividual rdf:about="http://w3id.org/um/cbcm/eu-cm-ontology#pld049">
        <rdf:type rdf:resource="http://w3id.org/um/cbcm/eu-cm-ontology#CompanyLegalForm"/>
        <dc:title xml:lang="en">open pension fund</dc:title>
        <dc:title xml:lang="pl">otwarte fundusze emerytalne</dc:title>
        <rdfs:label rdf:datatype="http://www.w3.org/2001/XMLSchema#string">OFE</rdfs:label>
    </owl:NamedIndividual>
    


    <!-- http://w3id.org/um/cbcm/eu-cm-ontology#poland -->

    <owl:NamedIndividual rdf:about="http://w3id.org/um/cbcm/eu-cm-ontology#poland">
        <rdf:type rdf:resource="http://w3id.org/um/cbcm/eu-cm-ontology#EUCountry"/>
        <cbcm:countryHasCompanyForm rdf:resource="http://w3id.org/um/cbcm/eu-cm-ontology#pla019"/>
        <cbcm:countryHasCompanyForm rdf:resource="http://w3id.org/um/cbcm/eu-cm-ontology#pla115"/>
        <cbcm:countryHasCompanyForm rdf:resource="http://w3id.org/um/cbcm/eu-cm-ontology#pla116"/>
        <cbcm:countryHasCompanyForm rdf:resource="http://w3id.org/um/cbcm/eu-cm-ontology#pla117"/>
        <cbcm:countryHasCompanyForm rdf:resource="http://w3id.org/um/cbcm/eu-cm-ontology#pla118"/>
        <cbcm:countryHasCompanyForm rdf:resource="http://w3id.org/um/cbcm/eu-cm-ontology#pla120"/>
        <cbcm:countryHasCompanyForm rdf:resource="http://w3id.org/um/cbcm/eu-cm-ontology#pla121"/>
        <cbcm:countryHasCompanyForm rdf:resource="http://w3id.org/um/cbcm/eu-cm-ontology#pla126"/>
        <cbcm:countryHasCompanyForm rdf:resource="http://w3id.org/um/cbcm/eu-cm-ontology#pld049"/>
        <cbcm:iso2code>PL</cbcm:iso2code>
        <rdfs:label xml:lang="en">Poland</rdfs:label>
        <rdfs:label xml:lang="pl">Polska</rdfs:label>
        <rdfs:label xml:lang="en">Republic of Poland</rdfs:label>
        <rdfs:label xml:lang="pl">Rzeczpospolita Polska</rdfs:label>
    </owl:NamedIndividual>
    


    <!-- http://w3id.org/um/cbcm/eu-cm-ontology#portugal -->

    <owl:NamedIndividual rdf:about="http://w3id.org/um/cbcm/eu-cm-ontology#portugal">
        <rdf:type rdf:resource="http://w3id.org/um/cbcm/eu-cm-ontology#EUCountry"/>
        <cbcm:countryHasCompanyForm rdf:resource="http://w3id.org/um/cbcm/eu-cm-ontology#pt111"/>
        <cbcm:countryHasCompanyForm rdf:resource="http://w3id.org/um/cbcm/eu-cm-ontology#pt121"/>
        <cbcm:countryHasCompanyForm rdf:resource="http://w3id.org/um/cbcm/eu-cm-ontology#pt122"/>
        <cbcm:countryHasCompanyForm rdf:resource="http://w3id.org/um/cbcm/eu-cm-ontology#pt131"/>
        <cbcm:countryHasCompanyForm rdf:resource="http://w3id.org/um/cbcm/eu-cm-ontology#pt141"/>
        <cbcm:countryHasCompanyForm rdf:resource="http://w3id.org/um/cbcm/eu-cm-ontology#pt151"/>
        <cbcm:countryHasCompanyForm rdf:resource="http://w3id.org/um/cbcm/eu-cm-ontology#pt171"/>
        <cbcm:countryHasCompanyForm rdf:resource="http://w3id.org/um/cbcm/eu-cm-ontology#pt182"/>
        <cbcm:countryHasCompanyForm rdf:resource="http://w3id.org/um/cbcm/eu-cm-ontology#pt211"/>
        <cbcm:countryHasCompanyForm rdf:resource="http://w3id.org/um/cbcm/eu-cm-ontology#pt221"/>
        <cbcm:countryHasCompanyForm rdf:resource="http://w3id.org/um/cbcm/eu-cm-ontology#pt231"/>
        <cbcm:countryHasCompanyForm rdf:resource="http://w3id.org/um/cbcm/eu-cm-ontology#pt311"/>
        <cbcm:countryHasCompanyForm rdf:resource="http://w3id.org/um/cbcm/eu-cm-ontology#pt312"/>
        <cbcm:countryHasCompanyForm rdf:resource="http://w3id.org/um/cbcm/eu-cm-ontology#pt321"/>
        <cbcm:countryHasCompanyForm rdf:resource="http://w3id.org/um/cbcm/eu-cm-ontology#pt331"/>
        <cbcm:countryHasCompanyForm rdf:resource="http://w3id.org/um/cbcm/eu-cm-ontology#pt411"/>
        <cbcm:countryHasCompanyForm rdf:resource="http://w3id.org/um/cbcm/eu-cm-ontology#pt901"/>
        <cbcm:iso2code>PT</cbcm:iso2code>
        <rdfs:label xml:lang="en">Portugal</rdfs:label>
        <rdfs:label xml:lang="en">Portuguese Republic</rdfs:label>
        <rdfs:label xml:lang="pt">República Portuguesa</rdfs:label>
    </owl:NamedIndividual>
    


    <!-- http://w3id.org/um/cbcm/eu-cm-ontology#pt111 -->

    <owl:NamedIndividual rdf:about="http://w3id.org/um/cbcm/eu-cm-ontology#pt111">
        <rdf:type rdf:resource="http://w3id.org/um/cbcm/eu-cm-ontology#CompanyLegalForm"/>
        <dc:title xml:lang="pt">Agrupamento Complementar de Empresas (ACE)</dc:title>
        <dc:title xml:lang="en">Complementary Grouping of Companies </dc:title>
        <rdfs:label rdf:datatype="http://www.w3.org/2001/XMLSchema#string">ACE</rdfs:label>
    </owl:NamedIndividual>
    


    <!-- http://w3id.org/um/cbcm/eu-cm-ontology#pt121 -->

    <owl:NamedIndividual rdf:about="http://w3id.org/um/cbcm/eu-cm-ontology#pt121">
        <rdf:type rdf:resource="http://w3id.org/um/cbcm/eu-cm-ontology#CompanyLegalForm"/>
        <dc:title xml:lang="en">Private limited company</dc:title>
        <dc:title xml:lang="pt">Sociedade por Quotas</dc:title>
        <rdfs:label rdf:datatype="http://www.w3.org/2001/XMLSchema#string">Lda</rdfs:label>
    </owl:NamedIndividual>
    


    <!-- http://w3id.org/um/cbcm/eu-cm-ontology#pt122 -->

    <owl:NamedIndividual rdf:about="http://w3id.org/um/cbcm/eu-cm-ontology#pt122">
        <rdf:type rdf:resource="http://w3id.org/um/cbcm/eu-cm-ontology#CompanyLegalForm"/>
        <dc:title xml:lang="en">Single holder private limited company</dc:title>
        <dc:title xml:lang="pt">Sociedade Unipessoal Por Quotas</dc:title>
        <rdfs:label rdf:datatype="http://www.w3.org/2001/XMLSchema#string">SUni</rdfs:label>
    </owl:NamedIndividual>
    


    <!-- http://w3id.org/um/cbcm/eu-cm-ontology#pt131 -->

    <owl:NamedIndividual rdf:about="http://w3id.org/um/cbcm/eu-cm-ontology#pt131">
        <rdf:type rdf:resource="http://w3id.org/um/cbcm/eu-cm-ontology#CompanyLegalForm"/>
        <dc:title xml:lang="en">Public limited company</dc:title>
        <dc:title xml:lang="pt">Sociedade Anónima</dc:title>
        <rdfs:label rdf:datatype="http://www.w3.org/2001/XMLSchema#string">SAxa0</rdfs:label>
    </owl:NamedIndividual>
    


    <!-- http://w3id.org/um/cbcm/eu-cm-ontology#pt141 -->

    <owl:NamedIndividual rdf:about="http://w3id.org/um/cbcm/eu-cm-ontology#pt141">
        <rdf:type rdf:resource="http://w3id.org/um/cbcm/eu-cm-ontology#CompanyLegalForm"/>
        <dc:title xml:lang="en">Limited partnership</dc:title>
        <dc:title xml:lang="pt">Sociedades em Comandita</dc:title>
        <rdfs:label rdf:datatype="http://www.w3.org/2001/XMLSchema#string">Coman</rdfs:label>
    </owl:NamedIndividual>
    


    <!-- http://w3id.org/um/cbcm/eu-cm-ontology#pt151 -->

    <owl:NamedIndividual rdf:about="http://w3id.org/um/cbcm/eu-cm-ontology#pt151">
        <rdf:type rdf:resource="http://w3id.org/um/cbcm/eu-cm-ontology#CompanyLegalForm"/>
        <dc:title xml:lang="en">Partnerships</dc:title>
        <dc:title xml:lang="pt">Sociedades em Nome Coletivo</dc:title>
        <rdfs:label rdf:datatype="http://www.w3.org/2001/XMLSchema#string">SNC</rdfs:label>
    </owl:NamedIndividual>
    


    <!-- http://w3id.org/um/cbcm/eu-cm-ontology#pt171 -->

    <owl:NamedIndividual rdf:about="http://w3id.org/um/cbcm/eu-cm-ontology#pt171">
        <rdf:type rdf:resource="http://w3id.org/um/cbcm/eu-cm-ontology#CompanyLegalForm"/>
        <dc:title xml:lang="en">Civil society</dc:title>
        <dc:title xml:lang="pt">Sociedade Civil</dc:title>
        <rdfs:label rdf:datatype="http://www.w3.org/2001/XMLSchema#string">SOCI</rdfs:label>
    </owl:NamedIndividual>
    


    <!-- http://w3id.org/um/cbcm/eu-cm-ontology#pt182 -->

    <owl:NamedIndividual rdf:about="http://w3id.org/um/cbcm/eu-cm-ontology#pt182">
        <rdf:type rdf:resource="http://w3id.org/um/cbcm/eu-cm-ontology#CompanyLegalForm"/>
        <dc:title xml:lang="pt">Estabelecimento Individual de Responsabilidade Limitada</dc:title>
        <dc:title xml:lang="en">Individual business with limited liability</dc:title>
        <rdfs:label rdf:datatype="http://www.w3.org/2001/XMLSchema#string">EIRL</rdfs:label>
    </owl:NamedIndividual>
    


    <!-- http://w3id.org/um/cbcm/eu-cm-ontology#pt211 -->

    <owl:NamedIndividual rdf:about="http://w3id.org/um/cbcm/eu-cm-ontology#pt211">
        <rdf:type rdf:resource="http://w3id.org/um/cbcm/eu-cm-ontology#CompanyLegalForm"/>
        <dc:title xml:lang="pt">Cooperativa</dc:title>
        <dc:title xml:lang="en">Cooperative</dc:title>
        <rdfs:label rdf:datatype="http://www.w3.org/2001/XMLSchema#string">Coop</rdfs:label>
    </owl:NamedIndividual>
    


    <!-- http://w3id.org/um/cbcm/eu-cm-ontology#pt221 -->

    <owl:NamedIndividual rdf:about="http://w3id.org/um/cbcm/eu-cm-ontology#pt221">
        <rdf:type rdf:resource="http://w3id.org/um/cbcm/eu-cm-ontology#CompanyLegalForm"/>
        <dc:title xml:lang="en">Association</dc:title>
        <dc:title xml:lang="pt">Associação</dc:title>
        <rdfs:label rdf:datatype="http://www.w3.org/2001/XMLSchema#string">Assoc</rdfs:label>
    </owl:NamedIndividual>
    


    <!-- http://w3id.org/um/cbcm/eu-cm-ontology#pt231 -->

    <owl:NamedIndividual rdf:about="http://w3id.org/um/cbcm/eu-cm-ontology#pt231">
        <rdf:type rdf:resource="http://w3id.org/um/cbcm/eu-cm-ontology#CompanyLegalForm"/>
        <dc:title xml:lang="en">Foundation</dc:title>
        <dc:title xml:lang="pt">Fundação</dc:title>
        <rdfs:label rdf:datatype="http://www.w3.org/2001/XMLSchema#string">Fund</rdfs:label>
    </owl:NamedIndividual>
    


    <!-- http://w3id.org/um/cbcm/eu-cm-ontology#pt311 -->

    <owl:NamedIndividual rdf:about="http://w3id.org/um/cbcm/eu-cm-ontology#pt311">
        <rdf:type rdf:resource="http://w3id.org/um/cbcm/eu-cm-ontology#CompanyLegalForm"/>
        <dc:title xml:lang="pt">Entidade Pública Empresarial</dc:title>
        <dc:title xml:lang="en">Public corporation</dc:title>
        <rdfs:label rdf:datatype="http://www.w3.org/2001/XMLSchema#string">EPE</rdfs:label>
    </owl:NamedIndividual>
    


    <!-- http://w3id.org/um/cbcm/eu-cm-ontology#pt312 -->

    <owl:NamedIndividual rdf:about="http://w3id.org/um/cbcm/eu-cm-ontology#pt312">
        <rdf:type rdf:resource="http://w3id.org/um/cbcm/eu-cm-ontology#CompanyLegalForm"/>
        <dc:title xml:lang="pt">Pessoa Coletiva de Direito Público</dc:title>
        <dc:title xml:lang="en">Public law institution</dc:title>
        <rdfs:label rdf:datatype="http://www.w3.org/2001/XMLSchema#string">PCDP</rdfs:label>
    </owl:NamedIndividual>
    


    <!-- http://w3id.org/um/cbcm/eu-cm-ontology#pt321 -->

    <owl:NamedIndividual rdf:about="http://w3id.org/um/cbcm/eu-cm-ontology#pt321">
        <rdf:type rdf:resource="http://w3id.org/um/cbcm/eu-cm-ontology#CompanyLegalForm"/>
        <dc:title xml:lang="en"> Intermunicipal and Regional public company</dc:title>
        <dc:title xml:lang="pt"> Intermunicipal e Regional</dc:title>
        <dc:title xml:lang="pt">Entidade Pública Municipal</dc:title>
        <dc:title xml:lang="en">Municipal</dc:title>
        <rdfs:label rdf:datatype="http://www.w3.org/2001/XMLSchema#string">EPMR</rdfs:label>
    </owl:NamedIndividual>
    


    <!-- http://w3id.org/um/cbcm/eu-cm-ontology#pt331 -->

    <owl:NamedIndividual rdf:about="http://w3id.org/um/cbcm/eu-cm-ontology#pt331">
        <rdf:type rdf:resource="http://w3id.org/um/cbcm/eu-cm-ontology#CompanyLegalForm"/>
        <dc:title xml:lang="pt">Organismo da Administração Pública</dc:title>
        <dc:title xml:lang="en">Public Institution</dc:title>
        <rdfs:label rdf:datatype="http://www.w3.org/2001/XMLSchema#string">OAP</rdfs:label>
    </owl:NamedIndividual>
    


    <!-- http://w3id.org/um/cbcm/eu-cm-ontology#pt411 -->

    <owl:NamedIndividual rdf:about="http://w3id.org/um/cbcm/eu-cm-ontology#pt411">
        <rdf:type rdf:resource="http://w3id.org/um/cbcm/eu-cm-ontology#CompanyLegalForm"/>
        <dc:title xml:lang="pt">Pessoa Colectiva Religiosa</dc:title>
        <dc:title xml:lang="en">Religious legal person</dc:title>
        <rdfs:label rdf:datatype="http://www.w3.org/2001/XMLSchema#string">PCR</rdfs:label>
    </owl:NamedIndividual>
    


    <!-- http://w3id.org/um/cbcm/eu-cm-ontology#pt901 -->

    <owl:NamedIndividual rdf:about="http://w3id.org/um/cbcm/eu-cm-ontology#pt901">
        <rdf:type rdf:resource="http://w3id.org/um/cbcm/eu-cm-ontology#CompanyLegalForm"/>
        <dc:title xml:lang="en">International Organizations</dc:title>
        <dc:title xml:lang="pt">Organizações Internacionais</dc:title>
        <rdfs:label rdf:datatype="http://www.w3.org/2001/XMLSchema#string">OI</rdfs:label>
    </owl:NamedIndividual>
    


    <!-- http://w3id.org/um/cbcm/eu-cm-ontology#ro101 -->

    <owl:NamedIndividual rdf:about="http://w3id.org/um/cbcm/eu-cm-ontology#ro101">
        <rdf:type rdf:resource="http://w3id.org/um/cbcm/eu-cm-ontology#CompanyLegalForm"/>
        <dc:title xml:lang="en">Joint Stock Company</dc:title>
        <dc:title xml:lang="ro">Societate pe acţiuni</dc:title>
        <rdfs:label rdf:datatype="http://www.w3.org/2001/XMLSchema#string">SAxa0</rdfs:label>
    </owl:NamedIndividual>
    


    <!-- http://w3id.org/um/cbcm/eu-cm-ontology#ro102 -->

    <owl:NamedIndividual rdf:about="http://w3id.org/um/cbcm/eu-cm-ontology#ro102">
        <rdf:type rdf:resource="http://w3id.org/um/cbcm/eu-cm-ontology#CompanyLegalForm"/>
        <dc:title xml:lang="en">Limited Liability Company (Ltd)</dc:title>
        <dc:title xml:lang="ro">Societate cu răspundere limitată</dc:title>
        <rdfs:label rdf:datatype="http://www.w3.org/2001/XMLSchema#string">SRL</rdfs:label>
    </owl:NamedIndividual>
    


    <!-- http://w3id.org/um/cbcm/eu-cm-ontology#ro103 -->

    <owl:NamedIndividual rdf:about="http://w3id.org/um/cbcm/eu-cm-ontology#ro103">
        <rdf:type rdf:resource="http://w3id.org/um/cbcm/eu-cm-ontology#CompanyLegalForm"/>
        <dc:title xml:lang="en">Limited partnership</dc:title>
        <dc:title xml:lang="ro">Societate în comandită simplă</dc:title>
        <rdfs:label rdf:datatype="http://www.w3.org/2001/XMLSchema#string">SCS</rdfs:label>
    </owl:NamedIndividual>
    


    <!-- http://w3id.org/um/cbcm/eu-cm-ontology#ro104 -->

    <owl:NamedIndividual rdf:about="http://w3id.org/um/cbcm/eu-cm-ontology#ro104">
        <rdf:type rdf:resource="http://w3id.org/um/cbcm/eu-cm-ontology#CompanyLegalForm"/>
        <dc:title xml:lang="en">Limited partnership with shares</dc:title>
        <dc:title xml:lang="ro">Societate în comandită pe acţiuni</dc:title>
        <rdfs:label rdf:datatype="http://www.w3.org/2001/XMLSchema#string">SCA</rdfs:label>
    </owl:NamedIndividual>
    


    <!-- http://w3id.org/um/cbcm/eu-cm-ontology#ro107 -->

    <owl:NamedIndividual rdf:about="http://w3id.org/um/cbcm/eu-cm-ontology#ro107">
        <rdf:type rdf:resource="http://w3id.org/um/cbcm/eu-cm-ontology#CompanyLegalForm"/>
        <dc:title xml:lang="en">Non-Governmental Organization / Non-Profit institution</dc:title>
        <dc:title xml:lang="ro">Organizație non-guvernamentală</dc:title>
        <rdfs:label rdf:datatype="http://www.w3.org/2001/XMLSchema#string">ONG</rdfs:label>
    </owl:NamedIndividual>
    


    <!-- http://w3id.org/um/cbcm/eu-cm-ontology#ro108 -->

    <owl:NamedIndividual rdf:about="http://w3id.org/um/cbcm/eu-cm-ontology#ro108">
        <rdf:type rdf:resource="http://w3id.org/um/cbcm/eu-cm-ontology#CompanyLegalForm"/>
        <dc:title xml:lang="en">General partnership</dc:title>
        <dc:title xml:lang="ro">Societate în nume colectiv</dc:title>
        <rdfs:label rdf:datatype="http://www.w3.org/2001/XMLSchema#string">SNC</rdfs:label>
    </owl:NamedIndividual>
    


    <!-- http://w3id.org/um/cbcm/eu-cm-ontology#ro110 -->

    <owl:NamedIndividual rdf:about="http://w3id.org/um/cbcm/eu-cm-ontology#ro110">
        <rdf:type rdf:resource="http://w3id.org/um/cbcm/eu-cm-ontology#CompanyLegalForm"/>
        <dc:title xml:lang="en">Public company</dc:title>
        <dc:title xml:lang="ro">Regie autonomă</dc:title>
        <rdfs:label rdf:datatype="http://www.w3.org/2001/XMLSchema#string">RA</rdfs:label>
    </owl:NamedIndividual>
    


    <!-- http://w3id.org/um/cbcm/eu-cm-ontology#ro111 -->

    <owl:NamedIndividual rdf:about="http://w3id.org/um/cbcm/eu-cm-ontology#ro111">
        <rdf:type rdf:resource="http://w3id.org/um/cbcm/eu-cm-ontology#CompanyLegalForm"/>
        <dc:title xml:lang="en">Economic interest grouping</dc:title>
        <dc:title xml:lang="ro">Grupul de interes economic</dc:title>
        <rdfs:label rdf:datatype="http://www.w3.org/2001/XMLSchema#string">GIE</rdfs:label>
    </owl:NamedIndividual>
    


    <!-- http://w3id.org/um/cbcm/eu-cm-ontology#romania -->

    <owl:NamedIndividual rdf:about="http://w3id.org/um/cbcm/eu-cm-ontology#romania">
        <rdf:type rdf:resource="http://w3id.org/um/cbcm/eu-cm-ontology#EUCountry"/>
        <cbcm:countryHasCompanyForm rdf:resource="http://w3id.org/um/cbcm/eu-cm-ontology#ro101"/>
        <cbcm:countryHasCompanyForm rdf:resource="http://w3id.org/um/cbcm/eu-cm-ontology#ro102"/>
        <cbcm:countryHasCompanyForm rdf:resource="http://w3id.org/um/cbcm/eu-cm-ontology#ro103"/>
        <cbcm:countryHasCompanyForm rdf:resource="http://w3id.org/um/cbcm/eu-cm-ontology#ro104"/>
        <cbcm:countryHasCompanyForm rdf:resource="http://w3id.org/um/cbcm/eu-cm-ontology#ro107"/>
        <cbcm:countryHasCompanyForm rdf:resource="http://w3id.org/um/cbcm/eu-cm-ontology#ro108"/>
        <cbcm:countryHasCompanyForm rdf:resource="http://w3id.org/um/cbcm/eu-cm-ontology#ro110"/>
        <cbcm:countryHasCompanyForm rdf:resource="http://w3id.org/um/cbcm/eu-cm-ontology#ro111"/>
        <cbcm:iso2code>RO</cbcm:iso2code>
        <rdfs:label xml:lang="en">Romania</rdfs:label>
        <rdfs:label xml:lang="ro">România</rdfs:label>
    </owl:NamedIndividual>
    


    <!-- http://w3id.org/um/cbcm/eu-cm-ontology#se31 -->

    <owl:NamedIndividual rdf:about="http://w3id.org/um/cbcm/eu-cm-ontology#se31">
        <rdf:type rdf:resource="http://w3id.org/um/cbcm/eu-cm-ontology#CompanyLegalForm"/>
        <dc:title xml:lang="se"> KB) </dc:title>
        <dc:title xml:lang="se"> kommanditbolag (HB</dc:title>
        <dc:title xml:lang="se">Handelsbolag</dc:title>
        <dc:title xml:lang="en">Limited partnership</dc:title>
        <rdfs:label rdf:datatype="http://www.w3.org/2001/XMLSchema#string">HB</rdfs:label>
        <rdfs:label rdf:datatype="http://www.w3.org/2001/XMLSchema#string">KB</rdfs:label>
    </owl:NamedIndividual>
    


    <!-- http://w3id.org/um/cbcm/eu-cm-ontology#se41 -->

    <owl:NamedIndividual rdf:about="http://w3id.org/um/cbcm/eu-cm-ontology#se41">
        <rdf:type rdf:resource="http://w3id.org/um/cbcm/eu-cm-ontology#CompanyLegalForm"/>
        <dc:title xml:lang="se">Bankaktiebolag (AB)</dc:title>
        <dc:title xml:lang="en">Limited banking companies</dc:title>
        <rdfs:label rdf:datatype="http://www.w3.org/2001/XMLSchema#string">AB</rdfs:label>
    </owl:NamedIndividual>
    


    <!-- http://w3id.org/um/cbcm/eu-cm-ontology#se42 -->

    <owl:NamedIndividual rdf:about="http://w3id.org/um/cbcm/eu-cm-ontology#se42">
        <rdf:type rdf:resource="http://w3id.org/um/cbcm/eu-cm-ontology#CompanyLegalForm"/>
        <dc:title xml:lang="se">Försäkringsaktiebolag (AB)</dc:title>
        <dc:title xml:lang="en">Limited insurance companies</dc:title>
        <rdfs:label rdf:datatype="http://www.w3.org/2001/XMLSchema#string">AB</rdfs:label>
    </owl:NamedIndividual>
    


    <!-- http://w3id.org/um/cbcm/eu-cm-ontology#se49 -->

    <owl:NamedIndividual rdf:about="http://w3id.org/um/cbcm/eu-cm-ontology#se49">
        <rdf:type rdf:resource="http://w3id.org/um/cbcm/eu-cm-ontology#CompanyLegalForm"/>
        <dc:title xml:lang="en">Other limited companies</dc:title>
        <dc:title xml:lang="se">Övriga aktiebolag (AB)</dc:title>
        <rdfs:label rdf:datatype="http://www.w3.org/2001/XMLSchema#string">AB</rdfs:label>
    </owl:NamedIndividual>
    


    <!-- http://w3id.org/um/cbcm/eu-cm-ontology#se51 -->

    <owl:NamedIndividual rdf:about="http://w3id.org/um/cbcm/eu-cm-ontology#se51">
        <rdf:type rdf:resource="http://w3id.org/um/cbcm/eu-cm-ontology#CompanyLegalForm"/>
        <dc:title xml:lang="en">Economic association (minimum three members)</dc:title>
        <dc:title xml:lang="se">Ekonomisk förening (Ek. för.) </dc:title>
        <rdfs:label rdf:datatype="http://www.w3.org/2001/XMLSchema#string">Ek.för.</rdfs:label>
    </owl:NamedIndividual>
    


    <!-- http://w3id.org/um/cbcm/eu-cm-ontology#se53 -->

    <owl:NamedIndividual rdf:about="http://w3id.org/um/cbcm/eu-cm-ontology#se53">
        <rdf:type rdf:resource="http://w3id.org/um/cbcm/eu-cm-ontology#CompanyLegalForm"/>
        <dc:title xml:lang="se">Bostadsrättsförening (BRF) </dc:title>
        <dc:title xml:lang="en">Tenant owners’ associations</dc:title>
        <rdfs:label rdf:datatype="http://www.w3.org/2001/XMLSchema#string">BRF</rdfs:label>
    </owl:NamedIndividual>
    


    <!-- http://w3id.org/um/cbcm/eu-cm-ontology#se93 -->

    <owl:NamedIndividual rdf:about="http://w3id.org/um/cbcm/eu-cm-ontology#se93">
        <rdf:type rdf:resource="http://w3id.org/um/cbcm/eu-cm-ontology#CompanyLegalForm"/>
        <dc:title xml:lang="en">Savings banks</dc:title>
        <dc:title xml:lang="se">Sparbanker (Spb)</dc:title>
        <rdfs:label rdf:datatype="http://www.w3.org/2001/XMLSchema#string">Spb</rdfs:label>
    </owl:NamedIndividual>
    


    <!-- http://w3id.org/um/cbcm/eu-cm-ontology#se_conversion -->

    <owl:NamedIndividual rdf:about="http://w3id.org/um/cbcm/eu-cm-ontology#se_conversion">
        <rdf:type rdf:resource="http://w3id.org/um/cbcm/eu-cm-ontology#SEType"/>
    </owl:NamedIndividual>
    


    <!-- http://w3id.org/um/cbcm/eu-cm-ontology#se_holding -->

    <owl:NamedIndividual rdf:about="http://w3id.org/um/cbcm/eu-cm-ontology#se_holding">
        <rdf:type rdf:resource="http://w3id.org/um/cbcm/eu-cm-ontology#SEType"/>
    </owl:NamedIndividual>
    


    <!-- http://w3id.org/um/cbcm/eu-cm-ontology#se_merger -->

    <owl:NamedIndividual rdf:about="http://w3id.org/um/cbcm/eu-cm-ontology#se_merger">
        <rdf:type rdf:resource="http://w3id.org/um/cbcm/eu-cm-ontology#SEType"/>
    </owl:NamedIndividual>
    


    <!-- http://w3id.org/um/cbcm/eu-cm-ontology#se_subsidiary -->

    <owl:NamedIndividual rdf:about="http://w3id.org/um/cbcm/eu-cm-ontology#se_subsidiary">
        <rdf:type rdf:resource="http://w3id.org/um/cbcm/eu-cm-ontology#SEType"/>
    </owl:NamedIndividual>
    


    <!-- http://w3id.org/um/cbcm/eu-cm-ontology#se_unsure -->

    <owl:NamedIndividual rdf:about="http://w3id.org/um/cbcm/eu-cm-ontology#se_unsure">
        <rdf:type rdf:resource="http://w3id.org/um/cbcm/eu-cm-ontology#SEType"/>
    </owl:NamedIndividual>
    


    <!-- http://w3id.org/um/cbcm/eu-cm-ontology#si101 -->

    <owl:NamedIndividual rdf:about="http://w3id.org/um/cbcm/eu-cm-ontology#si101">
        <rdf:type rdf:resource="http://w3id.org/um/cbcm/eu-cm-ontology#CompanyLegalForm"/>
        <dc:title xml:lang="si">Družba z neomejeno odgovornostjo d.n.o.</dc:title>
        <dc:title xml:lang="en">Unlimited company (UK)</dc:title>
        <rdfs:label rdf:datatype="http://www.w3.org/2001/XMLSchema#string">d.n.o.</rdfs:label>
    </owl:NamedIndividual>
    


    <!-- http://w3id.org/um/cbcm/eu-cm-ontology#si102 -->

    <owl:NamedIndividual rdf:about="http://w3id.org/um/cbcm/eu-cm-ontology#si102">
        <rdf:type rdf:resource="http://w3id.org/um/cbcm/eu-cm-ontology#CompanyLegalForm"/>
        <dc:title xml:lang="si">Komanditna družba k.d.</dc:title>
        <dc:title xml:lang="en">Limited partnership (UK)</dc:title>
        <rdfs:label rdf:datatype="http://www.w3.org/2001/XMLSchema#string">k.d.</rdfs:label>
    </owl:NamedIndividual>
    


    <!-- http://w3id.org/um/cbcm/eu-cm-ontology#si103 -->

    <owl:NamedIndividual rdf:about="http://w3id.org/um/cbcm/eu-cm-ontology#si103">
        <rdf:type rdf:resource="http://w3id.org/um/cbcm/eu-cm-ontology#CompanyLegalForm"/>
        <dc:title xml:lang="si">Družba z omejeno odgovornostjo d.o.o.</dc:title>
        <dc:title xml:lang="en">Ltd (UK)</dc:title>
        <rdfs:label rdf:datatype="http://www.w3.org/2001/XMLSchema#string">d.o.o.</rdfs:label>
    </owl:NamedIndividual>
    


    <!-- http://w3id.org/um/cbcm/eu-cm-ontology#si104 -->

    <owl:NamedIndividual rdf:about="http://w3id.org/um/cbcm/eu-cm-ontology#si104">
        <rdf:type rdf:resource="http://w3id.org/um/cbcm/eu-cm-ontology#CompanyLegalForm"/>
        <dc:title xml:lang="si">Delniška družba d.d.</dc:title>
        <dc:title xml:lang="en">Plc (UK)</dc:title>
        <rdfs:label rdf:datatype="http://www.w3.org/2001/XMLSchema#string">d.d.</rdfs:label>
    </owl:NamedIndividual>
    


    <!-- http://w3id.org/um/cbcm/eu-cm-ontology#si105 -->

    <owl:NamedIndividual rdf:about="http://w3id.org/um/cbcm/eu-cm-ontology#si105">
        <rdf:type rdf:resource="http://w3id.org/um/cbcm/eu-cm-ontology#CompanyLegalForm"/>
        <dc:title xml:lang="si">Komanditna delniška družba k.d.d.</dc:title>
        <dc:title xml:lang="en">Limited partnership with share capital</dc:title>
        <rdfs:label rdf:datatype="http://www.w3.org/2001/XMLSchema#string">k.d.d.</rdfs:label>
    </owl:NamedIndividual>
    


    <!-- http://w3id.org/um/cbcm/eu-cm-ontology#si108 -->

    <owl:NamedIndividual rdf:about="http://w3id.org/um/cbcm/eu-cm-ontology#si108">
        <rdf:type rdf:resource="http://w3id.org/um/cbcm/eu-cm-ontology#CompanyLegalForm"/>
        <dc:title xml:lang="en">Economic Interest Grouping EIG</dc:title>
        <dc:title xml:lang="si">Gospodarsko interesno združenje GIZ</dc:title>
        <rdfs:label rdf:datatype="http://www.w3.org/2001/XMLSchema#string">GIZ</rdfs:label>
    </owl:NamedIndividual>
    


    <!-- http://w3id.org/um/cbcm/eu-cm-ontology#si112 -->

    <owl:NamedIndividual rdf:about="http://w3id.org/um/cbcm/eu-cm-ontology#si112">
        <rdf:type rdf:resource="http://w3id.org/um/cbcm/eu-cm-ontology#CompanyLegalForm"/>
        <dc:title xml:lang="en">Cooperative z.o.o.</dc:title>
        <dc:title xml:lang="si">Zadruga z.o.o.</dc:title>
        <rdfs:label rdf:datatype="http://www.w3.org/2001/XMLSchema#string">z.o.o.</rdfs:label>
    </owl:NamedIndividual>
    


    <!-- http://w3id.org/um/cbcm/eu-cm-ontology#si113 -->

    <owl:NamedIndividual rdf:about="http://w3id.org/um/cbcm/eu-cm-ontology#si113">
        <rdf:type rdf:resource="http://w3id.org/um/cbcm/eu-cm-ontology#CompanyLegalForm"/>
        <dc:title xml:lang="en">Cooperative z.b.o.</dc:title>
        <dc:title xml:lang="si">Zadruga z.b.o.</dc:title>
        <rdfs:label rdf:datatype="http://www.w3.org/2001/XMLSchema#string">z.b.o.</rdfs:label>
    </owl:NamedIndividual>
    


    <!-- http://w3id.org/um/cbcm/eu-cm-ontology#si211 -->

    <owl:NamedIndividual rdf:about="http://w3id.org/um/cbcm/eu-cm-ontology#si211">
        <rdf:type rdf:resource="http://w3id.org/um/cbcm/eu-cm-ontology#CompanyLegalForm"/>
        <dc:title xml:lang="si">Družba za vzajemno zavarovanje d.v.z.</dc:title>
        <dc:title xml:lang="en">Mutual insurance company d.v.z.</dc:title>
        <rdfs:label rdf:datatype="http://www.w3.org/2001/XMLSchema#string">d.v.z.</rdfs:label>
    </owl:NamedIndividual>
    


    <!-- http://w3id.org/um/cbcm/eu-cm-ontology#sk111 -->

    <owl:NamedIndividual rdf:about="http://w3id.org/um/cbcm/eu-cm-ontology#sk111">
        <rdf:type rdf:resource="http://w3id.org/um/cbcm/eu-cm-ontology#CompanyLegalForm"/>
        <dc:title xml:lang="en">Public commercial company</dc:title>
        <dc:title xml:lang="sk">Verejná obchodná spoločnosť</dc:title>
        <rdfs:label rdf:datatype="http://www.w3.org/2001/XMLSchema#string">v.o.s.</rdfs:label>
    </owl:NamedIndividual>
    


    <!-- http://w3id.org/um/cbcm/eu-cm-ontology#sk112 -->

    <owl:NamedIndividual rdf:about="http://w3id.org/um/cbcm/eu-cm-ontology#sk112">
        <rdf:type rdf:resource="http://w3id.org/um/cbcm/eu-cm-ontology#CompanyLegalForm"/>
        <dc:title xml:lang="en">Limited liability company</dc:title>
        <dc:title xml:lang="sk">Spoločnosť s ručením obmedzeným</dc:title>
        <rdfs:label rdf:datatype="http://www.w3.org/2001/XMLSchema#string">s.r.o.</rdfs:label>
    </owl:NamedIndividual>
    


    <!-- http://w3id.org/um/cbcm/eu-cm-ontology#sk113 -->

    <owl:NamedIndividual rdf:about="http://w3id.org/um/cbcm/eu-cm-ontology#sk113">
        <rdf:type rdf:resource="http://w3id.org/um/cbcm/eu-cm-ontology#CompanyLegalForm"/>
        <dc:title xml:lang="sk">Komanditná spoločnosť</dc:title>
        <dc:title xml:lang="en">Société commandite</dc:title>
        <rdfs:label rdf:datatype="http://www.w3.org/2001/XMLSchema#string">k.s.</rdfs:label>
    </owl:NamedIndividual>
    


    <!-- http://w3id.org/um/cbcm/eu-cm-ontology#sk119 -->

    <owl:NamedIndividual rdf:about="http://w3id.org/um/cbcm/eu-cm-ontology#sk119">
        <rdf:type rdf:resource="http://w3id.org/um/cbcm/eu-cm-ontology#CompanyLegalForm"/>
        <dc:title xml:lang="sk">Nezisková organizácia</dc:title>
        <dc:title xml:lang="en">Not profitable organization</dc:title>
        <rdfs:label rdf:datatype="http://www.w3.org/2001/XMLSchema#string">N.O.</rdfs:label>
    </owl:NamedIndividual>
    


    <!-- http://w3id.org/um/cbcm/eu-cm-ontology#sk121 -->

    <owl:NamedIndividual rdf:about="http://w3id.org/um/cbcm/eu-cm-ontology#sk121">
        <rdf:type rdf:resource="http://w3id.org/um/cbcm/eu-cm-ontology#CompanyLegalForm"/>
        <dc:title xml:lang="sk">Akciová spoločnosť</dc:title>
        <dc:title xml:lang="en">Joint stock company</dc:title>
        <rdfs:label rdf:datatype="http://www.w3.org/2001/XMLSchema#string">a.s.</rdfs:label>
    </owl:NamedIndividual>
    


    <!-- http://w3id.org/um/cbcm/eu-cm-ontology#sk301 -->

    <owl:NamedIndividual rdf:about="http://w3id.org/um/cbcm/eu-cm-ontology#sk301">
        <rdf:type rdf:resource="http://w3id.org/um/cbcm/eu-cm-ontology#CompanyLegalForm"/>
        <dc:title xml:lang="en">State enterprise</dc:title>
        <dc:title xml:lang="sk">Štátny podnik</dc:title>
        <rdfs:label rdf:datatype="http://www.w3.org/2001/XMLSchema#string">š.p.</rdfs:label>
    </owl:NamedIndividual>
    


    <!-- http://w3id.org/um/cbcm/eu-cm-ontology#sk803 -->

    <owl:NamedIndividual rdf:about="http://w3id.org/um/cbcm/eu-cm-ontology#sk803">
        <rdf:type rdf:resource="http://w3id.org/um/cbcm/eu-cm-ontology#CompanyLegalForm"/>
        <dc:title xml:lang="en">Office of local government (regional level)</dc:title>
        <dc:title xml:lang="sk">Samosprávny kraj (úrad samosprávneho kraja)</dc:title>
        <rdfs:label rdf:datatype="http://www.w3.org/2001/XMLSchema#string">VÚC</rdfs:label>
    </owl:NamedIndividual>
    


    <!-- http://w3id.org/um/cbcm/eu-cm-ontology#slovakia -->

    <owl:NamedIndividual rdf:about="http://w3id.org/um/cbcm/eu-cm-ontology#slovakia">
        <rdf:type rdf:resource="http://w3id.org/um/cbcm/eu-cm-ontology#EUCountry"/>
        <cbcm:countryHasCompanyForm rdf:resource="http://w3id.org/um/cbcm/eu-cm-ontology#sk111"/>
        <cbcm:countryHasCompanyForm rdf:resource="http://w3id.org/um/cbcm/eu-cm-ontology#sk112"/>
        <cbcm:countryHasCompanyForm rdf:resource="http://w3id.org/um/cbcm/eu-cm-ontology#sk113"/>
        <cbcm:countryHasCompanyForm rdf:resource="http://w3id.org/um/cbcm/eu-cm-ontology#sk119"/>
        <cbcm:countryHasCompanyForm rdf:resource="http://w3id.org/um/cbcm/eu-cm-ontology#sk121"/>
        <cbcm:countryHasCompanyForm rdf:resource="http://w3id.org/um/cbcm/eu-cm-ontology#sk301"/>
        <cbcm:countryHasCompanyForm rdf:resource="http://w3id.org/um/cbcm/eu-cm-ontology#sk803"/>
        <cbcm:iso2code>SK</cbcm:iso2code>
        <rdfs:label xml:lang="en">Slovak Republic</rdfs:label>
        <rdfs:label xml:lang="en">Slovakia</rdfs:label>
        <rdfs:label xml:lang="sk">Slovensko</rdfs:label>
        <rdfs:label xml:lang="sk">Slovenská republika</rdfs:label>
    </owl:NamedIndividual>
    


    <!-- http://w3id.org/um/cbcm/eu-cm-ontology#slovenia -->

    <owl:NamedIndividual rdf:about="http://w3id.org/um/cbcm/eu-cm-ontology#slovenia">
        <rdf:type rdf:resource="http://w3id.org/um/cbcm/eu-cm-ontology#EUCountry"/>
    </owl:NamedIndividual>
    


    <!-- http://w3id.org/um/cbcm/eu-cm-ontology#spain -->

    <owl:NamedIndividual rdf:about="http://w3id.org/um/cbcm/eu-cm-ontology#spain">
        <rdf:type rdf:resource="http://w3id.org/um/cbcm/eu-cm-ontology#EUCountry"/>
    </owl:NamedIndividual>
    


    <!-- http://w3id.org/um/cbcm/eu-cm-ontology#sweden -->

    <owl:NamedIndividual rdf:about="http://w3id.org/um/cbcm/eu-cm-ontology#sweden">
        <rdf:type rdf:resource="http://w3id.org/um/cbcm/eu-cm-ontology#EUCountry"/>
    </owl:NamedIndividual>
 
</rdf:RDF>



<!-- Generated by the OWL API (version 4.1.3) https://github.com/owlcs/owlapi -->

