@prefix : <http://ids.maastrichtuniversity.nl/ontologies/cbm/eu-cm-ontology#> .
@prefix dc: <http://purl.org/dc/elements/1.1/> .
@prefix obo: <http://purl.obolibrary.org/obo/> .
@prefix owl: <http://www.w3.org/2002/07/owl#> .
@prefix rdf: <http://www.w3.org/1999/02/22-rdf-syntax-ns#> .
@prefix xml: <http://www.w3.org/XML/1998/namespace> .
@prefix xsd: <http://www.w3.org/2001/XMLSchema#> .
@prefix cbcm: <http://w3id.org/um/cbcm/eu-cm-ontology#> .
@prefix foaf: <http://xmlns.com/foaf/0.1/> .
@prefix prov: <http://www.w3.org/ns/prov#> .
@prefix rdfs: <http://www.w3.org/2000/01/rdf-schema#> .
@prefix terms: <http://purl.org/dc/terms/> .
@prefix opla-sd: <http://ontologydesignpatterns.org/opla-sd#> .
@base <http://w3id.org/um/cbcm/eu-cm-ontology> .

<http://w3id.org/um/cbcm/eu-cm-ontology> rdf:type owl:Ontology ;
                                          owl:versionIRI <http://w3id.org/um/cbcm/eu-cm-ontology/1.2.2> ;
                                          owl:imports <http://purl.obolibrary.org/obo/bfo/2019-08-26/bfo.owl> ;
                                          <http://creativecommons.org/ns#license> "https://creativecommons.org/licenses/by-sa/4.0"^^xsd:string ;
                                          dc:creator <https://www.wikidata.org/wiki/Q59418334> ,
                                                     "Marcus Meyer"^^xsd:string ,
                                                     "Stephan Rammeloo"^^xsd:string ,
                                                     "Thomas Biermeyer"^^xsd:string ;
                                          dc:description "This ontology describes terms concerning companies, their cross-border movements within the European Union (EU), and associated EU company legislation."^^xsd:string ;
                                          dc:issued "2021-12-09T00:00:00"^^xsd:dateTime ;
                                          dc:publisher <http://www.wikidata.org/wiki/Q1137652> ;
                                          dc:rights "Copyright © 2021 Maastricht University"^^xsd:string ;
                                          dc:title "The European Union Company Mobility Ontology (EUCM ontology)"^^xsd:string ;
                                          terms:contributor <http://www.wikidata.org/wiki/Q58177227> ,
                                                            "Tobias Breuer"^^xsd:string ,
                                                            "Walter Simoncini"^^xsd:string ;
                                          <http://purl.org/vocab/vann/preferredNamespacePrefix> "eucm"^^xsd:string ;
                                          <http://purl.org/vocab/vann/preferredNamespaceUri> "http://w3id.org/um/cbcm/eu-cm-ontology#"^^xsd:string ;
                                          rdf:type <http://purl.org/vocommons/voaf#Vocabulary> ;
                                          rdfs:seeAlso "https://maastrichtu-ids.github.io/cbcm-ontology"^^xsd:anyURI ;
                                          owl:versionInfo "1.2.2"^^xsd:string ;
                                          prov:wasAttributedTo "Institute of Data Science at Maastricht University"^^xsd:string ,
                                                               "Maastricht University"^^xsd:string .

#################################################################
#    Annotation properties
#################################################################

###  http://creativecommons.org/ns#license
<http://creativecommons.org/ns#license> rdf:type owl:AnnotationProperty .


###  http://ontologydesignpatterns.org/opla-sd#entityPosition
opla-sd:entityPosition rdf:type owl:AnnotationProperty .


###  http://ontologydesignpatterns.org/opla-sd#entityPositionX
opla-sd:entityPositionX rdf:type owl:AnnotationProperty .


###  http://ontologydesignpatterns.org/opla-sd#entityPositionY
opla-sd:entityPositionY rdf:type owl:AnnotationProperty .


###  http://purl.org/dc/elements/1.1/creator
dc:creator rdf:type owl:AnnotationProperty .


###  http://purl.org/dc/elements/1.1/description
dc:description rdf:type owl:AnnotationProperty .


###  http://purl.org/dc/elements/1.1/issued
dc:issued rdf:type owl:AnnotationProperty .


###  http://purl.org/dc/elements/1.1/modified
dc:modified rdf:type owl:AnnotationProperty .


###  http://purl.org/dc/elements/1.1/publisher
dc:publisher rdf:type owl:AnnotationProperty .


###  http://purl.org/dc/elements/1.1/rights
dc:rights rdf:type owl:AnnotationProperty .


###  http://purl.org/dc/elements/1.1/title
dc:title rdf:type owl:AnnotationProperty .


###  http://purl.org/dc/terms/contributor
terms:contributor rdf:type owl:AnnotationProperty .


###  http://purl.org/dc/terms/description
terms:description rdf:type owl:AnnotationProperty .


###  http://purl.org/dc/terms/license
terms:license rdf:type owl:AnnotationProperty .


###  http://purl.org/vocab/vann/preferredNamespacePrefix
<http://purl.org/vocab/vann/preferredNamespacePrefix> rdf:type owl:AnnotationProperty .


###  http://purl.org/vocab/vann/preferredNamespaceUri
<http://purl.org/vocab/vann/preferredNamespaceUri> rdf:type owl:AnnotationProperty .


###  http://w3id.org/um/cbcm/eu-cm-ontology#example
cbcm:example rdf:type owl:AnnotationProperty ;
             rdfs:comment "Provides a human-readable written example of the entity in question."@en ;
             rdfs:label "Example"@en ;
             rdfs:subPropertyOf rdfs:comment .


###  http://w3id.org/um/cbcm/eu-cm-ontology#iso2code
cbcm:iso2code rdf:type owl:AnnotationProperty ;
              rdfs:subPropertyOf rdfs:label .


###  http://w3id.org/um/cbcm/eu-cm-ontology#requirement-level
cbcm:requirement-level rdf:type owl:AnnotationProperty ;
                       cbcm:example "Examples include: MUST, SHOULD, RECOMMENDED and OPTIONAL"@en ;
                       rdfs:comment "Specifies a phrase to indicate the degree to which the providing of a value for the entity (e.g. a data or object property) in question is compulsory, recommended or optional."@en ;
                       rdfs:label "Requirement level"@en ;
                       rdfs:subPropertyOf rdfs:comment .


###  http://www.w3.org/1999/02/22-rdf-syntax-ns#type
rdf:type rdf:type owl:AnnotationProperty .


###  http://www.w3.org/2003/06/sw-vocab-status/ns#term_status
<http://www.w3.org/2003/06/sw-vocab-status/ns#term_status> rdf:type owl:AnnotationProperty .


###  http://www.w3.org/ns/prov#wasAttributedTo
prov:wasAttributedTo rdf:type owl:AnnotationProperty .


#################################################################
#    Object Properties
#################################################################

###  http://w3id.org/um/cbcm/eu-cm-ontology#applicableTo
cbcm:applicableTo rdf:type owl:ObjectProperty ;
                  rdfs:subPropertyOf cbcm:cbcmObjectRelation ;
                  rdfs:domain cbcm:TransactionRight ;
                  rdfs:range cbcm:Agent ;
                  cbcm:example "(applicableTo creditorRight1 person1)"@en ;
                  rdfs:comment "(applicableTo ?ENTITY1 ?ENTITY2) means that some legal right ?ENTITY1 is awarded or assigned to a particular person or agent ?ENTITY2."@en ;
                  rdfs:label "applicable to"@en .


###  http://w3id.org/um/cbcm/eu-cm-ontology#authoredBy
cbcm:authoredBy rdf:type owl:ObjectProperty ;
                rdfs:subPropertyOf cbcm:cbcmDocumentRelation ;
                owl:inverseOf cbcm:authors ;
                rdfs:domain cbcm:CompanyMobilityDocument ;
                rdfs:range [ rdf:type owl:Class ;
                             owl:unionOf ( cbcm:Organisation
                                           cbcm:Person
                                         )
                           ] ;
                cbcm:example "(authoredBy independentExpertReport1 independentExpert1)" ;
                rdfs:comment "(authoredBy ?ENTITY1 ?ENTITY2) means that ?ENTITY1 is an instance of a publication that is created primarily by the entity referred to by ?ENTITY2."@en ;
                rdfs:label "authored by"@en ;
                rdfs:seeAlso cbcm:authors .


###  http://w3id.org/um/cbcm/eu-cm-ontology#authors
cbcm:authors rdf:type owl:ObjectProperty ;
             rdfs:subPropertyOf cbcm:cbcmDocumentRelation ;
             rdfs:comment "(authors ?ENTITY1 ?ENTITY2) means that (authoredBy ?ENTITY2 ?ENTITY1)"@en ;
             rdfs:label "authors"@en ;
             rdfs:seeAlso cbcm:authoredBy .


###  http://w3id.org/um/cbcm/eu-cm-ontology#cbcmDataProvenanceRelation
cbcm:cbcmDataProvenanceRelation rdf:type owl:ObjectProperty ;
                                rdfs:subPropertyOf cbcm:cbcmEntityRelation ;
                                rdfs:comment "(cbcmDataProvenanceRelation ?ENTITY1 ?ENTITY2) means that the relation between ?ENTITY1 and ?ENTITY2 captures provenance information for company transaction data."@en ;
                                rdfs:label "Cross-border company mobility data provenance relation"@en .


###  http://w3id.org/um/cbcm/eu-cm-ontology#cbcmDocumentRelation
cbcm:cbcmDocumentRelation rdf:type owl:ObjectProperty ;
                          rdfs:subPropertyOf cbcm:cbcmEntityRelation ;
                          rdfs:comment "(cbcmDocumentRelation ?ENTITY1 ?ENTITY2) means that the relation between ?ENTITY1 and ?ENTITY2 captures information pertaining to a company mobility document or similar information source relevant to corporate mobility."@en ;
                          rdfs:label "Cross-border company mobility document relation"@en ;
                          rdfs:seeAlso cbcm:CompanyMobilityDocument .


###  http://w3id.org/um/cbcm/eu-cm-ontology#cbcmEntityRelation
cbcm:cbcmEntityRelation rdf:type owl:ObjectProperty ;
                        rdfs:comment "(cbcmEntityRelation ?ENTITY1 ?ENTITY2) means that ?ENTITY1 is related to ?ENTITY2."@en ;
                        rdfs:label "Cross-border company mobility entity relation"@en .


###  http://w3id.org/um/cbcm/eu-cm-ontology#cbcmObjectRelation
cbcm:cbcmObjectRelation rdf:type owl:ObjectProperty ;
                        rdfs:subPropertyOf cbcm:cbcmEntityRelation ;
                        rdfs:comment "(cbcmObjectRelation ?ENTITY1 ?ENTITY2) means that the relation between ?ENTITY1 and ?ENTITY2 captures information pertaining to an object."@en ;
                        rdfs:label "Cross-border company mobility object relation"@en .


###  http://w3id.org/um/cbcm/eu-cm-ontology#cbcmOrganisationRelation
cbcm:cbcmOrganisationRelation rdf:type owl:ObjectProperty ;
                              rdfs:subPropertyOf cbcm:cbcmEntityRelation ;
                              rdfs:comment "(cbcmOrganisationRelation ?ENTITY1 ?ENTITY2) means that the relation between ?ENTITY1 and ?ENTITY2 captures information pertaining to an organisation."@en ;
                              rdfs:label "Cross-border company mobility organisation relation"@en ;
                              rdfs:seeAlso cbcm:Organisation .


###  http://w3id.org/um/cbcm/eu-cm-ontology#cbcmTransactionRelation
cbcm:cbcmTransactionRelation rdf:type owl:ObjectProperty ;
                             rdfs:subPropertyOf cbcm:cbcmEntityRelation ;
                             rdfs:comment "(cbcmTransactionRelation ?ENTITY1 ?ENTITY2) means that the relation between ?ENTITY1 and ?ENTITY2 captures information pertaining to a company mobility transaction."@en ;
                             rdfs:label "Cross-border company mobility transaction relation"@en ;
                             rdfs:seeAlso cbcm:CompanyTransaction .


###  http://w3id.org/um/cbcm/eu-cm-ontology#companyFormCountry
cbcm:companyFormCountry rdf:type owl:ObjectProperty ;
                        rdfs:subPropertyOf cbcm:cbcmEntityRelation ;
                        owl:inverseOf cbcm:countryHasCompanyForm ;
                        rdfs:domain cbcm:CompanyLegalForm ;
                        rdfs:range cbcm:Country ;
                        rdfs:comment "(companyFormCountry ?ENTITY1 ?ENTITY2) means that ?ENTITY1 is a company form recognized by the law of country ?ENTITY2."@en ;
                        rdfs:label "Company form country"@en .


###  http://w3id.org/um/cbcm/eu-cm-ontology#containedIn
cbcm:containedIn rdf:type owl:ObjectProperty ;
                 rdfs:subPropertyOf cbcm:cbcmDocumentRelation ;
                 rdfs:domain cbcm:CompanyMobilityDocument ;
                 rdfs:range cbcm:DocumentRepository ;
                 cbcm:example "(containedIn transactionNotice1 nationalRegistry1)"@en ;
                 rdfs:comment "(containedIn ?ENTITY1 ?ENTITY2) means that some document or publication ?ENTITY1 is archived or stored in some other document collection, database or data repository referred to by ?ENTITY2."@en ;
                 rdfs:label "contained in"@en .


###  http://w3id.org/um/cbcm/eu-cm-ontology#countryHasCompanyForm
cbcm:countryHasCompanyForm rdf:type owl:ObjectProperty ;
                           rdfs:subPropertyOf cbcm:cbcmEntityRelation ;
                           rdfs:domain cbcm:Country ;
                           rdfs:range cbcm:CompanyLegalForm ;
                           rdfs:comment "(countryHasCompanyForm ?ENTITY1 ?ENTITY2) means that ?ENTITY1 refers to a country the corporate law in that country permits and / or has occurrences of companies in that country which have the corporate legal structure (company legal form) referred to by ?ENTITY2."@en ;
                           rdfs:label "country has company form"@en .


###  http://w3id.org/um/cbcm/eu-cm-ontology#documentValidatedByDocument
cbcm:documentValidatedByDocument rdf:type owl:ObjectProperty ;
                                 rdfs:subPropertyOf cbcm:cbcmDocumentRelation ;
                                 rdfs:domain cbcm:CompanyMobilityDocument ;
                                 rdfs:range cbcm:CompanyMobilityDocument ;
                                 cbcm:example "(documentValidatedByDocument mergerPlan1 mergerCertificate1)"@en ;
                                 rdfs:comment "(documentValidatedByDocument ?ENTITY1 ?ENTITY2) means that some document or publication, ?ENTITY1, went through a process of approval and assessment through various criteria such as veracity, eligibility, legal relevance etc. and another document ?ENTITY2 was produced to prove the satisfaction of the critieria by ?ENTITY1."@en ;
                                 rdfs:label "document validated by document"@en .


###  http://w3id.org/um/cbcm/eu-cm-ontology#employedBy
cbcm:employedBy rdf:type owl:ObjectProperty ;
                rdfs:subPropertyOf cbcm:hasCompanyStakeholder ;
                owl:inverseOf cbcm:employs ;
                rdfs:domain [ rdf:type owl:Class ;
                              owl:unionOf ( cbcm:Organisation
                                            cbcm:Person
                                          )
                            ] ;
                rdfs:range [ rdf:type owl:Class ;
                             owl:unionOf ( cbcm:Organisation
                                           cbcm:Person
                                         )
                           ] ;
                cbcm:example "(employedBy person1 company1)"@en ;
                rdfs:comment "(employedBy ?ENTITY1 ?ENTITY2) means that some agent (person or organisation) ?ENTITY1 is promised and delivered an incentive (usually financial) to perform some work for ?ENTITY2 where ?ENTITY2 is an organisation. This exchange is usually governed by law and formal regulations in the particular country or social context in which the work is being performed."@en ;
                rdfs:label "employed by"@en .


###  http://w3id.org/um/cbcm/eu-cm-ontology#employs
cbcm:employs rdf:type owl:ObjectProperty ;
             rdfs:subPropertyOf cbcm:hasCompanyStakeholder ;
             rdfs:comment "(employs ?ENTITY1 ?ENTITY2) means (employedBy ?ENTITY2 ?ENTITY1)"@en ;
             rdfs:label "employs"@en ;
             rdfs:seeAlso cbcm:employedBy .


###  http://w3id.org/um/cbcm/eu-cm-ontology#generated
cbcm:generated rdf:type owl:ObjectProperty ;
               rdfs:subPropertyOf cbcm:cbcmDataProvenanceRelation ;
               owl:inverseOf cbcm:wasGeneratedBy ;
               rdfs:comment """Generation is the completion of production of a new entity by a process. This entity did not exist before generation and becomes available for usage after this generation.

Based (inverse of) on: https://www.w3.org/TR/prov-o/#wasGeneratedBy"""@en ;
               rdfs:label "Generated"@en .


###  http://w3id.org/um/cbcm/eu-cm-ontology#hasAcquiringCompany
cbcm:hasAcquiringCompany rdf:type owl:ObjectProperty ;
                         rdfs:subPropertyOf cbcm:hasTransactionResult ;
                         rdfs:domain cbcm:CompanyMerger ;
                         rdfs:range cbcm:Company ;
                         cbcm:example "(hasAcquiringCompany crossBorderMerger1 company1)" ;
                         rdfs:comment "(hasAcquiringCompany ?ENTITY1 ?ENTITY2) means that some company merger transaction ?ENTITY1 produces a new company or alters an existing one (?ENTITY2) such that ?ENTITY2 will acquire (via a universal transfer of assets and liabilities) one or more other companies involved in the process ?ENTITY1."@en ;
                         rdfs:label "has acquiring company"@en ;
                         rdfs:seeAlso cbcm:AcquiringCompany ,
                                      cbcm:CompanyMerger ,
                                      cbcm:MergingCompany .


###  http://w3id.org/um/cbcm/eu-cm-ontology#hasCompanyForm
cbcm:hasCompanyForm rdf:type owl:ObjectProperty ;
                    rdfs:subPropertyOf cbcm:cbcmOrganisationRelation ;
                    rdfs:domain cbcm:Company ;
                    rdfs:range cbcm:CompanyLegalForm ;
                    rdfs:comment "Company legal form. Name given to describe the structure of a corporation or buiness in the different legal orders. For example Limited (Ltd.), Public Limited Company (PLC), Gesellschaft mit beschränkter Haftung (GmbH), Aktiengesellschaft (AG). The company legal form is regulated under national law and grants specific rights and obligations to the company stakeholders (such as shareholders, management & employees)."@en ;
                    rdfs:label "Company Form"@en .


###  http://w3id.org/um/cbcm/eu-cm-ontology#hasCompanyStakeholder
cbcm:hasCompanyStakeholder rdf:type owl:ObjectProperty ;
                           rdfs:subPropertyOf cbcm:cbcmOrganisationRelation ;
                           rdfs:range cbcm:Agent ;
                           cbcm:example "(hasCompanyStakeholder company1 person1)"@en ;
                           rdfs:comment "(hasCompanyStakeholder ?ENTITY1 ?ENTITY2) means that some entity ?ENTITY1, which is either a significant process or agent has another agent ?ENTITY2 with personal interests in benefiting either financially or otherwise from the outcomes of ?ENTITY1 (if it is an event or process), or in its byproducts and profits (if it is an agent)."@en ;
                           rdfs:label "has company stakeholder"@en .


###  http://w3id.org/um/cbcm/eu-cm-ontology#hasDataProvenanceDocumentSource
cbcm:hasDataProvenanceDocumentSource rdf:type owl:ObjectProperty ;
                                     rdfs:subPropertyOf cbcm:cbcmEntityRelation ;
                                     rdfs:domain cbcm:CompanyTransaction ;
                                     rdfs:range cbcm:CompanyMobilityDocument ;
                                     rdfs:comment "In which document did the researcher find information about the transaction?"@en ;
                                     rdfs:label "has document source"@en .


###  http://w3id.org/um/cbcm/eu-cm-ontology#hasDataProvenanceRegistryCountry
cbcm:hasDataProvenanceRegistryCountry rdf:type owl:ObjectProperty ;
                                      rdfs:subPropertyOf cbcm:cbcmEntityRelation ;
                                      rdfs:domain cbcm:CompanyTransaction ;
                                      rdfs:range cbcm:Country ;
                                      rdfs:comment "In which countries' registry did the researcher find information about the transaction?"@en ;
                                      rdfs:label "data found in registry from country"@en .


###  http://w3id.org/um/cbcm/eu-cm-ontology#hasMember
cbcm:hasMember rdf:type owl:ObjectProperty ;
               rdfs:subPropertyOf cbcm:hasCompanyStakeholder ;
               rdfs:domain cbcm:Organisation ;
               rdfs:range cbcm:Person ;
               cbcm:example "(hasMember worksCouncil1 employee1)"@en ;
               rdfs:comment "(hasMember ?ENTITY1 ?ENTITY2) means that some agent ?ENTITY1 (usually an organisation) has a person ?ENTITY2 that participates in its activities. This need not represent an employment role nor imply financial incentives between the organisation and person."@en ;
               rdfs:label "has member"@en ;
               rdfs:seeAlso cbcm:employs .


###  http://w3id.org/um/cbcm/eu-cm-ontology#hasMergingCompany
cbcm:hasMergingCompany rdf:type owl:ObjectProperty ;
                       rdfs:subPropertyOf cbcm:hasTransactionInput ;
                       rdfs:domain cbcm:CompanyMerger ;
                       rdfs:range cbcm:Company ;
                       cbcm:example "(hasMergingCompany crossBorderMerger1 company1)" ;
                       rdfs:comment "(hasMergingCompany ?ENTITY1 ?ENTITY2) means that some company merger transaction ?ENTITY1 involves a company ?ENTITY2 which will be dissolved during the process of ?ENTITY1 and will be acquired (via a universal transfer of assets and liabilities) by another distinct company involved in ?ENTITY1."@en ;
                       rdfs:label "has merging company"@en ;
                       rdfs:seeAlso cbcm:AcquiringCompany ,
                                    cbcm:CompanyMerger ,
                                    cbcm:MergingCompany .


###  http://w3id.org/um/cbcm/eu-cm-ontology#hasOriginalCompany
cbcm:hasOriginalCompany rdf:type owl:ObjectProperty ;
                        rdfs:subPropertyOf cbcm:hasTransactionInput ;
                        rdfs:domain cbcm:CompanyDivision ;
                        rdfs:range cbcm:Company ;
                        cbcm:example "(hasOriginalCompany crossBorderDivision1 company1)" ;
                        rdfs:comment "(hasOriginalCompany ?ENTITY1 ?ENTITY2) means that some company division transaction ?ENTITY1 involves a company ?ENTITY2 which will be divided (or \"split\") into multiple recipient or emerging companies."@en ;
                        rdfs:label "has original company"@en ;
                        rdfs:seeAlso cbcm:CompanyDivision ,
                                     cbcm:EmergingCompany ,
                                     cbcm:OriginalCompany ,
                                     cbcm:RecipientCompany .


###  http://w3id.org/um/cbcm/eu-cm-ontology#hasParentCompany
cbcm:hasParentCompany rdf:type owl:ObjectProperty ;
                      rdfs:subPropertyOf cbcm:cbcmOrganisationRelation ;
                      owl:inverseOf cbcm:hasSubsidiaryCompany ;
                      rdfs:domain cbcm:Company ;
                      rdfs:range cbcm:Company ;
                      cbcm:example "(hasParentCompany company1 company2)"@en ;
                      rdfs:comment "(hasParentCompany ?ENTITY1 ?ENTITY2) means that some company ?ENTITY1 is owned and under direct or indirect control by the company ?ENTITY2."@en ;
                      rdfs:label "has parent company"@en ;
                      rdfs:seeAlso cbcm:hasSubsidiaryCompany .


###  http://w3id.org/um/cbcm/eu-cm-ontology#hasPart
cbcm:hasPart rdf:type owl:ObjectProperty ;
             rdfs:subPropertyOf cbcm:cbcmEntityRelation ;
             owl:inverseOf cbcm:partOf ;
             rdfs:comment "(hasPart ?ENTITY1 ?ENTITY2) means that the entity referred to by ?ENTITY1 has a constituent entity referred to by ?ENTITY2."@en ;
             rdfs:label "has part"@en ;
             rdfs:seeAlso cbcm:partOf .


###  http://w3id.org/um/cbcm/eu-cm-ontology#hasPostCompanyForm
cbcm:hasPostCompanyForm rdf:type owl:ObjectProperty ;
                        rdfs:subPropertyOf cbcm:hasTransactionResult ;
                        rdfs:domain cbcm:CompanyTransaction ;
                        rdfs:range cbcm:CompanyLegalForm ;
                        rdfs:comment "(?ENTITY1 hasPostCompanyForm ?ENTITY2) indicates the new company form of a company undergoing a cross border conversion or a national conversion."@en ;
                        rdfs:label "After-transaction company form"@en ;
                        rdfs:seeAlso cbcm:CompanyConversion .


###  http://w3id.org/um/cbcm/eu-cm-ontology#hasPrimaryRegistrationLocation
cbcm:hasPrimaryRegistrationLocation rdf:type owl:ObjectProperty ;
                                    rdfs:subPropertyOf cbcm:locatedIn ;
                                    rdfs:domain cbcm:Company ;
                                    rdfs:range cbcm:Country ;
                                    rdfs:comment "Primary country of registration (location) of a company as a full country name"@en ;
                                    rdfs:label "Company primary registration location"@en .


###  http://w3id.org/um/cbcm/eu-cm-ontology#hasPriorCompanyForm
cbcm:hasPriorCompanyForm rdf:type owl:ObjectProperty ;
                         rdfs:subPropertyOf cbcm:hasTransactionInput ;
                         rdfs:domain cbcm:CompanyTransaction ;
                         rdfs:range cbcm:CompanyLegalForm ;
                         rdfs:comment "(?ENTITY1 hasPriorCompanyForm ?ENTITY2) indicates the original company form of a company undergoing a cross border conversion or a national conversion."@en ;
                         rdfs:label "Pre-transaction company form"@en ;
                         rdfs:seeAlso cbcm:CompanyConversion .


###  http://w3id.org/um/cbcm/eu-cm-ontology#hasRecipientCompany
cbcm:hasRecipientCompany rdf:type owl:ObjectProperty ;
                         rdfs:subPropertyOf cbcm:hasTransactionResult ;
                         rdfs:domain cbcm:CompanyDivision ;
                         rdfs:range cbcm:Company ;
                         cbcm:example "(hasMergingCompany crossBorderMerger1 company1)" ;
                         rdfs:comment "(hasRecipientCompany ?ENTITY1 ?ENTITY2) means that some company division transaction ?ENTITY1 produces two or more distinct companies, one of which is ?ENTITY2 (a so-called \"recipient company\")."@en ;
                         rdfs:label "has recipient company"@en ;
                         rdfs:seeAlso cbcm:AcquiringCompany ,
                                      cbcm:CompanyMerger ,
                                      cbcm:MergingCompany .


###  http://w3id.org/um/cbcm/eu-cm-ontology#hasSecondaryRegistrationLocation
cbcm:hasSecondaryRegistrationLocation rdf:type owl:ObjectProperty ;
                                      rdfs:subPropertyOf cbcm:locatedIn ;
                                      rdfs:domain cbcm:Company ;
                                      rdfs:range cbcm:Country ;
                                      rdfs:comment "Country of secondary registration (location) of a company"@en ;
                                      rdfs:label "Company secondary registration location"@en .


###  http://w3id.org/um/cbcm/eu-cm-ontology#hasSubProcedure
cbcm:hasSubProcedure rdf:type owl:ObjectProperty ;
                     rdfs:subPropertyOf cbcm:cbcmTransactionRelation ;
                     rdfs:domain cbcm:CompanyTransaction ;
                     cbcm:example "(hasSubProcedure seatTransfer1 changeOfCompanyAddress1)" ;
                     rdfs:comment "(hasSubProcedure ?ENTITY1 ?ENTITY2) means that some process ?ENTITY1 contains another (shorter) process ?ENTITY2 that should be completed before ?ENTITY1 can complete."@en ;
                     rdfs:label "has sub procedure"@en .


###  http://w3id.org/um/cbcm/eu-cm-ontology#hasSubsidiaryCompany
cbcm:hasSubsidiaryCompany rdf:type owl:ObjectProperty ;
                          rdfs:subPropertyOf cbcm:cbcmOrganisationRelation ;
                          rdfs:comment "(hasSubsidiaryCompany ?ENTITY1 ?ENTITY2) means (hasParentCompany ?ENTITY2 ?ENTITY1)"@en ;
                          rdfs:label "has subsidiary company"@en ;
                          rdfs:seeAlso cbcm:hasParentCompany .


###  http://w3id.org/um/cbcm/eu-cm-ontology#hasTransactionInput
cbcm:hasTransactionInput rdf:type owl:ObjectProperty ;
                         rdfs:subPropertyOf cbcm:cbcmTransactionRelation ;
                         owl:inverseOf cbcm:isTransactionInputOf ;
                         rdfs:domain cbcm:CompanyTransaction ;
                         rdfs:range cbcm:Company ;
                         cbcm:example "(hasTransactionInput crossBorderMerger1 company1)" ;
                         rdfs:comment "(hasTransactionInput ?ENTITY1 ?ENTITY2) means that some company transaction ?ENTITY1 has a prerequisite entity ?ENTITY2 that needs to be considered, assessed, or modified during the transaction referred to by ?ENTITY1."@en ;
                         rdfs:label "has transaction input"@en ;
                         rdfs:seeAlso cbcm:CompanyTransaction .


###  http://w3id.org/um/cbcm/eu-cm-ontology#hasTransactionResult
cbcm:hasTransactionResult rdf:type owl:ObjectProperty ;
                          rdfs:subPropertyOf cbcm:cbcmTransactionRelation ;
                          owl:inverseOf cbcm:isTransactionResultOf ;
                          rdfs:domain cbcm:CompanyTransaction ;
                          rdfs:range cbcm:Company ;
                          cbcm:example "(hasTransactionResult crossBorderMerger1 acquiringCompany1)" ,
                                       "(hasTransactionResult crossBorderMerger1 mergerCertificate1)" ;
                          rdfs:comment "(hasTransactionResult ?ENTITY1 ?ENTITY2) means that some company transaction ?ENTITY1 has a byproduct ?ENTITY2 (e.g. a company, transaction certificate etc.) after completion of the process."@en ;
                          rdfs:label "has transaction result"@en ;
                          rdfs:seeAlso cbcm:CompanyTransaction .


###  http://w3id.org/um/cbcm/eu-cm-ontology#involvesChangeOf
cbcm:involvesChangeOf rdf:type owl:ObjectProperty ;
                      rdfs:subPropertyOf cbcm:cbcmEntityRelation ;
                      cbcm:example "(involvesChangeOf seatTransfer1 businessAddress1)"@en ;
                      rdfs:comment "(involvesChangeOf ?ENTITY1 ?ENTITY2) means that the process ?ENTITY1 requires the modification or alteration of the entity or object ?ENTITY2."@en ;
                      rdfs:label "involves the change of"@en .


###  http://w3id.org/um/cbcm/eu-cm-ontology#involvesCountry
cbcm:involvesCountry rdf:type owl:ObjectProperty ;
                     rdfs:subPropertyOf cbcm:cbcmTransactionRelation ;
                     rdfs:domain cbcm:CompanyTransaction ;
                     rdfs:range cbcm:Country ;
                     cbcm:example "(involvesCountry crossBorderMerger1 france)" ;
                     rdfs:comment "(involvesCountry ?ENTITY1 ?ENTITY2) means that some company transaction ?ENTITY1 includes the modification of a company whose place of business is located in the country referred to by ?ENTITY2"@en ;
                     rdfs:label "involves country"@en ;
                     rdfs:seeAlso cbcm:Company ,
                                  cbcm:Country .


###  http://w3id.org/um/cbcm/eu-cm-ontology#isTransactionInputOf
cbcm:isTransactionInputOf rdf:type owl:ObjectProperty ;
                          rdfs:subPropertyOf cbcm:cbcmTransactionRelation ;
                          cbcm:example cbcm:hasTransactionInput ;
                          rdfs:comment "(isTransactionInputOf ?ENTITY1 ?ENTITY2) means (hasTransactionInput ?ENTITY2 ?ENTITY1)"@en ;
                          rdfs:label "is transaction input of"@en .


###  http://w3id.org/um/cbcm/eu-cm-ontology#isTransactionResultOf
cbcm:isTransactionResultOf rdf:type owl:ObjectProperty ;
                           rdfs:subPropertyOf cbcm:cbcmTransactionRelation ;
                           cbcm:example cbcm:hasTransactionResult ;
                           rdfs:comment "(isTransactionResultOf ?ENTITY1 ?ENTITY2) means (hasTransactionResult ?ENTITY2 ?ENTITY1)"@en ;
                           rdfs:label "is transaction result of"@en .


###  http://w3id.org/um/cbcm/eu-cm-ontology#issuedByOrganisation
cbcm:issuedByOrganisation rdf:type owl:ObjectProperty ;
                          rdfs:subPropertyOf cbcm:cbcmDocumentRelation ;
                          rdfs:domain cbcm:CompanyMobilityDocument ;
                          rdfs:range cbcm:Organisation ;
                          cbcm:example "(issuedByOrganisation document1 organisation1)"@en ;
                          rdfs:comment "(issuedByOrganisation ?ENTITY1 ?ENTITY2) means that some document or publication, ?ENTITY1, was created (and possibly delivered or administered to another entity) by some entity ?ENTITY2."@en ;
                          rdfs:label "issued by organisation"@en .


###  http://w3id.org/um/cbcm/eu-cm-ontology#locatedIn
cbcm:locatedIn rdf:type owl:ObjectProperty ;
               rdfs:subPropertyOf cbcm:cbcmOrganisationRelation ;
               rdfs:comment "(locatedIn ?ENTITY1 ?ENTITY2) means that some entity ?ENTITY1 occupies the spatial region referred to by ?ENTITY2."@en ;
               rdfs:label "located in"@en .


###  http://w3id.org/um/cbcm/eu-cm-ontology#maintainedBy
cbcm:maintainedBy rdf:type owl:ObjectProperty ;
                  rdfs:subPropertyOf cbcm:cbcmDocumentRelation ;
                  owl:inverseOf cbcm:maintains ;
                  cbcm:example "(maintainedBy officialJournalRepository1 officialJournalAdministration1)"@en ;
                  rdfs:comment "(maintainedBy ?ENTITY1 ?ENTITY2) means that some digital resource ?ENTITY1 (e.g. database, website, document repository etc.) has stewardship by some agent or organisation ?ENTITY2 who is responsible for the upkeep of ?ENTITY1."@en ;
                  rdfs:label "maintained by"@en .


###  http://w3id.org/um/cbcm/eu-cm-ontology#maintains
cbcm:maintains rdf:type owl:ObjectProperty ;
               rdfs:subPropertyOf cbcm:cbcmDocumentRelation ;
               rdfs:comment "(maintains ?ENTITY1 ?ENTITY2) means (maintainedBy ?ENTITY2 ?ENTITY1)"@en ;
               rdfs:label "maintains"@en ;
               rdfs:seeAlso cbcm:maintainedBy .


###  http://w3id.org/um/cbcm/eu-cm-ontology#ownedBy
cbcm:ownedBy rdf:type owl:ObjectProperty ;
             rdfs:subPropertyOf cbcm:hasCompanyStakeholder ;
             owl:inverseOf cbcm:owns ;
             cbcm:example "(ownedBy company1 company2)"@en ;
             rdfs:comment "(ownedBy ?ENTITY1 ?ENTITY2) means that some agent ?ENTITY2 has proprietorship over another object or organisational agent ?ENTITY1."@en ;
             rdfs:label "owned by"@en ;
             rdfs:seeAlso cbcm:owns .


###  http://w3id.org/um/cbcm/eu-cm-ontology#owns
cbcm:owns rdf:type owl:ObjectProperty ;
          rdfs:subPropertyOf cbcm:hasCompanyStakeholder ;
          rdfs:domain [ rdf:type owl:Class ;
                        owl:unionOf ( cbcm:Organisation
                                      cbcm:Person
                                    )
                      ] ;
          rdfs:range cbcm:Organisation ;
          rdfs:comment "(owns ?ENTITY1 ?ENTITY2) means (owns ?ENTITY2 ?ENTITY1)"@en ;
          rdfs:label "owns"@en ;
          rdfs:seeAlso cbcm:ownedBy .


###  http://w3id.org/um/cbcm/eu-cm-ontology#partOf
cbcm:partOf rdf:type owl:ObjectProperty ;
            rdfs:subPropertyOf cbcm:cbcmEntityRelation ;
            rdfs:comment "(partOf ?ENTITY1 ?ENTITY2) means (hasPart ?ENTITY2 ?ENTITY1)"@en ;
            rdfs:label "part of"@en ;
            rdfs:seeAlso cbcm:hasPart .


###  http://w3id.org/um/cbcm/eu-cm-ontology#reportedIn
cbcm:reportedIn rdf:type owl:ObjectProperty ;
                rdfs:subPropertyOf cbcm:cbcmDocumentRelation ;
                rdfs:domain cbcm:CompanyTransaction ;
                rdfs:range cbcm:TransactionNotice ;
                cbcm:example "(reportedIn crossBorderMerger1 transactionNotice1)"@en ;
                rdfs:comment "(reportedIn ?ENTITY1 ?ENTITY2) means that some significant event, process or statement ?ENTITY1 is published or mentioned or declared in writing in some publication, document or database ?ENTITY2."@en ;
                rdfs:label "reported in"@en .


###  http://w3id.org/um/cbcm/eu-cm-ontology#requiresDocument
cbcm:requiresDocument rdf:type owl:ObjectProperty ;
                      rdfs:subPropertyOf cbcm:cbcmDocumentRelation ;
                      rdfs:domain cbcm:CompanyTransaction ;
                      rdfs:range cbcm:CompanyMobilityDocument ;
                      cbcm:example "(requiresDocument crossBorderMerger1 mergerPlan1)"@en ;
                      rdfs:comment "(requiresDocument ?ENTITY1 ?ENTITY2) means that some significant event or process ?ENTITY1 needs a compulsory document ?ENTITY2 to be submitted and reviewed before the process ?ENTITY1 can be completed."@en ;
                      rdfs:label "requires document"@en .


###  http://w3id.org/um/cbcm/eu-cm-ontology#sourceCountry
cbcm:sourceCountry rdf:type owl:ObjectProperty ;
                   rdfs:subPropertyOf cbcm:involvesCountry ;
                   cbcm:example "(sourceCountry crossBorderMerger1 france)" ;
                   rdfs:comment "(sourceCountry ?ENTITY1 ?ENTITY2) means that some company transaction ?ENTITY1 has some transaction input (a company) whose place of business is located in the country ?ENTITY2."@en ;
                   rdfs:label "source country"@en ;
                   rdfs:seeAlso cbcm:Country ,
                                cbcm:hasTransactionInput .


###  http://w3id.org/um/cbcm/eu-cm-ontology#targetCountry
cbcm:targetCountry rdf:type owl:ObjectProperty ;
                   rdfs:subPropertyOf cbcm:involvesCountry ;
                   cbcm:example "(targetCountry crossBorderMerger1 belgium)" ;
                   rdfs:comment "(targetCountry ?ENTITY1 ?ENTITY2) means that some company transaction ?ENTITY1 has some transaction result (a company) whose place of business is located in the country ?ENTITY2."@en ;
                   rdfs:label "target country"@en ;
                   rdfs:seeAlso cbcm:Country ,
                                cbcm:hasTransactionResult .


###  http://w3id.org/um/cbcm/eu-cm-ontology#transactionValidatedByDocument
cbcm:transactionValidatedByDocument rdf:type owl:ObjectProperty ;
                                    rdfs:subPropertyOf cbcm:cbcmDocumentRelation ;
                                    rdfs:domain cbcm:CompanyTransaction ;
                                    rdfs:range cbcm:CompanyMobilityDocument ;
                                    cbcm:example "(transactionValidatedByDocument crossBorderMerger1 mergerCertificate1)"@en ;
                                    rdfs:comment "(transactionValidatedByDocument ?ENTITY1 ?ENTITY2) means that some company transaction ?ENTITY1 went through a process of approval and assessment through various criteria such as veracity, eligibility, legal relevance etc. and a document ?ENTITY2 was produced to prove the satisfaction of the critieria by ?ENTITY1."@en ;
                                    rdfs:label "transaction validated by document"@en ;
                                    rdfs:seeAlso cbcm:CompanyMobilityDocument ,
                                                 cbcm:CompanyTransaction .


###  http://w3id.org/um/cbcm/eu-cm-ontology#typeOfSE
cbcm:typeOfSE rdf:type owl:ObjectProperty ;
              rdfs:subPropertyOf cbcm:cbcmTransactionRelation ;
              rdfs:domain cbcm:CompanyTransaction ;
              rdfs:range cbcm:SEType ;
              rdfs:comment "Variable indicating the SE-establishment mode: by merger, conversion, holding-SE, subsidiary-SE or unsure"@en ;
              rdfs:label "Type of SE"@en .


###  http://w3id.org/um/cbcm/eu-cm-ontology#used
cbcm:used rdf:type owl:ObjectProperty ;
          rdfs:subPropertyOf cbcm:cbcmDataProvenanceRelation ;
          rdfs:comment """Usage is the beginning of utilizing an entity by an activity. Before usage, the activity had not begun to utilize this entity and could not have been affected by the entity.

Based on: https://www.w3.org/TR/prov-o/#used"""@en ;
          rdfs:label "Used"@en .


###  http://w3id.org/um/cbcm/eu-cm-ontology#usedDataProvenanceDocumentSource
cbcm:usedDataProvenanceDocumentSource rdf:type owl:ObjectProperty ;
                                      rdfs:subPropertyOf cbcm:used ;
                                      rdfs:domain cbcm:CompanyTransaction ;
                                      rdfs:range cbcm:CompanyMobilityDocument ;
                                      rdfs:comment "In which document did the researcher find information about the transaction?"@en ;
                                      rdfs:label "Has document source"@en .


###  http://w3id.org/um/cbcm/eu-cm-ontology#usedDataProvenanceRegistryCountry
cbcm:usedDataProvenanceRegistryCountry rdf:type owl:ObjectProperty ;
                                       rdfs:subPropertyOf cbcm:used ;
                                       rdfs:domain cbcm:CompanyTransaction ;
                                       rdfs:range cbcm:Country ;
                                       rdfs:comment "In which countries' registry did the researcher find information about the transaction?"@en ;
                                       rdfs:label "Data found in registry from country"@en .


###  http://w3id.org/um/cbcm/eu-cm-ontology#wasAssociatedWith
cbcm:wasAssociatedWith rdf:type owl:ObjectProperty ;
                       rdfs:subPropertyOf cbcm:cbcmDataProvenanceRelation ;
                       rdfs:range cbcm:Agent ;
                       rdfs:comment """An activity association is an assignment of responsibility to an agent for a process, indicating that the agent had a role in the activity.

Based on: https://www.w3.org/TR/prov-o/#wasAssociatedWith"""@en ;
                       rdfs:label "Associated with"@en .


###  http://w3id.org/um/cbcm/eu-cm-ontology#wasGeneratedBy
cbcm:wasGeneratedBy rdf:type owl:ObjectProperty ;
                    rdfs:subPropertyOf cbcm:cbcmDataProvenanceRelation ;
                    rdfs:comment """Generation is the completion of production of a new entity by a process. This entity did not exist before generation and becomes available for usage after this generation.

Based on: https://www.w3.org/TR/prov-o/#wasGeneratedBy"""@en ;
                    rdfs:label "Generated by"@en .


#################################################################
#    Data properties
#################################################################

###  http://w3id.org/um/cbcm/eu-cm-ontology#acEmploymentFigureAtTransaction
cbcm:acEmploymentFigureAtTransaction rdf:type owl:DatatypeProperty ;
                                     rdfs:domain cbcm:CompanyTransaction ;
                                     rdfs:range xsd:nonNegativeInteger ;
                                     rdfs:comment "number of employees of the acquiring company - at the moment of the transaction"@en ;
                                     rdfs:label "AC Employees count at transaction"@en .


###  http://w3id.org/um/cbcm/eu-cm-ontology#acLastEmploymentFigure
cbcm:acLastEmploymentFigure rdf:type owl:DatatypeProperty ;
                            rdfs:domain cbcm:CompanyTransaction ;
                            rdfs:range xsd:nonNegativeInteger ;
                            rdfs:comment "The last available annual employment figure for the acquiring company"@en ;
                            rdfs:label "Last employment figure for the acquiring company"@en .


###  http://w3id.org/um/cbcm/eu-cm-ontology#acTotalEUEmploymentFigure
cbcm:acTotalEUEmploymentFigure rdf:type owl:DatatypeProperty ;
                               rdfs:domain cbcm:CompanyTransaction ;
                               rdfs:range xsd:nonNegativeInteger ;
                               rdfs:comment "total number of employees of the acquiring company in the EU at the moment of the transaction"@en ;
                               rdfs:label "Total EU employees"@en .


###  http://w3id.org/um/cbcm/eu-cm-ontology#acYearEmploymentFigure
cbcm:acYearEmploymentFigure rdf:type owl:DatatypeProperty ;
                            rdfs:domain cbcm:CompanyTransaction ;
                            rdfs:range xsd:dateTime ;
                            rdfs:comment "The year the last annual employment figure was obtained for acquiring companies"@en ;
                            rdfs:label "AC Last employment figure year"@en .


###  http://w3id.org/um/cbcm/eu-cm-ontology#bler
cbcm:bler rdf:type owl:DatatypeProperty ;
          rdfs:domain cbcm:CompanyTransaction ;
          rdfs:range xsd:boolean ;
          rdfs:comment """Is an employee board level representation/participation (BLER) mechanism applicable prior to the cross-border transaction?

0 = no BLER prior to cross-border transaction
1 = BLER existing prior to cross-border transaction"""@en ;
          rdfs:label "is BLER existing prior"@en ;
          rdfs:seeAlso cbcm:BoardLevelEmployeeRepresentationRight .


###  http://w3id.org/um/cbcm/eu-cm-ontology#blerComposition
cbcm:blerComposition rdf:type owl:DatatypeProperty ;
                     rdfs:domain cbcm:CompanyTransaction ;
                     rdfs:range [ rdf:type rdfs:Datatype ;
                                  owl:onDatatype xsd:float ;
                                  owl:withRestrictions ( [ xsd:minInclusive "0.0"^^xsd:float
                                                         ]
                                                         [ xsd:maxInclusive "1.0"^^xsd:float
                                                         ]
                                                       )
                                ] ;
                     rdfs:comment """What is the employee board level representation (BLER) ratio going to be after the completion of the transaction?

The ratio is ranging from 0.00 (no BLER) to 0.33 (1/3 BLER) to 0.5 (50-50 Mitbestimmung) to (theoretically) 1.00, which would be 100% employee representatives on the board and no shareholder representatives."""@en ;
                     rdfs:label "BLER composition"@en .


###  http://w3id.org/um/cbcm/eu-cm-ontology#companiesHaveEconomicCommittee
cbcm:companiesHaveEconomicCommittee rdf:type owl:DatatypeProperty ;
                                    rdfs:domain cbcm:CompanyTransaction ;
                                    rdfs:range xsd:boolean ;
                                    rdfs:comment """Are the companies involved in the transaction having an economic committee?

An economic committee advises the work council about the financial parts of the transaction."""@en ;
                                    rdfs:label "Companies have Economic Committee"@en .


###  http://w3id.org/um/cbcm/eu-cm-ontology#companiesHaveEmployees
cbcm:companiesHaveEmployees rdf:type owl:DatatypeProperty ;
                            rdfs:domain cbcm:CompanyTransaction ;
                            rdfs:range xsd:boolean ;
                            rdfs:comment "Are the companies involved in the transaction having employees? Only one company needs to have employees for this property to be true"@en ;
                            rdfs:label "Companies have employees"@en .


###  http://w3id.org/um/cbcm/eu-cm-ontology#companiesHaveWorksCouncil
cbcm:companiesHaveWorksCouncil rdf:type owl:DatatypeProperty ;
                               rdfs:domain cbcm:CompanyTransaction ;
                               rdfs:range xsd:boolean ;
                               rdfs:comment "Are the companies involved in the transaction having a works council? Works councils safeguard employees' welfare"@en ;
                               rdfs:label "Companies have Works Council"@en .


###  http://w3id.org/um/cbcm/eu-cm-ontology#divergingEmploymentFigure
cbcm:divergingEmploymentFigure rdf:type owl:DatatypeProperty ;
                               rdfs:domain cbcm:CompanyTransaction ;
                               rdfs:range xsd:nonNegativeInteger ;
                               rdfs:comment "If a different employee number for the acquiring company is found, it is recorded in this field"@en ;
                               rdfs:label "Diverging employment figure"@en .


###  http://w3id.org/um/cbcm/eu-cm-ontology#endedAtTime
cbcm:endedAtTime rdf:type owl:DatatypeProperty ;
                 rdfs:range xsd:dateTime ;
                 rdfs:comment "The date and time a process ended"@en ;
                 rdfs:label "Ended at"@en .


###  http://w3id.org/um/cbcm/eu-cm-ontology#ewc
cbcm:ewc rdf:type owl:DatatypeProperty ;
         rdfs:domain cbcm:Company ;
         rdfs:range xsd:boolean ;
         rdfs:comment "Is the company having a European Works Council (EWC)?"@en ;
         rdfs:label "Has EWC"@en .


###  http://w3id.org/um/cbcm/eu-cm-ontology#impactOnEmployees
cbcm:impactOnEmployees rdf:type owl:DatatypeProperty ;
                       rdfs:domain cbcm:CompanyTransaction ;
                       rdfs:range xsd:string ;
                       rdfs:comment """Is the impact on employees of the envisaged transaction specified in the transaction document (e.g. the merger plan)?

Part of merger plan that specifies how the transaction will affect employees.

- Yes: there is an impact on employees (positive or negative);
- No: no impact on employees;
- Not applicable: the conditions are not met (e.g. no employees, BLER threshold not met) for this criterion to be applicable;
- Unclear: the wording of the document is unclear with regard to the impact/effect/measures taken;
- Not mentioned: given the parameters, this aspect should be addressed in the transaction document, but is not mentioned"""@en ;
                       rdfs:label "Impact on employees"@en .


###  http://w3id.org/um/cbcm/eu-cm-ontology#isListed
cbcm:isListed rdf:type owl:DatatypeProperty ;
              rdfs:domain cbcm:Company ;
              rdfs:range xsd:boolean ;
              rdfs:comment "Whether the company is publicly listed. A company whose shares are bought and sold on a particular stock market."@en ;
              rdfs:label "Is listed"@en .


###  http://w3id.org/um/cbcm/eu-cm-ontology#isSECreation
cbcm:isSECreation rdf:type owl:DatatypeProperty ;
                  rdfs:domain cbcm:CompanyTransaction ;
                  rdfs:range xsd:boolean ;
                  rdfs:comment "Variable indicating whether this case concerns an SE-creation (yes/no) to distinguish creations of SEs from other transactions"@en ;
                  rdfs:label "Is SE creation"@en .


###  http://w3id.org/um/cbcm/eu-cm-ontology#lastWWEmploymentFigure
cbcm:lastWWEmploymentFigure rdf:type owl:DatatypeProperty ;
                            rdfs:domain cbcm:Company ;
                            rdfs:range xsd:nonNegativeInteger ;
                            rdfs:comment "Last available employment figure for the total worldwide employees"@en ;
                            rdfs:label "Last WW employment figure"@en .


###  http://w3id.org/um/cbcm/eu-cm-ontology#lawfirm
cbcm:lawfirm rdf:type owl:DatatypeProperty ;
             rdfs:domain cbcm:CompanyTransaction ;
             rdfs:range xsd:string ;
             rdfs:comment "Name of the lawfirm involved in the transaction, if available (for internal use; cross-border divisions and seat transfers are currently not possible within an EU legal framework.)"@en ;
             rdfs:label "Law Firm"@en .


###  http://w3id.org/um/cbcm/eu-cm-ontology#legalFormAcronym
cbcm:legalFormAcronym rdf:type owl:DatatypeProperty ;
                      rdfs:domain cbcm:CompanyLegalForm ;
                      rdfs:range xsd:string ;
                      rdfs:comment "The acronym of a company legal form"@en ;
                      rdfs:label "Legal form acronym"@en .


###  http://w3id.org/um/cbcm/eu-cm-ontology#mcEmploymentFigureAtTransaction
cbcm:mcEmploymentFigureAtTransaction rdf:type owl:DatatypeProperty ;
                                     rdfs:domain cbcm:CompanyTransaction ;
                                     rdfs:range xsd:nonNegativeInteger ;
                                     rdfs:comment "Number of employees of the acquiring company - at the moment of the transaction"@en ;
                                     rdfs:label "MC Employees count at transaction"@en .


###  http://w3id.org/um/cbcm/eu-cm-ontology#mcLastEmploymentFigure
cbcm:mcLastEmploymentFigure rdf:type owl:DatatypeProperty ;
                            rdfs:domain cbcm:CompanyTransaction ;
                            rdfs:range xsd:nonNegativeInteger ;
                            rdfs:comment "The last available annual employment figure for the merging company"@en ;
                            rdfs:label "Last employment figure for the merging company"@en .


###  http://w3id.org/um/cbcm/eu-cm-ontology#mcYearEmploymentFigure
cbcm:mcYearEmploymentFigure rdf:type owl:DatatypeProperty ;
                            rdfs:domain cbcm:CompanyTransaction ;
                            rdfs:range xsd:dateTime ;
                            rdfs:comment "The year the last annual employment figure was obtained for merging companies"@en ;
                            rdfs:label "MC Last employment figure year"@en .


###  http://w3id.org/um/cbcm/eu-cm-ontology#multiCBM
cbcm:multiCBM rdf:type owl:DatatypeProperty ;
              rdfs:domain cbcm:CompanyTransaction ;
              rdfs:range xsd:boolean ;
              rdfs:comment "A transaction whereby more than two companies (i.e. multiple merging companies) are involved and merged into one acquiring company"@en ;
              rdfs:label "Multi-transaction"@en .


###  http://w3id.org/um/cbcm/eu-cm-ontology#naceCode
cbcm:naceCode rdf:type owl:DatatypeProperty ;
              rdfs:domain cbcm:Company ;
              rdfs:range [ rdf:type rdfs:Datatype ;
                           owl:onDatatype xsd:positiveInteger ;
                           owl:withRestrictions ( [ xsd:minInclusive "1000"^^xsd:positiveInteger
                                                  ]
                                                  [ xsd:maxInclusive "9999"^^xsd:positiveInteger
                                                  ]
                                                )
                         ] ;
              rdfs:comment "NACE Classification Code for companies. NACE (Nomenclature des Activités Économiques dans la Communauté Européenne) is a European industry standard classification system similar in function to Standard Industry Classification (SIC) and North American Industry Classification System (NAICS) for classifying business activities. From EUROSTAT"@en ;
              rdfs:label "NACE code"@en .


###  http://w3id.org/um/cbcm/eu-cm-ontology#naceSector
cbcm:naceSector rdf:type owl:DatatypeProperty ;
                rdfs:domain cbcm:Company ;
                rdfs:range [ rdf:type rdfs:Datatype ;
                             owl:onDatatype xsd:string ;
                             owl:withRestrictions ( [ xsd:length "1"^^xsd:positiveInteger
                                                    ]
                                                  )
                           ] ;
                rdfs:comment "Company NACE sector. NACE (Nomenclature of Economic Activities) is the European statistical classification of economic activities. Classification of a company according to which kinds of sector (i.e. industry / market / product type) they deal in. From EUROSTAT"@en ;
                rdfs:label "NACE sector"@en .


###  http://w3id.org/um/cbcm/eu-cm-ontology#name
cbcm:name rdf:type owl:DatatypeProperty ;
          rdfs:range xsd:string ;
          rdfs:comment "The name of the organization"@en ;
          rdfs:label "Organization name"@en .


###  http://w3id.org/um/cbcm/eu-cm-ontology#natRegistrationNumber
cbcm:natRegistrationNumber rdf:type owl:DatatypeProperty ;
                           rdfs:domain cbcm:Company ;
                           rdfs:range xsd:string ;
                           rdfs:comment "The national registration number of an acquiring/receiving/entry company. A company registration number is a unique combination of numbers and/or letters. It is used to identify a company and verify its legal existence as an incorporated entity."@en ;
                           rdfs:label "NAT registration number"@en .


###  http://w3id.org/um/cbcm/eu-cm-ontology#negotiatedAgreement
cbcm:negotiatedAgreement rdf:type owl:DatatypeProperty ;
                         rdfs:domain cbcm:CompanyTransaction ;
                         rdfs:range xsd:string ;
                         rdfs:comment """Is the management of the companies involved starting the process of setting up a Special Negotiating Body (SNB) in order to reach a negotiated agreement on the future employee participation mechanism (BLER) after the transaction?

BLER (Board-Level Employee Represenation): highest level of employee involvement in a company in the supervisory board. They can take co-determine decisions of the company's management and where the company is heading.

- Yes: there is a negotiated agreement to be negotiated with the SNB;
- No: no negotiated agreement;
- Not applicable: the conditions are not met (e.g. no employees, BLER threshold not met) for this criterion to be applicable;
- Unclear: the wording of the document is unclear with regard to the impact/effect/measures taken;
- Not mentioned: given the parameters, this aspect should be addressed in the transaction document, but is not mentioned"""@en ;
                         rdfs:label "Has negotiated agreement"@en .


###  http://w3id.org/um/cbcm/eu-cm-ontology#rawTransactionID
cbcm:rawTransactionID rdf:type owl:DatatypeProperty ;
                      rdfs:domain cbcm:CompanyTransaction ;
                      rdfs:range xsd:positiveInteger ;
                      rdfs:comment """unique identifier before database entry.

This id is the old ID-structure used before entry into the CbCMdb"""@en ;
                      rdfs:label "Raw transaction ID"@en .


###  http://w3id.org/um/cbcm/eu-cm-ontology#registeredOffice
cbcm:registeredOffice rdf:type owl:DatatypeProperty ;
                      rdfs:comment "Deprecated property"@en ;
                      rdfs:label "Registered Office"@en .


###  http://w3id.org/um/cbcm/eu-cm-ontology#sbnVoluntaryApplication
cbcm:sbnVoluntaryApplication rdf:type owl:DatatypeProperty ;
                             rdfs:domain cbcm:CompanyTransaction ;
                             rdfs:range xsd:string ;
                             rdfs:comment """Is a Special Negotiating Body (SNB) set up voluntary?

Whether or not a SNB is created/will be created voluntarily.

- Yes: an SNB is created voluntarily;
- No: no voluntary SNB set up;
- Not applicable: the conditions are not met (e.g. no employees, BLER threshold not met) for this criterion to be applicable;
- Unclear: the wording of the document is unclear with regard to the impact/effect/measures taken;
- Not mentioned: given the parameters, this aspect should be addressed in the transaction document, but is not mentioned"""@en ;
                             rdfs:label "SNB voluntary application"@en .


###  http://w3id.org/um/cbcm/eu-cm-ontology#standardRulesApplication
cbcm:standardRulesApplication rdf:type owl:DatatypeProperty ;
                              rdfs:domain cbcm:CompanyTransaction ;
                              rdfs:range xsd:string ;
                              rdfs:comment """Are the standard rules applied directly without and instead of the start of negotiations with a Special Negotiating Body (SNB)?

Instead of an SNB being set up, the standard rules are applied instead.

- Yes: the standard rules are applied;
- No: standard rules ar enot applied;
- Not applicable: the conditions are not met (e.g. no employees, BLER threshold not met) for this criterion to be applicable;
- Unclear: the wording of the document is unclear with regard to the impact/effect/measures taken;
- Not mentioned: given the parameters, this aspect should be addressed in the transaction document, but is not mentioned"""@en ;
                              rdfs:label "Standard rules application"@en .


###  http://w3id.org/um/cbcm/eu-cm-ontology#tnic
cbcm:tnic rdf:type owl:DatatypeProperty ;
          rdfs:domain cbcm:Company ;
          rdfs:range xsd:boolean ;
          rdfs:comment """Is the company having a transnational information and consultation agreement in place? Does the company have an internal body which discusses employee rights and welfare?

Different from works council. TNIC is global."""@en ;
          rdfs:label "Has TNIC"@en .


###  http://w3id.org/um/cbcm/eu-cm-ontology#toBeNegotiatedBLER
cbcm:toBeNegotiatedBLER rdf:type owl:DatatypeProperty ;
                        rdfs:domain cbcm:CompanyTransaction ;
                        rdfs:range xsd:string ;
                        rdfs:comment """Is an employee board level representation/participation (BLER) mechanism going to be re-negotiated in the process of the cross-border transaction?

- Yes: BLER be (re-)negotiated with the SNB;
- No: no BLER-(re-)negotiation;
- Not applicable: the conditions are not met (e.g. no employees, BLER threshold not met) for this criterion to be applicable;
- Unclear: the wording of the document is unclear with regard to the impact/effect/measures taken;
- Not mentioned: given the parameters, this aspect should be addressed in the transaction document, but is not mentioned"""@en ;
                        rdfs:label "BLER to be negotiated"@en .


###  http://w3id.org/um/cbcm/eu-cm-ontology#transactionComment
cbcm:transactionComment rdf:type owl:DatatypeProperty ;
                        rdfs:domain cbcm:CompanyTransaction ;
                        rdfs:range xsd:string ;
                        rdfs:comment "Notes from researcher about the transaction"@en ;
                        rdfs:label "Transaction comment"@en .


###  http://w3id.org/um/cbcm/eu-cm-ontology#transactionCompletionDate
cbcm:transactionCompletionDate rdf:type owl:DatatypeProperty ;
                               rdfs:domain cbcm:CompanyTransaction ;
                               rdfs:range xsd:dateTime ;
                               rdfs:comment """Date on which the transaction was effectuated (the date that the competent authority e.g., business registry of that country, says that the criteria have been met by merging and acquiring companies and the merging/transferring company is dissolved).

This is the final step of a transaction process"""@en ;
                               rdfs:label "Transaction completion date"@en .


###  http://w3id.org/um/cbcm/eu-cm-ontology#transactionID
cbcm:transactionID rdf:type owl:DatatypeProperty ;
                   rdfs:domain cbcm:CompanyTransaction ;
                   rdfs:range xsd:positiveInteger ;
                   rdfs:comment "unique identifier for a transaction"@en ;
                   rdfs:label "Transaction ID"@en .


###  http://w3id.org/um/cbcm/eu-cm-ontology#transactionPlan
cbcm:transactionPlan rdf:type owl:DatatypeProperty ;
                     rdfs:domain cbcm:CompanyTransaction ;
                     rdfs:range xsd:boolean ;
                     rdfs:comment """Is the transaction plan available for analysis?

Merger plan, Seat transfer plan or Division plan. Transaction notice is where the transaction is announced. The other documents are where the nature and details of the transaction are specified."""@en ;
                     rdfs:label "Transaction plan available"@en .


###  http://w3id.org/um/cbcm/eu-cm-ontology#transactionStartDate
cbcm:transactionStartDate rdf:type owl:DatatypeProperty ;
                          rdfs:domain cbcm:CompanyTransaction ;
                          rdfs:range xsd:dateTime ;
                          rdfs:comment "Date of the transaction notice (document announcing the transaction) constituting the start of the transaction process. Date that the document was published (which is the important date because this is when it becomes legally binding)"@en ;
                          rdfs:label "Transaction notice date"@en .


###  http://w3id.org/um/cbcm/eu-cm-ontology#website
cbcm:website rdf:type owl:DatatypeProperty ;
             rdfs:domain cbcm:Organisation ;
             rdfs:range xsd:string ;
             rdfs:comment "Homepage of a company/organization website"@en ;
             rdfs:label "Website"@en .


###  http://w3id.org/um/cbcm/eu-cm-ontology#wwEmploymentFigureAtTransaction
cbcm:wwEmploymentFigureAtTransaction rdf:type owl:DatatypeProperty ;
                                     rdfs:domain cbcm:CompanyTransaction ;
                                     rdfs:range xsd:nonNegativeInteger ;
                                     rdfs:comment "number of employees of company group worldwide at the moment of the transaction"@en ;
                                     rdfs:label "Total WW employees at transaction"@en .


###  http://w3id.org/um/cbcm/eu-cm-ontology#yearDivergingEmploymentFigure
cbcm:yearDivergingEmploymentFigure rdf:type owl:DatatypeProperty ;
                                   rdfs:domain cbcm:CompanyTransaction ;
                                   rdfs:range xsd:dateTime ;
                                   rdfs:comment "The year for which a diverging employee number is recorded"@en ;
                                   rdfs:label "Diverging employment figure year"@en .


###  http://w3id.org/um/cbcm/eu-cm-ontology#yearWWEmploymentFigure
cbcm:yearWWEmploymentFigure rdf:type owl:DatatypeProperty ;
                            rdfs:domain cbcm:CompanyTransaction ;
                            rdfs:range xsd:dateTime ;
                            rdfs:comment "Year in which the last worldwide employment figure was recorded"@en ;
                            rdfs:label "Last WW employment figure year"@en .


#################################################################
#    Classes
#################################################################

###  http://w3id.org/um/cbcm/eu-cm-ontology#AcquiringCompany
cbcm:AcquiringCompany rdf:type owl:Class ;
                      rdfs:subClassOf cbcm:Company ,
                                      [ rdf:type owl:Restriction ;
                                        owl:onProperty cbcm:isTransactionResultOf ;
                                        owl:someValuesFrom cbcm:CompanyMerger
                                      ] ;
                      rdfs:comment "Acquiring Company means the resulting or surviving company in a transaction that takes over another, merging company."@en ;
                      rdfs:isDefinedBy cbcm: ;
                      rdfs:label "Acquiring company"@en ;
                      rdfs:seeAlso <http://data.europa.eu/eli/dir/2017/1132/oj> .


###  http://w3id.org/um/cbcm/eu-cm-ontology#Agent
cbcm:Agent rdf:type owl:Class ;
           rdfs:subClassOf obo:BFO_0000040 ;
           terms:description "An entity or group of entities (either biological or non-biological) that is able to perform actions autonomously in the world."@en ;
           rdfs:comment "An entity or group of entities (either biological or non-biological) that is able to perform actions autonomously in the world."@en ;
           rdfs:isDefinedBy cbcm: ;
           rdfs:label "Agent" .


###  http://w3id.org/um/cbcm/eu-cm-ontology#AnnualAccount
cbcm:AnnualAccount rdf:type owl:Class ;
                   owl:equivalentClass cbcm:AnnualReport ;
                   rdfs:subClassOf cbcm:CompanyMobilityDocument ;
                   rdfs:comment "Annual reports measure a company's financial health. They focus on past and present financial performance, and make predictions about future prospects. The revenue and financial performance of a company."@en ;
                   rdfs:isDefinedBy cbcm: ;
                   rdfs:label "Annual account"@en .


###  http://w3id.org/um/cbcm/eu-cm-ontology#AnnualReport
cbcm:AnnualReport rdf:type owl:Class ;
                  rdfs:subClassOf cbcm:CompanyMobilityDocument ;
                  rdfs:comment "Annual reports measure a company's financial health. They focus on past and present financial performance, and make predictions about future prospects. The revenue and financial performance of a company."@en ;
                  rdfs:isDefinedBy cbcm: ;
                  rdfs:label "Annual report"@en .


###  http://w3id.org/um/cbcm/eu-cm-ontology#Attribute
cbcm:Attribute rdf:type owl:Class ;
               rdfs:subClassOf obo:BFO_0000141 ;
               terms:description "An attribute is a characteristic of some entity."@en ;
               rdfs:comment "An attribute is a characteristic of some entity."@en ;
               rdfs:isDefinedBy cbcm: ;
               rdfs:label "Attribute" .


###  http://w3id.org/um/cbcm/eu-cm-ontology#Behaviour
cbcm:Behaviour rdf:type owl:Class ;
               rdfs:subClassOf obo:BFO_0000015 ;
               owl:disjointWith cbcm:Procedure ;
               terms:description "Behaviour is the set of actions and mannerisms made by systems (biological or otherwise) in response to stimuli or inputs, whether internal or external, conscious or subconscious, overt or covert, and voluntary or involuntary."@en ;
               rdfs:comment "Behaviour is the set of actions and mannerisms made by systems (biological or otherwise) in response to stimuli or inputs, whether internal or external, conscious or subconscious, overt or covert, and voluntary or involuntary."@en ;
               rdfs:isDefinedBy cbcm: ;
               rdfs:label "Behaviour" ;
               <http://www.w3.org/2003/06/sw-vocab-status/ns#term_status> "deprecated"^^xsd:string .


###  http://w3id.org/um/cbcm/eu-cm-ontology#BoardLevelEmployeeRepresentationRight
cbcm:BoardLevelEmployeeRepresentationRight rdf:type owl:Class ;
                                           rdfs:subClassOf cbcm:SocialRight ;
                                           rdfs:comment "Board-level representation of employees (BLER) refers to the phenomenon where employees or their representatives elect or appoint representatives to the strategic decision-making body of a company (i.e. the supervisory board or non-executive board in a one-tier system). The BLER right requires that if such a system of BLER exists prior to a cross-border company transaction, such a right must be upheld in the acquiring/recipient company under the \"before-and-after-principle\"."@en ;
                                           rdfs:isDefinedBy cbcm: ;
                                           rdfs:label "Board-level employee representation right"@en ;
                                           rdfs:seeAlso <http://data.europa.eu/eli/dir/2017/1132/oj> .


###  http://w3id.org/um/cbcm/eu-cm-ontology#BoardResolution
cbcm:BoardResolution rdf:type owl:Class ;
                     rdfs:subClassOf cbcm:Resolution ;
                     rdfs:comment "A Board Resolution, or Company Resolution, is a way of documenting a decision made by a Company's Board of Directors on behalf of the company. After the resolution is made during a meeting, a Board Resolution document is typically used to get the specifics of the resolution in writing."@en ;
                     rdfs:isDefinedBy cbcm: ;
                     rdfs:label "Board resolution"@en .


###  http://w3id.org/um/cbcm/eu-cm-ontology#CBCMResearcher
cbcm:CBCMResearcher rdf:type owl:Class ;
                    rdfs:subClassOf cbcm:Person ;
                    rdfs:comment "A person that is interested in research about cross-border company mobility, and actively collects and analyses data concerning cross-border company mobility."@en ;
                    rdfs:isDefinedBy cbcm: ;
                    rdfs:label "Cross-border company mobility researcher"@en .


###  http://w3id.org/um/cbcm/eu-cm-ontology#City
cbcm:City rdf:type owl:Class ;
          rdfs:subClassOf cbcm:GeoPoliticalRegion ,
                          [ rdf:type owl:Restriction ;
                            owl:onProperty cbcm:locatedIn ;
                            owl:qualifiedCardinality "1"^^xsd:nonNegativeInteger ;
                            owl:onClass cbcm:Country
                          ] ;
          rdfs:comment "A city (plural \"cities\") is a geo-political region in which there is a large human settlement. The distinction with the term \"town\" (plural \"towns\") is that cities are generally larger than towns. Countries are generally larger than cities and, in fact, usually consist of multiple cities."@en ;
          rdfs:isDefinedBy cbcm: ;
          rdfs:label "City"@en .


###  http://w3id.org/um/cbcm/eu-cm-ontology#Company
cbcm:Company rdf:type owl:Class ;
             rdfs:subClassOf cbcm:Organisation ,
                             [ rdf:type owl:Restriction ;
                               owl:onProperty cbcm:hasMember ;
                               owl:someValuesFrom cbcm:Employee
                             ] ,
                             [ rdf:type owl:Restriction ;
                               owl:onProperty cbcm:hasPart ;
                               owl:qualifiedCardinality "1"^^xsd:nonNegativeInteger ;
                               owl:onClass cbcm:CompanyCentralAdministration
                             ] ,
                             [ rdf:type owl:Restriction ;
                               owl:onProperty cbcm:hasPart ;
                               owl:qualifiedCardinality "1"^^xsd:nonNegativeInteger ;
                               owl:onClass cbcm:CompanyRegisteredOffice
                             ] ;
             rdfs:comment "A company is a legal entity formed by a group of individuals to engage in and operate a business—commercial or industrial—enterprise. A company may be organized in various ways for tax and financial liability purposes depending on the corporate law of its jurisdiction."@en ;
             rdfs:isDefinedBy cbcm: ;
             rdfs:label "Company"@en .


###  http://w3id.org/um/cbcm/eu-cm-ontology#CompanyCentralAdministration
cbcm:CompanyCentralAdministration rdf:type owl:Class ;
                                  owl:equivalentClass cbcm:CompanyHeadQuarter ;
                                  rdfs:subClassOf cbcm:OrganisationalUnit ;
                                  rdfs:comment "The headquarters or body of a company which governs it's financial and administrative activities"@en ;
                                  rdfs:isDefinedBy cbcm: ;
                                  rdfs:label "Central Administration"@en .


###  http://w3id.org/um/cbcm/eu-cm-ontology#CompanyConversion
cbcm:CompanyConversion rdf:type owl:Class ;
                       owl:equivalentClass [ owl:intersectionOf ( cbcm:CompanyTransaction
                                                                  [ rdf:type owl:Restriction ;
                                                                    owl:onProperty cbcm:hasTransactionInput ;
                                                                    owl:qualifiedCardinality "1"^^xsd:nonNegativeInteger ;
                                                                    owl:onClass cbcm:Company
                                                                  ]
                                                                  [ rdf:type owl:Restriction ;
                                                                    owl:onProperty cbcm:hasTransactionResult ;
                                                                    owl:qualifiedCardinality "1"^^xsd:nonNegativeInteger ;
                                                                    owl:onClass cbcm:Company
                                                                  ]
                                                                  [ rdf:type owl:Restriction ;
                                                                    owl:onProperty cbcm:involvesChangeOf ;
                                                                    owl:qualifiedCardinality "1"^^xsd:nonNegativeInteger ;
                                                                    owl:onClass cbcm:CompanyLegalForm
                                                                  ]
                                                                ) ;
                                             rdf:type owl:Class
                                           ] ;
                       rdfs:subClassOf cbcm:CompanyTransaction ,
                                       [ rdf:type owl:Restriction ;
                                         owl:onProperty cbcm:requiresDocument ;
                                         owl:someValuesFrom cbcm:ConversionPlan
                                       ] ,
                                       [ rdf:type owl:Restriction ;
                                         owl:onProperty cbcm:sourceCountry ;
                                         owl:someValuesFrom cbcm:Country
                                       ] ,
                                       [ rdf:type owl:Restriction ;
                                         owl:onProperty cbcm:targetCountry ;
                                         owl:someValuesFrom cbcm:Country
                                       ] ;
                       rdfs:comment "The process of changing or converting the corporate structure of a company. For example, a limited liability company of one country to one of another country, or from a private to a public limited liability company, or vice-versa by means of the continuance of an entity into another entity."@en ;
                       rdfs:isDefinedBy cbcm: ;
                       rdfs:label "Company conversion"@en .


###  http://w3id.org/um/cbcm/eu-cm-ontology#CompanyDivision
cbcm:CompanyDivision rdf:type owl:Class ;
                     owl:equivalentClass [ owl:intersectionOf ( cbcm:CompanyTransaction
                                                                [ rdf:type owl:Restriction ;
                                                                  owl:onProperty cbcm:hasTransactionResult ;
                                                                  owl:minQualifiedCardinality "2"^^xsd:nonNegativeInteger ;
                                                                  owl:onClass cbcm:Company
                                                                ]
                                                                [ rdf:type owl:Restriction ;
                                                                  owl:onProperty cbcm:hasTransactionInput ;
                                                                  owl:qualifiedCardinality "1"^^xsd:nonNegativeInteger ;
                                                                  owl:onClass cbcm:Company
                                                                ]
                                                              ) ;
                                           rdf:type owl:Class
                                         ] ;
                     rdfs:subClassOf cbcm:CompanyTransaction ,
                                     [ rdf:type owl:Restriction ;
                                       owl:onProperty cbcm:hasRecipientCompany ;
                                       owl:someValuesFrom cbcm:Company
                                     ] ,
                                     [ rdf:type owl:Restriction ;
                                       owl:onProperty cbcm:requiresDocument ;
                                       owl:someValuesFrom cbcm:DivisionPlan
                                     ] ,
                                     [ rdf:type owl:Restriction ;
                                       owl:onProperty cbcm:sourceCountry ;
                                       owl:someValuesFrom cbcm:Country
                                     ] ,
                                     [ rdf:type owl:Restriction ;
                                       owl:onProperty cbcm:targetCountry ;
                                       owl:someValuesFrom cbcm:Country
                                     ] ;
                     rdfs:comment """Article 160b - Division means:
a) company being divided, on being dissolved without going into liquidation, transfers all its assets and liabilities to two or more newly formed companies (‘the recipient companies’), in exchange for the issue to the members of the company being divided of securities or shares in the recipient companies and, if any, a cash payment not exceeding 10 % of the nominal value of those securities or shares or, where they have no nominal value, a cash payment not exceeding 10% of the accounting par value of their securities or shares ('full division');

(b) 	a company being divided transfers part of its assets and liabilities to one or more newly formed companies (‘the recipient companies’), in exchange for the issue to the members of the company being divided of securities or shares in the recipient companies or in the company being divided or in both the recipient companies and in the company being divided, and if any a cash payment not exceeding 10 % of the nominal value of those securities or shares, or in the absence of a nominal value, a cash payment not exceeding 10 % of the accounting par value of their securities or shares (‘partial division’).
   	
(c) 	a company being divided transfers part of its assets and liabilities to one or more newly formed companies (‘the recipient companies’), in exchange for the issue of securities or shares in the recipient companies to the company being divided (‘division by separation’)."""@en ;
                     rdfs:isDefinedBy cbcm: ;
                     rdfs:label "Company division"@en ;
                     rdfs:seeAlso <https://www.europarl.europa.eu/doceo/document/TA-8-2019-0429_EN.html> .


###  http://w3id.org/um/cbcm/eu-cm-ontology#CompanyHeadQuarter
cbcm:CompanyHeadQuarter rdf:type owl:Class ;
                        rdfs:subClassOf cbcm:OrganisationalUnit ;
                        rdfs:comment "The location of a company headquarter"@en ;
                        rdfs:isDefinedBy cbcm: ;
                        rdfs:label "Company headquarter"@en ;
                        rdfs:seeAlso "http://w3id.org/um/cbcm/eu-cm-ontology#CompanyCentralAdministration"@en .


###  http://w3id.org/um/cbcm/eu-cm-ontology#CompanyLegalForm
cbcm:CompanyLegalForm rdf:type owl:Class ;
                      rdfs:subClassOf cbcm:Attribute ;
                      rdfs:comment "Name given to describe the structure of a corporation or business in the different legal orders. For example Limited (Ltd.), Public Limited Company (PLC), Gesellschaft mit beschränkter Haftung (GmbH), Aktiengesellschaft (AG). The company legal form is regulated under national law and grants specific rights and obligations to the company stakeholders (such as shareholders, management & employees)."@en ;
                      rdfs:isDefinedBy cbcm: ;
                      rdfs:label "Company form"@en ;
                      rdfs:seeAlso <https://www.ecb.europa.eu/stats/money/aggregates/anacredit/shared/pdf/List_of_legal_forms.xlsx> .


###  http://w3id.org/um/cbcm/eu-cm-ontology#CompanyMerger
cbcm:CompanyMerger rdf:type owl:Class ;
                   owl:equivalentClass [ owl:intersectionOf ( cbcm:CompanyTransaction
                                                              [ rdf:type owl:Restriction ;
                                                                owl:onProperty cbcm:hasTransactionInput ;
                                                                owl:minQualifiedCardinality "2"^^xsd:nonNegativeInteger ;
                                                                owl:onClass cbcm:Company
                                                              ]
                                                              [ rdf:type owl:Restriction ;
                                                                owl:onProperty cbcm:hasTransactionResult ;
                                                                owl:qualifiedCardinality "1"^^xsd:nonNegativeInteger ;
                                                                owl:onClass cbcm:Company
                                                              ]
                                                            ) ;
                                         rdf:type owl:Class
                                       ] ;
                   rdfs:subClassOf cbcm:CompanyTransaction ,
                                   [ rdf:type owl:Restriction ;
                                     owl:onProperty cbcm:requiresDocument ;
                                     owl:someValuesFrom cbcm:MergerPlan
                                   ] ;
                   rdfs:comment """‘merger’ in Directive (EU) 2017/1132 means an operation whereby:

(a) one or more companies, on being dissolved without going into liquidation, transfer all their assets and liabilities to another existing company, the acquiring company, in exchange for the issue to their members of securities or shares representing the capital of that other company and, if applicable, a cash payment not exceeding 10 % of the nominal value, or, in the absence of a nominal value, of the accounting par value of those securities or shares; or

(b) two or more companies, on being dissolved without going into liquidation, transfer all their assets and liabilities to a company that they form, the new company, in exchange for the issue to their members of securities or shares representing the capital of that new company and, if applicable, a cash payment not exceeding 10 % of the nominal value, or in the absence of a nominal value, of the accounting par value of those securities or shares; or

(c) a company, on being dissolved without going into liquidation, transfers all its assets and liabilities to the company holding all the securities or shares representing its capital;\"

(d) one or more companies, on being dissolved without going into liquidation, transfer all their assets and liabilities to another existing company, the acquiring company, without the issue of any new shares by the acquiring company, provided that one person holds directly or indirectly all the shares in the merging companies or the members of the merging companies hold their shares in the same proportion in all merging companies.\";"""@en ;
                   rdfs:isDefinedBy cbcm: ;
                   rdfs:label "Company merger"@en .


###  http://w3id.org/um/cbcm/eu-cm-ontology#CompanyMobilityDocument
cbcm:CompanyMobilityDocument rdf:type owl:Class ;
                             rdfs:subClassOf obo:BFO_0000030 ;
                             rdfs:comment "A legal document which provides information related to, or influencing, a company's mobility within a specific country or across national boundaries."@en ;
                             rdfs:isDefinedBy cbcm: ;
                             rdfs:label "Company mobility document"@en .


###  http://w3id.org/um/cbcm/eu-cm-ontology#CompanyRegisteredOffice
cbcm:CompanyRegisteredOffice rdf:type owl:Class ;
                             rdfs:subClassOf cbcm:GeoPoliticalRegion ;
                             rdfs:comment "The physical address or location at which the primary business activities of a company are carried out."@en ;
                             rdfs:isDefinedBy cbcm: ;
                             rdfs:label "Registered office"@en .


###  http://w3id.org/um/cbcm/eu-cm-ontology#CompanySeatTransfer
cbcm:CompanySeatTransfer rdf:type owl:Class ;
                         owl:equivalentClass [ owl:intersectionOf ( cbcm:CompanyTransaction
                                                                    [ rdf:type owl:Restriction ;
                                                                      owl:onProperty cbcm:hasTransactionInput ;
                                                                      owl:qualifiedCardinality "1"^^xsd:nonNegativeInteger ;
                                                                      owl:onClass cbcm:Company
                                                                    ]
                                                                    [ rdf:type owl:Restriction ;
                                                                      owl:onProperty cbcm:hasTransactionResult ;
                                                                      owl:qualifiedCardinality "1"^^xsd:nonNegativeInteger ;
                                                                      owl:onClass cbcm:Company
                                                                    ]
                                                                    [ rdf:type owl:Restriction ;
                                                                      owl:onProperty cbcm:involvesChangeOf ;
                                                                      owl:qualifiedCardinality "1"^^xsd:nonNegativeInteger ;
                                                                      owl:onClass cbcm:CompanyCentralAdministration
                                                                    ]
                                                                    [ rdf:type owl:Restriction ;
                                                                      owl:onProperty cbcm:involvesChangeOf ;
                                                                      owl:qualifiedCardinality "1"^^xsd:nonNegativeInteger ;
                                                                      owl:onClass cbcm:CompanyRegisteredOffice
                                                                    ]
                                                                  ) ;
                                               rdf:type owl:Class
                                             ] ;
                         rdfs:subClassOf cbcm:CompanyTransaction ,
                                         [ rdf:type owl:Restriction ;
                                           owl:onProperty cbcm:requiresDocument ;
                                           owl:someValuesFrom cbcm:SeatTransferPlan
                                         ] ,
                                         [ rdf:type owl:Restriction ;
                                           owl:onProperty cbcm:sourceCountry ;
                                           owl:someValuesFrom cbcm:Country
                                         ] ,
                                         [ rdf:type owl:Restriction ;
                                           owl:onProperty cbcm:targetCountry ;
                                           owl:someValuesFrom cbcm:Country
                                         ] ,
                                         [ rdf:type owl:Restriction ;
                                           owl:onProperty cbcm:hasSubProcedure ;
                                           owl:qualifiedCardinality "1"^^xsd:nonNegativeInteger ;
                                           owl:onClass cbcm:TransferOfCentralAdministration
                                         ] ,
                                         [ rdf:type owl:Restriction ;
                                           owl:onProperty cbcm:hasSubProcedure ;
                                           owl:qualifiedCardinality "1"^^xsd:nonNegativeInteger ;
                                           owl:onClass cbcm:TransferOfRegisteredOffice
                                         ] ,
                                         [ rdf:type owl:Restriction ;
                                           owl:onProperty cbcm:hasTransactionInput ;
                                           owl:qualifiedCardinality "1"^^xsd:nonNegativeInteger ;
                                           owl:onClass cbcm:Company
                                         ] ,
                                         [ rdf:type owl:Restriction ;
                                           owl:onProperty cbcm:hasTransactionResult ;
                                           owl:qualifiedCardinality "1"^^xsd:nonNegativeInteger ;
                                           owl:onClass cbcm:Company
                                         ] ;
                         rdfs:comment "The act of changing the location where the company’s business was managed (registered office or headquarters) or the place where that company’s primary business was actually conducted (central administration)."@en ;
                         rdfs:isDefinedBy cbcm: ;
                         rdfs:label "Company seat transfer"@en .


###  http://w3id.org/um/cbcm/eu-cm-ontology#CompanyShareholder
cbcm:CompanyShareholder rdf:type owl:Class ;
                        rdfs:subClassOf cbcm:CompanyStakeholder ,
                                        [ rdf:type owl:Restriction ;
                                          owl:onProperty cbcm:partOf ;
                                          owl:someValuesFrom cbcm:Company
                                        ] ;
                        rdfs:comment "An individual, group, or organization that owns one or more shares in a company, and in whose name the share certificate is issued."@en ;
                        rdfs:isDefinedBy cbcm: ;
                        rdfs:label "Company shareholder"@en .


###  http://w3id.org/um/cbcm/eu-cm-ontology#CompanyStakeholder
cbcm:CompanyStakeholder rdf:type owl:Class ;
                        rdfs:subClassOf cbcm:Agent ,
                                        [ rdf:type owl:Class ;
                                          owl:unionOf ( cbcm:Organisation
                                                        cbcm:Person
                                                      )
                                        ] ;
                        rdfs:comment "A person, group or organization that has interest or concern in an organization or company in particular. Stakeholders can affect or be affected by the company's actions, objectives and policies."@en ;
                        rdfs:isDefinedBy cbcm: ;
                        rdfs:label "Stakeholder in a company"@en .


###  http://w3id.org/um/cbcm/eu-cm-ontology#CompanyTransaction
cbcm:CompanyTransaction rdf:type owl:Class ;
                        rdfs:subClassOf cbcm:Procedure ,
                                        [ rdf:type owl:Restriction ;
                                          owl:onProperty cbcm:hasTransactionResult ;
                                          owl:someValuesFrom cbcm:Company
                                        ] ,
                                        [ rdf:type owl:Restriction ;
                                          owl:onProperty cbcm:reportedIn ;
                                          owl:someValuesFrom cbcm:TransactionNotice
                                        ] ,
                                        [ rdf:type owl:Restriction ;
                                          owl:onProperty cbcm:transactionValidatedByDocument ;
                                          owl:someValuesFrom cbcm:TransactionCertificate
                                        ] ;
                        rdfs:comment "An action taken by a company that modifies its corporate structure with a change of control (for e.g. through either a merger, division, conversion or seat transfer in a domestic or cross-border setting). It involves one or more companies, each of which have a company legal form valid in a Member State of the European Union."@en ;
                        rdfs:isDefinedBy cbcm: ;
                        rdfs:label "Company transaction"@en .


###  http://w3id.org/um/cbcm/eu-cm-ontology#CompetentAuthority
cbcm:CompetentAuthority rdf:type owl:Class ;
                        rdfs:subClassOf cbcm:Organisation ;
                        rdfs:comment "The monitoring of the completion and legality of the decision-making process in each company involved in a transaction is carried out by a national authority having jurisdiction over each of those companies. The national authority could be a court, a notary or any other competent authority appointed by the Member State concerned."@en ;
                        rdfs:isDefinedBy cbcm: ;
                        rdfs:label "Competent authority"@en ;
                        rdfs:seeAlso <http://data.europa.eu/eli/dir/2017/1132/oj> .


###  http://w3id.org/um/cbcm/eu-cm-ontology#ConsultationRight
cbcm:ConsultationRight rdf:type owl:Class ;
                       rdfs:subClassOf cbcm:SocialRight ;
                       rdfs:comment "The right of employees or their representatives to be consulted and to give advice on a business decision, such as an intended merger/division/conversion/seat transfer."@en ;
                       rdfs:isDefinedBy cbcm: ;
                       rdfs:label "Consultation right"@en ;
                       rdfs:seeAlso <http://data.europa.eu/eli/dir/2002/14/oj> ,
                                    <http://data.europa.eu/eli/dir/2017/1132/oj> .


###  http://w3id.org/um/cbcm/eu-cm-ontology#ConversionCertificate
cbcm:ConversionCertificate rdf:type owl:Class ;
                           rdfs:subClassOf cbcm:TransactionCertificate ;
                           rdfs:comment "A document issued by a Competent Authority declaring that the legally required steps of a conversion are completed. The certificate needs to be presented by a company to either be registered in another company registry or to be removed from a company register."@en ;
                           rdfs:isDefinedBy cbcm: ;
                           rdfs:label "Company conversion certificate"@en .


###  http://w3id.org/um/cbcm/eu-cm-ontology#ConversionPlan
cbcm:ConversionPlan rdf:type owl:Class ;
                    rdfs:subClassOf cbcm:TransactionDocument ;
                    rdfs:comment "A document providing details of how the conversion of a company will be implemented. Article 86d: The management or administrative organ of the company shall draw up the draft terms of a cross-border conversion. The draft terms of a cross-border conversion shall include at least the particulars listed in article 86d"@en ;
                    rdfs:isDefinedBy cbcm: ;
                    rdfs:label "Company conversion plan"@en ;
                    rdfs:seeAlso <https://www.europarl.europa.eu/doceo/document/TA-8-2019-0429_EN.html> .


###  http://w3id.org/um/cbcm/eu-cm-ontology#Country
cbcm:Country rdf:type owl:Class ;
             rdfs:subClassOf cbcm:GeoPoliticalRegion ;
             terms:description "A geo-political region that has a distinct and common political governance structure for people that inhabit it for a significant portion of their lives. The majority of people that inhabit such a region are also usually united by common descent, history, culture and language."@en ;
             rdfs:comment "A geo-political region that has a distinct and common political governance structure for people that inhabit it for a significant portion of their lives. The majority of people that inhabit such a region are also usually united by common descent, history, culture and language."@en ;
             rdfs:isDefinedBy cbcm: ;
             rdfs:label "Country" .


###  http://w3id.org/um/cbcm/eu-cm-ontology#Court
cbcm:Court rdf:type owl:Class ;
           rdfs:subClassOf cbcm:CompetentAuthority ;
           rdfs:comment "Legal forum in which a body of people presided over by a judge, judges, or magistrate, and acting as a tribunal in civil and criminal cases resolve legal disputes."@en ;
           rdfs:isDefinedBy cbcm: ;
           rdfs:label "Court"@en .


###  http://w3id.org/um/cbcm/eu-cm-ontology#Creditor
cbcm:Creditor rdf:type owl:Class ;
              rdfs:subClassOf cbcm:CompanyStakeholder ;
              rdfs:comment "A person, organization, or government that is owed money. A creditor's claims and the safeguarding of these creditor rights is laid down in the company law of the Member States and EU law."@en ;
              rdfs:isDefinedBy cbcm: ;
              rdfs:label "Creditor"@en ;
              rdfs:seeAlso <http://data.europa.eu/eli/dir/2017/1132/oj> .


###  http://w3id.org/um/cbcm/eu-cm-ontology#CreditorDecisionRight
cbcm:CreditorDecisionRight rdf:type owl:Class ;
                           rdfs:subClassOf cbcm:CreditorRight ;
                           rdfs:comment "The right of a creditor to influence or take a decision in the context of a transaction."@en ;
                           rdfs:isDefinedBy cbcm: ;
                           rdfs:label "Creditor decision right"@en ;
                           rdfs:seeAlso <http://data.europa.eu/eli/dir/2017/1132/oj> .


###  http://w3id.org/um/cbcm/eu-cm-ontology#CreditorExitRight
cbcm:CreditorExitRight rdf:type owl:Class ;
                       rdfs:subClassOf cbcm:CreditorRight ;
                       rdfs:comment "The creditors right to be paid out and therefore to exit the company in the context of a transaction."@en ;
                       rdfs:isDefinedBy cbcm: ;
                       rdfs:label "Creditor exit right"@en ;
                       rdfs:seeAlso <http://data.europa.eu/eli/dir/2017/1132/oj> .


###  http://w3id.org/um/cbcm/eu-cm-ontology#CreditorInformationRight
cbcm:CreditorInformationRight rdf:type owl:Class ;
                              rdfs:subClassOf cbcm:CreditorRight ;
                              rdfs:comment "The information rights of creditors in the context of a company transaction, which includes for instance access to documents."@en ;
                              rdfs:isDefinedBy cbcm: ;
                              rdfs:label "Creditor information right"@en ;
                              rdfs:seeAlso <http://data.europa.eu/eli/dir/2017/1132/oj> .


###  http://w3id.org/um/cbcm/eu-cm-ontology#CreditorRight
cbcm:CreditorRight rdf:type owl:Class ;
                   rdfs:subClassOf cbcm:TransactionRight ,
                                   [ rdf:type owl:Restriction ;
                                     owl:onProperty cbcm:applicableTo ;
                                     owl:someValuesFrom cbcm:Creditor
                                   ] ;
                   rdfs:comment "The rights of creditors, which includes debenture holders, vis-a-vis the company that obtained credit from the individual or organisation. Legal safeguards are put in place to ensure that rights of creditors are not negatively affected by a company transaction."@en ;
                   rdfs:isDefinedBy cbcm: ;
                   rdfs:label "Creditor right"@en ;
                   rdfs:seeAlso <http://data.europa.eu/eli/dir/2017/1132/oj> .


###  http://w3id.org/um/cbcm/eu-cm-ontology#CreditorSecurityRight
cbcm:CreditorSecurityRight rdf:type owl:Class ;
                           rdfs:subClassOf cbcm:CreditorRight ;
                           rdfs:comment "Member States shall provide for an adequate system of protection of the interest of creditors, and shall ensure that creditors who are dissatisfied with the safeguards offered in the draft terms of the transaction, as provided for in Article 86d (1) point (f), may apply to the appropriate administrative or judicial authority for adequate safeguards provided that they can credibly demonstrate that due to the transaction the satisfaction of their claims is at stake and that no adequate safeguards have been obtained from the company."@en ;
                           rdfs:isDefinedBy cbcm: ;
                           rdfs:label "Creditor security right"@en ;
                           rdfs:seeAlso <http://data.europa.eu/eli/dir/2017/1132/oj> ,
                                        <https://www.europarl.europa.eu/doceo/document/TA-8-2019-0429_EN.html> .


###  http://w3id.org/um/cbcm/eu-cm-ontology#CrossBorderConversion
cbcm:CrossBorderConversion rdf:type owl:Class ;
                           rdfs:subClassOf cbcm:CompanyConversion ,
                                           [ rdf:type owl:Restriction ;
                                             owl:onProperty cbcm:hasTransactionResult ;
                                             owl:someValuesFrom cbcm:Company
                                           ] ,
                                           [ rdf:type owl:Restriction ;
                                             owl:onProperty cbcm:requiresDocument ;
                                             owl:someValuesFrom cbcm:PreConversionCertificate
                                           ] ,
                                           [ rdf:type owl:Restriction ;
                                             owl:onProperty cbcm:involvesCountry ;
                                             owl:qualifiedCardinality "2"^^xsd:nonNegativeInteger ;
                                             owl:onClass cbcm:Country
                                           ] ;
                           rdfs:comment "A cross-border conversion is an operation through which a company, formed in one country (with the EU/EEA set of countries) is converted into a company governed by the law of another."@en ;
                           rdfs:isDefinedBy cbcm: ;
                           rdfs:label "Cross-border conversion"@en .


###  http://w3id.org/um/cbcm/eu-cm-ontology#CrossBorderDivision
cbcm:CrossBorderDivision rdf:type owl:Class ;
                         owl:equivalentClass [ owl:intersectionOf ( cbcm:CompanyDivision
                                                                    [ rdf:type owl:Restriction ;
                                                                      owl:onProperty cbcm:involvesCountry ;
                                                                      owl:minQualifiedCardinality "2"^^xsd:nonNegativeInteger ;
                                                                      owl:onClass cbcm:Country
                                                                    ]
                                                                  ) ;
                                               rdf:type owl:Class
                                             ] ;
                         rdfs:subClassOf cbcm:CompanyDivision ;
                         rdfs:comment "A company which in a process of the cross-border division in case of a full division transfers all its assets and liabilities to two or more companies, or in case of a partial division or division by separation transfers part of its assets and liabilities to one or more companies. The companies involved in the process are located in multiple (two or more) distinct countries."@en ;
                         rdfs:isDefinedBy cbcm: ;
                         rdfs:label "Cross-border company division"@en .


###  http://w3id.org/um/cbcm/eu-cm-ontology#CrossBorderMerger
cbcm:CrossBorderMerger rdf:type owl:Class ;
                       owl:equivalentClass [ owl:intersectionOf ( cbcm:CompanyMerger
                                                                  [ rdf:type owl:Restriction ;
                                                                    owl:onProperty cbcm:sourceCountry ;
                                                                    owl:someValuesFrom cbcm:Country
                                                                  ]
                                                                  [ rdf:type owl:Restriction ;
                                                                    owl:onProperty cbcm:involvesCountry ;
                                                                    owl:minQualifiedCardinality "2"^^xsd:nonNegativeInteger ;
                                                                    owl:onClass cbcm:Country
                                                                  ]
                                                                  [ rdf:type owl:Restriction ;
                                                                    owl:onProperty cbcm:targetCountry ;
                                                                    owl:qualifiedCardinality "1"^^xsd:nonNegativeInteger ;
                                                                    owl:onClass cbcm:Country
                                                                  ]
                                                                ) ;
                                             rdf:type owl:Class
                                           ] ;
                       rdfs:subClassOf cbcm:CompanyMerger ,
                                       [ rdf:type owl:Restriction ;
                                         owl:onProperty cbcm:hasTransactionInput ;
                                         owl:someValuesFrom cbcm:AcquiringCompany
                                       ] ,
                                       [ rdf:type owl:Restriction ;
                                         owl:onProperty cbcm:hasTransactionInput ;
                                         owl:someValuesFrom cbcm:MergingCompany
                                       ] ,
                                       [ rdf:type owl:Restriction ;
                                         owl:onProperty cbcm:sourceCountry ;
                                         owl:someValuesFrom cbcm:Country
                                       ] ,
                                       [ rdf:type owl:Restriction ;
                                         owl:onProperty cbcm:targetCountry ;
                                         owl:qualifiedCardinality "1"^^xsd:nonNegativeInteger ;
                                         owl:onClass cbcm:Country
                                       ] ;
                       rdfs:comment "A cross border merger involves at least one company based in an EU Member State and one company that is registered elsewhere within the European Union and is leading to a universal transfer of assets and liabilities from the merging company to the acquiring company."@en ;
                       rdfs:isDefinedBy cbcm: ;
                       rdfs:label "Cross-border merger"@en ;
                       rdfs:seeAlso <http://data.europa.eu/eli/dir/2017/1132/oj> .


###  http://w3id.org/um/cbcm/eu-cm-ontology#CrossBorderMergerByAcquisition
cbcm:CrossBorderMergerByAcquisition rdf:type owl:Class ;
                                    owl:equivalentClass [ owl:intersectionOf ( cbcm:CrossBorderMerger
                                                                               [ rdf:type owl:Restriction ;
                                                                                 owl:onProperty cbcm:hasMergingCompany ;
                                                                                 owl:someValuesFrom cbcm:Company
                                                                               ]
                                                                               [ rdf:type owl:Restriction ;
                                                                                 owl:onProperty cbcm:hasAcquiringCompany ;
                                                                                 owl:qualifiedCardinality "1"^^xsd:nonNegativeInteger ;
                                                                                 owl:onClass cbcm:Company
                                                                               ]
                                                                             ) ;
                                                          rdf:type owl:Class
                                                        ] ;
                                    rdfs:subClassOf cbcm:CrossBorderMerger ;
                                    rdfs:comment "Article 89: The operation whereby one or more companies are wound up without going into liquidation and transfer to another all their assets and liabilities in exchange for the issue to the shareholders of the company or companies being acquired of shares in the acquiring company and a cash payment, if any, not exceeding 10 % of the nominal value of the shares so issued or, where they have no nominal value, of their accounting par value. Companies involved come from two or more distinct countries."@en ;
                                    rdfs:isDefinedBy cbcm: ;
                                    rdfs:label "Cross-border company merger by acquisition"@en .


###  http://w3id.org/um/cbcm/eu-cm-ontology#CrossBorderMergerIntoNewCompany
cbcm:CrossBorderMergerIntoNewCompany rdf:type owl:Class ;
                                     rdfs:subClassOf cbcm:CrossBorderMerger ;
                                     rdfs:comment "Article 90: the operation whereby several companies are wound up without going into liquidation and transfer to a company that they set up all their assets and liabilities in exchange for the issue to their shareholders of shares in the new company and a cash payment, if any, not exceeding 10 % of the nominal value of the shares so issued or, where they have no nominal value, of their accounting par value. Companies involved come from two or more distinct countries."@en ;
                                     rdfs:isDefinedBy cbcm: ;
                                     rdfs:label "Cross-border merger into a new company"@en .


###  http://w3id.org/um/cbcm/eu-cm-ontology#CrossBorderSeatTransfer
cbcm:CrossBorderSeatTransfer rdf:type owl:Class ;
                             owl:equivalentClass [ owl:intersectionOf ( cbcm:CompanySeatTransfer
                                                                        [ rdf:type owl:Restriction ;
                                                                          owl:onProperty cbcm:involvesCountry ;
                                                                          owl:qualifiedCardinality "2"^^xsd:nonNegativeInteger ;
                                                                          owl:onClass cbcm:Country
                                                                        ]
                                                                        [ rdf:type owl:Restriction ;
                                                                          owl:onProperty cbcm:sourceCountry ;
                                                                          owl:qualifiedCardinality "1"^^xsd:nonNegativeInteger ;
                                                                          owl:onClass cbcm:Country
                                                                        ]
                                                                        [ rdf:type owl:Restriction ;
                                                                          owl:onProperty cbcm:targetCountry ;
                                                                          owl:qualifiedCardinality "1"^^xsd:nonNegativeInteger ;
                                                                          owl:onClass cbcm:Country
                                                                        ]
                                                                      ) ;
                                                   rdf:type owl:Class
                                                 ] ;
                             rdfs:subClassOf cbcm:CompanySeatTransfer ,
                                             [ rdf:type owl:Restriction ;
                                               owl:onProperty cbcm:hasTransactionInput ;
                                               owl:qualifiedCardinality "1"^^xsd:nonNegativeInteger ;
                                               owl:onClass cbcm:Company
                                             ] ,
                                             [ rdf:type owl:Restriction ;
                                               owl:onProperty cbcm:sourceCountry ;
                                               owl:qualifiedCardinality "1"^^xsd:nonNegativeInteger ;
                                               owl:onClass cbcm:Country
                                             ] ,
                                             [ rdf:type owl:Restriction ;
                                               owl:onProperty cbcm:targetCountry ;
                                               owl:qualifiedCardinality "1"^^xsd:nonNegativeInteger ;
                                               owl:onClass cbcm:Country
                                             ] ;
                             rdfs:comment "The act of changing the location where the company’s business was managed (registered office or headquarters) or the place where that company’s primary business was actually conducted (central administration), across national boundaries."@en ;
                             rdfs:isDefinedBy cbcm: ;
                             rdfs:label "Cross-border company seat transfer"@en .


###  http://w3id.org/um/cbcm/eu-cm-ontology#DataCurationActivity
cbcm:DataCurationActivity rdf:type owl:Class ;
                          rdfs:subClassOf cbcm:Procedure ,
                                          [ rdf:type owl:Restriction ;
                                            owl:onProperty cbcm:used ;
                                            owl:someValuesFrom cbcm:DocumentRepository
                                          ] ,
                                          [ rdf:type owl:Restriction ;
                                            owl:onProperty cbcm:wasAssociatedWith ;
                                            owl:qualifiedCardinality "1"^^xsd:nonNegativeInteger ;
                                            owl:onClass cbcm:Agent
                                          ] ;
                          rdfs:comment "A data curation activity represents a researcher's involvement in annotating cross border transactions"@en ;
                          rdfs:isDefinedBy cbcm: ;
                          rdfs:label "Data curation activity"@en ;
                          <http://www.w3.org/2003/06/sw-vocab-status/ns#term_status> "testing"^^xsd:string .


###  http://w3id.org/um/cbcm/eu-cm-ontology#DecisionRight
cbcm:DecisionRight rdf:type owl:Class ;
                   rdfs:subClassOf cbcm:ShareholderRight ;
                   rdfs:comment "The shareholders can take a number of decisions affecting the company, such as amending the company's articles of association, appointing or dismissing board members and to approve important transactions (e.g. mergers, divisions and conversions/seat transfers). These are taken through a shareholder resolution."@en ;
                   rdfs:isDefinedBy cbcm: ;
                   rdfs:label "Shareholder decision right"@en ;
                   rdfs:seeAlso <http://data.europa.eu/eli/dir/2017/1132/oj> .


###  http://w3id.org/um/cbcm/eu-cm-ontology#DivisionCertificate
cbcm:DivisionCertificate rdf:type owl:Class ;
                         rdfs:subClassOf cbcm:TransactionCertificate ;
                         rdfs:comment "A document issued by a Competent Authority declaring that the legally required steps of a division are completed. The certificate needs to be presented by a company to either be registered (or register a newly established emerging/recipient company) in another company registry or to be removed from a company register."@en ;
                         rdfs:isDefinedBy cbcm: ;
                         rdfs:label "Company division certificate"@en .


###  http://w3id.org/um/cbcm/eu-cm-ontology#DivisionPlan
cbcm:DivisionPlan rdf:type owl:Class ;
                  rdfs:subClassOf cbcm:TransactionDocument ;
                  rdfs:comment "The management or administrative organ of the company shall draw up the draft terms of a division. The draft terms of a division shall include at least the particulars listed in article 160d."@en ;
                  rdfs:isDefinedBy cbcm: ;
                  rdfs:label "Company division plan"@en ;
                  rdfs:seeAlso <https://www.europarl.europa.eu/doceo/document/TA-8-2019-0429_EN.html> .


###  http://w3id.org/um/cbcm/eu-cm-ontology#DocumentRepository
cbcm:DocumentRepository rdf:type owl:Class ;
                        rdfs:subClassOf obo:BFO_0000030 ;
                        rdfs:comment "A digital document repository containing documents related to company mobility."@en ;
                        rdfs:isDefinedBy cbcm: ;
                        rdfs:label "Company mobility document repository"@en .


###  http://w3id.org/um/cbcm/eu-cm-ontology#DomesticConversion
cbcm:DomesticConversion rdf:type owl:Class ;
                        rdfs:subClassOf cbcm:CompanyConversion ,
                                        [ rdf:type owl:Restriction ;
                                          owl:onProperty cbcm:involvesCountry ;
                                          owl:qualifiedCardinality "1"^^xsd:nonNegativeInteger ;
                                          owl:onClass cbcm:Country
                                        ] ;
                        rdfs:comment "A domestic conversion is an operation through which a company's form is converted into a another while still remaining governed by the same law as the original company. For instance, the modification of a company's form from a public to a private limited company."@en ;
                        rdfs:isDefinedBy cbcm: ;
                        rdfs:label "Domestic company conversion"@en .


###  http://w3id.org/um/cbcm/eu-cm-ontology#DomesticDivision
cbcm:DomesticDivision rdf:type owl:Class ;
                      rdfs:subClassOf cbcm:CompanyDivision ,
                                      [ rdf:type owl:Restriction ;
                                        owl:onProperty cbcm:involvesCountry ;
                                        owl:qualifiedCardinality "1"^^xsd:nonNegativeInteger ;
                                        owl:onClass cbcm:Country
                                      ] ;
                      rdfs:comment "A company which in a process of the domestic division - in case of a full division - transfers all its assets and liabilities to two or more companies, or - in case of a partial division or division by separation - transfers part of its assets and liabilities to one or more companies. All companies involved in the process are located in a single country."@en ;
                      rdfs:isDefinedBy cbcm: ;
                      rdfs:label "Company domestic division"@en .


###  http://w3id.org/um/cbcm/eu-cm-ontology#DomesticMerger
cbcm:DomesticMerger rdf:type owl:Class ;
                    rdfs:subClassOf cbcm:CompanyMerger ,
                                    [ rdf:type owl:Restriction ;
                                      owl:onProperty cbcm:hasTransactionInput ;
                                      owl:someValuesFrom cbcm:AcquiringCompany
                                    ] ,
                                    [ rdf:type owl:Restriction ;
                                      owl:onProperty cbcm:hasTransactionInput ;
                                      owl:someValuesFrom cbcm:MergingCompany
                                    ] ,
                                    [ rdf:type owl:Restriction ;
                                      owl:onProperty cbcm:involvesCountry ;
                                      owl:qualifiedCardinality "1"^^xsd:nonNegativeInteger ;
                                      owl:onClass cbcm:Country
                                    ] ;
                    rdfs:comment "A domestic merger involves at least two companies based in the same EU Member State and is leading to a universal transfer of assets and liabilities from the merging company to the acquiring company."@en ;
                    rdfs:isDefinedBy cbcm: ;
                    rdfs:label "Company domestic merger"@en .


###  http://w3id.org/um/cbcm/eu-cm-ontology#DomesticMergerByAcquisition
cbcm:DomesticMergerByAcquisition rdf:type owl:Class ;
                                 rdfs:subClassOf cbcm:DomesticMerger ,
                                                 [ rdf:type owl:Restriction ;
                                                   owl:onProperty cbcm:hasTransactionResult ;
                                                   owl:someValuesFrom cbcm:MergingCompany
                                                 ] ,
                                                 [ rdf:type owl:Restriction ;
                                                   owl:onProperty cbcm:hasTransactionInput ;
                                                   owl:qualifiedCardinality "1"^^xsd:nonNegativeInteger ;
                                                   owl:onClass cbcm:AcquiringCompany
                                                 ] ;
                                 owl:disjointWith cbcm:DomesticMergerIntoNewCompany ;
                                 rdfs:comment "Article 89: The operation whereby one or more companies are wound up without going into liquidation and transfer to another all their assets and liabilities in exchange for the issue to the shareholders of the company or companies being acquired of shares in the acquiring company and a cash payment, if any, not exceeding 10 % of the nominal value of the shares so issued or, where they have no nominal value, of their accounting par value. All companies involved are from a single country."@en ;
                                 rdfs:isDefinedBy cbcm: ;
                                 rdfs:label "Domestic company merger by acquisition"@en ;
                                 rdfs:seeAlso <http://data.europa.eu/eli/dir/2017/1132/oj> .


###  http://w3id.org/um/cbcm/eu-cm-ontology#DomesticMergerIntoNewCompany
cbcm:DomesticMergerIntoNewCompany rdf:type owl:Class ;
                                  rdfs:subClassOf cbcm:DomesticMerger ,
                                                  [ rdf:type owl:Restriction ;
                                                    owl:onProperty cbcm:hasTransactionInput ;
                                                    owl:someValuesFrom cbcm:MergingCompany
                                                  ] ,
                                                  [ rdf:type owl:Restriction ;
                                                    owl:onProperty cbcm:hasTransactionResult ;
                                                    owl:someValuesFrom cbcm:EmergingCompany
                                                  ] ;
                                  rdfs:comment "Article 90: the operation whereby several companies are wound up without going into liquidation and transfer to a company that they set up all their assets and liabilities in exchange for the issue to their shareholders of shares in the new company and a cash payment, if any, not exceeding 10 % of the nominal value of the shares so issued or, where they have no nominal value, of their accounting par value. All companies involved are from a single country."@en ;
                                  rdfs:isDefinedBy cbcm: ;
                                  rdfs:label "Domestic merger into a new company"@en ;
                                  rdfs:seeAlso <http://data.europa.eu/eli/dir/2017/1132/oj> .


###  http://w3id.org/um/cbcm/eu-cm-ontology#DomesticSeatTransfer
cbcm:DomesticSeatTransfer rdf:type owl:Class ;
                          owl:equivalentClass [ owl:intersectionOf ( cbcm:CompanySeatTransfer
                                                                     [ rdf:type owl:Restriction ;
                                                                       owl:onProperty cbcm:involvesCountry ;
                                                                       owl:qualifiedCardinality "1"^^xsd:nonNegativeInteger ;
                                                                       owl:onClass cbcm:Country
                                                                     ]
                                                                     [ rdf:type owl:Restriction ;
                                                                       owl:onProperty cbcm:sourceCountry ;
                                                                       owl:qualifiedCardinality "1"^^xsd:nonNegativeInteger ;
                                                                       owl:onClass cbcm:Country
                                                                     ]
                                                                     [ rdf:type owl:Restriction ;
                                                                       owl:onProperty cbcm:targetCountry ;
                                                                       owl:qualifiedCardinality "1"^^xsd:nonNegativeInteger ;
                                                                       owl:onClass cbcm:Country
                                                                     ]
                                                                   ) ;
                                                rdf:type owl:Class
                                              ] ;
                          rdfs:subClassOf cbcm:CompanySeatTransfer ,
                                          [ rdf:type owl:Restriction ;
                                            owl:onProperty cbcm:involvesCountry ;
                                            owl:qualifiedCardinality "1"^^xsd:nonNegativeInteger ;
                                            owl:onClass cbcm:Country
                                          ] ;
                          rdfs:comment "The act of changing the location where the company’s business was managed (registered office or headquarters) or the place where that company’s primary business was actually conducted (central administration), within a specific country."@en ;
                          rdfs:isDefinedBy cbcm: ;
                          rdfs:label "Domestic company seat transfer"@en .


###  http://w3id.org/um/cbcm/eu-cm-ontology#EEACountry
cbcm:EEACountry rdf:type owl:Class ;
                rdfs:subClassOf cbcm:Country ;
                owl:disjointWith cbcm:NonEEACountry ;
                rdfs:comment "Created in 1994, the European Economic Area (EEA) combines the countries of the European Union (EU) and member countries of the European Free Trade Association (EFTA) to facilitate participation in the European Market trade and movement without having to apply to be one of the EU member countries"@en ;
                rdfs:isDefinedBy cbcm: ;
                rdfs:label "European Economic Area country"@en .


###  http://w3id.org/um/cbcm/eu-cm-ontology#EUCountry
cbcm:EUCountry rdf:type owl:Class ;
               rdfs:subClassOf cbcm:EEACountry ;
               owl:disjointWith cbcm:NonEUCountry ;
               terms:description "A country which forms part of the European Union. The European Union is a conglomeration of European countries whose governance structures agree to abide with common political and economic criteria to improve efficiency of goods and services trading as well as movement and migration of inhabitants between these countries"@en ;
               rdfs:comment "A country which forms part of the European Union. The European Union is a conglomeration of European countries whose governance structures agree to abide with common political and economic criteria to improve efficiency of goods and services trading as well as movement and migration of inhabitants between these countries"@en ;
               rdfs:isDefinedBy cbcm: ;
               rdfs:label "EU country" .


###  http://w3id.org/um/cbcm/eu-cm-ontology#EmergingCompany
cbcm:EmergingCompany rdf:type owl:Class ;
                     rdfs:subClassOf cbcm:Company ;
                     rdfs:comment "A company being divided transfers part of its assets and liabilities to one or more newly formed companies, which are the recipient companies in a (cross-border) division."@en ;
                     rdfs:isDefinedBy cbcm: ;
                     rdfs:label "Emerging company"@en .


###  http://w3id.org/um/cbcm/eu-cm-ontology#Employee
cbcm:Employee rdf:type owl:Class ;
              owl:equivalentClass [ owl:intersectionOf ( cbcm:Person
                                                         [ rdf:type owl:Restriction ;
                                                           owl:onProperty cbcm:employedBy ;
                                                           owl:someValuesFrom owl:Thing
                                                         ]
                                                       ) ;
                                    rdf:type owl:Class
                                  ] ;
              rdfs:subClassOf cbcm:CompanyStakeholder ,
                              cbcm:Person ;
              rdfs:comment "The workforce of a company. An employee is a party to an employment relationship characterised as a contract of employment (or contract of service) between the employer and employee. However, this is only one of several different legal formulations of the concept of ‘worker’ in the EU which differ between Member States."@en ;
              rdfs:isDefinedBy cbcm: ;
              rdfs:label "Company employee"@en ;
              rdfs:seeAlso <https://www.eurofound.europa.eu/observatories/eurwork/industrial-relations-dictionary/employee> .


###  http://w3id.org/um/cbcm/eu-cm-ontology#FinancialServiceAuthority
cbcm:FinancialServiceAuthority rdf:type owl:Class ;
                               rdfs:subClassOf cbcm:CompetentAuthority ;
                               rdfs:comment "A body that regulates the financial services industry in a country (e.g. the UK), including most financial services markets, exchanges and firms."@en ;
                               rdfs:isDefinedBy cbcm: ;
                               rdfs:label "Financial service authority"@en .


###  http://w3id.org/um/cbcm/eu-cm-ontology#GeoPoliticalRegion
cbcm:GeoPoliticalRegion rdf:type owl:Class ;
                        rdfs:subClassOf obo:BFO_0000028 ;
                        terms:description "A spatial region on earth whose boundaries are determined by a combination of geographical, ecological, climatic, socio-economic and political criteria."@en ;
                        rdfs:comment "A spatial region on earth whose boundaries are determined by a combination of geographical, ecological, climatic, socio-economic and political criteria."@en ;
                        rdfs:isDefinedBy cbcm: ;
                        rdfs:label "Geo-political region" .


###  http://w3id.org/um/cbcm/eu-cm-ontology#GlobalUltimateOwner
cbcm:GlobalUltimateOwner rdf:type owl:Class ;
                         rdfs:subClassOf cbcm:CompanyStakeholder ,
                                         [ rdf:type owl:Restriction ;
                                           owl:onProperty cbcm:owns ;
                                           owl:someValuesFrom cbcm:Company
                                         ] ;
                         rdfs:comment "A global ultimate owner (GUO) is the individual or entity at the top of the corporate ownership structure."@en ;
                         rdfs:isDefinedBy cbcm: ;
                         rdfs:label "Global ultimate owner"@en .


###  http://w3id.org/um/cbcm/eu-cm-ontology#ImpactOnEmploymentRight
cbcm:ImpactOnEmploymentRight rdf:type owl:Class ;
                             rdfs:subClassOf cbcm:InformationRight ;
                             rdfs:comment "The right of employees or their representatives to be informed on the likely repercussions of the cross-border transaction on employment, which includes the dismissal as well as the hiring of employees or relocation of work. See for instance article 122 of Directive 2017/1132."@en ;
                             rdfs:isDefinedBy cbcm: ;
                             rdfs:label "Impact on employment information right"@en ;
                             rdfs:seeAlso <http://data.europa.eu/eli/dir/2017/1132/oj> .


###  http://w3id.org/um/cbcm/eu-cm-ontology#IndependentExpert
cbcm:IndependentExpert rdf:type owl:Class ;
                       rdfs:subClassOf cbcm:CompanyStakeholder ;
                       rdfs:comment "An Independent Expert provides impartial advice to shareholders and other company stakeholders on the fairness and/or reasonableness of a transaction.  A company may be required to commission an Independent Expert Report (IER) in the case of a (cross-border) merger, division or conversion."@en ;
                       rdfs:isDefinedBy cbcm: ;
                       rdfs:label "Independent expert"@en ;
                       rdfs:seeAlso <http://data.europa.eu/eli/dir/2017/1132/oj> ,
                                    <https://www.europarl.europa.eu/doceo/document/TA-8-2019-0429_EN.html> .


###  http://w3id.org/um/cbcm/eu-cm-ontology#IndependentExpertReport
cbcm:IndependentExpertReport rdf:type owl:Class ;
                             rdfs:subClassOf cbcm:TransactionDocument ,
                                             [ rdf:type owl:Restriction ;
                                               owl:onProperty cbcm:authoredBy ;
                                               owl:someValuesFrom cbcm:IndependentExpert
                                             ] ;
                             rdfs:comment "Article 86g and 160i: Member States must ensure that an independent expert examines the draft terms of the transaction and draws up a report intended for members which is made available to them not less than one month before the date of the general meeting. Depending on the law of Member States, the expert may be a natural person or a legal person. The report must assess the cash compensation proposed and valuation method."@en ;
                             rdfs:isDefinedBy cbcm: ;
                             rdfs:label "Report by an independent expert"@en ;
                             rdfs:seeAlso <https://www.europarl.europa.eu/doceo/document/TA-8-2019-0429_EN.html> .


###  http://w3id.org/um/cbcm/eu-cm-ontology#InformationRight
cbcm:InformationRight rdf:type owl:Class ;
                      rdfs:subClassOf cbcm:SocialRight ;
                      rdfs:comment "The right of employees or their representatives to be informed and to receive any documents necessary for the exercise of their consultation and board-level employee representation rights in the context of an intended merger/division/conversion/seat transfer."@en ;
                      rdfs:isDefinedBy cbcm: ;
                      rdfs:label "Information right"@en ;
                      rdfs:seeAlso <http://data.europa.eu/eli/dir/2002/14/oj> ,
                                   <http://data.europa.eu/eli/dir/2017/1132/oj> .


###  http://w3id.org/um/cbcm/eu-cm-ontology#InterimAccount
cbcm:InterimAccount rdf:type owl:Class ;
                    rdfs:subClassOf cbcm:AnnualAccount ;
                    rdfs:comment "Interim accounts are accounts that are published during a company's financial year and that show the financial situation on a given accounting date."@en ;
                    rdfs:isDefinedBy cbcm: ;
                    rdfs:label "Interim account"@en .


###  http://w3id.org/um/cbcm/eu-cm-ontology#ManagementBoard
cbcm:ManagementBoard rdf:type owl:Class ;
                     rdfs:subClassOf cbcm:Manager ,
                                     [ rdf:type owl:Restriction ;
                                       owl:onProperty cbcm:partOf ;
                                       owl:someValuesFrom cbcm:Company
                                     ] ;
                     rdfs:comment "The group of persons comprising the governing body of the legal entity that is entrusted with the decision-making in the company. It is also called Executive Board in a one-tier board system."@en ;
                     rdfs:isDefinedBy cbcm: ;
                     rdfs:label "Management board"@en .


###  http://w3id.org/um/cbcm/eu-cm-ontology#ManagementReport
cbcm:ManagementReport rdf:type owl:Class ;
                      rdfs:subClassOf cbcm:TransactionDocument ;
                      rdfs:comment "A report drawn up by the company's management on the intended transaction, laying out the main features of the transactions and its consequences."@en ;
                      rdfs:isDefinedBy cbcm: ;
                      rdfs:label "Management report"@en .


###  http://w3id.org/um/cbcm/eu-cm-ontology#Manager
cbcm:Manager rdf:type owl:Class ;
             rdfs:subClassOf cbcm:CompanyStakeholder ;
             rdfs:comment "A person or group of persons that are responsible for overseeing the operations of a company."@en ;
             rdfs:isDefinedBy cbcm: ;
             rdfs:label "Manager"@en .


###  http://w3id.org/um/cbcm/eu-cm-ontology#ManagerDecisionRight
cbcm:ManagerDecisionRight rdf:type owl:Class ;
                          rdfs:subClassOf cbcm:ManagerRight ;
                          rdfs:comment "The right of the board of management or individual managers to take decisions or to not take a decision in the context of a transaction. These are in the form of a board resolution."@en ;
                          rdfs:isDefinedBy cbcm: ;
                          rdfs:label "Manager decision right"@en .


###  http://w3id.org/um/cbcm/eu-cm-ontology#ManagerExitRight
cbcm:ManagerExitRight rdf:type owl:Class ;
                      rdfs:subClassOf cbcm:ManagerRight ;
                      rdfs:comment "The right of a manager or the board of management to resign and therefore exit a company."@en ;
                      rdfs:isDefinedBy cbcm: ;
                      rdfs:label "Manager exit right"@en .


###  http://w3id.org/um/cbcm/eu-cm-ontology#ManagerInformationRight
cbcm:ManagerInformationRight rdf:type owl:Class ;
                             rdfs:subClassOf cbcm:ManagerRight ;
                             rdfs:comment "The right of a manager to information and access to documents that he or she has in accordance with national or European company law."@en ;
                             rdfs:isDefinedBy cbcm: ;
                             rdfs:label "Manager information right"@en .


###  http://w3id.org/um/cbcm/eu-cm-ontology#ManagerRight
cbcm:ManagerRight rdf:type owl:Class ;
                  rdfs:subClassOf cbcm:TransactionRight ,
                                  [ rdf:type owl:Restriction ;
                                    owl:onProperty cbcm:applicableTo ;
                                    owl:someValuesFrom cbcm:Manager
                                  ] ;
                  rdfs:comment "The rights of members of the management in the context of a company transaction."@en ;
                  rdfs:isDefinedBy cbcm: ;
                  rdfs:label "Manager right"@en .


###  http://w3id.org/um/cbcm/eu-cm-ontology#MemberStateOfficialJournal
cbcm:MemberStateOfficialJournal rdf:type owl:Class ;
                                rdfs:subClassOf cbcm:OfficialJournal ;
                                rdfs:comment "The national gazette or record in a particular Member State. In the official journal companies publish company transaction notices in order to inform concerned stakeholders and interested parties."@en ;
                                rdfs:isDefinedBy cbcm: ;
                                rdfs:label "Member State Official Journal" .


###  http://w3id.org/um/cbcm/eu-cm-ontology#MergerCertificate
cbcm:MergerCertificate rdf:type owl:Class ;
                       rdfs:subClassOf cbcm:TransactionCertificate ;
                       rdfs:comment "A document issued by a Competent Authority declaring that the legally required steps of a merger are completed. The certificate needs to be presented by a company to either be registered in another company registry or to be removed from a company register (depending on the company being the merging or acquiring company)."@en ;
                       rdfs:isDefinedBy cbcm: ;
                       rdfs:label "Company merger certificate"@en ;
                       rdfs:seeAlso <http://data.europa.eu/eli/dir/2017/1132/oj> .


###  http://w3id.org/um/cbcm/eu-cm-ontology#MergerPlan
cbcm:MergerPlan rdf:type owl:Class ;
                rdfs:subClassOf cbcm:TransactionDocument ;
                rdfs:comment "Article 91: The administrative or management bodies of the merging companies shall draw up draft terms of merger in writing by specifying at least the elements mentioned in article 91."@en ;
                rdfs:isDefinedBy cbcm: ;
                rdfs:label "Company merger plan"@en ;
                rdfs:seeAlso <http://data.europa.eu/eli/dir/2017/1132/oj> .


###  http://w3id.org/um/cbcm/eu-cm-ontology#MergingCompany
cbcm:MergingCompany rdf:type owl:Class ;
                    rdfs:subClassOf cbcm:Company ,
                                    [ rdf:type owl:Restriction ;
                                      owl:onProperty cbcm:isTransactionInputOf ;
                                      owl:someValuesFrom cbcm:CompanyMerger
                                    ] ;
                    rdfs:comment "Merging Company means the dissolving company that is being acquired by another (acquiring) company in the process of a transaction. In the context of company mobility, this means a universal transfer of assets and liabilities from the merging to the acquiring company (see article 131 of Directive 2017/1132)."@en ;
                    rdfs:isDefinedBy cbcm: ;
                    rdfs:label "Merging company"@en ;
                    rdfs:seeAlso <http://data.europa.eu/eli/dir/2017/1132/oj> .


###  http://w3id.org/um/cbcm/eu-cm-ontology#NationalRegistry
cbcm:NationalRegistry rdf:type owl:Class ;
                      rdfs:subClassOf cbcm:Organisation ;
                      rdfs:comment "A national registry is a business registry in a Member State, which includes information on the population of companies in the jurisdiction and holds inter alia data on registration numbers, place of registration, notices and transaction documents in the national registry repository."@en ;
                      rdfs:isDefinedBy cbcm: ;
                      rdfs:label "National registry"@en .


###  http://w3id.org/um/cbcm/eu-cm-ontology#NationalRegistryRepository
cbcm:NationalRegistryRepository rdf:type owl:Class ;
                                rdfs:subClassOf cbcm:DocumentRepository ,
                                                [ rdf:type owl:Restriction ;
                                                  owl:onProperty cbcm:maintainedBy ;
                                                  owl:someValuesFrom cbcm:NationalRegistry
                                                ] ;
                                rdfs:comment "The digital repository in which documents published in the official journal or by by the national registry (on behalf of a company) are kept as well as related documents. In some EU Member States, this repository is overlapping or identical with the Official Journal Repository."@en ;
                                rdfs:isDefinedBy cbcm: ;
                                rdfs:label "National registry repository"@en .


###  http://w3id.org/um/cbcm/eu-cm-ontology#NonEEACountry
cbcm:NonEEACountry rdf:type owl:Class ;
                   rdfs:subClassOf cbcm:NonEUCountry ;
                   rdfs:comment "A country which does not belong to the European Economic Area (EEA)."@en ;
                   rdfs:isDefinedBy cbcm: ;
                   rdfs:label "Non-EEA country"@en .


###  http://w3id.org/um/cbcm/eu-cm-ontology#NonEUCountry
cbcm:NonEUCountry rdf:type owl:Class ;
                  rdfs:subClassOf cbcm:Country ;
                  rdfs:comment "A country that does not officially belong to the EU conglomeration"@en ;
                  rdfs:isDefinedBy cbcm: ;
                  rdfs:label "Non-EU country"@en .


###  http://w3id.org/um/cbcm/eu-cm-ontology#Notary
cbcm:Notary rdf:type owl:Class ;
            rdfs:subClassOf cbcm:CompetentAuthority ;
            rdfs:comment "A person authorized to perform certain legal formalities, especially to draw up or certify contracts, deeds, and other documents for use in other jurisdictions."@en ;
            rdfs:isDefinedBy cbcm: ;
            rdfs:label "Notary"@en .


###  http://w3id.org/um/cbcm/eu-cm-ontology#OfficialJournal
cbcm:OfficialJournal rdf:type owl:Class ;
                     rdfs:subClassOf cbcm:Organisation ;
                     rdfs:comment "The official gazette of record for the European Union or national gazette of record of a Member State. In the official journal companies publish transaction notices in order to inform concerned stakeholders and interested parties."@en ;
                     rdfs:isDefinedBy cbcm: ;
                     rdfs:label "Official journal"@en .


###  http://w3id.org/um/cbcm/eu-cm-ontology#OfficialJournalPublication
cbcm:OfficialJournalPublication rdf:type owl:Class ;
                                rdfs:subClassOf cbcm:CompanyMobilityDocument ;
                                rdfs:comment "Publication of a legally valid record or act in an official national gazette to inform stakeholders."@en ;
                                rdfs:isDefinedBy cbcm: ;
                                rdfs:label "Official journal publication"@en .


###  http://w3id.org/um/cbcm/eu-cm-ontology#OfficialJournalRepository
cbcm:OfficialJournalRepository rdf:type owl:Class ;
                               rdfs:subClassOf cbcm:DocumentRepository ,
                                               [ rdf:type owl:Restriction ;
                                                 owl:onProperty cbcm:maintainedBy ;
                                                 owl:someValuesFrom cbcm:OfficialJournal
                                               ] ;
                               rdfs:comment "The digital repository in which documents published in the official journal are kept as well as related documents. In some EU Member States, this repository is overlapping or identical with the National Registry Repository."@en ;
                               rdfs:isDefinedBy cbcm: ;
                               rdfs:label "Official journal repository"@en .


###  http://w3id.org/um/cbcm/eu-cm-ontology#Organisation
cbcm:Organisation rdf:type owl:Class ;
                  rdfs:subClassOf cbcm:Agent ;
                  owl:disjointWith cbcm:Person ;
                  rdfs:comment "Represents a collection of people organized together into a community or other social, commercial or political structure. The group has some common purpose or reason for existence which goes beyond the set of people belonging to it and can act as an Agent. Organizations are often decomposable into hierarchical structures."@en ;
                  rdfs:isDefinedBy cbcm: ;
                  rdfs:label "Organisation"@en .


###  http://w3id.org/um/cbcm/eu-cm-ontology#OrganisationalUnit
cbcm:OrganisationalUnit rdf:type owl:Class ;
                        rdfs:subClassOf cbcm:Agent ;
                        owl:disjointWith cbcm:Person ;
                        rdfs:comment "A division of a large organization such as a government, university, or business, dealing with a specific area of activity."@en ;
                        rdfs:isDefinedBy cbcm: ;
                        rdfs:label "Organisational unit"@en .


###  http://w3id.org/um/cbcm/eu-cm-ontology#OriginalCompany
cbcm:OriginalCompany rdf:type owl:Class ;
                     rdfs:subClassOf cbcm:Company ,
                                     [ rdf:type owl:Restriction ;
                                       owl:onProperty cbcm:isTransactionInputOf ;
                                       owl:someValuesFrom cbcm:CompanyTransaction
                                     ] ;
                     rdfs:comment "An original company, in the context of a (cross-border) division, means a company which - in case of a full division - transfers all its assets and liabilities to two or more companies, or - in case of a partial division or division by separation - transfers part of its assets and liabilities to one or more companies."@en ;
                     rdfs:isDefinedBy cbcm: ;
                     rdfs:label "Original company"@en ;
                     rdfs:seeAlso <https://www.europarl.europa.eu/doceo/document/TA-8-2019-0429_EN.html> .


###  http://w3id.org/um/cbcm/eu-cm-ontology#ParentCompany
cbcm:ParentCompany rdf:type owl:Class ;
                   owl:equivalentClass [ owl:intersectionOf ( cbcm:Company
                                                              [ rdf:type owl:Restriction ;
                                                                owl:onProperty cbcm:hasSubsidiaryCompany ;
                                                                owl:someValuesFrom cbcm:Company
                                                              ]
                                                            ) ;
                                         rdf:type owl:Class
                                       ] ;
                   rdfs:comment "A parent company is a company that has a controlling interest in another company, the subsidiary company, giving it control of its operations through a majority stock-ownership, decisive control over management appointments and therefore over the decision-making process. In the absence of a natural person as ultimate beneficial owner, the highest parent company in a chain of companies is the global ultimate owner."@en ;
                   rdfs:isDefinedBy cbcm: ;
                   rdfs:label "Parent company"@en ;
                   rdfs:seeAlso <http://data.europa.eu/eli/dir/2017/1132/oj> .


###  http://w3id.org/um/cbcm/eu-cm-ontology#Person
cbcm:Person rdf:type owl:Class ;
            rdfs:subClassOf cbcm:Agent ;
            terms:description "A person is an object that has certain capacities or attributes constituting personhood. A human being that has existed or continues to exist in the world (either deceased or living). Fictional human beings cannot be  instances of this class."@en ;
            rdfs:comment "A person is an object that has certain capacities or attributes constituting personhood. A human being that has existed or continues to exist in the world (either deceased or living). Fictional human beings cannot be  instances of this class."@en ;
            rdfs:isDefinedBy cbcm: ;
            rdfs:label "Person"@en .


###  http://w3id.org/um/cbcm/eu-cm-ontology#PreConversionCertificate
cbcm:PreConversionCertificate rdf:type owl:Class ;
                              rdfs:subClassOf cbcm:TransactionCertificate ;
                              rdfs:comment "Article 86m: a pre-conversion certificate attests compliance with all the relevant conditions and the proper completion of all procedures and formalities in the departure Member State."@en ;
                              rdfs:isDefinedBy cbcm: ;
                              rdfs:label "Company pre-conversion certificate"@en ;
                              rdfs:seeAlso <https://www.europarl.europa.eu/doceo/document/TA-8-2019-0429_EN.html> .


###  http://w3id.org/um/cbcm/eu-cm-ontology#PreDivisionCertificate
cbcm:PreDivisionCertificate rdf:type owl:Class ;
                            rdfs:subClassOf cbcm:TransactionCertificate ;
                            rdfs:comment "Article 160o: a pre-division certificate attests compliance with all the relevant conditions and the proper completion of all procedures and formalities in the Member State concerned."@en ;
                            rdfs:isDefinedBy cbcm: ;
                            rdfs:label "Company pre-division certificate"@en ;
                            rdfs:seeAlso <https://www.europarl.europa.eu/doceo/document/TA-8-2019-0429_EN.html> .


###  http://w3id.org/um/cbcm/eu-cm-ontology#PreMergerCertificate
cbcm:PreMergerCertificate rdf:type owl:Class ;
                          rdfs:subClassOf cbcm:TransactionCertificate ;
                          rdfs:comment "Article 127: a pre-merger certificate attests compliance with all the relevant conditions and the proper completion of all procedures and formalities in the Member State of the merging company."@en ;
                          rdfs:isDefinedBy cbcm: ;
                          rdfs:label "Company pre-merger certificate"@en ;
                          rdfs:seeAlso <http://data.europa.eu/eli/dir/2017/1132/oj> .


###  http://w3id.org/um/cbcm/eu-cm-ontology#Procedure
cbcm:Procedure rdf:type owl:Class ;
               rdfs:subClassOf obo:BFO_0000015 ;
               terms:description "A procedure is a process that attempts to achieve one or more objectives by following an established set of actions."@en ;
               rdfs:comment "A procedure is a process that attempts to achieve one or more objectives by following an established set of actions."@en ;
               rdfs:isDefinedBy cbcm: ;
               rdfs:label "Procedure" .


###  http://w3id.org/um/cbcm/eu-cm-ontology#RecipientCompany
cbcm:RecipientCompany rdf:type owl:Class ;
                      rdfs:subClassOf cbcm:Company ,
                                      [ rdf:type owl:Restriction ;
                                        owl:onProperty cbcm:isTransactionResultOf ;
                                        owl:someValuesFrom cbcm:CompanyDivision
                                      ] ;
                      rdfs:comment "A company being divided transfers part of its assets and liabilities to one or more newly formed companies, which are the recipient companies in a (cross-border) division."@en ;
                      rdfs:isDefinedBy cbcm: ;
                      rdfs:label "Recipient company"@en .


###  http://w3id.org/um/cbcm/eu-cm-ontology#Resolution
cbcm:Resolution rdf:type owl:Class ;
                rdfs:subClassOf cbcm:TransactionDocument ;
                rdfs:comment "A document detailing a decision made by an individual or group of natural or legal persons. This can be a decision concerning the restructuring of a company by its shareholders."@en ;
                rdfs:isDefinedBy cbcm: ;
                rdfs:label "Resolution"@en .


###  http://w3id.org/um/cbcm/eu-cm-ontology#SEType
cbcm:SEType rdf:type owl:Class ;
            rdfs:subClassOf cbcm:Attribute ;
            rdfs:comment "Variable indicating the SE-establishment mode: by merger, conversion, holding-SE, subsidiary-SE or unsure (cases)"@en ;
            rdfs:isDefinedBy cbcm: ;
            rdfs:label "Societas Europaea (SE) type"@en ;
            rdfs:seeAlso cbcm:SocietasEuropaeaMerger .


###  http://w3id.org/um/cbcm/eu-cm-ontology#SeatTransferPlan
cbcm:SeatTransferPlan rdf:type owl:Class ;
                      rdfs:subClassOf cbcm:TransactionDocument ;
                      rdfs:comment "The management or administrative organ of the company draws up the draft terms of a cross-border seat transfer. The draft terms of a cross-border seat transfer must include at least the particulars specified under national law."@en ;
                      rdfs:isDefinedBy cbcm: ;
                      rdfs:label "Company seat transfer plan"@en .


###  http://w3id.org/um/cbcm/eu-cm-ontology#ShareholderExitRight
cbcm:ShareholderExitRight rdf:type owl:Class ;
                          rdfs:subClassOf cbcm:ShareholderRight ;
                          rdfs:comment "The right of a shareholder to exit the company by being bought out."@en ;
                          rdfs:isDefinedBy cbcm: ;
                          rdfs:label "Shareholder exit right"@en ;
                          rdfs:seeAlso <http://data.europa.eu/eli/dir/2017/1132/oj> .


###  http://w3id.org/um/cbcm/eu-cm-ontology#ShareholderInformationRight
cbcm:ShareholderInformationRight rdf:type owl:Class ;
                                 rdfs:subClassOf cbcm:ShareholderRight ;
                                 rdfs:comment "It is particularly important that the shareholders of the companies involved in a transaction be kept adequately informed in an objective manner, and that their rights be suitably protected. This includes for instance the availability of documents for inspection by shareholders (e.g. article 97 of Directive 2017/1132)."@en ;
                                 rdfs:isDefinedBy cbcm: ;
                                 rdfs:label "Shareholder information right"@en ;
                                 rdfs:seeAlso <http://data.europa.eu/eli/dir/2017/1132/oj> .


###  http://w3id.org/um/cbcm/eu-cm-ontology#ShareholderResolution
cbcm:ShareholderResolution rdf:type owl:Class ;
                           rdfs:subClassOf cbcm:Resolution ;
                           rdfs:comment "a shareholder resolution is a proposal submitted by shareholders for a vote at the company's shareholder meeting."@en ;
                           rdfs:isDefinedBy cbcm: ;
                           rdfs:label "Shareholder resolution"@en .


###  http://w3id.org/um/cbcm/eu-cm-ontology#ShareholderRight
cbcm:ShareholderRight rdf:type owl:Class ;
                      rdfs:subClassOf cbcm:TransactionRight ,
                                      [ rdf:type owl:Restriction ;
                                        owl:onProperty cbcm:applicableTo ;
                                        owl:someValuesFrom cbcm:CompanyShareholder
                                      ] ;
                      rdfs:comment "The rights of shareholders of a company in the context of a transaction. Often, shreholder resolutions are used to effectuate shareholder rights. Many rights are laid down in the so-called Shareholder Rights Directive."@en ;
                      rdfs:isDefinedBy cbcm: ;
                      rdfs:label "Shareholder right"@en ;
                      rdfs:seeAlso <http://data.europa.eu/eli/dir/2017/1132/oj> .


###  http://w3id.org/um/cbcm/eu-cm-ontology#SocialRight
cbcm:SocialRight rdf:type owl:Class ;
                 rdfs:subClassOf cbcm:TransactionRight ,
                                 [ rdf:type owl:Restriction ;
                                   owl:onProperty cbcm:applicableTo ;
                                   owl:someValuesFrom cbcm:Employee
                                 ] ;
                 rdfs:comment "Social rights, as opposed to rights arising from natural law, are rights for legal entities that entitle them to certain levels of societal living conditions (e.g. the right to housing, to food, to health care etc.)"@en ;
                 rdfs:isDefinedBy cbcm: ;
                 rdfs:label "Social right"@en .


###  http://w3id.org/um/cbcm/eu-cm-ontology#SocietasEuropaeaMerger
cbcm:SocietasEuropaeaMerger rdf:type owl:Class ;
                            rdfs:subClassOf cbcm:CrossBorderMergerIntoNewCompany ;
                            rdfs:comment "This is a cross-border merger where two or more companies from different Member States merge into a new company that has a special legal form called a Societas Europaea (SE) which allows the behavior of this new company to be regulated under European Law (rather than national law)."@en ;
                            rdfs:isDefinedBy cbcm: ;
                            rdfs:label "Cross-border merger into a new company with a Societas Europaea form"@en ;
                            rdfs:seeAlso <http://eur-lex.europa.eu/legal-content/EN/TXT/?uri=celex:32001R2157> .


###  http://w3id.org/um/cbcm/eu-cm-ontology#Society
cbcm:Society rdf:type owl:Class ;
             rdfs:subClassOf cbcm:CompanyStakeholder ;
             rdfs:comment "The society at large is a stakeholder in a company through, inter alia, the government and its agencies, suppliers, customers, trade unions and the communities from which the business draws its resources."@en ;
             rdfs:isDefinedBy cbcm: ;
             rdfs:label "Society"@en .


###  http://w3id.org/um/cbcm/eu-cm-ontology#SpecialNegotiationBody
cbcm:SpecialNegotiationBody rdf:type owl:Class ;
                            rdfs:subClassOf cbcm:Organisation ;
                            rdfs:comment "The Special Negotiation Body (SNB) or Special Negotiating Body is an organisation that represents the employees of companies in negotiations with the company authorities in order to reach a written agreement on the involvement of employees in company transactions."@en ;
                            rdfs:isDefinedBy cbcm: ;
                            rdfs:label "Special negotiating body"@en .


###  http://w3id.org/um/cbcm/eu-cm-ontology#SpecialNegotiationBodyAgreement
cbcm:SpecialNegotiationBodyAgreement rdf:type owl:Class ;
                                     rdfs:subClassOf cbcm:TransactionDocument ;
                                     rdfs:comment "A written agreement concerning the involvement of employees in company transactions. Special Negotiating Body (SNB) organisation represents employees in the negotiation of the terms of this agreement with the company authorities. The agreement must be reached in accordance with the EU Company Law Directive and is laid down in the SNB-agreement."@en ;
                                     rdfs:isDefinedBy cbcm: ;
                                     rdfs:label "Special negotiating body agreement"@en ;
                                     rdfs:seeAlso <http://data.europa.eu/eli/dir/2017/1132/oj> ,
                                                  cbcm:SpecialNegotiationBody .


###  http://w3id.org/um/cbcm/eu-cm-ontology#SubsidiaryCompany
cbcm:SubsidiaryCompany rdf:type owl:Class ;
                       owl:equivalentClass [ owl:intersectionOf ( cbcm:Company
                                                                  [ rdf:type owl:Restriction ;
                                                                    owl:onProperty cbcm:hasParentCompany ;
                                                                    owl:someValuesFrom cbcm:Company
                                                                  ]
                                                                ) ;
                                             rdf:type owl:Class
                                           ] ;
                       rdfs:comment "A subsidiary, subsidiary company or daughter company is a company that is owned or controlled by another company, which is called the parent company, parent, or holding company."@en ;
                       rdfs:isDefinedBy cbcm: ;
                       rdfs:label "Subsidiary company"@en .


###  http://w3id.org/um/cbcm/eu-cm-ontology#SupervisoryAuthority
cbcm:SupervisoryAuthority rdf:type owl:Class ;
                          rdfs:subClassOf cbcm:Organisation ;
                          rdfs:comment "An individual authority established by its member state to supervise the compliance with a specific regulation."@en ;
                          rdfs:isDefinedBy cbcm: ;
                          rdfs:label "SupervisoryAuthority"@en .


###  http://w3id.org/um/cbcm/eu-cm-ontology#SupervisoryBoard
cbcm:SupervisoryBoard rdf:type owl:Class ;
                      rdfs:subClassOf cbcm:Manager ,
                                      [ rdf:type owl:Restriction ;
                                        owl:onProperty cbcm:partOf ;
                                        owl:someValuesFrom cbcm:Company
                                      ] ;
                      rdfs:comment "A supervisory board must approve of major business decisions. It is a group of individuals chosen by the shareholders - and employee representatives in board-level employee representation systems - of a company to promote their interests through the governance of the company and to hire and supervise the management board. It is also called non-executive board in a one-tier board system."@en ;
                      rdfs:isDefinedBy cbcm: ;
                      rdfs:label "Supervisory board"@en .


###  http://w3id.org/um/cbcm/eu-cm-ontology#TaxAuthority
cbcm:TaxAuthority rdf:type owl:Class ;
                  rdfs:subClassOf cbcm:CompetentAuthority ;
                  rdfs:comment "Tax Authority means any governmental authority having jurisdiction over the assessment, determination, collection or imposition of any tax."@en ;
                  rdfs:isDefinedBy cbcm: ;
                  rdfs:label "Tax authority"@en .


###  http://w3id.org/um/cbcm/eu-cm-ontology#TransactionCertificate
cbcm:TransactionCertificate rdf:type owl:Class ;
                            rdfs:subClassOf cbcm:TransactionDocument ;
                            rdfs:comment "A document issued by a Competent Authority declaring that certain steps of the transaction are completed."@en ;
                            rdfs:isDefinedBy cbcm: ;
                            rdfs:label "Company transaction certificate"@en .


###  http://w3id.org/um/cbcm/eu-cm-ontology#TransactionDocument
cbcm:TransactionDocument rdf:type owl:Class ;
                         rdfs:subClassOf cbcm:CompanyMobilityDocument ;
                         rdfs:comment "Document required by law to document the step of a company transaction or an agreement made between stakeholders involved in the transaction that are either printed, inserted and mailed, or electronically presented."@en ;
                         rdfs:isDefinedBy cbcm: ;
                         rdfs:label "Transaction document"@en .


###  http://w3id.org/um/cbcm/eu-cm-ontology#TransactionNotice
cbcm:TransactionNotice rdf:type owl:Class ;
                       rdfs:subClassOf cbcm:TransactionDocument ,
                                       [ rdf:type owl:Restriction ;
                                         owl:onProperty cbcm:containedIn ;
                                         owl:someValuesFrom cbcm:OfficialJournalRepository
                                       ] ;
                       rdfs:comment "A written notice, published in an official journal of a Member State of the EU and/or the European Official Journal indicating the intention to engage in a transaction and which informs  the members, creditors and representatives of the employees of the company, or, where there are no such representatives, the employees themselves of said transaction."@en ;
                       rdfs:isDefinedBy cbcm: ;
                       rdfs:label "Company transaction notice"@en .


###  http://w3id.org/um/cbcm/eu-cm-ontology#TransactionRight
cbcm:TransactionRight rdf:type owl:Class ;
                      rdfs:subClassOf obo:BFO_0000017 ;
                      rdfs:comment "A legal right of a legal entity involved in the process of a company transaction. A legal right here refers to the entitlement of a person to be allowed to perform an activity, or to possess or obtain access to an object."@en ;
                      rdfs:isDefinedBy cbcm: ;
                      rdfs:label "Transaction right"@en .


###  http://w3id.org/um/cbcm/eu-cm-ontology#TransferOfCentralAdministration
cbcm:TransferOfCentralAdministration rdf:type owl:Class ;
                                     rdfs:subClassOf cbcm:Procedure ;
                                     rdfs:comment "Act of modifying the location where the company’s business was managed or the place where that company’s business was actually conducted."@en ;
                                     rdfs:isDefinedBy cbcm: ;
                                     rdfs:label "Transfer of company central administration"@en .


###  http://w3id.org/um/cbcm/eu-cm-ontology#TransferOfRegisteredOffice
cbcm:TransferOfRegisteredOffice rdf:type owl:Class ;
                                rdfs:subClassOf cbcm:Procedure ;
                                rdfs:comment "The act of changing the registered office, which is the official address of an incorporated company, association or any other legal entity."@en ;
                                rdfs:isDefinedBy cbcm: ;
                                rdfs:label "Transfer of company registered office"@en .


###  http://w3id.org/um/cbcm/eu-cm-ontology#TransferringCompany
cbcm:TransferringCompany rdf:type owl:Class ;
                         rdfs:subClassOf cbcm:Company ;
                         rdfs:comment "Transferring Company means the company transferring its assets and liabilities to a recipient company."@en ;
                         rdfs:isDefinedBy cbcm: ;
                         rdfs:label "Transferring company"@en .


###  http://w3id.org/um/cbcm/eu-cm-ontology#UltimateBeneficialOwner
cbcm:UltimateBeneficialOwner rdf:type owl:Class ;
                             rdfs:subClassOf cbcm:CompanyShareholder ,
                                             cbcm:Person ,
                                             [ rdf:type owl:Restriction ;
                                               owl:onProperty cbcm:owns ;
                                               owl:someValuesFrom [ owl:intersectionOf ( cbcm:Company
                                                                                         [ rdf:type owl:Class ;
                                                                                           owl:complementOf [ rdf:type owl:Restriction ;
                                                                                                              owl:onProperty cbcm:hasParentCompany ;
                                                                                                              owl:someValuesFrom owl:Thing
                                                                                                            ]
                                                                                         ]
                                                                                       ) ;
                                                                    rdf:type owl:Class
                                                                  ]
                                             ] ;
                             rdfs:comment "Ultimate Beneficial owner refers to the natural person(s) who ultimately owns or controls a customer and/or the natural person on whose behalf a transaction is being conducted. It also includes those persons who exercise ultimate effective control over a legal person or arrangement."@en ;
                             rdfs:isDefinedBy cbcm: ;
                             rdfs:label "Ultimate beneficial owner"@en .


###  http://w3id.org/um/cbcm/eu-cm-ontology#WorksCouncil
cbcm:WorksCouncil rdf:type owl:Class ;
                  rdfs:subClassOf cbcm:CompanyStakeholder ,
                                  cbcm:Organisation ,
                                  cbcm:OrganisationalUnit ,
                                  [ rdf:type owl:Restriction ;
                                    owl:onProperty cbcm:hasMember ;
                                    owl:someValuesFrom cbcm:Employee
                                  ] ,
                                  [ rdf:type owl:Restriction ;
                                    owl:onProperty cbcm:partOf ;
                                    owl:someValuesFrom cbcm:Company
                                  ] ;
                  rdfs:comment "The exercise of employee participation through the representation of employees vis-a-vis the management of a company. The works council is a shop-floor level representation mechanism with information, consultation and veto-rights - depending on the extent of rights given in a Member State - and also at EU level through European Works Councils."@en ;
                  rdfs:isDefinedBy cbcm: ;
                  rdfs:label "Employee works council"@en ;
                  rdfs:seeAlso <http://data.europa.eu/eli/dir/2002/14/oj> ,
                               <https://www.worker-participation.eu/National-Industrial-Relations/Across-Europe> .


#################################################################
#    Individuals
#################################################################

###  http://w3id.org/um/cbcm/eu-cm-ontology#austria
cbcm:austria rdf:type owl:NamedIndividual ,
                      cbcm:EUCountry ;
             cbcm:iso2code "AT" ;
             rdfs:label "Austria"@en ,
                        "Österreich"@de .


###  http://w3id.org/um/cbcm/eu-cm-ontology#belgium
cbcm:belgium rdf:type owl:NamedIndividual ,
                      cbcm:EUCountry ;
             cbcm:iso2code "BE" ;
             rdfs:label "Belgique"@fr ,
                        "Belgium"@en .


###  http://w3id.org/um/cbcm/eu-cm-ontology#bulgaria
cbcm:bulgaria rdf:type owl:NamedIndividual ,
                       cbcm:EUCountry ;
              cbcm:iso2code "BG" ;
              rdfs:label "Bulgaria"@en ,
                         "Bǎlgariya"@bg ,
                         "България"@bg .


###  http://w3id.org/um/cbcm/eu-cm-ontology#croatia
cbcm:croatia rdf:type owl:NamedIndividual ,
                      cbcm:EUCountry ;
             cbcm:iso2code "HR" ;
             rdfs:label "Croatia"@en ,
                        "Hrvatska"@hr .


###  http://w3id.org/um/cbcm/eu-cm-ontology#cyprus
cbcm:cyprus rdf:type owl:NamedIndividual ,
                     cbcm:EUCountry ;
            cbcm:iso2code "CY" ;
            rdfs:label "Cyprus"@en .


###  http://w3id.org/um/cbcm/eu-cm-ontology#czechia
cbcm:czechia rdf:type owl:NamedIndividual ,
                      cbcm:EUCountry ;
             cbcm:iso2code "CZ" ;
             rdfs:label "Czech Republic"@en ,
                        "Czechia"@en ,
                        "Česká republika"@cz .


###  http://w3id.org/um/cbcm/eu-cm-ontology#denmark
cbcm:denmark rdf:type owl:NamedIndividual ,
                      cbcm:EUCountry ;
             cbcm:iso2code "DK" ;
             rdfs:label "Danmark"@dk ,
                        "Denmark"@en ,
                        "Kingdom of Denmark"@en .


###  http://w3id.org/um/cbcm/eu-cm-ontology#estonia
cbcm:estonia rdf:type owl:NamedIndividual ,
                      cbcm:EUCountry ;
             cbcm:iso2code "EE" ;
             rdfs:label "Eesti"@ee ,
                        "Estonia"@en .


###  http://w3id.org/um/cbcm/eu-cm-ontology#euOfficialJournal
cbcm:euOfficialJournal rdf:type owl:NamedIndividual ,
                                cbcm:OfficialJournal .


###  http://w3id.org/um/cbcm/eu-cm-ontology#finland
cbcm:finland rdf:type owl:NamedIndividual ,
                      cbcm:EUCountry ;
             cbcm:iso2code "FI" ;
             rdfs:label "Finland"@en ,
                        "Suomi"@fi .


###  http://w3id.org/um/cbcm/eu-cm-ontology#france
cbcm:france rdf:type owl:NamedIndividual ,
                     cbcm:EUCountry ;
            cbcm:iso2code "FR" ;
            rdfs:label "France"@en ,
                       "French Republic"@en ,
                       "République française"@fr .


###  http://w3id.org/um/cbcm/eu-cm-ontology#germany
cbcm:germany rdf:type owl:NamedIndividual ,
                      cbcm:EUCountry ;
             cbcm:iso2code "DE" ;
             rdfs:label "Deutschland"@de ,
                        "Germany"@en .


###  http://w3id.org/um/cbcm/eu-cm-ontology#greece
cbcm:greece rdf:type owl:NamedIndividual ,
                     cbcm:EUCountry ;
            cbcm:iso2code "EL" ,
                          "GR" ;
            rdfs:label "Ellada"@gr ,
                       "Greece"@en ,
                       "Ελλάδα"@gr .


###  http://w3id.org/um/cbcm/eu-cm-ontology#hungary
cbcm:hungary rdf:type owl:NamedIndividual ,
                      cbcm:EUCountry ;
             cbcm:iso2code "HU" ;
             rdfs:label "Hungary"@en ,
                        "Magyarország"@hu .


###  http://w3id.org/um/cbcm/eu-cm-ontology#iceland
cbcm:iceland rdf:type owl:NamedIndividual ,
                      cbcm:EEACountry ;
             cbcm:iso2code "IS" ;
             rdfs:label "Iceland"@en ,
                        "Ísland"@is .


###  http://w3id.org/um/cbcm/eu-cm-ontology#ireland
cbcm:ireland rdf:type owl:NamedIndividual ,
                      cbcm:EUCountry ;
             cbcm:iso2code "IE" ;
             rdfs:label "Ireland"@en ,
                        "Éire"@ga .


###  http://w3id.org/um/cbcm/eu-cm-ontology#italy
cbcm:italy rdf:type owl:NamedIndividual ,
                    cbcm:EUCountry ;
           cbcm:iso2code "IT" ;
           rdfs:label "Italia"@it ,
                      "Italian Republic"@en ,
                      "Italy"@en ,
                      "Repubblica Italiana"@it .


###  http://w3id.org/um/cbcm/eu-cm-ontology#latvia
cbcm:latvia rdf:type owl:NamedIndividual ,
                     cbcm:EUCountry ;
            cbcm:iso2code "LV" ;
            rdfs:label "Latvia"@en ,
                       "Latvija"@lv ,
                       "Latvijas Republika"@lv ,
                       "Republic of Latvia"@en .


###  http://w3id.org/um/cbcm/eu-cm-ontology#liechtenstein
cbcm:liechtenstein rdf:type owl:NamedIndividual ,
                            cbcm:EEACountry ;
                   cbcm:iso2code "LI" ;
                   rdfs:label "Fürstentum Liechtenstein"@de ,
                              "Liechtenstein"@en ,
                              "Principality of Liechtenstein"@en .


###  http://w3id.org/um/cbcm/eu-cm-ontology#lithuania
cbcm:lithuania rdf:type owl:NamedIndividual ,
                        cbcm:EUCountry ;
               cbcm:iso2code "LT" ;
               rdfs:label "Lietuva"@lt ,
                          "Lietuvos Respublika"@lt ,
                          "Lithuania"@en ,
                          "Republic of Lithuania"@en .


###  http://w3id.org/um/cbcm/eu-cm-ontology#luxembourg
cbcm:luxembourg rdf:type owl:NamedIndividual ,
                         cbcm:EUCountry ;
                cbcm:iso2code "LU" ;
                rdfs:label "Grand Duchy of Luxembourg"@en ,
                           "Grand-Duché de Luxembourg"@fr ,
                           "Groussherzogtum Lëtzebuerg"@lb ,
                           "Großherzogtum Luxemburg​"@de ,
                           "Luxembourg"@en ,
                           "Lëtzebuerg"@lb .


###  http://w3id.org/um/cbcm/eu-cm-ontology#malta
cbcm:malta rdf:type owl:NamedIndividual ,
                    cbcm:EUCountry ;
           cbcm:iso2code "MT" ;
           rdfs:label "Malta"@en ,
                      "Melita"@en ,
                      "Repubblika ta' Malta"@mt .


###  http://w3id.org/um/cbcm/eu-cm-ontology#netherlands
cbcm:netherlands rdf:type owl:NamedIndividual ,
                          cbcm:EUCountry ;
                 cbcm:iso2code "NL" ;
                 rdfs:label "Holland"@en ,
                            "Nederland"@nl ,
                            "Netherlands"@en ,
                            "The Netherlands"@en .


###  http://w3id.org/um/cbcm/eu-cm-ontology#norway
cbcm:norway rdf:type owl:NamedIndividual ,
                     cbcm:EEACountry ;
            cbcm:iso2code "NO" ;
            rdfs:label "Kingdom of Norway"@en ,
                       "Kongeriket Noreg"@no ,
                       "Kongeriket Norge"@no ,
                       "Noreg"@no ,
                       "Norge"@no ,
                       "Norgga"@no ,
                       "Norgga gonagasriika"@no ,
                       "Norway"@en ,
                       "Nöörjen"@no ,
                       "Vuona"@no .


###  http://w3id.org/um/cbcm/eu-cm-ontology#poland
cbcm:poland rdf:type owl:NamedIndividual ,
                     cbcm:EUCountry ;
            cbcm:iso2code "PL" ;
            rdfs:label "Poland"@en ,
                       "Polska"@pl ,
                       "Republic of Poland"@en ,
                       "Rzeczpospolita Polska"@pl .


###  http://w3id.org/um/cbcm/eu-cm-ontology#portugal
cbcm:portugal rdf:type owl:NamedIndividual ,
                       cbcm:EUCountry ;
              cbcm:iso2code "PT" ;
              rdfs:label "Portugal"@en ,
                         "Portuguese Republic"@en ,
                         "República Portuguesa"@pt .


###  http://w3id.org/um/cbcm/eu-cm-ontology#romania
cbcm:romania rdf:type owl:NamedIndividual ,
                      cbcm:EUCountry ;
             cbcm:iso2code "RO" ;
             rdfs:label "Romania"@en ,
                        "România"@ro .


###  http://w3id.org/um/cbcm/eu-cm-ontology#se_conversion
cbcm:se_conversion rdf:type owl:NamedIndividual ,
                            cbcm:SEType .


###  http://w3id.org/um/cbcm/eu-cm-ontology#se_holding
cbcm:se_holding rdf:type owl:NamedIndividual ,
                         cbcm:SEType .


###  http://w3id.org/um/cbcm/eu-cm-ontology#se_merger
cbcm:se_merger rdf:type owl:NamedIndividual ,
                        cbcm:SEType .


###  http://w3id.org/um/cbcm/eu-cm-ontology#se_subsidiary
cbcm:se_subsidiary rdf:type owl:NamedIndividual ,
                            cbcm:SEType .


###  http://w3id.org/um/cbcm/eu-cm-ontology#se_unsure
cbcm:se_unsure rdf:type owl:NamedIndividual ,
                        cbcm:SEType .


###  http://w3id.org/um/cbcm/eu-cm-ontology#slovakia
cbcm:slovakia rdf:type owl:NamedIndividual ,
                       cbcm:EUCountry ;
              cbcm:iso2code "SK" ;
              rdfs:label "Slovak Republic"@en ,
                         "Slovakia"@en ,
                         "Slovensko"@sk ,
                         "Slovenská republika"@sk .


###  http://w3id.org/um/cbcm/eu-cm-ontology#slovenia
cbcm:slovenia rdf:type owl:NamedIndividual ,
                       cbcm:EUCountry .


###  http://w3id.org/um/cbcm/eu-cm-ontology#spain
cbcm:spain rdf:type owl:NamedIndividual ,
                    cbcm:EUCountry .


###  http://w3id.org/um/cbcm/eu-cm-ontology#sweden
cbcm:sweden rdf:type owl:NamedIndividual ,
                     cbcm:EUCountry .


###  http://w3id.org/um/cbcm/eu-cm-ontology#switzerland
cbcm:switzerland rdf:type owl:NamedIndividual ,
                          cbcm:EEACountry .


###  http://w3id.org/um/cbcm/eu-cm-ontology#unitedkingdom
cbcm:unitedkingdom rdf:type owl:NamedIndividual ,
                            cbcm:EUCountry .

###  Generated by the OWL API (version 4.5.12.2019-05-06T20:49:08Z) https://github.com/owlcs/owlapi